# baseURI: https://w3id.org/i40/sto/

@prefix : <https://w3id.org/i40/sto/> .
@prefix cc: <http://creativecommons.org/ns#> .
@prefix dbo: <http://dbpedia.org/ontology#> .
@prefix dbr: <http://dbpedia.org/resource#> .
@prefix dc: <http://purl.org/dc/terms/> .
@prefix dc11: <http://purl.org/dc/elements/1.1/> .
@prefix dcterms: <http://purl.org/dc/terms/> .
@prefix deo: <http://purl.org/spar/deo/> .
@prefix doap: <http://usefulinc.com/ns/doap#> .
@prefix dul: <http://www.ontologydesignpatterns.org/ont/dul/DUL.owl#> .
@prefix foaf: <http://xmlns.com/foaf/0.1/> .
@prefix geo: <http://www.geonames.org/ontology#> .
@prefix ids: <https://w3id.org/ids/core/> .
@prefix idsram: <https://w3id.org/ids/ram/> .
@prefix lang: <http://lexvo.org/id/iso639-3/> .
@prefix muto: <http://purl.org/muto/core#> .
@prefix oa: <https://www.w3.org/ns/oa> .
@prefix obda: <https://w3id.org/obda/vocabulary#> .
@prefix om2: <http://www.ontology-of-units-of-measure.org/resource/om-2/> .
@prefix owl: <http://www.w3.org/2002/07/owl#> .
@prefix prov: <http://www.w3.org/ns/prov#> .
@prefix rami: <https://w3id.org/i40/rami#> .
@prefix rdf: <http://www.w3.org/1999/02/22-rdf-syntax-ns#> .
@prefix rdfs: <http://www.w3.org/2000/01/rdf-schema#> .
@prefix schema: <http://schema.org/> .
@prefix skos: <http://www.w3.org/2004/02/skos/core#> .
@prefix sto: <https://w3id.org/i40/sto#> .
@prefix terms: <http://purl.org/dc/terms/> .
@prefix vann: <http://purl.org/vocab/vann/> .
@prefix voaf: <http://purl.org/vocommons/voaf#> .
@prefix xml: <http://www.w3.org/XML/1998/namespace> .
@prefix xsd: <http://www.w3.org/2001/XMLSchema#> .

cc:attributionName
  a owl:DatatypeProperty ;
.
cc:attributionURL
  a owl:AnnotationProperty ;
.
<http://data.semanticweb.org/person/steffen-lohmann>
  a owl:NamedIndividual ;
  a foaf:Person ;
.
dbo:Country
  a owl:Class ;
.
dbo:Place
  a owl:Class ;
.
dbr:Beijing
  a dbo:Place ;
  a owl:NamedIndividual ;
  rdfs:comment "Refers to a place called Beijing."@en ;
  rdfs:label "Beijing"@en ;
.
dbr:Berlin
  a dbo:Place ;
  a owl:NamedIndividual ;
  rdfs:comment "Refers to a place called Berlin."@en ;
  rdfs:label "Berlin"@en ;
.
dbr:Boston
  a dbo:Place ;
  a owl:NamedIndividual ;
  rdfs:comment "Refers to a place called Boston."@en ;
  rdfs:label "Boston"@en ;
.
dbr:Chicago
  a dbo:Place ;
  a owl:NamedIndividual ;
  rdfs:comment "Refers to a place called Chicago."@en ;
  rdfs:label "Chicago"@en ;
.
dbr:China
  a dbo:Country ;
  a owl:NamedIndividual ;
  rdfs:comment "Refers to a Country called China."@en ;
  rdfs:label "China"@en ;
.
dbr:Cologne
  a dbo:Place ;
  a owl:NamedIndividual ;
  rdfs:comment "Refers to a place called Cologne."@en ;
  rdfs:label "Cologne"@en ;
.
dbr:Eumseong
  a dbo:Place ;
  a owl:NamedIndividual ;
  rdfs:comment "Refers to a place called Eumseong."@en ;
  rdfs:label "Eumseong"@en ;
.
dbr:Frankfurt
  a dbo:Place ;
  a owl:NamedIndividual ;
  rdfs:comment "Refers to a place called Frankfurt."@en ;
  rdfs:label "Frankfurt"@en ;
.
dbr:Geneva
  a dbo:Place ;
  a owl:NamedIndividual ;
  rdfs:comment "Refers to a place called Geneva."@en ;
  rdfs:label "Geneva"@en ;
.
dbr:Germany
  a dbo:Country ;
  a owl:NamedIndividual ;
  rdfs:comment "Refers to a Country called Germany."@en ;
  rdfs:label "Germany"@en ;
.
dbr:Hoehenkirchen-Siegertsbrunn
  a dbo:Place ;
  a owl:NamedIndividual ;
  rdfs:comment "Refers to a place called Berlin."@en ;
  rdfs:label "Berlin"@en ;
.
dbr:Hoehenkirchen_Siegertsbrunn
  a dbo:Place ;
  a owl:NamedIndividual ;
  rdfs:comment "Refers to a place called Hoehenkirchen-Siegertsbrunn."@en ;
  rdfs:label "Hoehenkirchen-Siegertsbrunn"@en ;
.
dbr:New_York_City
  a dbo:Place ;
  a owl:NamedIndividual ;
  rdfs:comment "Refers to a place called New York City."@en ;
  rdfs:label "New_York_City"@en ;
.
dbr:Paris
  a dbo:Place ;
  a owl:NamedIndividual ;
  rdfs:comment "Refers to a place called Paris."@en ;
  rdfs:label "Paris"@en ;
.
dbr:South_Korea
  a dbo:Country ;
  a owl:NamedIndividual ;
  rdfs:comment "Refers to a Country called South Korea."@en ;
  rdfs:label "South Korea"@en ;
.
dbr:Switzerland
  a dbo:Country ;
  a owl:NamedIndividual ;
  rdfs:comment "Refers to a Country called Switzerland."@en ;
  rdfs:label "Switzerland"@en ;
.
dbr:United_States
  a dbo:Country ;
  a owl:NamedIndividual ;
  rdfs:comment "Refers to a Country called United_States."@en ;
  rdfs:label "United States"@en ;
.
dbr:Valbonne
  a dbo:Place ;
  a owl:NamedIndividual ;
  rdfs:comment "Refers to a place called Valbonne."@en ;
  rdfs:label "Valbonne"@en ;
.
<http://dbpedia.org/resource#Washington,_D.C.>
  a dbo:Place ;
  a owl:NamedIndividual ;
  rdfs:comment "Refers to a place called Washington D.C."@en ;
  rdfs:label "Washington D.C"@en ;
.
dbr:_Arizona
  a dbo:Place ;
  a owl:NamedIndividual ;
  rdfs:comment "Refers to a place called Arizona."@en ;
  rdfs:label "Arizona"@en ;
.
dbr:_California
  a dbo:Place ;
  a owl:NamedIndividual ;
  rdfs:comment "Refers to a place called California."@en ;
  rdfs:label "_California"@en ;
.
dbr:_Georgia
  a dbo:Place ;
  a owl:NamedIndividual ;
  rdfs:comment "Refers to a place called Georgia."@en ;
  rdfs:label "Georgia"@en ;
.
dbr:_Maryland
  a dbo:Place ;
  a owl:NamedIndividual ;
  rdfs:comment "Refers to a place called Maryland."@en ;
  rdfs:label "Maryland"@en ;
.
dbr:_Massachusetts
  a dbo:Place ;
  a owl:NamedIndividual ;
  rdfs:comment "Refers to a place called Massachusetts."@en ;
  rdfs:label "Massachusetts"@en ;
.
dbr:_Michigan
  a dbo:Place ;
  a owl:NamedIndividual ;
  rdfs:comment "Refers to a place called Michigan."@en ;
  rdfs:label "Michigan"@en ;
.
dbr:_New_York
  a dbo:Place ;
  a owl:NamedIndividual ;
  rdfs:comment "Refers to a place called New York."@en ;
  rdfs:label "New York"@en ;
.
dbr:_North_Carolina
  a dbo:Place ;
  a owl:NamedIndividual ;
  rdfs:comment "Refers to a place called North Carolina."@en ;
  rdfs:label "North Carolina"@en ;
.
dbr:_Texas
  a dbo:Place ;
  a owl:NamedIndividual ;
  rdfs:comment "Refers to a place called Texas."@en ;
  rdfs:label "_Texas"@en ;
.
lang:eng
  a terms:LinguisticSystem ;
  a owl:NamedIndividual ;
.
lang:fra
  a terms:LinguisticSystem ;
  a owl:NamedIndividual ;
.
lang:rus
  a terms:LinguisticSystem ;
  a owl:NamedIndividual ;
.
lang:spa
  a terms:LinguisticSystem ;
  a owl:NamedIndividual ;
.
<http://purl.oclc.org/NET/mvco.owl#EndUser>
  a <http://voag.linkedmodel.org/voag#StakeholderGroup> ;
  a owl:NamedIndividual ;
.
dc11:date
  a owl:AnnotationProperty ;
.
dc11:description
  a owl:AnnotationProperty ;
  terms:description "Description may include but is not limited to: an abstract, a table of contents, a graphical representation, or a free-text account of the resource."@en ;
  terms:hasVersion <http://dublincore.org/usage/terms/history/#description-006> ;
  terms:issued "1999-07-02"^^xsd:date ;
  terms:modified "2008-01-14"^^xsd:date ;
  rdfs:comment "An account of the resource."@en ;
  rdfs:isDefinedBy dc11: ;
  rdfs:label "Description"@en ;
  skos:note "A second property with the same name as this property has been declared in the dcterms: namespace (http://purl.org/dc/terms/).  See the Introduction to the document \"DCMI Metadata Terms\" (http://dublincore.org/documents/dcmi-terms/) for an explanation."@en ;
.
dc11:relation
  a owl:AnnotationProperty ;
.
dc11:title
  a owl:AnnotationProperty ;
  terms:hasVersion <http://dublincore.org/usage/terms/history/#title-006> ;
  terms:issued "1999-07-02"^^xsd:date ;
  terms:modified "2008-01-14"^^xsd:date ;
  rdfs:comment "A name given to the resource."@en ;
  rdfs:isDefinedBy dc11: ;
  rdfs:label "Title"@en ;
  skos:note "A second property with the same name as this property has been declared in the dcterms: namespace (http://purl.org/dc/terms/).  See the Introduction to the document \"DCMI Metadata Terms\" (http://dublincore.org/documents/dcmi-terms/) for an explanation."@en ;
.
terms:LicenseDocument
  a owl:Class ;
  rdfs:comment "A legal document giving official permission to do something with a Resource."@en ;
  rdfs:isDefinedBy terms: ;
  rdfs:label "License Document"@en ;
.
terms:LinguisticSystem
  a owl:Class ;
.
terms:creator
  a owl:ObjectProperty ;
  terms:description "Examples of a Creator include a person, an organization, or a service."@en ;
  terms:hasVersion <http://dublincore.org/usage/terms/history/#creatorT-002> ;
  terms:issued "2008-01-14"^^xsd:date ;
  terms:modified "2010-10-11"^^xsd:date ;
  rdfs:comment "An entity primarily responsible for making the resource."@en ;
  rdfs:isDefinedBy terms: ;
  rdfs:label "has Creator"@en ;
  owl:equivalentProperty foaf:maker ;
.
terms:description
  a owl:AnnotationProperty ;
  terms:description "Description may include but is not limited to: an abstract, a table of contents, a graphical representation, or a free-text account of the resource."@en ;
  terms:hasVersion <http://dublincore.org/usage/terms/history/#descriptionT-001> ;
  terms:issued "2008-01-14"^^xsd:date ;
  terms:modified "2008-01-14"^^xsd:date ;
  rdfs:comment "An account of the resource."@en ;
  rdfs:isDefinedBy terms: ;
  rdfs:label "Description"@en ;
.
terms:hasLicense
  a owl:AnnotationProperty ;
  terms:hasVersion <http://dublincore.org/usage/terms/history/#license-002> ;
  terms:issued "2004-06-14"^^xsd:date ;
  terms:modified "2017-12-19"^^xsd:date ;
  rdfs:comment "A legal document giving official permission to do something with the resource. In this ontology denotes the license of a Standard."@en ;
  rdfs:isDefinedBy terms: ;
  rdfs:label "has License"@en ;
.
terms:hasVersion
  a owl:AnnotationProperty ;
  terms:hasVersion <http://dublincore.org/usage/terms/history/#hasVersion-003> ;
  terms:issued "2000-07-11"^^xsd:date ;
  terms:modified "2008-01-14"^^xsd:date ;
  rdfs:comment "A related resource that is a version, edition, or adaptation of the described resource."@en ;
  rdfs:isDefinedBy terms: ;
  rdfs:label "Has Version"@en ;
  skos:note "This term is intended to be used with non-literal values as defined in the DCMI Abstract Model (http://dublincore.org/documents/abstract-model/).  As of December 2007, the DCMI Usage Board is seeking a way to express this intention with a formal range declaration."@en ;
.
terms:issued
  a owl:AnnotationProperty ;
  terms:hasVersion <http://dublincore.org/usage/terms/history/#issued-003> ;
  terms:issued "2000-07-11"^^xsd:date ;
  terms:modified "2008-01-14"^^xsd:date ;
  rdfs:comment "Date of formal issuance (e.g., publication) of the resource."@en ;
  rdfs:isDefinedBy terms: ;
  rdfs:label "Date Issued"@en ;
.
terms:language
  a owl:ObjectProperty ;
.
terms:license
  a owl:AnnotationProperty ;
  terms:hasVersion <http://dublincore.org/usage/terms/history/#license-002> ;
  terms:issued "2004-06-14"^^xsd:date ;
  terms:modified "2017-12-19"^^xsd:date ;
  rdfs:comment "A legal document giving official permission to do something with the resource. In this ontology denotes the license of a Standard."@en ;
  rdfs:comment "A legal document giving official permission to do something with the resource."@en ;
  rdfs:comment "Represent the license document for a given Standard"@en ;
  rdfs:isDefinedBy terms: ;
  rdfs:label "has License"@en ;
.
terms:modified
  a owl:AnnotationProperty ;
  terms:hasVersion <http://dublincore.org/usage/terms/history/#modified-003> ;
  terms:issued "2000-07-11"^^xsd:date ;
  terms:modified "2008-01-14"^^xsd:date ;
  rdfs:comment "Date on which the resource was changed."@en ;
  rdfs:isDefinedBy terms: ;
  rdfs:label "Date Modified"@en ;
.
terms:title
  a owl:AnnotationProperty ;
  terms:hasVersion <http://dublincore.org/usage/terms/history/#titleT-002> ;
  terms:issued "2008-01-14"^^xsd:date ;
  terms:modified "2010-10-11"^^xsd:date ;
  rdfs:comment "A name given to the resource."@en ;
  rdfs:isDefinedBy terms: ;
  rdfs:label "Title"@en ;
.
muto:Tag
  a rdfs:Datatype ;
.
<http://swrl.stanford.edu/ontologies/3.3/swrla.owl#isRuleEnabled>
  a owl:AnnotationProperty ;
.
<http://voag.linkedmodel.org/voag#StakeholderGroup>
  a owl:Class ;
  a owl:NamedIndividual ;
  terms:creator sto:sebastian ;
  rdfs:comment "A Stakeholder Group is a party of people who have common interests and concerns."@en ;
  rdfs:comment "A stakeholder is everyone with an interest in a system."@en ;
  rdfs:label "Stakeholder Group"@en ;
  skos:note "Stakeholders are interpreted in the same manner as outlined by ISO 42010: '<system> individual, team, organization, or classes thereof, having an interest in a system'"@en ;
.
<http://voag.linkedmodel.org/voag#hasStakeholder>
  a owl:AnnotationProperty ;
.
<http://w3id.org/ids/ram/Perspective>
  a owl:Class ;
  rdfs:label "IDS RAM Perspective"@en ;
  rdfs:subClassOf sto:StandardClassification ;
  owl:equivalentClass [
      a owl:Class ;
      owl:oneOf (
          sto:IDSRAMCertification
          sto:IDSRAMGovernance
          sto:IDSRAMSecurity
        ) ;
    ] ;
.
om2:Measure
  a owl:Class ;
.
om2:Unit
  a owl:Class ;
.
om2:hasNumericalValue
  a owl:DatatypeProperty ;
  rdfs:label "has numerical value"@en ;
.
om2:hasUnit
  a owl:ObjectProperty ;
  rdfs:label "has unit"@en ;
  rdfs:range om2:Unit ;
.
om2:kilobyte
  a om2:Unit ;
  a owl:NamedIndividual ;
.
dul:Collection
  a owl:Class ;
.
dul:associatedWith
  a owl:ObjectProperty ;
.
dul:isComponentOf
  a owl:ObjectProperty ;
  rdfs:comment "Represents Standards that are component of other Standards. This relation is not transitive"@en ;
  rdfs:domain sto:Standard ;
  rdfs:isDefinedBy <http://www.ontologydesignpatterns.org/ont/dul/DUL.owl> ;
  rdfs:label "is Component Of"@en ;
  rdfs:range [
      a owl:Class ;
      owl:unionOf (
          sto:Standard
          sto:StandardPart
        ) ;
    ] ;
  rdfs:subPropertyOf sto:relatedTo ;
.
dul:isMemberOf
  a owl:ObjectProperty ;
  rdfs:comment "A relation between collections and entities, e.g. 'the Night Watch by Rembrandt is in the Rijksmuseum collection'; 'Davide is member of the Pen Club', 'Igor is one the subjects chosen for the experiment'."@en ;
  rdfs:isDefinedBy <http://www.ontologydesignpatterns.org/ont/dul/DUL.owl> ;
  rdfs:label "is member of"@en ;
  rdfs:label "è membro di"@it ;
  rdfs:range dul:Collection ;
  rdfs:subPropertyOf dul:associatedWith ;
.
dul:isPartOf
  a owl:ObjectProperty ;
  rdfs:label "isPartOf"@en ;
.
xsd:date
  a rdfs:Datatype ;
.
xsd:gYear
  a rdfs:Datatype ;
.
skos:altLabel
  a owl:AnnotationProperty ;
  rdfs:label "alternative label"@en ;
.
skos:definition
  a owl:AnnotationProperty ;
  rdfs:label "definition"@en ;
.
skos:narrower
  a owl:AnnotationProperty ;
.
skos:note
  a owl:AnnotationProperty ;
  rdfs:label "note"@en ;
.
skos:prefLabel
  a owl:AnnotationProperty ;
  rdfs:label "preferred label"@en ;
.
prov:wasGeneratedBy
  a owl:ObjectProperty ;
  rdfs:comment "Standard A has influences in Standard B. For example, IEC_61499 hasInfluenceIn IEC_61804-2(EDDL)"@en ;
  rdfs:isDefinedBy "https://www.w3.org/TR/prov-o/#wasGeneratedBy"@en ;
  rdfs:label "was Generated By"@en ;
  rdfs:subPropertyOf sto:relatedTo ;
.
prov:wasRevisionOf
  a owl:AnnotationProperty ;
.
foaf:Document
  a owl:Class ;
.
foaf:Organization
  a owl:Class ;
.
foaf:Person
  a owl:Class ;
.
foaf:familyName
  a owl:AnnotationProperty ;
  rdfs:label "Family Name"@en ;
.
foaf:maker
  a owl:ObjectProperty ;
.
foaf:mbox
  a owl:AnnotationProperty ;
  rdfs:label "mbox"@en ;
.
foaf:name
  a owl:AnnotationProperty ;
  rdfs:label "name"@en ;
.
<https://doi.org/10.1016/j.compind.2018.04.015>
  a owl:NamedIndividual ;
  a sto:Publication ;
  rdfs:label "The industrial internet of things (IIoT): An analysis framework" ;
.
<https://doi.org/10.1016/j.jksuci.2016.10.003>
  a owl:NamedIndividual ;
  a sto:Publication ;
  dc11:title "A survey on Internet of Things architectures" ;
  rdfs:label "A survey on Internet of Things architectures" ;
.
rami:AdminShellGeneral
  a owl:NamedIndividual ;
  a rami:AdminShellSubmodel ;
  a sto:StandardClassification ;
  sto:isDescribedin sto:AdministrationShell ;
.
rami:AdminShellSubmodel
  a owl:Class ;
  rdfs:comment "Describes the Administration Shell concept to organize/classify standards into submodels"@en ;
  rdfs:isDefinedBy <https://www.plattform-i40.de/I40/Redaktion/EN/Downloads/Publikation/structure-of-the-administration-shell.pdf?__blob=publicationFile&v=7> ;
  rdfs:label "Admin Shell Sub Model"@en ;
  rdfs:subClassOf sto:StandardClassification ;
.
rami:ConditionMonitoring
  a owl:NamedIndividual ;
  a rami:AdminShellSubmodel ;
  a sto:StandardClassification ;
  sto:isDescribedin sto:AdministrationShell ;
.
rami:Configuration
  a owl:NamedIndividual ;
  a rami:AdminShellSubmodel ;
  a sto:StandardClassification ;
  skos:note "Publications referred: '<https://doi.org/10.1016/j.jksuci.2016.10.003>' '2.2.2. Middleware enablement' 'Page 300'" ;
  sto:isDescribedin sto:AdministrationShell ;
.
rami:Engineering
  a owl:NamedIndividual ;
  a rami:AdminShellSubmodel ;
  a sto:StandardClassification ;
  dul:associatedWith sto:IviActivityLayer ;
  dul:associatedWith sto:IviActivityView ;
  dul:associatedWith sto:IviSpecificationLayer ;
  sto:alignsWith sto:IviActivityLayer ;
  sto:alignsWith sto:IviActivityView ;
  sto:alignsWith sto:IviSpecificationLayer ;
  sto:isDescribedin sto:AdministrationShell ;
.
rami:Identification
  a owl:NamedIndividual ;
  a rami:AdminShellSubmodel ;
  a sto:StandardClassification ;
  dul:associatedWith sto:Identification ;
  rdfs:label "RAMI Identification"@en ;
  sto:alignsWith sto:Identification ;
  sto:isDescribedin sto:AdministrationShell ;
.
rami:InstanceMaintenance
  a owl:NamedIndividual ;
  a rami:RAMILifeCycleLayer ;
  a sto:StandardClassification ;
  rdfs:label "Instance Maintenance"@en ;
.
rami:InstanceProduction
  a owl:NamedIndividual ;
  a rami:RAMILifeCycleLayer ;
  a sto:StandardClassification ;
  rdfs:label "Instance Production"@en ;
.
rami:Lifecycle_Status
  a owl:NamedIndividual ;
  a rami:AdminShellSubmodel ;
  a sto:StandardClassification ;
  rdfs:label "Lifecycle Status" ;
  sto:isDescribedin sto:AdministrationShell ;
.
rami:Other
  a owl:NamedIndividual ;
  a sto:StandardClassification ;
.
rami:ProcessPlanning
  a owl:NamedIndividual ;
  a rami:AdminShellSubmodel ;
  a sto:StandardClassification ;
  rdfs:comment "Process planning frames everything related to model, plan and manage business workflows and processes."@en ;
  rdfs:label "Process planning"@en ;
  sto:isDescribedin sto:AdministrationShell ;
.
rami:RAMIHierarchyLevel
  a owl:Class ;
  rdfs:label "RAMI Hierarchy Level"@en ;
  rdfs:subClassOf sto:StandardClassification ;
  owl:equivalentClass [
      a owl:Class ;
      owl:oneOf (
          sto:RAMIConnectedWorld
          sto:RAMIControlDevice
          sto:RAMIEnterprise
          sto:RAMIFieldDevice
          sto:RAMIProduct
          sto:RAMIStation
          sto:RAMIWorkCenter
        ) ;
    ] ;
.
rami:RAMIITLayer
  a owl:Class ;
  rdfs:label "RAMI IT Layer"@en ;
  rdfs:subClassOf sto:StandardClassification ;
  owl:equivalentClass [
      a owl:Class ;
      owl:oneOf (
          sto:RAMIAssetlayer
          sto:RAMIBusinessLayer
          sto:RAMICommunicationlayer
          sto:RAMIFunctionalLayer
          sto:RAMIInformationLayer
          sto:RAMIIntegrationLayer
        ) ;
    ] ;
.
rami:RAMILifeCycleLayer
  a owl:Class ;
  rdfs:label "RAMI Life Cycle Layer"@en ;
  rdfs:seeAlso "http://www.zvei.org/en/subjects/Industry-40/Pages/The-Reference-Architectural-Model-RAMI-40-and-the-Industrie-40-Component.aspx" ;
  rdfs:subClassOf sto:StandardClassification ;
  skos:definition "It describes the different Life Cycle and Value Stream layers for the RAMI model according to the IEC 62890 Standard."@en ;
  skos:prefLabel "RAMI Life Cycle Layer"@en ;
.
rami:Safety
  a owl:NamedIndividual ;
  a rami:AdminShellSubmodel ;
  a sto:StandardClassification ;
  rdfs:label "RAMI Safety"@en ;
  sto:isDescribedin sto:AdministrationShell ;
.
rami:Security
  a owl:NamedIndividual ;
  a rami:AdminShellSubmodel ;
  a sto:StandardClassification ;
  dul:associatedWith sto:BdvaCyberSecurityTrust ;
  dul:associatedWith sto:DtpSecurityPrivacy ;
  dul:associatedWith sto:FiwareSecurity ;
  rdfs:label "RAMI Security"@en ;
  sto:alignsWith sto:BdvaCyberSecurityTrust ;
  sto:alignsWith sto:DtpSecurityPrivacy ;
  sto:alignsWith sto:FiwareSecurity ;
  sto:alignsWith sto:OcfSecurity ;
  sto:isDescribedin sto:AdministrationShell ;
.
rami:TypeDevelopment
  a owl:NamedIndividual ;
  a rami:RAMILifeCycleLayer ;
  a sto:StandardClassification ;
  dul:associatedWith sto:IviSpecificationLayer ;
  rdfs:label "Type Development"@en ;
  sto:alignsWith sto:IviSpecificationLayer ;
.
rami:TypeMaintenance
  a owl:NamedIndividual ;
  a rami:RAMILifeCycleLayer ;
  a sto:StandardClassification ;
  rdfs:label "Type Maintenance"@en ;
.
sto:AI
  a owl:NamedIndividual ;
  a sto:Concern ;
  terms:creator sto:sebastian ;
  rdfs:comment "Artificial intelligence (AI) is intelligence exhibited by machines. In computer science, an ideal \"intelligent\" machine is a flexible rational agent that perceives its environment and takes actions that maximize its chance of success at some goal. Colloquially, the term \"artificial intelligence\" is applied when a machine mimics \"cognitive\" functions that humans associate with other human minds, such as \"learning\" and \"problem solving\". (source: wikipedia)"@en ;
  rdfs:label "Artificial Intelligence"@en ;
  sto:hasDBpediaResource <http://dbpedia.org/resource/Artificial_intelligence> ;
  sto:hasDBpediaResource ""@en ;
  sto:supports sto:DataAnalytics ;
.
sto:AMQP
  a owl:NamedIndividual ;
  a foaf:Document ;
  a sto:Publication ;
  a sto:TechnicalSpecification ;
  terms:creator sto:sebastian ;
  rdfs:comment "AMQP (Advanced Message Queuing Protocol): An open standard application layer protocol for message-oriented middleware. The defining features of AMQP are message orientation, queuing, routing (including point-to-point and publish-and-subscribe), reliability and security. (source: https://www.postscapes.com/internet-of-things-protocols/)"@en ;
  rdfs:label "AMQP"@en ;
  sto:hasOfficialResource <http://www.amqp.org/> ;
.
sto:ANSI
  a owl:NamedIndividual ;
  a foaf:Organization ;
  a sto:StandardOrganization ;
  rdfs:comment "The American National Standards Institute is a private non-profit organization that oversees the development of voluntary consensus standards for products, services, processes, systems, and personnel in the United States. The organization also coordinates U.S. standards with international standards so that American products can be used worldwide. ANSI accredits standards that are developed by representatives of other standards organizations, government agencies, consumer groups, companies, and others. These standards ensure that the characteristics and performance of products are consistent, that people use the same definitions and terms, and that products are tested the same way. ANSI also accredits organizations that carry out product or personnel certification in accordance with requirements defined in international standards."@en ;
  rdfs:label "ANSI"@en ;
  sto:abbreviation "ANSI" ;
  sto:formationDate "1918-05-14"^^xsd:date ;
  sto:hasDBpediaResource <http://dbpedia.org/resource/American_National_Standards_Institute> ;
  sto:hasHeadquaterIn <http://dbpedia.org/resource#Washington,_D.C.> ;
  sto:hasOfficialResource <https://www.ansi.org/> ;
  sto:hasWikipediaArticle <https://en.wikipedia.org/wiki/American_National_Standards_Institute?oldformat=true> ;
  sto:orgName "American National Standards Institute"@en ;
.
sto:ANT
  a owl:NamedIndividual ;
  a foaf:Document ;
  a sto:Publication ;
  a sto:TechnicalSpecification ;
  terms:creator sto:sebastian ;
  rdfs:comment "ANT is a proprietary wireless sensor network technology featuring a wireless communications protocol stack that enables semiconductor radios operating in the 2.4 GHz Industrial, Scientific and Medical allocation of the RF spectrum (ISM band) to communicate by establishing standard rules for co-existence, data representation, signalling, authentication and error detection.  (source: https://www.postscapes.com/internet-of-things-protocols/)"@en ;
  rdfs:label "ANT"@en ;
  sto:hasWikipediaArticle <https://en.wikipedia.org/wiki/ANT_(network)> ;
.
sto:APICS
  a owl:NamedIndividual ;
  a foaf:Organization ;
  a sto:StandardOrganization ;
  rdfs:comment "American Production and Inventory Control Society."@en ;
  rdfs:label "APICS"@en ;
  sto:formationDate "1957-01-01"^^xsd:date ;
  sto:hasDBpediaResource <http://dbpedia.org/page/APICS> ;
  sto:hasHeadquaterIn dbr:Chicago ;
  sto:hasOfficialResource <http://www.apics.org/apics> ;
  sto:hasWikipediaArticle <https://en.wikipedia.org/wiki/APICS> ;
  sto:orgName "American Production and Inventory Control Society"@en ;
.
sto:ASAM
  a owl:NamedIndividual ;
  a foaf:Organization ;
  a sto:StandardOrganization ;
  rdfs:comment "Association for Standardization of Automation and Measuring Systems or ASAM is an incorporated association under German law. Its members are primarily international car manufacturers, suppliers and engineering service providers from the automotive industry. The association coordinates the development of technical standards, which are developed by working groups composed of experts from its member companies. ASAM pursues the vision that the tools of a development process chain can be freely interconnected and allow a seamless exchange of data. The standards define protocols, data models, file formats and application programming interfaces (APIs) for the use in the development and testing of automotive electronic control units. A large amount of popular tools in the areas of simulation, measurement, calibration and test automation are compliant to ASAM standards. Compliance shall guarantee interoperability of tools from different vendors, allow data exchange without the need for converters, and facilitate the exchange of unambiguous specification between customers and suppliers."@en ;
  rdfs:label "ASAM" ;
  sto:abbreviation "ASAM" ;
  sto:belongsTo dbr:Germany ;
  sto:formationDate "1998-12-01"^^xsd:date ;
  sto:hasDBpediaResource <http://dbpedia.org/page/Association_for_Standardisation_of_Automation_and_Measuring_Systems> ;
  sto:hasHeadquaterIn dbr:Hoehenkirchen_Siegertsbrunn ;
  sto:hasOfficialResource <https://www.asam.net/> ;
  sto:hasWikipediaArticle <https://en.wikipedia.org/wiki/Association_for_Standardisation_of_Automation_and_Measuring_Systems> ;
  sto:orgName "Association for Standardization of Automation and Measuring Systems"@en ;
.
sto:ASAM_ODS
  a owl:NamedIndividual ;
  a foaf:Document ;
  a sto:Publication ;
  a sto:Standard ;
  terms:creator sto:ASAM ;
  rdfs:comment "Set up a test data management system on top of test systems that produce measured or calculated data from testing activities"@en ;
  rdfs:label "ASAM ODS"@en ;
  foaf:maker sto:ASAM ;
  sto:hasOfficialResource <https://wiki.asam.net/display/STANDARDS/ASAM+ODS> ;
  sto:hasPublisher sto:ASAM ;
.
sto:ASME
  a owl:NamedIndividual ;
  a foaf:Organization ;
  a sto:StandardOrganization ;
  rdfs:comment "The American Society of Mechanical Engineers (ASME) is a professional association that, promotes the art, science, and practice of multidisciplinary engineering and allied sciences around the globe via continuing education, training and professional development, codes and standards, research, conferences and publications, government relations, and other forms of outreach."@en ;
  sto:abbreviation "ASME" ;
  sto:formationDate "1880-01-01"^^xsd:date ;
  sto:hasDBpediaResource <http://dbpedia.org/resource/ASME> ;
  sto:hasHeadquaterIn dbr:New_York_City ;
  sto:hasOfficialResource <https://www.asme.org/> ;
  sto:hasWikipediaArticle <https://en.wikipedia.org/wiki/ASME> ;
  sto:orgName "American Society of Mechanical Engineers"@en ;
.
sto:ASME_Y1441
  a owl:NamedIndividual ;
  a foaf:Document ;
  a sto:Publication ;
  a sto:Standard ;
  terms:creator sto:ASME ;
  rdfs:comment "ASME Y14.41 establishs requirements for model-based definition upon CAD software and those who use CAD software to create product definition within the 3D model."@en ;
  rdfs:label "ASME Y14.41"@en ;
  foaf:maker sto:ASME ;
  sto:hasClassification sto:ModelingPractice ;
  sto:hasDBpediaResource <http://dbpedia.org/resource/ASME_Y14.41> ;
  sto:hasOfficialResource <https://www.asme.org/products/codes-standards/y1441-2012-digital-product-definition-data> ;
  sto:hasPublisher sto:ASME ;
  sto:hasWikipediaArticle <https://en.wikipedia.org/wiki/ASME_Y14.41> ;
.
sto:AccessPolicy
  a owl:NamedIndividual ;
  a sto:Concern ;
  terms:creator sto:sebastian ;
  rdfs:comment "Access to the service shall be regulated by access policies. Users entitled in access policies to envoke a given service must be able to actually envoke it."@en ;
  rdfs:label "Access Policy"@en ;
  rdfs:seeAlso "IoT-A Requirement UNI.604" ;
  rdfs:seeAlso "https://ieeexplore.ieee.org/document/6188257"@en ;
  rdfs:seeAlso "https://ieeexplore.ieee.org/document/8552311"@en ;
  sto:supports sto:DataAccessControl ;
.
sto:Access_Rights_for_IoT-Cloud
  a owl:NamedIndividual ;
  a sto:Concern ;
  terms:creator sto:MuhammadUsman ;
  rdfs:label "Access Rights for IoT-Cloud"@en ;
  rdfs:seeAlso "https://ieeexplore.ieee.org/document/7919553"@en ;
  skos:note "TODO what is the IoT Cloud?" ;
  sto:hasWikipediaArticle "https://en.wikipedia.org/wiki/Access_rights"@en ;
  sto:supports sto:Cloud_Connectivity ;
.
sto:Accountability
  a owl:NamedIndividual ;
  a sto:Concern ;
  rdfs:comment "A system built using the ARM shall support the reversing of the pseudonymization processes in order to guarantee mutual accountability"@en ;
  rdfs:label "Accountability"@en ;
  rdfs:seeAlso "IoT-A Requirement UNI.605" ;
.
sto:Actuation
  a owl:NamedIndividual ;
  a sto:Concern ;
  terms:creator sto:sebastian ;
  rdfs:comment "Sending data or a signal to a kind of actuating device, which leads to a change in a defined environment."@en ;
  rdfs:label "Actuation"@en ;
  skos:note "Publications referred: 'IIC:PUB:G1:V1.80:20170131' '6.1 THE CONTROL DOMAIN' 'Page 28' " ;
  sto:hasDBpediaResource <http://dbpedia.org/resource/Actuator> ;
  sto:supports sto:IoT ;
.
sto:Adaptability
  a owl:NamedIndividual ;
  a sto:Concern ;
  terms:creator sto:MuhammadUsman ;
  rdfs:comment """Because of clients' need and time's requirements, there ought to be constant change in the system of associated devices for Internet of Things. Adaptability is
continuously a need for survival and development of Internet of Things."""@en ;
  rdfs:label "Adaptability"@en ;
  rdfs:seeAlso "https://ieeexplore.ieee.org/document/6188257"@en ;
  skos:note "TODO merge with programmability or evolveability" ;
  sto:hasWikipediaArticle "https://en.wikipedia.org/wiki/Adaptability"@en ;
  sto:supports sto:IoT ;
.
sto:AdministrationShell
  a owl:NamedIndividual ;
  a sto:StandardClassification ;
  a sto:StandardizationFramework ;
  dul:associatedWith ids:TrustedConnector ;
  rdfs:comment "Represents the classifications of the standards according to the submodels of the administration shell."@en ;
  rdfs:label "Administration Shell"@en ;
  sto:alignsWith ids:TrustedConnector ;
  sto:frames rami:Lifecycle_Status ;
  sto:frames sto:Availability ;
  sto:frames sto:BusinessContext ;
  sto:frames sto:Communication ;
  sto:frames sto:DataAccess ;
  sto:frames sto:DynamicAdjustability ;
  sto:frames sto:EndpointInvocation ;
  sto:frames sto:Identification ;
  sto:frames sto:IdentityManagement ;
  sto:frames sto:IntegrityProtection ;
  sto:frames sto:Interoperability ;
  sto:frames sto:SecureCommunication ;
  sto:frames sto:Security ;
  sto:frames sto:SemanticInteroperability ;
  sto:frames sto:ServiceChoreography ;
  sto:frames sto:ServiceComposition ;
  sto:frames sto:ServiceOrchestration ;
  sto:frames sto:SyntacticInteroperability ;
  sto:frames sto:ThingDescription ;
  sto:frames sto:ThingRepresentation ;
  sto:frames sto:Trustworthiness ;
  sto:hasPublisher sto:PlatformIndustry40 ;
.
sto:Aeron
  a owl:NamedIndividual ;
  a foaf:Document ;
  a sto:Publication ;
  a sto:TechnicalSpecification ;
  terms:creator sto:sebastian ;
  rdfs:comment "Aeron - Efficient reliable UDP unicast, UDP multicast, and IPC message transport. (source: https://www.postscapes.com/internet-of-things-protocols/)"@en ;
  rdfs:label "Aeron"@en ;
  sto:hasOfficialResource <https://github.com/real-logic/Aeron> ;
.
sto:Agility
  a owl:NamedIndividual ;
  a sto:Concern ;
  rdfs:comment """Agility as a key pillar that enables quick and astute business operational decisions for an OpenFog System. The predicted scale of the data generated by IoT means that it is highly unlikely that humans alone will be able to comprehend the data, derive knowledge and make wise decisions about how to best leverage their IoT assets for the benefit of their businesses. In the OpenFog architecture the agility pillar is about making sure that the valuable data generated in the IoT can be rapidly transformed into actionable insights that drive rapid decisions and further levels of automation to support business interest.
Spurce: OpenFog Consortum Architecture Whitepaper"""@en ;
  skos:note "Publications referred: '<https://www.openfogconsortium.org/wp-content/uploads/OpenFog_Reference_Architecture_2_09_17-FINAL.pdf> OPFRA001.020817' '4.7 Agility Pillar' 'Page 31' " ;
  sto:supports sto:BusinessContext ;
.
sto:AiiClassification
  a owl:Class ;
  rdfs:label "Alliance of Industrial Internet Architecture Classification"@en ;
  rdfs:subClassOf sto:StandardClassification ;
.
sto:AiiData
  a owl:NamedIndividual ;
  a :AiiClassification ;
  rdfs:label "AII Data Classification"@en ;
  sto:alignsWith sto:IDSRAMInformationLayer ;
  sto:alignsWith sto:InformationDomain ;
  sto:frames sto:DataAnalytics ;
  sto:frames sto:DataProcessing ;
  sto:frames sto:Data_Collection ;
  sto:frames sto:EdgeComputing ;
  sto:frames sto:SemanticInteroperability ;
  sto:isDescribedin :IndustrialInternetArchitecture ;
.
sto:AiiDataAnno
  a <https://www.w3.org/ns/oaAnnotation> ;
  <https://www.w3.org/ns/oahasBody> sto:AiiData ;
  <https://www.w3.org/ns/oahasTarget> [
      a <https://www.w3.org/ns/oaSpecificResource> ;
      <https://www.w3.org/ns/oahasSelector> [
          a <https://www.w3.org/ns/oaRangeSelector> ;
          <https://www.w3.org/ns/oahasEndSelector> [
              a <https://www.w3.org/ns/oaXPathSelector> ;
              rdf:value "Page 32" ;
            ] ;
          <https://www.w3.org/ns/oahasStartSelector> [
              a <https://www.w3.org/ns/oaXPathSelector> ;
              rdf:value "Page 25" ;
            ] ;
        ] ;
      <https://www.w3.org/ns/oahasSource> sto:Industrial_Internet_Architecture_Version_1 ;
    ] ;
.
sto:AiiNetwork
  a owl:NamedIndividual ;
  a :AiiClassification ;
  rdfs:label "AII Network Classification"@en ;
  sto:alignsWith sto:IDSRAMSystemLayer ;
  sto:alignsWith sto:IIRAConnectivity ;
  sto:alignsWith sto:RAMICommunicationlayer ;
  sto:alignsWith sto:RAMIIntegrationLayer ;
  sto:frames sto:Communication ;
  sto:frames sto:Connectivity ;
  sto:frames sto:Identification ;
  sto:frames sto:SyntacticInteroperability ;
  sto:isDescribedin :IndustrialInternetArchitecture ;
.
sto:AiiNetworkAnno
  a <https://www.w3.org/ns/oaAnnotation> ;
  <https://www.w3.org/ns/oahasBody> sto:AiiNetwork ;
  <https://www.w3.org/ns/oahasTarget> [
      a <https://www.w3.org/ns/oaSpecificResource> ;
      terms:format "pdf" ;
      <https://www.w3.org/ns/oahasSelector> [
          a <https://www.w3.org/ns/oaRangeSelector> ;
          <https://www.w3.org/ns/oahasEndSelector> [
              a <https://www.w3.org/ns/oaXPathSelector> ;
              rdf:value "Page 25" ;
            ] ;
          <https://www.w3.org/ns/oahasStartSelector> [
              a <https://www.w3.org/ns/oaXPathSelector> ;
              rdf:value "Page 10" ;
            ] ;
        ] ;
      <https://www.w3.org/ns/oahasSource> sto:Industrial_Internet_Architecture_Version_1 ;
    ] ;
.
sto:AiiSecurity
  a owl:NamedIndividual ;
  a :AiiClassification ;
  rdfs:label "AII Security Classification"@en ;
  sto:alignsWith sto:IDSRAMSecurity ;
  sto:alignsWith sto:IIRASecurity ;
  sto:frames sto:DataAccess ;
  sto:frames sto:Security ;
  sto:isDescribedin :IndustrialInternetArchitecture ;
.
sto:AiiSecurityAnno
  a <https://www.w3.org/ns/oaAnnotation> ;
  <https://www.w3.org/ns/oahasBody> sto:AiiSecurity ;
  <https://www.w3.org/ns/oahasTarget> [
      a <https://www.w3.org/ns/oaSpecificResource> ;
      terms:format "pdf" ;
      <https://www.w3.org/ns/oahasSelector> [
          a <https://www.w3.org/ns/oaRangeSelector> ;
          <https://www.w3.org/ns/oahasEndSelector> [
              a <https://www.w3.org/ns/oaXPathSelector> ;
              rdf:value "Page 37" ;
            ] ;
          <https://www.w3.org/ns/oahasStartSelector> [
              a <https://www.w3.org/ns/oaXPathSelector> ;
              rdf:value "Page 32" ;
            ] ;
        ] ;
      <https://www.w3.org/ns/oahasSource> sto:Industrial_Internet_Architecture_Version_1 ;
    ] ;
.
sto:AllSeenAlliance
  a owl:NamedIndividual ;
  a foaf:Organization ;
  a sto:IIoTConsortium ;
  terms:creator sto:sebastian ;
  rdfs:comment "The AllSeen Alliance is a nonprofit consortium dedicated to enabling and driving the widespread adoption of products, systems and services that support the Internet of Everything with an open, universal development framework supported by a vibrant ecosystem and thriving technical community' (source: https://www.postscapes.com/internet-of-things-protocols/)"@en ;
  rdfs:label "AllSeen Alliance"@en ;
  sto:hasOfficialResource <https://allseenalliance.org/> ;
.
sto:Alljoyn
  a owl:NamedIndividual ;
  a foaf:Document ;
  a sto:Publication ;
  a sto:TechnicalSpecification ;
  terms:creator sto:sebastian ;
  rdfs:comment "Alljoyn - An open source software framework that makes it easy for devices and apps to discover and communicate with each other. (source: https://www.postscapes.com/internet-of-things-protocols/)"@en ;
  rdfs:label "Alljoyn"@en ;
  sto:hasOfficialResource <https://allseenalliance.org/framework> ;
.
sto:AnnoActuation
  a <https://www.w3.org/ns/oaAnnotation> ;
  <https://www.w3.org/ns/oahasBody> sto:Actuation ;
  <https://www.w3.org/ns/oahasTarget> [
      a <https://www.w3.org/ns/oaSpecificResource> ;
      terms:format "pdf" ;
      <https://www.w3.org/ns/oahasSelector> [
          a <https://www.w3.org/ns/oaRangeSelector> ;
          <https://www.w3.org/ns/oahasEndSelector> [
              a <https://www.w3.org/ns/oaXPathSelector> ;
              rdf:value "Page 29" ;
            ] ;
          <https://www.w3.org/ns/oahasStartSelector> [
              a <https://www.w3.org/ns/oaXPathSelector> ;
              rdf:value "Page 28" ;
            ] ;
        ] ;
      <https://www.w3.org/ns/oahasSource> sto:IIC_PUB_G1_V1_80_20170131 ;
    ] ;
.
sto:AnnoAiiClassification
  a <https://www.w3.org/ns/oaAnnotation> ;
  <https://www.w3.org/ns/oahasBody> sto:AiiClassification ;
  <https://www.w3.org/ns/oahasTarget> [
      a <https://www.w3.org/ns/oaSpecificResource> ;
      terms:format "pdf" ;
      <https://www.w3.org/ns/oahasSource> sto:Industrial_Internet_Architecture_Version_1 ;
    ] ;
.
sto:Anonymity
  a owl:NamedIndividual ;
  a sto:Concern ;
  <http://voag.linkedmodel.org/voag#hasStakeholder> <http://purl.oclc.org/NET/mvco.owl#EndUser> ;
  rdfs:comment "Anonymity is the guarantee for a user to interact with a system without being tracked or connected to its real-world identity."@en ;
  rdfs:label "Anonymity"@en ;
  rdfs:seeAlso "IoT-A Requirement UNI.001" ;
  rdfs:seeAlso "IoT-A Requirement UNI.322" ;
  rdfs:seeAlso "UNI.322"@en ;
  sto:hasDBpediaResource <http://dbpedia.org/resource/Anonymity> ;
  sto:hasDBpediaResource <http://dbpedia.org/resource/Anonymous_web_browsing> ;
  sto:supports sto:Privacy ;
.
sto:AoutonomousCommunication
  rdfs:seeAlso "IoT-A Requirement UNI.247" ;
.
sto:ArchitectureDescription
  a owl:Class ;
  rdfs:comment """A Reference Architecture describes the structure of a system with its element types and their structures, as well as their interaction types, among each other and with their environment. Describing this, a Reference Architecture defines restrictions for an instantiation (concrete architecture). Through abstraction from individual details, a Reference Architecture is universally valid within a specific domain. Further architectures with the same functional requirements can be constructed based on the reference architecture. Along with reference architectures comes a recommendation, based on experiences from existing developments as well as from a wide acceptance and recognition by its users or per definition. [ISO/IEC42010]

Note: It is important to distinguish the Reference Architecture from a Reference Architecture Description. While the first refers to a mental model or shared concept, the second is potentially only one of several different documents describing this model."""@en ;
  rdfs:comment "ISO 42010 definition of an Architecture Description"@en ;
  rdfs:label "Architecture Description" ;
  rdfs:seeAlso "https://www.iso.org/standard/50508.html" ;
  rdfs:subClassOf sto:StandardizationFramework ;
.
sto:ArrowheadFramework
  a owl:NamedIndividual ;
  a sto:IIoTConsortium ;
  a sto:StandardizationFramework ;
  rdfs:label "Arrowhead Framework" ;
  sto:hasPublisher :ArrowheadProject ;
  sto:seeAlso <http://www.arrowhead.eu/> ;
.
sto:AssetManagement
  a owl:NamedIndividual ;
  a sto:Concern ;
  terms:creator sto:Priyanka ;
  rdfs:comment "The concern of being able to manage the system onboarding, configuration, policy, software/firmware updates and other lifecycle management operations."@en ;
  rdfs:label "Asset Management"@en ;
  skos:note "Publications referred: 'IIC:PUB:G1:V1.80:20170131' '6.1 THE CONTROL DOMAIN' 'Page 29' " ;
  sto:hasWikipediaArticle <https://en.wikipedia.org/wiki/Asset_management#Physical_and_Infrastructure_asset_management> ;
  sto:supports sto:IoT ;
.
sto:Authentication
  a owl:NamedIndividual ;
  a sto:Concern ;
  terms:creator sto:sebastian ;
  rdfs:comment "Authentication before opening a valid connection; this can be done by just verifying the server identity or doing mutual authentication."@en ;
  rdfs:label "Authentication"@en ;
  rdfs:seeAlso "IoT-A Requirement UNI.612" ;
  rdfs:seeAlso "IoT-A Requirement UNI.618" ;
  rdfs:seeAlso "https://ieeexplore.ieee.org/document/6188257"@en ;
  rdfs:seeAlso "https://ieeexplore.ieee.org/document/7919553"@en ;
  rdfs:seeAlso "https://ieeexplore.ieee.org/document/8327600" ;
  rdfs:seeAlso "https://ieeexplore.ieee.org/document/8552311"@en ;
  sto:supports sto:IdentityManagement ;
.
sto:Authorization
  a owl:NamedIndividual ;
  a sto:Concern ;
  rdfs:seeAlso "IoT-A Requirement UNI.319" ;
  rdfs:seeAlso "IoT-A Requirement UNI.502" ;
  rdfs:seeAlso "IoT-A Requirement UNI.503" ;
  rdfs:seeAlso "https://ieeexplore.ieee.org/document/7919553"@en ;
  rdfs:seeAlso "https://ieeexplore.ieee.org/document/8552311"@en ;
  sto:supports sto:Privacy ;
.
sto:Auto_Scaling
  a owl:NamedIndividual ;
  a sto:Concern ;
  terms:creator sto:MuhammadUsman ;
  rdfs:comment "Autoscaling, also spelled auto scaling or auto-scaling, and sometimes also called automatic scaling, is a method used in cloud computing, whereby the amount of computational resources in a server farm, typically measured in terms of the number of active servers, scales automatically based on the load on the farm. It is closely related to, and builds upon, the idea of load balancing."@en ;
  rdfs:label "Auto Scaling"@en ;
  skos:note "TODO already covered by scalability?"@en ;
  sto:hasWikipediaArticle "https://en.wikipedia.org/wiki/Autoscaling"@en ;
  sto:supports sto:Scalability ;
.
sto:Automation
  a owl:NamedIndividual ;
  a sto:RelevantSubject ;
  rdfs:comment "Technology with which a process or procedure is performed with minimal human intervention "@en ;
  rdfs:label "Automation"@en ;
  sto:hasWikipediaArticle <https://en.wikipedia.org/wiki/Automation> ;
.
sto:AutonomousCommunication
  a owl:NamedIndividual ;
  a sto:Concern ;
  <http://voag.linkedmodel.org/voag#hasStakeholder> <https://www.wikidata.org/wiki/Q1548249> ;
  rdfs:comment "Authonomous Communication frames all requirements in order to autonomously establish communication channels between participants of a network. In most cases, this will be a machine-to-machine communication channel. Main challenges are related to interoperability."@en ;
  rdfs:label "Autonomous Communication"@en ;
  rdfs:seeAlso "IoT-A Requirement UNI.005" ;
  rdfs:seeAlso "IoT-A Requirement UNI.012" ;
  rdfs:seeAlso "IoT-A Requirement UNI.708" ;
  sto:supports sto:Communication ;
  sto:supports sto:ServiceChoreography ;
.
sto:AutonomousConfiguration
  a owl:NamedIndividual ;
  a sto:Concern ;
  <http://voag.linkedmodel.org/voag#hasStakeholder> <https://www.wikidata.org/wiki/Q1548249> ;
  rdfs:comment "A system built using the Reference Architecture shall be able to remotely control and configure devices."@en ;
  rdfs:label "Autonomous Configuration"@en ;
  rdfs:seeAlso "IoT-A Requirement UNI.015" ;
  rdfs:seeAlso "IoT-A Requirement UNI.031" ;
  rdfs:seeAlso "IoT-A Requirement UNI.032" ;
  rdfs:seeAlso "IoT-A Requirement UNI.060" ;
  rdfs:seeAlso "IoT-A Requirement UNI.247" ;
  rdfs:seeAlso "IoT-A Requirement UNI.509" ;
  rdfs:seeAlso "IoT-A Requirement UNI.704" ;
  rdfs:seeAlso "IoT-A Requirement UNI.706" ;
  rdfs:seeAlso "IoT-A Requirement UNI.717" ;
  skos:note "Publications referred: '<https://doi.org/10.1016/j.jksuci.2016.10.003>' '1.2. Utilities of IoT' 'Page 295'" ;
  sto:supports sto:ServiceChoreography ;
.
sto:Availability
  a owl:NamedIndividual ;
  a sto:Concern ;
  terms:creator sto:sebastian ;
  rdfs:comment "In reliability theory and reliability engineering, the term availability has the following meanings: * The degree to which a system, subsystem or equipment is in a specified operable and committable state at the start of a mission, when the mission is called for at an unknown, i.e. a random, time. Simply put, availability is the proportion of time a system is in a functioning condition. This is often described as a mission capable rate. Mathematically, this is expressed as 100% minus unavailability. * The ratio of (a) the total time a functional unit is capable of being used during a given interval to (b) the length of the interval. For example, a unit that is capable of being used 100 hours per week (168 hours) would have an availability of 100/168. However, typical availability values are specified in decimal (such as 0.9998). In high availability applications, a metric known as nines, corresponding to the number of nines following the decimal point, is used. With this convention, \"five nines\" equals 0.99999 (or 99.999%) availability. (source: wikipedia)"@en ;
  rdfs:label "Availability"@en ;
  rdfs:seeAlso sto:OpenFogArchitecture ;
  rdfs:seeAlso "IoT-A Requirement UNI.058" ;
  rdfs:seeAlso "IoT-A Requirement UNI.064" ;
  rdfs:seeAlso "IoT-A Requirement UNI.239" ;
  rdfs:seeAlso "IoT-A Requirement UNI.321" ;
  rdfs:seeAlso "IoT-A Requirement UNI.601" ;
  rdfs:seeAlso "IoT-A Requirement UNI.610" ;
  rdfs:seeAlso "IoT-A Requirement UNI.616" ;
  rdfs:seeAlso "https://dl.acm.org/citation.cfm?doid=3108421.3108426"@en ;
  rdfs:seeAlso "https://ieeexplore.ieee.org/document/7919553"@en ;
  rdfs:seeAlso "https://ieeexplore.ieee.org/document/8327600" ;
  rdfs:seeAlso "https://ieeexplore.ieee.org/document/8463303"@en ;
  rdfs:seeAlso "https://ieeexplore.ieee.org/document/8474855"@en ;
  skos:note "Publications referred: '<https://www.openfogconsortium.org/wp-content/uploads/OpenFog_Reference_Architecture_2_09_17-FINAL.pdf> OPFRA001.020817' '4.6 Reliability, Availability, and Serviceability (RAS)Pillar' 'Page 29' " ;
  sto:hasDBpediaResource <http://dbpedia.org/resource/Availability> ;
  sto:supports sto:Reliability ;
.
sto:Awareness
  a owl:NamedIndividual ;
  a sto:Concern ;
  terms:creator sto:MuhammadUsman ;
  rdfs:comment "Awareness is the ability to directly know and perceive, to feel, or to be cognizant of events. More broadly, it is the state of being conscious of something. Another definition describes it as a state wherein a subject is aware of some information when that information is directly available to bring to bear in the direction of a wide range of behavioral processes. The concept is often synonymous to consciousness and is also understood as being consciousness itself."@en ;
  rdfs:label "Awareness"@en ;
  rdfs:seeAlso "https://ieeexplore.ieee.org/document/7488250" ;
  sto:hasWikipediaArticle "https://en.wikipedia.org/wiki/Awareness"@en ;
  sto:supports sto:EdgeComputing ;
.
sto:B2MML
  a owl:NamedIndividual ;
  a foaf:Document ;
  a sto:Publication ;
  a sto:Standard ;
  terms:creator sto:MESA ;
  rdfs:comment "B2MML or Business To Manufacturing Markup Language is an XML implementation of the ANSI/ISA-95 family of standards (ISA-95)"@en ;
  rdfs:label "Business To Manufacturing Markup Language" ;
  skos:altLabel "IEC 62264"@en ;
  foaf:maker sto:MESA ;
  sto:hasClassification sto:BusinessProcessExecution ;
  sto:hasClassification sto:EnterpriseLevel ;
  sto:hasDBpediaResource <http://dbpedia.org/resource/B2MML> ;
  sto:hasDeveloper sto:MESA ;
  sto:hasOfficialResource <https://services.mesa.org/ResourceLibrary/ShowResource/0f47758b-60f0-40c6-a71b-fa7b2363fb3a> ;
  sto:hasPublisher sto:MESA ;
  sto:hasWikipediaArticle <https://en.wikipedia.org/wiki/B2MML> ;
  sto:isImplementationOf sto:ISA-95 ;
  sto:relatedTo sto:B2MML ;
  sto:relatedTo sto:IEC_62264 ;
  sto:relatedTo sto:ISA-95 ;
.
sto:BBF
  a owl:NamedIndividual ;
  a foaf:Organization ;
  a sto:StandardOrganization ;
  rdfs:comment "The Broadband Forum is a non-profit industry consortium dedicated to developing broadband network specifications. Members include telecommunications networking and service provider companies, broadband device and equipment vendors, consultants and independent testing labs (ITLs). Service provider members are primarily wire-line service providers (non-mobile) telephone companies."@en ;
  rdfs:label "Broadband Forum"@en ;
  sto:abbreviation "BBF" ;
  sto:formationDate "2008-01-01"^^xsd:date ;
  sto:hasDBpediaResource <http://dbpedia.org/resource/Broadband_Forum> ;
  sto:hasHeadquaterIn dbr:_California ;
  sto:hasOfficialResource <https://www.broadband-forum.org/> ;
  sto:hasWikipediaArticle <https://en.wikipedia.org/wiki/Broadband_Forum> ;
  sto:orgName "Broadband Forum"@en ;
.
sto:BBF_TR-069
  a owl:NamedIndividual ;
  a foaf:Document ;
  a sto:Publication ;
  a sto:Standard ;
  terms:creator sto:BBF ;
  rdfs:comment "Digital Enhanced Cordless Telecommunications (DECT) is the ETSI standard for short-range cordless communications, which can be adapted for many applications and can be used over unlicensed frequency allocations world-wide."@en ;
  rdfs:label "BBF TR-069"@en ;
  foaf:maker sto:BBF ;
  sto:hasDBpediaResource <http://dbpedia.org/resource/TR-069> ;
  sto:hasDeveloper sto:BBF ;
  sto:hasOfficialResource <https://www.broadband-forum.org/standards-and-software/technical-specifications/tr-069-files-tools> ;
  sto:hasPublisher sto:BBF ;
  sto:hasTag "CPE WAN Management Protocol"@en ;
  sto:hasWikipediaArticle <https://en.wikipedia.org/wiki/TR-069> ;
.
sto:BDI
  a owl:NamedIndividual ;
  a foaf:Organization ;
  a sto:StandardOrganization ;
  terms:creator sto:sebastian ;
  terms:title "The Federation of German Industries"@en ;
  rdfs:comment "The Federation of German Industries represents a large proportion of the German manufacturing industry."@en ;
  sto:hasOfficialResource <https://english.bdi.eu/> ;
.
sto:BPEL
  a owl:NamedIndividual ;
  a foaf:Document ;
  a sto:Publication ;
  a sto:Standard ;
  terms:creator sto:OASIS ;
  rdfs:comment "The Web Services Business Process Execution Language (WS-BPEL), commonly known as BPEL Business Process Execution Language, is a standard executable language for specifying actions within business processes with web services."@en ;
  rdfs:label "Business Process Execution Language"@en ;
  foaf:maker sto:OASIS ;
  sto:hasClassification sto:BusinessProcessExecution ;
  sto:hasDBpediaResource <http://dbpedia.org/resource/Business_Process_Execution_Language> ;
  sto:hasOfficialResource <https://www.oasis-open.org/committees/tc_home.php?wg_abbrev=wsbpel> ;
  sto:hasPublisher sto:OASIS ;
  sto:hasTag "BPEL"@en ;
  sto:hasWikipediaArticle <https://en.wikipedia.org/wiki/Business_Process_Execution_Language> ;
.
sto:BPMN
  a owl:NamedIndividual ;
  a foaf:Document ;
  a sto:Publication ;
  a sto:Standard ;
  terms:creator sto:OMG ;
  rdfs:comment "Business Process Model and Notation is a graphical representation for specifying business processes in a business process model."@en ;
  rdfs:label "Business Process Model Notation"@en ;
  foaf:maker sto:OMG ;
  sto:hasClassification sto:SCM ;
  sto:hasDBpediaResource <http://dbpedia.org/page/Business_Process_Model_and_Notation> ;
  sto:hasDeveloper sto:OMG ;
  sto:hasOfficialResource <http://www.bpmn.org/> ;
  sto:hasTag "BPMN"@en ;
  sto:hasWikipediaArticle <https://en.wikipedia.org/wiki/Business_Process_Model_and_Notation> ;
.
sto:Bandwidth
  a owl:NamedIndividual ;
  a sto:Concern ;
  terms:creator sto:MuhammadUsman ;
  rdfs:comment "In computing, bandwidth is the maximum rate of data transfer across a given path. Bandwidth may be characterized as network bandwidth, data bandwidth, or digital bandwidth."@en ;
  rdfs:label "Bandwidth"@en ;
  rdfs:seeAlso "https://ieeexplore.ieee.org/document/6188257"@en ;
  rdfs:seeAlso "https://ieeexplore.ieee.org/document/7488250" ;
  sto:hasWikipediaArticle "https://en.wikipedia.org/wiki/Bandwidth_(computing)"@en ;
  sto:supports sto:Communication ;
.
sto:BdvaCloudAndHighPerformanceComputing
  a owl:NamedIndividual ;
  a sto:BdvaConcern ;
  a sto:StandardClassification ;
  terms:creator sto:sebastian ;
  dul:associatedWith sto:IIRAApplicationDomain ;
  rdfs:comment "The Cloud and High Performance Computing (HPC): Effective Big Data processing and data management might imply the effective usage of Cloud and High Performance Computing infrastructures. This area is separately elaborated further in collaboration with the Cloud and High Performance Computing (ETP4HPC) communities."@en ;
  rdfs:label "BDVA Cloud and High Performance Computing"@en ;
  sto:alignsWith sto:IIRAApplicationDomain ;
  sto:frames sto:AI ;
  sto:frames sto:BigDataApplications ;
  sto:frames sto:CloudComputing ;
  sto:frames sto:DataAnalytics ;
  sto:frames sto:DataProcessing ;
  sto:frames sto:DataPublishing ;
  sto:frames sto:MachineLearning ;
  sto:isDescribedin sto:BdvaSira ;
.
sto:BdvaCloudAndHighPerformanceComputingAnno
  a <https://www.w3.org/ns/oaAnnotation> ;
  <https://www.w3.org/ns/oahasBody> sto:BdvaCloudAndHighPerformanceComputing ;
  <https://www.w3.org/ns/oahasTarget> [
      a <https://www.w3.org/ns/oaSpecificResource> ;
      <https://www.w3.org/ns/oahasSelector> [
          a <https://www.w3.org/ns/oaRangeSelector> ;
          <https://www.w3.org/ns/oahasEndSelector> [
              a <https://www.w3.org/ns/oaXPathSelector> ;
              rdf:value "Page 40" ;
            ] ;
          <https://www.w3.org/ns/oahasStartSelector> [
              a <https://www.w3.org/ns/oaXPathSelector> ;
              rdf:value "Page 37" ;
            ] ;
        ] ;
      <https://www.w3.org/ns/oahasSource> sto:European_BDV_SRIA_version_4_0 ;
    ] ;
.
sto:BdvaCommunicationConnectivity
  a owl:NamedIndividual ;
  a sto:BdvaConcern ;
  a sto:StandardClassification ;
  terms:creator sto:sebastian ;
  rdfs:comment "Effective communication and connectivity mechanisms are necessary in providing support for Big Data. This area is separately further elaborated, along with various communication communities, such as the 5G community."@en ;
  rdfs:label "BDVA Communication and Connectivity"@en ;
  sto:frames sto:Communication ;
  sto:frames sto:DataAccess ;
  sto:frames sto:DataAnalytics ;
  sto:frames sto:Interoperability ;
  sto:frames sto:QualityOfService ;
  sto:frames sto:SemanticInteroperability ;
  sto:frames sto:ServiceDescription ;
  sto:isDescribedin sto:BdvaSira ;
.
sto:BdvaCommunicationConnectivityAnno
  a <https://www.w3.org/ns/oaAnnotation> ;
  <https://www.w3.org/ns/oahasBody> sto:BdvaCommunicationConnectivity ;
  <https://www.w3.org/ns/oahasTarget> [
      a <https://www.w3.org/ns/oaSpecificResource> ;
      <https://www.w3.org/ns/oahasSelector> [
          a <https://www.w3.org/ns/oaRangeSelector> ;
          <https://www.w3.org/ns/oahasEndSelector> [
              a <https://www.w3.org/ns/oaXPathSelector> ;
              rdf:value "Page 40" ;
            ] ;
          <https://www.w3.org/ns/oahasStartSelector> [
              a <https://www.w3.org/ns/oaXPathSelector> ;
              rdf:value "Page 37" ;
            ] ;
        ] ;
      <https://www.w3.org/ns/oahasSource> sto:European_BDV_SRIA_version_4_0 ;
    ] ;
.
sto:BdvaConcern
  a owl:Class ;
  a owl:NamedIndividual ;
  terms:creator sto:sebastian ;
  terms:creator "sebastian" ;
  terms:creator "sebastian"@en ;
  rdfs:comment """The BDV Reference Model distinguishes between two different elements. On the one hand, it describes the elements that are at the core of the BDVA; on the other, it outlines the features that are developed in strong collaboration with related European activities. The BDV Reference Model is structured into horizontal and vertical concerns.
Horizontal concerns cover specific aspects along the data processing
Vertical concerns address cross-cutting issues, which may affect all the horizontal concerns. In addition, vertical concerns may also involve non-technical aspects."""@en ;
  rdfs:comment """The BDV Reference Model distinguishes between two different elements. On the one hand, it describes the elements that are at the core of the BDVA; on the other, it outlines the features that are developed in strong collaboration with related European activities. The BDV Reference Model is structured into horizontal and vertical concerns.
Horizontal concerns cover specific aspects along the data processing Vertical concerns address cross-cutting issues, which may affect all the horizontal concerns. In addition, vertical concerns may also involve non-technical aspects."""@en ;
  rdfs:comment "The BDV Reference Model distinguishes between two different elements. On the one hand, it describes the elements that are at the core of the BDVA; on the other, it outlines the features that are developed in strong collaboration with related European activities. The BDV Reference Model is structured into horizontal and vertical concerns. Horizontal concerns cover specific aspects along the data processing Vertical concerns address cross-cutting issues, which may affect all the horizontal concerns. In addition, vertical concerns may also involve non-technical aspects."@en ;
  rdfs:label "BDVA Concern"@en ;
  rdfs:subClassOf sto:StandardClassification ;
  sto:hasOfficialResource <http://www.bdva.eu/sites/default/files/BDVA_SRIA_v4_Ed1.1.pdf> ;
.
sto:BdvaConcernAnno
  a <https://www.w3.org/ns/oaAnnotation> ;
  <https://www.w3.org/ns/oahasBody> sto:BdvaConcern ;
  <https://www.w3.org/ns/oahasTarget> [
      a <https://www.w3.org/ns/oaSpecificResource> ;
      <https://www.w3.org/ns/oahasSelector> [
          a <https://www.w3.org/ns/oaRangeSelector> ;
          <https://www.w3.org/ns/oahasEndSelector> [
              a <https://www.w3.org/ns/oaXPathSelector> ;
              rdf:value "Page 40" ;
            ] ;
          <https://www.w3.org/ns/oahasStartSelector> [
              a <https://www.w3.org/ns/oaXPathSelector> ;
              rdf:value "Page 37" ;
            ] ;
        ] ;
      <https://www.w3.org/ns/oahasSource> sto:European_BDV_SRIA_version_4_0 ;
    ] ;
  <https://www.w3.org/ns/oahasTarget> [
      a <https://www.w3.org/ns/oaSpecificResource> ;
      <https://www.w3.org/ns/oahasSelector> [
          a <https://www.w3.org/ns/oaRangeSelector> ;
          <https://www.w3.org/ns/oahasEndSelector> [
              a <https://www.w3.org/ns/oaXPathSelector> ;
              rdf:value "Page 40" ;
            ] ;
          <https://www.w3.org/ns/oahasStartSelector> [
              a <https://www.w3.org/ns/oaXPathSelector> ;
              rdf:value "Page 38" ;
            ] ;
        ] ;
      <https://www.w3.org/ns/oahasSource> sto:European_BDV_SRIA_version_4_0 ;
    ] ;
.
sto:BdvaCyberSecurityTrust
  a owl:NamedIndividual ;
  a sto:BdvaConcern ;
  a sto:StandardClassification ;
  terms:creator sto:sebastian ;
  dul:associatedWith rami:Security ;
  dul:associatedWith sto:IDSRAMSecurity ;
  dul:associatedWith sto:IIRASecurityFramework ;
  rdfs:comment """Big Data often need support to maintain security and trust beyond privacy and anonymisation. The aspect of trust frequently has links to trust 
mechanisms such as blockchain technologies, smart contracts and various forms of encryption."""@en ;
  rdfs:label "BDVA Cybersecurity and Trust"@en ;
  sto:alignsWith rami:Security ;
  sto:alignsWith sto:IDSRAMSecurity ;
  sto:alignsWith sto:IIRASecurityFramework ;
  sto:frames sto:Communication ;
  sto:frames sto:DataSovereignty ;
  sto:frames sto:IntegrityProtection ;
  sto:frames sto:Privacy ;
  sto:frames sto:SecureCommunication ;
  sto:frames sto:Security ;
  sto:frames sto:Trustworthiness ;
  sto:isDescribedin sto:BdvaSira ;
.
sto:BdvaCyberSecurityTrustAnno
  a <https://www.w3.org/ns/oaAnnotation> ;
  <https://www.w3.org/ns/oahasBody> sto:BdvaCyberSecurityTrust ;
  <https://www.w3.org/ns/oahasTarget> [
      a <https://www.w3.org/ns/oaSpecificResource> ;
      <https://www.w3.org/ns/oahasSelector> [
          a <https://www.w3.org/ns/oaRangeSelector> ;
          <https://www.w3.org/ns/oahasEndSelector> [
              a <https://www.w3.org/ns/oaXPathSelector> ;
              rdf:value "Page 40" ;
            ] ;
          <https://www.w3.org/ns/oahasStartSelector> [
              a <https://www.w3.org/ns/oaXPathSelector> ;
              rdf:value "Page 37" ;
            ] ;
        ] ;
      <https://www.w3.org/ns/oahasSource> sto:European_BDV_SRIA_version_4_0 ;
    ] ;
.
sto:BdvaDataAnalytics
  a owl:NamedIndividual ;
  a sto:BdvaConcern ;
  a sto:StandardClassification ;
  terms:creator sto:sebastian ;
  dul:associatedWith sto:IDSRAMProcessLayer ;
  dul:associatedWith sto:InformationDomain ;
  dul:associatedWith sto:RAMIFunctionalLayer ;
  dul:associatedWith sto:RAMIInformationLayer ;
  rdfs:comment "Data analytics to improve data understanding, deep learning and the meaningfulness of data."@en ;
  rdfs:label "BDVA Data Analytics"@en ;
  sto:alignsWith sto:IDSRAMProcessLayer ;
  sto:alignsWith sto:InformationDomain ;
  sto:alignsWith sto:RAMIFunctionalLayer ;
  sto:alignsWith sto:RAMIInformationLayer ;
  sto:frames sto:AI ;
  sto:frames sto:DataAnalytics ;
  sto:frames sto:DataProcessing ;
  sto:frames sto:MachineLearning ;
  sto:frames sto:StreamProcessing ;
  sto:frames sto:Trustworthiness ;
  sto:isDescribedin sto:BdvaSira ;
.
sto:BdvaDataAnalyticsAnno
  a <https://www.w3.org/ns/oaAnnotation> ;
  <https://www.w3.org/ns/oahasBody> sto:BdvaDataAnalytics ;
  <https://www.w3.org/ns/oahasTarget> [
      a <https://www.w3.org/ns/oaSpecificResource> ;
      <https://www.w3.org/ns/oahasSelector> [
          a <https://www.w3.org/ns/oaRangeSelector> ;
          <https://www.w3.org/ns/oahasEndSelector> [
              a <https://www.w3.org/ns/oaXPathSelector> ;
              rdf:value "Page 40" ;
            ] ;
          <https://www.w3.org/ns/oahasStartSelector> [
              a <https://www.w3.org/ns/oaXPathSelector> ;
              rdf:value "Page 37" ;
            ] ;
        ] ;
      <https://www.w3.org/ns/oahasSource> sto:European_BDV_SRIA_version_4_0 ;
    ] ;
.
sto:BdvaDataManagement
  a owl:NamedIndividual ;
  a sto:BdvaConcern ;
  a sto:StandardClassification ;
  terms:creator sto:sebastian ;
  dul:associatedWith sto:IDSRAMInformationLayer ;
  dul:associatedWith sto:IDSRAMProcessLayer ;
  dul:associatedWith sto:RAMIInformationLayer ;
  rdfs:comment "Principles and techniques for data management"@en ;
  rdfs:label "BDVA Data Management"@en ;
  sto:alignsWith sto:IDSRAMInformationLayer ;
  sto:alignsWith sto:IDSRAMProcessLayer ;
  sto:alignsWith sto:RAMIInformationLayer ;
  sto:frames sto:BigDataApplications ;
  sto:frames sto:DataQuality ;
  sto:frames sto:Interoperability ;
  sto:frames sto:ProvenanceTracking ;
  sto:frames sto:Security ;
  sto:frames sto:SemanticInteroperability ;
  sto:frames sto:SyntacticInteroperability ;
  sto:frames sto:Trustworthiness ;
  sto:isDescribedin sto:BdvaSira ;
.
sto:BdvaDataManagementAnno
  a <https://www.w3.org/ns/oaAnnotation> ;
  <https://www.w3.org/ns/oahasBody> sto:BdvaDataManagement ;
  <https://www.w3.org/ns/oahasTarget> [
      a <https://www.w3.org/ns/oaSpecificResource> ;
      <https://www.w3.org/ns/oahasSelector> [
          a <https://www.w3.org/ns/oaRangeSelector> ;
          <https://www.w3.org/ns/oahasEndSelector> [
              a <https://www.w3.org/ns/oaXPathSelector> ;
              rdf:value "Page 40" ;
            ] ;
          <https://www.w3.org/ns/oahasStartSelector> [
              a <https://www.w3.org/ns/oaXPathSelector> ;
              rdf:value "Page 37" ;
            ] ;
        ] ;
      <https://www.w3.org/ns/oahasSource> sto:European_BDV_SRIA_version_4_0 ;
    ] ;
.
sto:BdvaDataProcessingArchitectures
  a owl:NamedIndividual ;
  a sto:BdvaConcern ;
  a sto:StandardClassification ;
  terms:creator sto:sebastian ;
  dul:associatedWith sto:IDSRAMProcessLayer ;
  dul:associatedWith sto:IIRAConnectivity ;
  dul:associatedWith sto:InformationDomain ;
  rdfs:comment "Optimised and scalable architectures for analytics of both data-at-rest and data-in-motion, with low latency delivering real-time analytics."@en ;
  rdfs:label "BDVA Data Processing Architectures"@en ;
  sto:alignsWith sto:IDSRAMProcessLayer ;
  sto:alignsWith sto:IIRAConnectivity ;
  sto:alignsWith sto:InformationDomain ;
  sto:frames sto:BigDataApplications ;
  sto:frames sto:Communication ;
  sto:frames sto:DataAtRest ;
  sto:frames sto:DataInMotion ;
  sto:frames sto:DataProcessing ;
  sto:frames sto:Scalability ;
  sto:frames sto:StreamProcessing ;
  sto:isDescribedin sto:BdvaSira ;
.
sto:BdvaDataProcessingArchitecturesAnno
  a <https://www.w3.org/ns/oaAnnotation> ;
  <https://www.w3.org/ns/oahasBody> sto:BdvaDataProcessingArchitectures ;
  <https://www.w3.org/ns/oahasTarget> [
      a <https://www.w3.org/ns/oaSpecificResource> ;
      <https://www.w3.org/ns/oahasSelector> [
          a <https://www.w3.org/ns/oaRangeSelector> ;
          <https://www.w3.org/ns/oahasEndSelector> [
              a <https://www.w3.org/ns/oaXPathSelector> ;
              rdf:value "Page 40" ;
            ] ;
          <https://www.w3.org/ns/oahasStartSelector> [
              a <https://www.w3.org/ns/oaXPathSelector> ;
              rdf:value "Page 37" ;
            ] ;
        ] ;
      <https://www.w3.org/ns/oahasSource> sto:European_BDV_SRIA_version_4_0 ;
    ] ;
.
sto:BdvaDataProtection
  a owl:NamedIndividual ;
  a sto:BdvaConcern ;
  a sto:StandardClassification ;
  terms:creator sto:sebastian ;
  dul:associatedWith sto:IDSRAMSecurity ;
  dul:associatedWith sto:IIRASecurityFramework ;
  rdfs:comment "Privacy and anonymisation mechanisms to facilitate data protection. This is shown related to data management and processing as there is a strong link here, but it can also be associated with the area of cybersecurity."@en ;
  rdfs:label "BDVA Data Protection"@en ;
  sto:alignsWith sto:IDSRAMSecurity ;
  sto:alignsWith sto:IIRASecurityFramework ;
  sto:frames sto:DataProtection ;
  sto:frames sto:DataSovereignty ;
  sto:frames sto:Privacy ;
  sto:frames sto:Trustworthiness ;
  sto:isDescribedin sto:BdvaSira ;
.
sto:BdvaDataProtectionAnno
  a <https://www.w3.org/ns/oaAnnotation> ;
  <https://www.w3.org/ns/oahasBody> sto:BdvaDataProtection ;
  <https://www.w3.org/ns/oahasTarget> [
      a <https://www.w3.org/ns/oaSpecificResource> ;
      <https://www.w3.org/ns/oahasSelector> [
          a <https://www.w3.org/ns/oaRangeSelector> ;
          <https://www.w3.org/ns/oahasEndSelector> [
              a <https://www.w3.org/ns/oaXPathSelector> ;
              rdf:value "Page 40" ;
            ] ;
          <https://www.w3.org/ns/oahasStartSelector> [
              a <https://www.w3.org/ns/oaXPathSelector> ;
              rdf:value "Page 37" ;
            ] ;
        ] ;
      <https://www.w3.org/ns/oahasSource> sto:European_BDV_SRIA_version_4_0 ;
    ] ;
.
sto:BdvaDataSharingPlatforms
  a owl:NamedIndividual ;
  a sto:BdvaConcern ;
  a sto:StandardClassification ;
  terms:creator sto:sebastian ;
  dul:associatedWith sto:IDSRAMReferenceArchitectureModel ;
  dul:associatedWith sto:IIRA ;
  rdfs:comment "Data sharing and trading are seen as important ecosystem enablers in the data economy, although closed and personal data present particular challenges for the free flow of data. The following two conceptual solutions – Industrial Data Platforms (IDPs) and Personal Data Platforms (PDPs) – introduce new approaches to addressing this particular need to regulate closed proprietary and personal data."@en ;
  rdfs:label "BDVA Data Sharing Platforms"@en ;
  sto:frames sto:BusinessContext ;
  sto:frames sto:DataEconomy ;
  sto:frames sto:DataPublishing ;
  sto:isDescribedin sto:BdvaSira ;
.
sto:BdvaDataSharingPlatformsAnno
  a <https://www.w3.org/ns/oaAnnotation> ;
  <https://www.w3.org/ns/oahasBody> sto:BdvaDataSharingPlatforms ;
  <https://www.w3.org/ns/oahasTarget> [
      a <https://www.w3.org/ns/oaSpecificResource> ;
      <https://www.w3.org/ns/oahasSelector> [
          a <https://www.w3.org/ns/oaRangeSelector> ;
          <https://www.w3.org/ns/oahasEndSelector> [
              a <https://www.w3.org/ns/oaXPathSelector> ;
              rdf:value "Page 40" ;
            ] ;
          <https://www.w3.org/ns/oahasStartSelector> [
              a <https://www.w3.org/ns/oaXPathSelector> ;
              rdf:value "Page 37" ;
            ] ;
        ] ;
      <https://www.w3.org/ns/oahasSource> sto:European_BDV_SRIA_version_4_0 ;
    ] ;
.
sto:BdvaDataVisualizationAndUserInteraction
  a owl:NamedIndividual ;
  a sto:BdvaConcern ;
  a sto:StandardClassification ;
  terms:creator sto:sebastian ;
  dul:associatedWith sto:IIRAUsageViewpoint ;
  dul:associatedWith sto:RAMIFunctionalLayer ;
  rdfs:comment "Engineering and DevOps for building Big Data Value systems: This topic will be elaborated in greater detail along with the NESSI Software and Service community."@en ;
  rdfs:label "Data Visualisation and User Interaction"@en ;
  sto:alignsWith sto:IIRAUsageViewpoint ;
  sto:alignsWith sto:RAMIFunctionalLayer ;
  sto:frames sto:BigDataApplications ;
  sto:isDescribedin sto:BdvaSira ;
.
sto:BdvaDataVisualizationAndUserInteractionAnno
  a <https://www.w3.org/ns/oaAnnotation> ;
  <https://www.w3.org/ns/oahasBody> sto:BdvaDataVisualizationAndUserInteraction ;
  <https://www.w3.org/ns/oahasTarget> [
      a <https://www.w3.org/ns/oaSpecificResource> ;
      <https://www.w3.org/ns/oahasSelector> [
          a <https://www.w3.org/ns/oaRangeSelector> ;
          <https://www.w3.org/ns/oahasEndSelector> [
              a <https://www.w3.org/ns/oaXPathSelector> ;
              rdf:value "Page 40" ;
            ] ;
          <https://www.w3.org/ns/oahasStartSelector> [
              a <https://www.w3.org/ns/oaXPathSelector> ;
              rdf:value "Page 37" ;
            ] ;
        ] ;
      <https://www.w3.org/ns/oahasSource> sto:European_BDV_SRIA_version_4_0 ;
    ] ;
.
sto:BdvaDevelopmentEngineering
  a owl:NamedIndividual ;
  a sto:BdvaConcern ;
  a sto:StandardClassification ;
  terms:creator sto:sebastian ;
  rdfs:comment "Engineering and DevOps for building Big Data Value systems: This topic will be elaborated in greater detail along with the NESSI Software and Service community."@en ;
  rdfs:label "BDVA Engineering and DevOps"@en ;
  sto:isDescribedin sto:BdvaSira ;
.
sto:BdvaDevelopmentEngineeringAnno
  a <https://www.w3.org/ns/oaAnnotation> ;
  <https://www.w3.org/ns/oahasBody> sto:BdvaDevelopmentEngineering ;
  <https://www.w3.org/ns/oahasTarget> [
      a <https://www.w3.org/ns/oaSpecificResource> ;
      <https://www.w3.org/ns/oahasSelector> [
          a <https://www.w3.org/ns/oaRangeSelector> ;
          <https://www.w3.org/ns/oahasEndSelector> [
              a <https://www.w3.org/ns/oaXPathSelector> ;
              rdf:value "Page 40" ;
            ] ;
          <https://www.w3.org/ns/oahasStartSelector> [
              a <https://www.w3.org/ns/oaXPathSelector> ;
              rdf:value "Page 37" ;
            ] ;
        ] ;
      <https://www.w3.org/ns/oahasSource> sto:European_BDV_SRIA_version_4_0 ;
    ] ;
.
sto:BdvaSira
  a owl:NamedIndividual ;
  a sto:StandardizationFramework ;
  terms:creator sto:sebastian ;
  terms:title "BDVA Strategic Research and Innovation Agenda"@en ;
  rdfs:comment "This Strategic Research and Innovation Agenda (SRIA) defines the overall goals, main technical and non-technical priorities, and a research and innovation roadmap for the European Public Private Partnership (PPP) on Big Data Value. The SRIA has been developed by the Big Data Value Association (BDVA), an industry-led organisation representing large businesses, small and medium-sized enterprises (SMEs), and research organisations in Europe."@en ;
  rdfs:label "BDVA SIRA"@en ;
  sto:hasPublisher :BDVA ;
.
sto:BdvaSiraAnno
  a <https://www.w3.org/ns/oaAnnotation> ;
  <https://www.w3.org/ns/oahasBody> sto:BdvaSira ;
  <https://www.w3.org/ns/oahasTarget> [
      a <https://www.w3.org/ns/oaSpecificResource> ;
      <https://www.w3.org/ns/oahasSelector> [
          a <https://www.w3.org/ns/oaRangeSelector> ;
          <https://www.w3.org/ns/oahasEndSelector> [
              a <https://www.w3.org/ns/oaXPathSelector> ;
              rdf:value "Page 106" ;
            ] ;
          <https://www.w3.org/ns/oahasStartSelector> [
              a <https://www.w3.org/ns/oaXPathSelector> ;
              rdf:value "Page 1" ;
            ] ;
        ] ;
      <https://www.w3.org/ns/oahasSource> sto:European_BDV_SRIA_version_4_0 ;
    ] ;
.
sto:BdvaStandards
  a owl:NamedIndividual ;
  a sto:BdvaConcern ;
  a sto:StandardClassification ;
  terms:creator sto:sebastian ;
  rdfs:comment "Standardisation of Big Data technology areas to facilitate data integration, sharing and interoperability"@en ;
  rdfs:label "BDVA Standards"@en ;
  sto:frames sto:BusinessContext ;
  sto:frames sto:Communication ;
  sto:frames sto:DataEconomy ;
  sto:frames sto:Interoperability ;
  sto:isDescribedin sto:BdvaSira ;
.
sto:BdvaStandardsAnno
  a <https://www.w3.org/ns/oaAnnotation> ;
  <https://www.w3.org/ns/oahasBody> sto:BdvaStandards ;
  <https://www.w3.org/ns/oahasTarget> [
      a <https://www.w3.org/ns/oaSpecificResource> ;
      <https://www.w3.org/ns/oahasSelector> [
          a <https://www.w3.org/ns/oaRangeSelector> ;
          <https://www.w3.org/ns/oahasEndSelector> [
              a <https://www.w3.org/ns/oaXPathSelector> ;
              rdf:value "Page 40" ;
            ] ;
          <https://www.w3.org/ns/oahasStartSelector> [
              a <https://www.w3.org/ns/oaXPathSelector> ;
              rdf:value "Page 37" ;
            ] ;
        ] ;
      <https://www.w3.org/ns/oahasSource> sto:European_BDV_SRIA_version_4_0 ;
    ] ;
.
sto:BdvaThingsAssetsSensorsActuators
  a owl:NamedIndividual ;
  a sto:BdvaConcern ;
  a sto:StandardClassification ;
  terms:creator sto:sebastian ;
  rdfs:comment "IoT, CPS, Edge and Fog Computing: A main source of Big Data is sensor data from an IoT context and actuator interaction in Cyber Physical Systems. In order to meet real-time needs it will often be necessary to handle Big Data aspects at the edge of the system. This area is separately elaborated further in collaboration with the IoT (Alliance for Internet of Things Innovation (AIOTI)) and CPS communities"@en ;
  rdfs:label "BDVA IoT CPS and Edge Computing"@en ;
  sto:frames sto:IoT ;
  sto:isDescribedin sto:BdvaSira ;
.
sto:BdvaThingsAssetsSensorsActuatorsAnno
  a <https://www.w3.org/ns/oaAnnotation> ;
  <https://www.w3.org/ns/oahasBody> sto:BdvaThingsAssetsSensorsActuators ;
  <https://www.w3.org/ns/oahasTarget> [
      a <https://www.w3.org/ns/oaSpecificResource> ;
      <https://www.w3.org/ns/oahasSelector> [
          a <https://www.w3.org/ns/oaRangeSelector> ;
          <https://www.w3.org/ns/oahasEndSelector> [
              a <https://www.w3.org/ns/oaXPathSelector> ;
              rdf:value "Page 40" ;
            ] ;
          <https://www.w3.org/ns/oahasStartSelector> [
              a <https://www.w3.org/ns/oaXPathSelector> ;
              rdf:value "Page 37" ;
            ] ;
        ] ;
      <https://www.w3.org/ns/oahasSource> sto:European_BDV_SRIA_version_4_0 ;
    ] ;
.
sto:BigDataApplications
  a owl:NamedIndividual ;
  a sto:Concern ;
  rdfs:comment "Big data is a term for data sets that are so large or complex that traditional data processing applications are inadequate to deal with them. Challenges include analysis, capture, data curation, search, sharing, storage, transfer, visualization, querying, updating and information privacy. The term \"big data\" often refers simply to the use of predictive analytics, user behavior analytics, or certain other advanced data analytics methods that extract value from data, and seldom to a particular size of data set. (source: wikipedia)"@en ;
  rdfs:label "Big Data Applications"@en ;
  sto:hasDBpediaResource <http://dbpedia.org/resource/Big_data> ;
  sto:supports sto:DataAnalytics ;
.
sto:Blockchain
  a owl:NamedIndividual ;
  a foaf:Document ;
  a sto:Publication ;
  a sto:TechnicalSpecification ;
  rdfs:comment "The term Blockchain refers to a set of technologies for distributed databases."@en ;
  rdfs:label "Blockchain"@en ;
  rdfs:seeAlso <https://web.archive.org/web/20140320135003/https://bitcoin.org/bitcoin.pdf> ;
  sto:hasDBpediaResource <http://dbpedia.org/resource/Blockchain.info> ;
.
sto:Bluetooth
  a owl:NamedIndividual ;
  a foaf:Document ;
  a sto:Publication ;
  a sto:TechnicalSpecification ;
  terms:creator sto:sebastian ;
  rdfs:comment "Bluetooth works in the 2.4 GHz ISM band and uses frequency hopping. With a data rate up to 3 Mbps and maximum range of 100m. Each application type which can use Bluetooth has its own profile.  (source: https://www.postscapes.com/internet-of-things-protocols/)"@en ;
  rdfs:label "Bluetooth"@en ;
  sto:hasClassification sto:RAMICommunicationLayer ;
  sto:hasOfficialResource <http://www.bluetooth.com/Pages/Bluetooth-Home.aspx> ;
.
sto:BusinessContext
  a owl:NamedIndividual ;
  a sto:Concern ;
  terms:creator sto:sebastian ;
  rdfs:comment "Electronic business, or e-business, is the application of information and communication technologies in support of all the activities of business. Commerce constitutes the exchange of products and services between businesses, groups and individuals and can be seen as one of the essential activities of any business. (source: wikipedia)"@en ;
  rdfs:label "Business Context"@en ;
  sto:hasDBpediaResource <http://dbpedia.org/resource/Electronic_business> ;
.
sto:BusinessCycleSCM
  a owl:Class ;
  rdfs:comment "Suply Chain Management Business Cycle."@en ;
  rdfs:isDefinedBy <http://nvlpubs.nist.gov/nistpubs/ir/2016/NIST.IR.8107.pdf> ;
  rdfs:label "Business Cycle SCM"@en ;
  rdfs:seeAlso "https://en.wikipedia.org/wiki/Supply_chain_management" ;
  rdfs:subClassOf sto:StandardClassification ;
.
sto:BusinessManager
  rdfs:comment " A business manager is responsible for the running of the business and to make large profits." ;
  rdfs:label "Business Manager"@en ;
  rdfs:seeAlso "IIC:PUB:G1:V1.80:20170131" ;
  rdfs:type sto:Stakeholder ;
  skos:note "Publications referred: 'IIC:PUB:G1:V1.80:20170131' '1.5 AUDIENCE' 'Page 7' " ;
  sto:hasWikipediaArticle "https://en.wikipedia.org/wiki/Business_manager" ;
.
sto:BusinessProcessExecution
  a owl:NamedIndividual ;
  a sto:BusinessCycleSCM ;
  a sto:StandardClassification ;
  rdfs:comment "Describes Business Process Execution concept."@en ;
  rdfs:label "Business Process Execution"@en ;
  sto:isDescribedin sto:NISTInitiative ;
.
sto:BusinessProcessManagement
  a owl:NamedIndividual ;
  a sto:Concern ;
  terms:title "Business process management"@en ;
  rdfs:comment "Business process management (BPM) is a field in operations management that focuses on improving corporate performance by managing and optimizing a company's business processes. It can therefore be described as a \"process optimization process.\" It is argued that BPM enables organizations to be more efficient, more effective and more capable of change than a functionally focused, traditional hierarchical management approach. These processes can impact the cost and revenue generation of an organization. As a policy-making approach, BPM sees processes as important assets of an organization that must be understood, managed, and developed to announce value-added products and services to clients or customers. This approach closely resembles other total quality management or continual improvement process methodologies and BPM proponents also claim that this approach can be supported, or enabled, through technology. As such, many BPM articles and scholars frequently discuss BPM from one of two viewpoints: people and/or technology. (source: wikipedia)"@en ;
  rdfs:label "BPM"@en ;
  rdfs:seeAlso "IoT-A Requirement UNI.211" ;
  rdfs:seeAlso "IoT-A Requirement UNI.212" ;
  rdfs:seeAlso "IoT-A Requirement UNI.214" ;
  rdfs:seeAlso "IoT-A Requirement UNI.215" ;
  rdfs:seeAlso "IoT-A Requirement UNI.229" ;
  sto:hasDBpediaResource <http://dbpedia.org/resource/Business_process_management> ;
  sto:supports sto:BusinessContext ;
.
sto:BusinessTransactions
  a owl:NamedIndividual ;
  a sto:Concern ;
  terms:creator sto:sebastian ;
  rdfs:comment "A financial transaction is an agreement, communication, or movement carried out between a buyer and a seller to exchange an asset for payment. It involves a change in the status of the finances of two or more businesses or individuals. The buyer and seller are separate entities or objects, often involving the exchange of items of value, such as information, goods, services, and money. It is still a transaction if the goods are exchanged at one time, and the money at another. This is known as a two-part transaction: part one is giving the money, part two is receiving the goods. (source: wikipedia)"@en ;
  rdfs:label "Business Transactions"@en ;
  sto:hasDBpediaResource <http://dbpedia.org/resource/Financial_transaction> ;
  sto:supports sto:BusinessContext ;
.
sto:BusinessValue
  a owl:NamedIndividual ;
  a sto:Concern ;
  terms:creator sto:sebastian ;
  rdfs:label "Business Value"@en ;
  skos:note "Publications referred: '(IIC:PUB:G1:V1.80:20170131' '4 BUSINESS VIEWPOINT' 'Page 20' " ;
  sto:supports sto:BusinessContext ;
.
sto:CAD
  a owl:NamedIndividual ;
  a sto:Domain ;
  rdfs:comment "Computer-Aided Design"@en ;
  rdfs:isDefinedBy <https://en.wikipedia.org/wiki/Computer-aided_design> ;
  rdfs:label "CAD" ;
  sto:domainName "Computer-Aided Design"@en ;
  sto:hasDBpediaResource <http://dbpedia.org/resource/Computer-aided_design> ;
.
sto:CASAGRAS
  a owl:NamedIndividual ;
  a foaf:Organization ;
  a sto:IIoTConsortium ;
  terms:creator sto:sebastian ;
  rdfs:comment "We are a key group of international partners representing Europe, the USA, China, Japan and Korea who has joined a strategic EU funded 7th Framework initiative that will look at global standards, regulatory and other issues concerning RFID and its role in realising an Internet of Things.  (source: https://www.postscapes.com/internet-of-things-protocols/)"@en ;
  rdfs:label "CASAGRAS"@en ;
  sto:hasOfficialResource <http://www.iot-casagras.org/page/standards-and-regulations> ;
.
sto:CCN
  a owl:NamedIndividual ;
  a foaf:Document ;
  a sto:Publication ;
  a sto:TechnicalSpecification ;
  terms:creator sto:sebastian ;
  rdfs:comment "Content-Centric Networking (CCN). Next-gen network architecture to solve challenges in content distribution scalability, mobility, and security. CCN directly routes and delivers named pieces of content at the packet level of the network, enabling automatic and application-neutral caching in memory wherever it’s located in the network. The result? Efficient and effective delivery of content wherever and whenever it is needed. Since the architecture enables these caching effects as an automatic side effect of packet delivery, memory can be used without building expensive application-level caching services. (source: https://www.postscapes.com/internet-of-things-protocols/)"@en ;
  rdfs:label "CCN"@en ;
  sto:hasOfficialResource <http://www.ccnx.org/> ;
.
sto:CGMES
  a owl:NamedIndividual ;
  a sto:RelevantSubject ;
  rdfs:comment "Specification for Energy Management"@en ;
  rdfs:label "CGMES: Common Grid Model Exchange Specification "@en ;
  sto:hasOpenResource <https://docstore.entsoe.eu/Documents/CIM_documents/IOP/CGMES_2_5_TechnicalSpecification_61970-600_Part%201_Ed2.pdf> ;
  sto:seeAlso <https://docstore.entsoe.eu/major-projects/common-information-model-cim/cim-for-grid-models-exchange/standards/Pages/default.aspx> ;
.
sto:CardinalityOfDataSources
  a owl:NamedIndividual ;
  a sto:Concern ;
  sto:supports sto:Interoperability ;
.
sto:CardinalityOfParticipants
  a owl:NamedIndividual ;
  a sto:Concern ;
  terms:creator sto:sebastian ;
  rdfs:comment "Data Artefacts from different Data Providers are delivered in order to provide additional insights (e.g. Collaborative Predictive Maintenance)."@en ;
  rdfs:label "Cardinality of Participants"@en ;
  sto:hasDBpediaResource <http://dbpedia.org/resource/Cardinality_(computer_engineering)> ;
  sto:supports sto:interoperability ;
.
sto:Certification
  a owl:NamedIndividual ;
  a sto:Concern ;
  terms:creator sto:sebastian ;
  rdfs:comment "Certification refers to the confirmation of certain characteristics of an object, person, or organization. This confirmation is often, but not always, provided by some form of external review, education, assessment, or audit. Accreditation is a specific organization's process of certification. (source: wikipedia)"@en ;
  rdfs:label "Certification"@en ;
  sto:hasDBpediaResource <http://dbpedia.org/resource/Certification> ;
  sto:supports sto:Security ;
  sto:supports sto:Trustworthiness ;
.
sto:CloudComputing
  a owl:NamedIndividual ;
  a sto:Concern ;
  terms:creator sto:sebastian ;
  dul:isPartOf sto:DataProcessing ;
  rdfs:comment "Cloud computing is a type of Internet-based computing that provides shared computer processing resources and data to computers and other devices on demand. It is a model for enabling ubiquitous, on-demand access to a shared pool of configurable computing resources (e.g., computer networks, servers, storage, applications and services), which can be rapidly provisioned and released with minimal management effort. Cloud computing and storage solutions provide users and enterprises with various capabilities to store and process their data in third-party data centers that may be located far from the user–ranging in distance from across a city to across the world. Cloud computing relies on sharing of resources to achieve coherence and economy of scale, similar to a utility (like the electricity grid) over an electricity network. (source: wikipedia)"@en ;
  rdfs:label "Cloud Computing Capability"@en ;
  rdfs:seeAlso "IoT-A Requirement UNI.102" ;
  rdfs:seeAlso "IoT-A Requirement UNI.234" ;
  sto:hasDBpediaResource <http://dbpedia.org/resource/Cloud_computing> ;
.
sto:Cloud_Connectivity
  a owl:NamedIndividual ;
  sto:supports sto:CloudComputing ;
.
sto:Communication
  a owl:NamedIndividual ;
  a rami:AdminShellSubmodel ;
  a sto:Concern ;
  a sto:StandardClassification ;
  rdfs:seeAlso "IoT-A Requirement UNI.021" ;
  rdfs:seeAlso "IoT-A Requirement UNI.095" ;
  rdfs:seeAlso "IoT-A Requirement UNI.303" ;
  rdfs:seeAlso "IoT-A Requirement UNI.306" ;
  rdfs:seeAlso "IoT-A Requirement UNI.307" ;
  rdfs:seeAlso "IoT-A Requirement UNI.308" ;
  rdfs:seeAlso "IoT-A Requirement UNI.309" ;
  rdfs:seeAlso "IoT-A Requirement UNI.310" ;
  rdfs:seeAlso "IoT-A Requirement UNI.311" ;
  rdfs:seeAlso "IoT-A Requirement UNI.312" ;
  rdfs:seeAlso "IoT-A Requirement UNI.313" ;
  rdfs:seeAlso "IoT-A Requirement UNI.315" ;
  rdfs:seeAlso "IoT-A Requirement UNI.318" ;
  rdfs:seeAlso "IoT-A Requirement UNI.321" ;
  rdfs:seeAlso "IoT-A Requirement UNI.324" ;
  rdfs:seeAlso "IoT-A Requirement UNI.716" ;
  sto:isDescribedin sto:AdministrationShell ;
  sto:supports sto:Interoperability ;
.
sto:ComplexEventProcessing
  a owl:NamedIndividual ;
  a sto:Concern ;
  terms:title "Complex Event Processing"@en ;
  rdfs:comment "Event processing is a method of tracking and analyzing (processing) streams of information (data) about things that happen (events), and deriving a conclusion from them. Complex event processing, or CEP, is event processing that combines data from multiple sources to infer events or patterns that suggest more complicated circumstances. The goal of complex event processing is to identify meaningful events (such as opportunities or threats) and respond to them as quickly as possible. (source: wikipedia)"@en ;
  rdfs:label "CEP"@en ;
  rdfs:seeAlso "IoT-A Requirement UNI.232" ;
  sto:hasDBpediaResource <http://dbpedia.org/page/Complex_event_processing> ;
  sto:supports sto:DataAnalytics ;
.
sto:Compliance
  a owl:NamedIndividual ;
  a sto:Concern ;
  terms:creator sto:sebastian ;
  rdfs:comment "In general, compliance means conforming to a rule, such as a specification, policy, standard or law. Regulatory compliance describes the goal that organisations aspire to achieve in their efforts to ensure that they are aware of and take steps to comply with relevant laws and regulations. Due to the increasing number of regulations and need for operational transparency, organizations are increasingly adopting the use of consolidated and harmonized sets of compliance controls. This approach is used to ensure that all necessary governance requirements can be met without the unnecessary duplication of effort and activity from resources. (source: wikipedia)"@en ;
  rdfs:label "Compliance"@en ;
  sto:hasDBpediaResource <http://dbpedia.org/resource/Regulatory_compliance> ;
  sto:supports sto:Reliability ;
.
sto:Concern
  a owl:Class ;
  terms:creator sto:sebastian ;
  rdfs:comment "A concern regards a specific challenge or topic as defined by ISO42010. Each concern should at least be regarded by one view of an architecture."@en ;
  rdfs:label "Concern" ;
  sto:hasDBpediaResource <http://dbpedia.org/resource/ISO/IEC_42010> ;
  sto:hasOfficialResource <http://www.iso-architecture.org/42010/> ;
  sto:hasWikipediaArticle <https://en.wikipedia.org/wiki/ISO/IEC_42010#Conceptual_Model_-_Concern> ;
.
sto:Confidentiality
  a owl:NamedIndividual ;
  a sto:Concern ;
  terms:creator sto:MuhammadUsman ;
  rdfs:comment "Confidentiality involves a set of rules or a promise usually executed through confidentiality agreements that limits access or places restrictions on certain types of information."@en ;
  rdfs:label "Confidentiality"@en ;
  rdfs:seeAlso "https://dl.acm.org/citation.cfm?doid=3108421.3108426"@en ;
  rdfs:seeAlso "https://ieeexplore.ieee.org/document/8327600" ;
  sto:hasWikipediaArticle "https://en.wikipedia.org/wiki/Confidentiality"@en ;
  sto:supports sto:Privacy ;
.
sto:Connectivity
  a owl:NamedIndividual ;
  a sto:Concern ;
  terms:creator sto:MuhammadUsman ;
  rdfs:comment """Internet of Things associates various smart devices through the Internet, and it gives a facility to concentrated checking and control of associated
equipment."""@en ;
  rdfs:label "Connectivity"@en ;
  rdfs:seeAlso "https://ieeexplore.ieee.org/document/6188257"@en ;
  sto:hasDBpediaResource "http://dbpedia.org/property/connectivity"@en ;
  sto:hasWikipediaArticle "https://en.wikipedia.org/wiki/Connectivity"@en ;
  sto:supports sto:SyntacticInteroperability ;
.
sto:ConstrainedDevices
  a owl:NamedIndividual ;
  a sto:Concern ;
  terms:creator sto:sebastian ;
  <http://voag.linkedmodel.org/voag#hasStakeholder> "System Architect TODO"@en ;
  rdfs:comment "Data-memory-constrained devices must be able to participate in communication. This means that a system built using the ARM shall support communication stacks with small data footprint."@en ;
  rdfs:comment "Small devices with limited CPU, memory, and power resources, so-called \"constrained devices\" (often used as sensors/actuators, smart objects, or smart devices) can form a network, becoming \"constrained nodes\" in that network.  Such a network may itself exhibit constraints, e.g., with unreliable or lossy channels, limited and unpredictable bandwidth, and a highly dynamic topology. (source: https://tools.ietf.org/html/rfc7228)"@en ;
  rdfs:label "Constrained Devices"@en ;
  rdfs:seeAlso "IoT-A Requirement UNI.306" ;
  rdfs:seeAlso "IoT-A Requirement UNI.307" ;
  rdfs:seeAlso "UNI.306"@en ;
  sto:supports sto:IoT ;
.
sto:ContextAwareness
  a owl:NamedIndividual ;
  a sto:Concern ;
  <http://voag.linkedmodel.org/voag#hasStakeholder> "Developer"@en ;
  rdfs:comment "The look-up service of the system shall withold or grant information depending on context. Context includes application involved, requesting entity, and security permissions."@en ;
  rdfs:label "Context Awareness"@en ;
  rdfs:seeAlso "IoT-A Requirement UNI.407" ;
  rdfs:seeAlso "IoT-A Requirement UNI.420" ;
  rdfs:seeAlso "IoT-A Requirement UNI.421" ;
  rdfs:seeAlso "UNI.407"@en ;
  skos:note "Publications referred: '<https://doi.org/10.1016/j.jksuci.2016.10.003>' '1.2. Utilities of IoT' 'Page 296'" ;
  sto:hasDBpediaResource <http://dbpedia.org/resource/Context_awareness> ;
  sto:supports sto:AutonomousCommunication ;
.
sto:CostEfficiency
  a owl:NamedIndividual ;
  a sto:Concern ;
  terms:creator sto:SebastianBader ;
  rdfs:comment ""@en ;
  rdfs:label "Cost Efficiency"@en ;
  rdfs:label "DataRecovery"@en ;
  rdfs:seeAlso "https://dl.acm.org/citation.cfm?doid=3266237.3266263"@en ;
  sto:supports sto:BusinessContext ;
.
sto:CrossDomainIdentityManagement
  a owl:NamedIndividual ;
  a sto:Concern ;
  terms:creator sto:sebastian ;
  <http://voag.linkedmodel.org/voag#hasStakeholder> "System Architect"@en ;
  rdfs:comment "A system built using the ARM shall support identity-locator split, i.e. making the device's identity independent from its locator."@en ;
  rdfs:label "Cross-domain Identity Management"@en ;
  rdfs:seeAlso "IoT-A Requirement UNI.314" ;
  sto:hasDBpediaResource <http://dbpedia.org/resource/System_for_Cross-domain_Identity_Management> ;
  sto:supports sto:IdentityManagement ;
.
sto:CrossLevel
  a owl:NamedIndividual ;
  a sto:ISA95Level ;
  a sto:StandardClassification ;
  rdfs:comment "Describes the cross-level according to the ISA95 level classification. It means standards that are used at more than one level, e.g., manufacturing system security, etc"@en ;
  rdfs:label "Cross Level"@en ;
  sto:isDescribedin sto:ISA95 ;
.
sto:Customer
  a <http://voag.linkedmodel.org/voag#StakeholderGroup> ;
  a owl:NamedIndividual ;
.
sto:Customization
  a owl:NamedIndividual ;
  a sto:Concern ;
  terms:creator sto:MuhammadUsman ;
  rdfs:comment "The resources sharing by contrasting users keeps cloud service provider from having the capacity to customize their services to meet the diverse necessities of customers"@en ;
  rdfs:label "Customization"@en ;
  rdfs:seeAlso "https://dl.acm.org/citation.cfm?doid=3108421.3108426"@en ;
  sto:hasWikipediaArticle "https://en.wikipedia.org/wiki/Customization"@en ;
  sto:supports sto:BusinessContext ;
  sto:supports sto:Scalability ;
.
sto:CyberSecurity
  a owl:NamedIndividual ;
  a sto:RelevantSubject ;
  rdfs:comment " Protection of Computer Systems from damage of all kinds "@en ;
  rdfs:label "Cyber Security"@en ;
  sto:hasWikipediaArticle <https://en.wikipedia.org/wiki/Computer_security> ;
.
sto:DDS
  a owl:NamedIndividual ;
  a foaf:Document ;
  a sto:Publication ;
  a sto:TechnicalSpecification ;
  terms:creator sto:sebastian ;
  rdfs:comment "DDS (Data-Distribution Service for Real-Time Systems): The first open international middleware standard directly addressing publish-subscribe communications for real-time and embedded systems. (source: https://www.postscapes.com/internet-of-things-protocols/)"@en ;
  rdfs:label "DDS"@en ;
  sto:hasOfficialResource <http://portals.omg.org/dds/> ;
.
sto:DIN
  a owl:NamedIndividual ;
  a foaf:Organization ;
  a sto:StandardOrganization ;
  rdfs:comment "Deutsches Institut für Normung e.V. (DIN; in English, the German Institute for Standardization) is the German national organization for standardization and is the German ISO member body. DIN is a German Registered Association (e.V.) headquartered in Berlin. There are currently around thirty thousand DIN Standards, covering nearly every field of technology"@en ;
  rdfs:label "DIN"@en ;
  rdfs:label "Deutsches Institut für Normung"@de ;
  rdfs:label "German Institute for Standardization"@en ;
  sto:abbreviation "DIN"@de ;
  sto:belongsTo dbr:Germany ;
  sto:formationDate "1918-01-01"^^xsd:date ;
  sto:hasDBpediaResource <http://dbpedia.org/page/Deutsches_Institut_f%C3%BCr_Normung> ;
  sto:hasHeadquaterIn dbr:Berlin ;
  sto:hasOfficialResource <http://www.din.de/en/about-standards/din-standards> ;
  sto:hasWikipediaArticle <https://en.wikipedia.org/wiki/Deutsches_Institut_f%C3%BCr_Normung> ;
  sto:orgName "Deutsches Institut für Normung"@en ;
.
sto:DIN_77005_P1
  a owl:NamedIndividual ;
  a foaf:Document ;
  a sto:Publication ;
  a sto:Standard ;
  terms:creator sto:DIN ;
  rdfs:comment "Lifecycle record of technical objects - Part 1: Structural and content-related specifications"@en ;
  rdfs:label "DIN 77005-1:2018-09"@en ;
  foaf:maker sto:DIN ;
  sto:frames sto:DataLifecycleManagment ;
  sto:hasOfficialResource <https://www.beuth.de/en/standard/din-77005-1/290281150> ;
  sto:hasPublicationDate "2018-09-01"^^xsd:date ;
  sto:hasPublisher sto:DIN ;
  sto:hasTag "DIN 77005-1:2018-09" ;
.
sto:DIN_EN_50128
  a owl:NamedIndividual ;
  a foaf:Document ;
  a sto:Publication ;
  a sto:Standard ;
  terms:creator sto:DIN ;
  rdfs:comment "Die EN 50128 ist eine Europäische Norm für sicherheitsrelevante Software der Eisenbahn, sowohl strecken- als auch zugseitig. Zusammen mit der EN 50129 für die Hardware und den Zulassungsprozessen ist die EN 50128 eine Spezialisierung der EN 61508. Die EN 50128 ist eine Prozessnorm. Sie stellt dar, welche Verfahren, Prinzipien und Maßnahmen anzuwenden sind, damit die Software als sicher gilt."@de ;
  rdfs:label "DIN EN 50128"@en ;
  foaf:maker sto:DIN ;
  sto:frames sto:Safety ;
  sto:hasClassification sto:IDSRAMCertification ;
  sto:hasOfficialResource <https://www.beuth.de/de/norm/din-en-50128/148018416> ;
  sto:hasPublicationDate "2012-03-01"^^xsd:date ;
  sto:hasPublisher sto:DIN ;
.
sto:DIN_EN_50129
  a owl:NamedIndividual ;
  a foaf:Document ;
  a sto:Publication ;
  a sto:Standard ;
  terms:creator sto:DIN ;
  terms:title "Railway applications - Communications, signalling and processing systems - Safety related electronic systems for signalling"@en ;
  rdfs:comment "Für alle Eisenbahnsignalsysteme, -Teilsysteme und -Einrichtungen sind jedoch Gefährdungsanalyse und Risikobewertungsprozesse, wie in DIN EN 50126 und in dieser Norm definiert, notwendig, um die Sicherheitsanforderungen zu identifizieren."@de ;
  rdfs:comment "Specifies risk analysis for railway systems"@en ;
  rdfs:label "DIN EN 50129"@en ;
  foaf:maker sto:DIN ;
  <https://w3id.org/i40/hasTargetConcern> sto:Safety ;
  sto:hasClassification sto:IDSRAMCertification ;
  sto:hasOfficialResource <https://www.beuth.de/de/norm/din-en-50129/67478433> ;
  sto:hasPublisher sto:DIN ;
.
sto:DIN_EN_50155
  a owl:NamedIndividual ;
  a foaf:Document ;
  a sto:Publication ;
  a sto:Standard ;
  terms:title "Railway applications - Rolling stock - Electronic equipment"@en ;
  rdfs:comment "Diese Norm wird bei der Konstruktion, Fertigung und Prüfung von auf Schienenfahrzeugen eingebauten elektronischen Betriebsmitteln verwendet. Sie beschreibt außerdem die elektrischen sowie die Umweltbedingungen für den Betrieb. Die Norm gilt für alle elektronischen Betriebsmittel für die Steuerung, die Regelung, den Schutz, die Diagnose, die Versorgung und so weiter, die auf Schienenfahrzeugen installiert sind. Als ein elektronisches Betriebsmittel gilt dabei ein Betriebsmittel, das hauptsächlich aus Halbleiterbauelementen und üblicherweise zugehörigen Bauelementen aufgebaut ist. Auch Sensoren (Strom, Spannung, Geschwindigkeit und so weiter) und bestückte Leiterplatten von Zündeinheiten für leistungselektronische Geräte sind von dieser Norm umfasst. Vollständige Zündeinheiten und leistungselektronische Schaltkreise sind in EN 61287-1 enthalten. Die Norm umfasst die Betriebsbedingungen, die Konstruktionsanforderungen, die Dokumentation und die Prüfung der elektronischen Betriebsmittel sowie die grundlegenden Hardware- und Softwareanforderungen, die für ein leistungsfähiges, zuverlässiges Betriebsmittel als erforderlich erachtet werden. Zuständig ist das DKE/UK 351.1 \"Fahrzeuge\" der DKE Deutsche Kommission Elektrotechnik Elektronik Informationstechnik in DIN und VDE."@de ;
  rdfs:comment "EN 50155:2017 is an international standard covering electronic equipment used on rolling stock for railway applications. The standard covers aspects of this electronic equipment, including temperature, humidity, shock, vibration, and other parameters. A copy of the standard may be purchased from authorised standards agencies, e.g. BSI in the UK."@en ;
  rdfs:label "DIN EN 50155"@en ;
  <https://w3id.org/i40/hasTargetConcern> sto:Safety ;
  sto:hasClassification sto:IDSRAMCertification ;
  sto:hasDBpediaResource <http://dbpedia.org/resource/EN_50155> ;
  sto:hasOfficialResource <https://www.beuth.de/de/norm/din-en-50155/275256249> ;
  sto:hasWikipediaArticle <https://en.wikipedia.org/wiki/EN_50155> ;
.
sto:DIN_EN_50159
  a owl:NamedIndividual ;
  a foaf:Document ;
  a sto:Publication ;
  a sto:Standard ;
  terms:title "Railway applications - Communication, signalling and processing systems - Safety-related communication in transmission systems"@en ;
  rdfs:comment "This European Standard is applicable for safety-relevant electronic systems which use a transmission system for digital communication purposes which has not been necessarily designed for safety-relevant applications and which - remains under the control of the designer and does not change during the life cycle, or - which is partly unknown and also does not remain constant, for which unauthorized access can be excluded, however, or - which is not under control of the designer and where unauthorized access shall also be considered. The responsible Committee is Subcommittee UK 351.3 \"Bahn-Signalanlagen\" (\"Signalling systems for railways\") of the DKE (German Commission for Electrical, Electronic and Information Technologies) at DIN and VDE."@en ;
  rdfs:label "DIN EN 50159"@en ;
  sto:hasClassification sto:IDSRAMCertification ;
  sto:hasOfficialResource <https://www.beuth.de/de/norm/din-en-50159/137853742> ;
  sto:hasTargetConcern sto:Safety ;
.
sto:DIN_EN_61511
  a owl:NamedIndividual ;
  a foaf:Document ;
  a sto:Publication ;
  a sto:Standard ;
  terms:creator sto:DIN ;
  terms:title "Functional safety - Safety instrumented systems for the process industry sector - Part 1: Framework, definitions, system, hardware and software requirements"@en ;
  rdfs:comment "This standard gives requirements for the specification, design, installation, operation and maintenance of a safety instrumented system (SIS), so that it can be confidently entrusted to achieve or maintain a safe state of the process. This standard has been developed as a process sector implementation of IEC 61508."@en ;
  rdfs:label "DIN EN 61511"@en ;
  foaf:maker sto:DIN ;
  <https://w3id.org/i40/hasTargetConcern> sto:Safety ;
  sto:hasClassification sto:IDSRAMCertification ;
  sto:hasPublisher sto:DIN ;
.
sto:DIN_EN_ISO_13849
  a owl:NamedIndividual ;
  a foaf:Document ;
  a sto:Publication ;
  a sto:Standard ;
  terms:creator sto:DIN ;
  terms:creator sto:ISO ;
  rdfs:comment """ISO 13849 is a safety standard which deals with safety-related design principles of employed control systems to establish different safety Performance Levels (PL). It replaced EN 954-1 in December 2011.
    Part 1 defines the general principles for design.
    Part 2 describes the validation."""@en ;
  rdfs:label "DIN EN ISO 13849"@en ;
  foaf:maker sto:DIN ;
  foaf:maker sto:ISO ;
  <https://w3id.org/i40/hasTargetConcern> sto:Safety ;
  sto:hasClassification sto:IDSRAMCertification ;
  sto:hasDBpediaResource <http://dbpedia.org/resource/ISO_13849> ;
  sto:hasPublisher sto:DIN ;
  sto:hasPublisher sto:ISO ;
  sto:hasWikipediaArticle <https://en.wikipedia.org/wiki/ISO_13849> ;
.
sto:DIN_EN_ISO_IEC_17025
  a owl:NamedIndividual ;
  a foaf:Document ;
  a sto:Publication ;
  a sto:Standard ;
  terms:creator sto:DIN ;
  terms:creator sto:IEC ;
  terms:creator sto:ISO ;
  terms:title "General requirements for the competence of testing and calibration laboratories"@en ;
  rdfs:comment "DIN EN ISO/IEC 17025 legt allgemeine Anforderungen an die Kompetenz, an die Unparteilichkeit und für die einheitliche Arbeitsweise von Laboratorien fest. Die Norm ist auf alle Organisationen anwendbar, die Labortätigkeiten durchführen, unabhängig von der Anzahl der Mitarbeiter. Sie reiht sich in die Normenreihe DIN EN ISO/IEC 17000 ein. Kunden von Laboratorien, Behörden, Organisationen und Programme, die eine Begutachtung unter Gleichrangigen anwenden, Akkreditierungsstellen und andere können diese Norm zur Bestätigung oder Anerkennung der Kompetenz von Laboratorien nutzen."@de ;
  rdfs:comment "ISO 17025 specifies general requirements for laboratories."@en ;
  rdfs:label "DIN EN ISO/IEC 17025"@en ;
  foaf:maker sto:DIN ;
  foaf:maker sto:IEC ;
  foaf:maker sto:ISO ;
  sto:hasClassification sto:IDSRAMCertification ;
  sto:hasOfficialResource <https://www.beuth.de/de/norm/din-en-iso-iec-17025/278030106> ;
  sto:hasPublisher sto:DIN ;
  sto:hasPublisher sto:IEC ;
  sto:hasPublisher sto:ISO ;
.
sto:DIN_ISO_14638
  a owl:NamedIndividual ;
  a foaf:Document ;
  a sto:Publication ;
  a sto:Standard ;
  terms:creator sto:DIN ;
  terms:creator sto:ISO ;
  rdfs:comment "Geometrical product specifications (GPS) - Matrix model (ISO 14638:2015); German version EN ISO 14638:2015"@en ;
  rdfs:label "DIN EN ISO 14638:2015-12"@en ;
  foaf:maker sto:DIN ;
  sto:frames sto:ThingDescription ;
  sto:hasOfficialResource <https://www.beuth.de/en/standard/din-en-iso-14638/208096393> ;
  sto:hasPublicationDate "2015-12-01"^^xsd:date ;
  sto:hasPublisher sto:DIN ;
  sto:hasTag "ISO GPS" ;
.
sto:DIN_SPEC_16592
  a owl:NamedIndividual ;
  a foaf:Document ;
  a sto:Publication ;
  a sto:Standard ;
  terms:creator sto:DIN ;
  rdfs:comment "Combining OPC Unified Architecture and Automation Markup Language."@en ;
  rdfs:label "DIN SPEC 16592"@en ;
  prov:wasGeneratedBy sto:IEC_62541 ;
  prov:wasGeneratedBy sto:IEC_62714 ;
  foaf:maker sto:DIN ;
  sto:hasDeveloper sto:DIN ;
  sto:hasOfficialResource <https://www.beuth.de/de/technische-regel/din-spec-16592/265597431> ;
  sto:hasPublisher sto:DIN ;
  sto:relatedTo sto:DIN_SPEC_16592 ;
  sto:relatedTo sto:IEC_61131 ;
  sto:relatedTo sto:IEC_61360 ;
  sto:relatedTo sto:IEC_61499 ;
  sto:relatedTo sto:IEC_61804 ;
  sto:relatedTo sto:IEC_61850 ;
  sto:relatedTo sto:IEC_61987_X ;
  sto:relatedTo sto:IEC_62424 ;
  sto:relatedTo sto:IEC_62453 ;
  sto:relatedTo sto:IEC_62541 ;
  sto:relatedTo sto:IEC_62714 ;
  sto:relatedTo sto:ISO_13584 ;
  sto:relatedTo sto:ISO_14306 ;
  sto:relatedTo sto:ISO_15746 ;
  sto:relatedTo sto:ISO_15926 ;
  sto:relatedTo sto:ISO_18629 ;
  sto:relatedTo sto:ISO_18828-2 ;
  sto:relatedTo sto:ISO_20922 ;
  sto:relatedTo sto:ISO_22400 ;
  sto:relatedTo sto:ISO_29002 ;
  sto:relatedTo sto:ISO_ASTM_52915 ;
  sto:relatedTo sto:ISO_PAS_17506 ;
  sto:relatedTo sto:MathML ;
  sto:relatedTo sto:SysML ;
  sto:relatedTo sto:eClass ;
.
sto:DIN_SPEC_16593_P1
  a owl:NamedIndividual ;
  a foaf:Document ;
  a sto:Publication ;
  a sto:Standard ;
  terms:creator sto:DIN ;
  rdfs:comment "RM-SA - Reference Model for Industrie 4.0 Service Architectures - Part 1: Basic Concepts of an Interaction-based Architecture; Text in English"@en ;
  rdfs:label "DIN SPEC 16593-1:2018-04"@en ;
  foaf:maker sto:DIN ;
  sto:frames sto:ServiceDescription ;
  sto:hasOfficialResource <https://www.beuth.de/en/technical-rule/din-spec-16593-1/287632675> ;
  sto:hasPublicationDate "2018-04-01"^^xsd:date ;
  sto:hasPublisher sto:DIN ;
  sto:hasTag "DIN SPEC 16593-1:2018-04" ;
.
sto:DIN_SPEC_27070
  a owl:NamedIndividual ;
  a foaf:Document ;
  a sto:Publication ;
  a sto:Standard ;
  a sto:StandardClassification ;
  terms:creator sto:DIN ;
  terms:title "Reference architecture of a security gateway for the exchange of industry data and services"@en ;
  dul:associatedWith sto:TrustedConnector ;
  rdfs:comment "security gateway for data protection of personal data"@en ;
  rdfs:label "DIN SPEC 27070"@en ;
  foaf:maker sto:DIN ;
  sto:alignsWith sto:TrustedConnector ;
  sto:hasClassification sto:IDSRAMSecurity ;
  sto:hasPublisher sto:DIN ;
.
sto:DIN_SPEC_91345
  a owl:NamedIndividual ;
  a foaf:Document ;
  a sto:Publication ;
  a sto:Standard ;
  a <https://www.w3.org/ns/oaSpecificResource> ;
  terms:creator sto:DIN ;
  terms:title "Reference Architecture Model Industrie 4.0 (RAMI4.0) English translation of DIN SPEC 91345:2016-04"@en ;
  rdfs:comment ""@de ;
  rdfs:label "DIN SPEC 91345:2016-04"@en ;
  rdfs:label "Reference Architecture Model Industrie 4.0 (RAMI4.0) English translation of DIN SPEC 91345:2016-04"@en ;
  foaf:maker sto:DIN ;
  sto:hasAvailableLanguage lang:eng ;
  sto:hasICS sto:ICS_03_100_01 ;
  sto:hasICS sto:ICS_25_040_01 ;
  sto:hasICS sto:ICS_35_240_50 ;
  sto:hasImplementationFormat "Document"@en ;
  sto:hasOfficialResource <https://www.beuth.de/en/technical-rule/din-spec-91345/250940128> ;
  sto:hasPages "40"^^xsd:int ;
  sto:hasPublicationDate "2016-04-01"^^xsd:date ;
  sto:hasPublisher sto:DIN ;
.
sto:DIN_SPEC_92222
  a owl:NamedIndividual ;
  a foaf:Document ;
  a sto:Publication ;
  a sto:Standard ;
  terms:creator sto:DIN ;
  terms:title "Reference Model for Industrial Cloud Federation"@en ;
  rdfs:comment "ensuring interoperability and communication of IT systems in cloud scenarios"@en ;
  rdfs:label "DIN SPEC 92222"@en ;
  foaf:maker sto:DIN ;
  sto:frames sto:CloudComputing ;
  sto:frames sto:communication ;
  sto:frames sto:interoperability ;
  sto:hasClassification sto:IDSRAMSecurity ;
  sto:hasDeveloper sto:DIN ;
  sto:hasOfficialResource <https://www.beuth.de/de/publikation/referenzmodell-industrielle-cloud-federation/296675641> ;
.
sto:DMA
  a owl:NamedIndividual ;
  a foaf:Organization ;
  a sto:StandardOrganization ;
  terms:creator sto:sebastian ;
  terms:creator "sebastian" ;
  terms:title "Data & Marketing Association"@en ;
  rdfs:comment "The Data & Marketing Association (formerly, Direct Marketing Association), also known as the DMA, is a trade organization for marketers which seeks to advance and protect responsible data-driven marketing."@en ;
  rdfs:label "DMA"@en ;
  sto:hasWikipediaArticle <https://en.wikipedia.org/wiki/Data_%26_Marketing_Association> ;
.
sto:DMSC
  a owl:NamedIndividual ;
  a foaf:Organization ;
  a sto:StandardOrganization ;
  rdfs:comment "Dimensional Metrology Standards Consortium (DMSC) is to identify urgently needed standards in the field of dimensional metrology, and to promote, foster, and encourage the development and interoperability of these standards, along with related and supporting standards that will benefit the industry as a whole."@en ;
  rdfs:label "Dimensional Metrology Standards Consortium"@en ;
  sto:hasHeadquaterIn dbr:_Texas ;
  sto:hasOfficialResource <http://www.dmis.org/> ;
.
sto:DTLS
  a owl:NamedIndividual ;
  a foaf:Document ;
  a sto:Publication ;
  a sto:Standard ;
  terms:creator sto:sebastian ;
  rdfs:comment "Datagram Transport Layer - The DTLS protocol provides communications privacy for datagram protocols. The protocol allows client/server applications to communicate in a way that is designed to prevent eavesdropping, tampering, or message forgery. The DTLS protocol is based on the Transport Layer Security (TLS) protocol and provides equivalent security guarantees. (source: https://www.postscapes.com/internet-of-things-protocols/)"@en ;
  rdfs:label "DTLS"@en ;
  sto:hasOfficialResource <https://tools.ietf.org/html/rfc4347> ;
.
sto:DataAccess
  a owl:NamedIndividual ;
  a sto:Concern ;
  terms:creator sto:sebastian ;
  rdfs:comment "Data access typically refers to software and activities related to storing, retrieving, or acting on data housed in a database or other repository. [...] Data access crucially involves authorization to access different data repositories. (source: wikipedia)"@en ;
  rdfs:label "Data Access"@en ;
  rdfs:seeAlso "IoT-A Requirement UNI.022" ;
  sto:hasDBpediaResource <http://dbpedia.org/resource/Data_access> ;
.
sto:DataAccessControl
  a owl:NamedIndividual ;
  a sto:Concern ;
  terms:creator sto:sebastian ;
  <http://voag.linkedmodel.org/voag#hasStakeholder> <http://purl.oclc.org/NET/mvco.owl#EndUser> ;
  <http://voag.linkedmodel.org/voag#hasStakeholder> <https://w3id.org/i40/DataOwner> ;
  rdfs:comment "Automated access control based on formalized descriptions."@en ;
  rdfs:comment "In the fields of physical security and information security, access control (AC) is the selective restriction of access to a place or other resource. The act of accessing may mean consuming, entering, or using. Permission to access a resource is called authorization. Locks and login credentials are two analogous mechanisms of access control. (source: wikipedia)"@en ;
  rdfs:label "Data Access Control"@en ;
  rdfs:seeAlso "IoT-A Requirement UNI.002" ;
  rdfs:seeAlso "IoT-A Requirement UNI.067" ;
  rdfs:seeAlso "IoT-A Requirement UNI.410" ;
  rdfs:seeAlso "IoT-A Requirement UNI.411" ;
  rdfs:seeAlso "IoT-A Requirement UNI.412" ;
  rdfs:seeAlso "IoT-A Requirement UNI.413" ;
  rdfs:seeAlso "IoT-A Requirement UNI.504" ;
  sto:hasDBpediaResource <http://dbpedia.org/resource/Access_control> ;
  sto:supports sto:Authorization ;
.
sto:DataAggregation
  a owl:NamedIndividual ;
  a sto:Concern ;
  rdfs:comment "Data Aggregation is the compiling the data before Data Processing"@en ;
  rdfs:label "Data Aggregation"@en ;
  rdfs:seeAlso "https://ieeexplore.ieee.org/document/7566346"@en ;
  rdfs:seeAlso "https://www.researchgate.net/publication/319283535_Data_aggregation_mechanisms_in_the_Internet_of_things_A_systematic_review_of_the_literature_and_recommendations_for_future_research"@en ;
  skos:narrower sto:DataProcessing ;
  sto:hasWikipediaArticle "https://en.wikipedia.org/wiki/Data_aggregation"@en ;
.
sto:DataAnalytics
  a owl:NamedIndividual ;
  a sto:Concern ;
  terms:creator sto:sebastian ;
  rdfs:comment "Analysis of data is a process of inspecting, cleaning, transforming, and modeling data with the goal of discovering useful information, suggesting conclusions, and supporting decision-making. Data analysis has multiple facets and approaches, encompassing diverse techniques under a variety of names, in different business, science, and social science domains. Data mining is a particular data analysis technique that focuses on modeling and knowledge discovery for predictive rather than purely descriptive purposes. Business intelligence covers data analysis that relies heavily on aggregation, focusing on business information. (source: wikipedia)"@en ;
  rdfs:label "Data Analytics"@en ;
  rdfs:seeAlso "IoT-A Requirement UNI.232" ;
  sto:hasDBpediaResource <http://dbpedia.org/resource/Data_analysis> ;
.
sto:DataAtRest
  a owl:NamedIndividual ;
  a sto:Concern ;
  terms:creator sto:sebastian ;
  rdfs:comment "Data at rest in information technology means inactive data that is stored physically in any digital form (e.g. databases, data warehouses, spreadsheets, archives, tapes, off-site backups, mobile devices etc.). Data at rest is used as a complement to the terms data in use and data in transit which together define the three states of digital Data. (source: wikipedia)"@en ;
  rdfs:label "Data at rest"@en ;
  sto:hasDBpediaResource <http://dbpedia.org/resource/Data_at_rest> ;
  sto:supports sto:Communication ;
.
sto:DataConsumer
  a <http://voag.linkedmodel.org/voag#StakeholderGroup> ;
  a owl:NamedIndividual ;
.
sto:DataDescription
  a owl:NamedIndividual ;
  a sto:Concern ;
  terms:creator sto:sebastian ;
  <http://voag.linkedmodel.org/voag#hasStakeholder> <http://dbpedia.org/ontology/developer> ;
  rdfs:comment <http://dbpedia.org/resource/Data_model> ;
  rdfs:comment "Methods to unambiguously describe data resources."@en ;
  rdfs:label "Data Description"@en ;
  rdfs:seeAlso "IoT-A Requirement UNI.004" ;
  rdfs:seeAlso "IoT-A Requirement UNI.240" ;
  sto:supports sto:SemanticInteroperability ;
.
sto:DataDiscovery
  a owl:NamedIndividual ;
  a sto:Concern ;
  terms:creator sto:sebastian ;
  terms:creator "sebastian"@en ;
  rdfs:comment "How to find desired resources, Data Assets, Data Artifacts in a defined environment."@en ;
  rdfs:label "Data Discovery"@en ;
  rdfs:seeAlso "IoT-A Requirement UNI.236" ;
  rdfs:seeAlso "IoT-A Requirement UNI.408" ;
  rdfs:seeAlso "IoT-A Requirement UNI.422" ;
  sto:supports sto:Interoperability ;
.
sto:DataEconomy
  a owl:NamedIndividual ;
  a sto:Concern ;
  terms:creator sto:sebastian ;
  rdfs:comment "Business aspects of data exchange"@en ;
  rdfs:comment "Digital economy refers to an economy that is based on digital computing technologies. The digital economy is also sometimes called the Internet Economy, the New Economy, or Web Economy. Increasingly, the \"digital economy\" is intertwined with the traditional economy making a clear delineation harder. (source: wikipedia)"@en ;
  rdfs:label "Data Economy"@en ;
  sto:hasDBpediaResource <http://dbpedia.org/resource/Digital_economy> ;
  sto:supports sto:BusinessContext ;
.
sto:DataEncryption
  a owl:NamedIndividual ;
  a sto:Concern ;
  terms:creator sto:MuhammadUsman ;
  rdfs:comment ""@en ;
  rdfs:comment "The resources sharing by contrasting users keeps cloud service provider from having the capacity to customize their services to meet the diverse necessities of customers"@en ;
  rdfs:label "Customization"@en ;
  rdfs:label "Data secrecy and encryption"@en ;
  rdfs:seeAlso "https://dl.acm.org/citation.cfm?doid=3108421.3108426"@en ;
  rdfs:seeAlso "https://ieeexplore.ieee.org/document/6188257"@en ;
  sto:hasWikipediaArticle "https://en.wikipedia.org/wiki/Customization"@en ;
  sto:hasWikipediaArticle "https://en.wikipedia.org/wiki/Encryption"@en ;
  sto:supports sto:BusinessContext ;
  sto:supports sto:SecureCommunication ;
.
sto:DataIntegrity
  a owl:NamedIndividual ;
  a sto:Concern ;
  terms:creator sto:MuhammadUsman ;
  rdfs:comment "Data integrity is the maintenance of, and the assurance of the accuracy and consistency of, data over its entire life-cycle, and is a critical aspect to the design, implementation and usage of any system which stores, processes, or retrieves data."@en ;
  rdfs:label "Data Integrity"@en ;
  rdfs:seeAlso "https://ieeexplore.ieee.org/document/6188257"@en ;
  rdfs:seeAlso "https://ieeexplore.ieee.org/document/8327600" ;
  rdfs:seeAlso "https://ieeexplore.ieee.org/document/8487479"@en ;
  sto:hasWikipediaArticle "https://en.wikipedia.org/wiki/Data_integrity"@en ;
  sto:supports sto:Privacy ;
.
sto:DataIsolation
  a owl:NamedIndividual ;
  a sto:Concern ;
  rdfs:comment "Isolation is one of the ACID (Atomicity, Consistency, Isolation, Durability) properties adopted by the database systems"@en ;
  rdfs:label "Data Isolation"@en ;
  skos:narrower sto:Isolation ;
  sto:hasWikipediaArticle "https://en.wikipedia.org/wiki/Isolation_(database_systems)"@en ;
  sto:supports sto:DataIntegrity ;
.
sto:DataLifecycleManagement
  rdfs:seeAlso "IoT-A Requirement UNI.097" ;
.
sto:DataLifecycleManagment
  a owl:NamedIndividual ;
  a sto:Concern ;
  rdfs:comment "Data lifecycle management includes every phase of a \"record\" from its beginning to its end. And while it is generally applied to information that rises to the classic definition of a record (and thus related to records management), it applies to all informational assets. During its existence, information can become a record by being identified as documenting a business transaction or as satisfying a business need. (source: wikipedia)"@en ;
  rdfs:label "Data lifecycle management"@en ;
  sto:hasDBpediaResource <http://dbpedia.org/resource/Information_lifecycle_management> ;
  sto:supports sto:DataAnalytics ;
.
sto:DataLocation
  a owl:NamedIndividual ;
  a sto:Concern ;
  terms:creator sto:MuhammadUsman ;
  rdfs:comment "One of the features of cloud computing is geodistribution of data among several servers. But this can be an issue for the enterprise, as the location of the data is unknown to the user."@en ;
  rdfs:label "Data Location"@en ;
  rdfs:seeAlso "https://dl.acm.org/citation.cfm?doid=2735399.2735405"@en ;
  rdfs:seeAlso "https://dl.acm.org/citation.cfm?doid=3286606.3286865"@en ;
  rdfs:seeAlso "https://ieeexplore.ieee.org/document/8249113"@en ;
  sto:supports sto:DataUsageControl ;
.
sto:DataMarketAustria
  a owl:NamedIndividual ;
  a foaf:Organization ;
  a sto:DataSharingInitiative ;
  a sto:StandardOrganization ;
  terms:creator sto:sebastian ;
  terms:title "Data Market Austria"@en ;
  rdfs:label "DMA"@en ;
  sto:hasOfficialResource <http://www.datamarket.at/> ;
.
sto:DataMarkets
  a owl:NamedIndividual ;
  a sto:Concern ;
  terms:creator sto:sebastian ;
  rdfs:comment "Data as an economic good; it's offered, demanded, and priced."@en ;
  rdfs:label "Data Markets"@en ;
  sto:supports sto:DataEconomy ;
.
sto:DataOwner
  a <http://voag.linkedmodel.org/voag#StakeholderGroup> ;
  a owl:NamedIndividual ;
.
sto:DataOwnership
  a owl:NamedIndividual ;
  a sto:Concern ;
  terms:creator sto:sebastian ;
  rdfs:comment "Data Ownership declare the possesion on an information resource that is independent of its location, e.g. personal data belongs to the related person no matter where it is stored."@en ;
  rdfs:label "Data Ownership"@en ;
  sto:hasDBpediaResource <http://dbpedia.org/resource/Data_ownership> ;
  sto:supports sto:Privacy ;
.
sto:DataProcessing
  a owl:NamedIndividual ;
  a sto:Concern ;
  terms:creator sto:sebastian ;
  <http://voag.linkedmodel.org/voag#hasStakeholder> <https://www.wikidata.org/wiki/Q1548249> ;
  rdfs:comment "Data processing and analytic components from the App Store create flexible data processing pipelines."@en ;
  rdfs:label "Data Processing"@en ;
  rdfs:seeAlso "IoT-A Requirement UNI.018" ;
  rdfs:seeAlso "https://dl.acm.org/citation.cfm?doid=3098208.3098210" ;
  sto:hasDBpediaResource <http://dbpedia.org/resource/Data_processing> ;
.
sto:DataProtection
  a owl:NamedIndividual ;
  a sto:Concern ;
  terms:creator sto:sebastian ;
  rdfs:comment "Data protection is the relationship between collection and dissemination of data, technology, the public expectation of privacy, and the legal and political issues surrounding them. Privacy concerns exist wherever personally identifiable information or other sensitive information is collected, stored, used, and finally destroyed or deleted – in digital form or otherwise. Improper or non-existent disclosure control can be the root cause for privacy issues. (source: wikipedia)"@en ;
  rdfs:label "Data Protection"@en ;
  skos:altLabel "Datenschutz"@de ;
  skos:altLabel "Information privacy"@en ;
  sto:hasDBpediaResource <http://dbpedia.org/resource/Information_privacy> ;
  sto:supports sto:Privacy ;
.
sto:DataProvider
  a <http://voag.linkedmodel.org/voag#StakeholderGroup> ;
  a owl:NamedIndividual ;
.
sto:DataPublishing
  a owl:NamedIndividual ;
  a sto:Concern ;
  terms:creator sto:sebastian ;
  rdfs:comment "Data Publishing is the concern regarding all aspects of getting data (publicly) available."@en ;
  rdfs:label "Data Publishing"@en ;
  sto:supports sto:DataAccessControl ;
.
sto:DataQuality
  a owl:NamedIndividual ;
  a sto:Concern ;
  terms:creator sto:sebastian ;
  rdfs:comment "Data quality refers to the level of quality of data. There are many definitions of data quality but data are generally considered high quality if \"they are fit for their intended uses in operations, decision making and planning.\" (Tom Redman<Redman, T.C. (2008). Data driven: Profiting from your most important business asset (p. 56). Boston, Mass.: Harvard Business Press.>). Alternatively, data is deemed of high quality if it correctly represents the real-world construct to which it refers. Furthermore, apart from these definitions, as data volume increases, the question of internal consistency within data becomes significant, regardless of fitness for use for any particular external purpose. People's views on data quality can often be in disagreement, even when discussing the same set of data used for the same purpose. (source: wikipedia)"@en ;
  rdfs:label "Data Quality"@en ;
  rdfs:seeAlso "IoT-A Requirement UNI.235" ;
  rdfs:seeAlso "IoT-A Requirement UNI.236" ;
  rdfs:seeAlso "IoT-A Requirement UNI.237" ;
  sto:hasDBpediaResource <http://dbpedia.org/resource/Data_quality> ;
  sto:supports sto:QualityOfService ;
.
sto:DataSecurity
  a owl:NamedIndividual ;
  a sto:Concern ;
  rdfs:seeAlso "https://ieeexplore.ieee.org/document/6188257"@en ;
  rdfs:seeAlso "https://ieeexplore.ieee.org/document/8249113"@en ;
  owl:sameAs sto:DataProtection ;
  sto:hasWikipediaArticle "https://en.wikipedia.org/wiki/Data_security"@en ;
.
sto:DataSharingInitiative
  a owl:Class ;
  a owl:NamedIndividual ;
  terms:creator sto:sebastian ;
  rdfs:comment "This class frames all organizations with the main intend to create, specify and implement a data sharing concept with according interfaces, components, data descriptions, and retrieval algorithms."@en ;
  rdfs:label "Data Sharing Initiative"@en ;
  rdfs:subClassOf foaf:Organization ;
.
sto:DataSovereignty
  a owl:NamedIndividual ;
  a sto:Concern ;
  a sto:StandardClassification ;
  terms:creator sto:sebastian ;
  rdfs:label "Data Sovereignty"@en ;
  sto:hasDBpediaResource <http://dbpedia.org/resource/Cyber_sovereignty> ;
  sto:hasWikipediaArticle <https://en.wikipedia.org/wiki/Data_sovereignty> ;
.
sto:DataStorage
  a owl:NamedIndividual ;
  a sto:Concern ;
  terms:creator sto:MuhammadUsman ;
  terms:creator sto:sebastian ;
  rdfs:comment "The IoT data are collected from various data sources in different structures and formats. IoT enables the collected data to be stored both in physical devices and cloud storage."@en ;
  rdfs:label "Data Storage"@en ;
  rdfs:seeAlso "https://ieeexplore.ieee.org/document/8102372"@en ;
  sto:hasWikipediaArticle "https://en.wikipedia.org/wiki/Data_storage"@en ;
  sto:supports sto:DataProcessing ;
.
sto:DataTransferProject
  a owl:NamedIndividual ;
  a foaf:Organization ;
  a sto:DataSharingInitiative ;
  terms:creator sto:sebastian ;
  dul:associatedWith sto:DtpArchitecture ;
  rdfs:comment "The Data Transfer Project (DTP) extends data portability beyond a user’s ability to download a copy of their data from their service provider (“provider”), to providing the user the ability 1 to initiate a direct transfer of their data into and out of any participating provider. The Data Transfer Project is an open source initiative to encourage participation of as many providers as possible. The DTP will enhance the data portability ecosystem by reducing the infrastructure burden on both providers and users, which should in turn increase the number of services offering portability. The protocols and methodology of the DTP enable direct, service-to-service data transfer with streamlined engineering work."@en ;
  rdfs:label "Data Transfer Project"@en ;
  sto:hasOfficialResource <https://github.com/google/data-transfer-project> ;
.
sto:DataTransferProjectAnno
  a <https://www.w3.org/ns/oaAnnotation> ;
  <https://www.w3.org/ns/oahasBody> sto:DataTransferProject ;
.
sto:DataTransferProjectWhitepaper
  a owl:NamedIndividual ;
  a foaf:Document ;
  a sto:Publication ;
  terms:creator sto:DataTransferProject ;
  terms:creator sto:sebastian ;
  rdfs:comment "The Data Transfer Project Whitepaper provides a brief overview on the intends of the Data Transfer Project and the targeted approach."@en ;
  rdfs:label "Data Transfer Project Whitepaper"@en ;
  foaf:maker sto:DataTransferProject ;
  sto:hasClassification sto:DtpDeploymentView ;
  sto:hasClassification sto:DtpEcosystemView ;
  sto:hasClassification sto:DtpSecurityPrivacy ;
  sto:hasClassification sto:DtpSystemView ;
  sto:hasDBpediaResource <http://dbpedia.org/page/Data_Transfer_Project> ;
  sto:hasDeveloper sto:DataTransferProject ;
  sto:hasPublisher sto:DataTransferProject ;
  sto:hasTargetConcern sto:DataSovereignty ;
  sto:hasTargetConcern sto:IdentityManagement ;
  sto:hasTargetConcern sto:Privacy ;
  sto:hasTargetConcern sto:SecureCommunication ;
  sto:hasTargetConcern sto:UserPreferences ;
  sto:hasWikipediaArticle <https://en.wikipedia.org/wiki/Data_Transfer_Project> ;
.
sto:DataUsageControl
  a owl:NamedIndividual ;
  a sto:Concern ;
  terms:creator sto:sebastian ;
  rdfs:comment "Data usage control can be seen as an extension of data access control. It is about the specification and enforcement of restrictions regulating what is allowed to happen with data, and what is not. Data usage control thus is concerned with requirements that pertain to data processing (obligations) rather than data access (provisions). It is primarily relevant in the context of intellectual property protection, privacy protection, compliance with regulations, and digital rights management."@en ;
  rdfs:label "Data Usage Control"@en ;
  sto:supports sto:Authorization ;
.
sto:Data_Collection
  a owl:NamedIndividual ;
  a sto:Concern ;
  terms:creator sto:MuhammadUsman ;
  rdfs:comment "The data in IoT are always mass, distributed, and time-related and position related. At the same time, the data sources of the IoT are heterogeneous. There is a vast amount of real-time data collected by the IoT devices."@en ;
  rdfs:label "Data Collection"@en ;
  rdfs:seeAlso "https://ieeexplore.ieee.org/document/8102372"@en ;
  sto:hasDBpediaResource "http://dbpedia.org/page/Data_collection"@en ;
  sto:hasWikipediaArticle "https://en.wikipedia.org/wiki/Data_collection"@en ;
  sto:supports sto:DataAnalytics ;
.
sto:Data_Confidentiality
  a owl:NamedIndividual ;
  a sto:Concern ;
  terms:creator sto:MuhammadUsman ;
  rdfs:comment "In edge computing, user private data is outsourced to the edge server and its ownership and control are separated, which causes users to lose their physical control over the outsourced data."@en ;
  rdfs:label "Data Confidentiality"@en ;
  rdfs:seeAlso "https://ieeexplore.ieee.org/document/6188257"@en ;
  rdfs:seeAlso "https://ieeexplore.ieee.org/document/8327600"@en ;
  sto:supports sto:Privacy ;
.
sto:Data_Transfer_Project_Overview_and_Fundamentals
  a <https://www.w3.org/ns/oaSpecificResource> ;
  rdfs:label "Data Transfer Project Overview and Fundamentals"@en ;
  sto:hasOpenResource <https://datatransferproject.dev/dtp-overview.pdf> ;
.
sto:DecisionMaker
  a owl:NamedIndividual ;
  a sto:Stakeholder ;
  rdfs:comment "These are business Decision makers"@en ;
  rdfs:label "Decision maker"@en ;
  skos:note "Publications referred: '(IIC:PUB:G1:V1.80:20170131' '3.5.1 BUSINESS VIEWPOINT' 'Page 15' 'Priyanka'" ;
.
sto:Developer
  a <http://voag.linkedmodel.org/voag#StakeholderGroup> ;
  a owl:NamedIndividual ;
.
sto:DeviceLevel
  a owl:NamedIndividual ;
  a sto:ISA95Level ;
  a sto:StandardClassification ;
  rdfs:comment "Describes the device level according to the ISA95 level classification."@en ;
  rdfs:label "Device Level"@en ;
.
sto:DeviceSecurity
  a owl:NamedIndividual ;
  a sto:Concern ;
  terms:creator sto:SebastianBader ;
  rdfs:comment ""@en ;
  rdfs:label "Device Security"@en ;
  rdfs:seeAlso "https://ieeexplore.ieee.org/document/8552311"@en ;
  skos:narrower sto:Security ;
  sto:supports sto:Objects_Safety_and_security ;
.
sto:Device_Authentication
  a owl:NamedIndividual ;
  a sto:Concern ;
  terms:creator sto:MuhammadUsman ;
  rdfs:label "Device Authentication"@en ;
  rdfs:seeAlso "https://ieeexplore.ieee.org/document/7919553"@en ;
  sto:hasWikipediaArticle "https://en.wikipedia.org/wiki/Authentication"@en ;
  sto:supports sto:Authentication ;
.
sto:DigiMesh
  a owl:NamedIndividual ;
  a foaf:Document ;
  a sto:Publication ;
  a sto:TechnicalSpecification ;
  terms:creator sto:sebastian ;
  rdfs:comment "DigiMesh is a proprietary peer-to-peer networking topology for use in wireless end-point connectivity solutions. (source: https://www.postscapes.com/internet-of-things-protocols/)"@en ;
  rdfs:label "DigiMesh"@en ;
  sto:hasOfficialResource <http://www.digi.com/technology/digimesh/> ;
.
sto:DmaArchitecture
  a owl:NamedIndividual ;
  a sto:ArchitectureDescription ;
  a sto:StandardizationFramework ;
  terms:creator sto:sebastian ;
  rdfs:label "DMA Architecture"@en ;
  sto:hasPublisher sto:DataMarketAustria ;
.
sto:DmaServiceTechnologySpecificationAndDevelopmentRoadmap
  a owl:NamedIndividual ;
  a foaf:Document ;
  a sto:Publication ;
  a sto:StandardizationFramework ;
  terms:creator sto:DataMarketAustria ;
  dul:associatedWith sto:Blockchain ;
  dul:associatedWith sto:REST ;
  dul:associatedWith sto:RFC_6750 ;
  rdfs:comment """This document presents the DMA Data Technology Specification and Development Roadmap regarding the ongoing work in WP6 of the DMA project. The document relates to deliverable D2.2 “D2.2 Community-driven Data-Services Ecosystem Requirements (1st version)” which formulates
the requirements of the DMA community. It will be explained in what way the requirements formulated in D2.2 are going to be addressed. The document gives an overview about the components which are going to be developed in WP6 and how these components are planned to be employed to provide DMA core services. The expected outputs of these services are described and a procedure of describing a 3rd party service for DMA platform is addressed."""@en ;
  rdfs:label "DMA Service Technology Specification and Development Roadmap"@en ;
  foaf:maker sto:DataMarketAustria ;
  sto:hasOfficialResource <https://datamarket.at/wp-content/uploads/2017/10/DMA_Deliverable_D6.1_FINAL_v01.pdf> ;
  sto:hasPublisher sto:DataMarketAustria ;
  sto:hasTargetConcern sto:Authentication ;
  sto:hasTargetConcern sto:Authorization ;
  sto:hasTargetConcern sto:BigDataApplications ;
  sto:hasTargetConcern sto:Billing ;
  sto:hasTargetConcern sto:CloudComputing ;
  sto:hasTargetConcern sto:DataAccess ;
  sto:hasTargetConcern sto:DataQuality ;
  sto:hasTargetConcern sto:Privacy ;
  sto:hasTargetConcern sto:SecureCommunication ;
  sto:hasTargetConcern sto:Security ;
  sto:hasTargetConcern sto:SemanticInteroperability ;
  sto:hasTargetConcern sto:StreamProcessing ;
  sto:hasTargetConcern sto:SyntacticInteroperability ;
  sto:hasTargetConcern sto:Trustworthiness ;
.
sto:Domain
  a owl:Class ;
  rdfs:comment "Represents the Domains in which the Standards can be used"@en ;
  rdfs:label "Domain"@en ;
.
sto:DtpArchitecture
  a owl:NamedIndividual ;
  a sto:ArchitectureDescription ;
  a sto:StandardizationFramework ;
  terms:creator sto:sebastian ;
  rdfs:comment "The architecture description of the Data Transfer Project has not yet been published in a sufficient manner."@en ;
  rdfs:label "Data Transfer Project Architecture"@en ;
  sto:hasPublisher sto:DataTransferProject ;
.
sto:DtpDeploymentView
  a owl:NamedIndividual ;
  a sto:StandardClassification ;
  a sto:Viewpoint ;
  dul:associatedWith sto:IDSRAMProcessLayer ;
  dul:associatedWith sto:IIRAImplementationViewpoint ;
  rdfs:label "DTP Deployment"@en ;
  sto:alignsWith sto:IDSRAMProcessLayer ;
  sto:alignsWith sto:IIRAImplementationViewpoint ;
  sto:frames sto:Identification ;
  sto:frames sto:IdentityManagement ;
  sto:frames sto:Security ;
  sto:frames sto:ServiceDeployment ;
  sto:frames sto:ServiceLifecycleManagement ;
  sto:frames sto:Trustworthiness ;
  sto:frames sto:UserInteraction ;
  sto:isDescribedin sto:DtpArchitecture ;
.
sto:DtpEcosystemView
  a owl:NamedIndividual ;
  a sto:StandardClassification ;
  a sto:Viewpoint ;
  dul:associatedWith sto:IDSRAMGovernance ;
  dul:associatedWith sto:IIRAUsageViewpoint ;
  rdfs:label "DTP Ecosystem"@en ;
  sto:alignsWith sto:IDSRAMGovernance ;
  sto:alignsWith sto:IIRAUsageViewpoint ;
  sto:isDescribedin sto:DtpArchitecture ;
.
sto:DtpSecurityPrivacy
  a owl:NamedIndividual ;
  a sto:StandardClassification ;
  a sto:Viewpoint ;
  dul:associatedWith rami:Security ;
  dul:associatedWith sto:IDSRAMGovernance ;
  dul:associatedWith sto:IIRAPrivacy ;
  dul:associatedWith sto:IIRASecurity ;
  rdfs:label "DTP Security & Privacy"@en ;
  sto:alignsWith rami:Security ;
  sto:alignsWith sto:IDSRAMGovernance ;
  sto:alignsWith sto:IIRAPrivacy ;
  sto:alignsWith sto:Security ;
  sto:isDescribedin sto:DtpArchitecture ;
.
sto:DtpSystemView
  a owl:NamedIndividual ;
  a sto:StandardClassification ;
  a sto:Viewpoint ;
  dul:associatedWith sto:IDSRAMSystemLayer ;
  dul:associatedWith sto:IIRAConnectivity ;
  dul:associatedWith sto:IIRAOperationsDomain ;
  dul:associatedWith sto:InformationDomain ;
  dul:associatedWith sto:RAMIFunctionalLayer ;
  dul:associatedWith sto:RAMIIntegrationLayer ;
  dul:associatedWith sto:RFC_6750 ;
  rdfs:label "DTP System"@en ;
  sto:alignsWith sto:IDSRAMSystemLayer ;
  sto:alignsWith sto:IIRAConnectivity ;
  sto:alignsWith sto:IIRAOperationsDomain ;
  sto:alignsWith sto:InformationDomain ;
  sto:alignsWith sto:RAMIFunctionalLayer ;
  sto:alignsWith sto:RAMIIntegrationLayer ;
  sto:frames sto:Authentication ;
  sto:frames sto:Communication ;
  sto:frames sto:DataAccess ;
  sto:frames sto:Interoperability ;
  sto:frames sto:SecureCommunication ;
  sto:frames sto:Security ;
  sto:frames sto:SemanticInteroperability ;
  sto:frames sto:SyntacticInteroperability ;
  sto:frames sto:Trustworthiness ;
  sto:isDescribedin sto:DtpArchitecture ;
.
sto:DynamicAdjustability
  a owl:NamedIndividual ;
  a sto:Concern ;
  rdfs:comment "A systems ability to adjust its behaviour on dynamic changes in its environment."@en ;
  rdfs:label "Dynamic Adjustability"@en ;
  rdfs:seeAlso "IoT-A Requirement UNI.713" ;
  sto:supports sto:ServiceChoreography ;
  sto:supports sto:ServiceComposition ;
  sto:supports sto:ServiceOrchestration ;
.
sto:DynamicDiscovery
  a owl:NamedIndividual ;
  a sto:Concern ;
  rdfs:comment "A systems ability to retrive according information on required assets and components on-the-fly."@en ;
  rdfs:label "Dynamic Discovery"@en ;
  rdfs:seeAlso "IoT-A Requirement UNI.418" ;
  rdfs:seeAlso "IoT-A Requirement UNI.419" ;
  rdfs:seeAlso "IoT-A Requirement UNI.420" ;
  rdfs:seeAlso "IoT-A Requirement UNI.421" ;
  sto:supports sto:DataDiscovery ;
  sto:supports sto:ServiceDiscovery ;
.
sto:ENISA
  a owl:NamedIndividual ;
  a foaf:Organization ;
  a sto:StandardOrganization ;
  terms:title "European Union Agency for Network and Information Security"@en ;
  rdfs:comment "ENISA provides recommendations on cybersecurity, supports policy development and its implementation, and collaborates with operational teams throughout Europe."@en ;
  rdfs:label "ENISA"@en ;
  sto:hasOfficialResource <https://www.enisa.europa.eu/> ;
.
sto:ENISA_CloudComputing
  a owl:NamedIndividual ;
  a foaf:Document ;
  a sto:Domain ;
  a sto:Publication ;
  a sto:Standard ;
  terms:creator sto:ENISA ;
  terms:title "Cloud Computing - Benefits, risks and recommendations for information security"@en ;
  rdfs:comment "ENISA, supported by a group of subject matter expert comprising representatives from Industries, Academia and Governmental Organizations, has conducted, in the context of the Emerging and Future Risk Framework project, an risks assessment on cloud computing business model and technologies. The result is an in-depth and independent analysis that outlines some of the information security benefits and key security risks of cloud computing. The report provide also a set of practical recommendations.Produced by ENISA with contributions from a group of subject matter expert comprising representatives from Industry, Academia and Governmental Organizations, a risk assessment of cloud computing business model and technologies. This is an in-depth and independent analysis that outlines some of the information security benefits and key security risks of cloud computing. The report provide also a set of practical recommendations. It is produced in the context of the Emerging and Future Risk Framework project."@en ;
  rdfs:label "ENISA Cloud Computing"@en ;
  foaf:maker sto:ENISA ;
  sto:domainName "Cloud Computing"@en ;
  sto:hasClassification sto:IIRASecurity ;
  sto:hasOfficialResource <https://resilience.enisa.europa.eu/cloud-security-and-resilience/publications/cloud-computing-benefits-risks-and-recommendations-for-information-security> ;
  sto:hasPublicationDate "2012-12-01"^^xsd:date ;
  sto:hasPublisher sto:ENISA ;
.
sto:ETSI
  a owl:NamedIndividual ;
  a foaf:Organization ;
  a sto:StandardOrganization ;
  rdfs:comment "The European Telecommunications Standards Institute (ETSI) is an independent, not-for-profit, standardization organization in the telecommunications industry (equipment makers and network operators) in Europe, headquartered in Sophia-Antipolis, France, with worldwide projection. ETSI produces globally-applicable standards for Information and Communications Technologies (ICT), including fixed, mobile, radio, converged, broadcast and internet technologies."@en ;
  rdfs:label "ETSI"@en ;
  sto:abbreviation "ETSI"@en ;
  sto:formationDate "1988-01-01"^^xsd:date ;
  sto:hasDBpediaResource <http://dbpedia.org/resource/ETSI> ;
  sto:hasHeadquaterIn dbr:Valbonne ;
  sto:hasOfficialResource <http://www.etsi.org/> ;
  sto:hasWikipediaArticle <https://en.wikipedia.org/wiki/ETSI> ;
  sto:orgName "European Telecommunications Standards Institute"@en ;
.
sto:ETSI_DECT
  a owl:NamedIndividual ;
  a foaf:Document ;
  a sto:Publication ;
  a sto:Standard ;
  terms:creator sto:ETSI ;
  rdfs:comment "Digital Enhanced Cordless Telecommunications (DECT) is the ETSI standard for short-range cordless communications, which can be adapted for many applications and can be used over unlicensed frequency allocations world-wide."@en ;
  rdfs:label "ETSI DECT" ;
  foaf:maker sto:ETSI ;
  sto:hasDBpediaResource <http://dbpedia.org/resource/Digital_Enhanced_Cordless_Telecommunications> ;
  sto:hasDeveloper sto:ETSI ;
  sto:hasOfficialResource <http://www.etsi.org/technologies-clusters/technologies/dect> ;
  sto:hasPublisher sto:ETSI ;
  sto:hasTag "Digital Enhanced Cordless Telecommunications"@en ;
  sto:hasWikipediaArticle <https://en.wikipedia.org/wiki/Digital_Enhanced_Cordless_Telecommunications> ;
.
sto:ETSI_LTN
  a owl:NamedIndividual ;
  a foaf:Document ;
  a sto:Publication ;
  a sto:Standard ;
  terms:creator sto:ETSI ;
  rdfs:comment "Machine-to-Machine communications and the Internet of Things (IoT) involve the connection of potentially billions of connected objects which need only low throughput connectivity. The anticipated benefits of creating new dedicated IoT Low Throughput Networks (LTN) include lower costs, the creation of new applications, a reduction in electromagnetic radiation by improving data transmission efficiency LTN are expected to be crucial to the success of IoT standardization and implementation, and to provide the basis for many new and innovative applications. "@en ;
  rdfs:label "ETSI LTN"@en ;
  foaf:maker sto:ETSI ;
  sto:hasDeveloper sto:ETSI ;
  sto:hasDomain sto:M2M ;
  sto:hasOfficialResource <http://www.etsi.org/technologies-clusters/technologies/low-throughput-networks> ;
  sto:hasPublisher sto:ETSI ;
  sto:relatedTo sto:ETSI_DECT ;
  sto:relatedTo sto:ETSI_LTN ;
  sto:relatedTo sto:ETSI_ULE ;
.
sto:ETSI_ULE
  a owl:NamedIndividual ;
  a foaf:Document ;
  a sto:Publication ;
  a sto:Standard ;
  terms:creator sto:ETSI ;
  rdfs:comment "DECT Ultra Low Energy (DECT ULE) is a technology based on DECT, and intended for Machine-to-Machine communications such as Home and Industrial automation. The main characteristics of the technology are ultra-low power consumption (much lower than IEEE 802.11) and wider coverage (much wider than IEEE 802.15 and Bluetooth Low Energy)."@en ;
  rdfs:label "Ultra Low Energy"@en ;
  foaf:maker sto:ETSI ;
  sto:hasDBpediaResource <http://dbpedia.org/resource/ULE_-_Ultra_Low_Energy> ;
  sto:hasDeveloper sto:ETSI ;
  sto:hasOfficialResource <http://www.etsi.org/technologies-clusters/technologies/dect/dect-ule> ;
  sto:hasPublisher sto:ETSI ;
  sto:hasWikipediaArticle <https://en.wikipedia.org/wiki/DECT_Ultra_Low_Energy> ;
  sto:relatedTo sto:ETSI_DECT ;
  sto:relatedTo sto:ETSI_LTN ;
  sto:relatedTo sto:ETSI_ULE ;
.
sto:EcGsmIoT
  a owl:NamedIndividual ;
  a foaf:Document ;
  a sto:Publication ;
  a sto:TechnicalSpecification ;
  terms:creator sto:sebastian ;
  rdfs:comment "EC-GSM-IoT (Extended Coverage-GSM-IoT): Enables new capabilities of existing cellular networks for LPWA (Low Power Wide Area) IoT applications. EC-GSM-IoT can be activated through new software deployed over a very large GSM footprint, adding even more coverage to serve IoT devices. (source: https://www.postscapes.com/internet-of-things-protocols/)"@en ;
  rdfs:label "EC-GSM-IoT"@en ;
  sto:hasOfficialResource <https://www.ericsson.com/news/1987789> ;
.
sto:EclipsePaho
  a owl:NamedIndividual ;
  a foaf:Document ;
  a sto:Publication ;
  a sto:TechnicalSpecification ;
  terms:creator sto:sebastian ;
  rdfs:comment "The scope of the Paho project is to provide open source implementations of open and standard messaging protocols that support current and emerging requirements of M2M integration with Web and Enterprise middleware and applications. It will include client implementations for use on embedded platforms along with corresponding server support as determined by the community. (source: https://www.postscapes.com/internet-of-things-protocols/)"@en ;
  rdfs:label "Eclipse Paho Project"@en ;
  sto:hasOfficialResource <https://www.eclipse.org/proposals/technology.paho/> ;
.
sto:Eddystone
  a owl:NamedIndividual ;
  a foaf:Document ;
  a sto:Publication ;
  a sto:TechnicalSpecification ;
  terms:creator sto:sebastian ;
  rdfs:comment "Eddystone - A protocol specification that defines a Bluetooth low energy (BLE) message format for proximity beacon messages. (source: https://www.postscapes.com/internet-of-things-protocols/)"@en ;
  rdfs:label "Eddystone"@en ;
  sto:hasOfficialResource <https://github.com/google/eddystone> ;
.
sto:EdgeAnalytics
  a owl:NamedIndividual ;
  a sto:Concern ;
  terms:creator sto:Priyanka ;
  rdfs:comment "The concern of being able to understanding the states, conditions and behaviors of the systems under control and other systems by interpreting and correlating data gathered from sensors and other systems."@en ;
  rdfs:label "Edge Analytics"@en ;
  skos:narrower sto:Analytics ;
  skos:note "Publications referred: 'IIC:PUB:G1:V1.80:20170131' '6.1 THE CONTROL DOMAIN' 'Page 29' " ;
  sto:hasWikipediaArticle <https://en.wikipedia.org/wiki/Edge_computing> ;
.
sto:EdgeComputing
  a owl:NamedIndividual ;
  a sto:Concern ;
  rdfs:comment "Edge Computing is pushing the frontier of computing applications, data, and services away from centralized nodes to the logical extremes of a network. It enables analytics and knowledge generation to occur at the source of the data. This approach requires leveraging resources that may not be continuously connected to a network such as laptops, smartphones, tablets and sensors. Edge Computing covers a wide range of technologies including wireless sensor networks, mobile data acquisition, mobile signature analysis, cooperative distributed peer-to-peer ad hoc networking and processing also classifiable as Local Cloud/Fog computing and Grid/Mesh Computing, dew computing, mobile edge computing, cloudlet, distributed data storage and retrieval, autonomic self-healing networks, remote cloud services, augmented reality, and more. (source: wikipedia)"@en ;
  rdfs:label "Edge computing"@en ;
  sto:hasDBpediaResource <http://dbpedia.org/resource/Edge_computing> ;
  sto:supports sto:CloudComputing ;
  sto:supports sto:DataProcessing ;
.
sto:EdgecrossArchitecture
  a owl:NamedIndividual ;
  a sto:ArchitectureDescription ;
  a sto:StandardizationFramework ;
  rdfs:label "Edgecross Architecture"@en ;
  sto:hasPublisher sto:EdgecrossConsortium ;
.
sto:EdgecrossConsortium
  a owl:NamedIndividual ;
  a foaf:Organization ;
  a sto:IIoTConsortium ;
  a sto:StandardOrganization ;
  rdfs:label "Edgecross Consortium"@en ;
  sto:hasOfficialResource <https://www.edgecross.org/en/> ;
.
sto:EdgecrossEdgeComputingLayer
  a owl:NamedIndividual ;
  a sto:EdgecrossLayer ;
  a sto:StandardClassification ;
  dul:associatedWith sto:IDSRAMSystemLayer ;
  dul:associatedWith sto:IIRAControlDomain ;
  dul:associatedWith sto:IIRAOperationsDomain ;
  dul:associatedWith sto:InformationDomain ;
  dul:associatedWith sto:RAMIInformationLayer ;
  dul:associatedWith sto:RAMIIntegrationLayer ;
  rdfs:label "Edgecross Edgecomputing Layer"@en ;
  sto:alignsWith sto:IDSRAMSystemLayer ;
  sto:alignsWith sto:IIRAControlDomain ;
  sto:alignsWith sto:IIRAOperationsDomain ;
  sto:alignsWith sto:InformationDomain ;
  sto:alignsWith sto:RAMIInformationLayer ;
  sto:alignsWith sto:RAMIIntegrationLayer ;
  sto:frames sto:CloudComputing ;
  sto:frames sto:DataProcessing ;
  sto:frames sto:EdgeComputing ;
  sto:frames sto:Interoperability ;
  sto:frames sto:SemanticInteroperability ;
  sto:isDescribedin sto:EdgecrossArchitecture ;
.
sto:EdgecrossEdgeComputingLayerAnno
  a <https://www.w3.org/ns/oaAnnotation> ;
  <https://www.w3.org/ns/oahasBody> sto:EdgecrossEdgeComputingLayer ;
  <https://www.w3.org/ns/oahasTarget> [
      a <https://www.w3.org/ns/oaSpecificResource> ;
      terms:format "pdf" ;
      <https://www.w3.org/ns/oahasSelector> [
          a <https://www.w3.org/ns/oaRangeSelector> ;
          <https://www.w3.org/ns/oahasEndSelector> [
              a <https://www.w3.org/ns/oaXPathSelector> ;
              rdf:value "Page 15" ;
            ] ;
          <https://www.w3.org/ns/oahasStartSelector> [
              a <https://www.w3.org/ns/oaXPathSelector> ;
              rdf:value "Page 9" ;
            ] ;
        ] ;
      <https://www.w3.org/ns/oahasSource> sto:Edgecross_Consortium_to_Address_Edge_Integration_in_IIoT_enabled_Architectures ;
    ] ;
.
sto:EdgecrossFacilityLayer
  a owl:NamedIndividual ;
  a sto:EdgecrossLayer ;
  a sto:StandardClassification ;
  dul:associatedWith sto:IIRAPhysicalSystems ;
  dul:associatedWith sto:RAMIAssetlayer ;
  rdfs:label "Edgecross FA"@en ;
  sto:alignsWith sto:IIRAPhysicalSystems ;
  sto:alignsWith sto:RAMIAssetlayer ;
  sto:isDescribedin sto:EdgecrossArchitecture ;
.
sto:EdgecrossFacilityLayerAnno
  a <https://www.w3.org/ns/oaAnnotation> ;
  <https://www.w3.org/ns/oahasBody> sto:EdgecrossFacilityLayer ;
  <https://www.w3.org/ns/oahasTarget> [
      a <https://www.w3.org/ns/oaSpecificResource> ;
      terms:format "pdf" ;
      <https://www.w3.org/ns/oahasSelector> [
          a <https://www.w3.org/ns/oaRangeSelector> ;
          <https://www.w3.org/ns/oahasEndSelector> [
              a <https://www.w3.org/ns/oaXPathSelector> ;
              rdf:value "Page 15" ;
            ] ;
          <https://www.w3.org/ns/oahasStartSelector> [
              a <https://www.w3.org/ns/oaXPathSelector> ;
              rdf:value "Page 9" ;
            ] ;
        ] ;
      <https://www.w3.org/ns/oahasSource> sto:Edgecross_Consortium_to_Address_Edge_Integration_in_IIoT_enabled_Architectures ;
    ] ;
.
sto:EdgecrossItSystemsLayer
  a owl:NamedIndividual ;
  a sto:EdgecrossLayer ;
  a sto:StandardClassification ;
  dul:associatedWith sto:IDSRAMSystemLayer ;
  dul:associatedWith sto:IIRAApplicationDomain ;
  dul:associatedWith sto:RAMIIntegrationLayer ;
  rdfs:label "Edgecross IT Systems Layer"@en ;
  sto:alignsWith sto:IDSRAMSystemLayer ;
  sto:alignsWith sto:IIRAApplicationDomain ;
  sto:alignsWith sto:RAMIIntegrationLayer ;
  sto:frames sto:Communication ;
  sto:frames sto:DataAnalytics ;
  sto:frames sto:DataInMotion ;
  sto:isDescribedin sto:EdgecrossArchitecture ;
.
sto:EdgecrossItSystemsLayerAnno
  a <https://www.w3.org/ns/oaAnnotation> ;
  <https://www.w3.org/ns/oahasBody> sto:EdgecrossItSystemsLayer ;
  <https://www.w3.org/ns/oahasTarget> [
      a <https://www.w3.org/ns/oaSpecificResource> ;
      terms:format "pdf" ;
      <https://www.w3.org/ns/oahasSelector> [
          a <https://www.w3.org/ns/oaRangeSelector> ;
          <https://www.w3.org/ns/oahasEndSelector> [
              a <https://www.w3.org/ns/oaXPathSelector> ;
              rdf:value "Page 15" ;
            ] ;
          <https://www.w3.org/ns/oahasStartSelector> [
              a <https://www.w3.org/ns/oaXPathSelector> ;
              rdf:value "Page 9" ;
            ] ;
        ] ;
      <https://www.w3.org/ns/oahasSource> sto:Edgecross_Consortium_to_Address_Edge_Integration_in_IIoT_enabled_Architectures ;
    ] ;
.
sto:EdgecrossLayer
  a owl:Class ;
  rdfs:label "Edgecross Layer"@en ;
  rdfs:subClassOf sto:StandardClassification ;
  rdfs:subClassOf [
      a owl:Restriction ;
      owl:hasValue sto:EdgecrossArchitecture ;
      owl:onProperty sto:isDescribedin ;
    ] ;
.
sto:EdgecrossLayerAnno
  a <https://www.w3.org/ns/oaAnnotation> ;
  <https://www.w3.org/ns/oahasBody> sto:EdgecrossLayer ;
  <https://www.w3.org/ns/oahasTarget> [
      a <https://www.w3.org/ns/oaSpecificResource> ;
      terms:format "pdf" ;
      <https://www.w3.org/ns/oahasSource> sto:Edgecross_Consortium_to_Address_Edge_Integration_in_IIoT_enabled_Architectures ;
    ] ;
.
sto:EdgecrossWhitepaper
  a owl:NamedIndividual ;
  a foaf:Document ;
  a sto:Publication ;
  terms:creator sto:EdgecrossConsortium ;
  rdfs:label "Edgecross Whitepaper"@en ;
  foaf:maker sto:EdgecrossConsortium ;
  sto:hasClassification sto:EdgecrossEdgeComputingLayer ;
  sto:hasClassification sto:EdgecrossFacilityLayer ;
  sto:hasClassification sto:EdgecrossItSystemsLayer ;
  sto:hasOfficialResource <https://www.edgecross.org/ja/data-download/pdf/Edgecross_Consortium_WP(E).pdf> ;
  sto:hasPublisher sto:EdgecrossConsortium ;
  sto:hasTargetConcern sto:EdgeComputing ;
  sto:hasTargetConcern sto:Interoperability ;
.
sto:Edgecross_Consortium_to_Address_Edge_Integration_in_IIoT_enabled_Architectures
  a <https://www.w3.org/ns/oaSpecificResource> ;
  rdfs:label "Edgecross Consortium to Address Edge Integration in IIoT-enabled Architectures"@en ;
  sto:hasOpenResource <https://www.edgecross.org/ja/data-download/pdf/Edgecross_Consortium_WP(E).pdf> ;
.
sto:EnOcean
  a owl:NamedIndividual ;
  a foaf:Document ;
  a sto:Publication ;
  a sto:TechnicalSpecification ;
  terms:creator sto:sebastian ;
  rdfs:comment "EnOcean is a an energy harvesting wireless technology which works in the frequencies of 868 MHz for europe and 315 MHz for North America. The transmit range goes up to 30 meter in buildings and up to 300 meter outdoor. (source: https://www.postscapes.com/internet-of-things-protocols/)"@en ;
  rdfs:label "EnOcean"@en ;
  sto:hasOfficialResource <http://www.enocean.com/en/home/> ;
.
sto:EndpointDescription
  a owl:NamedIndividual ;
  a sto:Concern ;
  terms:creator sto:sebastian ;
  rdfs:comment "Methods to unambiguously describe client and server endpoints."@en ;
  rdfs:label "Endpoint Description"@en ;
  sto:supports sto:SemanticInteroperability ;
.
sto:EndpointInvocation
  a owl:NamedIndividual ;
  a sto:Concern ;
  terms:creator sto:sebastian ;
  rdfs:comment "Mechanisms to interact with a service and to access it through the network."@en ;
  rdfs:label "Endpoint Invocation"@en ;
  rdfs:seeAlso "IoT-A Requirement UNI.100" ;
  rdfs:seeAlso "IoT-A Requirement UNI.417" ;
  sto:supports sto:SyntacticInteroperability ;
.
sto:EnergyControl
  a owl:NamedIndividual ;
  a sto:Concern ;
  rdfs:label "Energy Control"@en ;
  rdfs:seeAlso "IoT-A Requirement UNI.100" ;
  rdfs:seeAlso "IoT-A Requirement UNI.101" ;
  rdfs:seeAlso "IoT-A Requirement UNI.309" ;
  rdfs:seeAlso "IoT-A Requirement UNI.310" ;
  rdfs:seeAlso "IoT-A Requirement UNI.505" ;
  rdfs:seeAlso "IoT-A Requirement UNI.512" ;
  rdfs:seeAlso "IoT-A Requirement UNI.714" ;
  rdfs:seeAlso "https://ieeexplore.ieee.org/document/7488250" ;
  sto:hasWikipediaArticle <https://en.wikipedia.org/wiki/Internet_of_things#Energy_management> ;
  sto:supports sto:EnergyEfficiency ;
.
sto:EnergyEfficiency
  a owl:NamedIndividual ;
  a rami:AdminShellSubmodel ;
  a sto:Concern ;
  a sto:StandardClassification ;
  rdfs:comment "Efficient energy use, sometimes simply called energy efficiency, is the goal to reduce the amount of energy required to provide products and services."@en ;
  rdfs:label "Energy Efficiency"@en ;
  rdfs:seeAlso "https://dl.acm.org/citation.cfm?doid=2508075.2508082"@en ;
  rdfs:seeAlso "https://dl.acm.org/citation.cfm?doid=3266237.3266263"@en ;
  sto:hasWikipediaArticle "https://en.wikipedia.org/wiki/Efficient_energy_use"@en ;
  sto:isDescribedin sto:AdministrationShell ;
  sto:supports sto:IoT ;
.
sto:EnterpriseIntegration
  a owl:NamedIndividual ;
  a sto:Domain ;
  rdfs:comment "Enterprise Integration deals primarily with system interconnection, electronic data interchange, product data exchange and distributed computing environments."@en ;
  rdfs:label "EnterpriseIntegration"@en ;
  sto:domainName "EnterpriseIntegration"@en ;
  sto:hasWikipediaArticle <https://en.wikipedia.org/wiki/Enterprise_integration> ;
.
sto:EnterpriseLevel
  a owl:NamedIndividual ;
  a sto:ISA95Level ;
  a sto:StandardClassification ;
  rdfs:comment "Describes the Enterprise level according to the ISA95 level classification."@en ;
  rdfs:label "Enterprise Level"@en ;
.
sto:EstonianInformationSystemAuthority
  a owl:NamedIndividual ;
  a foaf:Organization ;
  a sto:StandardOrganization ;
  rdfs:label "Information System Authority of Estonia"@en ;
  sto:hasOfficialResource <https://www.ria.ee/en.html> ;
.
sto:European_BDV_SRIA_version_4_0
  a <https://www.w3.org/ns/oaSpecificResource> ;
  rdfs:label "BDV SRIA European Big Data Value Strategic Research and Innovation Agenda version 4.0 October 2017"@en ;
  sto:hasOpenResource <http://bdva.eu/sites/default/files/BDVA_SRIA_v4_Ed1.1.pdf> ;
.
sto:EventDrivenMessaging
  a owl:NamedIndividual ;
  a sto:Concern ;
  <http://voag.linkedmodel.org/voag#hasStakeholder> <https://www.wikidata.org/wiki/Q1548249> ;
  rdfs:label "Event-Driven Messaging"@en ;
  rdfs:seeAlso "IoT-A Requirement UNI.005" ;
  rdfs:seeAlso "IoT-A Requirement UNI.233" ;
  sto:hasDBpediaResource <http://dbpedia.org/page/Event-Driven_Messaging> ;
  sto:supports sto:DataInMotion ;
.
sto:Evolvability
  a owl:NamedIndividual ;
  a sto:Concern ;
  terms:creator sto:sebastian ;
  rdfs:comment "A system shall accomodate fast developmental changes in applications and network."@en ;
  rdfs:label "Evolvability"@en ;
  rdfs:seeAlso "IoT-A Requirement UNI.701" ;
  rdfs:seeAlso "IoT-A Requirement UNI.702" ;
  sto:hasDBpediaResource <http://dbpedia.org/resource/Evolving_intelligent_system> ;
  sto:hasDBpediaResource <http://dbpedia.org/resource/Software_evolution> ;
  sto:supports sto:DynamicAdjustability ;
.
sto:Extensibility
  a owl:NamedIndividual ;
  a sto:Concern ;
  terms:creator sto:MuhammadUsman ;
  rdfs:comment "\"Extensibility could be a huge challenge at the edge of the network, unlike a mobile system, the things in the IoT could be very dynamic. When the owner purchases a new thing, can it be easily added to the current service without any problem? Or when one thing is replaced due to wearing out, can the previous service adopt a new node easily? These problems should be solved with a flexible and extensible design of service management layer in the edgeOS.\""@en ;
  rdfs:label "Extensibility"@en ;
  rdfs:seeAlso "https://ieeexplore.ieee.org/document/7488250" ;
  sto:hasWikipediaArticle "https://en.wikipedia.org/wiki/Extensibility"@en ;
  sto:supports sto:Evolvability ;
.
sto:FIWARE
  a owl:NamedIndividual ;
  a sto:ArchitectureDescription ;
  a sto:StandardizationFramework ;
  terms:creator sto:sebastian ;
  dul:associatedWith sto:IDSRAMSystemLayer ;
  dul:associatedWith sto:IIRAImplementationViewpoint ;
  rdfs:comment "The FIWARE platform contains market-ready open source software, combining components that enable the connection to IoT with Context Information Management and Big Data services in the Cloud."@en ;
  rdfs:label "FIWARE Architecture"@en ;
  sto:alignsWith sto:IDSRAMSystemLayer ;
  sto:alignsWith sto:IIRAImplementationViewpoint ;
  sto:hasOfficialResource <https://www.fiware.org/> ;
  sto:hasPublisher :Fiware ;
.
sto:FIWAREAnno
  a <https://www.w3.org/ns/oaAnnotation> ;
  <https://www.w3.org/ns/oahasBody> sto:FIWARE ;
  <https://www.w3.org/ns/oahasTarget> [
      a <https://www.w3.org/ns/oaSpecificResource> ;
      <https://www.w3.org/ns/oahasSource> <https://forge.fiware.org/plugins/mediawiki/wiki/fiware/index.php/Summary_of_FI-WARE_Open_Specifications> ;
    ] ;
.
sto:Fairness
  a owl:NamedIndividual ;
  a sto:Concern ;
  terms:creator sto:MuhammadUsman ;
  rdfs:comment "How can a fair and non-discriminating access to (compute and storage) resources be established?"@en ;
  rdfs:label "Fairness"@en ;
  rdfs:seeAlso "https://dl.acm.org/citation.cfm?doid=3098208.3098210" ;
  sto:hasWikipediaArticle "https://en.wikipedia.org/wiki/Fairness"@en ;
  sto:supports sto:BusinessContext ;
.
sto:FaultTolerance
  a owl:NamedIndividual ;
  a sto:Concern ;
  terms:creator sto:MuhammadUsman ;
  rdfs:comment "Fault tolerance is the property that enables a system to continue operating properly in the event of the failure of some (one or more faults within) of its components. If its operating quality decreases at all, the decrease is proportional to the severity of the failure, as compared to a naively designed system in which even a small failure can cause total breakdown."@en ;
  rdfs:label "Fault Tolerance"@en ;
  rdfs:seeAlso "https://dl.acm.org/citation.cfm?doid=2508075.2508082"@en ;
  rdfs:seeAlso "https://ieeexplore.ieee.org/document/6188257"@en ;
  rdfs:seeAlso "https://ieeexplore.ieee.org/document/8304465"@en ;
  sto:hasDBpediaResource "http://dbpedia.org/page/Category:Fault-tolerant_computer_systems"@en ;
  sto:hasWikipediaArticle "https://en.wikipedia.org/wiki/Fault_tolerance"@en ;
  sto:supports sto:Availability ;
.
sto:FileSizeIEC_60027_P6
  a om2:Measure ;
  a owl:NamedIndividual ;
  om2:hasNumericalValue "661.0"^^xsd:float ;
  om2:hasUnit om2:kilobyte ;
  rdfs:comment "Specifies the file size of the document for standard IEC 60027:2006"@en ;
  rdfs:label "FileSize IEC 60027-6:2006"@en ;
.
sto:FileSizeIEC_60038
  a om2:Measure ;
  a owl:NamedIndividual ;
  om2:hasNumericalValue "946.0"^^xsd:float ;
  om2:hasUnit om2:kilobyte ;
  rdfs:comment "Specifies the file size of the document for standard IEC 60038:2009"@en ;
  rdfs:label "FileSize IEC 60038:2009"@en ;
.
sto:FileSizeIEC_60050_P101
  a om2:Measure ;
  a owl:NamedIndividual ;
  om2:hasNumericalValue "1712.0"^^xsd:float ;
  om2:hasUnit om2:kilobyte ;
  rdfs:comment "Specifies the file size of the document for standard IEC 60050-101:1998 "@en ;
  rdfs:label "FileSize IEC 60050-101:1998"@en ;
.
sto:FileSizeIEC_60050_P351
  a om2:Measure ;
  a owl:NamedIndividual ;
  om2:hasNumericalValue "3999.0"^^xsd:float ;
  om2:hasUnit om2:kilobyte ;
  rdfs:comment "Specifies the file size of the document for standard IEC 60050-351:2013 "@en ;
  rdfs:label "FileSize IEC 60050-351:2013"@en ;
.
sto:FileSizeIEC_60050_P371
  a om2:Measure ;
  a owl:NamedIndividual ;
  om2:hasNumericalValue "2485.0"^^xsd:float ;
  om2:hasUnit om2:kilobyte ;
  rdfs:comment "Specifies the file size of the document for standard IEC 60050-101:1998 "@en ;
  rdfs:label "FileSize IEC 60050-371:1984"@en ;
.
sto:FileSizeIEC_60073
  a om2:Measure ;
  a owl:NamedIndividual ;
  om2:hasNumericalValue "525.0"^^xsd:float ;
  om2:hasUnit om2:kilobyte ;
  rdfs:comment "Specifies the file size of the document for standard IEC 60073:2002"@en ;
  rdfs:label "FileSize IEC 60073:2002"@en ;
.
sto:FileSizeIEC_60204
  a om2:Measure ;
  a owl:NamedIndividual ;
  om2:hasNumericalValue "494.0"^^xsd:float ;
  om2:hasUnit om2:kilobyte ;
  rdfs:comment "Specifies the file size of the document for standard IEC 60204:2000"@en ;
  rdfs:label "FileSize IEC 60204:2000"@en ;
.
sto:FileSizeIEC_60204_P11
  a owl:NamedIndividual ;
.
sto:FileSizeIEC_60255_P1
  a om2:Measure ;
  a owl:NamedIndividual ;
  om2:hasNumericalValue "1411.0"^^xsd:float ;
  om2:hasUnit om2:kilobyte ;
  rdfs:comment "Specifies the file size of the document for standard 60255-1:2009"@en ;
  rdfs:label "FileSize IEC 60255-1:2009"@en ;
.
sto:FileSizeIEC_60255_P127
  a om2:Measure ;
  a owl:NamedIndividual ;
  om2:hasNumericalValue "1215.0"^^xsd:float ;
  om2:hasUnit om2:kilobyte ;
  rdfs:comment "Specifies the file size of the document for standard IEC 60255-127:2010 "@en ;
  rdfs:label "FileSize 60255-127:2010"@en ;
.
sto:FileSizeIEC_60255_P149
  a om2:Measure ;
  a owl:NamedIndividual ;
  om2:hasNumericalValue "1722.0"^^xsd:float ;
  om2:hasUnit om2:kilobyte ;
  rdfs:comment "Specifies the file size of the document for standard IEC 60255-149:2013 "@en ;
  rdfs:label "FileSize 60255-149:2013"@en ;
.
sto:FileSizeIEC_60255_P151
  a om2:Measure ;
  a owl:NamedIndividual ;
  om2:hasNumericalValue "1341.0"^^xsd:float ;
  om2:hasUnit om2:kilobyte ;
  rdfs:comment "Specifies the file size of the document for standard IEC IEC 60255-151:2009"@en ;
  rdfs:label "FileSize IEC 60255-151:2009 "@en ;
.
sto:FileSizeIEC_60255_P27
  a om2:Measure ;
  a owl:NamedIndividual ;
  om2:hasNumericalValue "2520.0"^^xsd:float ;
  om2:hasUnit om2:kilobyte ;
  rdfs:comment "Specifies the file size of the document for standard IEC 60255-27:2013"@en ;
  rdfs:label "FileSize IEC 60255-27:2013"@en ;
.
sto:FileSizeIEC_60286_P3
  a om2:Measure ;
  a owl:NamedIndividual ;
  om2:hasNumericalValue "1764.0"^^xsd:float ;
  om2:hasUnit om2:kilobyte ;
  rdfs:comment "Specifies the file size of the document for standard IEC IEC 60286-3:2013 "@en ;
  rdfs:label "FileSize IEC 60286-3:2013  "@en ;
.
sto:FileSizeIEC_60286_P4
  a om2:Measure ;
  a owl:NamedIndividual ;
  om2:hasNumericalValue "1129.0"^^xsd:float ;
  om2:hasUnit om2:kilobyte ;
  rdfs:comment "Specifies the file size of the document for standard IEC IEC 60286-4:2013 "@en ;
  rdfs:label "FileSize IEC 60286-4:2013  "@en ;
.
sto:FileSizeIEC_60286_P5
  a om2:Measure ;
  a owl:NamedIndividual ;
  om2:hasNumericalValue "3481.0"^^xsd:float ;
  om2:hasUnit om2:kilobyte ;
  rdfs:comment "Specifies the file size of the document for standard IEC IEC 60286-5:2018 "@en ;
  rdfs:label "FileSize IEC 60286-5:2018  "@en ;
.
sto:FileSizeIEC_60381_P1
  a om2:Measure ;
  a owl:NamedIndividual ;
  om2:hasNumericalValue "507.0"^^xsd:float ;
  om2:hasUnit om2:kilobyte ;
  rdfs:comment "Specifies the file size of the document for standard IEC 60381-1:1982 "@en ;
  rdfs:label "FileSize IEC 60381-1:1982"@en ;
.
sto:FileSizeIEC_60381_P2
  a om2:Measure ;
  a owl:NamedIndividual ;
  om2:hasNumericalValue "483.0"^^xsd:float ;
  om2:hasUnit om2:kilobyte ;
  rdfs:comment "Specifies the file size of the document for standard IEC 60381-2:1978"@en ;
  rdfs:label "FileSize IEC 60381-2:1978"@en ;
.
sto:FileSizeIEC_60382
  a om2:Measure ;
  a owl:NamedIndividual ;
  om2:hasNumericalValue "1460.0"^^xsd:float ;
  om2:hasNumericalValue "557.0"^^xsd:float ;
  om2:hasUnit om2:kilobyte ;
  rdfs:comment "Specifies the file size of the document for standard  IEC 60382:1991."@en ;
  rdfs:comment "Specifies the file size of the document for standard IEC 60382:1991"@en ;
  rdfs:label "FileSize IEC 60382:1991"@en ;
.
sto:FileSizeIEC_60839_P5_S2
  a om2:Measure ;
  a owl:NamedIndividual ;
  om2:hasNumericalValue "1137.0"^^xsd:float ;
  om2:hasUnit om2:kilobyte ;
  rdfs:comment "Specifies the file size of the document for standard IEC 60839-5-2:2016"@en ;
  rdfs:label "FileSize IEC 60839-5-2:2016"@en ;
.
sto:FileSizeIEC_60839_P7_S1
  a om2:Measure ;
  a owl:NamedIndividual ;
  om2:hasNumericalValue "1137.0"^^xsd:float ;
  om2:hasUnit om2:kilobyte ;
  rdfs:comment "Specifies the file size of the document for standard IEC 60839-7-1:2001"@en ;
  rdfs:label "FileSize IEC 60839-7-1:2001"@en ;
.
sto:FileSizeIEC_60839_P7_S2
  a om2:Measure ;
  a owl:NamedIndividual ;
  om2:hasNumericalValue "1047.0"^^xsd:float ;
  om2:hasUnit om2:kilobyte ;
  rdfs:comment "Specifies the file size of the document for standard IEC 60839-7-2:2001"@en ;
  rdfs:label "FileSize IEC 60839-7-2:2001"@en ;
.
sto:FileSizeIEC_60839_P7_S3
  a om2:Measure ;
  a owl:NamedIndividual ;
  om2:hasNumericalValue "975.0"^^xsd:float ;
  om2:hasUnit om2:kilobyte ;
  rdfs:comment "Specifies the file size of the document for standard IEC 60839-7-3:2001"@en ;
  rdfs:label "FileSize IEC 60839-7-3:2001"@en ;
.
sto:FileSizeIEC_60839_P7_S4
  a om2:Measure ;
  a owl:NamedIndividual ;
  om2:hasNumericalValue "967.0"^^xsd:float ;
  om2:hasUnit om2:kilobyte ;
  rdfs:comment "Specifies the file size of the document for standard IEC 60839-7-4:2001"@en ;
  rdfs:label "FileSize IEC 60839-7-4:2001"@en ;
.
sto:FileSizeIEC_60839_P7_S5
  a om2:Measure ;
  a owl:NamedIndividual ;
  om2:hasNumericalValue "939.0"^^xsd:float ;
  om2:hasUnit om2:kilobyte ;
  rdfs:comment "Specifies the file size of the document for standard IEC 60839-7-5:2001"@en ;
  rdfs:label "FileSize IEC 60839-7-5:2001"@en ;
.
sto:FileSizeIEC_60839_P7_S6
  a om2:Measure ;
  a owl:NamedIndividual ;
  om2:hasNumericalValue "926.0"^^xsd:float ;
  om2:hasUnit om2:kilobyte ;
  rdfs:comment "Specifies the file size of the document for standard IEC 60839-7-6:2001"@en ;
  rdfs:label "FileSize IEC 60839-7-6:2001"@en ;
.
sto:FileSizeIEC_60839_P7_S7
  a om2:Measure ;
  a owl:NamedIndividual ;
  om2:hasNumericalValue "964.0"^^xsd:float ;
  om2:hasUnit om2:kilobyte ;
  rdfs:comment "Specifies the file size of the document for standard IEC 60839-7-7:2001"@en ;
  rdfs:label "FileSize IEC 60839-7-7:2001"@en ;
.
sto:FileSizeIEC_60848
  a om2:Measure ;
  a owl:NamedIndividual ;
  om2:hasNumericalValue "1784.0"^^xsd:float ;
  om2:hasUnit om2:kilobyte ;
  rdfs:comment "Specifies the file size of the document for standard IEC 60848:2013"@en ;
  rdfs:label "FileSize IEC 60848:2013"@en ;
.
sto:FileSizeIEC_60864_P1
  a om2:Measure ;
  a owl:NamedIndividual ;
  om2:hasNumericalValue "1540.0"^^xsd:float ;
  om2:hasUnit om2:kilobyte ;
  rdfs:comment "Specifies the file size of the document for standard IEC 60864-1:1986 "@en ;
  rdfs:label "FileSizeIEC 60864-1:1986"@en ;
.
sto:FileSizeIEC_60864_P2
  a om2:Measure ;
  a owl:NamedIndividual ;
  om2:hasNumericalValue "283.0"^^xsd:float ;
  om2:hasUnit om2:kilobyte ;
  rdfs:comment "Specifies the file size of the document for standard IEC 60864-2:1997"@en ;
  rdfs:label "FileSize IEC 60864-2:1997"@en ;
.
sto:FileSizeIEC_60870_1990_P5_S1
  a om2:Measure ;
  a owl:NamedIndividual ;
  om2:hasNumericalValue "2954.0"^^xsd:float ;
  om2:hasUnit om2:kilobyte ;
  rdfs:comment "Specifies the file size of the document for standard IEC 60870-5-1:1990"@en ;
  rdfs:label "FileSize IEC 60870-5-1:1990"@en ;
.
sto:FileSizeIEC_60870_1992_P5_S2
  a om2:Measure ;
  a owl:NamedIndividual ;
  om2:hasNumericalValue "3658.0"^^xsd:float ;
  om2:hasUnit om2:kilobyte ;
  rdfs:comment "Specifies the file size of the document for standard IEC 60870-5-2:1992"@en ;
  rdfs:label "FileSize IEC 60870-5-2:1992"@en ;
.
sto:FileSizeIEC_60870_1992_P5_S3
  a om2:Measure ;
  a owl:NamedIndividual ;
  om2:hasNumericalValue "1629.0"^^xsd:float ;
  om2:hasUnit om2:kilobyte ;
  rdfs:comment "Specifies the file size of the document for standard IEC 60870-5-3:1992"@en ;
  rdfs:label "FileSize IEC 60870-5-3:1992"@en ;
.
sto:FileSizeIEC_60870_1995_P2_S1
  a om2:Measure ;
  a owl:NamedIndividual ;
  om2:hasNumericalValue "1674.0"^^xsd:float ;
  om2:hasUnit om2:kilobyte ;
  rdfs:comment "Specifies the file size of the document for standard IEC 60870-2-1:1995"@en ;
  rdfs:label "FileSize IEC 60870-2-1:1995"@en ;
.
sto:FileSizeIEC_60870_1996_P2_S2
  a om2:Measure ;
  a owl:NamedIndividual ;
  om2:hasNumericalValue "1705.0"^^xsd:float ;
  om2:hasUnit om2:kilobyte ;
  rdfs:comment "Specifies the file size of the document for standard IEC 60870-2-2:1996"@en ;
  rdfs:label "FileSize IEC 60870-2-2:1996"@en ;
.
sto:FileSizeIEC_60870_P2_S1
  a owl:NamedIndividual ;
.
sto:FileSizeIEC_60870_P2_S2
  a owl:NamedIndividual ;
.
sto:FileSizeIEC_60870_P5_S1
  a owl:NamedIndividual ;
.
sto:FileSizeIEC_60870_P5_S101
  a owl:NamedIndividual ;
.
sto:FileSizeIEC_60870_P5_S101_2003
  a om2:Measure ;
  a owl:NamedIndividual ;
  om2:hasNumericalValue "2651.0"^^xsd:float ;
  om2:hasUnit om2:kilobyte ;
  rdfs:comment "Specifies the file size of the document for standard IEC 60870-5-101:2003"@en ;
  rdfs:label "FileSize IEC 60870-5-101:2003"@en ;
.
sto:FileSizeIEC_60870_P5_S102
  a om2:Measure ;
  a owl:NamedIndividual ;
  om2:hasNumericalValue "505.0"^^xsd:float ;
  om2:hasUnit om2:kilobyte ;
  rdfs:comment "Specifies the file size of the document for standard IEC 60870-5-102:1996"@en ;
  rdfs:label "FileSize IEC 60870-5-102:1996"@en ;
.
sto:FileSizeIEC_60870_P5_S103
  a om2:Measure ;
  a owl:NamedIndividual ;
  om2:hasNumericalValue "964.0"^^xsd:float ;
  om2:hasUnit om2:kilobyte ;
  rdfs:comment "Specifies the file size of the document for standard IEC 60870-5-103:1997"@en ;
  rdfs:label "FileSize IEC 60870-5-103:1997"@en ;
.
sto:FileSizeIEC_60870_P5_S104
  a om2:Measure ;
  a owl:NamedIndividual ;
  om2:hasNumericalValue "2994.0"^^xsd:float ;
  om2:hasUnit om2:kilobyte ;
  rdfs:comment "Specifies the file size of the document for standard IEC 60870-5-104:2006"@en ;
  rdfs:label "FileSize IEC 60870-5-104:2006"@en ;
.
sto:FileSizeIEC_60870_P5_S2
  a owl:NamedIndividual ;
.
sto:FileSizeIEC_60870_P5_S3
  a owl:NamedIndividual ;
.
sto:FileSizeIEC_60870_P5_S4
  a om2:Measure ;
  a owl:NamedIndividual ;
  om2:hasNumericalValue "1776.0"^^xsd:float ;
  om2:hasUnit om2:kilobyte ;
  rdfs:comment "Specifies the file size of the document for standard IEC 60870-5-4:1993"@en ;
  rdfs:label "FileSize IEC 60870-5-4:1993"@en ;
.
sto:FileSizeIEC_60870_P5_S5
  a om2:Measure ;
  a owl:NamedIndividual ;
  om2:hasNumericalValue "3347.0"^^xsd:float ;
  om2:hasUnit om2:kilobyte ;
  rdfs:comment "Specifies the file size of the document for standard IEC 60870-5-5:1995"@en ;
  rdfs:label "FileSize IEC 60870-5-5:1995"@en ;
.
sto:FileSizeIEC_60870_P5_S6
  a om2:Measure ;
  a owl:NamedIndividual ;
  om2:hasNumericalValue "1342.0"^^xsd:float ;
  om2:hasUnit om2:kilobyte ;
  rdfs:comment "Specifies the file size of the document for standard IEC 60870-5-6::2006."@en ;
  rdfs:label "FileSize IEC 60870-5-6:2006"@en ;
.
sto:FileSizeIEC_60870_P6_S2
  a om2:Measure ;
  a owl:NamedIndividual ;
  om2:hasNumericalValue "3524.0"^^xsd:float ;
  om2:hasUnit om2:kilobyte ;
  rdfs:comment "Specifies the file size of the document for standard IEC 60870-6-2:1995"@en ;
  rdfs:label "FileSize IEC 60870-6-2:1995"@en ;
.
sto:FileSizeIEC_60870_P6_S501
  a om2:Measure ;
  a owl:NamedIndividual ;
  om2:hasNumericalValue "578.0"^^xsd:float ;
  om2:hasUnit om2:kilobyte ;
  rdfs:comment "Specifies the file size of the document for standard IEC 60870-6-501:1995"@en ;
  rdfs:label "FileSize IEC 60870-6-501:1995"@en ;
.
sto:FileSizeIEC_60870_P6_S502
  a om2:Measure ;
  a owl:NamedIndividual ;
  om2:hasNumericalValue "1963.0"^^xsd:float ;
  om2:hasUnit om2:kilobyte ;
  rdfs:comment "Specifies the file size of the document for standard IEC 60870-6-502:1995"@en ;
  rdfs:label "FileSize IEC 60870-6-502:1995"@en ;
.
sto:FileSizeIEC_60870_P6_S503
  a om2:Measure ;
  a owl:NamedIndividual ;
  om2:hasNumericalValue "2630.0"^^xsd:float ;
  om2:hasUnit om2:kilobyte ;
  rdfs:comment "Specifies the file size of the document for standard IEC 60870-6-503:2014"@en ;
  rdfs:label "FileSize IEC 60870-6-503:2014"@en ;
.
sto:FileSizeIEC_60870_P6_S601
  a om2:Measure ;
  a owl:NamedIndividual ;
  om2:hasNumericalValue "1112.0"^^xsd:float ;
  om2:hasUnit om2:kilobyte ;
  rdfs:comment "Specifies the file size of the document for standard IEC 60870-6-601:1994"@en ;
  rdfs:label "FileSize IEC 60870-6-601:1994"@en ;
.
sto:FileSizeIEC_60870_P6_S701
  a om2:Measure ;
  a owl:NamedIndividual ;
  om2:hasNumericalValue "130.0"^^xsd:float ;
  om2:hasUnit om2:kilobyte ;
  rdfs:comment "Specifies the file size of the document for standard IEC 60870-6-701:1998"@en ;
  rdfs:label "FileSize IEC 60870-6-701:1998"@en ;
.
sto:FileSizeIEC_60870_P6_S702
  a om2:Measure ;
  a owl:NamedIndividual ;
  om2:hasNumericalValue "1374.0"^^xsd:float ;
  om2:hasUnit om2:kilobyte ;
  rdfs:comment "Specifies the file size of the document for standard IEC 60870-6-702:2014"@en ;
  rdfs:label "FileSize IEC 60870-6-702:2014"@en ;
.
sto:FileSizeIEC_60870_P6_S802
  a om2:Measure ;
  a owl:NamedIndividual ;
  om2:hasNumericalValue "1678.0"^^xsd:float ;
  om2:hasUnit om2:kilobyte ;
  rdfs:comment "Specifies the file size of the document for standard IEC 60870-6-802:2014"@en ;
  rdfs:label "FileSize IEC 60870-6-802:2014"@en ;
.
sto:FileSizeIEC_60946
  a om2:Measure ;
  a owl:NamedIndividual ;
  om2:hasNumericalValue "546.0"^^xsd:float ;
  om2:hasUnit om2:kilobyte ;
  rdfs:comment "Specifies the file size of the document for standard IEC 60946"@en ;
  rdfs:label "FileSize IEC 60946"@en ;
.
sto:FileSizeIEC_61000_P6_S2
  a om2:Measure ;
  a owl:NamedIndividual ;
  om2:hasNumericalValue "2028.0"^^xsd:float ;
  om2:hasUnit om2:kilobyte ;
  rdfs:comment "Specifies the file size of the document for standard IEC 61000-6-2:2016."@en ;
  rdfs:label "FileSize IEC 61000-6-2:2016"@en ;
.
sto:FileSizeIEC_61010_P2_S012
  a om2:Measure ;
  a owl:NamedIndividual ;
  om2:hasNumericalValue "2717.0"^^xsd:float ;
  om2:hasUnit om2:kilobyte ;
  rdfs:comment "Specifies the file size of the document for standard IEC 61010-2-012:2016."@en ;
  rdfs:label "FileSize IEC 61010-2-012:2016"@en ;
.
sto:FileSizeIEC_61010_P2_S201
  a om2:Measure ;
  a owl:NamedIndividual ;
  om2:hasNumericalValue "5743.0"^^xsd:float ;
  om2:hasUnit om2:kilobyte ;
  rdfs:comment "Specifies the file size of the document for standard IEC 61010-2-201:2017."@en ;
  rdfs:label "FileSize IEC 61010-2-201:2017"@en ;
.
sto:FileSizeIEC_61010_P2_S202
  a om2:Measure ;
  a owl:NamedIndividual ;
  om2:hasNumericalValue "1027.0"^^xsd:float ;
  om2:hasUnit om2:kilobyte ;
  rdfs:comment "Specifies the file size of the document for standard IEC 61010-2-202:2016."@en ;
  rdfs:label "FileSize IEC 61010-2-202:2016"@en ;
.
sto:FileSizeIEC_61160
  a om2:Measure ;
  a owl:NamedIndividual ;
  om2:hasNumericalValue "69.0"^^xsd:float ;
  om2:hasUnit om2:kilobyte ;
  rdfs:comment "Specifies the file size of the document for standard  IEC 61160:2005."@en ;
  rdfs:label "FileSize IEC 61160:2005"@en ;
.
sto:FileSizeIEC_61310_P1
  a om2:Measure ;
  a owl:NamedIndividual ;
  om2:hasNumericalValue "763.0"^^xsd:float ;
  om2:hasUnit om2:kilobyte ;
  rdfs:comment "Specifies the file size of the document for standard IEC 61310-1:2007."@en ;
  rdfs:label "FileSize IEC 61310-1:2007"@en ;
.
sto:FileSizeIEC_61310_P2
  a om2:Measure ;
  a owl:NamedIndividual ;
  om2:hasNumericalValue "724.0"^^xsd:float ;
  om2:hasUnit om2:kilobyte ;
  rdfs:comment "Specifies the file size of the document for standard IEC 61310-2:2007."@en ;
  rdfs:label "FileSize IEC 61310-2:2007"@en ;
.
sto:FileSizeIEC_61310_P3
  a om2:Measure ;
  a owl:NamedIndividual ;
  om2:hasNumericalValue "716.0"^^xsd:float ;
  om2:hasUnit om2:kilobyte ;
  rdfs:comment "Specifies the file size of the document for standard IEC 61310-3:2007."@en ;
  rdfs:label "FileSize IEC 61310-3:2007"@en ;
.
sto:FileSizeIEC_61334_P3_S1
  a om2:Measure ;
  a owl:NamedIndividual ;
  om2:hasNumericalValue "147.0"^^xsd:float ;
  om2:hasUnit om2:kilobyte ;
  rdfs:comment "Specifies the file size of the document for standard IEC 61334-3-1:1998 "@en ;
  rdfs:label "FileSize IEC 61334-3-1:1998 "@en ;
.
sto:FileSizeIEC_61334_P3_S21
  a om2:Measure ;
  a owl:NamedIndividual ;
  om2:hasNumericalValue "1112.0"^^xsd:float ;
  om2:hasUnit om2:kilobyte ;
  rdfs:comment "Specifies the file size of the document for standard IEC 61334-3-21:1996 "@en ;
  rdfs:label "FileSize IEC 61334-3-21:1996 "@en ;
.
sto:FileSizeIEC_61334_P3_S22
  a om2:Measure ;
  a owl:NamedIndividual ;
  om2:hasNumericalValue "165.0"^^xsd:float ;
  om2:hasUnit om2:kilobyte ;
  rdfs:comment "Specifies the file size of the document for standard IEC 61334-3-22:2001"@en ;
  rdfs:label "FileSize IEC 61334-3-22:2001"@en ;
.
sto:FileSizeIEC_61334_P4_S1
  a om2:Measure ;
  a owl:NamedIndividual ;
  om2:hasNumericalValue "1707.0"^^xsd:float ;
  om2:hasUnit om2:kilobyte ;
  rdfs:comment "Specifies the file size of the document for standard IEC 61334-4-1:1996"@en ;
  rdfs:label "FileSize IEC 61334-3-22:2000"@en ;
.
sto:FileSizeIEC_61334_P4_S3
  a owl:NamedIndividual ;
.
sto:FileSizeIEC_61334_P4_S32
  a om2:Measure ;
  a owl:NamedIndividual ;
  om2:hasNumericalValue "869.0"^^xsd:float ;
  om2:hasUnit om2:kilobyte ;
  rdfs:comment "Specifies the file size of the document for standard IEC 61334-4-32:1996 "@en ;
  rdfs:label "FileSize IEC 61334-4-32:1996 "@en ;
.
sto:FileSizeIEC_61334_P4_S33
  a om2:Measure ;
  a owl:NamedIndividual ;
  om2:hasNumericalValue "135.0"^^xsd:float ;
  om2:hasUnit om2:kilobyte ;
  rdfs:comment "Specifies the file size of the document for standard IEC 61334-4-33:1998 "@en ;
  rdfs:label "FileSize IEC 61334-4-33:1998"@en ;
.
sto:FileSizeIEC_61334_P4_S41
  a om2:Measure ;
  a owl:NamedIndividual ;
  om2:hasNumericalValue "834.0"^^xsd:float ;
  om2:hasUnit om2:kilobyte ;
  rdfs:comment "Specifies the file size of the document for standard IEC 61334-4-41:1996"@en ;
  rdfs:label "FileSize IEC 61334-4-41:1996"@en ;
.
sto:FileSizeIEC_61334_P4_S42
  a om2:Measure ;
  a owl:NamedIndividual ;
  om2:hasNumericalValue "305.0"^^xsd:float ;
  om2:hasUnit om2:kilobyte ;
  rdfs:comment "Specifies the file size of the document for standard IEC 61334-4-42:1996"@en ;
  rdfs:label "FileSize IEC 61334-4-42:1996"@en ;
.
sto:FileSizeIEC_61334_P4_S511
  a om2:Measure ;
  a owl:NamedIndividual ;
  om2:hasNumericalValue "203.0"^^xsd:float ;
  om2:hasUnit om2:kilobyte ;
  rdfs:comment "Specifies the file size of the document for standard IEC 61334-4-511:2000"@en ;
  rdfs:label "FileSize IEC 61334-4-511:2000"@en ;
.
sto:FileSizeIEC_61334_P4_S512
  a om2:Measure ;
  a owl:NamedIndividual ;
  om2:hasNumericalValue "459.0"^^xsd:float ;
  om2:hasUnit om2:kilobyte ;
  rdfs:comment "Specifies the file size of the document for standard IEC 61334-4-512:2001"@en ;
  rdfs:label "FileSize IEC 61334-4-512:2001"@en ;
.
sto:FileSizeIEC_61334_P4_S61
  a om2:Measure ;
  a owl:NamedIndividual ;
  om2:hasNumericalValue "753.0"^^xsd:float ;
  om2:hasUnit om2:kilobyte ;
  rdfs:comment "Specifies the file size of the document for standard IEC 61334-4-61:1998"@en ;
  rdfs:label "FileSize IEC 61334-4-61:1998"@en ;
.
sto:FileSizeIEC_61334_P5_S1
  a om2:Measure ;
  a owl:NamedIndividual ;
  om2:hasNumericalValue "723.0"^^xsd:float ;
  om2:hasUnit om2:kilobyte ;
  rdfs:comment "Specifies the file size of the document for standard IEC 61334-5-1:2001"@en ;
  rdfs:label "FileSize IEC 61334-5-1:2001"@en ;
.
sto:FileSizeIEC_61334_P6
  a om2:Measure ;
  a owl:NamedIndividual ;
  om2:hasNumericalValue "294.0"^^xsd:float ;
  om2:hasUnit om2:kilobyte ;
  rdfs:comment "Specifies the file size of the document for standard IEC 61334-6:2000"@en ;
  rdfs:label "FileSize IEC 61334-6:2000"@en ;
.
sto:FileSizeIEC_61400_P25_S1
  a om2:Measure ;
  a owl:NamedIndividual ;
  om2:hasNumericalValue "3644.0"^^xsd:float ;
  om2:hasUnit om2:kilobyte ;
  rdfs:comment "Specifies the file size of the document for standard  IEC 61400-25-1:2017."@en ;
  rdfs:label "FileSize IEC 61400-25-1:2017"@en ;
.
sto:FileSizeIEC_61400_P25_S2
  a om2:Measure ;
  a owl:NamedIndividual ;
  om2:hasNumericalValue "3707.0"^^xsd:float ;
  om2:hasUnit om2:kilobyte ;
  rdfs:comment "Specifies the file size of the document for standard IEC 61400-25-2:2015."@en ;
  rdfs:label "FileSize IEC 61400-25-2:2015"@en ;
.
sto:FileSizeIEC_61400_P25_S3
  a om2:Measure ;
  a owl:NamedIndividual ;
  om2:hasNumericalValue "2027.0"^^xsd:float ;
  om2:hasUnit om2:kilobyte ;
  rdfs:comment "Specifies the file size of the document for standard IEC 61400-25-3:2015."@en ;
  rdfs:label "FileSize IEC 61400-25-3:2015"@en ;
.
sto:FileSizeIEC_61400_P25_S4
  a om2:Measure ;
  a owl:NamedIndividual ;
  om2:hasNumericalValue "7800.0"^^xsd:float ;
  om2:hasUnit om2:kilobyte ;
  rdfs:comment "Specifies the file size of the document for standard IEC 61400-25-4:2016."@en ;
  rdfs:label "FileSize IEC 61400-25-4:2016"@en ;
.
sto:FileSizeIEC_61400_P25_S5
  a om2:Measure ;
  a owl:NamedIndividual ;
  om2:hasNumericalValue "1567.0"^^xsd:float ;
  om2:hasUnit om2:kilobyte ;
  rdfs:comment "Specifies the file size of the document for standard IEC 61400-25-5:2017."@en ;
  rdfs:label "FileSize IEC 61400-25-5:2017"@en ;
.
sto:FileSizeIEC_61400_P25_S6
  a om2:Measure ;
  a owl:NamedIndividual ;
  om2:hasNumericalValue "1673.0"^^xsd:float ;
  om2:hasUnit om2:kilobyte ;
  rdfs:comment "Specifies the file size of the document for standard IEC 61400-25-5:2017."@en ;
  rdfs:label "FileSize IEC 61400-25-6:2016"@en ;
.
sto:FileSizeIEC_61506
  a om2:Measure ;
  a owl:NamedIndividual ;
  om2:hasNumericalValue "294.0"^^xsd:float ;
  om2:hasUnit om2:kilobyte ;
  rdfs:comment "Specifies the file size of the document for standard  IEC 61506:1997."@en ;
  rdfs:label "FileSize IEC 61506:1997"@en ;
.
sto:FileSizeIEC_61690_P1
  a om2:Measure ;
  a owl:NamedIndividual ;
  om2:hasNumericalValue "1676.0"^^xsd:float ;
  om2:hasUnit om2:kilobyte ;
  rdfs:comment "Specifies the file size of the document for standard IEC 61690-1:2000 ."@en ;
  rdfs:label "FileSize IEC 61690-1:2000 "@en ;
.
sto:FileSizeIEC_61690_P2
  a om2:Measure ;
  a owl:NamedIndividual ;
  om2:hasNumericalValue "6700.0"^^xsd:float ;
  om2:hasUnit om2:kilobyte ;
  rdfs:comment "Specifies the file size of the document for standard IEC 61690-2:2000 ."@en ;
  rdfs:label "FileSize IEC 61690-2:2000 "@en ;
.
sto:FileSizeIEC_61691_P6
  a om2:Measure ;
  a owl:NamedIndividual ;
  om2:hasNumericalValue "5004.0"^^xsd:float ;
  om2:hasUnit om2:kilobyte ;
  rdfs:comment "Specifies the file size of the document for standard IEC 61691-6:2009."@en ;
  rdfs:label "FileSize IEC 61691-6:2009"@en ;
.
sto:FileSizeIEC_61804_P1
  a om2:Measure ;
  a owl:NamedIndividual ;
  om2:hasNumericalValue "977.0"^^xsd:float ;
  om2:hasUnit om2:kilobyte ;
  rdfs:comment "Specifies the file size of the document for standard IEC 61804-6:2012 "@en ;
  rdfs:label "FileSize IEC 61804-6:2012  "@en ;
.
sto:FileSizeIEC_61804_P3
  a om2:Measure ;
  a owl:NamedIndividual ;
  om2:hasNumericalValue "9306.0"^^xsd:float ;
  om2:hasUnit om2:kilobyte ;
  rdfs:comment "Specifies the file size of the document for standard IEC 61804-3:2015"@en ;
  rdfs:label "FileSize IEC 61804-3:2015"@en ;
.
sto:FileSizeIEC_61804_P4
  a om2:Measure ;
  a owl:NamedIndividual ;
  om2:hasNumericalValue "3514.0"^^xsd:float ;
  om2:hasUnit om2:kilobyte ;
  rdfs:comment "Specifies the file size of the document for standard IEC 61804-4:2015"@en ;
  rdfs:label "FileSize IEC 61804-4:2015"@en ;
.
sto:FileSizeIEC_61804_P5
  a om2:Measure ;
  a owl:NamedIndividual ;
  om2:hasNumericalValue "7931.0"^^xsd:float ;
  om2:hasUnit om2:kilobyte ;
  rdfs:comment "Specifies the file size of the document for standard IEC 61804-5:2015 "@en ;
  rdfs:label "FileSize IEC 61804-5:2015 "@en ;
.
sto:FileSizeIEC_61810_P2
  a om2:Measure ;
  a owl:NamedIndividual ;
  om2:hasNumericalValue "4364.0"^^xsd:float ;
  om2:hasUnit om2:kilobyte ;
  rdfs:comment "Specifies the file size of the document for standard IEC 61810-2:2017."@en ;
  rdfs:label "FileSize IEC 61810-2:2017"@en ;
.
sto:FileSizeIEC_61810_P7
  a om2:Measure ;
  a owl:NamedIndividual ;
  om2:hasNumericalValue "2204.0"^^xsd:float ;
  om2:hasUnit om2:kilobyte ;
  rdfs:comment "Specifies the file size of the document for standard IEC 61810-7:2006."@en ;
  rdfs:label "FileSize IEC 61810-7:2006"@en ;
.
sto:FileSizeIEC_61850_P10_E1
  a om2:Measure ;
  a owl:NamedIndividual ;
  om2:hasNumericalValue "452.0"^^xsd:float ;
  om2:hasUnit om2:kilobyte ;
  rdfs:comment "Specifies the file size of the document for standard IEC 61850-10:2005 ."@en ;
  rdfs:label "FileSize IEC 61850-10:2005 "@en ;
.
sto:FileSizeIEC_61850_P10_E2
  a om2:Measure ;
  a owl:NamedIndividual ;
  om2:hasNumericalValue "2121.0"^^xsd:float ;
  om2:hasUnit om2:kilobyte ;
  rdfs:comment "Specifies the file size of the document for standard IEC 61850-10:2012."@en ;
  rdfs:label "FileSize IEC 61850-10:2012 "@en ;
.
sto:FileSizeIEC_61850_P4_E1
  a om2:Measure ;
  a owl:NamedIndividual ;
  om2:hasNumericalValue "444.0"^^xsd:float ;
  om2:hasUnit om2:kilobyte ;
  rdfs:comment "Specifies the file size of the document for standard IEC 61850-4:2002 ."@en ;
  rdfs:label "FileSize IEC 61850-4:2002 "@en ;
.
sto:FileSizeIEC_61850_P4_E2
  a om2:Measure ;
  a owl:NamedIndividual ;
  om2:hasNumericalValue "1250.0"^^xsd:float ;
  om2:hasUnit om2:kilobyte ;
  rdfs:comment "Specifies the file size of the document for standard IEC 61850-4:2011 ."@en ;
  rdfs:label "FileSize IEC 61850-4:2011 "@en ;
.
sto:FileSizeIEC_61850_P7_S1_E1
  a om2:Measure ;
  a owl:NamedIndividual ;
  om2:hasNumericalValue "4106.0"^^xsd:float ;
  om2:hasUnit om2:kilobyte ;
  rdfs:comment "Specifies the file size of the document for standard IEC 61850-7-1:2003 ."@en ;
  rdfs:label "FileSize IEC 61850-7-1:2003 "@en ;
.
sto:FileSizeIEC_61850_P7_S1_E2
  a om2:Measure ;
  a owl:NamedIndividual ;
  om2:hasNumericalValue "8338.0"^^xsd:float ;
  om2:hasUnit om2:kilobyte ;
  rdfs:comment "Specifies the file size of the document for standard IEC 61850-7-1:2011 ."@en ;
  rdfs:label "FileSize IEC 61850-7-1:2011 "@en ;
.
sto:FileSizeIEC_61850_P7_S2_E1
  a om2:Measure ;
  a owl:NamedIndividual ;
  om2:hasNumericalValue "3596.0"^^xsd:float ;
  om2:hasUnit om2:kilobyte ;
  rdfs:comment "Specifies the file size of the document for standard IEC 61850-7-2:2003 ."@en ;
  rdfs:label "FileSize IEC 61850-7-2:2003 "@en ;
.
sto:FileSizeIEC_61850_P7_S2_E2
  a om2:Measure ;
  a owl:NamedIndividual ;
  om2:hasNumericalValue "2286.0"^^xsd:float ;
  om2:hasUnit om2:kilobyte ;
  rdfs:comment "Specifies the file size of the document for standard IEC 61850-7-2:2010."@en ;
  rdfs:label "FileSize IEC 61850-7-2:2010 "@en ;
.
sto:FileSizeIEC_61850_P7_S3_E1
  a om2:Measure ;
  a owl:NamedIndividual ;
  om2:hasNumericalValue "3236.0"^^xsd:float ;
  om2:hasUnit om2:kilobyte ;
  rdfs:comment "Specifies the file size of the document for standard IEC 61850-7-3:2003 ."@en ;
  rdfs:label "FileSize IEC 61850-7-3:2003 "@en ;
.
sto:FileSizeIEC_61850_P7_S3_E2
  a om2:Measure ;
  a owl:NamedIndividual ;
  om2:hasNumericalValue "2043.0"^^xsd:float ;
  om2:hasUnit om2:kilobyte ;
  rdfs:comment "Specifies the file size of the document for standard IEC 61850-7-3:2010."@en ;
  rdfs:label "FileSize IEC 61850-7-3:2010 "@en ;
.
sto:FileSizeIEC_61850_P7_S420_E1
  a om2:Measure ;
  a owl:NamedIndividual ;
  om2:hasNumericalValue "2026.0"^^xsd:float ;
  om2:hasUnit om2:kilobyte ;
  rdfs:comment "Specifies the file size of the document for standard IEC 61850-7-420:2009."@en ;
  rdfs:label "FileSize IEC 61850-7-420:2009 "@en ;
.
sto:FileSizeIEC_61850_P7_S4_E1
  a om2:Measure ;
  a owl:NamedIndividual ;
  om2:hasNumericalValue "3475.0"^^xsd:float ;
  om2:hasUnit om2:kilobyte ;
  rdfs:comment "Specifies the file size of the document for standard IEC 61850-7-4:2003 ."@en ;
  rdfs:label "FileSize IEC 61850-7-4:2003 "@en ;
.
sto:FileSizeIEC_61850_P7_S4_E2
  a om2:Measure ;
  a owl:NamedIndividual ;
  om2:hasNumericalValue "4326.0"^^xsd:float ;
  om2:hasUnit om2:kilobyte ;
  rdfs:comment "Specifies the file size of the document for standard IEC 61850-7-4:2010."@en ;
  rdfs:label "FileSize IEC 61850-7-4:2010 "@en ;
.
sto:FileSizeIEC_61968_P3_E1
  a om2:Measure ;
  a owl:NamedIndividual ;
  om2:hasNumericalValue "601.0"^^xsd:float ;
  om2:hasUnit om2:kilobyte ;
  rdfs:comment "Specifies the file size of the document for standard IEC 61968-3:2004 ."@en ;
  rdfs:label "FileSize IEC 61968-3:2004 "@en ;
.
sto:FileSizeIEC_61968_P3_E2
  a om2:Measure ;
  a owl:NamedIndividual ;
  om2:hasNumericalValue "8270.0"^^xsd:float ;
  om2:hasUnit om2:kilobyte ;
  rdfs:comment "Specifies the file size of the document for standard IEC 61968-3:2017."@en ;
  rdfs:label "FileSize IEC 61968-3:2017 "@en ;
.
sto:FileSizeIEC_61968_P4_E1
  a om2:Measure ;
  a owl:NamedIndividual ;
  om2:hasNumericalValue "3106.0"^^xsd:float ;
  om2:hasUnit om2:kilobyte ;
  rdfs:comment "Specifies the file size of the document for standard IEC 61968-4:2007."@en ;
  rdfs:label "FileSize IEC 61968-4:2007 "@en ;
.
sto:FileSizeIEC_61968_P4_E2
  a om2:Measure ;
  a owl:NamedIndividual ;
  om2:hasNumericalValue "8173.0"^^xsd:float ;
  om2:hasUnit om2:kilobyte ;
  rdfs:comment "Specifies the file size of the document for standard IEC 61968-4:2018 PRV."@en ;
  rdfs:label "FileSize IEC 61968-4:2018 PRV "@en ;
.
sto:FileSizeIEC_61968_P6_E1
  a om2:Measure ;
  a owl:NamedIndividual ;
  om2:hasNumericalValue "4059.0"^^xsd:float ;
  om2:hasUnit om2:kilobyte ;
  rdfs:comment "Specifies the file size of the document for standard IEC 61968-6:2015."@en ;
  rdfs:label "FileSize IEC 61968-6:2015 "@en ;
.
sto:FileSizeIEC_61968_P8_E1
  a om2:Measure ;
  a owl:NamedIndividual ;
  om2:hasNumericalValue "2555.0"^^xsd:float ;
  om2:hasUnit om2:kilobyte ;
  rdfs:comment "Specifies the file size of the document for standard IEC 61968-8:2015 ."@en ;
  rdfs:label "FileSize IEC 61968-8:2015  "@en ;
.
sto:FileSizeIEC_61968_P9_E1
  a om2:Measure ;
  a owl:NamedIndividual ;
  om2:hasNumericalValue "2745.0"^^xsd:float ;
  om2:hasUnit om2:kilobyte ;
  rdfs:comment "Specifies the file size of the document for standard IEC 61968-9:2009."@en ;
  rdfs:label "FileSize IEC 61968-9:2009 "@en ;
.
sto:FileSizeIEC_61968_P9_E2
  a om2:Measure ;
  a owl:NamedIndividual ;
  om2:hasNumericalValue "6943.0"^^xsd:float ;
  om2:hasUnit om2:kilobyte ;
  rdfs:comment "Specifies the file size of the document for standard IEC 61968-9:2013."@en ;
  rdfs:label "FileSize IEC 61968-9:2013 "@en ;
.
sto:FileSizeIEC_61970_P1_E1
  a om2:Measure ;
  a owl:NamedIndividual ;
  om2:hasNumericalValue "707.0"^^xsd:float ;
  om2:hasUnit om2:kilobyte ;
  rdfs:comment "Specifies the file size of the document for standard IEC 61970-1:2005 ."@en ;
  rdfs:label "FileSize IEC 61970-1:2005  "@en ;
.
sto:FileSizeIEC_61970_P301_E1
  a om2:Measure ;
  a owl:NamedIndividual ;
  om2:hasNumericalValue "2709.0"^^xsd:float ;
  om2:hasUnit om2:kilobyte ;
  rdfs:comment "Specifies the file size of the document for standard IEC 61970-301:2003."@en ;
  rdfs:label "FileSize IEC 61970-301:2003 "@en ;
.
sto:FileSizeIEC_61970_P301_E2
  a om2:Measure ;
  a owl:NamedIndividual ;
  om2:hasNumericalValue "2348.0"^^xsd:float ;
  om2:hasUnit om2:kilobyte ;
  rdfs:comment "Specifies the file size of the document for standard IEC 61970-301:2009."@en ;
  rdfs:label "FileSize IEC 61970-301:2009 "@en ;
.
sto:FileSizeIEC_61970_P301_E3
  a om2:Measure ;
  a owl:NamedIndividual ;
  om2:hasNumericalValue "4841.0"^^xsd:float ;
  om2:hasUnit om2:kilobyte ;
  rdfs:comment "Specifies the file size of the document for standard IEC 61970-301:2011."@en ;
  rdfs:label "FileSize IEC 61970-301:2011 "@en ;
.
sto:FileSizeIEC_61970_P301_E4
  a om2:Measure ;
  a owl:NamedIndividual ;
  om2:hasNumericalValue "5466.0"^^xsd:float ;
  om2:hasUnit om2:kilobyte ;
  rdfs:comment "Specifies the file size of the document for standard IEC 61970-301:2013."@en ;
  rdfs:label "FileSize IEC 61970-301:2013 "@en ;
.
sto:FileSizeIEC_61970_P301_E5
  a om2:Measure ;
  a owl:NamedIndividual ;
  om2:hasNumericalValue "8022.0"^^xsd:float ;
  om2:hasUnit om2:kilobyte ;
  rdfs:comment "Specifies the file size of the document for standard IEC 61970-301:2013."@en ;
  rdfs:label "FileSize IEC 61970-301:2013 "@en ;
.
sto:FileSizeIEC_61970_P301_E6
  a om2:Measure ;
  a owl:NamedIndividual ;
  om2:hasNumericalValue "17830.0"^^xsd:float ;
  om2:hasUnit om2:kilobyte ;
  rdfs:comment "Specifies the file size of the document for standard IEC 61970-301:2016."@en ;
  rdfs:label "FileSize IEC 61970-301:2016 "@en ;
.
sto:FileSizeIEC_61970_P301_E6_RLV
  a om2:Measure ;
  a owl:NamedIndividual ;
  om2:hasNumericalValue "24554.0"^^xsd:float ;
  om2:hasUnit om2:kilobyte ;
  rdfs:comment "Specifies the file size of the document for standard IEC 61970-301:2016 RLV Redline version."@en ;
  rdfs:label "FileSize IEC 61970-301:2016 RLV Redline version "@en ;
.
sto:FileSizeIEC_61970_P452_E1
  a om2:Measure ;
  a owl:NamedIndividual ;
  om2:hasNumericalValue "2015.0"^^xsd:float ;
  om2:hasUnit om2:kilobyte ;
  rdfs:comment "Specifies the file size of the document for standard IEC 61970-452:2013."@en ;
  rdfs:label "FileSize IEC 61970-452:2013 "@en ;
.
sto:FileSizeIEC_61970_P452_E2
  a om2:Measure ;
  a owl:NamedIndividual ;
  om2:hasNumericalValue "2238.0"^^xsd:float ;
  om2:hasUnit om2:kilobyte ;
  rdfs:comment "Specifies the file size of the document for standard IEC 61970-452:2015."@en ;
  rdfs:label "FileSize IEC 61970-452:2015 "@en ;
.
sto:FileSizeIEC_61970_P452_E3
  a om2:Measure ;
  a owl:NamedIndividual ;
  om2:hasNumericalValue "1533.0"^^xsd:float ;
  om2:hasNumericalValue "4157.0"^^xsd:float ;
  om2:hasUnit om2:kilobyte ;
  rdfs:comment "Specifies the file size of the document for standard IEC 61970-452:2017."@en ;
  rdfs:comment "Specifies the file size of the document for standard IEC IEC PAS 62264-6:2016."@en ;
  rdfs:label "FileSize IEC 61970-452:2017 "@en ;
  rdfs:label "FileSize IEC PAS 62264-6:2016 "@en ;
.
sto:FileSizeIEC_62769_P1
  a om2:Measure ;
  a owl:NamedIndividual ;
  om2:hasNumericalValue "1259.0"^^xsd:float ;
  om2:hasUnit om2:kilobyte ;
  rdfs:comment "Specifies the file size of the document for standard IECIEC 62769-1:2015 "@en ;
  rdfs:label "FileSize IEC 62769-1:2015   "@en ;
.
sto:FileSizeIEC_62832
  a om2:Measure ;
  a owl:NamedIndividual ;
  om2:hasNumericalValue "2722.0"^^xsd:float ;
  om2:hasUnit om2:kilobyte ;
.
sto:Final_architectural_reference_model_for_the_IoT_v3_0
  a <https://www.w3.org/ns/oaSpecificResource> ;
  rdfs:label "Internet of Things – Architecture IoT-A Final architectural reference model for the IoT v3.0"@en ;
  skos:note "Internet of Things – Architecture IoT-A Deliverable D1.5 – Final architectural reference model for the IoT v3.0" ;
  sto:hasOpenResource <http://cocoa.ethz.ch/downloads/2014/01/1360_D1%202_Initial_architectural_reference_model_for_IoT.pdf> ;
.
sto:FiwareAdvancedUi
  a owl:NamedIndividual ;
  a sto:FiwareChapter ;
  a sto:StandardClassification ;
  terms:creator sto:sebastian ;
  dul:associatedWith <http://purl.oclc.org/NET/mvco.owl#EndUser> ;
  dul:associatedWith sto:IIRAApplicationDomain ;
  dul:associatedWith sto:IIRAUsageViewpoint ;
  rdfs:comment """The Generic Enablers (GEs) from the Advanced Web-based User Interface (WebUI) chapter cover a set of GEs that provide an advanced user experience using HTML-5 and a Web-based UI approach.

The objective of the Advanced Web-based UI GE is to significantly improve the user experience for the Future Internet by adding new user input and interaction capabilities, such as interactive 3D graphics, immersive interaction with the real and virtual world via Augmented Reality, virtualizing the display and driving them over the network, and many more."""@en ;
  rdfs:label "FIWARE Advanced Web-based User Interface"@en ;
  sto:alignsWith sto:IIRAApplicationDomain ;
  sto:alignsWith sto:IIRAUsageViewpoint ;
  sto:frames sto:UserInteraction ;
  sto:isDescribedin sto:FIWARE ;
.
sto:FiwareAdvancedUiAnno
  a <https://www.w3.org/ns/oaAnnotation> ;
  <https://www.w3.org/ns/oahasBody> sto:FiwareAdvancedUi ;
  <https://www.w3.org/ns/oahasTarget> [
      a <https://www.w3.org/ns/oaSpecificResource> ;
      <https://www.w3.org/ns/oahasSource> <https://forge.fiware.org/plugins/mediawiki/wiki/fiware/index.php/Advanced_Middleware_and_Web_UI_Architecture> ;
    ] ;
.
sto:FiwareApplicationsServicesAndDataDelivery
  a owl:NamedIndividual ;
  a sto:FiwareChapter ;
  a sto:StandardClassification ;
  terms:creator sto:sebastian ;
  dul:associatedWith sto:IDSRAMProcessLayer ;
  dul:associatedWith sto:IIRAConnectivity ;
  dul:associatedWith sto:NgsiLdArchitecture ;
  rdfs:comment """The Generic Enablers (GE) for the Apps Chapter together build an ecosystem of applications, services and data that is sustainable and fosters innovation as well as cross-fertilization. In particular the Apps Generic Enablers supports managing applications, services and data in a business framework across the whole service life cycle from creation through composition of applications and data to monetization and revenue sharing.

A couple of basic GEs are important to realize the vision of such an applications, services and data business framework, which enables new business models in an agile and flexible way. Among them: a store, a marketplace, a revenue sharing engine, an application composer through mashup and a data visualization and analysis component.

The Business Framework is heavily relying on USDL as common uniform description format for services which does not only focus on technical aspects of service, but also on business aspects as well as functional and non-functional service attributes.

The Application Mashup GE aims at allowing end users without programming skills to quickly compose beautiful web applications and dashboards/cockpits mashing up widgets, operators and data sources from a shared catalogue.

The Data Visualisation GE aims at creating agile, beautiful visualizations and meaningful reports useful to present the large variety of datasets. Data stakeholders will bring in the play as well as providing customisable data analytics."""@en ;
  rdfs:label "FIWARE Applications Services and Data Delivery"@en ;
  sto:alignsWith sto:IDSRAMProcessLayer ;
  sto:alignsWith sto:IIRAConnectivity ;
  sto:alignsWith sto:NgsiLdArchitecture ;
  sto:frames sto:DataAnalytics ;
  sto:frames sto:DataSelection ;
  sto:frames sto:ServiceComposition ;
  sto:frames sto:ServiceSelection ;
  sto:isDescribedin sto:FIWARE ;
.
sto:FiwareApplicationsServicesAndDataDeliveryAnno
  a <https://www.w3.org/ns/oaAnnotation> ;
  <https://www.w3.org/ns/oahasBody> sto:FiwareApplicationsServicesAndDataDelivery ;
  <https://www.w3.org/ns/oahasTarget> [
      a <https://www.w3.org/ns/oaSpecificResource> ;
      <https://www.w3.org/ns/oahasSource> <https://forge.fiware.org/plugins/mediawiki/wiki/fiware/index.php/Architecture_of_Applications,_Services_and_Data_Delivery_R3> ;
    ] ;
.
sto:FiwareChapter
  a owl:Class ;
  a owl:NamedIndividual ;
  terms:creator sto:sebastian ;
  terms:creator "sebastian"@en ;
  rdfs:comment "Following is a description of the Reference Architecture linked to the different chapters of FIWARE. A description of FIWARE Generic Enablers (GEs) being supported in each chapter is provided, including the high-level description of the APIs that each FIWARE Generic Enabler (GE) exposes to application developers or it uses to connect to another FIWARE GEs."@en ;
  rdfs:label "Fiware Chapter"@en ;
  rdfs:subClassOf sto:StandardClassification ;
.
sto:FiwareChapterAnno
  a <https://www.w3.org/ns/oaAnnotation> ;
  <https://www.w3.org/ns/oahasBody> sto:FiwareChapter ;
  <https://www.w3.org/ns/oahasTarget> [
      a <https://www.w3.org/ns/oaSpecificResource> ;
      <https://www.w3.org/ns/oahasSource> <https://forge.fiware.org/plugins/mediawiki/wiki/fiware/index.php/Summary_of_FI-WARE_Open_Specifications> ;
    ] ;
.
sto:FiwareCloudHosting
  a owl:NamedIndividual ;
  a sto:FiwareChapter ;
  a sto:StandardClassification ;
  terms:creator sto:sebastian ;
  dul:associatedWith sto:IDSRAMSystemLayer ;
  dul:associatedWith sto:IIRAApplicationDomain ;
  dul:associatedWith sto:IIRADistributedDataManagement ;
  dul:associatedWith sto:IIRAScalability ;
  dul:associatedWith sto:NgsiLdArchitecture ;
  rdfs:comment """The Cloud Chapter offers Generic Enablers (GEs) that comprise the foundation for designing a modern cloud hosting infrastructure that can be used to develop, deploy and manage Future Internet applications and services. Provided hosting capabilities are of several kinds and at several levels of resource abstraction -- aiming at the needs of different applications hosted on the cloud.

The IaaS Data Center Resource Management (DCRM) GE is offering provisioning and life cycle management of virtualized resources (compute, storage, network) associated with virtual machines. The Object Storage GE offers provisioning and life cycle management of object-based storage containers and elements. The Job Scheduler GE offers the application to submit and manage computational jobs in a unified and scalable manner. The Edgelet Management GE offers the capability to host lightweight application components, called edgelets. Moreover, the IaaS Service Management (SM) GE provides the means to host complex applications. Lastly, the PaaS Management GE uses the above capabilities to offer provisioning and management of complete PaaS environments, leveraging also the Software Deployment and Configuration (SDC) GE which offers a flexible framework for installation and customization of software products (via Chef recipes) within individual virtual machines."""@en ;
  rdfs:label "FIWARE Cloud Hosting"@en ;
  sto:alignsWith sto:IDSRAMSystemLayer ;
  sto:alignsWith sto:IIRAApplicationDomain ;
  sto:alignsWith sto:IIRADistributedDataManagement ;
  sto:alignsWith sto:IIRAScalability ;
  sto:alignsWith sto:NgsiLdArchitecture ;
  sto:frames sto:Availability ;
  sto:frames sto:CloudComputing ;
  sto:frames sto:DataProcessing ;
  sto:frames sto:DataSovereignty ;
  sto:frames sto:IntegrityProtection ;
  sto:frames sto:Privacy ;
  sto:frames sto:Reliability ;
  sto:frames sto:Safety ;
  sto:frames sto:Security ;
  sto:frames sto:ServiceComposition ;
  sto:frames sto:ServiceDeployment ;
  sto:frames sto:ServiceLifecycleManagement ;
  sto:frames sto:ServiceOrchestration ;
  sto:frames sto:Trustworthiness ;
  sto:isDescribedin sto:FIWARE ;
.
sto:FiwareCloudHostingAnno
  a <https://www.w3.org/ns/oaAnnotation> ;
  <https://www.w3.org/ns/oahasBody> sto:FiwareCloudHosting ;
  <https://www.w3.org/ns/oahasTarget> [
      a <https://www.w3.org/ns/oaSpecificResource> ;
      <https://www.w3.org/ns/oahasSource> <https://forge.fiware.org/plugins/mediawiki/wiki/fiware/index.php/Cloud_Hosting_Architecture_R3> ;
    ] ;
.
sto:FiwareDataContextManagement
  a owl:NamedIndividual ;
  a sto:FiwareChapter ;
  a sto:StandardClassification ;
  terms:creator sto:sebastian ;
  dul:associatedWith sto:NgsiLdApiOperation ;
  dul:associatedWith sto:NgsiLdDataRepresentation ;
  dul:associatedWith sto:NgsiLdInformationModel ;
  rdfs:comment """The Data/Context Management FIWARE chapter aims at providing outperforming and platform-like GEs that will ease development and provision of innovative Applications that require gathering, publication, processing and exploitation of information and data streams in real-time and at massive scale. Combined with GEs coming from the Apps Chapters, Application Providers will be able to build innovative business models based on exploitation of massive data provided by end users.

FIWARE Data/Context Management GEs allow to gather information from context and other sources (Context Broker), mediate metadata among GEs and applications (Metadata pre-processor) query stored information through an homogeneous layer (Query Broker), , annotate existing information (Semantic Annotation), store and manage semantic information (Semantic Application Support), generate new knowledge from big data stores using a Map & Reduce paradigm (Big Data analysis) and react to different types of scenarios (Complex Event Processing). It also provides GEs for media management, as easy creation of advanced video applications (Stream Oriented GE) and specifically, video analysis in the compressed domain (CDVA)."""@en ;
  rdfs:label "FIWARE Data/Context Management"@en ;
  sto:alignsWith sto:NgsiLdApiOperation ;
  sto:alignsWith sto:NgsiLdDataRepresentation ;
  sto:alignsWith sto:NgsiLdInformationModel ;
  sto:frames sto:BigDataApplications ;
  sto:frames sto:DataDiscovery ;
  sto:frames sto:DataProcessing ;
  sto:frames sto:Interoperability ;
  sto:frames sto:StreamProcessing ;
  sto:isDescribedin sto:FIWARE ;
.
sto:FiwareDataContextManagementAnno
  a <https://www.w3.org/ns/oaAnnotation> ;
  <https://www.w3.org/ns/oahasBody> sto:FiwareDataContextManagement ;
  <https://www.w3.org/ns/oahasTarget> [
      a <https://www.w3.org/ns/oaSpecificResource> ;
      <https://www.w3.org/ns/oahasSource> <https://forge.fiware.org/plugins/mediawiki/wiki/fiware/index.php/Data/Context_Management_Architecture_R3> ;
    ] ;
.
sto:FiwareIotServicesEnablement
  a owl:NamedIndividual ;
  a sto:FiwareChapter ;
  a sto:StandardClassification ;
  terms:creator sto:sebastian ;
  dul:associatedWith sto:IDSRAMSystemLayer ;
  dul:associatedWith sto:IIRAControlDomain ;
  dul:associatedWith sto:RAMICommunicationlayer ;
  dul:associatedWith sto:RAMIIntegrationLayer ;
  rdfs:comment """The deployment of the architecture of the IoT Service Enablement chapter is typically distributed across a large number of Devices, several Gateways and the Backend.

A device is a hardware entity, component or system that either measures properties of a thing/group of things or influences the properties of a thing/group of things or both measures/influences. Sensors and actuators are devices.

IoT Resources are computational elements (software) that provide the technical means to perform sensing and/or actuation on the device. The resource is usually hosted on the device.

IoT GEs have been spread in two different domains: Gateway and Backend. While IoT Gateway GEs provide inter-networking and protocol conversion functionalities between devices and the IoT Backend GEs, the IoT Backend GEs provide management functionalities for the devices and IoT domain-specific support for the applications."""@en ;
  rdfs:label "FIWARE IoT Services Enablement"@en ;
  sto:alignsWith sto:IDSRAMSystemLayer ;
  sto:alignsWith sto:IIRAControlDomain ;
  sto:alignsWith sto:RAMICommunicationlayer ;
  sto:alignsWith sto:RAMIIntegrationLayer ;
  sto:frames sto:CloudComputing ;
  sto:frames sto:DataDiscovery ;
  sto:frames sto:DataProcessing ;
  sto:frames sto:EdgeComputing ;
  sto:frames sto:EndpointInvocation ;
  sto:frames sto:Interoperability ;
  sto:frames sto:IoT ;
  sto:frames sto:SyntacticInteroperability ;
  sto:isDescribedin sto:FIWARE ;
.
sto:FiwareIotServicesEnablementAnno
  a <https://www.w3.org/ns/oaAnnotation> ;
  <https://www.w3.org/ns/oahasBody> sto:FiwareIotServicesEnablement ;
  <https://www.w3.org/ns/oahasTarget> [
      a <https://www.w3.org/ns/oaSpecificResource> ;
      <https://www.w3.org/ns/oahasSource> <https://forge.fiware.org/plugins/mediawiki/wiki/fiware/index.php/Internet_of_Things_(IoT)_Services_Enablement_Architecture_R3> ;
    ] ;
.
sto:FiwareSecurity
  a owl:NamedIndividual ;
  a sto:FiwareChapter ;
  a sto:StandardClassification ;
  terms:creator sto:sebastian ;
  dul:associatedWith rami:Security ;
  dul:associatedWith sto:IDSRAMSecurity ;
  dul:associatedWith sto:IIRASecurity ;
  dul:associatedWith sto:XACML ;
  rdfs:comment """The Future Internet services will always be exposed to different types of threats that can lead to severe misuse and damage. Creating secured and trusted services without sacrificing much of the desired functionality, usability, performance and cost efficiency is a great challenge, especially in a dynamic environment where new threats and attack methods emerge on a daily basis.

The overall ambition of the Security Architecture of FIWARE is to demonstrate that the Vision of an Internet that is \"secure by design\" is becoming reality. Based on achievements to date and/or to come in the short-term (both from a technological but also a standardization perspective) we will show that \"secure by design\" is possible.

Security, Privacy and Trust in FIWARE is mainly focusing on delivering tools and techniques to have the above-mentioned security needs properly met. Furthermore a decision making support and the automation of countermeasures allow alleviating the workload of users and administrators while raising their security awareness.

The high-level Reference Architecture is formed by four main blocks of GEs: Cybersecurity, Identity and Access Management (and Enforcement), Privacy, Trust and Trustworthiness."""@en ;
  rdfs:label "FIWARE Security"@en ;
  sto:alignsWith rami:Security ;
  sto:alignsWith sto:IDSRAMSecurity ;
  sto:alignsWith sto:IIRASecurity ;
  sto:frames sto:Authentication ;
  sto:frames sto:Authorization ;
  sto:frames sto:DataAccessControl ;
  sto:frames sto:DataSovereignty ;
  sto:frames sto:IdentityManagement ;
  sto:frames sto:Privacy ;
  sto:frames sto:Security ;
  sto:frames sto:Trustworthiness ;
  sto:isDescribedin sto:FIWARE ;
.
sto:FiwareSecurityAnno
  a <https://www.w3.org/ns/oaAnnotation> ;
  <https://www.w3.org/ns/oahasBody> sto:FiwareSecurity ;
  <https://www.w3.org/ns/oahasTarget> [
      a <https://www.w3.org/ns/oaSpecificResource> ;
      <https://www.w3.org/ns/oahasSource> <https://forge.fiware.org/plugins/mediawiki/wiki/fiware/index.php/Security_Architecture_R3> ;
    ] ;
.
sto:FunctionalSafety
  a owl:NamedIndividual ;
  a sto:Domain ;
  rdfs:comment "Functional Safety"@en ;
  rdfs:label "Functional Safety"@en ;
.
sto:GPLv2
  a terms:LicenseDocument ;
  a owl:NamedIndividual ;
  rdfs:comment "Published under Open Content License."@en ;
  rdfs:label "GNU General Public License"@en ;
  rdfs:seeAlso <https://opcfoundation.org/license/gpl.htm> ;
  skos:prefLabel "OCL 1.0" ;
.
sto:GeoTracking
  a owl:NamedIndividual ;
  a sto:Concern ;
  <http://voag.linkedmodel.org/voag#hasStakeholder> <http://purl.oclc.org/NET/mvco.owl#EndUser> ;
  rdfs:comment "A system built using the ARM shall support physical entity location tracking (geo spatial and/or logical location)"@en ;
  rdfs:label "Geo tracking"@en ;
  rdfs:seeAlso "IoT-A Requirement UNI.016" ;
  sto:hasDBpediaResource <http://dbpedia.org/resource/Track_and_trace> ;
  sto:supports sto:ContextAwareness ;
.
sto:GeospatialData
  a owl:NamedIndividual ;
  a sto:Concern ;
  rdfs:comment "Discovery and lookup services of the system shall allow locating physical entities based on geographical parameters."@en ;
  rdfs:label "Geospatial data and information"@en ;
  rdfs:seeAlso "IoT-A Requirement UNI.402" ;
  rdfs:seeAlso "IoT-A Requirement UNI.403" ;
  rdfs:seeAlso "IoT-A Requirement UNI.404" ;
  rdfs:seeAlso "IoT-A Requirement UNI.405" ;
  rdfs:seeAlso "IoT-A Requirement UNI.406" ;
  rdfs:seeAlso "IoT-A Requirement UNI.415" ;
  rdfs:seeAlso "IoT-A Requirement UNI.420" ;
  rdfs:seeAlso "IoT-A Requirement UNI.421" ;
  rdfs:seeAlso "UNI.401"@en ;
  rdfs:seeAlso "UNI.402"@en ;
  rdfs:seeAlso "UNI.403"@en ;
  rdfs:seeAlso "UNI.404"@en ;
  sto:hasDBpediaResource <http://dbpedia.org/resource/Geographic_data_and_information> ;
  sto:supports sto:DataAnalytics ;
.
sto:GeospatialQuery
  rdfs:seeAlso "IoT-A Requirement UNI.401" ;
.
sto:Governance
  a owl:NamedIndividual ;
  a sto:Concern ;
  sto:supports sto:BusinessContext ;
.
sto:Greening_of_IoT
  a owl:NamedIndividual ;
  a sto:Concern ;
  terms:creator sto:MuhammadUsman ;
  rdfs:comment """The system energy consumption is expanding at a high rate because of increment in information rates, an increment in quantity of Internet-empowered services
and fast development of Internet associated edgedevices. The future IoT will cause a critical increase in the network energy consumption."""@en ;
  rdfs:label "Greening of IoT"@en ;
  rdfs:seeAlso "https://ieeexplore.ieee.org/document/6188257"@en ;
  sto:hasWikipediaArticle "https://en.wikipedia.org/wiki/Green_computing"@en ;
  sto:supports sto:EnergyControl ;
.
sto:HTML
  a owl:NamedIndividual ;
  a foaf:Document ;
  a sto:Publication ;
  a sto:TechnicalSpecification ;
  terms:creator sto:IETF ;
  rdfs:label "HTML"@en ;
  foaf:maker sto:IETF ;
  sto:hasDeveloper sto:IETF ;
  sto:hasPublisher sto:IETF ;
.
sto:HTTP
  a owl:NamedIndividual ;
  a foaf:Document ;
  a sto:Publication ;
  a sto:TechnicalSpecification ;
  terms:creator sto:IETF ;
  terms:creator sto:sebastian ;
  rdfs:comment "HTTP is the most widely used protocol for internet communication."@en ;
  rdfs:label "HTTP"@en ;
  foaf:maker sto:IETF ;
  sto:hasDBpediaResource <http://dbpedia.org/resource/Hypertext_Transfer_Protocol> ;
  sto:hasDeveloper sto:IETF ;
  sto:hasOfficialResource <https://tools.ietf.org/html/rfc7230> ;
  sto:hasOfficialResource <https://tools.ietf.org/html/rfc7231> ;
  sto:hasOfficialResource <https://tools.ietf.org/html/rfc7232> ;
  sto:hasOfficialResource <https://tools.ietf.org/html/rfc7233> ;
  sto:hasOfficialResource <https://tools.ietf.org/html/rfc7234> ;
  sto:hasOfficialResource <https://tools.ietf.org/html/rfc7235> ;
  sto:hasPublisher sto:IETF ;
  sto:hasWikipediaArticle <https://en.wikipedia.org/wiki/Hypertext_Transfer_Protocol> ;
.
sto:HTTP2
  a owl:NamedIndividual ;
  a foaf:Document ;
  a sto:Publication ;
  a sto:TechnicalSpecification ;
  terms:creator sto:IETF ;
  terms:creator sto:sebastian ;
  rdfs:comment "HTTP/2 - Enables a more efficient use of network resources and a reduced perception of latency by introducing header field compression and allowing multiple concurrent exchanges on the same connection. (source: https://www.postscapes.com/internet-of-things-protocols/)"@en ;
  rdfs:label "HTTP/2"@en ;
  foaf:maker sto:IETF ;
  sto:hasDeveloper sto:IETF ;
  sto:hasOfficialResource <http://httpwg.org/specs/rfc7540.html> ;
  sto:hasPublisher sto:IETF ;
.
sto:HyperCat
  a owl:NamedIndividual ;
  a foaf:Document ;
  a sto:Publication ;
  a sto:TechnicalSpecification ;
  terms:creator sto:sebastian ;
  rdfs:comment "HyperCat - An open, lightweight JSON-based hypermedia catalogue format for exposing collections of URIs. (source: https://www.postscapes.com/internet-of-things-protocols/)"@en ;
  rdfs:label "HyperCat"@en ;
  sto:hasOfficialResource <http://www.hypercat.io/standard.html> ;
.
sto:IBM
  a owl:NamedIndividual ;
  a foaf:Organization ;
  a sto:StandardOrganization ;
  rdfs:comment "International Business Machines Corporation (commonly referred to as IBM) is an American multinational technology and consulting corporation, with corporate headquarters in Armonk, New York. IBM manufactures and markets computer hardware, middleware and software, and offers infrastructure, hosting and consulting services in areas ranging from mainframe computers to nanotechnology.On August 6, 2015, IBM announced that it will buy Merge Healthcare Inc for $1 billion." ;
  sto:abbreviation "IBM" ;
  sto:formationDate "1911-06-16"^^xsd:date ;
  sto:hasDBpediaResource <http://dbpedia.org/resource/IBM> ;
  sto:hasHeadquaterIn dbr:_New_York ;
  sto:hasOfficialResource <http://www.ibm.com> ;
  sto:hasWikipediaArticle <https://en.wikipedia.org/wiki/IBM> ;
  sto:orgName "International Business Machines Corporation"@en ;
.
sto:ICS_01_040_07
  a owl:NamedIndividual ;
  a sto:InternationalClassificationForStandards ;
  terms:title "Natural and applied sciences (Vocabularies)"@en ;
  rdfs:comment "This is ICS for Natural and applied sciences (Vocabularies)"@en ;
  rdfs:label "ICS 01.040.07"@en ;
.
sto:ICS_01_040_35
  a owl:NamedIndividual ;
  a sto:InternationalClassificationForStandards ;
  terms:title " Information technology. Office machines (Vocabularies)"@en ;
  rdfs:comment "This is ICS for  Information technology. Office machines (Vocabularies)"@en ;
  rdfs:label "ICS 01.040.35"@en ;
.
sto:ICS_01_060
  a owl:NamedIndividual ;
  a sto:InternationalClassificationForStandards ;
  terms:title "Quantities and units "@en ;
  rdfs:comment "This is ICS for Quantities and units"@en ;
  rdfs:label "ICS 01.060"@en ;
.
sto:ICS_01_070
  a owl:NamedIndividual ;
  a sto:InternationalClassificationForStandards ;
  terms:title "Colour coding  "@en ;
  rdfs:comment "This is ICS for Colour coding "@en ;
  rdfs:label "ICS 01.070"@en ;
.
sto:ICS_03_100_40
  a owl:NamedIndividual ;
  a sto:InternationalClassificationForStandards ;
  terms:title "Research and development"@en ;
  rdfs:comment "This is ICS for “Research and development  ”"@en ;
  rdfs:label "ICS 03.100.40"@en ;
.
sto:ICS_03_120_01
  a owl:NamedIndividual ;
  a sto:InternationalClassificationForStandards ;
  terms:title "Quality in general "@en ;
  rdfs:comment "This is ICS for “Quality in general  ”"@en ;
  rdfs:label "ICS 03.120.01"@en ;
.
sto:ICS_13_110
  a owl:NamedIndividual ;
  a sto:InternationalClassificationForStandards ;
  terms:title "Safety of machinery"@en ;
  rdfs:comment "This is ICS for Safety of machinery "@en ;
  rdfs:label "ICS 13.110"@en ;
.
sto:ICS_13_320
  a owl:NamedIndividual ;
  a sto:InternationalClassificationForStandards ;
  terms:title "Alarm and warning systems"@en ;
  rdfs:comment "This is ICS for Alarm and warning systems"@en ;
  rdfs:label "ICS 13.320"@en ;
.
sto:ICS_17_020
  a owl:NamedIndividual ;
  a sto:InternationalClassificationForStandards ;
  terms:title "Metrology and measurement in general "@en ;
  rdfs:comment "This is ICS for “Metrology and measurement in general ”"@en ;
  rdfs:label "ICS 17.020"@en ;
.
sto:ICS_19_020
  a owl:NamedIndividual ;
  a sto:InternationalClassificationForStandards ;
  terms:title "Test conditions and procedures in general"@en ;
  rdfs:comment "This is ICS for “Test conditions and procedures in general"@en ;
  rdfs:label "ICS 19.020"@en ;
.
sto:ICS_19_08
  a owl:NamedIndividual ;
  a sto:InternationalClassificationForStandards ;
  terms:title "Electrical and electronic testing"@en ;
  rdfs:comment "This is ICS for “Electrical and electronic testing”"@en ;
  rdfs:label "ICS 19.08"@en ;
.
sto:ICS_25_040_01
  a owl:NamedIndividual ;
  a sto:InternationalClassificationForStandards ;
  terms:title "Industrial automation systems in general"@en ;
  rdfs:comment "This is ICS for Industrial automation systems in general"@en ;
  rdfs:label "ICS 25.040.01"@en ;
.
sto:ICS_25_040_40
  a owl:NamedIndividual ;
  a sto:InternationalClassificationForStandards ;
  terms:title "Industrial process measurement and control"@en ;
  rdfs:comment "This is ICS for industrial process measurement and control"@en ;
  rdfs:label "ICS 25.040.40"@en ;
.
sto:ICS_27_180
  a owl:NamedIndividual ;
  a sto:InternationalClassificationForStandards ;
  terms:title "Wind turbine energy systems"@en ;
  rdfs:comment "This is ICS for “Wind turbine energy systems”"@en ;
  rdfs:label "ICS 27.180"@en ;
.
sto:ICS_29_020
  a owl:NamedIndividual ;
  a sto:InternationalClassificationForStandards ;
  terms:title "Electrical engineering in general "@en ;
  rdfs:comment "This is ICS for Electrical engineering in general"@en ;
  rdfs:label "ICS 29.020"@en ;
.
sto:ICS_29_120_70
  a owl:NamedIndividual ;
  a sto:InternationalClassificationForStandards ;
  terms:title "Relays"@en ;
  rdfs:comment "This is ICS for Relays"@en ;
  rdfs:comment "This is ICS for “Relays”"@en ;
  rdfs:label "ICS 29.120.70"@en ;
.
sto:ICS_29_240_20
  a owl:NamedIndividual ;
  a sto:InternationalClassificationForStandards ;
  terms:title "Power transmission and distribution lines"@en ;
  rdfs:comment "This is ICS for “Power transmission and distribution lines”"@en ;
  rdfs:label "ICS 29.240.20"@en ;
.
sto:ICS_31_020
  a owl:NamedIndividual ;
  a sto:InternationalClassificationForStandards ;
  terms:title "Electronic components in general "@en ;
  rdfs:comment "This is ICS for Electronic components in general "@en ;
  rdfs:label "ICS 31.020"@en ;
.
sto:ICS_31_240
  a owl:NamedIndividual ;
  a sto:InternationalClassificationForStandards ;
  terms:title "Mechanical structures for electronic equipment"@en ;
  rdfs:comment "This is ICS for  Mechanical structures for electronic equipment"@en ;
  rdfs:label "ICS 31.240"@en ;
.
sto:ICS_33_040_40
  a owl:NamedIndividual ;
  a sto:InternationalClassificationForStandards ;
  terms:title "Data communication networks "@en ;
  rdfs:comment "This is ICS for “Data communication networks”"@en ;
  rdfs:label "ICS 33.040.40"@en ;
.
sto:ICS_33_060_20
  a owl:NamedIndividual ;
  a sto:InternationalClassificationForStandards ;
  terms:title "Receiving and transmitting equipment"@en ;
  rdfs:comment "This is ICS for Receiving and transmitting equipment"@en ;
  rdfs:label "ICS 33.060.20"@en ;
.
sto:ICS_33_100_10
  a owl:NamedIndividual ;
  a sto:InternationalClassificationForStandards ;
  terms:title "Emission"@en ;
  rdfs:comment "This is ICS for “Emission”"@en ;
  rdfs:label "ICS 33.100.10"@en ;
.
sto:ICS_33_100_20
  a owl:NamedIndividual ;
  a sto:InternationalClassificationForStandards ;
  terms:title "Immunity"@en ;
  rdfs:comment "This is ICS for “Immunity”"@en ;
  rdfs:label "ICS 33.100.20"@en ;
.
sto:ICS_33_200
  a owl:NamedIndividual ;
  a sto:InternationalClassificationForStandards ;
  terms:title "Telecontrol. Telemetering Including Supervising, Control and Data Acquisition System (SCADA)"@en ;
  rdfs:comment "This is ICS for Telecontrol. Telemetering Including Supervising, Control and Data Acquisition System (SCADA)"@en ;
  rdfs:label "ICS 33.200"@en ;
.
sto:ICS_35_060
  a owl:NamedIndividual ;
  a sto:InternationalClassificationForStandards ;
  terms:title "Languages used in information technology"@en ;
  rdfs:comment "This is ICS for “Languages used in information technology”"@en ;
  rdfs:label "ICS 35.060"@en ;
.
sto:ICS_35_240_50
  a owl:NamedIndividual ;
  a sto:InternationalClassificationForStandards ;
  terms:title "IT applications in industry"@en ;
  rdfs:comment "This is ICS for IT applications in industry"@en ;
  rdfs:comment "This is ICS for “IT applications in industry)”"@en ;
  rdfs:label "ICS 35.240.50"@en ;
.
sto:ID4me
  a owl:NamedIndividual ;
  a foaf:Document ;
  a sto:Publication ;
  a sto:TechnicalSpecification ;
  terms:creator sto:sebastian ;
  terms:creator "sebastian" ;
  rdfs:comment "ID4me is a federated digital identity service that aims to provide two main functions: (1) Authorization of a user for access to any third party accepting ID4me identifiers (“single sign-on” on an Internet scale); (2) Controlled communication of the user’s personal information to the third parties accessed by the user."@en ;
  rdfs:label "ID4me"@en ;
  sto:hasOfficialResource <https://id4me.org/files/ID4me_Technical_Overview_v1.3.pdf> ;
  sto:hasTargetConcern sto:Identification ;
  sto:hasTargetConcern sto:IdentityManagement ;
.
sto:IDSA
  a owl:NamedIndividual ;
  a foaf:Organization ;
  a sto:IIoTConsortium ;
  terms:creator sto:sebastian ;
  terms:creator "sebastian" ;
  terms:title "International Data Spaces Association"@en ;
  rdfs:comment "IDSA ensures that the special economic interests of business are specifically integrated into the research work of Industrial Date Space."@en ;
  rdfs:label "IDSA"@en ;
  sto:hasOfficialResource <https://www.internationaldataspaces.org/en/> ;
  sto:hasWikipediaArticle <https://de.wikipedia.org/wiki/Industrial_Data_Space#Industrial_Data_Space_Association> ;
.
sto:IDSRAMBusinessLayer
  a owl:NamedIndividual ;
  a sto:IDSRAMLayer ;
  a sto:StandardClassification ;
  dul:associatedWith sto:IIRABusinessDomain ;
  dul:associatedWith sto:OceanSystemViewpoint ;
  dul:associatedWith sto:RAMIBusinessLayer ;
  dul:associatedWith sto:xRoadSystemComponents ;
  rdfs:label "IDS RAM Business Layer"@en ;
  sto:alignsWith sto:IIRABusinessDomain ;
  sto:alignsWith sto:OceanSystemViewpoint ;
  sto:alignsWith sto:RAMIBusinessLayer ;
  sto:alignsWith sto:xRoadSystemComponents ;
  sto:frames sto:RoleCategorization ;
  sto:isDescribedin sto:IDSRAMReferenceArchitectureModel ;
.
sto:IDSRAMBusinessLayerAnno
  a <https://www.w3.org/ns/oaAnnotation> ;
  <https://www.w3.org/ns/oahasBody> sto:IDSRAMBusinessLayer ;
  <https://www.w3.org/ns/oahasTarget> [
      a <https://www.w3.org/ns/oaSpecificResource> ;
      terms:format "pdf" ;
      <https://www.w3.org/ns/oahasSelector> [
          a <https://www.w3.org/ns/oaRangeSelector> ;
          <https://www.w3.org/ns/oahasEndSelector> [
              a <https://www.w3.org/ns/oaXPathSelector> ;
              rdf:value "Page 21" ;
            ] ;
          <https://www.w3.org/ns/oahasStartSelector> [
              a <https://www.w3.org/ns/oaXPathSelector> ;
              rdf:value "Page 17" ;
            ] ;
        ] ;
      <https://www.w3.org/ns/oahasSource> sto:IDS_REFERENCE_ARCHITECTURE_MODEL_INDUSTRIAL_DATA_SPACE_VERSION_2_0 ;
    ] ;
.
sto:IDSRAMCertification
  a <http://w3id.org/ids/ram/Perspective> ;
  a owl:NamedIndividual ;
  a sto:StandardClassification ;
  rdfs:label "IDS RAM Certification Perspective"@en ;
  sto:frames sto:Certification ;
  sto:frames sto:Safety ;
  sto:frames sto:Security ;
  sto:isDescribedin sto:IDSRAMReferenceArchitectureModel ;
.
sto:IDSRAMCertificationAnno
  a <https://www.w3.org/ns/oaAnnotation> ;
  <https://www.w3.org/ns/oahasBody> sto:IDSRAMCertification ;
  <https://www.w3.org/ns/oahasTarget> [
      a <https://www.w3.org/ns/oaSpecificResource> ;
      terms:format "pdf" ;
      <https://www.w3.org/ns/oahasSelector> [
          a <https://www.w3.org/ns/oaRangeSelector> ;
          <https://www.w3.org/ns/oahasEndSelector> [
              a <https://www.w3.org/ns/oaXPathSelector> ;
              rdf:value "Page 84" ;
            ] ;
          <https://www.w3.org/ns/oahasStartSelector> [
              a <https://www.w3.org/ns/oaXPathSelector> ;
              rdf:value "Page 79" ;
            ] ;
        ] ;
      <https://www.w3.org/ns/oahasSource> sto:IDS_REFERENCE_ARCHITECTURE_MODEL_INDUSTRIAL_DATA_SPACE_VERSION_2_0 ;
    ] ;
.
sto:IDSRAMDataMarket
  a owl:NamedIndividual ;
  a sto:StandardClassification ;
  rdfs:label "IDS Data Market"@en ;
  sto:isDescribedin sto:IDSRAMReferenceArchitectureModel ;
.
sto:IDSRAMFunctionalLayer
  a owl:NamedIndividual ;
  a sto:IDSRAMLayer ;
  a sto:StandardClassification ;
  dul:associatedWith sto:DataSovereignty ;
  dul:associatedWith sto:Interoperability ;
  rdfs:label "IDS RAM Functional Layer"@en ;
  sto:isDescribedin sto:IDSRAMReferenceArchitectureModel ;
.
sto:IDSRAMFunctionalLayerAnno
  a <https://www.w3.org/ns/oaAnnotation> ;
  <https://www.w3.org/ns/oahasBody> sto:IDSRAMFunctionalLayer ;
  <https://www.w3.org/ns/oahasTarget> [
      a <https://www.w3.org/ns/oaSpecificResource> ;
      terms:format "pdf" ;
      <https://www.w3.org/ns/oahasSelector> [
          a <https://www.w3.org/ns/oaRangeSelector> ;
          <https://www.w3.org/ns/oahasEndSelector> [
              a <https://www.w3.org/ns/oaXPathSelector> ;
              rdf:value "Page 25" ;
            ] ;
          <https://www.w3.org/ns/oahasStartSelector> [
              a <https://www.w3.org/ns/oaXPathSelector> ;
              rdf:value "Page 21" ;
            ] ;
        ] ;
      <https://www.w3.org/ns/oahasSource> sto:IDS_REFERENCE_ARCHITECTURE_MODEL_INDUSTRIAL_DATA_SPACE_VERSION_2_0 ;
    ] ;
.
sto:IDSRAMGovernance
  a <http://w3id.org/ids/ram/Perspective> ;
  a owl:NamedIndividual ;
  a sto:StandardClassification ;
  dul:associatedWith sto:DtpEcosystemView ;
  dul:associatedWith sto:DtpSecurityPrivacy ;
  dul:associatedWith sto:IICFFrameworkLayer ;
  dul:associatedWith sto:RAMIBusinessLayer ;
  rdfs:label "IDS RAM Governance Perspective"@en ;
  sto:alignsWith sto:DtpEcosystemView ;
  sto:alignsWith sto:DtpSecurityPrivacy ;
  sto:alignsWith sto:IICFFrameworkLayer ;
  sto:alignsWith sto:RAMIBusinessLayer ;
  sto:frames sto:Compliance ;
  sto:frames sto:Trustworthiness ;
  sto:isDescribedin sto:IDSRAMReferenceArchitectureModel ;
.
sto:IDSRAMGovernanceAnno
  a <https://www.w3.org/ns/oaAnnotation> ;
  <https://www.w3.org/ns/oahasBody> sto:IDSRAMGovernance ;
  <https://www.w3.org/ns/oahasTarget> [
      a <https://www.w3.org/ns/oaSpecificResource> ;
      terms:format "pdf" ;
      <https://www.w3.org/ns/oahasSelector> [
          a <https://www.w3.org/ns/oaRangeSelector> ;
          <https://www.w3.org/ns/oahasEndSelector> [
              a <https://www.w3.org/ns/oaXPathSelector> ;
              rdf:value "Page 88" ;
            ] ;
          <https://www.w3.org/ns/oahasStartSelector> [
              a <https://www.w3.org/ns/oaXPathSelector> ;
              rdf:value "Page 84" ;
            ] ;
        ] ;
      <https://www.w3.org/ns/oahasSource> sto:IDS_REFERENCE_ARCHITECTURE_MODEL_INDUSTRIAL_DATA_SPACE_VERSION_2_0 ;
    ] ;
.
sto:IDSRAMInformationLayer
  a owl:NamedIndividual ;
  a sto:IDSRAMLayer ;
  a sto:StandardClassification ;
  dul:associatedWith sto:BdvaDataManagement ;
  dul:associatedWith sto:InformationDomain ;
  dul:associatedWith sto:IotaInformationViewpoint ;
  dul:associatedWith sto:NgsiLdDataRepresentation ;
  dul:associatedWith sto:NgsiLdInformationModel ;
  dul:associatedWith sto:RAMIInformationLayer ;
  dul:associatedWith sto:Vocabulary ;
  rdfs:label "IDS RAM Information Layer"@en ;
  sto:alignsWith sto:BdvaDataManagement ;
  sto:alignsWith sto:InformationDomain ;
  sto:alignsWith sto:IotaInformationViewpoint ;
  sto:alignsWith sto:NgsiLdDataRepresentation ;
  sto:alignsWith sto:NgsiLdInformationModel ;
  sto:alignsWith sto:RAMIInformationLayer ;
  sto:alignsWith sto:Vocabulary ;
  sto:isDescribedin sto:IDSRAMReferenceArchitectureModel ;
.
sto:IDSRAMInformationLayerAnno
  a <https://www.w3.org/ns/oaAnnotation> ;
  <https://www.w3.org/ns/oahasBody> sto:IDSRAMInformationLayer ;
  <https://www.w3.org/ns/oahasTarget> [
      a <https://www.w3.org/ns/oaSpecificResource> ;
      terms:format "pdf" ;
      <https://www.w3.org/ns/oahasSelector> [
          a <https://www.w3.org/ns/oaRangeSelector> ;
          <https://www.w3.org/ns/oahasEndSelector> [
              a <https://www.w3.org/ns/oaXPathSelector> ;
              rdf:value "Page 56" ;
            ] ;
          <https://www.w3.org/ns/oahasStartSelector> [
              a <https://www.w3.org/ns/oaXPathSelector> ;
              rdf:value "Page 32" ;
            ] ;
        ] ;
      <https://www.w3.org/ns/oahasSource> sto:IDS_REFERENCE_ARCHITECTURE_MODEL_INDUSTRIAL_DATA_SPACE_VERSION_2_0 ;
    ] ;
.
sto:IDSRAMInteroperability
  a owl:NamedIndividual ;
  a sto:StandardClassification ;
  rdfs:label "IDS Interoperability"@en ;
  sto:isDescribedin sto:IDSRAMReferenceArchitectureModel ;
.
sto:IDSRAMLayer
  a owl:Class ;
  rdfs:label "IDS RAM Layer"@en ;
  rdfs:subClassOf sto:StandardClassification ;
  owl:equivalentClass [
      a owl:Class ;
      owl:oneOf (
          sto:IDSRAMBusinessLayer
          sto:IDSRAMFunctionalLayer
          sto:IDSRAMInformationLayer
          sto:IDSRAMProcessLayer
          sto:IDSRAMSystemLayer
        ) ;
    ] ;
.
sto:IDSRAMLayerAnno
  a <https://www.w3.org/ns/oaAnnotation> ;
  <https://www.w3.org/ns/oahasBody> sto:IDSRAMLayer ;
  <https://www.w3.org/ns/oahasTarget> [
      a <https://www.w3.org/ns/oaSpecificResource> ;
      terms:format "pdf" ;
      <https://www.w3.org/ns/oahasSource> sto:IDS_REFERENCE_ARCHITECTURE_MODEL_INDUSTRIAL_DATA_SPACE_VERSION_2_0 ;
    ] ;
.
sto:IDSRAMProcessLayer
  a owl:NamedIndividual ;
  a sto:IDSRAMLayer ;
  a sto:StandardClassification ;
  dul:associatedWith sto:BdvaDataAnalytics ;
  dul:associatedWith sto:BdvaDataManagement ;
  dul:associatedWith sto:BdvaDataProcessingArchitectures ;
  dul:associatedWith sto:DtpDeploymentView ;
  dul:associatedWith sto:FiwareApplicationsServicesAndDataDelivery ;
  dul:associatedWith sto:IIRAApplicationDomain ;
  dul:associatedWith sto:IIRAOperationsDomain ;
  dul:associatedWith sto:InformationDomain ;
  dul:associatedWith sto:InterfaceNetworksDevices ;
  dul:associatedWith sto:IotaFunctionalViewpoint ;
  dul:associatedWith sto:IotaInformationViewpoint ;
  dul:associatedWith sto:NgsiLdApiOperation ;
  dul:associatedWith sto:OceanSystemViewpoint ;
  dul:associatedWith sto:RAMIFunctionalLayer ;
  dul:associatedWith sto:xRoadProtocolsInterfaces ;
  dul:associatedWith sto:xRoadSystemComponents ;
  rdfs:label "IDS RAM Process Layer"@en ;
  sto:alignsWith sto:BdvaDataAnalytics ;
  sto:alignsWith sto:BdvaDataManagement ;
  sto:alignsWith sto:BdvaDataProcessingArchitectures ;
  sto:alignsWith sto:DtpDeploymentView ;
  sto:alignsWith sto:FiwareApplicationsServicesAndDataDelivery ;
  sto:alignsWith sto:IIRAApplicationDomain ;
  sto:alignsWith sto:IIRAOperationsDomain ;
  sto:alignsWith sto:InformationDomain ;
  sto:alignsWith sto:InterfaceNetworksDevices ;
  sto:alignsWith sto:IotaFunctionalViewpoint ;
  sto:alignsWith sto:IotaInformationViewpoint ;
  sto:alignsWith sto:NgsiLdApiOperation ;
  sto:alignsWith sto:OceanSystemViewpoint ;
  sto:alignsWith sto:RAMIFunctionalLayer ;
  sto:alignsWith sto:xRoadProtocolsInterfaces ;
  sto:alignsWith sto:xRoadSystemComponents ;
  sto:frames sto:ServiceChoreography ;
  sto:frames sto:ServiceComposition ;
  sto:frames sto:ServiceOrchestration ;
  sto:isDescribedin sto:IDSRAMReferenceArchitectureModel ;
.
sto:IDSRAMProcessLayerAnno
  a <https://www.w3.org/ns/oaAnnotation> ;
  <https://www.w3.org/ns/oahasBody> sto:IDSRAMProcessLayer ;
  <https://www.w3.org/ns/oahasTarget> [
      a <https://www.w3.org/ns/oaSpecificResource> ;
      terms:format "pdf" ;
      <https://www.w3.org/ns/oahasSelector> [
          a <https://www.w3.org/ns/oaRangeSelector> ;
          <https://www.w3.org/ns/oahasEndSelector> [
              a <https://www.w3.org/ns/oaXPathSelector> ;
              rdf:value "Page 32" ;
            ] ;
          <https://www.w3.org/ns/oahasStartSelector> [
              a <https://www.w3.org/ns/oaXPathSelector> ;
              rdf:value "Page 25" ;
            ] ;
        ] ;
      <https://www.w3.org/ns/oahasSource> sto:IDS_REFERENCE_ARCHITECTURE_MODEL_INDUSTRIAL_DATA_SPACE_VERSION_2_0 ;
    ] ;
.
sto:IDSRAMReferenceArchitectureModel
  a owl:NamedIndividual ;
  a sto:ArchitectureDescription ;
  a sto:StandardizationFramework ;
  terms:title "Industrial Data Space Reference Architecture Model"@en ;
  dul:associatedWith sto:IIRAFunctionalViewpoint ;
  rdfs:label "IDS RAM"@en ;
  sto:alignsWith sto:IIRAFunctionalViewpoint ;
  sto:hasPublisher sto:IDSA ;
.
sto:IDSRAMSecurity
  a <http://w3id.org/ids/ram/Perspective> ;
  a owl:NamedIndividual ;
  a sto:StandardClassification ;
  dul:associatedWith sto:BdvaCyberSecurityTrust ;
  dul:associatedWith sto:BdvaDataProtection ;
  dul:associatedWith sto:FiwareSecurity ;
  dul:associatedWith sto:IIRASecurity ;
  dul:associatedWith sto:IIRASecurityFramework ;
  dul:associatedWith sto:IotaFunctionalViewpoint ;
  dul:associatedWith sto:IotaTrustSecurityPrivacy ;
  dul:associatedWith sto:RAMI ;
  rdfs:comment "The IDS Security Architecture provides means to identify participants, protect communication and data exchange transactions between them, and control the use of data after it has been sent."@en ;
  rdfs:label "IDS RAM Security Perspective"@en ;
  sto:alignsWith sto:BdvaCyberSecurityTrust ;
  sto:alignsWith sto:BdvaDataProtection ;
  sto:alignsWith sto:FiwareSecurity ;
  sto:alignsWith sto:IIRASecurity ;
  sto:alignsWith sto:IIRASecurityFramework ;
  sto:alignsWith sto:IotaFunctionalViewpoint ;
  sto:alignsWith sto:IotaTrustSecurityPrivacy ;
  sto:alignsWith sto:OcfSecurity ;
  sto:frames sto:Authentication ;
  sto:frames sto:Authorization ;
  sto:frames sto:Communication ;
  sto:frames sto:DataAccessControl ;
  sto:frames sto:DataSovereignty ;
  sto:frames sto:DataUsageControl ;
  sto:frames sto:Identification ;
  sto:frames sto:IdentityManagement ;
  sto:frames sto:Privacy ;
  sto:frames sto:SecureCommunication ;
  sto:frames sto:Security ;
  sto:frames sto:ServiceIsolation ;
  sto:frames sto:Trustworthiness ;
  sto:isDescribedin sto:IDSRAMReferenceArchitectureModel ;
.
sto:IDSRAMSecurityAnno
  a <https://www.w3.org/ns/oaAnnotation> ;
  <https://www.w3.org/ns/oahasBody> sto:IDSRAMSecurity ;
  <https://www.w3.org/ns/oahasTarget> [
      a <https://www.w3.org/ns/oaSpecificResource> ;
      terms:format "pdf" ;
      <https://www.w3.org/ns/oahasSelector> [
          a <https://www.w3.org/ns/oaRangeSelector> ;
          <https://www.w3.org/ns/oahasEndSelector> [
              a <https://www.w3.org/ns/oaXPathSelector> ;
              rdf:value "Page 79" ;
            ] ;
          <https://www.w3.org/ns/oahasStartSelector> [
              a <https://www.w3.org/ns/oaXPathSelector> ;
              rdf:value "Page 63" ;
            ] ;
        ] ;
      <https://www.w3.org/ns/oahasSource> sto:IDS_REFERENCE_ARCHITECTURE_MODEL_INDUSTRIAL_DATA_SPACE_VERSION_2_0 ;
    ] ;
.
sto:IDSRAMSystemLayer
  a owl:NamedIndividual ;
  a sto:IDSRAMLayer ;
  a sto:StandardClassification ;
  terms:creator sto:sebastian ;
  terms:creator "sebastian" ;
  dul:associatedWith sto:DtpSystemView ;
  dul:associatedWith sto:EdgecrossEdgeComputingLayer ;
  dul:associatedWith sto:EdgecrossItSystemsLayer ;
  dul:associatedWith sto:FIWARE ;
  dul:associatedWith sto:FiwareCloudHosting ;
  dul:associatedWith sto:FiwareIotServicesEnablement ;
  dul:associatedWith sto:IICFFrameworkLayer ;
  dul:associatedWith sto:IIRAControlDomain ;
  dul:associatedWith sto:IIRAImplementationViewpoint ;
  dul:associatedWith sto:IIRAPhysicalSystems ;
  dul:associatedWith sto:InterfaceNetworksDevices ;
  dul:associatedWith sto:IotaDeploymentOperationViewpoint ;
  dul:associatedWith sto:NgsiLdApiOperation ;
  dul:associatedWith sto:NgsiLdArchitecture ;
  dul:associatedWith sto:RAMICommunicationlayer ;
  dul:associatedWith sto:RAMIIntegrationLayer ;
  dul:associatedWith sto:xRoadDeploymentView ;
  rdfs:label "IDS RAM System Layer"@en ;
  sto:alignsWith sto:DtpSystemView ;
  sto:alignsWith sto:EdgecrossEdgeComputingLayer ;
  sto:alignsWith sto:EdgecrossItSystemsLayer ;
  sto:alignsWith sto:FIWARE ;
  sto:alignsWith sto:FiwareCloudHosting ;
  sto:alignsWith sto:FiwareIotServicesEnablement ;
  sto:alignsWith sto:IICFFrameworkLayer ;
  sto:alignsWith sto:IIRAControlDomain ;
  sto:alignsWith sto:IIRAPhysicalSystems ;
  sto:alignsWith sto:InterfaceNetworksDevices ;
  sto:alignsWith sto:IotaDeploymentOperationViewpoint ;
  sto:alignsWith sto:NgsiLdApiOperation ;
  sto:alignsWith sto:NgsiLdArchitecture ;
  sto:alignsWith sto:RAMICommunicationlayer ;
  sto:alignsWith sto:RAMIIntegrationLayer ;
  sto:alignsWith sto:xRoadDeploymentView ;
  sto:isDescribedin sto:IDSRAMReferenceArchitectureModel ;
.
sto:IDSRAMSystemLayerAnno
  a <https://www.w3.org/ns/oaAnnotation> ;
  <https://www.w3.org/ns/oahasBody> sto:IDSRAMSystemLayer ;
  <https://www.w3.org/ns/oahasTarget> [
      a <https://www.w3.org/ns/oaSpecificResource> ;
      terms:format "pdf" ;
      <https://www.w3.org/ns/oahasSelector> [
          a <https://www.w3.org/ns/oaRangeSelector> ;
          <https://www.w3.org/ns/oahasEndSelector> [
              a <https://www.w3.org/ns/oaXPathSelector> ;
              rdf:value "Page 62" ;
            ] ;
          <https://www.w3.org/ns/oahasStartSelector> [
              a <https://www.w3.org/ns/oaXPathSelector> ;
              rdf:value "Page 56" ;
            ] ;
        ] ;
      <https://www.w3.org/ns/oahasSource> sto:IDS_REFERENCE_ARCHITECTURE_MODEL_INDUSTRIAL_DATA_SPACE_VERSION_2_0 ;
    ] ;
.
sto:IDS_REFERENCE_ARCHITECTURE_MODEL_INDUSTRIAL_DATA_SPACE_VERSION_2_0
  a <https://www.w3.org/ns/oaSpecificResource> ;
  rdfs:label "IDS REFERENCE ARCHITECTURE MODEL INDUSTRIAL DATA SPACE VERSION 2.0"@en ;
  sto:hasOpenResource <https://www.fraunhofer.de/content/dam/zv/de/Forschungsfelder/industrial-data-space/IDS_Referenz_Architecture.pdf> ;
.
sto:IEC
  a dul:Collection ;
  a owl:NamedIndividual ;
  a foaf:Organization ;
  a sto:StandardOrganization ;
  rdfs:comment "Is a non-profit, non-governmental international standards organization that prepares and publishes International Standards for all electrical, electronic and related technologies – collectively known as \"electrotechnology\". IEC standards cover a vast range of technologies from power generation, transmission and distribution to home appliances and office equipment, semiconductors, fiber optics, batteries, solar energy, nanotechnology and marine energy as well as many others. The IEC also manages three global conformity assessment systems that certify whether equipment, system or components conform to its International Standards."@en ;
  sto:abbreviation "IEC" ;
  sto:formationDate "1906-06-26"^^xsd:date ;
  sto:hasDBpediaResource <http://dbpedia.org/resource/International_Electrotechnical_Commission> ;
  sto:hasHeadquaterIn dbr:Geneva ;
  sto:hasOfficialResource <http://www.iec.ch/> ;
  sto:hasWikipediaArticle <https://en.wikipedia.org/wiki/International_Electrotechnical_Commission> ;
  sto:orgName "Commission électrotechnique internationale"@fr ;
  sto:orgName "International Electrotechnical Commission"@en ;
.
sto:IEC_11404
  a owl:NamedIndividual ;
  a foaf:Document ;
  a sto:Publication ;
  a sto:Standard ;
  terms:creator sto:IEC ;
  terms:creator sto:ISO ;
  foaf:maker sto:IEC ;
  foaf:maker sto:ISO ;
  sto:hasDeveloper sto:IEC ;
  sto:hasDeveloper sto:ISO ;
  sto:hasPublicationDate "2007-12-01"^^xsd:date ;
  sto:hasPublisher sto:ISO ;
.
sto:IEC_14443
  a owl:NamedIndividual ;
  a foaf:Document ;
  a sto:Publication ;
  a sto:Standard ;
  terms:creator sto:IEC ;
  terms:creator sto:ISO ;
  rdfs:comment "The ISO/IEC 14443 standard is a four-part international standard for contact-less smart cards operating at 13.56 MHz in close proximity (~10cm) with a reader antenna. This ISO standard describes the modulation and transmission protocols between card and reader to create interoperability for contact-less smart card products. There are two main communication protocols supported by the ISO/IEC 14443 standard, they are addressed as Type A and Type B. Most High Frequency (13.56 MHz) proximity tags are using these guidelines for their communication."@en ;
  rdfs:label "ISO/IEC 14443"@en ;
  foaf:maker sto:IEC ;
  foaf:maker sto:ISO ;
  sto:hasDBpediaResource <http://dbpedia.org/resource/ISO/IEC_14443> ;
  sto:hasOfficialResource <https://webstore.iec.ch/publication/62997> ;
  sto:hasOfficialResource <https://www.iso.org/standard/73596.html> ;
  sto:hasOpenResource <http://www.icedev.se/proxmark3/docs/ISO-14443-3.pdf> ;
  sto:hasOpenResource <https://webstore.iec.ch/preview/info_isoiec14443-2%7Bed3.0%7Den.pdf> ;
  sto:hasOpenResource <https://www.sis.se/api/document/preview/912600/> ;
  sto:hasPublisher sto:IEC ;
  sto:hasPublisher sto:ISO ;
  sto:hasWikipediaArticle <https://en.wikipedia.org/wiki/ISO/IEC_14443> ;
.
sto:IEC_15408
  a owl:NamedIndividual ;
  a foaf:Document ;
  a sto:Publication ;
  a sto:Standard ;
  terms:creator sto:ISO ;
  foaf:maker sto:ISO ;
  sto:hasClassification sto:IIRASecurity ;
  sto:hasPublisher sto:ISO ;
.
sto:IEC_15459
  a owl:NamedIndividual ;
  a foaf:Document ;
  a sto:Publication ;
  a sto:Standard ;
  terms:creator sto:IEC ;
  terms:creator sto:ISO ;
  rdfs:comment "ISO/IEC 15459-1:2014 specifies a unique string of characters for the identification of individual transport units. The character string is intended to be represented in a bar code label or other AIDC media attached to the entity to meet management needs. To address management needs, different types of entities are recognized in the various parts of ISO/IEC 15459, which allows different requirements to be met by the identities associated with each type. The rules for the unique identification for individual transport units, to identify physical logistical transfers, with the identity relevant for the duration of one or more items in the load being held or transported as part of that load, are defined and supported by example."@en ;
  rdfs:label "IEC 15459"@en ;
  foaf:maker sto:IEC ;
  foaf:maker sto:ISO ;
  sto:hasOfficialResource <https://webstore.iec.ch/publication/10334> ;
  sto:hasOfficialResource <https://www.iso.org/standard/54779.html> ;
  sto:hasPublisher sto:IEC ;
  sto:hasPublisher sto:ISO ;
.
sto:IEC_24760
  a owl:NamedIndividual ;
  a foaf:Document ;
  a sto:Publication ;
  a sto:Standard ;
  a sto:StandardClassification ;
  terms:creator sto:IEC ;
  dul:associatedWith sto:Identification ;
  rdfs:comment "ISO/IEC 24760: it defines terms for identity management, and also specifies core concepts of identity and identity management and their relationships. It is applicable to any information system that processes identity information. A bibliography of documents describing various aspects of identity information management is provided."@en ;
  rdfs:label "IEC 24760"@en ;
  foaf:maker sto:IEC ;
  sto:alignsWith sto:Identification ;
  sto:hasClassification rami:Safety ;
  sto:hasClassification rami:Security ;
  sto:hasClassification sto:IIRASecurity ;
  sto:hasClassification sto:ProductModelDataExchange ;
  sto:hasClassification sto:RAMIControlDevice ;
  sto:hasClassification sto:RAMIFieldDevice ;
  sto:hasClassification sto:RAMIInformationLayer ;
  sto:hasClassification sto:RAMIProduct ;
  sto:hasClassification sto:RAMIStation ;
  sto:hasOfficialResource <https://webstore.iec.ch/publication/11190> ;
  sto:hasOfficialResource <https://www.iso.org/standard/57914.html> ;
  sto:hasPublicationDate "2011-01-12"^^xsd:date ;
  sto:hasPublisher sto:IEC ;
  sto:relatedTo sto:IEC_24760 ;
  sto:relatedTo sto:IEC_62443 ;
  sto:relatedTo sto:ISO_24760 ;
.
sto:IEC_27018
  a owl:NamedIndividual ;
  a foaf:Document ;
  a sto:Publication ;
  a sto:Standard ;
  terms:creator sto:IEC ;
  terms:creator sto:ISO ;
  foaf:maker sto:IEC ;
  foaf:maker sto:ISO ;
  sto:hasClassification sto:IIRAPrivacy ;
  sto:hasClassification sto:IIRASecurity ;
  sto:hasPublicationDate "2014-08-01"^^xsd:date ;
  sto:hasPublisher sto:IEC ;
  sto:hasPublisher sto:ISO ;
.
sto:IEC_27031
  a owl:NamedIndividual ;
  a foaf:Document ;
  a sto:Domain ;
  a sto:Publication ;
  a sto:Standard ;
  terms:creator sto:IEC ;
  terms:creator sto:ISO ;
  foaf:maker sto:IEC ;
  foaf:maker sto:ISO ;
  sto:domainName "Business Continuity"@en ;
  sto:hasClassification sto:IIRASecurity ;
  sto:hasPublicationDate "2011-03-01"^^xsd:date ;
  sto:hasPublisher sto:IEC ;
  sto:hasPublisher sto:ISO ;
.
sto:IEC_27036
  a owl:NamedIndividual ;
  a foaf:Document ;
  a sto:Publication ;
  a sto:Standard ;
  terms:creator sto:IEC ;
  terms:creator sto:ISO ;
  foaf:maker sto:IEC ;
  foaf:maker sto:ISO ;
  sto:hasClassification sto:IIRASecurity ;
  sto:hasPublicationDate "2016-10-01"^^xsd:date ;
  sto:hasPublisher sto:IEC ;
  sto:hasPublisher sto:ISO ;
.
sto:IEC_29100
  a owl:NamedIndividual ;
  a foaf:Document ;
  a sto:Publication ;
  a sto:Standard ;
  terms:creator sto:IEC ;
  terms:creator sto:ISO ;
  foaf:maker sto:IEC ;
  foaf:maker sto:ISO ;
  sto:hasClassification sto:IIRAPrivacy ;
  sto:hasClassification sto:IIRASecurity ;
  sto:hasPublicationDate "2011-12-01"^^xsd:date ;
  sto:hasPublisher sto:IEC ;
  sto:hasPublisher sto:ISO ;
.
sto:IEC_29115
  a owl:NamedIndividual ;
  a foaf:Document ;
  a sto:Publication ;
  a sto:Standard ;
  terms:creator sto:IEC ;
  terms:creator sto:ISO ;
  terms:title "Information technology -- Security techniques -- Entity authentication assurance framework"@en ;
  rdfs:comment """ISO/IEC 29115:2013 provides a framework for managing entity authentication assurance in a given context. In particular, it:

- specifies four levels of entity authentication assurance;

- specifies criteria and guidelines for achieving each of the four levels of entity authentication assurance;

- provides guidance for mapping other authentication assurance schemes to the four LoAs;

- provides guidance for exchanging the results of authentication that are based on the four LoAs; and

- provides guidance concerning controls that should be used to mitigate authentication threats."""@en ;
  rdfs:label "IEC 29115"@en ;
  foaf:maker sto:IEC ;
  foaf:maker sto:ISO ;
  sto:hasClassification sto:IIRASecurity ;
  sto:hasOfficialResource <https://webstore.iec.ch/publication/11351> ;
  sto:hasOfficialResource <https://www.iso.org/standard/45138.html> ;
  sto:hasPublisher sto:IEC ;
  sto:hasPublisher sto:ISO ;
  sto:hasTargetConcern sto:Authentication ;
  sto:hasTargetConcern sto:Identification ;
.
sto:IEC_29161
  a owl:NamedIndividual ;
  a foaf:Document ;
  a sto:Publication ;
  a sto:Standard ;
  terms:creator sto:IEC ;
  terms:creator sto:ISO ;
  rdfs:comment "ISO/IEC 29161:2016 establishes a unique identification scheme for the Internet of Things (IoT), based on existing and evolving data structures. This International Standard specifies the common rules applicable for unique identification that are required to ensure full compatibility across different identities. The unique identification is a universal construct for any physical object, virtual object, or person. It is used in IoT information systems that need to track or otherwise refer to entities. It is intended for use with any IoT media."@en ;
  rdfs:label "IEC 29161"@en ;
  foaf:maker sto:IEC ;
  foaf:maker sto:ISO ;
  sto:hasDomain "Automatic identification and data capture techniques"@en ;
  sto:hasOfficialResource <https://webstore.iec.ch/publication/60834> ;
  sto:hasOfficialResource <https://www.iso.org/standard/45240.html> ;
  sto:hasPublicationDate "2016-08-01"^^xsd:date ;
  sto:hasPublisher sto:IEC ;
  sto:hasPublisher sto:ISO ;
.
sto:IEC_29182-1
  a owl:NamedIndividual ;
.
sto:IEC_29182_P1
  a owl:NamedIndividual ;
  a sto:Standard ;
  terms:creator sto:IEC ;
  terms:creator sto:ISO ;
  rdfs:comment "ISO/IEC 29182-1: provides a general overview of the characteristics of a sensor network and the organization of the entities that comprise such a network. It also describes the general requirements that are identified for sensor networks."@en ;
  rdfs:label "IEC 29182-1"@en ;
  foaf:maker sto:IEC ;
  foaf:maker sto:ISO ;
  sto:hasClassification sto:ProductionSystemModelData ;
  sto:hasClassification sto:RAMICommunicationlayer ;
  sto:hasClassification sto:RAMIControlDevice ;
  sto:hasClassification sto:RAMIFieldDevice ;
  sto:hasOfficialResource <https://webstore.iec.ch/publication/11411> ;
  sto:hasOfficialResource <https://www.iso.org/standard/45261.html> ;
  sto:hasPublicationDate "2013-06-01"^^xsd:date ;
  sto:hasPublisher sto:IEC ;
  sto:hasPublisher sto:ISO ;
  sto:relatedTo sto:IEC_29182-1 ;
  sto:relatedTo sto:IEC_61158 ;
  sto:relatedTo sto:IEC_61784 ;
  sto:relatedTo sto:OMG_DDS ;
.
sto:IEC_29190
  a owl:NamedIndividual ;
  a foaf:Document ;
  a sto:Publication ;
  a sto:Standard ;
  terms:creator sto:IEC ;
  terms:creator sto:ISO ;
  foaf:maker sto:IEC ;
  foaf:maker sto:ISO ;
  sto:hasClassification sto:IIRAPrivacy ;
  sto:hasClassification sto:IIRASecurity ;
  sto:hasPublicationDate "2015-08-01"^^xsd:date ;
  sto:hasPublisher sto:IEC ;
  sto:hasPublisher sto:ISO ;
.
sto:IEC_42010
  a owl:NamedIndividual ;
  a foaf:Document ;
  a sto:Publication ;
  a sto:Standard ;
  terms:creator sto:IEC ;
  terms:creator sto:ISO ;
  rdfs:comment "ISO/IEC/IEEE 42010:2011 defines requirements on the description of system, software and enterprise architectures. It aims to standardise the practice of architecture description by defining standard terms, presenting a conceptual foundation for expressing, communicating and reviewing architectures and specifying requirements that apply to architecture descriptions, architecture frameworks and architecture description languages."@en ;
  rdfs:label "IEC 42010"@en ;
  owl:sameAs sto:ISO_42010 ;
  skos:note "The IIRA is based on this standards" ;
  foaf:maker sto:IEC ;
  foaf:maker sto:ISO ;
  sto:hasDBpediaResource <http://dbpedia.org/page/ISO/IEC_42010> ;
  sto:hasOfficialResource <http://www.iso-architecture.org/ieee-1471/> ;
  sto:hasOfficialResource <https://standards.ieee.org/standard/42010-2011.html> ;
  sto:hasOfficialResource <https://webstore.iec.ch/publication/11978> ;
  sto:hasOfficialResource <https://www.iso.org/standard/50508.html> ;
  sto:hasOpenResource <http://cabibbo.dia.uniroma3.it/asw/altrui/iso-iec-ieee-42010-2011.pdf> ;
  sto:hasPublisher sto:IEC ;
  sto:hasPublisher sto:IEEE ;
  sto:hasPublisher sto:ISO ;
  sto:hasWikipediaArticle <https://en.wikipedia.org/wiki/ISO/IEC_42010> ;
.
sto:IEC_60027_P6_E1
  a owl:NamedIndividual ;
  a sto:Standard ;
  terms:creator sto:IEC ;
  terms:language lang:eng ;
  terms:language lang:fra ;
  terms:language lang:spa ;
  terms:title "Letter symbols to be used in electrical technology - Part 6: Control technology"@en ;
  rdfs:comment "This part of IEC 60027 is applicable to control technology. It gives names and symbols for quantities, signals and functions, and their units."@en ;
  rdfs:label "IEC 60027-6:2006"@en ;
  foaf:maker sto:IEC ;
  sto:hasAvailableLanguage lang:eng ;
  sto:hasAvailableLanguage lang:fra ;
  sto:hasAvailableLanguage lang:spa ;
  sto:hasDBpediaResource <http://dbpedia.org/page/IEC_60027> ;
  sto:hasEdition "1.0"^^xsd:float ;
  sto:hasFileSize sto:FileSizeIEC_60027_P6 ;
  sto:hasICS sto:ICS_01_060 ;
  sto:hasImplementationFormat "Document"@en ;
  sto:hasOfficialResource <https://webstore.iec.ch/publication/96> ;
  sto:hasPages "29"^^xsd:int ;
  sto:hasPublicationDate "2006-12-14"^^xsd:date ;
  sto:hasPublisher sto:IEC ;
  sto:hasStabilityDate "2019"^^xsd:gYear ;
  sto:hasStatus "Valid"@en ;
  sto:hasTechnicalCommittee sto:TC_25 ;
  sto:hasWikipediaArticle <https://en.wikipedia.org/wiki/IEC_60027> ;
.
sto:IEC_60038_E7
  a owl:NamedIndividual ;
  a sto:Standard ;
  terms:creator sto:IEC ;
  terms:language lang:eng ;
  terms:language lang:fra ;
  terms:language lang:spa ;
  terms:title " IEC standard voltages "@en ;
  rdfs:comment "IEC 60038:2009 specifies standard voltage values which are intended to serve as preferential values for the nominal voltage of electrical supply systems, and as reference values for equipment and system design. This seventh edition supersedes the sixth edition (1993), its Amendment 1 (1994) and its Amendment 2 (1997). It constitutes a technical revision. The significant technical changes are: -the addition of the values of 230 V (50 Hz) and 230/400 V (60 Hz) to Table 1;-the replacement of the utilization voltage range at LV by a reference to the relevant standard and an informative annex;- the addition of the value of 30 kV to Table 3;- the replacement of the value of 1 050 kV by 1 100 kV in Table 5. It has the status of a horizontal standard in accordance with IEC Guide 108."@en ;
  rdfs:label "IEC 60038:2009"@en ;
  foaf:maker sto:IEC ;
  sto:hasAvailableLanguage lang:eng ;
  sto:hasAvailableLanguage lang:fra ;
  sto:hasAvailableLanguage lang:spa ;
  sto:hasDBpediaResource <http://dbpedia.org/page/IEC_60038> ;
  sto:hasEdition "7.0"^^xsd:float ;
  sto:hasFileSize sto:FileSizeIEC_60038 ;
  sto:hasICS sto:ICS_29_020 ;
  sto:hasImplementationFormat "Document"@en ;
  sto:hasOfficialResource <https://webstore.iec.ch/publication/153> ;
  sto:hasPages "26"^^xsd:int ;
  sto:hasPublicationDate "2009-06-17"^^xsd:date ;
  sto:hasPublisher sto:IEC ;
  sto:hasStabilityDate "2020"^^xsd:gYear ;
  sto:hasStatus "Valid"@en ;
  sto:hasTechnicalCommittee sto:TC_8 ;
  sto:hasWikipediaArticle <https://en.wikipedia.org/wiki/IEC_60038> ;
  sto:isRelevantFor sto:RuralElectrification ;
.
sto:IEC_60050
  a owl:NamedIndividual ;
  a foaf:Document ;
  a sto:Publication ;
  a sto:Standard ;
  rdfs:comment "The International Electrotechnical Vocabulary (IEV) serves to promote the global unification of terminology in the field of electrotechnology, electronics and telecommunications."@en ;
  rdfs:label "IEC 60050"@en ;
  skos:altLabel "Electropedia"@en ;
  sto:hasDBpediaResource <http://dbpedia.org/page/International_Electrotechnical_Vocabulary> ;
  sto:hasWikipediaArticle <https://en.wikipedia.org/wiki/International_Electrotechnical_Vocabulary> ;
  sto:relatedTo sto:IEC_60050 ;
  sto:relatedTo sto:IEC_60050_1984 ;
  sto:relatedTo sto:IEC_60050_1998 ;
  sto:relatedTo sto:IEC_60050_2013 ;
.
sto:IEC_60050_1984
  a owl:NamedIndividual ;
.
sto:IEC_60050_1998
  a owl:NamedIndividual ;
.
sto:IEC_60050_2013
  a owl:NamedIndividual ;
.
sto:IEC_60050_P101_E2
  a owl:NamedIndividual ;
  a sto:StandardPart ;
  terms:creator sto:IEC ;
  terms:language lang:eng ;
  terms:language lang:fra ;
  terms:language lang:spa ;
  terms:title "International Electrotechnical Vocabulary - Part 101: Mathematics"@en ;
  dul:isComponentOf sto:IEC_60050 ;
  rdfs:comment "It has the status of a horizontal standard in accordance with IEC Guide 108."@en ;
  rdfs:label "IEC 60050-101:1998"@en ;
  foaf:maker sto:IEC ;
  sto:hasAvailableLanguage lang:eng ;
  sto:hasAvailableLanguage lang:fra ;
  sto:hasAvailableLanguage lang:spa ;
  sto:hasDBpediaResource <http://dbpedia.org/page/International_Electrotechnical_Vocabulary> ;
  sto:hasEdition "2.0"^^xsd:float ;
  sto:hasFileSize sto:FileSizeIEC_60050_P101 ;
  sto:hasICS sto:ICS_01_040_07 ;
  sto:hasImplementationFormat "Document"@en ;
  sto:hasOfficialResource <https://webstore.iec.ch/publication/159> ;
  sto:hasPages "129"^^xsd:int ;
  sto:hasPublicationDate "1998-04-30"^^xsd:date ;
  sto:hasPublisher sto:IEC ;
  sto:hasStatus "Replaced"@en ;
  sto:hasTechnicalCommittee sto:TC_1 ;
  sto:hasWikipediaArticle <https://en.wikipedia.org/wiki/International_Electrotechnical_Vocabulary> ;
  sto:relatedTo sto:IEC_60050 ;
  sto:relatedTo sto:IEC_60050_1984 ;
  sto:relatedTo sto:IEC_60050_1998 ;
  sto:relatedTo sto:IEC_60050_2013 ;
.
sto:IEC_60050_P351_E4
  a owl:NamedIndividual ;
  a sto:StandardPart ;
  terms:creator sto:IEC ;
  terms:language lang:eng ;
  terms:language lang:fra ;
  terms:title "International Electrotechnical Vocabulary - Part 351: Control technology"@en ;
  dul:isComponentOf sto:IEC_60050 ;
  rdfs:comment "IEC 60050-351:2013 gives the general terminology used in control technology, as well as general terms pertaining to specific applications and associated technologies. This new edition reviews and complements the previous one. It has the status of a horizontal standard in accordance with IEC Guide 108."@en ;
  rdfs:label "IEC 60050-351:2013"@en ;
  foaf:maker sto:IEC ;
  sto:hasAvailableLanguage lang:eng ;
  sto:hasAvailableLanguage lang:fra ;
  sto:hasEdition "4.0"^^xsd:float ;
  sto:hasFileSize sto:FileSizeIEC_60050_P351 ;
  sto:hasICS sto:ICS_01_040_07 ;
  sto:hasICS sto:ICS_25_040_40 ;
  sto:hasImplementationFormat "Document"@en ;
  sto:hasOfficialResource <https://webstore.iec.ch/publication/194> ;
  sto:hasPages "457"^^xsd:int ;
  sto:hasPublicationDate "2013-11-25"^^xsd:date ;
  sto:hasPublisher sto:IEC ;
  sto:hasStatus "Valid"@en ;
  sto:hasTechnicalCommittee sto:TC_1 ;
  sto:relatedTo sto:IEC_60050 ;
  sto:relatedTo sto:IEC_60050_1984 ;
  sto:relatedTo sto:IEC_60050_1998 ;
  sto:relatedTo sto:IEC_60050_2013 ;
.
sto:IEC_60050_P371_E1
  a owl:NamedIndividual ;
  a sto:StandardPart ;
  terms:creator sto:IEC ;
  terms:language lang:eng ;
  terms:language lang:fra ;
  terms:language lang:rus ;
  terms:title "International Electrotechnical Vocabulary. Chapter 371: Telecontrol"@en ;
  dul:isComponentOf sto:IEC_60050 ;
  rdfs:comment "Terms on telecontrol, teleprotection and associated telecommunications for electric power systems. It has the status of a horizontal standard in accordance with IEC Guide 108."@en ;
  rdfs:label "IEC 60050-371:1984"@en ;
  foaf:maker sto:IEC ;
  sto:hasAvailableLanguage lang:eng ;
  sto:hasAvailableLanguage lang:fra ;
  sto:hasAvailableLanguage lang:rus ;
  sto:hasEdition "1.0"^^xsd:float ;
  sto:hasFileSize sto:FileSizeIEC_60050_P371 ;
  sto:hasICS sto:ICS_01_040_35 ;
  sto:hasICS sto:ICS_35_240_50 ;
  sto:hasImplementationFormat "Document"@en ;
  sto:hasOfficialResource <https://webstore.iec.ch/publication/196> ;
  sto:hasPages "44"^^xsd:int ;
  sto:hasPublicationDate "1984-11-30"^^xsd:date ;
  sto:hasPublisher sto:IEC ;
  sto:hasStatus "Valid"@en ;
  sto:hasTechnicalCommittee sto:TC_1 ;
  sto:relatedTo sto:IEC_60050 ;
  sto:relatedTo sto:IEC_60050_1984 ;
  sto:relatedTo sto:IEC_60050_1998 ;
  sto:relatedTo sto:IEC_60050_2013 ;
.
sto:IEC_60073_E6
  a owl:NamedIndividual ;
  a sto:Standard ;
  terms:creator sto:IEC ;
  terms:language lang:eng ;
  terms:language lang:fra ;
  terms:language lang:spa ;
  terms:title "Basic and safety principles for man-machine interface, marking and identification - Coding principles for indicators and actuators"@en ;
  rdfs:comment "Establishes general rules for assigning particular meanings to certain visual, acoustsic and tactile indications. It has the status of a Basic Safety Publication in accordance with IEC Guide 104."@en ;
  rdfs:label "IEC 60073:2002 "@en ;
  foaf:maker sto:IEC ;
  sto:hasAvailableLanguage lang:eng ;
  sto:hasAvailableLanguage lang:fra ;
  sto:hasAvailableLanguage lang:spa ;
  sto:hasEdition "6.0"^^xsd:float ;
  sto:hasFileSize sto:FileSizeIEC_60073 ;
  sto:hasICS sto:ICS_01_070 ;
  sto:hasICS sto:ICS_29_020 ;
  sto:hasImplementationFormat "Document"@en ;
  sto:hasOfficialResource <https://webstore.iec.ch/publication/587> ;
  sto:hasPages "61"^^xsd:int ;
  sto:hasPublicationDate "2002-05-22"^^xsd:date ;
  sto:hasPublisher sto:IEC ;
  sto:hasStabilityDate "2025"^^xsd:gYear ;
  sto:hasStatus "Valid"@en ;
  sto:hasTag "IEC_60073:2002"@en ;
  sto:hasTechnicalCommittee sto:TC_3 ;
.
sto:IEC_60086
  a owl:NamedIndividual ;
  a foaf:Document ;
  a sto:Publication ;
  a sto:Standard ;
  terms:creator sto:IEC ;
  rdfs:comment "Standard battery nomenclature describes portable dry cell batteries that have physical dimensions and electrical characteristics interchangeable between manufacturers."@en ;
  rdfs:label "IEC 60086"@en ;
  foaf:maker sto:IEC ;
  sto:hasDBpediaResource <http://dbpedia.org/page/Battery_nomenclature#IEC_60086> ;
  sto:hasOfficialResource <https://webstore.iec.ch/publication/22991> ;
  sto:hasPublisher sto:IEC ;
  sto:hasWikipediaArticle <https://en.wikipedia.org/wiki/Battery_nomenclature#IEC_60086> ;
.
sto:IEC_60204_P11_E1
  a owl:NamedIndividual ;
  a sto:Standard ;
  terms:creator sto:IEC ;
  terms:language lang:eng ;
  terms:language lang:fra ;
  terms:language lang:spa ;
  terms:title "Safety of machinery - Electrical equipment of machines - Part 11: Requirements for HV equipment for voltages above 1 000 V a.c. or 1 500 V d.c. and not exceeding 36 kV"@en ;
  rdfs:comment "Applies to the electrical and electronic equipment and systems of machines, including a group of machines working together in a coordinated manner, but excluding higher level system aspects (i.e. communications between systems)."@en ;
  rdfs:label "IEC 60204-11:2000"@en ;
  foaf:maker sto:IEC ;
  sto:hasAvailableLanguage lang:eng ;
  sto:hasAvailableLanguage lang:fra ;
  sto:hasAvailableLanguage lang:spa ;
  sto:hasEdition "1.0"^^xsd:float ;
  sto:hasFileSize sto:FileSizeIEC_60204_P11 ;
  sto:hasICS sto:ICS_13_110 ;
  sto:hasICS sto:ICS_29_020 ;
  sto:hasImplementationFormat "Document"@en ;
  sto:hasOfficialResource <https://webstore.iec.ch/publication/1022> ;
  sto:hasPages "111"^^xsd:int ;
  sto:hasPublicationDate "2000-07-31"^^xsd:date ;
  sto:hasPublisher sto:IEC ;
  sto:hasStabilityDate "2018"^^xsd:gYear ;
  sto:hasStatus "Withdrawn"@en ;
  sto:hasTechnicalCommittee sto:TC_44 ;
.
sto:IEC_60255_P149_E1
  a owl:NamedIndividual ;
  a sto:Standard ;
  terms:creator sto:IEC ;
  terms:language lang:eng ;
  terms:language lang:fra ;
  terms:title "Measuring relays and protection equipment - Part 149: Functional requirements for thermal electrical relays"@en ;
  rdfs:comment "IEC 60255-149:2013 specifies minimum requirements for thermal protection relays. This standard includes specification of the protection function, measurement characteristics and test methodologies. The object is to establish a common and reproducible reference for evaluating dependent time relays which protect equipment from thermal damage by measuring a.c. current flowing through the equipment. Complementary input energizing quantities such as ambient, coolant, top oil and winding temperature may be applicable for the thermal protection specification set forth in this standard. This standard covers protection relays based on a thermal model with memory function."@en ;
  rdfs:label "IEC 60255-149:2013 "@en ;
  foaf:maker sto:IEC ;
  sto:hasAvailableLanguage lang:eng ;
  sto:hasAvailableLanguage lang:fra ;
  sto:hasEdition "1.0"^^xsd:float ;
  sto:hasFileSize sto:FileSizeIEC_60255_P149 ;
  sto:hasICS sto:ICS_29_120_70 ;
  sto:hasImplementationFormat "Document"@en ;
  sto:hasOfficialResource <https://webstore.iec.ch/publication/1165> ;
  sto:hasPages "93"^^xsd:int ;
  sto:hasPublicationDate "2013-07-30"^^xsd:date ;
  sto:hasPublisher sto:IEC ;
  sto:hasStatus "Valid"@en ;
  sto:hasTag "IEC 60255-149:2013 "@en ;
  sto:hasTechnicalCommittee sto:TC_95 ;
.
sto:IEC_60255_P151_E1
  a owl:NamedIndividual ;
  a sto:Standard ;
  terms:creator sto:IEC ;
  terms:language lang:eng ;
  terms:language lang:fra ;
  terms:title "Measuring relays and protection equipment - Part 151: Functional requirements for over/under current protection"@en ;
  rdfs:comment "IEC 60255-151:2009 specifies minimum requirements for over/under current relays. It includes a specification of the protection function, measurement characteristics and time delay characteristics. Defines the influencing factors that affect the accuracy under steady state conditions and performance characteristics during dynamic conditions."@en ;
  rdfs:label "IEC 60255-151:2009 "@en ;
  foaf:maker sto:IEC ;
  sto:hasAvailableLanguage lang:eng ;
  sto:hasAvailableLanguage lang:fra ;
  sto:hasEdition "1.0"^^xsd:float ;
  sto:hasFileSize sto:FileSizeIEC_60255_P151 ;
  sto:hasICS sto:ICS_29_120_70 ;
  sto:hasImplementationFormat "Document"@en ;
  sto:hasOfficialResource <https://webstore.iec.ch/publication/1166> ;
  sto:hasPages "63"^^xsd:int ;
  sto:hasPublicationDate "2009-08-28"^^xsd:date ;
  sto:hasPublisher sto:IEC ;
  sto:hasStatus "Valid"@en ;
  sto:hasTag "IEC 60255-151:2009 "@en ;
  sto:hasTechnicalCommittee sto:TC_95 ;
.
sto:IEC_60255_P1_E1
  a owl:NamedIndividual ;
  a sto:Standard ;
  terms:creator sto:IEC ;
  terms:language lang:eng ;
  terms:language lang:fra ;
  terms:language lang:spa ;
  terms:title "Measuring relays and protection equipment - Part 1: Common requirements"@en ;
  rdfs:comment "IEC 60255-1:2009 specifies common rules and requirements applicable to measuring relays and protection equipment including any combination of devices to form schemes for power system protection such as control, monitoring and process interface equipment in order to obtain uniformity of requirements and tests. Covers all measuring relays and protection equipment used for protection within the power system environment."@en ;
  rdfs:label "IEC 60255-1:2009 "@en ;
  foaf:maker sto:IEC ;
  sto:hasAvailableLanguage lang:eng ;
  sto:hasAvailableLanguage lang:fra ;
  sto:hasAvailableLanguage lang:spa ;
  sto:hasEdition "1.0"^^xsd:float ;
  sto:hasFileSize sto:FileSizeIEC_60255_P1 ;
  sto:hasICS sto:ICS_29_120_70 ;
  sto:hasImplementationFormat "Document"@en ;
  sto:hasOfficialResource <https://webstore.iec.ch/publication/1160> ;
  sto:hasPages "89"^^xsd:int ;
  sto:hasPublicationDate "2009-08-18"^^xsd:date ;
  sto:hasPublisher sto:IEC ;
  sto:hasStabilityDate "2018"^^xsd:gYear ;
  sto:hasStatus "Valid"@en ;
  sto:hasTag "IEC 60255-1:2009 "@en ;
  sto:hasTechnicalCommittee sto:TC_95 ;
.
sto:IEC_60255_P27_E2
  a owl:NamedIndividual ;
  a sto:Standard ;
  terms:creator sto:IEC ;
  terms:language lang:eng ;
  terms:language lang:fra ;
  terms:title "Measuring relays and protection equipment - Part 27: Product safety requirements"@en ;
  rdfs:comment "IEC 60255-27:2013 describes the product safety requirements for measuring relays and protection equipment having a rated a.c. voltage up to 1 000 V with a rated frequency up to 65 Hz, or a rated d.c. voltage up to 1 500 V. Above these limits, IEC 60664-1 is applicable for the determination of clearance, creepage distance and withstand test voltage. This standard details essential safety requirements to minimize the risk of fire and hazards caused by electric shock or injury to the user. This new edition includes the following significant technical changes with respect to the previous edition:- the removal of tables and diagrams which are from other standards and referring instead directly to the source standard;- all aspects of IEC 60255-5 have been covered and this standard will be withdrawn."@en ;
  rdfs:label "IEC 60255-27:2013 "@en ;
  foaf:maker sto:IEC ;
  sto:hasAvailableLanguage lang:eng ;
  sto:hasAvailableLanguage lang:fra ;
  sto:hasEdition "2.0"^^xsd:float ;
  sto:hasFileSize sto:FileSizeIEC_60255_P27 ;
  sto:hasICS sto:ICS_29_120_70 ;
  sto:hasImplementationFormat "Document"@en ;
  sto:hasOfficialResource <https://webstore.iec.ch/publication/1172> ;
  sto:hasPages "197"^^xsd:int ;
  sto:hasPublicationDate "2013-10-15"^^xsd:date ;
  sto:hasPublisher sto:IEC ;
  sto:hasStabilityDate "2018"^^xsd:gYear ;
  sto:hasStatus "Valid"@en ;
  sto:hasTag "IEC 60255-27:2013 "@en ;
  sto:hasTechnicalCommittee sto:TC_95 ;
.
sto:IEC_60286_P3_E5
  a owl:NamedIndividual ;
  a sto:Standard ;
  terms:creator sto:IEC ;
  terms:language lang:eng ;
  terms:language lang:fra ;
  terms:title "Packaging of components for automatic handling - Part 3: Packaging of surface mount components on continuous tapes"@en ;
  rdfs:comment "IEC 60286-3:2013 is applicable to the tape packaging of electronic components without leads or with lead stumps, intended to be connected to electronic circuits. It includes only those dimensions that are essential for the taping of components intended for the above-mentioned purposes. This standard also includes requirements related to the packaging of singulated die products including bare die and bumped die (flip chips). This fifth edition cancels and replaces the fourth edition, published in 2007, as well as IEC 60286-3-1, published in 2009 and IEC 60286-3-2, published in 2009. It constitutes a full layout revision. In addition, this edition includes the following significant technical changes with respect to the previous edition:a) IEC 60286-3:2013 is applicable to the tape packaging of electronic components without leads or with lead stumps, intended to be connected to electronic circuits. It includes only those dimensions that are essential for the taping of components intended for the above-mentioned purposes. This standard also includes requirements related to the packaging of singulated die products including bare die and bumped die (flip chips). This fifth edition cancels and replaces the fourth edition, published in 2007, as well as IEC 60286-3-1, published in 2009 and IEC 60286-3-2, published in 2009.It constitutes a full layout revision. In addition, this edition includes the following significant technical changes with respect to the previous edition:a) integration of IEC 60286-3-1:2009 as type 1b (Packaging of surface mount components on continuous pressed carrier tapes);b) integration of IEC 60286-3-2:2009 as type 2b (Packaging of surface mount components on blister carrier tapes 4 mm in width).ntegration of IEC 60286-3-1:2009 as type 1b (Packaging of surface mount components on continuous pressed carrier tapes);b) integration of IEC 60286-3-2:2009 as type 2b (Packaging of surface mount components on blister carrier tapes 4 mm in width)."@en ;
  rdfs:label "IEC 60286-3:2013"@en ;
  foaf:maker sto:IEC ;
  sto:hasAvailableLanguage lang:eng ;
  sto:hasAvailableLanguage lang:fra ;
  sto:hasEdition "5.0"^^xsd:float ;
  sto:hasFileSize sto:FileSizeIEC_60286_P3 ;
  sto:hasICS sto:ICS_31_020 ;
  sto:hasICS sto:ICS_31_240 ;
  sto:hasImplementationFormat "Document"@en ;
  sto:hasOfficialResource <https://webstore.iec.ch/publication/1258> ;
  sto:hasPages "77"^^xsd:int ;
  sto:hasPublicationDate "2013-05-17"^^xsd:date ;
  sto:hasPublisher sto:IEC ;
  sto:hasStabilityDate "2024"^^xsd:gYear ;
  sto:hasStatus "Valid"@en ;
  sto:hasTag "IEC 60286-3:2013"@en ;
  sto:hasTechnicalCommittee sto:TC_40 ;
.
sto:IEC_60286_P4_E3
  a owl:NamedIndividual ;
  a sto:Standard ;
  terms:creator sto:IEC ;
  terms:language lang:eng ;
  terms:language lang:fra ;
  terms:title "Packaging of components for automatic handling - Part 4: Stick magazines for electronic components encapsulated in packages of different forms"@en ;
  rdfs:comment "IEC 60286-4:2013 is applicable to stick magazines (including end stoppers) intended to be used for storage of electronic components, for transport from the manufacturer to the customer and for in-house use in the manufacturing plant. They are also used to feed automatic placement machines for surface mounting as well as for through-hole mounting of electronic components. This edition includes the following significant technical changes with respect to the previous edition: Clause 4 describes the guidelines for customer specific stick magazine design. It replaces the magazine design rules for IEC outlined components and rules for orientation of components in stick magazines which have been moved to Annexes A to D."@en ;
  rdfs:label "IEC 60286-4:2013"@en ;
  foaf:maker sto:IEC ;
  sto:hasAvailableLanguage lang:eng ;
  sto:hasAvailableLanguage lang:fra ;
  sto:hasEdition "3.0"^^xsd:float ;
  sto:hasFileSize sto:FileSizeIEC_60286_P4 ;
  sto:hasICS sto:ICS_31_020 ;
  sto:hasICS sto:ICS_31_240 ;
  sto:hasImplementationFormat "Document"@en ;
  sto:hasOfficialResource <https://webstore.iec.ch/publication/1259> ;
  sto:hasPages "32"^^xsd:int ;
  sto:hasPublicationDate "2013-07-26"^^xsd:date ;
  sto:hasPublisher sto:IEC ;
  sto:hasStabilityDate "2022"^^xsd:gYear ;
  sto:hasStatus "Valid"@en ;
  sto:hasTag "IEC 60286-3:2013"@en ;
  sto:hasTechnicalCommittee sto:TC_40 ;
.
sto:IEC_60286_P5_E3
  a owl:NamedIndividual ;
  a sto:Standard ;
  terms:creator sto:IEC ;
  terms:language lang:eng ;
  terms:title "Packaging of components for automatic handling - Part 5: Matrix trays"@en ;
  rdfs:comment "IEC 60286-5:2018 RLV contains the International Standard and its Redline version. The Redline version is available in English only. The Redline version provides you with a quick and easy way to compare all the changes between this standard and its previous edition. The Redline version is not an official IEC Standard, only the current version of the standard is to be considered the official document.IEC 60286-5:2018 describes the common dimensions, tolerances and characteristics of the tray. It includes only those dimensions that are essential for the handling of the trays for the stated purpose and for placing or removing components from the trays. This edition includes the following significant technical changes with respect to the previous edition: - The generic rules for the design of matrix trays are given in this document. Newly developed trays which follow these rules will not be listed individually. Only those trays which conform to the design rules set forth herein are classified as 'standard trays' and are thus preferred for use.- An update of the matrix trays, which do not conform to the design rules set forth herein, are considered as 'non-standard trays' and are not preferred for use, is listed in Annex A."@en ;
  rdfs:label "IEC 60286-5:2018"@en ;
  foaf:maker sto:IEC ;
  sto:hasAvailableLanguage lang:eng ;
  sto:hasEdition "3.0"^^xsd:float ;
  sto:hasFileSize sto:FileSizeIEC_60286_P5 ;
  sto:hasICS sto:ICS_31_020 ;
  sto:hasImplementationFormat "Document"@en ;
  sto:hasOfficialResource <https://webstore.iec.ch/publication/63037> ;
  sto:hasPages "71"^^xsd:int ;
  sto:hasPublicationDate "2018-04-25"^^xsd:date ;
  sto:hasPublisher sto:IEC ;
  sto:hasStabilityDate "2024"^^xsd:gYear ;
  sto:hasStatus "RLV-Redline version"@en ;
  sto:hasStatus "Valid"@en ;
  sto:hasTag "IEC 60286-5:2018"@en ;
  sto:hasTechnicalCommittee sto:TC_40 ;
.
sto:IEC_60364
  a owl:NamedIndividual ;
  a foaf:Document ;
  a sto:Publication ;
  a sto:Standard ;
  terms:creator sto:IEC ;
  rdfs:comment "Electrical Installations for Buildings is the International Electrotechnical Commission's international standard on electrical installations of buildings"@en ;
  rdfs:label "IEC 60364"@en ;
  foaf:maker sto:IEC ;
  sto:hasDBpediaResource <http://dbpedia.org/page/IEC_60364> ;
  sto:hasOfficialResource <https://webstore.iec.ch/publication/1865> ;
  sto:hasPublisher sto:IEC ;
  sto:hasWikipediaArticle <https://en.wikipedia.org/wiki/IEC_60364> ;
.
sto:IEC_60381_P1_E2
  a owl:NamedIndividual ;
  a sto:Standard ;
  terms:creator sto:IEC ;
  terms:language lang:eng ;
  terms:language lang:fra ;
  terms:title "Analogue signals for process control systems. Part 1: Direct current signals"@en ;
  rdfs:comment "Applicable to analogue direct current signals used in industrial-process measurement and control systems to transmit information between elements of systems. Does not apply to signals used entirely within an element."@en ;
  rdfs:label "IEC 60381-1:1982"@en ;
  foaf:maker sto:IEC ;
  sto:hasAvailableLanguage lang:eng ;
  sto:hasAvailableLanguage lang:fra ;
  sto:hasEdition "2.0"^^xsd:float ;
  sto:hasFileSize sto:FileSizeIEC_60381_P1 ;
  sto:hasICS sto:ICS_33_200 ;
  sto:hasImplementationFormat "Document"@en ;
  sto:hasOfficialResource <https://webstore.iec.ch/publication/1948> ;
  sto:hasPages "9"^^xsd:int ;
  sto:hasPublicationDate "1982-01-01"^^xsd:date ;
  sto:hasPublisher sto:IEC ;
  sto:hasStabilityDate "2018"^^xsd:gYear ;
  sto:hasStatus "Valid"@en ;
  sto:hasTag "IEC 60381-1:1982"@en ;
  sto:hasTechnicalCommittee sto:TC_40 ;
.
sto:IEC_60381_P2_E1
  a owl:NamedIndividual ;
  a sto:Standard ;
  terms:creator sto:IEC ;
  terms:language lang:eng ;
  terms:language lang:fra ;
  terms:language lang:rus ;
  terms:title "Analogue signals for process control systems. Part 2: Direct voltage signals"@en ;
  rdfs:comment "Applicable to analogue direct voltage signals used in industrial process measurement and control systems. lt specifies ranges of analogue direct voltage signals and the signal common; it also deals with ripple content. The analogue direct voltage signal, unlike the analogue direct current signal specified in IEC 60381-1, is not intended for transmission over long distances. This standard does not apply to signals used entirely within an element."@en ;
  rdfs:label "IEC 60381-2:1978"@en ;
  foaf:maker sto:IEC ;
  sto:hasAvailableLanguage lang:eng ;
  sto:hasAvailableLanguage lang:fra ;
  sto:hasAvailableLanguage lang:rus ;
  sto:hasEdition "1.0"^^xsd:float ;
  sto:hasFileSize sto:FileSizeIEC_60381_P2 ;
  sto:hasICS sto:ICS_33_200 ;
  sto:hasICS sto:ICS_35_240_50 ;
  sto:hasImplementationFormat "Document"@en ;
  sto:hasOfficialResource <https://webstore.iec.ch/publication/1949> ;
  sto:hasPages "9"^^xsd:int ;
  sto:hasPublicationDate "1978-01-01"^^xsd:date ;
  sto:hasPublisher sto:IEC ;
  sto:hasStabilityDate "2018"^^xsd:gYear ;
  sto:hasStatus "Valid"@en ;
  sto:hasTag "IEC 60381-2:1978"@en ;
  sto:hasTechnicalCommittee sto:TC_65 ;
.
sto:IEC_60382
  a owl:NamedIndividual ;
  a foaf:Document ;
  a sto:Publication ;
  a sto:Standard ;
  terms:creator sto:IEC ;
  terms:language lang:eng ;
  terms:language lang:fra ;
  terms:title "Analogue pneumatic signal for process control systems"@en ;
  rdfs:comment "Applies to analogue pneumatic signals used in process control systems to transmit information between the elements of systems and gives definitions, units and the recommended value of the range of the analogue pneumatic signal."@en ;
  rdfs:label "IEC 60382:1991"@en ;
  foaf:maker sto:IEC ;
  sto:hasAvailableLanguage lang:eng ;
  sto:hasAvailableLanguage lang:fra ;
  sto:hasEdition "2.0"^^xsd:float ;
  sto:hasFileSize sto:FileSizeIEC_60382 ;
  sto:hasICS sto:ICS_25_040_40 ;
  sto:hasOfficialResource <https://webstore.iec.ch/publication/1950> ;
  sto:hasPages "9"^^xsd:int ;
  sto:hasPublicationDate "1991-11-01"^^xsd:date ;
  sto:hasPublisher sto:IEC ;
  sto:hasStabilityDate "2018"^^xsd:gYear ;
  sto:hasTechnicalCommittee sto:TC_65 ;
.
sto:IEC_60382_E2
  a owl:NamedIndividual ;
  a sto:Standard ;
  terms:creator sto:IEC ;
  terms:language lang:eng ;
  terms:language lang:fra ;
  terms:title "Analogue pneumatic signal for process control systems"@en ;
  rdfs:comment "Applies to analogue pneumatic signals used in process control systems to transmit information between the elements of systems and gives definitions, units and the recommended value of the range of the analogue pneumatic signal."@en ;
  rdfs:label "IEC 60382:1991"@en ;
  foaf:maker sto:IEC ;
  sto:hasAvailableLanguage lang:eng ;
  sto:hasAvailableLanguage lang:fra ;
  sto:hasEdition "2.0"^^xsd:float ;
  sto:hasFileSize sto:FileSizeIEC_60382 ;
  sto:hasICS sto:ICS_25_040_40 ;
  sto:hasImplementationFormat "Document"@en ;
  sto:hasOfficialResource <https://webstore.iec.ch/publication/1950> ;
  sto:hasPages "9"^^xsd:int ;
  sto:hasPublicationDate "1991-11-01"^^xsd:date ;
  sto:hasPublisher sto:IEC ;
  sto:hasStabilityDate "2018"^^xsd:gYear ;
  sto:hasStatus "Valid"@en ;
  sto:hasTag "IEC 60382:1991"@en ;
  sto:hasTechnicalCommittee sto:TC_65 ;
.
sto:IEC_60839_P5_S2_E2
  a owl:NamedIndividual ;
  a sto:Standard ;
  terms:creator sto:IEC ;
  terms:title "Alarm and electronic security systems - Part 5-2: Alarm transmission systems - Requirements for supervised premises transceiver (SPT)"@en ;
  rdfs:comment "IEC 60839-5-2:2016 specifies the general equipment requirements for the performance, reliability, resilience, security and safety characteristics of supervised premises transceiver (SPT) installed in supervised premises and used in alarm transmission systems (ATS). A supervised premises transceiver can be a stand-alone device or an integrated part of an alarm system. These requirements also apply to the SPT sharing means of interconnection, control, communication and power supplies with other applications. The alarm transmission system requirements and classifications are defined within IEC 60839-5-1. This new edition includes the following significant technical changes with respect to the previous edition: reflects the current technological state of art (IP networks) ,harmonizes with the ATS categories introduced in IEC 60839-5-1:2014; introduces test requirements."@en ;
  rdfs:label "IEC 60839-5-2:2016"@en ;
  foaf:maker sto:IEC ;
  sto:hasAvailableLanguage lang:eng ;
  sto:hasAvailableLanguage lang:fra ;
  sto:hasClassification rami:Security ;
  sto:hasClassification sto:RAMICommunicationlayer ;
  sto:hasClassification sto:RAMIControlDevice ;
  sto:hasClassification sto:RAMIFieldDevice ;
  sto:hasEdition "2.0"^^xsd:float ;
  sto:hasFileSize sto:FileSizeIEC_60839_P5_S2 ;
  sto:hasICS sto:ICS_13_320 ;
  sto:hasImplementationFormat "Document"@en ;
  sto:hasOfficialResource <https://webstore.iec.ch/publication/24120> ;
  sto:hasPages "63"^^xsd:int ;
  sto:hasPublicationDate "2016-02-03"^^xsd:date ;
  sto:hasPublisher sto:IEC ;
  sto:hasStabilityDate "2019"^^xsd:gYear ;
  sto:hasStatus "Valid"@en ;
  sto:hasTag "IEC 60839-5-2:2016"@en ;
  sto:hasTechnicalCommittee sto:TC_79 ;
.
sto:IEC_60839_P7_S1_E1
  a owl:NamedIndividual ;
  a sto:Standard ;
  terms:creator sto:IEC ;
  terms:language lang:eng ;
  terms:language lang:fra ;
  terms:title "Alarm systems - Part 7-1: Message formats and protocols for serial data interfaces in alarm transmission systems – General"@en ;
  rdfs:comment "Describes the requirements for standard serial data interfaces in alarm transmission systems. Gives an outline of how alarm transmission systems are connected and the various types of serial data interfaces that might be employed."@en ;
  rdfs:label "IEC 60839-7-1:2001"@en ;
  foaf:maker sto:IEC ;
  sto:hasAvailableLanguage lang:eng ;
  sto:hasAvailableLanguage lang:fra ;
  sto:hasEdition "1.0"^^xsd:float ;
  sto:hasFileSize sto:FileSizeIEC_60839_P7_S1 ;
  sto:hasICS sto:ICS_13_320 ;
  sto:hasOfficialResource <https://webstore.iec.ch/publication/3666> ;
  sto:hasPages "39"^^xsd:int ;
  sto:hasPublicationDate "1968-03-01"^^xsd:date ;
  sto:hasPublicationDate "2001-03-09"^^xsd:date ;
  sto:hasPublisher sto:IEC ;
  sto:hasStabilityDate "2018"^^xsd:gYear ;
  sto:hasTag "IEC 60839-7-1:2001"@en ;
  sto:hasTechnicalCommittee sto:TC_79 ;
  sto:hasstatus "Valid" ;
.
sto:IEC_60839_P7_S2_E1
  a owl:NamedIndividual ;
  a sto:Standard ;
  terms:creator sto:IEC ;
  terms:language lang:eng ;
  terms:language lang:fra ;
  terms:title "Alarm systems - Part 7-2: Message formats and protocols for serial data interfaces in alarm transmission systems - Common application layer protocol"@en ;
  rdfs:comment "Specifies a common application layer protocol (message structure, formats and transmission procedures) to be used at standard interfaces in alarm transmission systems. Should be used at all such interfaces where equipment from one supplier is intended to inter-work with equipment from other suppliers."@en ;
  rdfs:label "IEC 60839-7-2:2001"@en ;
  foaf:maker sto:IEC ;
  sto:hasAvailableLanguage lang:eng ;
  sto:hasAvailableLanguage lang:fra ;
  sto:hasEdition "1.0"^^xsd:float ;
  sto:hasFileSize sto:FileSizeIEC_60839_P7_S2 ;
  sto:hasICS sto:ICS_13_320 ;
  sto:hasOfficialResource <https://webstore.iec.ch/publication/3669> ;
  sto:hasPages "53"^^xsd:int ;
  sto:hasPublicationDate "1968-03-01"^^xsd:date ;
  sto:hasPublicationDate "2001-03-09"^^xsd:date ;
  sto:hasPublisher sto:IEC ;
  sto:hasStabilityDate "2018"^^xsd:gYear ;
  sto:hasTag "IEC 60839-7-2:2001"@en ;
  sto:hasTechnicalCommittee sto:TC_79 ;
  sto:hasstatus "Valid" ;
.
sto:IEC_60839_P7_S3_E1
  a owl:NamedIndividual ;
  a sto:Standard ;
  terms:creator sto:IEC ;
  terms:language lang:eng ;
  terms:language lang:fra ;
  terms:title "Alarm systems - Part 7-3: Message formats and protocols for serial data interfaces in alarm transmission systems - Common data link layer protocol"@en ;
  rdfs:comment "Specifies the data link layer message structure, formats and transmission procedures which should be used at standard serial data interfaces in alarm transmission systems where the transmission network employed does not offer a standard protocol. Is necessary in order to ensure compatibility of equipment from different suppliers."@en ;
  rdfs:label "IEC 60839-7-3:2001"@en ;
  foaf:maker sto:IEC ;
  sto:hasAvailableLanguage lang:eng ;
  sto:hasAvailableLanguage lang:fra ;
  sto:hasEdition "1.0"^^xsd:float ;
  sto:hasFileSize sto:FileSizeIEC_60839_P7_S3 ;
  sto:hasICS sto:ICS_13_320 ;
  sto:hasOfficialResource <https://webstore.iec.ch/publication/3671> ;
  sto:hasPages "29"^^xsd:int ;
  sto:hasPublicationDate "1968-03-01"^^xsd:date ;
  sto:hasPublicationDate "2001-03-09"^^xsd:date ;
  sto:hasPublisher sto:IEC ;
  sto:hasStabilityDate "2018"^^xsd:gYear ;
  sto:hasTag "IEC 60839-7-3:2001"@en ;
  sto:hasTechnicalCommittee sto:TC_79 ;
  sto:hasstatus "Valid" ;
.
sto:IEC_60839_P7_S4_E1
  a owl:NamedIndividual ;
  a sto:Standard ;
  terms:creator sto:IEC ;
  terms:language lang:eng ;
  terms:language lang:fra ;
  terms:title "Alarm systems - Part 7-4: Message formats and protocols for serial data interfaces in alarm transmission systems - Common transport layer protocol"@en ;
  rdfs:comment "Specifies the transport layer message structure, formats and transmission procedures to be used at standard interfaces in alarm transmission systems. Should be used at all such interfaces where equipment from one supplier is intended to inter-work with equipment from other suppliers, and where the underlying system architecture does not provide the necessary facilities to support the common application layer."@en ;
  rdfs:label "IEC 60839-7-4:2001"@en ;
  foaf:maker sto:IEC ;
  sto:hasAvailableLanguage lang:eng ;
  sto:hasAvailableLanguage lang:fra ;
  sto:hasEdition "1.0"^^xsd:float ;
  sto:hasFileSize sto:FileSizeIEC_60839_P7_S4 ;
  sto:hasICS sto:ICS_13_320 ;
  sto:hasOfficialResource <https://webstore.iec.ch/publication/3672> ;
  sto:hasPages "23"^^xsd:int ;
  sto:hasPublicationDate "1968-03-01"^^xsd:date ;
  sto:hasPublicationDate "2001-03-09"^^xsd:date ;
  sto:hasPublisher sto:IEC ;
  sto:hasStabilityDate "2018"^^xsd:gYear ;
  sto:hasTag "IEC 60839-7-4:2001"@en ;
  sto:hasTechnicalCommittee sto:TC_79 ;
  sto:hasstatus "Valid" ;
.
sto:IEC_60839_P7_S5_E1
  a owl:NamedIndividual ;
  a sto:Standard ;
  terms:creator sto:IEC ;
  terms:language lang:eng ;
  terms:language lang:fra ;
  terms:title "Alarm systems - Part 7-5: Message formats and protocols for serial data interfaces in alarm transmission systems - Alarm system interfaces employing a two-wire configuration in accordance with ISO/IEC 8482"@en ;
  rdfs:comment "Specifies the requirements for standard interfaces using a two-wire connection employing ISO/IEC 8482 signalling for use between the control and indicating equipment of an alarm system and one or more alarm system transceivers connected to alarm transmission systems."@en ;
  rdfs:label "IEC 60839-7-5:2001"@en ;
  foaf:maker sto:IEC ;
  sto:hasAvailableLanguage lang:eng ;
  sto:hasAvailableLanguage lang:fra ;
  sto:hasEdition "1.0"^^xsd:float ;
  sto:hasFileSize sto:FileSizeIEC_60839_P7_S5 ;
  sto:hasICS sto:ICS_13_320 ;
  sto:hasOfficialResource <https://webstore.iec.ch/publication/3673> ;
  sto:hasPages "13"^^xsd:int ;
  sto:hasPublicationDate "1968-03-01"^^xsd:date ;
  sto:hasPublicationDate "2001-03-09"^^xsd:date ;
  sto:hasPublisher sto:IEC ;
  sto:hasStabilityDate "2018"^^xsd:gYear ;
  sto:hasTag "IEC 60839-7-5:2001"@en ;
  sto:hasTechnicalCommittee sto:TC_79 ;
  sto:hasstatus "Valid" ;
.
sto:IEC_60839_P7_S6_E1
  a owl:NamedIndividual ;
  a sto:Standard ;
  terms:creator sto:IEC ;
  terms:language lang:eng ;
  terms:language lang:fra ;
  terms:title "Alarm systems - Part 7-6: Message formats and protocols for serial data interfaces in alarm transmission systems - Alarm system interfaces employing ITU-T Recommendation V.24/V.28 signalling"@en ;
  rdfs:comment "Specifies the requirements for standard interfaces employing ITU-T V.24/V.28 signalling for communications between the control and indicating equipment of an alarm system and transmission equipment used for remote communications, where the transmission equipment is general purpose equipment. Is intended to be used as interfacing to standard modems, packet switching networks, X.25 PADs, etc."@en ;
  rdfs:label "IEC 60839-7-6:2001"@en ;
  foaf:maker sto:IEC ;
  sto:hasAvailableLanguage lang:eng ;
  sto:hasAvailableLanguage lang:fra ;
  sto:hasEdition "1.0"^^xsd:float ;
  sto:hasFileSize sto:FileSizeIEC_60839_P7_S6 ;
  sto:hasICS sto:ICS_13_320 ;
  sto:hasOfficialResource <https://webstore.iec.ch/publication/3674> ;
  sto:hasPages "9"^^xsd:int ;
  sto:hasPublicationDate "1968-03-01"^^xsd:date ;
  sto:hasPublicationDate "2001-03-09"^^xsd:date ;
  sto:hasPublisher sto:IEC ;
  sto:hasStabilityDate "2018"^^xsd:gYear ;
  sto:hasTag "IEC 60839-7-6:2001"@en ;
  sto:hasTechnicalCommittee sto:TC_79 ;
  sto:hasstatus "Valid" ;
.
sto:IEC_60839_P7_S7_E1
  a owl:NamedIndividual ;
  a sto:Standard ;
  terms:creator sto:IEC ;
  terms:language lang:eng ;
  terms:language lang:fra ;
  terms:title "Alarm systems - Part 7-7: Message formats and protocols for serial data interfaces in alarm transmission systems - Alarm system interfaces for plug-in alarm system transceivers"@en ;
  rdfs:comment "Specifies the requirements for standard interfaces between the control and indicating equipment (CIE) of an alarm system and an alarm system transceiver where the alarm system transceiver is intended to plug into a standard space inside the CIE of the alarm system."@en ;
  rdfs:label "IEC 60839-7-7:2001"@en ;
  foaf:maker sto:IEC ;
  sto:hasAvailableLanguage lang:eng ;
  sto:hasAvailableLanguage lang:fra ;
  sto:hasEdition "1.0"^^xsd:float ;
  sto:hasFileSize sto:FileSizeIEC_60839_P7_S7 ;
  sto:hasICS sto:ICS_13_320 ;
  sto:hasOfficialResource <https://webstore.iec.ch/publication/3675> ;
  sto:hasPages "21"^^xsd:int ;
  sto:hasPublicationDate "1968-03-01"^^xsd:date ;
  sto:hasPublicationDate "2001-03-09"^^xsd:date ;
  sto:hasPublisher sto:IEC ;
  sto:hasStabilityDate "2018"^^xsd:gYear ;
  sto:hasTag "IEC 60839-7-7:2001"@en ;
  sto:hasTechnicalCommittee sto:TC_79 ;
  sto:hasstatus "Valid" ;
.
sto:IEC_60848_E3
  a owl:NamedIndividual ;
  a sto:Standard ;
  terms:creator sto:IEC ;
  terms:language lang:eng ;
  terms:language lang:fra ;
  terms:title "GRAFCET specification language for sequential function charts"@en ;
  rdfs:comment "IEC 60848:2013 defines the GRAFCET specification language for the functional description of the behaviour of the sequential part of a control system. It specifies the symbols and rules for the graphical representation of this language, as well as for its interpretation and has been prepared for automated production systems of industrial applications. This third edition cancels and replaces the second edition published in 2002 and constitutes a global technical revision with the extended definition of the concept of variables introducing: internal variable, input variable and output variable."@en ;
  rdfs:label "IEC 60848:2013"@en ;
  foaf:maker sto:IEC ;
  sto:hasAvailableLanguage lang:eng ;
  sto:hasAvailableLanguage lang:fra ;
  sto:hasEdition "3.0"^^xsd:float ;
  sto:hasFileSize sto:FileSizeIEC_60848 ;
  sto:hasICS sto:ICS_29_020 ;
  sto:hasOfficialResource <https://webstore.iec.ch/publication/3684> ;
  sto:hasPages "109"^^xsd:int ;
  sto:hasPublicationDate "1958-02-13"^^xsd:date ;
  sto:hasPublicationDate "2013-02-27"^^xsd:date ;
  sto:hasPublisher sto:IEC ;
  sto:hasStabilityDate "2020"^^xsd:gYear ;
  sto:hasTag "IEC 60848:2013"@en ;
  sto:hasTechnicalCommittee sto:TC_3 ;
  sto:hasstatus "Valid" ;
.
sto:IEC_60864_P1_E1
  a owl:NamedIndividual ;
  a sto:Standard ;
  terms:creator sto:IEC ;
  terms:language lang:eng ;
  terms:language lang:fra ;
  terms:title "Standardization of interconnections between broadcasting transmitters or transmitter systems and supervisory equipment. Part 1: Interface standards for systems using dedicated interconnections"@en ;
  rdfs:comment "Applies to all classes of transmitters for sound and television broadcasting. Deals with the interface between a transmitter (or system of transmitters) and the supervisory equipment which is intended to remotely monitor and/or control the transmitter(s). Details the interconnections and facilities to be provided with a view to achieving compatibility between different types and makes of transmitters and supervisory equipment."@en ;
  rdfs:label "IEC 60864-1:1986 "@en ;
  foaf:maker sto:IEC ;
  sto:hasAvailableLanguage lang:eng ;
  sto:hasAvailableLanguage lang:fra ;
  sto:hasEdition "1.0"^^xsd:float ;
  sto:hasFileSize sto:FileSizeIEC_60864_P1 ;
  sto:hasICS sto:ICS_33_060_20 ;
  sto:hasICS sto:ICS_33_200 ;
  sto:hasOfficialResource <https://webstore.iec.ch/publication/3727> ;
  sto:hasPages "43"^^xsd:int ;
  sto:hasPublicationDate "1986-01-01"^^xsd:date ;
  sto:hasPublisher sto:IEC ;
  sto:hasStabilityDate "2020"^^xsd:gYear ;
  sto:hasTag "IEC 60864-1:1986 "@en ;
  sto:hasTechnicalCommittee sto:TC_103 ;
  sto:hasstatus "Valid" ;
.
sto:IEC_60864_P2_E1
  a owl:NamedIndividual ;
  a sto:Standard ;
  terms:creator sto:IEC ;
  terms:language lang:eng ;
  terms:language lang:fra ;
  terms:title "Standardization of interconnections between broadcasting transmitters or transmitter systems and supervisory equipment - Part 2: Interface standards for systems using data bus type interconnections"@en ;
  rdfs:comment "Deals with the interface between a transmitter (or system of transmitters) and the supervisory equipment which is entended to remotely monitor and/or control the transmitter(s). It details the interconnections and facilities to be provided with a view to achieving compatibility between different types and makes of transmitters and supervisory equipement."@en ;
  rdfs:comment "Deals with the itnerface between a transmitter (or system of transmitters) and the supervisory equipment which is entended to remotely monitor and/or control the transmitter(s). It details the interconnections and facilities to be provided with a view to achieving compatibility between different types and makes of transmitters and supervisory equipement."@en ;
  rdfs:label "IEC 60864-2:1997"@en ;
  foaf:maker sto:IEC ;
  sto:hasAvailableLanguage lang:eng ;
  sto:hasAvailableLanguage lang:fra ;
  sto:hasEdition "1.0"^^xsd:float ;
  sto:hasFileSize sto:FileSizeIEC_60864_P2 ;
  sto:hasICS sto:ICS_33_060_20 ;
  sto:hasICS sto:ICS_33_200 ;
  sto:hasOfficialResource <https://webstore.iec.ch/publication/3728> ;
  sto:hasPages "79"^^xsd:int ;
  sto:hasPublicationDate "1997-06-17"^^xsd:date ;
  sto:hasPublisher sto:IEC ;
  sto:hasStabilityDate "2020"^^xsd:gYear ;
  sto:hasTag "IEC 60864-2:1997"@en ;
  sto:hasTechnicalCommittee sto:TC_103 ;
  sto:hasstatus "Valid" ;
.
sto:IEC_60870
  a owl:NamedIndividual ;
  a foaf:Document ;
  a sto:Publication ;
  a sto:Standard ;
  terms:creator sto:IEC ;
  rdfs:comment "In electrical engineering and power system automation, the IEC 60870 series define systems used for telecontrol (supervisory control and data acquisition)"@en ;
  rdfs:label "IEC 60870"@en ;
  foaf:maker sto:IEC ;
  sto:hasDBpediaResource <http://dbpedia.org/page/IEC_60870> ;
  sto:hasPublisher sto:IEC ;
  sto:hasWikipediaArticle <https://en.wikipedia.org/wiki/IEC_60870> ;
.
sto:IEC_60870_P2_S1_E2
  a owl:NamedIndividual ;
  a sto:Standard ;
  terms:creator sto:IEC ;
  terms:language lang:eng ;
  terms:language lang:fra ;
  terms:language lang:spa ;
  terms:title "Telecontrol equipment and systems - Part 2: Operating conditions - Section 1: Power supply and electromagnetic compatibility"@en ;
  rdfs:comment "Specifies classes for environmental conditions under which telecontrol equipment has to operate."@en ;
  rdfs:label "IEC 60870-2-1:1995"@en ;
  foaf:maker sto:IEC ;
  sto:hasAvailableLanguage lang:eng ;
  sto:hasAvailableLanguage lang:fra ;
  sto:hasAvailableLanguage lang:spa ;
  sto:hasDBpediaResource <https://dbpedia.org/resource/IEC_60870> ;
  sto:hasEdition "2.0"^^xsd:float ;
  sto:hasFileSize sto:FileSizeIEC_60870_P2_S1 ;
  sto:hasICS sto:ICS_29_020 ;
  sto:hasICS sto:ICS_33_100_10 ;
  sto:hasICS sto:ICS_33_200 ;
  sto:hasOfficialResource <https://webstore.iec.ch/publication/3738> ;
  sto:hasPages "43"^^xsd:int ;
  sto:hasPublicationDate "1995-12-08"^^xsd:date ;
  sto:hasPublisher sto:IEC ;
  sto:hasStabilityDate "2018"^^xsd:gYear ;
  sto:hasTag "IEC 60870-2-1:1995"@en ;
  sto:hasTechnicalCommittee sto:TC_57 ;
  sto:hasWikipediaArticle <https://en.wikipedia.org/wiki/IEC_60870> ;
  sto:hasstatus "Valid" ;
.
sto:IEC_60870_P2_S2_E1
  a owl:NamedIndividual ;
  a sto:Standard ;
  terms:creator sto:IEC ;
  terms:language lang:eng ;
  terms:language lang:fra ;
  terms:language lang:spa ;
  terms:title "Telecontrol equipment and systems - Part 2: Operating conditions -Section 2: Environmental conditions (climatic, mechanical and othernon electrical influences)"@en ;
  rdfs:comment "Applies to telecontrol equipment and systems with coded bit serial data transmission for monitoring and control of geographically wides pread processes. Specifies classes for environmental conditions under which the various components of the systems have to operate."@en ;
  rdfs:label "IEC 60870-2-2:1996"@en ;
  foaf:maker sto:IEC ;
  sto:hasAvailableLanguage lang:eng ;
  sto:hasAvailableLanguage lang:fra ;
  sto:hasAvailableLanguage lang:spa ;
  sto:hasDBpediaResource <https://dbpedia.org/resource/IEC_60870> ;
  sto:hasEdition "1.0"^^xsd:float ;
  sto:hasFileSize sto:FileSizeIEC_60870_P2_S2 ;
  sto:hasICS sto:ICS_29_020 ;
  sto:hasICS sto:ICS_33_200 ;
  sto:hasOfficialResource <https://webstore.iec.ch/publication/3739> ;
  sto:hasPages "33"^^xsd:int ;
  sto:hasPublicationDate "1996-08-19"^^xsd:date ;
  sto:hasPublisher sto:IEC ;
  sto:hasStabilityDate "2018"^^xsd:gYear ;
  sto:hasTag "IEC 60870-2-2:1996"@en ;
  sto:hasTechnicalCommittee sto:TC_57 ;
  sto:hasWikipediaArticle <https://en.wikipedia.org/wiki/IEC_60870> ;
  sto:hasstatus "Valid" ;
.
sto:IEC_60870_P5_S101_E2_1
  a owl:NamedIndividual ;
  a sto:Standard ;
  terms:creator sto:IEC ;
  terms:language lang:eng ;
  terms:title "Telecontrol equipment and systems - Part 5-101: Transmissionprotocols - Companion standard for basic telecontrol tasks"@en ;
  rdfs:comment """IEC 60870-5-101:2003+A1:2015 Applies to telecontrol equipment and systems with coded bit serial data transmission for monitoring and controlling geographically widespread processes. Defines a telecontrol companion standard that enables interoperability among compatible telecontrol equipment. The defined telecontrol companion standard utilizes standards of the IEC 60870-5 series of documents. 
This publication is of high relevance for Smart Grid. This consolidated version consists of the second edition (2003) and its amendment 1 (2015). Therefore, no need to order amendment in addition to this publication."""@en ;
  rdfs:comment "IEC 60870-5-101:2003+A1:2015 Applies to telecontrol equipment and systems with coded bit serial data transmission for monitoring and controlling geographically widespread processes. Defines a telecontrol companion standard that enables interoperability among compatible telecontrol equipment. The defined telecontrol companion standard utilizes standards of the IEC 60870-5 series of documents. This publication is of high relevance for Smart Grid. This consolidated version consists of the second edition (2003) and its amendment 1 (2015). Therefore, no need to order amendment in addition to this publication."@en ;
  rdfs:comment "IEC 60870-5-101:2003+A1:2015 Applies to telecontrol equipment and systems with coded bit serial data transmission for monitoring and controlling geographically widespread processes. Defines a telecontrol companion standard that enables interoperability among compatible telecontrol equipment. The defined telecontrol companion standard utilizes standards of the IEC 60870-5 series of documents. nThis publication is of high relevance for Smart Grid. This consolidated version consists of the second edition (2003) and its amendment 1 (2015). Therefore, no need to order amendment in addition to this publication."@en ;
  rdfs:label "IEC 60870-5-101:2003"@en ;
  foaf:maker sto:IEC ;
  sto:hasAvailableLanguage lang:eng ;
  sto:hasDBpediaResource <https://dbpedia.org/resource/IEC_60870> ;
  sto:hasEdition "2.1"^^xsd:float ;
  sto:hasFileSize sto:FileSizeIEC_60870_P5_S101 ;
  sto:hasICS sto:ICS_33_200 ;
  sto:hasOfficialResource <https://webstore.iec.ch/publication/23822> ;
  sto:hasPages "360"^^xsd:int ;
  sto:hasPublicationDate "2015-11-26"^^xsd:date ;
  sto:hasPublicationDate "2015-11-30"^^xsd:date ;
  sto:hasPublisher sto:IEC ;
  sto:hasStabilityDate "2018"^^xsd:gYear ;
  sto:hasTag "IEC 60870-5-101:2003"@en ;
  sto:hasTechnicalCommittee sto:TC_57 ;
  sto:hasWikipediaArticle <https://en.wikipedia.org/wiki/IEC_60870> ;
  sto:hasstatus "Valid" ;
.
sto:IEC_60870_P5_S102_E1
  a owl:NamedIndividual ;
  a sto:Standard ;
  terms:creator sto:IEC ;
  terms:language lang:eng ;
  terms:language lang:fra ;
  terms:title "Telecontrol equipment and systems - Part 5: Transmission protocols - Section 102: Companion standard for the transmission of integrated totals in electric power systems"@en ;
  rdfs:comment """Standardizes the transmission of integrated totals representing the amount of electrical energy transferred between power utilities, or between a power utility and independent producers on a high voltage or medium voltage network.
This publication is of high relevance for Smart Grid."""@en ;
  rdfs:comment "Standardizes the transmission of integrated totals representing the amount of electrical energy transferred between power utilities, or between a power utility and independent producers on a high voltage or medium voltage network.nThis publication is of high relevance for Smart Grid."@en ;
  rdfs:label "IEC 60870-5-102:1996"@en ;
  foaf:maker sto:IEC ;
  sto:hasAvailableLanguage lang:eng ;
  sto:hasAvailableLanguage lang:fra ;
  sto:hasDBpediaResource <https://dbpedia.org/resource/IEC_60870> ;
  sto:hasEdition "1.0"^^xsd:float ;
  sto:hasFileSize sto:FileSizeIEC_60870_P5_S102 ;
  sto:hasICS sto:ICS_33_200 ;
  sto:hasOfficialResource <https://webstore.iec.ch/publication/3744> ;
  sto:hasPages "99"^^xsd:int ;
  sto:hasPublicationDate "1996-06-18"^^xsd:date ;
  sto:hasPublisher sto:IEC ;
  sto:hasStabilityDate "2018"^^xsd:gYear ;
  sto:hasTag "IEC 60870-5-102:1996"@en ;
  sto:hasTechnicalCommittee sto:TC_57 ;
  sto:hasWikipediaArticle <https://en.wikipedia.org/wiki/IEC_60870> ;
  sto:hasstatus "Valid" ;
.
sto:IEC_60870_P5_S103_E1
  a owl:NamedIndividual ;
  a sto:Standard ;
  terms:creator sto:IEC ;
  terms:language lang:eng ;
  terms:language lang:fra ;
  terms:title "Telecontrol equipment and systems - Part 5-103: Transmission protocols - Companion standard for the informative interface of protection equipment"@en ;
  rdfs:comment """Applies to protection equipment with coded bit serial data transmission for exchanging information with control systems. Defines a companion standard that enables interoperability between protection equipment and devices of a control system in a substation.
This publication is of high relevance for Smart Grid."""@en ;
  rdfs:comment "Applies to protection equipment with coded bit serial data transmission for exchanging information with control systems. Defines a companion standard that enables interoperability between protection equipment and devices of a control system in a substation.nThis publication is of high relevance for Smart Grid."@en ;
  rdfs:label "IEC 60870-5-103:1997"@en ;
  foaf:maker sto:IEC ;
  sto:hasAvailableLanguage lang:eng ;
  sto:hasAvailableLanguage lang:fra ;
  sto:hasDBpediaResource <https://dbpedia.org/resource/IEC_60870> ;
  sto:hasEdition "1.0"^^xsd:float ;
  sto:hasFileSize sto:FileSizeIEC_60870_P5_S103 ;
  sto:hasICS sto:ICS_33_200 ;
  sto:hasOfficialResource <https://webstore.iec.ch/publication/3745> ;
  sto:hasPages "203"^^xsd:int ;
  sto:hasPublicationDate "1997-12-11"^^xsd:date ;
  sto:hasPublisher sto:IEC ;
  sto:hasStabilityDate "2018"^^xsd:gYear ;
  sto:hasTag "IEC 60870-5-103:1997"@en ;
  sto:hasTechnicalCommittee sto:TC_57 ;
  sto:hasWikipediaArticle <https://en.wikipedia.org/wiki/IEC_60870> ;
  sto:hasstatus "Valid" ;
.
sto:IEC_60870_P5_S104_E2_1
  a owl:NamedIndividual ;
  a sto:Standard ;
  terms:creator sto:IEC ;
  terms:language lang:eng ;
  terms:language lang:fra ;
  terms:title "Telecontrol equipment and systems - Part 5-104: Transmission protocols - Network access for IEC 60870-5-101 using standardtransport profiles"@en ;
  rdfs:comment """IEC 60870-5-104:2006+A1:2016 Defines a telecontrol companion standard that enables interoperability among compatible telecontrol equipment. Applies to telecontrol equipment and systems with coded bit serial data transmission for monitoring and controlling geographically widespread processes. 
This publication is of high relevance for Smart Grid. This consolidated version consists of the second edition (2006) and its amendment 1 (2012). Therefore, no need to order amendment in addition to this publication."""@en ;
  rdfs:comment "IEC 60870-5-104:2006+A1:2016 Defines a telecontrol companion standard that enables interoperability among compatible telecontrol equipment. Applies to telecontrol equipment and systems with coded bit serial data transmission for monitoring and controlling geographically widespread processes. nThis publication is of high relevance for Smart Grid. This consolidated version consists of the second edition (2006) and its amendment 1 (2012). Therefore, no need to order amendment in addition to this publication."@en ;
  rdfs:label "IEC 60870-5-104:2006"@en ;
  foaf:maker sto:IEC ;
  sto:hasAvailableLanguage lang:eng ;
  sto:hasAvailableLanguage lang:fra ;
  sto:hasDBpediaResource <https://dbpedia.org/resource/IEC_60870> ;
  sto:hasEdition "2.1"^^xsd:float ;
  sto:hasFileSize sto:FileSizeIEC_60870_P5_S104 ;
  sto:hasICS sto:ICS_33_200 ;
  sto:hasOfficialResource <https://webstore.iec.ch/publication/25035> ;
  sto:hasPages "281"^^xsd:int ;
  sto:hasPublicationDate "2016-06-07"^^xsd:date ;
  sto:hasPublisher sto:IEC ;
  sto:hasStabilityDate "2018"^^xsd:gYear ;
  sto:hasTag "IEC 60870-5-104:2006"@en ;
  sto:hasTechnicalCommittee sto:TC_57 ;
  sto:hasWikipediaArticle <https://en.wikipedia.org/wiki/IEC_60870> ;
  sto:hasstatus "Valid" ;
.
sto:IEC_60870_P5_S1_E1
  a owl:NamedIndividual ;
  a sto:Standard ;
  terms:creator sto:IEC ;
  terms:language lang:eng ;
  terms:language lang:fra ;
  terms:title "Telecontrol equipment and systems. Part 5: Transmission protocols - Section One: Transmission frame formats"@en ;
  rdfs:comment "Covers asynchronous data transmission with half duplex and duplex link protocols operating with window size one for message transfers. Specifies the basic requirements for services to be provided by the link plus physical layers, for telecontrol applications. In particular it specifies standards on coding, formatting and synchronizing data frames of variable and filed lengths which meet specified data integrity requirements."@en ;
  rdfs:label "IEC 60870-5-1:1990"@en ;
  foaf:maker sto:IEC ;
  sto:hasAvailableLanguage lang:eng ;
  sto:hasAvailableLanguage lang:fra ;
  sto:hasDBpediaResource <https://dbpedia.org/resource/IEC_60870> ;
  sto:hasEdition "1.0"^^xsd:float ;
  sto:hasFileSize sto:FileSizeIEC_60870_P5_S1 ;
  sto:hasICS sto:ICS_33_200 ;
  sto:hasOfficialResource <https://webstore.iec.ch/publication/3742> ;
  sto:hasPages "79"^^xsd:int ;
  sto:hasPublicationDate "1990-02-01"^^xsd:date ;
  sto:hasPublisher sto:IEC ;
  sto:hasStabilityDate "2018"^^xsd:gYear ;
  sto:hasTag "IEC 60870-5-1:1990"@en ;
  sto:hasTechnicalCommittee sto:TC_57 ;
  sto:hasWikipediaArticle <https://en.wikipedia.org/wiki/IEC_60870> ;
  sto:hasstatus "Valid" ;
.
sto:IEC_60870_P5_S2_E1
  a owl:NamedIndividual ;
  a sto:Standard ;
  terms:creator sto:IEC ;
  terms:language lang:eng ;
  terms:language lang:fra ;
  terms:title "Telecontrol equipment and systems - Part 5: Transmission protocols - Section 2: Link transmission procedures"@en ;
  rdfs:comment """Applies to telecontrol equipment and systems with coded bit serial data transmission for monitoring and controlling geographically widespread processes. 
This publication is of high relevance for Smart Grid."""@en ;
  rdfs:comment "Applies to telecontrol equipment and systems with coded bit serial data transmission for monitoring and controlling geographically widespread processes. nThis publication is of high relevance for Smart Grid."@en ;
  rdfs:label "IEC 60870-5-2:1992"@en ;
  foaf:maker sto:IEC ;
  sto:hasAvailableLanguage lang:eng ;
  sto:hasAvailableLanguage lang:fra ;
  sto:hasDBpediaResource <https://dbpedia.org/resource/IEC_60870> ;
  sto:hasEdition "1.0"^^xsd:float ;
  sto:hasFileSize sto:FileSizeIEC_60870_P5_S2 ;
  sto:hasICS sto:ICS_33_200 ;
  sto:hasOfficialResource <https://webstore.iec.ch/publication/3747> ;
  sto:hasPages "99"^^xsd:int ;
  sto:hasPublicationDate "1992-04-30"^^xsd:date ;
  sto:hasPublisher sto:IEC ;
  sto:hasStabilityDate "2018"^^xsd:gYear ;
  sto:hasTag "IEC 60870-5-2:1992"@en ;
  sto:hasTechnicalCommittee sto:TC_57 ;
  sto:hasWikipediaArticle <https://en.wikipedia.org/wiki/IEC_60870> ;
  sto:hasstatus "Valid" ;
.
sto:IEC_60870_P5_S3_E1
  a owl:NamedIndividual ;
  a sto:Standard ;
  terms:creator sto:IEC ;
  terms:language lang:eng ;
  terms:language lang:fra ;
  terms:title "Telecontrol equipment and systems - Part 5: Transmission protocols - Section 3: General structure of application data"@en ;
  rdfs:comment """Applies to telecontrol equipment and systems with coded bit serial data transmission for monitoring and controlling geographically widespread processes; specifies rules for structuring application data units in transmission frames of telecontrol systems.
This publication is of high relevance for Smart Grid."""@en ;
  rdfs:comment "Applies to telecontrol equipment and systems with coded bit serial data transmission for monitoring and controlling geographically widespread processes; specifies rules for structuring application data units in transmission frames of telecontrol systems.nThis publication is of high relevance for Smart Grid."@en ;
  rdfs:label "IEC 60870-5-3:1992"@en ;
  foaf:maker sto:IEC ;
  sto:hasAvailableLanguage lang:eng ;
  sto:hasAvailableLanguage lang:fra ;
  sto:hasDBpediaResource <https://dbpedia.org/resource/IEC_60870> ;
  sto:hasEdition "1.0"^^xsd:float ;
  sto:hasFileSize sto:FileSizeIEC_60870_P5_S3 ;
  sto:hasICS sto:ICS_33_200 ;
  sto:hasOfficialResource <https://webstore.iec.ch/publication/3748> ;
  sto:hasPages "43"^^xsd:int ;
  sto:hasPublicationDate "1992-09-29"^^xsd:date ;
  sto:hasPublisher sto:IEC ;
  sto:hasStabilityDate "2018"^^xsd:gYear ;
  sto:hasTag "IEC 60870-5-3:1992"@en ;
  sto:hasTechnicalCommittee sto:TC_57 ;
  sto:hasWikipediaArticle <https://en.wikipedia.org/wiki/IEC_60870> ;
  sto:hasstatus "Valid" ;
.
sto:IEC_60870_P5_S4_E1
  a owl:NamedIndividual ;
  a sto:Standard ;
  terms:creator sto:IEC ;
  terms:language lang:eng ;
  terms:language lang:fra ;
  terms:title "Telecontrol equipment and systems - Part 5: Transmission protocols - Section 4: Definition and coding of application information elements"@en ;
  rdfs:comment """Gives rules for defining information elements and presents a set of information elements, in particular of digital and analog process variables frequently used in telecontrol applications. 
This publication is of high relevance for Smart Grid."""@en ;
  rdfs:comment "Gives rules for defining information elements and presents a set of information elements, in particular of digital and analog process variables frequently used in telecontrol applications. nThis publication is of high relevance for Smart Grid."@en ;
  rdfs:label "IEC 60870-5-4:1993"@en ;
  foaf:maker sto:IEC ;
  sto:hasAvailableLanguage lang:eng ;
  sto:hasAvailableLanguage lang:fra ;
  sto:hasDBpediaResource <https://dbpedia.org/resource/IEC_60870> ;
  sto:hasEdition "1.0"^^xsd:float ;
  sto:hasFileSize sto:FileSizeIEC_60870_P5_S4 ;
  sto:hasICS sto:ICS_33_200 ;
  sto:hasOfficialResource <https://webstore.iec.ch/publication/3749> ;
  sto:hasPages "45"^^xsd:int ;
  sto:hasPublicationDate "1993-08-06"^^xsd:date ;
  sto:hasPublisher sto:IEC ;
  sto:hasStabilityDate "2018"^^xsd:gYear ;
  sto:hasTag "IEC 60870-5-4:1993"@en ;
  sto:hasTechnicalCommittee sto:TC_57 ;
  sto:hasWikipediaArticle <https://en.wikipedia.org/wiki/IEC_60870> ;
  sto:hasstatus "Valid" ;
.
sto:IEC_60870_P5_S5_E1
  a owl:NamedIndividual ;
  a sto:Standard ;
  terms:creator sto:IEC ;
  terms:language lang:eng ;
  terms:language lang:fra ;
  terms:title "Telecontrol equipment and systems - Part 5: Transmission protocols - Section 5: Basic application functions"@en ;
  rdfs:comment """Applies to telecontrol equipment and systems with coded bit serial data transmission for monitoring and controlling geographically widespread processes. It defines a telecontrol companion standard that enables interoperability among compatible telecontrol equipment. 
This publication is of high relevance for Smart Grid."""@en ;
  rdfs:comment "Applies to telecontrol equipment and systems with coded bit serial data transmission for monitoring and controlling geographically widespread processes. It defines a telecontrol companion standard that enables interoperability among compatible telecontrol equipment. nThis publication is of high relevance for Smart Grid."@en ;
  rdfs:label "IEC 60870-5-5:1995"@en ;
  foaf:maker sto:IEC ;
  sto:hasAvailableLanguage lang:eng ;
  sto:hasAvailableLanguage lang:fra ;
  sto:hasDBpediaResource <https://dbpedia.org/resource/IEC_60870> ;
  sto:hasEdition "1.0"^^xsd:float ;
  sto:hasFileSize sto:FileSizeIEC_60870_P5_S5 ;
  sto:hasICS sto:ICS_33_200 ;
  sto:hasOfficialResource <https://webstore.iec.ch/publication/3750> ;
  sto:hasPages "101"^^xsd:int ;
  sto:hasPublicationDate "1995-06-04"^^xsd:date ;
  sto:hasPublisher sto:IEC ;
  sto:hasStabilityDate "2018"^^xsd:gYear ;
  sto:hasTag "IEC 60870-5-5:1995"@en ;
  sto:hasTechnicalCommittee sto:TC_57 ;
  sto:hasWikipediaArticle <https://en.wikipedia.org/wiki/IEC_60870> ;
  sto:hasstatus "Valid" ;
.
sto:IEC_60870_P5_S6_E1
  a owl:NamedIndividual ;
  a sto:Standard ;
  terms:creator sto:IEC ;
  terms:language lang:eng ;
  terms:language lang:fra ;
  terms:title "Telecontrol equipment and systems - Part 5-6: Guidelines for conformance testing for the IEC 60870-5 companion standards"@en ;
  rdfs:comment "IEC 60870-5-6:2006 Specifies methods for conformance testing of telecontrol equipment, amongst substation automation systems and telecontrol systems, including front-end functions of SCADA. Facilitates interoperability by providing a standard method of testing protocol implementations. Is expected to minimize the risk of non-interoperability."@en ;
  rdfs:label "IEC 60870-5-6:2006"@en ;
  foaf:maker sto:IEC ;
  sto:hasAvailableLanguage lang:eng ;
  sto:hasAvailableLanguage lang:fra ;
  sto:hasDBpediaResource <https://dbpedia.org/resource/IEC_60870> ;
  sto:hasEdition "1.0"^^xsd:float ;
  sto:hasFileSize sto:FileSizeIEC_60870_P5_S6 ;
  sto:hasICS sto:ICS_33_200 ;
  sto:hasOfficialResource <https://webstore.iec.ch/publication/3751> ;
  sto:hasPages "46"^^xsd:int ;
  sto:hasPublicationDate "2006-03-08"^^xsd:date ;
  sto:hasPublisher sto:IEC ;
  sto:hasStabilityDate "2018"^^xsd:gYear ;
  sto:hasTag "IEC 60870-5-6:2006"@en ;
  sto:hasTechnicalCommittee sto:TC_57 ;
  sto:hasWikipediaArticle <https://en.wikipedia.org/wiki/IEC_60870> ;
  sto:hasstatus "Valid" ;
.
sto:IEC_60870_P6_S2_E1
  a owl:NamedIndividual ;
  a sto:Standard ;
  terms:creator sto:IEC ;
  terms:language lang:eng ;
  terms:language lang:fra ;
  terms:title "Telecontrol equipment and systems - Part 6: Telecontrol protocols compatible with ISO standards and ITU-T recommendations - Section 2: Use of basic standards (OSI layers 1-4)"@en ;
  rdfs:comment """Considers the standards related to layers 1-4 of the OSI reference model and describes the role and the functions carried out by each layer.
This publication is of high relevance for Smart Grid."""@en ;
  rdfs:comment "Considers the standards related to layers 1-4 of the OSI reference model and describes the role and the functions carried out by each layer.nThis publication is of high relevance for Smart Grid."@en ;
  rdfs:label "IEC 60870-6-2:1995"@en ;
  foaf:maker sto:IEC ;
  sto:hasAvailableLanguage lang:eng ;
  sto:hasAvailableLanguage lang:fra ;
  sto:hasDBpediaResource <https://dbpedia.org/resource/IEC_60870> ;
  sto:hasEdition "1.0"^^xsd:float ;
  sto:hasFileSize sto:FileSizeIEC_60870_P6_S2 ;
  sto:hasICS sto:ICS_33_200 ;
  sto:hasOfficialResource <https://webstore.iec.ch/publication/3757> ;
  sto:hasPages "83"^^xsd:int ;
  sto:hasPublicationDate "1995-10-31"^^xsd:date ;
  sto:hasPublisher sto:IEC ;
  sto:hasStabilityDate "2018"^^xsd:gYear ;
  sto:hasTag "IEC 60870-6-2:1995"@en ;
  sto:hasTechnicalCommittee sto:TC_57 ;
  sto:hasWikipediaArticle <https://en.wikipedia.org/wiki/IEC_60870> ;
  sto:hasstatus "Valid" ;
.
sto:IEC_60870_P6_S501_E1
  a owl:NamedIndividual ;
  a sto:Standard ;
  terms:creator sto:IEC ;
  terms:language lang:eng ;
  terms:language lang:fra ;
  terms:title "Telecontrol equipment and systems - Part 6: Telecontrol protocols compatible with ISO standards and ITU-T recommendations - Section 501: TASE.1 Service definitions"@en ;
  rdfs:comment """Defines the services provided by a telecontrol specific application-service-element - the Telecontrol Application Service Element No. 1 (TASE.1) - for the exchange of process data in telecontrol systems.
This publication is of high relevance for Smart Grid."""@en ;
  rdfs:comment "Defines the services provided by a telecontrol specific application-service-element - the Telecontrol Application Service Element No. 1 (TASE.1) - for the exchange of process data in telecontrol systems.nThis publication is of high relevance for Smart Grid."@en ;
  rdfs:label "IEC 60870-6-501:1995"@en ;
  foaf:maker sto:IEC ;
  sto:hasAvailableLanguage lang:eng ;
  sto:hasAvailableLanguage lang:fra ;
  sto:hasDBpediaResource <https://dbpedia.org/resource/IEC_60870> ;
  sto:hasEdition "1.0"^^xsd:float ;
  sto:hasFileSize sto:FileSizeIEC_60870_P6_S501 ;
  sto:hasICS sto:ICS_33_200 ;
  sto:hasOfficialResource <https://webstore.iec.ch/publication/3758> ;
  sto:hasPages "170"^^xsd:int ;
  sto:hasPublicationDate "1995-12-18"^^xsd:date ;
  sto:hasPublisher sto:IEC ;
  sto:hasStabilityDate "2018"^^xsd:gYear ;
  sto:hasTag "IEC 60870-6-501:1995"@en ;
  sto:hasTechnicalCommittee sto:TC_57 ;
  sto:hasWikipediaArticle <https://en.wikipedia.org/wiki/IEC_60870> ;
  sto:hasstatus "Valid" ;
.
sto:IEC_60870_P6_S502_E1
  a owl:NamedIndividual ;
  a sto:Standard ;
  terms:creator sto:IEC ;
  terms:language lang:eng ;
  terms:language lang:fra ;
  terms:title "Telecontrol equipment and systems - Part 6: Telecontrol protocols compatible with ISO standards and ITU-T recommendations - Section 502: TASE.1 Protocol definitions"@en ;
  rdfs:comment """Specifies the protocol for the services provided by an application-service-element - the Telecontrol Application Service Element No. 1 (TASE.1) - to support the exchange of process data between telecontrol systems.
This publication is of high relevance for Smart Grid."""@en ;
  rdfs:comment "Specifies the protocol for the services provided by an application-service-element - the Telecontrol Application Service Element No. 1 (TASE.1) - to support the exchange of process data between telecontrol systems.nThis publication is of high relevance for Smart Grid."@en ;
  rdfs:label "IEC 60870-6-502:1995"@en ;
  foaf:maker sto:IEC ;
  sto:hasAvailableLanguage lang:eng ;
  sto:hasAvailableLanguage lang:fra ;
  sto:hasDBpediaResource <https://dbpedia.org/resource/IEC_60870> ;
  sto:hasEdition "1.0"^^xsd:float ;
  sto:hasFileSize sto:FileSizeIEC_60870_P6_S502 ;
  sto:hasICS sto:ICS_33_200 ;
  sto:hasOfficialResource <https://webstore.iec.ch/publication/3759> ;
  sto:hasPages "57"^^xsd:int ;
  sto:hasPublicationDate "1995-12-05"^^xsd:date ;
  sto:hasPublisher sto:IEC ;
  sto:hasStabilityDate "2018"^^xsd:gYear ;
  sto:hasTag "IEC 60870-6-502:1995"@en ;
  sto:hasTechnicalCommittee sto:TC_57 ;
  sto:hasWikipediaArticle <https://en.wikipedia.org/wiki/IEC_60870> ;
  sto:hasstatus "Valid" ;
.
sto:IEC_60870_P6_S503_E3
  a owl:NamedIndividual ;
  a sto:Standard ;
  terms:creator sto:IEC ;
  terms:language lang:eng ;
  terms:language lang:fra ;
  terms:title "Telecontrol equipment and systems - Part 6-503: Telecontrol protocols compatible with ISO standards and ITU-T recommendations - TASE.2 Services and protocol"@en ;
  rdfs:comment "IEC 60870-6-503:2014 specifies a method of exchanging time-critical control centre data through wide-area and local-area networks using a full ISO compliant protocol stack. It contains provisions for supporting both centralized and distributed architectures. This standard includes the exchange of real-time data indications, control operations, time-series data, scheduling and accounting information, remote program control and event notification. This new edition includes the following significant technical changes with respect to the previous edition: - certain objects were made informative; - services associated with the informative objects were made informative; - certain TASE.2 conformance blocks were made out-of-scope."@en ;
  rdfs:comment "IEC 60870-6-503:2014 specifies a method of exchanging time-critical control centre data through wide-area and local-area networks using a full ISO compliant protocol stack. It contains provisions for supporting both centralized and distributed architectures. This standard includes the exchange of real-time data indications, control operations, time-series data, scheduling and accounting information, remote program control and event notification. This new edition includes the following significant technical changes with respect to the previous edition:n- certain objects were made informative;n- services associated with the informative objects were made informative;n- certain TASE.2 conformance blocks were made out-of-scope."@en ;
  rdfs:label "IEC 60870-6-503:2014"@en ;
  foaf:maker sto:IEC ;
  sto:hasAvailableLanguage lang:eng ;
  sto:hasAvailableLanguage lang:fra ;
  sto:hasDBpediaResource <https://dbpedia.org/resource/IEC_60870> ;
  sto:hasEdition "3.0"^^xsd:float ;
  sto:hasFileSize sto:FileSizeIEC_60870_P6_S503 ;
  sto:hasICS sto:ICS_33_200 ;
  sto:hasOfficialResource <https://webstore.iec.ch/publication/3760> ;
  sto:hasPages "310"^^xsd:int ;
  sto:hasPublicationDate "2014-07-15"^^xsd:date ;
  sto:hasPublisher sto:IEC ;
  sto:hasStabilityDate "2018"^^xsd:gYear ;
  sto:hasTag "IEC 60870-6-503:2014"@en ;
  sto:hasTechnicalCommittee sto:TC_57 ;
  sto:hasWikipediaArticle <https://en.wikipedia.org/wiki/IEC_60870> ;
  sto:hasstatus "Valid" ;
.
sto:IEC_60870_P6_S601_E1
  a owl:NamedIndividual ;
  a sto:Standard ;
  terms:creator sto:IEC ;
  terms:language lang:eng ;
  terms:language lang:fra ;
  terms:title "Telecontrol equipment and systems - Part 6: Telecontrol protocol s compatible with ISO standards and ITU-T recommendations - Sect ion 601: Functional profile for providing the connection-oriente d transport service in an end system connected via permanent acc ess to a packet switched data network"@en ;
  rdfs:comment """Defines the functional profile which provides the connection-oriented transport service in an end system connected via permanent access to a packet switched data network.
This publication is of high relevance for Smart Grid."""@en ;
  rdfs:comment "Defines the functional profile which provides the connection-oriented transport service in an end system connected via permanent access to a packet switched data network.nThis publication is of high relevance for Smart Grid."@en ;
  rdfs:label "IEC 60870-6-601:1994"@en ;
  foaf:maker sto:IEC ;
  sto:hasAvailableLanguage lang:eng ;
  sto:hasAvailableLanguage lang:fra ;
  sto:hasDBpediaResource <https://dbpedia.org/resource/IEC_60870> ;
  sto:hasEdition "1.0"^^xsd:float ;
  sto:hasFileSize sto:FileSizeIEC_60870_P6_S601 ;
  sto:hasICS sto:ICS_33_200 ;
  sto:hasOfficialResource <https://webstore.iec.ch/publication/3765> ;
  sto:hasPages "25"^^xsd:int ;
  sto:hasPublicationDate "1994-12-21"^^xsd:date ;
  sto:hasPublisher sto:IEC ;
  sto:hasStabilityDate "2018"^^xsd:gYear ;
  sto:hasTag "IEC 60870-6-601:1994"@en ;
  sto:hasTechnicalCommittee sto:TC_57 ;
  sto:hasWikipediaArticle <https://en.wikipedia.org/wiki/IEC_60870> ;
  sto:hasstatus "Valid" ;
.
sto:IEC_60870_P6_S701_E1
  a owl:NamedIndividual ;
  a sto:Standard ;
  terms:creator sto:IEC ;
  terms:language lang:eng ;
  terms:language lang:fra ;
  terms:title "Telecontrol equipment and systems - Part 6-701: Telecontrol protocols compatible with ISO standards and ITU-T recommendations - Functional profile for providing the TASE.1 application service in end systems"@en ;
  rdfs:comment """Describes the functional profile which defines the provision of the TASE.1 communication services between two control centre end systems.
This publication is of high relevance for Smart Grid"""@en ;
  rdfs:comment "Describes the functional profile which defines the provision of the TASE.1 communication services between two control centre end systems.nThis publication is of high relevance for Smart Grid"@en ;
  rdfs:label "IEC 60870-6-701:1998"@en ;
  foaf:maker sto:IEC ;
  sto:hasAvailableLanguage lang:eng ;
  sto:hasAvailableLanguage lang:fra ;
  sto:hasDBpediaResource <https://dbpedia.org/resource/IEC_60870> ;
  sto:hasEdition "1.0"^^xsd:float ;
  sto:hasFileSize sto:FileSizeIEC_60870_P6_S701 ;
  sto:hasICS sto:ICS_33_200 ;
  sto:hasOfficialResource <https://webstore.iec.ch/publication/3767> ;
  sto:hasPages "37"^^xsd:int ;
  sto:hasPublicationDate "1998-08-07"^^xsd:date ;
  sto:hasPublisher sto:IEC ;
  sto:hasStabilityDate "2018"^^xsd:gYear ;
  sto:hasTag "IEC 60870-6-701:1998"@en ;
  sto:hasTechnicalCommittee sto:TC_57 ;
  sto:hasWikipediaArticle <https://en.wikipedia.org/wiki/IEC_60870> ;
  sto:hasstatus "Valid" ;
.
sto:IEC_60870_P6_S702_E2
  a owl:NamedIndividual ;
  a sto:Standard ;
  terms:creator sto:IEC ;
  terms:language lang:eng ;
  terms:language lang:fra ;
  terms:title "Telecontrol equipment and systems - Part 6-702: Telecontrol protocols compatible with ISO standards and ITU-T recommendations - Functional profile for providing the TASE.2 application service in end systems"@en ;
  rdfs:comment """IEC 60870-6-702:2014 is a functional profile (FP) and defines the provision of the TASE.2 communications services between two control centre end systems. It is supported by the transport services implemented in accordance with transport-profiles defined for the type of network that interconnects the control centre end systems. The main changes with respect to the previous edition are listed below:
- certain objects were moved from being normative to informative
- certain TASE.2 conformance blocks have been made out-of-scope. These changes were made in order to remove TASE.2 blocks that were seldom used and whose capabilities are typically implemented by some other means besides TASE.2. This was done to promote interoperability of implementations from an application perspective."""@en ;
  rdfs:comment "IEC 60870-6-702:2014 is a functional profile (FP) and defines the provision of the TASE.2 communications services between two control centre end systems. It is supported by the transport services implemented in accordance with transport-profiles defined for the type of network that interconnects the control centre end systems. The main changes with respect to the previous edition are listed below:n- certain objects were moved from being normative to informative;n- certain TASE.2 conformance blocks have been made out-of-scope. These changes were made in order to remove TASE.2 blocks that were seldom used and whose capabilities are typically implemented by some other means besides TASE.2. This was done to promote interoperability of implementations from an application perspective."@en ;
  rdfs:label "IEC 60870-6-702:2014"@en ;
  foaf:maker sto:IEC ;
  sto:hasAvailableLanguage lang:eng ;
  sto:hasAvailableLanguage lang:fra ;
  sto:hasDBpediaResource <https://dbpedia.org/resource/IEC_60870> ;
  sto:hasEdition "2.0"^^xsd:float ;
  sto:hasFileSize sto:FileSizeIEC_60870_P6_S702 ;
  sto:hasICS sto:ICS_33_200 ;
  sto:hasOfficialResource <https://webstore.iec.ch/publication/3768> ;
  sto:hasPages "71"^^xsd:int ;
  sto:hasPublicationDate "2014-07-15"^^xsd:date ;
  sto:hasPublisher sto:IEC ;
  sto:hasStabilityDate "2018"^^xsd:gYear ;
  sto:hasTag "IEC 60870-6-702:2014"@en ;
  sto:hasTechnicalCommittee sto:TC_57 ;
  sto:hasWikipediaArticle <https://en.wikipedia.org/wiki/IEC_60870> ;
  sto:hasstatus "Valid" ;
.
sto:IEC_60870_P6_S802_E3
  a owl:NamedIndividual ;
  a sto:Standard ;
  terms:creator sto:IEC ;
  terms:language lang:eng ;
  terms:language lang:fra ;
  terms:title "Telecontrol equipment and systems - Part 6-802: Telecontrol protocols compatible with ISO standards and ITU-T recommendations - TASE.2 Object models"@en ;
  rdfs:comment "IEC 60870-6-802:2014 specifies a method of exchanging time-critical control centre data through wide-area and local-area networks using a full ISO compliant protocol stack. It contains provisions for supporting both centralized and distributed architectures. The standard includes the exchange of real-time data indications, control operations, time series data, scheduling and accounting information, remote program control and event notification. This new edition includes the following significant technical changes with respect to the previous edition: -certain objects have been changed from informative to normative; - certain TASE.2 conformance blocks have been made out of scope."@en ;
  rdfs:comment "IEC 60870-6-802:2014 specifies a method of exchanging time-critical control centre data through wide-area and local-area networks using a full ISO compliant protocol stack. It contains provisions for supporting both centralized and distributed architectures. The standard includes the exchange of real-time data indications, control operations, time series data, scheduling and accounting information, remote program control and event notification. This new edition includes the following significant technical changes with respect to the previous edition:n- certain objects have been changed from informative to normative;n- certain TASE.2 conformance blocks have been made out of scope."@en ;
  rdfs:label "IEC 60870-6-802:2014"@en ;
  foaf:maker sto:IEC ;
  sto:hasAvailableLanguage lang:eng ;
  sto:hasAvailableLanguage lang:fra ;
  sto:hasDBpediaResource <https://dbpedia.org/resource/IEC_60870> ;
  sto:hasEdition "3.0"^^xsd:float ;
  sto:hasFileSize sto:FileSizeIEC_60870_P6_S802 ;
  sto:hasICS sto:ICS_33_200 ;
  sto:hasOfficialResource <https://webstore.iec.ch/publication/3769> ;
  sto:hasPages "188"^^xsd:int ;
  sto:hasPublicationDate "2014-07-15"^^xsd:date ;
  sto:hasPublisher sto:IEC ;
  sto:hasStabilityDate "2019"^^xsd:gYear ;
  sto:hasTag "IEC 60870-6-802:2014"@en ;
  sto:hasTechnicalCommittee sto:TC_57 ;
  sto:hasWikipediaArticle <https://en.wikipedia.org/wiki/IEC_60870> ;
  sto:hasstatus "Valid" ;
.
sto:IEC_60904
  a owl:NamedIndividual ;
  a foaf:Document ;
  a sto:Publication ;
  a sto:Standard ;
  terms:creator sto:IEC ;
  rdfs:comment "Photovoltaic devices"@en ;
  rdfs:label "IEC 60904"@en ;
  foaf:maker sto:IEC ;
  sto:hasOfficialResource <https://webstore.iec.ch/publication/3881> ;
  sto:hasPublicationDate "2017-05-18"^^xsd:date ;
  sto:hasPublisher sto:IEC ;
.
sto:IEC_60946_E1
  a owl:NamedIndividual ;
  a sto:Standard ;
  terms:creator sto:IEC ;
  terms:language lang:eng ;
  terms:language lang:fra ;
  terms:title "Binary direct voltage signals for process measurement and control systems"@en ;
  rdfs:comment "Applies to non-multiplexed two wire binary direct voltage signals of nominal 24 V level that are used in industrial-process measurement and control systems to transmit information between elements of systems."@en ;
  rdfs:label "IEC 60946:1988"@en ;
  foaf:maker sto:IEC ;
  sto:hasAvailableLanguage lang:eng ;
  sto:hasAvailableLanguage lang:fra ;
  sto:hasEdition "1.0"^^xsd:float ;
  sto:hasFileSize sto:FileSizeIEC_60946 ;
  sto:hasICS sto:ICS_25_040_40 ;
  sto:hasOfficialResource <https://webstore.iec.ch/publication/3961> ;
  sto:hasPages "13"^^xsd:int ;
  sto:hasPublicationDate "1988-09-29"^^xsd:date ;
  sto:hasPublisher sto:IEC ;
  sto:hasStabilityDate "2018"^^xsd:gYear ;
  sto:hasTag "IEC 60946:1988"@en ;
  sto:hasTechnicalCommittee sto:TC_65 ;
  sto:hasstatus "Valid" ;
.
sto:IEC_61000_P6_S2_E3
  a owl:NamedIndividual ;
  a sto:Standard ;
  terms:creator sto:IEC ;
  terms:language lang:eng ;
  terms:title "Electromagnetic compatibility (EMC) - Part 6-2: Generic standards - Immunity standard for industrial environments"@en ;
  rdfs:comment """IEC 61000-6-2:2016 RLV contains the International Standard and its Redline version. The Redline version is available in English only. The Redline version provides you with a quick and easy way to compare all the changes between this standard and its previous edition. The Redline version is not an official IEC Standard, only the current version of the standard is to be considered the official document.
IEC 61000-6-2:2016 for EMC immunity requirements applies to electrical and electronic equipment intended for use in industrial locations, as described below. Immunity requirements in the frequency range 0 Hz to 400 GHz are covered. No tests need to be performed at frequencies where no requirements are specified. This generic EMC immunity standard is applicable if no relevant dedicated product or product-family EMC immunity standard exists. This third edition cancels and replaces the second edition published in 2005. This edition constitutes a technical revision."""@en ;
  rdfs:comment "IEC 61000-6-2:2016 RLV contains the International Standard and its Redline version. The Redline version is available in English only. The Redline version provides you with a quick and easy way to compare all the changes between this standard and its previous edition. The Redline version is not an official IEC Standard, only the current version of the standard is to be considered the official document. IEC 61000-6-2:2016 for EMC immunity requirements applies to electrical and electronic equipment intended for use in industrial locations, as described below. Immunity requirements in the frequency range 0 Hz to 400 GHz are covered. No tests need to be performed at frequencies where no requirements are specified. This generic EMC immunity standard is applicable if no relevant dedicated product or product-family EMC immunity standard exists. This third edition cancels and replaces the second edition published in 2005. This edition constitutes a technical revision."@en ;
  rdfs:comment "IEC 61000-6-2:2016 RLV contains the International Standard and its Redline version. The Redline version is available in English only. The Redline version provides you with a quick and easy way to compare all the changes between this standard and its previous edition. The Redline version is not an official IEC Standard, only the current version of the standard is to be considered the official document.nIEC 61000-6-2:2016 for EMC immunity requirements applies to electrical and electronic equipment intended for use in industrial locations, as described below. Immunity requirements in the frequency range 0 Hz to 400 GHz are covered. No tests need to be performed at frequencies where no requirements are specified. This generic EMC immunity standard is applicable if no relevant dedicated product or product-family EMC immunity standard exists. This third edition cancels and replaces the second edition published in 2005. This edition constitutes a technical revision."@en ;
  rdfs:label "IEC 61000-6-2:2016"@en ;
  foaf:maker sto:IEC ;
  sto:hasAvailableLanguage lang:eng ;
  sto:hasEdition "3.0"^^xsd:float ;
  sto:hasFileSize sto:FileSizeIEC_61000_P6_S2 ;
  sto:hasICS sto:ICS_33_100_20 ;
  sto:hasOfficialResource <https://webstore.iec.ch/publication/25629> ;
  sto:hasPages "57"^^xsd:int ;
  sto:hasPublicationDate "2016-08-10"^^xsd:date ;
  sto:hasPublisher sto:IEC ;
  sto:hasStabilityDate "2020"^^xsd:gYear ;
  sto:hasTag " IEC 61000-6-2:2016 "@en ;
  sto:hasTechnicalCommittee sto:TC_77 ;
  sto:hasstatus "Redline version" ;
.
sto:IEC_61010_P2_S012_E1
  a owl:NamedIndividual ;
  a sto:Standard ;
  terms:creator sto:IEC ;
  terms:language lang:eng ;
  terms:language lang:fra ;
  terms:title "Safety requirements for electrical equipment for measurement, control, and laboratory use - Part 2-012: Particular requirements for climatic and environmental testing and other temperature conditioning equipment"@en ;
  rdfs:comment """IEC 61010-2-012:2016 specifies safety requirements for electrical equipment and their accessories within the categories a) through c), wherever they are intended to be used, whenever that equipment incorporates one or more of the following characteristics:
- A REFRIGERATING SYSTEM that is acted on or impacted by an integral heating function such that the combined heating and cooling system generates additional and/or more severe HAZARDS than those for the two systems if treated separately.
- The materials being treated in the intended application introduce significant heat into the REFRIGERATING SYSTEM that the cooling system in the application yield additional and/or more severe HAZARDS than those for the cooling system if operated at the maximum RATED ambient alone.
- An irradiation function for the materials being treated presenting additional HAZARDS.
- A function to expose the materials being treated to excessive humidity, carbon dioxide, salt mist, or other substances which may result in additional HAZARDS.
- A function of MECHANICAL MOVEMENT presenting additional HAZARDS.
- Provision for an OPERATOR to walk-in to the operating area to load or unload the materials being treated.
It has the status of a group safety publication in accordance with IEC Guide 104.
This publication is to be read in conjunction with IEC 61010-1:2010."""@en ;
  rdfs:comment "IEC 61010-2-012:2016 specifies safety requirements for electrical equipment and their accessories within the categories a) through c), wherever they are intended to be used, whenever that equipment incorporates one or more of the following characteristics:- A REFRIGERATING SYSTEM that is acted on or impacted by an integral heating function such that the combined heating and cooling system generates additional and/or more severe HAZARDS than those for the two systems if treated separately.- The materials being treated in the intended application introduce significant heat into the REFRIGERATING SYSTEM that the cooling system in the application yield additional and/or more severe HAZARDS than those for the cooling system if operated at the maximum RATED ambient alone.- An irradiation function for the materials being treated presenting additional HAZARDS.- A function to expose the materials being treated to excessive humidity, carbon dioxide, salt mist, or other substances which may result in additional HAZARDS.- A function of MECHANICAL MOVEMENT presenting additional HAZARDS.- Provision for an OPERATOR to walk-in to the operating area to load or unload the materials being treated.It has the status of a group safety publication in accordance with IEC Guide 104. This publication is to be read in conjunction with IEC 61010-1:2010."@en ;
  rdfs:comment "IEC 61010-2-012:2016 specifies safety requirements for electrical equipment and their accessories within the categories a) through c), wherever they are intended to be used, whenever that equipment incorporates one or more of the following characteristics:n- A REFRIGERATING SYSTEM that is acted on or impacted by an integral heating function such that the combined heating and cooling system generates additional and/or more severe HAZARDS than those for the two systems if treated separately.n- The materials being treated in the intended application introduce significant heat into the REFRIGERATING SYSTEM that the cooling system in the application yield additional and/or more severe HAZARDS than those for the cooling system if operated at the maximum RATED ambient alone.n- An irradiation function for the materials being treated presenting additional HAZARDS.n- A function to expose the materials being treated to excessive humidity, carbon dioxide, salt mist, or other substances which may result in additional HAZARDS.n- A function of MECHANICAL MOVEMENT presenting additional HAZARDS.n- Provision for an OPERATOR to walk-in to the operating area to load or unload the materials being treated.nIt has the status of a group safety publication in accordance with IEC Guide 104.nThis publication is to be read in conjunction with IEC 61010-1:2010."@en ;
  rdfs:label "IEC 61010-2-012:2016"@en ;
  foaf:maker sto:IEC ;
  sto:hasAvailableLanguage lang:eng ;
  sto:hasAvailableLanguage lang:fra ;
  sto:hasEdition "1.0"^^xsd:float ;
  sto:hasFileSize sto:FileSizeIEC_61010_P2_S012 ;
  sto:hasICS sto:ICS_19_08 ;
  sto:hasOfficialResource <https://webstore.iec.ch/publication/25400> ;
  sto:hasPages "174"^^xsd:int ;
  sto:hasPublicationDate "2016-07-12"^^xsd:date ;
  sto:hasPublisher sto:IEC ;
  sto:hasStabilityDate "2020"^^xsd:gYear ;
  sto:hasTechnicalCommittee sto:TC_66 ;
.
sto:IEC_61010_P2_S201_E2
  a owl:NamedIndividual ;
  a sto:Standard ;
  terms:creator sto:IEC ;
  terms:language lang:eng ;
  terms:title "Safety requirements for electrical equipment for measurement, control, and laboratory use - Part 2-201: Particular requirements for control equipment"@en ;
  rdfs:comment "IEC 61010-2-201:2017 RLV contains the International Standard and its Redline version. The Redline version is available in English only. The Redline version provides you with a quick and easy way to compare all the changes between this standard and its previous edition. The Redline version is not an official IEC Standard, only the current version of the standard is to be considered the official document.IEC 61010-2-201:2017 specifies safety requirements and related verification tests for any product performing the function of control equipment and/or their associated peripherals. In addition, these products have as their intended use the command and control of machines, automated manufacturing and industrial processes, e.g. discrete and continuous control.This second edition cancels and replaces the first edition published in 2013. This edition constitutes a technical revision. This second edition includes the following significant technical changes with respect to the previous edition;a) clarify, change, delete definitions which were causing confusion,b) change and clarify the temperature testing methodology,c) change documentation methodologies allowed,d) change some terminal markings,e) add clarity to some of the informative annexes,f) add Annex E with changes,g) add Annexes AA – FF."@en ;
  rdfs:comment "nIEC 61010-2-201:2017 RLV contains the International Standard and its Redline version. The Redline version is available in English only. The Redline version provides you with a quick and easy way to compare all the changes between this standard and its previous edition. The Redline version is not an official IEC Standard, only the current version of the standard is to be considered the official document.nnIEC 61010-2-201:2017 specifies safety requirements and related verification tests for any product performing the function of control equipment and/or their associated peripherals. In addition, these products have as their intended use the command and control of machines, automated manufacturing and industrial processes, e.g. discrete and continuous control.nThis second edition cancels and replaces the first edition published in 2013. This edition constitutes a technical revision. This second edition includes the following significant technical changes with respect to the previous edition;na) clarify, change, delete definitions which were causing confusion,nb) change and clarify the temperature testing methodology,nc) change documentation methodologies allowed,nd) change some terminal markings,ne) add clarity to some of the informative annexes,nf) add Annex E with changes,ng) add Annexes AA – FF."@en ;
  rdfs:label "IEC 61010-2-201:2017"@en ;
  foaf:maker sto:IEC ;
  sto:hasAvailableLanguage lang:eng ;
  sto:hasEdition "2.0"^^xsd:float ;
  sto:hasFileSize sto:FileSizeIEC_61010_P2_S201 ;
  sto:hasICS sto:ICS_17_020 ;
  sto:hasICS sto:ICS_19_020 ;
  sto:hasICS sto:ICS_25_040_40 ;
  sto:hasOfficialResource <https://webstore.iec.ch/publication/60204> ;
  sto:hasPages "235"^^xsd:int ;
  sto:hasPublicationDate "2017-03-24"^^xsd:date ;
  sto:hasPublisher sto:IEC ;
  sto:hasStabilityDate "2020"^^xsd:gYear ;
  sto:hasTag "IEC 61010-2-201:2017"@en ;
  sto:hasTechnicalCommittee sto:TC_65 ;
.
sto:IEC_61010_P2_S202_E1
  a owl:NamedIndividual ;
  a sto:Standard ;
  terms:creator sto:IEC ;
  terms:language lang:eng ;
  terms:language lang:fra ;
  terms:title "Safety requirements for electrical equipment for measurement, control and laboratory use - Part 2-202: Particular requirements for electrically operated valve actuators"@en ;
  rdfs:comment """IEC 61010-2-202:2016 specifies the safety requirements for electric ACTUATORs and SOLENOIDs, as applied to valves, intended to be installed in an industrial process or discrete control environment. 

This publication is to be read in conjunction with IEC 61010-1:2010."""@en ;
  rdfs:comment "IEC 61010-2-202:2016 specifies the safety requirements for electric ACTUATORs and SOLENOIDs, as applied to valves, intended to be installed in an industrial process or discrete control environment. nnThis publication is to be read in conjunction with IEC 61010-1:2010."@en ;
  rdfs:label "IEC 61010-2-202:2016"@en ;
  foaf:maker sto:IEC ;
  sto:hasAvailableLanguage lang:eng ;
  sto:hasAvailableLanguage lang:fra ;
  sto:hasEdition "1.0"^^xsd:float ;
  sto:hasFileSize sto:FileSizeIEC_61010_P2_S202 ;
  sto:hasICS sto:ICS_13_110 ;
  sto:hasICS sto:ICS_17_020 ;
  sto:hasICS sto:ICS_19_020 ;
  sto:hasOfficialResource <https://webstore.iec.ch/publication/25399> ;
  sto:hasPages "25"^^xsd:int ;
  sto:hasPublicationDate "2016-07-12"^^xsd:date ;
  sto:hasPublisher sto:IEC ;
  sto:hasStabilityDate "2019"^^xsd:gYear ;
  sto:hasTag "IEC 61010-2-202:2016"@en ;
  sto:hasTechnicalCommittee sto:TC_65 ;
.
sto:IEC_61131
  a owl:NamedIndividual ;
  a foaf:Document ;
  a sto:Publication ;
  a sto:Standard ;
  terms:creator sto:IEC ;
  dul:isComponentOf sto:IEC_62714 ;
  rdfs:comment "IEC 61131 is an IEC standard for programmable controllers. It was known as IEC 1131 before the change in numbering system by IEC. The parts of the IEC 61131 standard are prepared and maintained working group 7, programmable control systems, of subcommittee SC 65B of Technical Committee TC65 of the IEC."@en ;
  rdfs:label "IEC 61131"@en ;
  foaf:maker sto:IEC ;
  sto:hasClassification sto:RAMIControlDevice ;
  sto:hasClassification sto:RAMIStation ;
  sto:hasClassification sto:RAMIWorkCenter ;
  sto:hasDBpediaResource <http://dbpedia.org/page/IEC_61131> ;
  sto:hasOfficialResource <https://webstore.iec.ch/publication/4550> ;
  sto:hasPublisher sto:IEC ;
  sto:hasWikipediaArticle <https://en.wikipedia.org/wiki/IEC_61131> ;
  sto:relatedTo sto:DIN_SPEC_16592 ;
  sto:relatedTo sto:IEC_61131 ;
  sto:relatedTo sto:IEC_61360 ;
  sto:relatedTo sto:IEC_61499 ;
  sto:relatedTo sto:IEC_61804 ;
  sto:relatedTo sto:IEC_61850 ;
  sto:relatedTo sto:IEC_61987_X ;
  sto:relatedTo sto:IEC_62424 ;
  sto:relatedTo sto:IEC_62453 ;
  sto:relatedTo sto:IEC_62541 ;
  sto:relatedTo sto:IEC_62714 ;
  sto:relatedTo sto:ISO_13584 ;
  sto:relatedTo sto:ISO_14306 ;
  sto:relatedTo sto:ISO_15746 ;
  sto:relatedTo sto:ISO_15926 ;
  sto:relatedTo sto:ISO_18629 ;
  sto:relatedTo sto:ISO_18828-2 ;
  sto:relatedTo sto:ISO_20922 ;
  sto:relatedTo sto:ISO_22400 ;
  sto:relatedTo sto:ISO_29002 ;
  sto:relatedTo sto:ISO_ASTM_52915 ;
  sto:relatedTo sto:ISO_PAS_17506 ;
  sto:relatedTo sto:MathML ;
  sto:relatedTo sto:SysML ;
  sto:relatedTo sto:eClass ;
.
sto:IEC_61158
  a owl:NamedIndividual ;
  a foaf:Document ;
  a sto:Publication ;
  a sto:Standard ;
  terms:creator sto:IEC ;
  rdfs:comment "Fieldbus is the name of a family of industrial computer network protocols used for real-time distributed control, standardized as IEC 61158. A complex automated industrial system such as manufacturing assembly line usually needs a distributed control system an organized hierarchy of controller systems to function. In this hierarchy, there is usually a Human Machine Interface (HMI) at the top, where an operator can monitor or operate the system. This is typically linked to a middle layer of programmable logic controllers (PLC) via a non-time-critical communications system (e.g. Ethernet). At the bottom of the control chain is the fieldbus that links the PLCs to the components that actually do the work, such as sensors, actuators, electric motors, console lights, switches, valves and contactors"@en ;
  rdfs:label "IEC 61158"@en ;
  foaf:maker sto:IEC ;
  sto:hasDBpediaResource <http://dbpedia.org/page/Fieldbus> ;
  sto:hasOfficialResource <http://www.fieldbus.org/> ;
  sto:hasPublisher sto:IEC ;
  sto:hasTag "Fieldbus"@en ;
  sto:hasWikipediaArticle <https://en.wikipedia.org/wiki/Fieldbus> ;
  sto:relatedTo sto:IEC_29182-1 ;
  sto:relatedTo sto:IEC_61158 ;
  sto:relatedTo sto:IEC_61784 ;
  sto:relatedTo sto:OMG_DDS ;
.
sto:IEC_61160_E2
  a owl:NamedIndividual ;
  a sto:Standard ;
  terms:creator sto:IEC ;
  terms:language lang:eng ;
  terms:language lang:fra ;
  terms:language lang:spa ;
  terms:title "Design review"@en ;
  rdfs:comment "This International Standard makes recommendations for the implementation of design review as a means of verifying that the design input requirements have been met and stimulating the improvement of the product's design. The intention is for it to be applied during the design and development phase of a product's life cycle."@en ;
  rdfs:label "IEC 61160:2005"@en ;
  foaf:maker sto:IEC ;
  sto:hasAvailableLanguage lang:eng ;
  sto:hasAvailableLanguage lang:fra ;
  sto:hasAvailableLanguage lang:spa ;
  sto:hasEdition "2.0"^^xsd:float ;
  sto:hasFileSize sto:FileSizeIEC_61160 ;
  sto:hasICS sto:ICS_03_100_40 ;
  sto:hasICS sto:ICS_03_120_01 ;
  sto:hasOfficialResource <https://webstore.iec.ch/publication/4707> ;
  sto:hasPages "69"^^xsd:int ;
  sto:hasPublicationDate "2005-09-27"^^xsd:date ;
  sto:hasPublisher sto:IEC ;
  sto:hasStabilityDate "2020"^^xsd:gYear ;
  sto:hasTag "IEC 61160:2005"@en ;
  sto:hasTechnicalCommittee sto:TC_56 ;
.
sto:IEC_61310_P1_E2
  a owl:NamedIndividual ;
  a sto:Standard ;
  terms:creator sto:IEC ;
  terms:language lang:eng ;
  terms:language lang:fra ;
  terms:language lang:spa ;
  terms:title "Safety of machinery - Indication, marking and actuation - Part 1: Requirements for visual, acoustic and tactile signals"@en ;
  rdfs:comment "Specifies requirements for visual, acoustic and tactile methods of indicating safety-related information, at the human-machine interface and to exposed persons. It specifies a system of colours, safety signs, markings and other warnings, intended for use in the indication of hazardous situations and health hazards and for meeting certain emergencies. It also specifies ways of coding visual, acoustic and tactile signals for indicators and actuators to facilitate the safe use and monitoring of the machinery. It includes the following significant technical changes with respect to the previous edition: Adapted to the basic standards IEC 60073, IEC 60417, ISO 3864-1, ISO 7000 and ISO 7010"@en ;
  rdfs:label "IEC 61310-1:2007"@en ;
  foaf:maker sto:IEC ;
  sto:hasAvailableLanguage lang:eng ;
  sto:hasAvailableLanguage lang:fra ;
  sto:hasAvailableLanguage lang:spa ;
  sto:hasEdition "2.0"^^xsd:float ;
  sto:hasFileSize sto:FileSizeIEC_61310_P1 ;
  sto:hasICS sto:ICS_13_110 ;
  sto:hasOfficialResource <https://webstore.iec.ch/publication/5263> ;
  sto:hasPages "43"^^xsd:int ;
  sto:hasPublicationDate "2007-02-16"^^xsd:date ;
  sto:hasPublisher sto:IEC ;
  sto:hasStabilityDate "2021"^^xsd:gYear ;
  sto:hasTag "IEC 61310-1:2007"@en ;
  sto:hasTechnicalCommittee sto:TC_44 ;
.
sto:IEC_61310_P2_E2
  a owl:NamedIndividual ;
  a sto:Standard ;
  terms:creator sto:IEC ;
  terms:language lang:eng ;
  terms:language lang:fra ;
  terms:language lang:spa ;
  terms:title "Safety of machinery - Indication, marking and actuation - Part 2: Requirements for marking"@en ;
  rdfs:comment "It gives general rules on marking for identification of machinery, for safe use related to mechanical and electrical hazards, and for the avoidance of hazards arising from incorrect connections. Includes the following significant technical changes with respect to the previous edition: Annex A: additional safety signs included and updated."@en ;
  rdfs:label "IEC 61310-2:2007"@en ;
  foaf:maker sto:IEC ;
  sto:hasAvailableLanguage lang:eng ;
  sto:hasAvailableLanguage lang:fra ;
  sto:hasAvailableLanguage lang:spa ;
  sto:hasEdition "2.0"^^xsd:float ;
  sto:hasFileSize sto:FileSizeIEC_61310_P2 ;
  sto:hasICS sto:ICS_13_110 ;
  sto:hasOfficialResource <https://webstore.iec.ch/publication/5264> ;
  sto:hasPages "25"^^xsd:int ;
  sto:hasPublicationDate "2007-02-16"^^xsd:date ;
  sto:hasPublisher sto:IEC ;
  sto:hasStabilityDate "2021"^^xsd:gYear ;
  sto:hasTag "IEC 61310-2:2007"@en ;
  sto:hasTechnicalCommittee sto:TC_44 ;
.
sto:IEC_61310_P3_E2
  a owl:NamedIndividual ;
  a sto:Standard ;
  terms:creator sto:IEC ;
  terms:language lang:eng ;
  terms:language lang:fra ;
  terms:language lang:spa ;
  terms:title "Safety of machinery - Indication, marking and actuation - Part 3: Requirements for the location and operation of actuators"@en ;
  rdfs:comment "Specifies safety-related requirements for actuators, operated by the hand or by other parts of the human body, at the human-machine interface. It gives general requirements for the standard direction of movement for actuators; the arrangement of an actuator in relation to other actuators; the correlation between an action and its final effects. It includes the following significant technical changes with respect to the previous edition: Table 1, Table 2 and Table A.1 have been revised editorially."@en ;
  rdfs:label "IEC 61310-3:2007"@en ;
  foaf:maker sto:IEC ;
  sto:hasAvailableLanguage lang:eng ;
  sto:hasAvailableLanguage lang:fra ;
  sto:hasAvailableLanguage lang:spa ;
  sto:hasEdition "2.0"^^xsd:float ;
  sto:hasFileSize sto:FileSizeIEC_61310_P3 ;
  sto:hasICS sto:ICS_13_110 ;
  sto:hasOfficialResource <https://webstore.iec.ch/publication/5265> ;
  sto:hasPages "25"^^xsd:int ;
  sto:hasPublicationDate "2007-02-16"^^xsd:date ;
  sto:hasPublisher sto:IEC ;
  sto:hasStabilityDate "2021"^^xsd:gYear ;
  sto:hasTag "IEC 61310-3:2007"@en ;
  sto:hasTechnicalCommittee sto:TC_44 ;
.
sto:IEC_61334
  a owl:NamedIndividual ;
  a foaf:Document ;
  a sto:Publication ;
  a sto:Standard ;
  terms:creator sto:IEC ;
  rdfs:comment "IEC 61334 , known as Distribution automation using distribution line carrier systems, is a standard for low-speed reliable power line communications by electricity meters, water meters and SCADA."@en ;
  rdfs:label "IEC 61334"@en ;
  foaf:maker sto:IEC ;
  sto:hasDBpediaResource <http://dbpedia.org/page/IEC_61334> ;
  sto:hasOfficialResource <https://webstore.iec.ch/publication/5308> ;
  sto:hasPublisher sto:IEC ;
.
sto:IEC_61334_P3_S1_E1
  a owl:NamedIndividual ;
  a sto:Standard ;
  terms:creator sto:IEC ;
  terms:language lang:eng ;
  terms:language lang:fra ;
  terms:title "Distribution automation using distribution line carrier systems - Part 3-1: Mains signalling requirements - Frequency bands and output levels"@en ;
  rdfs:comment """Applies to electrical equipment used in distribution line carrier systems on both medium-voltage and low-voltage distribution networks. Specifies requirements such as frequency bands, output levels, spurious emissions, etc.
This publication is of high relevance for Smart Grid."""@en ;
  rdfs:comment "Applies to electrical equipment used in distribution line carrier systems on both medium-voltage and low-voltage distribution networks. Specifies requirements such as frequency bands, output levels, spurious emissions, etc.nThis publication is of high relevance for Smart Grid."@en ;
  rdfs:label "IEC 61334-3-1:1998 "@en ;
  foaf:maker sto:IEC ;
  sto:hasAvailableLanguage lang:eng ;
  sto:hasAvailableLanguage lang:fra ;
  sto:hasDBpediaResource <https://dbpedia.org/resource/IEC_61334> ;
  sto:hasEdition "1.0"^^xsd:float ;
  sto:hasFileSize sto:FileSizeIEC_61334_P3_S1 ;
  sto:hasICS sto:ICS_29_240_20 ;
  sto:hasICS sto:ICS_33_200 ;
  sto:hasOfficialResource <https://webstore.iec.ch/publication/5297> ;
  sto:hasPages "27"^^xsd:int ;
  sto:hasPublicationDate "1998-11-24"^^xsd:date ;
  sto:hasPublisher sto:IEC ;
  sto:hasStabilityDate "2018"^^xsd:gYear ;
  sto:hasTag "IEC 61334-3-1:1998 "@en ;
  sto:hasTechnicalCommittee sto:TC_57 ;
  sto:hasWikipediaArticle <https://en.wikipedia.org/wiki/IEC_61334> ;
.
sto:IEC_61334_P3_S21_E1
  a owl:NamedIndividual ;
  a sto:Standard ;
  terms:creator sto:IEC ;
  terms:language lang:eng ;
  terms:language lang:fra ;
  terms:title "Distribution automation using distribution line carrier systems - Part 3: Mains signalling requirements - Section 21: MV phase-to-phase isolated capacitive coupling device"@en ;
  rdfs:comment """Establishes definitions, requirements, methods of testing and rated values for phase-to-phase isolated capacitive coupling devices to be used in medium-voltage (MV) distribution line carrier systems.
This publication is of high relevance for Smart Grid."""@en ;
  rdfs:comment "Establishes definitions, requirements, methods of testing and rated values for phase-to-phase isolated capacitive coupling devices to be used in medium-voltage (MV) distribution line carrier systems.nThis publication is of high relevance for Smart Grid."@en ;
  rdfs:label "IEC 61334-3-21:1996 "@en ;
  foaf:maker sto:IEC ;
  sto:hasAvailableLanguage lang:eng ;
  sto:hasAvailableLanguage lang:fra ;
  sto:hasDBpediaResource <https://dbpedia.org/resource/IEC_61334> ;
  sto:hasEdition "1.0"^^xsd:float ;
  sto:hasFileSize sto:FileSizeIEC_61334_P3_S21 ;
  sto:hasICS sto:ICS_29_240_20 ;
  sto:hasICS sto:ICS_33_200 ;
  sto:hasOfficialResource <https://webstore.iec.ch/publication/5298> ;
  sto:hasPages "33"^^xsd:int ;
  sto:hasPublicationDate "1996-03-27"^^xsd:date ;
  sto:hasPublisher sto:IEC ;
  sto:hasStabilityDate "2018"^^xsd:gYear ;
  sto:hasTag "IEC 61334-3-21:1996 "@en ;
  sto:hasTechnicalCommittee sto:TC_57 ;
  sto:hasWikipediaArticle <https://en.wikipedia.org/wiki/IEC_61334> ;
.
sto:IEC_61334_P3_S22_E1
  a owl:NamedIndividual ;
  a sto:Standard ;
  terms:creator sto:IEC ;
  terms:language lang:eng ;
  terms:language lang:fra ;
  terms:title "Distribution automation using distribution line carrier systems - Part 3-22: Mains signalling requirements - MV phase-to-earth and screen-to-earth intrusive coupling devices"@en ;
  rdfs:comment """Establishes definitions, requirements, methods of testing and rated values for phase-to-earth capacitive and screen-to-earth intrusive inductive coupling devices to be used in medium voltage DLC systems.
This publication is of high relevance for Smart Grid."""@en ;
  rdfs:comment "Establishes definitions, requirements, methods of testing and rated values for phase-to-earth capacitive and screen-to-earth intrusive inductive coupling devices to be used in medium voltage DLC systems.nThis publication is of high relevance for Smart Grid."@en ;
  rdfs:label "IEC 61334-3-22:2001"@en ;
  foaf:maker sto:IEC ;
  sto:hasAvailableLanguage lang:eng ;
  sto:hasAvailableLanguage lang:fra ;
  sto:hasDBpediaResource <https://dbpedia.org/resource/IEC_61334> ;
  sto:hasEdition "1.0"^^xsd:float ;
  sto:hasFileSize sto:FileSizeIEC_61334_P3_S22 ;
  sto:hasICS sto:ICS_29_240_20 ;
  sto:hasICS sto:ICS_33_200 ;
  sto:hasOfficialResource <https://webstore.iec.ch/publication/5299> ;
  sto:hasPages "35"^^xsd:int ;
  sto:hasPublicationDate "2001-01-12"^^xsd:date ;
  sto:hasPublisher sto:IEC ;
  sto:hasStabilityDate "2018"^^xsd:gYear ;
  sto:hasTag "IEC 61334-3-22:2001 "@en ;
  sto:hasTechnicalCommittee sto:TC_57 ;
  sto:hasWikipediaArticle <https://en.wikipedia.org/wiki/IEC_61334> ;
.
sto:IEC_61334_P4_S1_E1
  a owl:NamedIndividual ;
  a sto:Standard ;
  terms:creator sto:IEC ;
  terms:language lang:eng ;
  terms:language lang:fra ;
  terms:title "Distribution automation using distribution line carrier systems - Part 4: Data communication protocols - Section 1: Reference model of the communication system"@en ;
  rdfs:comment """Provides a basic description of the communication system based on a three layer model. Application examples are control and monitoring of the distribution network, order broadcast, control of user interfaces, public lighting, automatic meter reading, etc.
This publication is of high relevance for Smart Grid."""@en ;
  rdfs:comment "Provides a basic description of the communication system based on a three layer model. Application examples are control and monitoring of the distribution network, order broadcast, control of user interfaces, public lighting, automatic meter reading, etc.nThis publication is of high relevance for Smart Grid."@en ;
  rdfs:label "IEC 61334-4-1:1996 "@en ;
  foaf:maker sto:IEC ;
  sto:hasAvailableLanguage lang:eng ;
  sto:hasAvailableLanguage lang:fra ;
  sto:hasDBpediaResource <https://dbpedia.org/resource/IEC_61334> ;
  sto:hasEdition "1.0"^^xsd:float ;
  sto:hasFileSize sto:FileSizeIEC_61334_P4_S1 ;
  sto:hasICS sto:ICS_29_240_20 ;
  sto:hasICS sto:ICS_33_200 ;
  sto:hasOfficialResource <https://webstore.iec.ch/publication/5300> ;
  sto:hasPages "43"^^xsd:int ;
  sto:hasPublicationDate "1996-07-31"^^xsd:date ;
  sto:hasPublisher sto:IEC ;
  sto:hasStabilityDate "2018"^^xsd:gYear ;
  sto:hasTag "IEC 61334-4-1:1996 "@en ;
  sto:hasTechnicalCommittee sto:TC_57 ;
  sto:hasWikipediaArticle <https://en.wikipedia.org/wiki/IEC_61334> ;
.
sto:IEC_61334_P4_S32_E1
  a owl:NamedIndividual ;
  a sto:Standard ;
  terms:creator sto:IEC ;
  terms:language lang:eng ;
  terms:language lang:fra ;
  terms:title "Distribution automation using distribution line carrier systems - Part 4: Data communication protocols - Section 32: Data link layer - Logical link control (LLC)"@en ;
  rdfs:comment """Covers the services required of, or by, the DCP Logical Link Control (LLC) sublayer entity at the logical interfaces with the application layer and the MAC sublayer.
This publication is of high relevance for Smart Grid."""@en ;
  rdfs:comment "Covers the services required of, or by, the DCP Logical Link Control (LLC) sublayer entity at the logical interfaces with the application layer and the MAC sublayer.nThis publication is of high relevance for Smart Grid."@en ;
  rdfs:label "IEC 61334-4-32:1996 "@en ;
  foaf:maker sto:IEC ;
  sto:hasAvailableLanguage lang:eng ;
  sto:hasAvailableLanguage lang:fra ;
  sto:hasDBpediaResource <https://dbpedia.org/resource/IEC_61334> ;
  sto:hasEdition "1.0"^^xsd:float ;
  sto:hasFileSize sto:FileSizeIEC_61334_P4_S32 ;
  sto:hasICS sto:ICS_29_240_20 ;
  sto:hasICS sto:ICS_33_200 ;
  sto:hasOfficialResource <https://webstore.iec.ch/publication/5301> ;
  sto:hasPages "69"^^xsd:int ;
  sto:hasPublicationDate "1996-09-26"^^xsd:date ;
  sto:hasPublisher sto:IEC ;
  sto:hasStabilityDate "2018"^^xsd:gYear ;
  sto:hasTag "IEC 61334-4-32:1996 "@en ;
  sto:hasTechnicalCommittee sto:TC_57 ;
  sto:hasWikipediaArticle <https://en.wikipedia.org/wiki/IEC_61334> ;
.
sto:IEC_61334_P4_S33_E1
  a owl:NamedIndividual ;
  a sto:Standard ;
  terms:creator sto:IEC ;
  terms:language lang:eng ;
  terms:language lang:fra ;
  terms:title "Distribution automation using distribution line carrier systems - Part 4-33: Data communication protocols - Data link layer - Connection oriented protocol"@en ;
  rdfs:comment "Covers the services required by the data communication protocol (DCP) logical link control (LLC) sublayer entity at the logical interfaces with the LLC -user layer and the MAC sublayer, using the connection-oriented LLC procedures.nThis publication is of high relevance for Smart Grid."@en ;
  rdfs:label "IEC 61334-4-33:1998 "@en ;
  foaf:maker sto:IEC ;
  sto:hasAvailableLanguage lang:eng ;
  sto:hasAvailableLanguage lang:fra ;
  sto:hasDBpediaResource <https://dbpedia.org/resource/IEC_61334> ;
  sto:hasEdition "1.0"^^xsd:float ;
  sto:hasFileSize sto:FileSizeIEC_61334_P4_S3 ;
  sto:hasICS sto:ICS_29_240_20 ;
  sto:hasICS sto:ICS_33_200 ;
  sto:hasOfficialResource <https://webstore.iec.ch/publication/5302> ;
  sto:hasPages "51"^^xsd:int ;
  sto:hasPublicationDate "1998-07-10"^^xsd:date ;
  sto:hasPublisher sto:IEC ;
  sto:hasStabilityDate "2018"^^xsd:gYear ;
  sto:hasTag "IEC 61334-4-33:1998 "@en ;
  sto:hasTechnicalCommittee sto:TC_57 ;
  sto:hasWikipediaArticle <https://en.wikipedia.org/wiki/IEC_61334> ;
.
sto:IEC_61334_P4_S41_E1
  a owl:NamedIndividual ;
  a sto:Standard ;
  terms:creator sto:IEC ;
  terms:language lang:eng ;
  terms:language lang:fra ;
  terms:title "Distribution automation using distribution line carrier systems - Part 4: Data communication protocols - Section 41: Application protocol - Distribution line message specification"@en ;
  rdfs:comment """Defines the distribution line message specification (DLMS) within the OSI application layer.
This publication is of high relevance for Smart Grid."""@en ;
  rdfs:comment "Defines the distribution line message specification (DLMS) within the OSI application layer.nThis publication is of high relevance for Smart Grid."@en ;
  rdfs:label "IEC 61334-4-41:1996"@en ;
  foaf:maker sto:IEC ;
  sto:hasAvailableLanguage lang:eng ;
  sto:hasAvailableLanguage lang:fra ;
  sto:hasDBpediaResource <https://dbpedia.org/resource/IEC_61334> ;
  sto:hasEdition "1.0"^^xsd:float ;
  sto:hasFileSize sto:FileSizeIEC_61334_P4_S41 ;
  sto:hasICS sto:ICS_29_240_20 ;
  sto:hasICS sto:ICS_33_200 ;
  sto:hasOfficialResource <https://webstore.iec.ch/publication/5303> ;
  sto:hasPages "247"^^xsd:int ;
  sto:hasPublicationDate "1996-08-13"^^xsd:date ;
  sto:hasPublisher sto:IEC ;
  sto:hasStabilityDate "2018"^^xsd:gYear ;
  sto:hasTag "IEC 61334-4-41:1996"@en ;
  sto:hasTechnicalCommittee sto:TC_57 ;
  sto:hasWikipediaArticle <https://en.wikipedia.org/wiki/IEC_61334> ;
.
sto:IEC_61334_P4_S42_E1
  a owl:NamedIndividual ;
  a sto:Standard ;
  terms:creator sto:IEC ;
  terms:language lang:eng ;
  terms:language lang:fra ;
  terms:title "Distribution automation using distribution line carrier systems -Part 4: Data communication protocols - Section 42: Applicationprotocols - Application laye"@en ;
  rdfs:comment """Describes the rules used to design an application service element, the ISO connectionless ACSE (Application Control Service Element), and the DLMS Application Service Element.
This publication is of high relevance for Smart Grid."""@en ;
  rdfs:comment "Describes the rules used to design an application service element, the ISO connectionless ACSE (Application Control Service Element), and the DLMS Application Service Element.nThis publication is of high relevance for Smart Grid."@en ;
  rdfs:label "IEC 61334-4-42:1996"@en ;
  foaf:maker sto:IEC ;
  sto:hasAvailableLanguage lang:eng ;
  sto:hasAvailableLanguage lang:fra ;
  sto:hasDBpediaResource <https://dbpedia.org/resource/IEC_61334> ;
  sto:hasEdition "1.0"^^xsd:float ;
  sto:hasFileSize sto:FileSizeIEC_61334_P4_S42 ;
  sto:hasICS sto:ICS_29_240_20 ;
  sto:hasICS sto:ICS_33_200 ;
  sto:hasOfficialResource <https://webstore.iec.ch/publication/5304> ;
  sto:hasPages "89"^^xsd:int ;
  sto:hasPublicationDate "1996-10-09"^^xsd:date ;
  sto:hasPublisher sto:IEC ;
  sto:hasStabilityDate "2018"^^xsd:gYear ;
  sto:hasTag "IEC 61334-4-42:1996"@en ;
  sto:hasTechnicalCommittee sto:TC_57 ;
  sto:hasWikipediaArticle <https://en.wikipedia.org/wiki/IEC_61334> ;
.
sto:IEC_61334_P4_S511_E1
  a owl:NamedIndividual ;
  a sto:Standard ;
  terms:creator sto:IEC ;
  terms:language lang:eng ;
  terms:language lang:fra ;
  terms:title "Distribution automation using distribution line carrier systems - Part 4-511: Data communication protocols - Systems management - CIASE protocol"@en ;
  rdfs:comment """Specifies the data communication protocol (DCP) management requirements. Describes the management services in an abstract way as well as the underlying protocol.
This publication is of high relevance for Smart Grid."""@en ;
  rdfs:comment "Specifies the data communication protocol (DCP) management requirements. Describes the management services in an abstract way as well as the underlying protocol.nThis publication is of high relevance for Smart Grid."@en ;
  rdfs:label "IEC 61334-4-511:2000"@en ;
  foaf:maker sto:IEC ;
  sto:hasAvailableLanguage lang:eng ;
  sto:hasAvailableLanguage lang:fra ;
  sto:hasDBpediaResource <https://dbpedia.org/resource/IEC_61334> ;
  sto:hasEdition "1.0"^^xsd:float ;
  sto:hasFileSize sto:FileSizeIEC_61334_P4_S511 ;
  sto:hasICS sto:ICS_33_040_40 ;
  sto:hasICS sto:ICS_33_200 ;
  sto:hasOfficialResource <https://webstore.iec.ch/publication/5305> ;
  sto:hasPages "65"^^xsd:int ;
  sto:hasPublicationDate "2000-04-18"^^xsd:date ;
  sto:hasPublisher sto:IEC ;
  sto:hasStabilityDate "2018"^^xsd:gYear ;
  sto:hasTag "IEC 61334-4-511:2000"@en ;
  sto:hasTechnicalCommittee sto:TC_57 ;
  sto:hasWikipediaArticle <https://en.wikipedia.org/wiki/IEC_61334> ;
.
sto:IEC_61334_P4_S512_E1
  a owl:NamedIndividual ;
  a sto:Standard ;
  terms:creator sto:IEC ;
  terms:language lang:eng ;
  terms:language lang:fra ;
  terms:title "Distribution automation using distribution line carrier systems - Part 4-512: Data communication protocols - System management using profile 61334-5-1 - Management Information Base (MIB)"@en ;
  rdfs:comment """Specifies the Management Information Base (MIB), which is used for the management of the communication profile defined by the following standards: IEC 61334-5-1, IEC 61334-4-32, IEC 61334-4-42, and IEC 61334-4-41.
This publication is of high relevance for Smart Grid."""@en ;
  rdfs:comment "Specifies the Management Information Base (MIB), which is used for the management of the communication profile defined by the following standards: IEC 61334-5-1, IEC 61334-4-32, IEC 61334-4-42, and IEC 61334-4-41.nThis publication is of high relevance for Smart Grid."@en ;
  rdfs:label "IEC 61334-4-512:2001"@en ;
  foaf:maker sto:IEC ;
  sto:hasAvailableLanguage lang:eng ;
  sto:hasAvailableLanguage lang:fra ;
  sto:hasDBpediaResource <https://dbpedia.org/resource/IEC_61334> ;
  sto:hasEdition "1.0"^^xsd:float ;
  sto:hasFileSize sto:FileSizeIEC_61334_P4_S512 ;
  sto:hasICS sto:ICS_33_200 ;
  sto:hasOfficialResource <https://webstore.iec.ch/publication/5306> ;
  sto:hasPages "47"^^xsd:int ;
  sto:hasPublicationDate "2001-10-30"^^xsd:date ;
  sto:hasPublisher sto:IEC ;
  sto:hasStabilityDate "2018"^^xsd:gYear ;
  sto:hasTag "IEC 61334-4-512:2001"@en ;
  sto:hasTechnicalCommittee sto:TC_57 ;
  sto:hasWikipediaArticle <https://en.wikipedia.org/wiki/IEC_61334> ;
.
sto:IEC_61334_P4_S61_E1
  a owl:NamedIndividual ;
  a sto:Standard ;
  terms:creator sto:IEC ;
  terms:language lang:eng ;
  terms:language lang:fra ;
  terms:title "Distribution automation using distribution line carrier systems - Part 4-61: Data communication protocols - Network layer - Connectionless protocol"@en ;
  rdfs:comment """Covers the services required by the data communication protocol (DCP) network layer (N) sublayer entity at the logical interfaces with the N user layer and the LLC sublayer, using the connectionless N procedures.
This publication is of high relevance for Smart Grid."""@en ;
  rdfs:comment "Covers the services required by the data communication protocol (DCP) network layer (N) sublayer entity at the logical interfaces with the N user layer and the LLC sublayer, using the connectionless N procedures.nThis publication is of high relevance for Smart Grid."@en ;
  rdfs:label "IEC 61334-4-61:1998"@en ;
  foaf:maker sto:IEC ;
  sto:hasAvailableLanguage lang:eng ;
  sto:hasAvailableLanguage lang:fra ;
  sto:hasDBpediaResource <https://dbpedia.org/resource/IEC_61334> ;
  sto:hasEdition "1.0"^^xsd:float ;
  sto:hasFileSize sto:FileSizeIEC_61334_P4_S61 ;
  sto:hasICS sto:ICS_29_240_20 ;
  sto:hasICS sto:ICS_33_200 ;
  sto:hasOfficialResource <https://webstore.iec.ch/publication/5307> ;
  sto:hasPages "63"^^xsd:int ;
  sto:hasPublicationDate "1998-07-10"^^xsd:date ;
  sto:hasPublisher sto:IEC ;
  sto:hasStabilityDate "2018"^^xsd:gYear ;
  sto:hasTag "IEC 61334-4-61:1998"@en ;
  sto:hasTechnicalCommittee sto:TC_57 ;
  sto:hasWikipediaArticle <https://en.wikipedia.org/wiki/IEC_61334> ;
.
sto:IEC_61334_P5_S1_E2
  a owl:NamedIndividual ;
  a sto:Standard ;
  terms:creator sto:IEC ;
  terms:language lang:eng ;
  terms:language lang:fra ;
  terms:title "Distribution automation using distribution line carrier systems - Part 5-1: Lower layer profiles - The spread frequency shift keying (S-FSK) profile"@en ;
  rdfs:comment """Describes the requirements of S-FSK (frequency shift keying modulation) in conjunction with the services provided by the physical layer entity and the MAC sublayer. The transmission medium is assumed to be the distribution network on both MV or LV level. To be used in conjunction with IEC 61334-4-32.
This publication is of high relevance for Smart Grid."""@en ;
  rdfs:comment "Describes the requirements of S-FSK (frequency shift keying modulation) in conjunction with the services provided by the physical layer entity and the MAC sublayer. The transmission medium is assumed to be the distribution network on both MV or LV level. To be used in conjunction with IEC 61334-4-32.nThis publication is of high relevance for Smart Grid."@en ;
  rdfs:label "IEC 61334-5-1:2001"@en ;
  foaf:maker sto:IEC ;
  sto:hasAvailableLanguage lang:eng ;
  sto:hasAvailableLanguage lang:fra ;
  sto:hasDBpediaResource <https://dbpedia.org/resource/IEC_61334> ;
  sto:hasEdition "2.0"^^xsd:float ;
  sto:hasFileSize sto:FileSizeIEC_61334_P5_S1 ;
  sto:hasICS sto:ICS_33_200 ;
  sto:hasOfficialResource <https://webstore.iec.ch/publication/5308> ;
  sto:hasPages "123"^^xsd:int ;
  sto:hasPublicationDate "2001-05-28"^^xsd:date ;
  sto:hasPublisher sto:IEC ;
  sto:hasStabilityDate "2018"^^xsd:gYear ;
  sto:hasTag "IEC 61334-5-1:2001"@en ;
  sto:hasTechnicalCommittee sto:TC_57 ;
  sto:hasWikipediaArticle <https://en.wikipedia.org/wiki/IEC_61334> ;
  sto:isRelevantFor sto:SmartCity ;
.
sto:IEC_61334_P6_E1
  a owl:NamedIndividual ;
  a sto:Standard ;
  terms:creator sto:IEC ;
  terms:language lang:eng ;
  terms:language lang:fra ;
  terms:title "Distribution automation using distribution line carrier systems - Part 6: A-XDR encoding rule"@en ;
  rdfs:comment """Defines a set of encoding rules that may be used to derive the specification of a transfer syntax for values of types defined in the DLMS core standard using the ASN.1 notation (see IEC 61334-4-41).
This publication is of high relevance for Smart Grid."""@en ;
  rdfs:comment "Defines a set of encoding rules that may be used to derive the specification of a transfer syntax for values of types defined in the DLMS core standard using the ASN.1 notation (see IEC 61334-4-41).nThis publication is of high relevance for Smart Grid."@en ;
  rdfs:label "IEC 61334-6:2000"@en ;
  foaf:maker sto:IEC ;
  sto:hasAvailableLanguage lang:eng ;
  sto:hasAvailableLanguage lang:fra ;
  sto:hasDBpediaResource <https://dbpedia.org/resource/IEC_61334> ;
  sto:hasEdition "1.0"^^xsd:float ;
  sto:hasFileSize sto:FileSizeIEC_61334_P6 ;
  sto:hasICS sto:ICS_29_240_20 ;
  sto:hasICS sto:ICS_33_200 ;
  sto:hasOfficialResource <https://webstore.iec.ch/publication/5313> ;
  sto:hasPages "75"^^xsd:int ;
  sto:hasPublicationDate "2000-06-16"^^xsd:date ;
  sto:hasPublisher sto:IEC ;
  sto:hasStabilityDate "2018"^^xsd:gYear ;
  sto:hasTag "IEC 61334-6:2000"@en ;
  sto:hasTechnicalCommittee sto:TC_57 ;
  sto:hasWikipediaArticle <https://en.wikipedia.org/wiki/IEC_61334> ;
.
sto:IEC_61360
  a owl:NamedIndividual ;
  a foaf:Document ;
  a sto:Publication ;
  a sto:Standard ;
  terms:creator sto:IEC ;
  rdfs:comment "IEC Common Data Dictionary (IEC CDD) is a common repository of concepts for all electrotechnical domains based on the methodology and the information model of IEC 61360 series. Standard data elements types with associated classification scheme for electric items."@en ;
  rdfs:label "IEC 61360"@en ;
  foaf:maker sto:IEC ;
  sto:hasClassification rami:Engineering ;
  sto:hasClassification sto:IDSRAMInformationLayer ;
  sto:hasClassification sto:ManufacturingModelData ;
  sto:hasClassification sto:RAMIAssetlayer ;
  sto:hasDomain "Electrotechnical"@en ;
  sto:hasMotivation "Standard data elements (properties) are used as elements in administration shell"@en ;
  sto:hasOfficialResource <http://cdd.iec.ch/cdd/iec61360/iec61360.nsf> ;
  sto:hasOfficialResource <https://webstore.iec.ch/publication/5380> ;
  sto:hasPublisher sto:IEC ;
  sto:hasTag "IEC Common Data Dictionary"@en ;
  sto:relatedTo sto:DIN_SPEC_16592 ;
  sto:relatedTo sto:IEC_61131 ;
  sto:relatedTo sto:IEC_61360 ;
  sto:relatedTo sto:IEC_61499 ;
  sto:relatedTo sto:IEC_61804 ;
  sto:relatedTo sto:IEC_61850 ;
  sto:relatedTo sto:IEC_61987_X ;
  sto:relatedTo sto:IEC_62424 ;
  sto:relatedTo sto:IEC_62453 ;
  sto:relatedTo sto:IEC_62541 ;
  sto:relatedTo sto:IEC_62714 ;
  sto:relatedTo sto:ISO_13584 ;
  sto:relatedTo sto:ISO_14306 ;
  sto:relatedTo sto:ISO_15746 ;
  sto:relatedTo sto:ISO_15926 ;
  sto:relatedTo sto:ISO_18629 ;
  sto:relatedTo sto:ISO_18828-2 ;
  sto:relatedTo sto:ISO_20922 ;
  sto:relatedTo sto:ISO_22400 ;
  sto:relatedTo sto:ISO_29002 ;
  sto:relatedTo sto:ISO_ASTM_52915 ;
  sto:relatedTo sto:ISO_PAS_17506 ;
  sto:relatedTo sto:MathML ;
  sto:relatedTo sto:SysML ;
  sto:relatedTo sto:eClass ;
.
sto:IEC_61400
  a owl:NamedIndividual ;
  a foaf:Document ;
  a sto:Publication ;
  a sto:Standard ;
  terms:creator sto:IEC ;
  rdfs:comment "IEC 61334 , known as Distribution automation using distribution line carrier systems, is a standard for low-speed reliable power line communications by electricity meters, water meters and SCADA."@en ;
  rdfs:label "IEC 61400"@en ;
  foaf:maker sto:IEC ;
  sto:hasDBpediaResource <http://dbpedia.org/page/IEC_61400> ;
  sto:hasOfficialResource <https://webstore.iec.ch/publication/26603> ;
  sto:hasPublicationDate "2017-03-03"^^xsd:date ;
  sto:hasPublisher sto:IEC ;
.
sto:IEC_61400_P25_S1_E2
  a owl:NamedIndividual ;
  a sto:Standard ;
  terms:creator sto:IEC ;
  terms:language lang:eng ;
  terms:title "Wind energy generation systems - Part 25-1: Communications for monitoring and control of wind power plants - Overall description of principles and models"@en ;
  rdfs:comment """IEC 61400-25-1:2017 RLV contains the International Standard and its Redline version. The Redline version is available in English only. The Redline version provides you with a quick and easy way to compare all the changes between this standard and its previous edition. The Redline version is not an official IEC Standard, only the current version of the standard is to be considered the official document.

IEC 61400-25-1:2017 gives an overall description of the principles and models used in the IEC 61400�25 series, which is designed for a communication environment supported by a client-server model. Three areas are defined, that are modelled separately to ensure the scalability of implementations: wind power plant information models, information exchange model, and mapping of these two models to a standard communication profile. This new edition includes the following significant technical changes with respect to the previous edition: general harmonization of text and overview models with the other parts of the IEC 61400�25 series, harmonization of definitions in other related standards."""@en ;
  rdfs:comment "IEC 61400-25-1:2017 RLV contains the International Standard and its Redline version. The Redline version is available in English only. The Redline version provides you with a quick and easy way to compare all the changes between this standard and its previous edition. The Redline version is not an official IEC Standard, only the current version of the standard is to be considered the official document.IEC 61400-25-1:2017 gives an overall description of the principles and models used in the IEC 61400�25 series, which is designed for a communication environment supported by a client-server model. Three areas are defined, that are modelled separately to ensure the scalability of implementations: wind power plant information models, information exchange model, and mapping of these two models to a standard communication profile. This new edition includes the following significant technical changes with respect to the previous edition: general harmonization of text and overview models with the other parts of the IEC 61400�25 series, harmonization of definitions in other related standards."@en ;
  rdfs:comment "IEC 61400-25-1:2017 RLV contains the International Standard and its Redline version. The Redline version is available in English only. The Redline version provides you with a quick and easy way to compare all the changes between this standard and its previous edition. The Redline version is not an official IEC Standard, only the current version of the standard is to be considered the official document.nnIEC 61400-25-1:2017 gives an overall description of the principles and models used in the IEC 61400�25 series, which is designed for a communication environment supported by a client-server model. Three areas are defined, that are modelled separately to ensure the scalability of implementations: wind power plant information models, information exchange model, and mapping of these two models to a standard communication profile. This new edition includes the following significant technical changes with respect to the previous edition: general harmonization of text and overview models with the other parts of the IEC 61400�25 series, harmonization of definitions in other related standards."@en ;
  rdfs:label "IEC 61400-25-1:2017"@en ;
  foaf:maker sto:IEC ;
  sto:hasAvailableLanguage lang:eng ;
  sto:hasEdition "2.0"^^xsd:float ;
  sto:hasFileSize sto:FileSizeIEC_61400_P25_S1 ;
  sto:hasICS sto:ICS_27_180 ;
  sto:hasOfficialResource <https://webstore.iec.ch/publication/61087> ;
  sto:hasPages "109"^^xsd:int ;
  sto:hasPublicationDate "2017-07-20"^^xsd:date ;
  sto:hasPublisher sto:IEC ;
  sto:hasStabilityDate "2020"^^xsd:gYear ;
  sto:hasTag "IEC 61400-25-1:2017"@en ;
  sto:hasTechnicalCommittee sto:TC_88 ;
.
sto:IEC_61400_P25_S2_E2
  a owl:NamedIndividual ;
  a sto:Standard ;
  terms:creator sto:IEC ;
  terms:language lang:eng ;
  terms:language lang:fra ;
  terms:title "Wind turbines - Part 25-2: Communications for monitoring and control of wind power plants - Information models"@en ;
  rdfs:comment """IEC 61400-25-2:2015 specifies the information model of devices and functions related to wind power plant applications. In particular, it specifies the compatible logical node names, and data names for communication between wind power plant components. This includes the relationship between logical devices, logical nodes and data. The names defined in the IEC 61400-25 series are used to build the hierarchical object references applied for communicating with components in wind power plants. Main changes with respect to the previous edition consist of:
- harmonization with newer editions of IEC 61850 standards;
- reduction of overlap between standards and simplification by increased referencing,
- extension of data objects for operation of smart grids,
- extended and enhanced semantics for existing data objects, etc."""@en ;
  rdfs:comment "IEC 61400-25-2:2015 specifies the information model of devices and functions related to wind power plant applications. In particular, it specifies the compatible logical node names, and data names for communication between wind power plant components. This includes the relationship between logical devices, logical nodes and data. The names defined in the IEC 61400-25 series are used to build the hierarchical object references applied for communicating with components in wind power plants. Main changes with respect to the previous edition consist of:- harmonization with newer editions of IEC 61850 standards;- reduction of overlap between standards and simplification by increased referencing,- extension of data objects for operation of smart grids,- extended and enhanced semantics for existing data objects, etc."@en ;
  rdfs:comment "IEC 61400-25-2:2015 specifies the information model of devices and functions related to wind power plant applications. In particular, it specifies the compatible logical node names, and data names for communication between wind power plant components. This includes the relationship between logical devices, logical nodes and data. The names defined in the IEC 61400-25 series are used to build the hierarchical object references applied for communicating with components in wind power plants. Main changes with respect to the previous edition consist of:n- harmonization with newer editions of IEC 61850 standards;n- reduction of overlap between standards and simplification by increased referencing,n- extension of data objects for operation of smart grids,n- extended and enhanced semantics for existing data objects, etc."@en ;
  rdfs:label "IEC 61400-25-2:2015 "@en ;
  foaf:maker sto:IEC ;
  sto:hasAvailableLanguage lang:eng ;
  sto:hasAvailableLanguage lang:fra ;
  sto:hasEdition "2.0"^^xsd:float ;
  sto:hasFileSize sto:FileSizeIEC_61400_P25_S2 ;
  sto:hasICS sto:ICS_27_180 ;
  sto:hasOfficialResource <https://webstore.iec.ch/publication/22813> ;
  sto:hasPages "221"^^xsd:int ;
  sto:hasPublicationDate "2015-06-30"^^xsd:date ;
  sto:hasPublisher sto:IEC ;
  sto:hasStabilityDate "2018"^^xsd:gYear ;
  sto:hasTag "IEC 61400-25-2:2015 "@en ;
  sto:hasTechnicalCommittee sto:TC_88 ;
.
sto:IEC_61400_P25_S3_E2
  a owl:NamedIndividual ;
  a sto:Standard ;
  terms:creator sto:IEC ;
  terms:language lang:eng ;
  terms:title "Wind turbines - Part 25-3: Communications for monitoring and control of wind power plants - Information exchange models"@en ;
  rdfs:comment """IEC 61400-25-3:2015 RLV contains the International Standard and its Redline version. The Redline version is available in English only. The Redline version provides you with a quick and easy way to compare all the changes between this standard and its previous edition. The Redline version is not an official IEC Standard, only the current version of the standard is to be considered the official document.
IEC 61400-25-3:2015 specifies an abstract communication service interface describing the information exchange between a client and a server for:
- data access and retrieval,
- device control,
- event reporting and logging,
- self-description of devices (device data dictionary),
- data typing and discovery of data types.
Main changes with respect to the previous edition consist of:
- harmonization with newer editions of IEC 61850 standards;
- reduction of overlap between standards and simplification by increased referencing, etc."""@en ;
  rdfs:comment "IEC 61400-25-3:2015 RLV contains the International Standard and its Redline version. The Redline version is available in English only. The Redline version provides you with a quick and easy way to compare all the changes between this standard and its previous edition. The Redline version is not an official IEC Standard, only the current version of the standard is to be considered the official document.IEC 61400-25-3:2015 specifies an abstract communication service interface describing the information exchange between a client and a server for:- data access and retrieval,- device control,- event reporting and logging,- self-description of devices (device data dictionary),- data typing and discovery of data types.Main changes with respect to the previous edition consist of:- harmonization with newer editions of IEC 61850 standards;- reduction of overlap between standards and simplification by increased referencing, etc."@en ;
  rdfs:comment "IEC 61400-25-3:2015 RLV contains the International Standard and its Redline version. The Redline version is available in English only. The Redline version provides you with a quick and easy way to compare all the changes between this standard and its previous edition. The Redline version is not an official IEC Standard, only the current version of the standard is to be considered the official document.nIEC 61400-25-3:2015 specifies an abstract communication service interface describing the information exchange between a client and a server for:n- data access and retrieval,n- device control,n- event reporting and logging,n- self-description of devices (device data dictionary),n- data typing and discovery of data types.nMain changes with respect to the previous edition consist of:n- harmonization with newer editions of IEC 61850 standards;n- reduction of overlap between standards and simplification by increased referencing, etc."@en ;
  rdfs:label "IEC 61400-25-3:2015"@en ;
  foaf:maker sto:IEC ;
  sto:hasAvailableLanguage lang:eng ;
  sto:hasEdition "2.0"^^xsd:float ;
  sto:hasFileSize sto:FileSizeIEC_61400_P25_S3 ;
  sto:hasICS sto:ICS_27_180 ;
  sto:hasOfficialResource <https://webstore.iec.ch/publication/22808> ;
  sto:hasPages "103"^^xsd:int ;
  sto:hasPublicationDate "2015-06-30"^^xsd:date ;
  sto:hasPublisher sto:IEC ;
  sto:hasStabilityDate "2018"^^xsd:gYear ;
  sto:hasTag "IEC 61400-25-3:2015"@en ;
  sto:hasTechnicalCommittee sto:TC_88 ;
.
sto:IEC_61400_P25_S4_E2
  a owl:NamedIndividual ;
  a sto:Standard ;
  terms:creator sto:IEC ;
  terms:language lang:eng ;
  terms:title "Wind energy generation systems - Part 25-4: Communications for monitoring and control of wind power plants - Mapping to communication profile"@en ;
  rdfs:comment """IEC 61400-25-4:2016 RLV contains the International Standard and its Redline version. The Redline version is available in English only. The Redline version provides you with a quick and easy way to compare all the changes between this standard and its previous edition. The Redline version is not an official IEC Standard, only the current version of the standard is to be considered the official document.

IEC 61400-25-4:2016 specifies the specific mappings to protocol stacks encoding the messages required for the information exchange between a client and a remote server for: data access and retrieval, device control, event reporting and logging, publisher/subscriber, self-description of devices (device data dictionary), data typing and discovery of data types. The mappings specified in this part of IEC 61400-25 comprise:
- a mapping to SOAP-based web services,
- a mapping to OPC/XML-DA,
- a mapping to IEC 61850-8-1 MMS,
- a mapping to IEC 60870-5-104,
- a mapping to DNP3.
The main technical changes with regard to the previous edition are as follows:
- general harmonization with information models in IEC 61400-25-2 and information exchange services in IEC 61400-25-3;
- reduction of overlap between standards and simplification by increased referencing."""@en ;
  rdfs:comment "IEC 61400-25-4:2016 RLV contains the International Standard and its Redline version. The Redline version is available in English only. The Redline version provides you with a quick and easy way to compare all the changes between this standard and its previous edition. The Redline version is not an official IEC Standard, only the current version of the standard is to be considered the official document.nnIEC 61400-25-4:2016 specifies the specific mappings to protocol stacks encoding the messages required for the information exchange between a client and a remote server for: data access and retrieval, device control, event reporting and logging, publisher/subscriber, self-description of devices (device data dictionary), data typing and discovery of data types. The mappings specified in this part of IEC 61400-25 comprise:n- a mapping to SOAP-based web services,n- a mapping to OPC/XML-DA,n- a mapping to IEC 61850-8-1 MMS,n- a mapping to IEC 60870-5-104,n- a mapping to DNP3.nThe main technical changes with regard to the previous edition are as follows:n- general harmonization with information models in IEC 61400-25-2 and information exchange services in IEC 61400-25-3;n- reduction of overlap between standards and simplification by increased referencing."@en ;
  rdfs:label "IEC 61400-25-4:2016"@en ;
  foaf:maker sto:IEC ;
  sto:hasAvailableLanguage lang:eng ;
  sto:hasEdition "2.0"^^xsd:float ;
  sto:hasFileSize sto:FileSizeIEC_61400_P25_S4 ;
  sto:hasICS sto:ICS_27_180 ;
  sto:hasOfficialResource <https://webstore.iec.ch/publication/59497> ;
  sto:hasPages "829"^^xsd:int ;
  sto:hasPublicationDate "2016-11-30"^^xsd:date ;
  sto:hasPublisher sto:IEC ;
  sto:hasStabilityDate "2018"^^xsd:gYear ;
  sto:hasTag "IEC 61400-25-4:2016"@en ;
  sto:hasTechnicalCommittee sto:TC_88 ;
.
sto:IEC_61400_P25_S5_E2
  a owl:NamedIndividual ;
  a sto:Standard ;
  terms:creator sto:IEC ;
  terms:language lang:eng ;
  terms:title "Wind energy generation systems - Part 25-5: Communications for monitoring and control of wind power plants - Compliance testing"@en ;
  rdfs:comment """IEC 61400-25-5:2017 specifies standard techniques for testing of compliance of implementations, as well as specific measurement techniques to be applied when declaring performance parameters. The use of these techniques will enhance the ability of users to purchase systems that integrate easily, operate correctly, and support the applications as intended. This part of IEC 61400-25 defines: the methods and abstract test cases for compliance testing of server and client devices used in wind power plants; the metrics to be measured in said devices according to the communication requirements specified in IEC 61400-25 (all parts). This new edition includes the following significant technical changes with respect to the previous edition:
- harmonization with structure and test cases in IEC 61850-10:2012;
- reduction of overlap between standards and simplification by increased referencing to the IEC 61850 standard series."""@en ;
  rdfs:comment "IEC 61400-25-5:2017 specifies standard techniques for testing of compliance of implementations, as well as specific measurement techniques to be applied when declaring performance parameters. The use of these techniques will enhance the ability of users to purchase systems that integrate easily, operate correctly, and support the applications as intended. This part of IEC 61400-25 defines: the methods and abstract test cases for compliance testing of server and client devices used in wind power plants; the metrics to be measured in said devices according to the communication requirements specified in IEC 61400-25 (all parts). This new edition includes the following significant technical changes with respect to the previous edition:n- harmonization with structure and test cases in IEC 61850-10:2012;n- reduction of overlap between standards and simplification by increased referencing to the IEC 61850 standard series."@en ;
  rdfs:label "IEC 61400-25-5:2017"@en ;
  foaf:maker sto:IEC ;
  sto:hasAvailableLanguage lang:eng ;
  sto:hasEdition "2.0"^^xsd:float ;
  sto:hasFileSize sto:FileSizeIEC_61400_P25_S5 ;
  sto:hasICS sto:ICS_27_180 ;
  sto:hasOfficialResource <https://webstore.iec.ch/publication/26560> ;
  sto:hasPages "56"^^xsd:int ;
  sto:hasPublicationDate "2017-09-20"^^xsd:date ;
  sto:hasPublisher sto:IEC ;
  sto:hasStabilityDate "2020"^^xsd:gYear ;
  sto:hasTag "IEC 61400-25-5:2017"@en ;
  sto:hasTechnicalCommittee sto:TC_88 ;
.
sto:IEC_61400_P25_S6_E2
  a owl:NamedIndividual ;
  a sto:Standard ;
  terms:creator sto:IEC ;
  terms:language lang:eng ;
  terms:title "Wind energy generation systems - Part 25-6: Communications for monitoring and control of wind power plants - Logical node classes and data classes for condition monitoring"@en ;
  rdfs:comment """IEC 61400-25-6:2016(E) specifies the information models related to condition monitoring for wind power plants and the information exchange of data values related to these models. This standard is to be used with other standards of the IEC 61400-25 series. This new edition includes the following significant technical changes with respect to the previous edition:
- major restructuring of the data model to accommodate flexibility; removal of UFF58 format;
- access to data using the standard reporting and logging functions;
- recommendations for creating data names to accommodate flexibility."""@en ;
  rdfs:comment "IEC 61400-25-6:2016(E) specifies the information models related to condition monitoring for wind power plants and the information exchange of data values related to these models. This standard is to be used with other standards of the IEC 61400-25 series. This new edition includes the following significant technical changes with respect to the previous edition:n- major restructuring of the data model to accommodate flexibility; removal of UFF58 format;n- access to data using the standard reporting and logging functions;n- recommendations for creating data names to accommodate flexibility."@en ;
  rdfs:label "IEC 61400-25-6:2016"@en ;
  foaf:maker sto:IEC ;
  sto:hasAvailableLanguage lang:eng ;
  sto:hasEdition "2.0"^^xsd:float ;
  sto:hasFileSize sto:FileSizeIEC_61400_P25_S6 ;
  sto:hasICS sto:ICS_27_180 ;
  sto:hasOfficialResource <https://webstore.iec.ch/publication/32580> ;
  sto:hasPages "49"^^xsd:int ;
  sto:hasPublicationDate "2016-12-16"^^xsd:date ;
  sto:hasPublisher sto:IEC ;
  sto:hasStabilityDate "2019"^^xsd:gYear ;
  sto:hasTechnicalCommittee sto:TC_88 ;
.
sto:IEC_61499
  a owl:NamedIndividual ;
  a foaf:Document ;
  a sto:Publication ;
  a sto:Standard ;
  terms:creator sto:IEC ;
  rdfs:comment "Function Blocks - Architecture Related Applications http://www.eclipse.org/4diac/ (sourceforge.net/projects/oooneida-fbench/) http://timeme.io/  not accepted by the Industry yet. http://www.holobloc.com/Proposed for IEC to overcome the restricctions of IEC 61131"@en ;
  rdfs:label "IEC 61499"@en ;
  foaf:maker sto:IEC ;
  sto:hasClassification sto:RAMIControlDevice ;
  sto:hasClassification sto:RAMIFieldDevice ;
  sto:hasDBpediaResource <http://dbpedia.org/resource/IEC_61499> ;
  sto:hasMotivation "Functional description, informational representation and communication mapping of application functionality. This standard describes how a distributed control application is composed of functional units (FB), which are executed in different context. It may help to describe how functions are distributed between different I40-Components and how the execution of the functions between the different I40-Components is controled."@en ;
  sto:hasOfficialResource <https://webstore.iec.ch/publication/5506> ;
  sto:hasPublicationDate "2012-11-07"^^xsd:date ;
  sto:hasPublisher sto:IEC ;
  sto:hasTag "FBs distributed systems"@en ;
  sto:hasWikipediaArticle <https://en.wikipedia.org/wiki/IEC_61499> ;
  sto:relatedTo sto:DIN_SPEC_16592 ;
  sto:relatedTo sto:IEC_61131 ;
  sto:relatedTo sto:IEC_61360 ;
  sto:relatedTo sto:IEC_61499 ;
  sto:relatedTo sto:IEC_61804 ;
  sto:relatedTo sto:IEC_61850 ;
  sto:relatedTo sto:IEC_61987_X ;
  sto:relatedTo sto:IEC_62424 ;
  sto:relatedTo sto:IEC_62453 ;
  sto:relatedTo sto:IEC_62541 ;
  sto:relatedTo sto:IEC_62714 ;
  sto:relatedTo sto:ISO_13584 ;
  sto:relatedTo sto:ISO_14306 ;
  sto:relatedTo sto:ISO_15746 ;
  sto:relatedTo sto:ISO_15926 ;
  sto:relatedTo sto:ISO_18629 ;
  sto:relatedTo sto:ISO_18828-2 ;
  sto:relatedTo sto:ISO_20922 ;
  sto:relatedTo sto:ISO_22400 ;
  sto:relatedTo sto:ISO_29002 ;
  sto:relatedTo sto:ISO_ASTM_52915 ;
  sto:relatedTo sto:ISO_PAS_17506 ;
  sto:relatedTo sto:MathML ;
  sto:relatedTo sto:SysML ;
  sto:relatedTo sto:eClass ;
.
sto:IEC_61506
  a owl:NamedIndividual ;
  a foaf:Document ;
  a sto:Publication ;
  a sto:Standard ;
  terms:creator sto:IEC ;
  terms:language lang:eng ;
  terms:language lang:fra ;
  terms:title "Industrial-process measurement and control - Documentation ofapplication software"@en ;
  rdfs:comment "Defines the requirements for the documentation of software in industrial process measurement and control systems."@en ;
  rdfs:label "IEC 61506:1997"@en ;
  foaf:maker sto:IEC ;
  sto:hasAvailableLanguage lang:eng ;
  sto:hasAvailableLanguage lang:fra ;
  sto:hasEdition "1.0"^^xsd:float ;
  sto:hasFileSize sto:FileSizeIEC_61506 ;
  sto:hasICS sto:ICS_25_040_40 ;
  sto:hasOfficialResource <https://webstore.iec.ch/publication/5513> ;
  sto:hasPages "119"^^xsd:int ;
  sto:hasPublicationDate "1997-02-28"^^xsd:date ;
  sto:hasPublisher sto:IEC ;
  sto:hasStabilityDate "2018"^^xsd:gYear ;
  sto:hasTag "IEC 61506:1997"@en ;
  sto:hasTechnicalCommittee sto:TC_65 ;
.
sto:IEC_61508
  a owl:NamedIndividual ;
  a foaf:Document ;
  a sto:Publication ;
  a sto:Standard ;
  terms:creator sto:IEC ;
  terms:creator sto:ISO ;
  terms:license sto:PrivateLicenseDocument ;
  rdfs:comment "Functional safety is a concept applicable across all industry sectors. It is fundamental to the enabling of complex technology used for safety-related systems. It provides the assurance that the safety-related systems will offer the necessary risk reduction required to achieve safety for the equipment. The oil and gas industry, nuclear plants and the machinery sector, to name but a few, all rely heavily on functional safety to achieve safety for the equipment giving rise to the hazards."@en ;
  rdfs:label "IEC 61508"@en ;
  owl:sameAs sto:ISO_61508 ;
  foaf:maker sto:IEC ;
  foaf:maker sto:ISO ;
  <https://w3id.org/i40/hasTargetConcern> sto:Safety ;
  sto:frames sto:Safety ;
  sto:hasClassification rami:Safety ;
  sto:hasClassification sto:IDSRAMCertification ;
  sto:hasClassification sto:Safety ;
  sto:hasDBpediaResource <http://dbpedia.org/resource/IEC_61508> ;
  sto:hasMotivation "Defines the functional safety requirements established by IEC 61508 in process industry sector terminology"@en ;
  sto:hasOfficialResource <http://www.iec.ch/functionalsafety/> ;
  sto:hasPublicationDate "1997-02-28"^^xsd:date ;
  sto:hasPublisher sto:IEC ;
  sto:hasPublisher sto:ISO ;
  sto:hasTag "Functional Safety of Electrical/Electronic/Programmable Electronic Safety-related Systems"@en ;
  sto:hasWikipediaArticle <https://en.wikipedia.org/wiki/IEC_61508> ;
  sto:relatedTo sto:IEC_61508 ;
  sto:relatedTo sto:IEC_61511 ;
  sto:relatedTo sto:IEC_62061 ;
  sto:relatedTo sto:ISO_13849 ;
.
sto:IEC_61511
  a owl:NamedIndividual ;
  a foaf:Document ;
  a sto:Publication ;
  a sto:Standard ;
  terms:creator sto:IEC ;
  terms:license sto:PrivateLicenseDocument ;
  rdfs:comment "IEC 61511 is a technical standard which sets out practices in the engineering of systems that ensure the safety of an industrial process through the use of instrumentation."@en ;
  rdfs:label "IEC 61511" ;
  foaf:maker sto:IEC ;
  <https://w3id.org/i40/hasTargetConcern> sto:Safety ;
  sto:hasClassification sto:IDSRAMCertification ;
  sto:hasDBpediaResource <http://dbpedia.org/resource/IEC_61511> ;
  sto:hasDomain sto:FunctionalSafety ;
  sto:hasMotivation "Defines the functional safety requirements established by IEC 61508 in process industry sector terminology"@en ;
  sto:hasOfficialResource <https://webstore.iec.ch/publication/24241> ;
  sto:hasPublicationDate "2016-02-24"^^xsd:date ;
  sto:hasPublisher sto:IEC ;
  sto:hasTag "Functional safety - Safety instrumented systems for the process industry sector"@en ;
  sto:hasWikipediaArticle <https://en.wikipedia.org/wiki/IEC_61511> ;
  sto:relatedTo sto:IEC_61508 ;
  sto:relatedTo sto:IEC_61511 ;
  sto:relatedTo sto:IEC_62061 ;
  sto:relatedTo sto:ISO_13849 ;
.
sto:IEC_61512
  a owl:NamedIndividual ;
  a foaf:Document ;
  a sto:Publication ;
  a sto:Standard ;
  terms:creator sto:IEC ;
  rdfs:comment "Batch control - Models and terminology"@en ;
  rdfs:label "IEC 61512"@en ;
  foaf:maker sto:IEC ;
  sto:hasClassification sto:RAMIControlDevice ;
  sto:hasClassification sto:RAMIProduct ;
  sto:hasClassification sto:RAMIStation ;
  sto:hasClassification sto:RAMIWorkCenter ;
  sto:hasDBpediaResource <http://dbpedia.org/resource/ISA-88> ;
  sto:hasMotivation "The standard sought to address the following problems: lack of a universal model for batch control, difficulty in communicating user requirement, integration among batch automation suppliers, difficulty in batch control configuration."@en ;
  sto:hasOfficialResource <https://webstore.iec.ch/publication/5528> ;
  sto:hasPublisher sto:IEC ;
  sto:hasTag "ISA-88"@en ;
  sto:hasWikipediaArticle <https://en.wikipedia.org/wiki/ISA-88> ;
.
sto:IEC_61513
  a owl:NamedIndividual ;
  a foaf:Document ;
  a sto:Publication ;
  a sto:Standard ;
  terms:creator sto:IEC ;
  rdfs:comment "IEC 61508 is intended to be a basic functional safety standard applicable to all kinds of industry. It defines functional safety as: “part of the overall safety relating to the EUC (Equipment Under Control) and the EUC control system which depends on the correct functioning of the E/E/PE safety-related systems, other technology safety-related systems and external risk reduction facilities.\""@en ;
  rdfs:label "IEC 61513"@en ;
  foaf:maker sto:IEC ;
  sto:hasClassification sto:Safety ;
  sto:hasOfficialResource <https://webstore.iec.ch/publication/5532> ;
  sto:hasPublisher sto:IEC ;
  sto:hasWikipediaArticle <https://en.wikipedia.org/wiki/IEC_61508> ;
.
sto:IEC_61690_P1_E1
  a owl:NamedIndividual ;
  a sto:Standard ;
  terms:creator sto:IEC ;
  terms:language lang:eng ;
  terms:language lang:fra ;
  terms:title "Electronic design interchange format (EDIF) - Part 1: Version 3 0 0. (This publication is available in electronic HTML format only)"@en ;
  rdfs:comment "IEC 61690-1:2000 defines the syntax and semantics for EDIF Version 3 0 0. EDIF Version 3 0 0 addresses EDIF Level 0 and Level 1. EDIF Version 3 0 0 completely addresses the Connectivity and Schematic views, including at Level 1 the ability to represent frames. It includes capabilities formerly found in the Document and Graphics views. A series of releases is planned in the near future to address those views not completely addressed in this version."@en ;
  rdfs:label "IEC 61690-1:2000"@en ;
  foaf:maker sto:IEC ;
  sto:hasAvailableLanguage lang:eng ;
  sto:hasAvailableLanguage lang:fra ;
  sto:hasEdition "1.0"^^xsd:float ;
  sto:hasFileSize sto:FileSizeIEC_61690_P1 ;
  sto:hasICS sto:ICS_35_240_50 ;
  sto:hasOfficialResource <https://webstore.iec.ch/publication/5723> ;
  sto:hasPublicationDate "2000-01-31"^^xsd:date ;
  sto:hasPublisher sto:IEC ;
  sto:hasStabilityDate "2018"^^xsd:gYear ;
  sto:hasTechnicalCommittee sto:TC_91 ;
.
sto:IEC_61690_P2_E1
  a owl:NamedIndividual ;
  a sto:Standard ;
  terms:creator sto:IEC ;
  terms:language lang:eng ;
  terms:language lang:fra ;
  terms:title "Electronic design interchange format (EDIF) - Part 2: Version 4 0 0. (This publication is available in electronic HTML format only)"@en ;
  rdfs:comment "IEC 61690-2:2000 defines the syntax and semantics for EDIF Version 4 0 0. EDIF Version 4 0 0 addresses EDIF Level 0 and Level 1. EDIF Version 3 0 0 provides support for Connectivity and Schematics; EDIF Version 4 0 0 offers additional capability by providing support for the representation of Printed Circuit Boards (PCBs) and Multi-chip Modules (MCMs) including technology rules and assembly drawings."@en ;
  rdfs:label "IEC 61690-2:2000"@en ;
  foaf:maker sto:IEC ;
  sto:hasAvailableLanguage lang:eng ;
  sto:hasAvailableLanguage lang:fra ;
  sto:hasEdition "1.0"^^xsd:float ;
  sto:hasFileSize sto:FileSizeIEC_61690_P2 ;
  sto:hasICS sto:ICS_35_240_50 ;
  sto:hasOfficialResource <https://webstore.iec.ch/publication/5724> ;
  sto:hasPublicationDate "2000-01-31"^^xsd:date ;
  sto:hasPublisher sto:IEC ;
  sto:hasStabilityDate "2018"^^xsd:gYear ;
  sto:hasTechnicalCommittee sto:TC_91 ;
.
sto:IEC_61691_P6_E1
  a owl:NamedIndividual ;
  a sto:Standard ;
  terms:creator sto:IEC ;
  terms:language lang:eng ;
  terms:title "Behavioural languages - Part 6: VHDL Analog and Mixed-Signal Extensions"@en ;
  rdfs:comment "IEC 61691-6:2009(E) Defines IEC 61691-6/IEEE Std 1076.1 language, a hardware description language for the description and the simulation of analog, digital, and mixed-signal systems. The language, also informally known as VHDLAMS, is built on the IEC 61691-1-1/IEEE 1076 (VHDL) language and extends it to provide capabilities of writing and simulating analog and mixed-signal models."@en ;
  rdfs:label "IEC 61691-6:2009"@en ;
  foaf:maker sto:IEC ;
  sto:hasAvailableLanguage lang:eng ;
  sto:hasEdition "1.0"^^xsd:float ;
  sto:hasFileSize sto:FileSizeIEC_61691_P6 ;
  sto:hasICS sto:ICS_25_040_01 ;
  sto:hasICS sto:ICS_35_060 ;
  sto:hasOfficialResource <https://webstore.iec.ch/publication/5726> ;
  sto:hasPages "332"^^xsd:int ;
  sto:hasPublicationDate "2009-12-14"^^xsd:date ;
  sto:hasPublisher sto:IEC ;
  sto:hasStabilityDate "2018"^^xsd:gYear ;
  sto:hasTechnicalCommittee sto:TC_91 ;
.
sto:IEC_61784
  a owl:NamedIndividual ;
  a foaf:Document ;
  a sto:Publication ;
  a sto:Standard ;
  terms:creator sto:IEC ;
  terms:license sto:PrivateLicenseDocument ;
  rdfs:comment "Industrial communication networks - Profiles - Ethernet-real-time-enabled"@en ;
  rdfs:label "IEC 61784"@en ;
  foaf:maker sto:IEC ;
  sto:hasClassification sto:RAMICommunicationlayer ;
  sto:hasClassification sto:RAMIControlDevice ;
  sto:hasClassification sto:RAMIFieldDevice ;
  sto:hasDBpediaResource <http://dbpedia.org/page/Profibus> ;
  sto:hasMotivation "Information description and communication mapping for fieldbus profiles"@en ;
  sto:hasOfficialResource <https://webstore.iec.ch/publication/5878> ;
  sto:hasPublicationDate "2014-08-19"^^xsd:date ;
  sto:hasPublisher sto:IEC ;
  sto:hasTag "IEC Fieldbus (Profibus)"@en ;
  sto:relatedTo sto:IEC_29182-1 ;
  sto:relatedTo sto:IEC_61158 ;
  sto:relatedTo sto:IEC_61784 ;
  sto:relatedTo sto:OMG_DDS ;
.
sto:IEC_61804
  a owl:NamedIndividual ;
  a foaf:Document ;
  a sto:Publication ;
  a sto:Standard ;
  terms:creator sto:IEC ;
  rdfs:comment "Function blocks (FB) for process control - Overview of system aspects "@en ;
  rdfs:label "IEC 61804"@en ;
  foaf:maker sto:IEC ;
  sto:hasClassification rami:Configuration ;
  sto:hasClassification sto:RAMIControlDevice ;
  sto:hasClassification sto:RAMIFieldDevice ;
  sto:hasDBpediaResource <http://dbpedia.org/resource/Device_Description_Language> ;
  sto:hasOfficialResource <https://webstore.iec.ch/publication/5953> ;
  sto:hasPublisher sto:IEC ;
  sto:hasTag "EDDL"@en ;
  sto:hasWikipediaArticle <https://en.wikipedia.org/wiki/Device_Description_Language> ;
  sto:relatedTo sto:DIN_SPEC_16592 ;
  sto:relatedTo sto:IEC_61131 ;
  sto:relatedTo sto:IEC_61360 ;
  sto:relatedTo sto:IEC_61499 ;
  sto:relatedTo sto:IEC_61804 ;
  sto:relatedTo sto:IEC_61850 ;
  sto:relatedTo sto:IEC_61987_X ;
  sto:relatedTo sto:IEC_62424 ;
  sto:relatedTo sto:IEC_62453 ;
  sto:relatedTo sto:IEC_62541 ;
  sto:relatedTo sto:IEC_62714 ;
  sto:relatedTo sto:ISO_13584 ;
  sto:relatedTo sto:ISO_14306 ;
  sto:relatedTo sto:ISO_15746 ;
  sto:relatedTo sto:ISO_15926 ;
  sto:relatedTo sto:ISO_18629 ;
  sto:relatedTo sto:ISO_18828-2 ;
  sto:relatedTo sto:ISO_20922 ;
  sto:relatedTo sto:ISO_22400 ;
  sto:relatedTo sto:ISO_29002 ;
  sto:relatedTo sto:ISO_ASTM_52915 ;
  sto:relatedTo sto:ISO_PAS_17506 ;
  sto:relatedTo sto:MathML ;
  sto:relatedTo sto:SysML ;
  sto:relatedTo sto:eClass ;
.
sto:IEC_61804_P3
  a owl:NamedIndividual ;
  a sto:Standard ;
  terms:creator sto:IEC ;
  terms:title "Function Blocks (FB) for process control and Electronic Device Description Language (EDDL) - Part 3: EDDL syntax and semantics"@en ;
  rdfs:comment "IEC 61804-3:2015 specifies the Electronic Device Description Language (EDDL) technology, which enables the integration of real product details using the tools of the engineering life cycle. It specifies EDDL as a generic language for describing the properties of automation system components. This third edition cancels and replaces the second edition published in 2010. This edition constitutes a technical revision. This edition includes the following significant technical changes with respect to the previous edition: Builtins and their profiles removed and relocated into IEC 61804-5. The following extensions are integrated in the EDDL specification to meet FDI requirements: - new contructs BLOB, PLUGIN; - component construct for communication server requirements (additional attributes); - extension of the class attribute; - new attributes PRIVATE, VISIBILITY, WRITE_MODE"@en ;
  rdfs:label "IEC 61804-3:2015"@en ;
  foaf:maker sto:IEC ;
  sto:frames sto:ThingDescription ;
  sto:hasAvailableLanguage lang:eng ;
  sto:hasAvailableLanguage lang:fra ;
  sto:hasEdition "3.0"^^xsd:float ;
  sto:hasFileSize sto:FileSizeIEC_61804_P3 ;
  sto:hasICS sto:ICS_25_040_40 ;
  sto:hasICS sto:ICS_35_240_50 ;
  sto:hasOfficialResource <https://webstore.iec.ch/publication/22636> ;
  sto:hasPages "694"^^xsd:int ;
  sto:hasPublicationDate "2015-06-09"^^xsd:date ;
  sto:hasPublisher sto:IEC ;
  sto:hasStabilityDate "2019"^^xsd:gYear ;
  sto:hasTag "IEC 61804-3:2015"@en ;
  sto:hasTechnicalCommittee sto:TC_65 ;
.
sto:IEC_61804_P4
  a owl:NamedIndividual ;
  a sto:Standard ;
  terms:creator sto:IEC ;
  terms:title "Function blocks (FB) for process control and electronic device description language (EDDL) - Part 4: EDD interpretation"@en ;
  rdfs:comment "IEC 61804-4:2015 specifies EDD interpretation for EDD applications and EDDs to support EDD interoperability. This document is intended to ensure that field device developers use the EDDL constructs consistently and that the EDD applications have the same interpretations of the EDD. It supplements the EDDL specification to promote EDDL application interoperability and improve EDD portability between EDDL applications. This first edition cancels and replaces IEC TR 61804-4 published in 2006. This edition constitutes a technical revision. This edition includes the following significant technical changes with respect to the previous edition: - New paragraph: EDDL data description; - EDDL METHOD programming and usage of builtins; - Edit session; - Offline and online configuration; - EDDL communication description and Enhancements in paragraph EDDL user interface descriptions."@en ;
  rdfs:label "IEC 61804-4:2015"@en ;
  foaf:maker sto:IEC ;
  sto:frames sto:ThingDescription ;
  sto:hasAvailableLanguage lang:eng ;
  sto:hasAvailableLanguage lang:fra ;
  sto:hasEdition "1.0"^^xsd:float ;
  sto:hasFileSize sto:FileSizeIEC_61804_P4 ;
  sto:hasICS sto:ICS_25_040_40 ;
  sto:hasICS sto:ICS_35_240_50 ;
  sto:hasOfficialResource <https://webstore.iec.ch/publication/23481> ;
  sto:hasPages "253"^^xsd:int ;
  sto:hasPublicationDate "2015-10-07"^^xsd:date ;
  sto:hasPublisher sto:IEC ;
  sto:hasStabilityDate "2019"^^xsd:gYear ;
  sto:hasTag "IEC 61804-4:2015"@en ;
  sto:hasTechnicalCommittee sto:TC_65 ;
.
sto:IEC_61804_P5
  a owl:NamedIndividual ;
  a sto:Standard ;
  terms:creator sto:IEC ;
  terms:title "Function blocks (FB) for process control and electronic device description language (EDDL) - Part 5: EDDL Builtin library"@en ;
  rdfs:comment "IEC 61804-5:2015 specifies the EDDL Builtin library and provides the profiles of the various fieldbuses."@en ;
  rdfs:label "IEC 61804-5:2015 "@en ;
  foaf:maker sto:IEC ;
  sto:frames sto:ThingDescription ;
  sto:hasAvailableLanguage lang:eng ;
  sto:hasAvailableLanguage lang:fra ;
  sto:hasEdition "1.0"^^xsd:float ;
  sto:hasFileSize sto:FileSizeIEC_61804_P5 ;
  sto:hasICS sto:ICS_25_040_40 ;
  sto:hasICS sto:ICS_35_240_50 ;
  sto:hasOfficialResource <https://webstore.iec.ch/publication/22637> ;
  sto:hasPages "472"^^xsd:int ;
  sto:hasPublicationDate "2015-06-09"^^xsd:date ;
  sto:hasPublisher sto:IEC ;
  sto:hasStabilityDate "2019"^^xsd:gYear ;
  sto:hasTag "IEC 61804-5:2015 "@en ;
  sto:hasTechnicalCommittee sto:TC_65 ;
.
sto:IEC_61804_P6
  a owl:NamedIndividual ;
  a sto:TechnicalReport ;
  terms:creator sto:IEC ;
  terms:title "Function blocks (FB) for process control - Electronic device description language (EDDL) - Part 6: Meeting the requirements for integrating fieldbus devices in engineering tools for field devices"@en ;
  rdfs:comment "IEC/TR 61804-6:2012(E) provides an evaluation and assessment of electronic device description language (EDDL) technology. It provides guidance to device and system manufacturers for how EDDL technology can help them meet user requirements. It provides guidance to system integrators, as well as instrumentation and maintenance practitioners at end-user companies, on how EDDL technology can help them integrate systems and incorporate device management in their work processes. It gives examples of requirements from the NAMUR NE 105 recommendation. It's intent is to illustrate how EDDL technology and products based on EDDL technology meet these requirements."@en ;
  rdfs:label "IEC 61804-6:2012 "@en ;
  foaf:maker sto:IEC ;
  sto:frames sto:ThingDescription ;
  sto:hasAvailableLanguage lang:eng ;
  sto:hasAvailableLanguage lang:fra ;
  sto:hasEdition "1.0"^^xsd:float ;
  sto:hasFileSize sto:FileSizeIEC_61804_P6 ;
  sto:hasICS sto:ICS_25_040_40 ;
  sto:hasICS sto:ICS_35_240_50 ;
  sto:hasOfficialResource <https://webstore.iec.ch/publication/59577> ;
  sto:hasPages "15"^^xsd:int ;
  sto:hasPublicationDate "2012-04-04"^^xsd:date ;
  sto:hasPublisher sto:IEC ;
  sto:hasStabilityDate "2022"^^xsd:gYear ;
  sto:hasTag "IEC 61804-6:2012  "@en ;
  sto:hasTechnicalCommittee sto:TC_65 ;
.
sto:IEC_61810_P2_E3
  a owl:NamedIndividual ;
  a sto:Standard ;
  terms:creator sto:IEC ;
  terms:language lang:eng ;
  terms:language lang:fra ;
  terms:title "Electromechanical elementary relays - Part 2: Reliability"@en ;
  rdfs:comment """IEC 61810-2:2017 covers test conditions and provisions for the evaluation of endurance tests using appropriate statistical methods to obtain reliability characteristics for relays.
This document applies to electromechanical elementary relays considered as non-repaired items (i.e. items which are not repaired after failure).
This document does not cover procedures for electromechanical elementary relays where enhanced requirements for the verification of reliability apply.
This edition includes the following significant technical changes with respect to the previous edition:
- not only graphical but also numerical methods are added;
- reduction of number of samples in specified cases;
- new subclauses of confidence intervals are added;
- the WeiBayes approach is added to facilitate compliance tests (routine test) with lower effort;
- annexes have been restructured into an Annex A for data analysis (normative) and Annex B (informative) where various examples of the data analysis are given;
- the former Annex C has been incorporated into the modified Annex B;
- a new Annex C replaces the old Annex D."""@en ;
  rdfs:comment "IEC 61810-2:2017 covers test conditions and provisions for the evaluation of endurance tests using appropriate statistical methods to obtain reliability characteristics for relays.nThis document applies to electromechanical elementary relays considered as non-repaired items (i.e. items which are not repaired after failure).nThis document does not cover procedures for electromechanical elementary relays where enhanced requirements for the verification of reliability apply.nThis edition includes the following significant technical changes with respect to the previous edition:n- not only graphical but also numerical methods are added;n- reduction of number of samples in specified cases;n- new subclauses of confidence intervals are added;n- the WeiBayes approach is added to facilitate compliance tests (routine test) with lower effort;n- annexes have been restructured into an Annex A for data analysis (normative) and Annex B (informative) where various examples of the data analysis are given;n- the former Annex C has been incorporated into the modified Annex B;n- a new Annex C replaces the old Annex D."@en ;
  rdfs:label "IEC 61810-2:2017"@en ;
  foaf:maker sto:IEC ;
  sto:hasAvailableLanguage lang:eng ;
  sto:hasAvailableLanguage lang:fra ;
  sto:hasEdition "3.0"^^xsd:float ;
  sto:hasFileSize sto:FileSizeIEC_61810_P2 ;
  sto:hasICS sto:ICS_29_120_70 ;
  sto:hasOfficialResource <https://webstore.iec.ch/publication/33869> ;
  sto:hasPages "86"^^xsd:int ;
  sto:hasPublicationDate "2017-05-30"^^xsd:date ;
  sto:hasPublisher sto:IEC ;
  sto:hasStabilityDate "2020"^^xsd:gYear ;
  sto:hasTag "IEC 61810-2:2017"@en ;
  sto:hasTechnicalCommittee sto:TC_94 ;
.
sto:IEC_61810_P7_E2
  a owl:NamedIndividual ;
  a sto:Standard ;
  terms:creator sto:IEC ;
  terms:language lang:eng ;
  terms:language lang:fra ;
  terms:language lang:spa ;
  terms:title "Electromechanical elementary relays - Part 7: Test and measurement procedures"@en ;
  rdfs:comment "IEC 61810-7:2006 Lays down the test and measurement procedures for electromechanical elementary relays. Covers basic considerations which are common to all types of electromechanical elementary relays. Supplementary requirements may be necessitated by specific designs or application."@en ;
  rdfs:label "IEC 61810-7:2006"@en ;
  foaf:maker sto:IEC ;
  sto:hasAvailableLanguage lang:eng ;
  sto:hasAvailableLanguage lang:fra ;
  sto:hasAvailableLanguage lang:spa ;
  sto:hasEdition "2.0"^^xsd:float ;
  sto:hasFileSize sto:FileSizeIEC_61810_P7 ;
  sto:hasICS sto:ICS_29_120_70 ;
  sto:hasOfficialResource <https://webstore.iec.ch/publication/5963> ;
  sto:hasPages "176"^^xsd:int ;
  sto:hasPublicationDate "2006-03-14"^^xsd:date ;
  sto:hasPublisher sto:IEC ;
  sto:hasStabilityDate "2018"^^xsd:gYear ;
  sto:hasTag "IEC 61810-7:2006"@en ;
  sto:hasTechnicalCommittee sto:TC_94 ;
.
sto:IEC_61850
  a owl:NamedIndividual ;
  a foaf:Document ;
  a sto:Publication ;
  a sto:Standard ;
  rdfs:comment "IEC 61850 is a standard for vendor-agnostic engineering of the configuration of Intelligent Electronic Devices for electrical substation automation systems to be able to communicate with each other.."@en ;
  rdfs:label "IEC 61850"@en ;
  sto:hasDBpediaResource <http://dbpedia.org/page/IEC_61850> ;
  sto:hasOfficialResource <https://webstore.iec.ch/publication/4550> ;
  sto:hasPublisher sto:IEC ;
  sto:hasWikipediaArticle <https://en.wikipedia.org/wiki/IEC_61850> ;
.
sto:IEC_61850_P10_E1
  a owl:NamedIndividual ;
  a sto:Standard ;
  terms:title "Communication networks and systems in substations - Part 10: Conformance testing"@en ;
  rdfs:comment "Specifies standard techniques for testing of conformance of implementations, as well as specific measurement techniques to be applied when declaring performance parameters. The use of these techniques will enhance the ability of the system integrator to integrate IEDs easily, operate IEDs correctly, and support the applications as intended.This publication is of core relevance for Smart Grid.."@en ;
  rdfs:label "IEC 61850-10:2005"@en ;
  sto:hasAvailableLanguage lang:eng ;
  sto:hasDBpediaResource <http://dbpedia.org/page/IEC_61850> ;
  sto:hasEdition "1.0"^^xsd:float ;
  sto:hasFileSize sto:FileSizeIEC_61850_P10_E1 ;
  sto:hasICS sto:ICS_33_200 ;
  sto:hasOfficialResource <https://webstore.iec.ch/publication/20072> ;
  sto:hasPages "43"^^xsd:int ;
  sto:hasPublicationDate "2005-05-30"^^xsd:date ;
  sto:hasPublisher sto:IEC ;
  sto:hasStatus "Withdrawn"@en ;
  sto:hasTag "IEC 61850-10:2005"@en ;
  sto:hasTechnicalCommittee sto:TC_57 ;
  sto:hasWikipediaArticle <https://en.wikipedia.org/wiki/IEC_61850> ;
.
sto:IEC_61850_P10_E2
  a owl:NamedIndividual ;
  a sto:Standard ;
  terms:title "Communication networks and systems for power utility automation - Part 10: Conformance testing"@en ;
  rdfs:comment "IEC 61850-10:2012 specifies standard techniques for testing of conformance of client, server and sampled value devices and engineering tools, as well as specific measurement techniques to be applied when declaring performance parameters. The use of these techniques will enhance the ability of the system integrator to integrate IEDs easily, operate IEDs correctly, and support the applications as intended. The major technical changes with regard to the previous edition are as follows:- updates to server device conformance test procedures;- additions of certain test procedures (client device conformance, sampled values device conformance, (engineering) tool related conformance, GOOSE performance).."@en ;
  rdfs:label "IEC 61850-10:2012"@en ;
  prov:wasRevisionOf sto:IEC_61850_P10_E1 ;
  sto:hasAvailableLanguage lang:eng ;
  sto:hasAvailableLanguage lang:fra ;
  sto:hasDBpediaResource <http://dbpedia.org/page/IEC_61850> ;
  sto:hasEdition "2.0"^^xsd:float ;
  sto:hasFileSize sto:FileSizeIEC_61850_P10_E2 ;
  sto:hasICS sto:ICS_33_200 ;
  sto:hasOfficialResource <https://webstore.iec.ch/publication/6008> ;
  sto:hasPages "170"^^xsd:int ;
  sto:hasPublicationDate "2012-12-14"^^xsd:date ;
  sto:hasPublisher sto:IEC ;
  sto:hasStabilityDate "2020"^^xsd:gYear ;
  sto:hasStatus "Valid"@en ;
  sto:hasTag "IEC 61850-10:2012 "@en ;
  sto:hasTechnicalCommittee sto:TC_57 ;
  sto:hasWikipediaArticle <https://en.wikipedia.org/wiki/IEC_61850> ;
.
sto:IEC_61850_P4_E1
  a owl:NamedIndividual ;
  a sto:Standard ;
  terms:title "Communication networks and systems for power utility automation - Part 4: System and project management"@en ;
  rdfs:comment "Describes the requirements of the system and project management process and of special supporting tools for engineering and testing.This publication is of core relevance for Smart Grid."@en ;
  rdfs:label "IEC 61850-4:2002"@en ;
  sto:hasAvailableLanguage lang:eng ;
  sto:hasAvailableLanguage lang:fra ;
  sto:hasEdition "1.0"^^xsd:float ;
  sto:hasFileSize sto:FileSizeIEC_61850_P4_E1 ;
  sto:hasICS sto:ICS_33_200 ;
  sto:hasOfficialResource <https://webstore.iec.ch/publication/20074> ;
  sto:hasPages "59"^^xsd:int ;
  sto:hasPublicationDate "2002-01-17"^^xsd:date ;
  sto:hasPublisher sto:IEC ;
  sto:hasStatus "Withdrawn"@en ;
  sto:hasTag "IEC 61850-4:2002"@en ;
  sto:hasTechnicalCommittee sto:TC_57 ;
.
sto:IEC_61850_P4_E2
  a owl:NamedIndividual ;
  a sto:Standard ;
  terms:title "Communication networks and systems for power utility automation - Part 4: System and project management"@en ;
  rdfs:comment "IEC 61850-4:2011 applies to projects associated with process near automation systems of power utilities (UAS, utility automation system), like e.g. substation automation systems (SAS). It defines the system and project management for UAS systems with communication between intelligent electronic devices (IEDs) in the substation respective plant and the related system requirements. This second edition constitutes a technical revision to align the document more closely with the other parts of the IEC 61850 series, in addition to enlarging the scope from substation automation systems to all utility automation systems.This publication is of core relevance for Smart Grid."@en ;
  rdfs:label "IEC 61850-4:2011"@en ;
  prov:wasRevisionOf sto:IEC_61850_P4_E1 ;
  sto:hasAvailableLanguage lang:eng ;
  sto:hasAvailableLanguage lang:fra ;
  sto:hasDBpediaResource <http://dbpedia.org/page/IEC_61850> ;
  sto:hasEdition "2.0"^^xsd:float ;
  sto:hasFileSize sto:FileSizeIEC_61850_P4_E2 ;
  sto:hasICS sto:ICS_33_200 ;
  sto:hasOfficialResource <https://webstore.iec.ch/publication/6011> ;
  sto:hasPages "74"^^xsd:int ;
  sto:hasPublicationDate "2011-04-11"^^xsd:date ;
  sto:hasPublisher sto:IEC ;
  sto:hasStabilityDate "2020"^^xsd:gYear ;
  sto:hasStatus "Valid"@en ;
  sto:hasTag "IEC 61850-4:2011"@en ;
  sto:hasTechnicalCommittee sto:TC_57 ;
  sto:hasWikipediaArticle <https://en.wikipedia.org/wiki/IEC_61850> ;
.
sto:IEC_61850_P7_S1_E1
  a owl:NamedIndividual ;
  a sto:Standard ;
  terms:title "Communication networks and systems for power utility automation - Part 7-1: Basic communication structure - Principles and models"@en ;
  rdfs:comment "Provides an overview of the architecture for communication and interactions between substation devices such as protection devices, breakers, transformers, substation hosts, etc. Uses simple examples of functions to describe the concepts and methods applied in the IEC 61850 series. Also describes the relationships between other parts of the IEC 61850 series and defines how inter-operability is reached.This publication is of core relevance for Smart Grid."@en ;
  rdfs:label "IEC 61850-7-1:2003"@en ;
  sto:hasAvailableLanguage lang:eng ;
  sto:hasDBpediaResource <http://dbpedia.org/page/IEC_61850> ;
  sto:hasEdition "1.0"^^xsd:float ;
  sto:hasFileSize sto:FileSizeIEC_61850_P7_S1_E1 ;
  sto:hasICS sto:ICS_33_200 ;
  sto:hasOfficialResource <https://webstore.iec.ch/publication/20077> ;
  sto:hasPages "110"^^xsd:int ;
  sto:hasPublicationDate "2003-07-23"^^xsd:date ;
  sto:hasPublisher sto:IEC ;
  sto:hasStatus "Withdrawn"@en ;
  sto:hasTag "IEC 61850-7-1:2003"@en ;
  sto:hasTechnicalCommittee sto:TC_57 ;
  sto:hasWikipediaArticle <https://en.wikipedia.org/wiki/IEC_61850> ;
.
sto:IEC_61850_P7_S1_E2
  a owl:NamedIndividual ;
  a sto:Standard ;
  terms:title "Communication networks and systems for power utility automation - Part 7-1: Basic communication structure - Principles and models"@en ;
  rdfs:comment "IEC 61850-7-1:2011 introduces the modelling methods, communication principles, and information models that are used in the various parts of the IEC 61850-7 series. The purpose is to provide - from a conceptual point of view - assistance to understand the basic modelling concepts and description methods for:- substation-specific information models for power utility automation systems,- device functions used for power utility automation purposes, and- communication systems to provide interoperability within power utility facilities. Compared to the first edition, this second edition introduces:- the model for statistical and historical statistical data,- the concepts of proxies, gateways, LD hierarchy and LN inputs,- the model for time synchronisation,- the concepts behind different testing facilities,- the extended logging function. It also clarifies certain items."@en ;
  rdfs:label "IEC 61850-7-1:2011"@en ;
  prov:wasRevisionOf sto:IEC_61850_P7_S1_E1 ;
  sto:hasAvailableLanguage lang:eng ;
  sto:hasAvailableLanguage lang:fra ;
  sto:hasDBpediaResource <http://dbpedia.org/page/IEC_61850> ;
  sto:hasEdition "2.0"^^xsd:float ;
  sto:hasFileSize sto:FileSizeIEC_61850_P7_S1_E2 ;
  sto:hasICS sto:ICS_33_200 ;
  sto:hasOfficialResource <https://webstore.iec.ch/publication/6011> ;
  sto:hasPages "289"^^xsd:int ;
  sto:hasPublicationDate "2011-07-15"^^xsd:date ;
  sto:hasPublisher sto:IEC ;
  sto:hasStabilityDate "2020"^^xsd:gYear ;
  sto:hasStatus "Valid"@en ;
  sto:hasTag "IEC 61850-7-1:2011"@en ;
  sto:hasTechnicalCommittee sto:TC_57 ;
  sto:hasWikipediaArticle <https://en.wikipedia.org/wiki/IEC_61850> ;
.
sto:IEC_61850_P7_S2_E1
  a owl:NamedIndividual ;
  a sto:Standard ;
  terms:title "Communication networks and systems in substations - Part 7-2: Basic communication structure for substation and feeder equipment - Abstract communication service interface (ACSI)"@en ;
  rdfs:comment "Applies to the ACSI communication in substations and feeder applications. The ACSI provides the abstract interface describing communications between a client and a remote server; and the abstract interface for fast and reliable system-wide event distribution between an application in one device and many remote applications in different devices and for transmission of sampled measured values."@en ;
  rdfs:label "IEC 61850-7-2:2003"@en ;
  sto:hasAvailableLanguage lang:eng ;
  sto:hasDBpediaResource <http://dbpedia.org/page/IEC_61850> ;
  sto:hasEdition "1.0"^^xsd:float ;
  sto:hasFileSize sto:FileSizeIEC_61850_P7_S2_E1 ;
  sto:hasICS sto:ICS_33_200 ;
  sto:hasOfficialResource <https://webstore.iec.ch/publication/20078> ;
  sto:hasPages "171"^^xsd:int ;
  sto:hasPublicationDate "2003-05-12"^^xsd:date ;
  sto:hasPublisher sto:IEC ;
  sto:hasStatus "Withdrawn"@en ;
  sto:hasTag "IEC 61850-7-2:2003"@en ;
  sto:hasTechnicalCommittee sto:TC_57 ;
  sto:hasWikipediaArticle <https://en.wikipedia.org/wiki/IEC_61850> ;
.
sto:IEC_61850_P7_S2_E2
  a owl:NamedIndividual ;
  a sto:Standard ;
  terms:title "Communication networks and systems for power utility automation - Part 7-2: Basic information and communication structure - Abstract communication service interface (ACSI)"@en ;
  rdfs:comment "IEC 61850-7-2:2010(E) applies to the ACSI communication for utility automation. The ACSI provides the following abstract communication service interfaces:- abstract interface describing communications between a client and a remote server;- and abstract interface for fast and reliable system-wide event distribution between an application in one device and many remote applications in different devices (publisher/sub-scriber) and for transmission of sampled measured values (publisher/subscriber).This publication is of core relevance for Smart Grid"@en ;
  rdfs:label "IEC 61850-7-2:2010"@en ;
  prov:wasRevisionOf sto:IEC_61850_P7_S2_E1 ;
  sto:hasAvailableLanguage lang:eng ;
  sto:hasDBpediaResource <http://dbpedia.org/page/IEC_61850> ;
  sto:hasEdition "2.0"^^xsd:float ;
  sto:hasFileSize sto:FileSizeIEC_61850_P7_S2_E2 ;
  sto:hasICS sto:ICS_33_200 ;
  sto:hasOfficialResource <https://webstore.iec.ch/publication/6015> ;
  sto:hasPages "213"^^xsd:int ;
  sto:hasPublicationDate "2010-08-24"^^xsd:date ;
  sto:hasPublisher sto:IEC ;
  sto:hasStabilityDate "2020"^^xsd:gYear ;
  sto:hasStatus "Valid"@en ;
  sto:hasTag "IEC 61850-7-2:2010 "@en ;
  sto:hasTechnicalCommittee sto:TC_57 ;
  sto:hasWikipediaArticle <https://en.wikipedia.org/wiki/IEC_61850> ;
.
sto:IEC_61850_P7_S3_E1
  a owl:NamedIndividual ;
  a sto:Standard ;
  terms:title "Communication networks and systems in substations - Part 7-3: Basic communication structure for substation and feeder equipment - Common data classes"@en ;
  rdfs:comment "Specifies common attribute types and common data classes related to substation applications. Specifies particularly: common data classes for status information, for measured information, for controllable status information, for controllable analogue set point information, for status settings, for analogue settings and attribute types used in these common data classes. Is applicable to the description of device models and functions of substations and feeder equipment. This publication is of core relevance for Smart Grid."@en ;
  rdfs:label "IEC 61850-7-3:2003"@en ;
  sto:hasAvailableLanguage lang:eng ;
  sto:hasDBpediaResource <http://dbpedia.org/page/IEC_61850> ;
  sto:hasEdition "1.0"^^xsd:float ;
  sto:hasFileSize sto:FileSizeIEC_61850_P7_S3_E1 ;
  sto:hasICS sto:ICS_33_200 ;
  sto:hasOfficialResource <https://webstore.iec.ch/publication/20079> ;
  sto:hasPages "64"^^xsd:int ;
  sto:hasPublicationDate "2003-05-12"^^xsd:date ;
  sto:hasPublisher sto:IEC ;
  sto:hasStatus "Withdrawn"@en ;
  sto:hasTag "61850-7-3:2003"@en ;
  sto:hasTechnicalCommittee sto:TC_57 ;
  sto:hasWikipediaArticle <https://en.wikipedia.org/wiki/IEC_61850> ;
.
sto:IEC_61850_P7_S3_E2
  a owl:NamedIndividual ;
  a sto:Standard ;
  terms:title "Communication networks and systems for power utility automation - Part 7-3: Basic communication structure - Common data classes"@en ;
  rdfs:comment "IEC 61850-7-3:2010 is applicable to the description of device models and functions of substations and feeder equipment. It specifies constructed attribute classes and common data classes related to substation applications. In particular, it specifies common data classes for status information, common data classes for measured information, common data classes for control, common data classes for status settings, common data classes for analogue settings and attribute types used in these common data classes. This second edition defines new common data classes used for new standards defining object models for other domains based on IEC 61850 and for the representation of statistical and historical data. This publication is of core relevance for Smart Grid."@en ;
  rdfs:label "IEC 61850-7-3:2010"@en ;
  prov:wasRevisionOf sto:IEC_61850_P7_S3_E1 ;
  sto:hasAvailableLanguage lang:eng ;
  sto:hasAvailableLanguage lang:fra ;
  sto:hasDBpediaResource <http://dbpedia.org/page/IEC_61850> ;
  sto:hasEdition "2.0"^^xsd:float ;
  sto:hasFileSize sto:FileSizeIEC_61850_P7_S3_E2 ;
  sto:hasICS sto:ICS_33_200 ;
  sto:hasOfficialResource <https://webstore.iec.ch/publication/6016> ;
  sto:hasPages "182"^^xsd:int ;
  sto:hasPublicationDate "2010-12-16"^^xsd:date ;
  sto:hasPublisher sto:IEC ;
  sto:hasStabilityDate "2020"^^xsd:gYear ;
  sto:hasStatus "Valid"@en ;
  sto:hasTag "IEC 61850-7-3:2010 "@en ;
  sto:hasTechnicalCommittee sto:TC_57 ;
  sto:hasWikipediaArticle <https://en.wikipedia.org/wiki/IEC_61850> ;
.
sto:IEC_61850_P7_S420_E1
  a owl:NamedIndividual ;
  a sto:Standard ;
  terms:title "Communication networks and systems for power utility automation - Part 7-420: Basic communication structure - Distributed energy resources logical nodes"@en ;
  rdfs:comment "IEC 61850-7-420:2009(E) defines IEC 61850 information models to be used in the exchange of information with distributed energy resources (DER), which comprise dispersed generation devices and dispersed storage devices, including reciprocating engines, fuel cells, microturbines, photovoltaics, combined heat and power, and energy storage. Utilizes existing IEC 61850-7-4 logical nodes where possible, but also defines DER-specific logical nodes where needed."@en ;
  rdfs:label " IEC 61850-7-420:2009"@en ;
  sto:hasAvailableLanguage lang:eng ;
  sto:hasDBpediaResource <http://dbpedia.org/page/IEC_61850> ;
  sto:hasEdition "1.0"^^xsd:float ;
  sto:hasFileSize sto:FileSizeIEC_61850_P7_S420_E1 ;
  sto:hasICS sto:ICS_33_200 ;
  sto:hasOfficialResource <https://webstore.iec.ch/publication/6019> ;
  sto:hasPages "99"^^xsd:int ;
  sto:hasPublicationDate "2009-03-10"^^xsd:date ;
  sto:hasPublisher sto:IEC ;
  sto:hasStabilityDate "2020"^^xsd:gYear ;
  sto:hasStatus "Valid"@en ;
  sto:hasTag " IEC 61850-7-420:2009 "@en ;
  sto:hasTechnicalCommittee sto:TC_57 ;
  sto:hasWikipediaArticle <https://en.wikipedia.org/wiki/IEC_61850> ;
.
sto:IEC_61850_P7_S4_E1
  a owl:NamedIndividual ;
  a sto:Standard ;
  terms:title "Communication networks and systems in substations - Part 7-4: Basic communication structure for substation and feeder equipment - Compatible logical node classes and data classes"@en ;
  rdfs:comment "Specifies the information model of devices and functions related to substation applications. Specifies in particular the compatible logical node names and data names for communication between Intelligent Electronic Devices, which includes the relationship between Logical Nodes and Data.."@en ;
  rdfs:label "IEC 61850-7-4:2003"@en ;
  sto:hasAvailableLanguage lang:eng ;
  sto:hasDBpediaResource <http://dbpedia.org/page/IEC_61850> ;
  sto:hasEdition "1.0"^^xsd:float ;
  sto:hasFileSize sto:FileSizeIEC_61850_P7_S4_E1 ;
  sto:hasICS sto:ICS_33_200 ;
  sto:hasOfficialResource <https://webstore.iec.ch/publication/20080> ;
  sto:hasPages "104"^^xsd:int ;
  sto:hasPublicationDate "2003-05-13"^^xsd:date ;
  sto:hasPublisher sto:IEC ;
  sto:hasStatus "Withdrawn"@en ;
  sto:hasTag "IEC 61850-7-4:2003"@en ;
  sto:hasTechnicalCommittee sto:TC_57 ;
  sto:hasWikipediaArticle <https://en.wikipedia.org/wiki/IEC_61850> ;
.
sto:IEC_61850_P7_S4_E2
  a owl:NamedIndividual ;
  a sto:Standard ;
  terms:title "Communication networks and systems for power utility automation - Part 7-4: Basic communication structure - Compatible logical node classes and data object classes"@en ;
  rdfs:comment "IEC 61850-7-4:2010 specifies the information model of devices and functions generally related to common use regarding applications in systems for power utility automation. It also contains the information model of devices and function-related applications in substations. In particular, it specifies the compatible logical node names and data object names for communication between intelligent electronic devices (IED). This includes the relationship between logical nodes and data objects. Major technical changes with regard to the previous edition are as follows:- corrections and clarifications according to technical issues raised by the users' community; extensions for new logical nodes for the power quality domain;- extensions for the model for statistical and historical statistical data;- extensions regarding IEC 61850-90-1;- extensions for new logical nodes for monitoring functions according to IEC 62271;- new logical nodes from IEC 61850-7-410 and IEC 61850-7-420 of general interest.This publication is of core relevance for Smart Grid."@en ;
  rdfs:label "IEC 61850-7-4:2010"@en ;
  prov:wasRevisionOf sto:IEC_61850_P7_S4_E1 ;
  sto:hasAvailableLanguage lang:eng ;
  sto:hasAvailableLanguage lang:fra ;
  sto:hasDBpediaResource <http://dbpedia.org/page/IEC_61850> ;
  sto:hasEdition "2.0"^^xsd:float ;
  sto:hasFileSize sto:FileSizeIEC_61850_P7_S4_E2 ;
  sto:hasICS sto:ICS_33_200 ;
  sto:hasOfficialResource <https://webstore.iec.ch/publication/6017> ;
  sto:hasPages "421"^^xsd:int ;
  sto:hasPublicationDate "2010-03-31"^^xsd:date ;
  sto:hasPublisher sto:IEC ;
  sto:hasStabilityDate "2020"^^xsd:gYear ;
  sto:hasStatus "Valid"@en ;
  sto:hasTag "IEC 61850-7-4:2010 "@en ;
  sto:hasTechnicalCommittee sto:TC_57 ;
  sto:hasWikipediaArticle <https://en.wikipedia.org/wiki/IEC_61850> ;
.
sto:IEC_61968_P3_E1
  a owl:NamedIndividual ;
  a sto:Standard ;
  terms:title "Application integration at electric utilities - System interfaces for distribution management - Part 3: Interface for network operations"@en ;
  rdfs:comment "Specifies the information content of a set of message types that can be used to support many of the business functions related to network operations. Typical uses of the message types defined in this part include data acquisition by external systems, fault isolation, fault restoration, trouble management, maintenance of the plant, and the commissioning of the plant. This publication is of core relevance for Smart Grid."@en ;
  rdfs:label "IEC 61968-3:2004"@en ;
  sto:hasAvailableLanguage lang:eng ;
  sto:hasEdition "1.0"^^xsd:float ;
  sto:hasFileSize sto:FileSizeIEC_61968_P3_E1 ;
  sto:hasICS sto:ICS_33_200 ;
  sto:hasOfficialResource <https://webstore.iec.ch/publication/6202> ;
  sto:hasPages "36"^^xsd:int ;
  sto:hasPublicationDate "2004-03-08"^^xsd:date ;
  sto:hasPublisher sto:IEC ;
  sto:hasStatus "Withdrawn"@en ;
  sto:hasTag "IEC 61968-3:2004"@en ;
  sto:hasTechnicalCommittee sto:TC_57 ;
  sto:hasWikipediaArticle <https://en.wikipedia.org/wiki/IEC_61968> ;
.
sto:IEC_61968_P3_E2
  a owl:NamedIndividual ;
  a sto:Standard ;
  terms:title "Application integration at electric utilities - System interfaces for distribution management - Part 3: Interface for network operations"@en ;
  rdfs:comment "IEC 61968-3:2017 defines a Network Operations function which provides utilities the means to supervise main substation topology (breaker and switch state) and control equipment status. It also provides the means for handling network connectivity and loading conditions. Finally, it makes it possible for utilities to locate customer telephone complaints and supervise the location of field crews. IEC 61968-3 specifies the information content of a set of message payloads that can be used to support many of the business functions related to network operations. Typical uses of the message payloads defined in IEC 61968-3 include data acquisition by external systems, fault isolation, fault restoration, trouble management, maintenance of plant, and the commissioning of plant. This edition includes the following significant technical changes with respect to the previous edition: replacement of certain function names, addition of other function names."@en ;
  rdfs:label "IEC 61968-3:2017"@en ;
  prov:wasRevisionOf sto:IEC_61968_P3_E1 ;
  sto:hasAvailableLanguage lang:eng ;
  sto:hasAvailableLanguage lang:fra ;
  sto:hasEdition "2.0"^^xsd:float ;
  sto:hasFileSize sto:FileSizeIEC_61968_P3_E2 ;
  sto:hasICS sto:ICS_33_200 ;
  sto:hasOfficialResource <https://webstore.iec.ch/publication/27527> ;
  sto:hasPages "322"^^xsd:int ;
  sto:hasPublicationDate "2017-04-11"^^xsd:date ;
  sto:hasPublisher sto:IEC ;
  sto:hasStabilityDate "2019"^^xsd:gYear ;
  sto:hasStatus "Valid"@en ;
  sto:hasTag "IEC 61968-3:2017 "@en ;
  sto:hasTechnicalCommittee sto:TC_57 ;
  sto:hasWikipediaArticle <https://en.wikipedia.org/wiki/IEC_61968> ;
.
sto:IEC_61968_P4_E1
  a owl:NamedIndividual ;
  a sto:Standard ;
  terms:title "Application integration at electric utilities - System interfaces for distribution management - Part 4: Interfaces for records and asset management"@en ;
  rdfs:comment "IEC 61968-4:2007 Specifies the information content of a set of message types that can be used to support many of the business functions related to records and asset management. Typical uses of the message types include network extension planning, copying feeder or other network data between systems, network or diagram edits and asset inspection.This publication is of core relevance for Smart Grid."@en ;
  rdfs:label "IEC 61968-4:2007"@en ;
  sto:hasAvailableLanguage lang:eng ;
  sto:hasAvailableLanguage lang:fra ;
  sto:hasEdition "1.0"^^xsd:float ;
  sto:hasFileSize sto:FileSizeIEC_61968_P4_E1 ;
  sto:hasICS sto:ICS_33_200 ;
  sto:hasOfficialResource <https://webstore.iec.ch/publication/6203> ;
  sto:hasPages "101"^^xsd:int ;
  sto:hasPublicationDate "2007-07-11"^^xsd:date ;
  sto:hasPublisher sto:IEC ;
  sto:hasStabilityDate "2020"^^xsd:gYear ;
  sto:hasStatus "Valid"@en ;
  sto:hasTag "IEC 61968-4:2007 "@en ;
  sto:hasTechnicalCommittee sto:TC_57 ;
  sto:hasWikipediaArticle <https://en.wikipedia.org/wiki/IEC_61968> ;
.
sto:IEC_61968_P4_E2
  a owl:NamedIndividual ;
  a sto:Standard ;
  terms:title "Application integration at electric utilities - System interfaces for distribution management - Part 4: Interfaces for records and asset management"@en ;
  rdfs:comment "This Final Draft International Standard is an up to 6 weeks' pre-release of the official publication. It is available for sale during its voting period: 2018-12-14 to 2019-01-25. By purchasing this FDIS now, you will automatically receive, in addition, the final publication.IEC 61968:2019 specifies the information content of a set of message types that can be used to support many of the business functions related to records and asset management. Typical uses of the message types defined in this document include network extension planning, copying feeder or other network data between systems, network or diagram edits and asset inspection. Message types defined in other parts of IEC 61968 may also be relevant to these use cases.This second edition cancels and replaces the first edition published in 2007. This edition constitutes a technical revision. This edition includes the following significant technical changes with respect to the previous edition:a) removal of edition 1 profiles whose functionality has been superseded by other parts of IEC 61970 and IEC 61968 standards. In particular, NetworkDataSet and ChangeSet have been superseded by standards such as CDPSM (IEC 61968-13) and other ongoing efforts such as change modelling; and Presentation has been superseded by Diagram Layout Profile (IEC 61970-453);b) revision of the edition 1 profiles AssetList, AssetCatalogue and TypeAssetCatalogue to realign with current use cases and the latest CIM UML release. These profiles are based on an old version of CIM UML and many of the classes in these profiles are no longer in the recent CIM UMLs;c) addition of several new profiles to enable the exchange of asset condition data, analytics results and alerts, assets' physical, functional and lifecycle details, and assets' work;d) informative annexes on how this document can be used to enable strategic asset management;e) informative annexes with illustrative examples for the application of this document;f) scope coordinated with IEC 61968-13 where applicable;g) use cases in IEC 62559-2 use case template;h) traceability of use cases to IEC 62913-2-1 use cases."@en ;
  rdfs:label "IEC 61968-4:2018 PRV"@en ;
  prov:wasRevisionOf sto:IEC_61968_P4_E1 ;
  sto:hasAvailableLanguage lang:eng ;
  sto:hasAvailableLanguage lang:fra ;
  sto:hasEdition "2.0"^^xsd:float ;
  sto:hasFileSize sto:FileSizeIEC_61968_P4_E2 ;
  sto:hasICS sto:ICS_33_200 ;
  sto:hasOfficialResource <https://webstore.iec.ch/publication/64397> ;
  sto:hasPages "344"^^xsd:int ;
  sto:hasPublicationDate "2018-12-14"^^xsd:date ;
  sto:hasPublisher sto:IEC ;
  sto:hasStabilityDate "2020"^^xsd:gYear ;
  sto:hasStatus "Pre release version (PRV)"@en ;
  sto:hasTag "IEC 61968-4:2018 PRV "@en ;
  sto:hasTechnicalCommittee sto:TC_57 ;
  sto:hasWikipediaArticle <https://en.wikipedia.org/wiki/IEC_61968> ;
.
sto:IEC_61968_P6_E1
  a owl:NamedIndividual ;
  a sto:Standard ;
  terms:title "Application integration at electric utilities - System interfaces for distribution management - Part 6: Interfaces for maintenance and construction"@en ;
  rdfs:comment "IEC 61968-6:2015 specifies the information content of a set of message types that can be used to support business functions related to maintenance and construction. Typical uses of the message types defined in this part of IEC 61968 include planned maintenance, unplanned maintenance, conditional maintenance, work management, new service requests, etc. Message types defined in other parts of IEC 61968 may also be relevant to these use cases."@en ;
  rdfs:label "IEC 61968-6:2015"@en ;
  sto:hasAvailableLanguage lang:eng ;
  sto:hasAvailableLanguage lang:fra ;
  sto:hasEdition "1.0"^^xsd:float ;
  sto:hasFileSize sto:FileSizeIEC_61968_P6_E1 ;
  sto:hasICS sto:ICS_33_200 ;
  sto:hasOfficialResource <https://webstore.iec.ch/publication/22834> ;
  sto:hasPages "291"^^xsd:int ;
  sto:hasPublicationDate "2015-07-07"^^xsd:date ;
  sto:hasPublisher sto:IEC ;
  sto:hasStabilityDate "2020"^^xsd:gYear ;
  sto:hasStatus "Valid"@en ;
  sto:hasTag "IEC 61968-6:2015 "@en ;
  sto:hasTechnicalCommittee sto:TC_57 ;
  sto:hasWikipediaArticle <https://en.wikipedia.org/wiki/IEC_61968> ;
.
sto:IEC_61968_P8_E1
  a owl:NamedIndividual ;
  a sto:Standard ;
  terms:title "Application integration at electric utilities - System interfaces for distribution management - Part 8: Interfaces for customer operations"@en ;
  rdfs:comment "IEC 61968-8:2015 specifies the information content of a set of message types that can be used to support many of the business functions related to customer support. Typical uses of the message types include service request, customer agreement, and trouble management. The purpose is to define a standard for the integration of customer support (CS), which would include customer service, trouble management and point of sale related components integrated with other systems and business functions within the scope of IEC 61968. The scope of this standard is the exchange of information between a customer support system and other systems within the utility enterprise."@en ;
  rdfs:label "IEC 61968-8:2015 "@en ;
  sto:hasAvailableLanguage lang:eng ;
  sto:hasAvailableLanguage lang:fra ;
  sto:hasEdition "1.0"^^xsd:float ;
  sto:hasFileSize sto:FileSizeIEC_61968_P8_E1 ;
  sto:hasICS sto:ICS_33_200 ;
  sto:hasOfficialResource <https://webstore.iec.ch/publication/22537> ;
  sto:hasPages "130"^^xsd:int ;
  sto:hasPublicationDate "2015-05-27"^^xsd:date ;
  sto:hasPublisher sto:IEC ;
  sto:hasStabilityDate "2020"^^xsd:gYear ;
  sto:hasStatus "Valid"@en ;
  sto:hasTag "IEC 61968-8:2015  "@en ;
  sto:hasTechnicalCommittee sto:TC_57 ;
  sto:hasWikipediaArticle <https://en.wikipedia.org/wiki/IEC_61968> ;
.
sto:IEC_61968_P9_E1
  a owl:NamedIndividual ;
  a sto:Standard ;
  terms:title "Application integration at electric utilities - System interfaces for distribution management - Part 9: Interfaces for meter reading and control"@en ;
  rdfs:comment "IEC 61968-9:2009(E) specifies the information content of a set of message types that can be used to support many of the business functions related to meter reading and control. Typical uses of the message types include meter reading, meter control, meter events, customer data synchronization and customer switching. Although intended primarily for electrical distribution networks, IEC 61968-9 can be used for other metering applications, including non-electrical metered quantities necessary to support gas and water networks. This publication is of core relevance for Smart Grid.."@en ;
  rdfs:label "IEC 61968-9:2009"@en ;
  sto:hasAvailableLanguage lang:eng ;
  sto:hasEdition "1.0"^^xsd:float ;
  sto:hasFileSize sto:FileSizeIEC_61968_P9_E1 ;
  sto:hasICS sto:ICS_33_200 ;
  sto:hasOfficialResource <https://webstore.iec.ch/publication/20183> ;
  sto:hasPages "257"^^xsd:int ;
  sto:hasPublicationDate "2009-09-16"^^xsd:date ;
  sto:hasPublisher sto:IEC ;
  sto:hasStatus "Withdrawn"@en ;
  sto:hasTag "IEC 61968-9:2009"@en ;
  sto:hasTechnicalCommittee sto:TC_57 ;
  sto:hasWikipediaArticle <https://en.wikipedia.org/wiki/IEC_61968> ;
.
sto:IEC_61968_P9_E2
  a owl:NamedIndividual ;
  a sto:Standard ;
  terms:title "Application integration at electric utilities - System interfaces for distribution management - Part 9: Interfaces for meter reading and control"@en ;
  rdfs:comment "IEC 61968-9:2013 specifies the information content of a set of message types that can be used to support many of the business functions related to meter reading and control. Typical uses of the message types include meter reading, controls, events, customer data synchronization and customer switching. The purpose of IEC 61968-9 is to define a standard for the integration of metering systems (MS), which includes traditional manual systems, and (one or two-way) automated meter reading (AMR) systems, and meter data management (MDM) systems with other enterprise systems and business functions within the scope of IEC 61968. The scope of IEC 61968-9 is the exchange of information between metering systems, MDM systems and other systems within the utility enterprise. This new edition includes the following significant technical changes with respect to the previous edition:- changes to and addition of new profiles to support PAN and UsagePoints;- extensions to support PAN devices generically as EndDevices;- extensions to the MeterReading model and profiles to support richer descriptions of metered quantities and to accommodate coincident readings.."@en ;
  rdfs:label "IEC 61968-9:2013"@en ;
  prov:wasRevisionOf sto:IEC_61968_P9_E1 ;
  sto:hasAvailableLanguage lang:eng ;
  sto:hasAvailableLanguage lang:fra ;
  sto:hasEdition "2.0"^^xsd:float ;
  sto:hasFileSize sto:FileSizeIEC_61968_P9_E2 ;
  sto:hasICS sto:ICS_33_200 ;
  sto:hasOfficialResource <https://webstore.iec.ch/publication/6204> ;
  sto:hasPages "919"^^xsd:int ;
  sto:hasPublicationDate "2013-10-16"^^xsd:date ;
  sto:hasPublisher sto:IEC ;
  sto:hasStabilityDate "2020"^^xsd:gYear ;
  sto:hasStatus "Valid"@en ;
  sto:hasTag "IEC 61968-9:2013 "@en ;
  sto:hasTechnicalCommittee sto:TC_57 ;
  sto:hasWikipediaArticle <https://en.wikipedia.org/wiki/IEC_61968> ;
.
sto:IEC_61970_P1_E1
  a owl:NamedIndividual ;
  a sto:Standard ;
  terms:title "Energy management system application program interface (EMS-API) - Part 1: Guidelines and general requirements"@en ;
  rdfs:comment "Provides a set of guidelines and general infrastructure capabilities required for the application of the EMS-API interface standards. Describes typical integration scenarios where these standards are to be applied and the types of applications to be integrated. Defines a reference model and provides a framework for the application of the other parts of these EMS-API standards.This publication is of core relevance for Smart Grid."@en ;
  rdfs:label "IEC 61970-1:2005 "@en ;
  sto:hasAvailableLanguage lang:eng ;
  sto:hasAvailableLanguage lang:fra ;
  sto:hasEdition "1.0"^^xsd:float ;
  sto:hasFileSize sto:FileSizeIEC_61970_P1_E1 ;
  sto:hasICS sto:ICS_33_200 ;
  sto:hasOfficialResource <https://webstore.iec.ch/publication/6208> ;
  sto:hasPages "81"^^xsd:int ;
  sto:hasPublicationDate "2005-12-07"^^xsd:date ;
  sto:hasPublisher sto:IEC ;
  sto:hasStabilityDate "2020"^^xsd:gYear ;
  sto:hasStatus "Valid"@en ;
  sto:hasTag "IEC 61970-1:2005  "@en ;
  sto:hasTechnicalCommittee sto:TC_57 ;
  sto:hasWikipediaArticle <https://en.wikipedia.org/wiki/IEC_61970> ;
.
sto:IEC_61970_P301_E1
  a owl:NamedIndividual ;
  a sto:Standard ;
  terms:title "Energy management system application program interface (EMS-API) - Part 301: Common information model (CIM) base"@en ;
  rdfs:comment "Defines the Common Information Model Base set of packages which provide a logical view of the physical aspects of Energy Management System information. Is part of the IEC 61970 series, which defines an Application Program Interface (API) for an Energy Management System (EMS)."@en ;
  rdfs:label "IEC 61970-301:2003"@en ;
  sto:hasAvailableLanguage lang:eng ;
  sto:hasAvailableLanguage lang:fra ;
  sto:hasEdition "1.0"^^xsd:float ;
  sto:hasFileSize sto:FileSizeIEC_61970_P301_E1 ;
  sto:hasICS sto:ICS_33_200 ;
  sto:hasOfficialResource <https://webstore.iec.ch/publication/20189> ;
  sto:hasPages "369"^^xsd:int ;
  sto:hasPublicationDate "2003-11-26"^^xsd:date ;
  sto:hasPublisher sto:IEC ;
  sto:hasStatus "Withdrawn"@en ;
  sto:hasTag "IEC 61970-301:2003 "@en ;
  sto:hasTechnicalCommittee sto:TC_57 ;
  sto:hasWikipediaArticle <https://en.wikipedia.org/wiki/IEC_61970> ;
.
sto:IEC_61970_P301_E2
  a owl:NamedIndividual ;
  a sto:Standard ;
  terms:title "Energy management system application program interface (EMS-API) - Part 301: Common information model (CIM) base"@en ;
  rdfs:comment "IEC 61970-301:2009(E) defines the Common Information Model (CIM) base set of packages which provide a logical view of the physical aspects of an energy management system including SCADA (Supervisory Control and Data Acquisition). Whilst there are multiple IEC standards dealing with different parts of the CIM, there is a single, unified normalized information model comprising the CIM behind all these individual standards documents. This second edition contains the following main changes with respect to the previous edition:- change of the naming hierarchy,- replacement of several classes,- addition of several new classes,- many editorial corrections to resolve issues included in the first edition. This publication is of core relevance for Smart Grid."@en ;
  rdfs:label "IEC 61970-301:2009"@en ;
  prov:wasRevisionOf sto:IEC_61970_P301_E1 ;
  sto:hasAvailableLanguage lang:eng ;
  sto:hasEdition "2.0"^^xsd:float ;
  sto:hasFileSize sto:FileSizeIEC_61970_P301_E2 ;
  sto:hasICS sto:ICS_33_200 ;
  sto:hasOfficialResource <https://webstore.iec.ch/publication/20190> ;
  sto:hasPages "211"^^xsd:int ;
  sto:hasPublicationDate "2009-04-07"^^xsd:date ;
  sto:hasPublisher sto:IEC ;
  sto:hasStatus "Withdrawn"@en ;
  sto:hasTag "IEC 61970-301:2009 "@en ;
  sto:hasTechnicalCommittee sto:TC_57 ;
  sto:hasWikipediaArticle <https://en.wikipedia.org/wiki/IEC_61970> ;
.
sto:IEC_61970_P301_E3
  a owl:NamedIndividual ;
  a sto:Standard ;
  terms:title "Energy management system application program interface (EMS-API) - Part 301: Common information model (CIM) base"@en ;
  rdfs:comment "IEC 61970-301:2011 deals with the common information model (CIM), an abstract model that represents all the major objects in an electric utility enterprise typically involved in utility operations. The object classes represented in the CIM are abstract in nature and may be used in a wide variety of applications. The use of the CIM goes far beyond its application in an EMS. This standard should be understood as a tool to enable integration in any domain where a common power system model is needed to facilitate interoperability and plug compatibility between applications and systems independent of any particular implementation. Major changes from the second edition include the following:- Addition of regulation control models;- new (OperationalLimits) package for equipment ratings;- addition of partial ownership specification;- enhancement of LoadResponseCharacteristic;- change from non-SI units to SI units."@en ;
  rdfs:label "IEC 61970-301:2011"@en ;
  prov:wasRevisionOf sto:IEC_61970_P301_E2 ;
  sto:hasAvailableLanguage lang:eng ;
  sto:hasAvailableLanguage lang:fra ;
  sto:hasEdition "3.0"^^xsd:float ;
  sto:hasFileSize sto:FileSizeIEC_61970_P301_E3 ;
  sto:hasICS sto:ICS_33_200 ;
  sto:hasOfficialResource <https://webstore.iec.ch/publication/20191> ;
  sto:hasPages "533"^^xsd:int ;
  sto:hasPublicationDate "2011-08-26"^^xsd:date ;
  sto:hasPublisher sto:IEC ;
  sto:hasStatus "Withdrawn"@en ;
  sto:hasTag "IEC 61970-301:2011 "@en ;
  sto:hasTechnicalCommittee sto:TC_57 ;
  sto:hasWikipediaArticle <https://en.wikipedia.org/wiki/IEC_61970> ;
.
sto:IEC_61970_P301_E4
  a owl:NamedIndividual ;
  a sto:Standard ;
  terms:title "Energy management system application program interface (EMS-API) - Part 301: Common information model (CIM) base"@en ;
  rdfs:comment "IEC 61970-301:2013 deals with the common information model (CIM), an abstract model that represents all the major objects in an electric utility enterprise typically involved in utility operations. The object classes represented in the CIM are abstract in nature and may be used in a wide variety of applications. The use of the CIM goes far beyond its application in an EMS. This standard is to be understood as a tool to enable integration in any domain where a common power system model is needed to facilitate interoperability and plug compatibility between applications and systems independent of any particular implementation. Major changes from the third edition include the following:- extensions have been added to support UCTE exchange;- the transformer regulation model has been expanded to support phase shifting transformer models needed by ENTSO-E;- zero and negative sequence impedance terms have been added;- new StateVariables package has been added;- additional classes have been added."@en ;
  rdfs:label "IEC 61970-301:2013"@en ;
  prov:wasRevisionOf sto:IEC_61970_P301_E3 ;
  sto:hasAvailableLanguage lang:eng ;
  sto:hasAvailableLanguage lang:fra ;
  sto:hasEdition "4.0"^^xsd:float ;
  sto:hasFileSize sto:FileSizeIEC_61970_P301_E4 ;
  sto:hasICS sto:ICS_33_200 ;
  sto:hasOfficialResource <https://webstore.iec.ch/publication/20192> ;
  sto:hasPages "644"^^xsd:int ;
  sto:hasPublicationDate "2013-05-23"^^xsd:date ;
  sto:hasPublisher sto:IEC ;
  sto:hasStatus "Withdrawn"@en ;
  sto:hasTag "IEC 61970-301:2013 "@en ;
  sto:hasTechnicalCommittee sto:TC_57 ;
  sto:hasWikipediaArticle <https://en.wikipedia.org/wiki/IEC_61970> ;
.
sto:IEC_61970_P301_E5
  a owl:NamedIndividual ;
  a sto:Standard ;
  terms:title "Energy management system application program interface (EMS-API) - Part 301: Common information model (CIM) base"@en ;
  rdfs:comment "IEC 61970-301:2013 defines the Common Information Model (CIM), that is an abstract model representing all the major objects in an electric utility enterprise typically involved in utility operations. By providing a standard way of representing power system resources as object classes and attributes, along with their relationships, the CIM facilitates the integration of Energy Management System (EMS) applications developed independently by different vendors, between entire EMS systems developed independently, or between an EMS system and other systems concerned with different aspects of power system operations, such as generation or distribution management. SCADA is modeled to the extent necessary to support power system simulation and inter-control center communication. The CIM facilitates integration by defining a common language (i.e. semantics) based on the CIM to enable these applications or systems to access public data and exchange information independent of how such information is represented internally. Major changes from the fourth edition include the following:- transformer models have been modified to be consistent for use by distribution and transmission purposes;- a more general and clear naming approach was added and several ambiguous attributes related to naming were dropped;- phase component wires models have been enhanced to describe internal phase specific attributes and connections;- addition of diagram layout models to facilitate the exchange of diagram layout information."@en ;
  rdfs:label "IEC 61970-301:2013"@en ;
  prov:wasRevisionOf sto:IEC_61970_P301_E4 ;
  sto:hasAvailableLanguage lang:eng ;
  sto:hasAvailableLanguage lang:fra ;
  sto:hasEdition "5.0"^^xsd:float ;
  sto:hasFileSize sto:FileSizeIEC_61970_P301_E5 ;
  sto:hasICS sto:ICS_33_200 ;
  sto:hasOfficialResource <https://webstore.iec.ch/publication/6210> ;
  sto:hasPages "766"^^xsd:int ;
  sto:hasPublicationDate "2013-12-13"^^xsd:date ;
  sto:hasPublisher sto:IEC ;
  sto:hasStatus "Withdrawn"@en ;
  sto:hasTag "IEC 61970-301:2013 "@en ;
  sto:hasTechnicalCommittee sto:TC_57 ;
  sto:hasWikipediaArticle <https://en.wikipedia.org/wiki/IEC_61970> ;
.
sto:IEC_61970_P301_E6
  a owl:NamedIndividual ;
  a sto:Standard ;
  terms:title "Energy management system application program interface (EMS-API) - Part 301: Common information model (CIM) base"@en ;
  rdfs:comment "IEC 61970-301:2016 is available as IEC 61970-301:2016 RLV which contains the International Standard and its Redline version, showing all changes of the technical content compared to the previous edition.IEC 61970-301:2016 lays down the common information model (CIM), which is an abstract model that represents all the major objects in an electric utility enterprise typically involved in utility operations. By providing a standard way of representing power system resources as object classes and attributes, along with their relationships, the CIM facilitates the integration of network applications developed independently by different vendors, between entire systems running network applications developed independently, or between a system running network applications and other systems concerned with different aspects of power system operations, such as generation or distribution management. SCADA is modeled to the extent necessary to support power system simulation and inter-control centre communication. The CIM facilitates integration by defining a common language (i.e. semantics) based on the CIM to enable these applications or systems to access public data and exchange information independent of how such information is represented internally. This new edition includes the following significant technical changes with respect to the previous edition:- new model for grounding including Petersen coils;- models for HVDC; addition of Static Var Compensation models;- phase shift transformer updates;- short circuit calculations based on IEC 60909;- addition of non-linear shunt compensator;- addition of model for steady state calculation inputs, Steady State Hypothesis;- addition of base frequency model;- Annex A with custom extensions added."@en ;
  rdfs:label "IEC 61970-301:2016"@en ;
  prov:wasRevisionOf sto:IEC_61970_P301_E5 ;
  sto:hasAvailableLanguage lang:eng ;
  sto:hasAvailableLanguage lang:fra ;
  sto:hasEdition "6.0"^^xsd:float ;
  sto:hasFileSize sto:FileSizeIEC_61970_P301_E6 ;
  sto:hasICS sto:ICS_33_200 ;
  sto:hasOfficialResource <https://webstore.iec.ch/publication/31356> ;
  sto:hasPages "938"^^xsd:int ;
  sto:hasPublicationDate "2016-12-16"^^xsd:date ;
  sto:hasPublisher sto:IEC ;
  sto:hasStabilityDate "2020"^^xsd:gYear ;
  sto:hasStatus "Valid"@en ;
  sto:hasTag "IEC 61970-301:2016 "@en ;
  sto:hasTechnicalCommittee sto:TC_57 ;
  sto:hasWikipediaArticle <https://en.wikipedia.org/wiki/IEC_61970> ;
.
sto:IEC_61970_P301_E6_RLV
  a owl:NamedIndividual ;
  a sto:Standard ;
  terms:title "Energy management system application program interface (EMS-API) - Part 301: Common information model (CIM) base"@en ;
  rdfs:comment "IEC 61970-301:2016 RLV contains both the official IEC International Standard and its Redline version. The Redline version is not an official document, it is available in English only and provides you with a quick and easy way to compare all the changes between the official IEC Standard and its previous edition.IEC 61970-301:2016 lays down the common information model (CIM), which is an abstract model that represents all the major objects in an electric utility enterprise typically involved in utility operations. By providing a standard way of representing power system resources as object classes and attributes, along with their relationships, the CIM facilitates the integration of network applications developed independently by different vendors, between entire systems running network applications developed independently, or between a system running network applications and other systems concerned with different aspects of power system operations, such as generation or distribution management. SCADA is modeled to the extent necessary to support power system simulation and inter-control centre communication. The CIM facilitates integration by defining a common language (i.e. semantics) based on the CIM to enable these applications or systems to access public data and exchange information independent of how such information is represented internally. This new edition includes the following significant technical changes with respect to the previous edition:- new model for grounding including Petersen coils;- models for HVDC; addition of Static Var Compensation models;- phase shift transformer updates;- short circuit calculations based on IEC 60909;- addition of non-linear shunt compensator;- addition of model for steady state calculation inputs, Steady State Hypothesis;- addition of base frequency model;- Annex A with custom extensions added."@en ;
  rdfs:label "IEC 61970-301:2016 RLV Redline version "@en ;
  prov:wasRevisionOf sto:IEC_61970_P301_E6 ;
  sto:hasAvailableLanguage lang:eng ;
  sto:hasAvailableLanguage lang:fra ;
  sto:hasEdition "6.0"^^xsd:float ;
  sto:hasFileSize sto:FileSizeIEC_61970_P301_E6_RLV ;
  sto:hasICS sto:ICS_33_200 ;
  sto:hasOfficialResource <https://webstore.iec.ch/publication/59669> ;
  sto:hasPages "1423"^^xsd:int ;
  sto:hasPublicationDate "2016-12-16"^^xsd:date ;
  sto:hasPublisher sto:IEC ;
  sto:hasStabilityDate "2020"^^xsd:gYear ;
  sto:hasStatus "RLV-Redline version"@en ;
  sto:hasTag "IEC 61970-301:2016 RLV Redline version "@en ;
  sto:hasTechnicalCommittee sto:TC_57 ;
  sto:hasWikipediaArticle <https://en.wikipedia.org/wiki/IEC_61970> ;
.
sto:IEC_61970_P452_E1
  a owl:NamedIndividual ;
  a sto:Standard ;
  terms:title "Energy management system application program interface (EMS-API) - Part 452: CIM Static transmission network model profiles"@en ;
  rdfs:comment "IEC 61970-452:2013 rigorously defines the subset of classes, class attributes, and roles from the CIM necessary to execute state estimation and power flow applications. This international standard is intended for two distinct audiences, data producers and data recipients, and may be read from two perspectives."@en ;
  rdfs:label "IEC 61970-452:2013"@en ;
  sto:hasAvailableLanguage lang:eng ;
  sto:hasAvailableLanguage lang:fra ;
  sto:hasEdition "1.0"^^xsd:float ;
  sto:hasFileSize sto:FileSizeIEC_61970_P452_E1 ;
  sto:hasICS sto:ICS_33_200 ;
  sto:hasOfficialResource <https://webstore.iec.ch/publication/6212> ;
  sto:hasPages "244"^^xsd:int ;
  sto:hasPublicationDate "2013-08-12"^^xsd:date ;
  sto:hasPublisher sto:IEC ;
  sto:hasStatus "Withdrawn"@en ;
  sto:hasTag "IEC 61970-452:2013 "@en ;
  sto:hasTechnicalCommittee sto:TC_57 ;
  sto:hasWikipediaArticle <https://en.wikipedia.org/wiki/IEC_61970> ;
.
sto:IEC_61970_P452_E2
  a owl:NamedIndividual ;
  a sto:Standard ;
  terms:title "Energy management system application program interface (EMS-API) - Part 452: CIM model exchange specification"@en ;
  rdfs:comment "IEC 61970-452:2015 rigorously defines the subset of classes, class attributes, and roles from the CIM necessary to execute state estimation and power flow applications. These requirements are based on prior industry practices for exchanging power system model data for use primarily in planning studies. This standard is intended for two distinct audiences, data producers and data recipients, and may be used from these two perspectives.."@en ;
  rdfs:label "IEC 61970-452:2015"@en ;
  prov:wasRevisionOf sto:IEC_61970_P452_E1 ;
  sto:hasAvailableLanguage lang:eng ;
  sto:hasAvailableLanguage lang:fra ;
  sto:hasEdition "2.0"^^xsd:float ;
  sto:hasFileSize sto:FileSizeIEC_61970_P452_E2 ;
  sto:hasICS sto:ICS_33_200 ;
  sto:hasOfficialResource <https://webstore.iec.ch/publication/22090> ;
  sto:hasPages "203"^^xsd:int ;
  sto:hasPublicationDate "2015-04-09"^^xsd:date ;
  sto:hasPublisher sto:IEC ;
  sto:hasStatus "Withdrawn"@en ;
  sto:hasTag "IEC 61970-452:2015 "@en ;
  sto:hasTechnicalCommittee sto:TC_57 ;
  sto:hasWikipediaArticle <https://en.wikipedia.org/wiki/IEC_61970> ;
.
sto:IEC_61970_P452_E3
  a owl:NamedIndividual ;
  a sto:Standard ;
  terms:title "Energy management system application program interface (EMS-API) - Part 452: CIM static transmission network model profiles"@en ;
  rdfs:comment "IEC 61970-452:2017 defines the subset of classes, class attributes, and roles from the CIM necessary to execute state estimation and power flow applications. This standard is intended for two distinct audiences, data producers and data recipients, and may be read from two perspectives. From the standpoint of model export software used by a data producer, the document describes a minimum subset of CIM classes, attributes, and associations which must be present in an XML formatted data file for model exchange. This new edition includes the following significant technical changes with respect to the previous edition: the Equipment profile has been split into three separate profiles, CoreEquipment, Operation and ShortCircuit; the HVDC model has been replaced with the new model defined in Edition 6 of 61970‑301."@en ;
  rdfs:label "IEC 61970-452:2017"@en ;
  prov:wasRevisionOf sto:IEC_61970_P452_E2 ;
  sto:hasAvailableLanguage lang:eng ;
  sto:hasAvailableLanguage lang:fra ;
  sto:hasEdition "3.0"^^xsd:float ;
  sto:hasFileSize sto:FileSizeIEC_61970_P452_E3 ;
  sto:hasICS sto:ICS_33_200 ;
  sto:hasOfficialResource <https://webstore.iec.ch/publication/30444> ;
  sto:hasPages "342"^^xsd:int ;
  sto:hasPublicationDate "2017-07-26"^^xsd:date ;
  sto:hasPublisher sto:IEC ;
  sto:hasStatus "Valid"@en ;
  sto:hasTag "IEC 61970-452:2017 "@en ;
  sto:hasTechnicalCommittee sto:TC_57 ;
  sto:hasWikipediaArticle <https://en.wikipedia.org/wiki/IEC_61970> ;
  sto:isRelevantFor sto:Automation ;
  sto:isRelevantFor sto:CGMES ;
  sto:isRelevantFor sto:CyberSecurity ;
  sto:isRelevantFor sto:SmartCity ;
  sto:isRelevantFor sto:SmartEnergy ;
  sto:isRelevantFor sto:SmartGrid ;
.
sto:IEC_61987_X
  a owl:NamedIndividual ;
  a foaf:Document ;
  a sto:Publication ;
  a sto:Standard ;
  terms:creator sto:IEC ;
  terms:license sto:PrivateLicenseDocument ;
  rdfs:comment "Industrial-process measurement and control - Data structures and elements in process equipment catalogs - Measuring equipment with analogue and digital output"@en ;
  rdfs:label "IEC 61987_X"@en ;
  foaf:maker sto:IEC ;
  sto:hasClassification rami:Engineering ;
  sto:hasClassification sto:RAMIControlDevice ;
  sto:hasClassification sto:RAMIEnterprise ;
  sto:hasClassification sto:RAMIFieldDevice ;
  sto:hasClassification sto:RAMIProduct ;
  sto:hasClassification sto:RAMIStation ;
  sto:hasClassification sto:RAMIWorkCenter ;
  sto:hasMotivation "Properties and LOPs as an informational representation of the features of measuring equipment. The referenced standards define general principles (e.g. part 11) as well as specific LOPs for specific device types. These international standards also may serve as examples for description of products."@en ;
  sto:hasOfficialResource <https://webstore.iec.ch/publication/6225> ;
  sto:hasPublisher sto:IEC ;
  sto:hasTag "LOPs in PA"@en ;
.
sto:IEC_62061
  a owl:NamedIndividual ;
  a foaf:Document ;
  a sto:Publication ;
  a sto:Standard ;
  terms:creator sto:IEC ;
  rdfs:comment "provides requirements that are applicable to the system level design of all types of machinery safety-related electrical control systems and also for the design of non-complex subsystems or devices."@en ;
  rdfs:label "IEC 60061"@en ;
  foaf:maker sto:IEC ;
  sto:hasClassification rami:Safety ;
  sto:hasDBpediaResource <http://dbpedia.org/resource/IEC_62061> ;
  sto:hasOfficialResource <https://webstore.iec.ch/publication/22797> ;
  sto:hasPublisher sto:IEC ;
  sto:hasTag "Safety of machinery"@en ;
  sto:hasWikipediaArticle <https://en.wikipedia.org/wiki/IEC_62061> ;
  sto:relatedTo sto:IEC_61508 ;
  sto:relatedTo sto:IEC_61511 ;
  sto:relatedTo sto:IEC_62061 ;
  sto:relatedTo sto:ISO_13849 ;
.
sto:IEC_62237
  a owl:NamedIndividual ;
  a foaf:Document ;
  a sto:Publication ;
  a sto:Standard ;
  a sto:TechnicalSpecification ;
  terms:creator sto:IEC ;
  rdfs:comment "Live working - Insulating hoses with fittings for use with hydraulic tools and equipment."@en ;
  rdfs:label "IEC 62237"@en ;
  foaf:maker sto:IEC ;
  sto:hasClassification rami:AdminShellGeneral ;
  sto:hasClassification sto:ProductionSystemModelData ;
  sto:hasClassification sto:RAMIControlDevice ;
  sto:hasClassification sto:RAMIFieldDevice ;
  sto:hasClassification sto:RAMIStation ;
  sto:hasClassification sto:RAMIWorkCenter ;
  sto:hasDomain sto:IndustrialAutomation ;
  sto:hasOfficialResource <https://webstore.iec.ch/publication/6626> ;
  sto:hasPublicationDate "2003-10-26"^^xsd:date ;
  sto:hasPublisher sto:IEC ;
  sto:relatedTo sto:IEC_62237 ;
  sto:relatedTo sto:IEC_62337 ;
.
sto:IEC_62264
  a owl:NamedIndividual ;
  a foaf:Document ;
  a sto:Publication ;
  a sto:Standard ;
  terms:creator sto:IEC ;
  terms:creator sto:MESA ;
  terms:license sto:PrivateLicenseDocument ;
  rdfs:comment "Enterprise-control system integration - Models and terminology"@en ;
  rdfs:comment "IEC 62264 is an international standard for enterprise-control system integration. This standard is based upon ANSI/ISA-95."@en ;
  rdfs:label "IEC 62264"@en ;
  rdfs:seeAlso <https://en.wikipedia.org/wiki/B2MML> ;
  skos:altLabel "B2MML" ;
  foaf:maker sto:IEC ;
  foaf:maker sto:MESA ;
  sto:hasClassification sto:RAMIFunctional ;
  sto:hasDBpediaResource <http://dbpedia.org/resource/IEC_62264> ;
  sto:hasDeveloper sto:IEC ;
  sto:hasDomain "Enterprise Control"@en ;
  sto:hasMotivation "Informational representation of MES and ERP models."@en ;
  sto:hasOfficialResource <http://www.iso.org/iso/catalogue_detail.htm?csnumber=63740> ;
  sto:hasOfficialResource <https://webstore.iec.ch/publication/6675> ;
  sto:hasOfficialResource <https://www.iso.org/standard/57308.html> ;
  sto:hasPublisher sto:IEC ;
  sto:hasPublisher sto:MESA ;
  sto:hasTag "Enterprise control systems"@en ;
  sto:hasTag "Enterprise-control system integration"@en ;
  sto:hasWikipediaArticle <https://en.wikipedia.org/wiki/IEC_62264> ;
  sto:relatedTo sto:ISA-95 ;
.
sto:IEC_62264_P6
  a owl:NamedIndividual ;
  a sto:Standard ;
  terms:title "Enterprise-control system integration - Part 6: Messaging Service Model"@en ;
  rdfs:comment "IEC PAS 62264-6:2016(E) defines a model of a set of messaging services for information exchanges across Levels 3 and 4, and within Level 3, between applications performing business and manufacturing activities. It defines a standard interface for information exchange between systems."@en ;
  rdfs:label " IEC PAS 62264-6:2016"@en ;
  sto:frames sto:communication ;
  sto:hasAvailableLanguage lang:eng ;
  sto:hasEdition "1.0"^^xsd:float ;
  sto:hasFileSize sto:FileSizeIEC_62264_P6 ;
  sto:hasICS sto:ICS_25_040_99 ;
  sto:hasICS sto:ICS_35_100 ;
  sto:hasICS sto:ICS_35_100_50 ;
  sto:hasOfficialResource <https://webstore.iec.ch/publication/25315> ;
  sto:hasPages "50"^^xsd:int ;
  sto:hasPublicationDate "2016-07-05"^^xsd:date ;
  sto:hasPublisher sto:IEC ;
  sto:hasTag "IEC PAS 62264-6:2016"@en ;
  sto:hasTechnicalCommittee sto:TC_65 ;
.
sto:IEC_62279
  a owl:NamedIndividual ;
  a foaf:Document ;
  a sto:Publication ;
  a sto:Standard ;
  terms:creator sto:IEC ;
  rdfs:comment "IEC 62279:2015 specifies the process and technical requirements for the development of software for programmable electronic systems for use in railway control and protection applications. It is aimed at use in any area where there are safety implications. These systems can be implemented using dedicated microprocessors, programmable logic controllers, multiprocessor distributed systems, larger scale central processor systems or other architectures."@en ;
  rdfs:label "IEC 62279"@en ;
  foaf:maker sto:IEC ;
  sto:hasClassification sto:Safety ;
  sto:hasDomain sto:ITSecurity ;
  sto:hasOfficialResource <https://webstore.iec.ch/publication/22781> ;
  sto:hasPublicationDate "2015-06-25"^^xsd:date ;
  sto:hasPublisher sto:IEC ;
.
sto:IEC_62337
  a owl:NamedIndividual ;
  a foaf:Document ;
  a sto:Publication ;
  a sto:Standard ;
  terms:creator sto:IEC ;
  rdfs:comment "Commissioning of electrical, instrumentation and control systems in the process industry - Specific phases and milestones."@en ;
  rdfs:label "IEC 62337"@en ;
  foaf:maker sto:IEC ;
  sto:hasClassification rami:ConditionMonitoring ;
  sto:hasClassification rami:Lifecycle_Status ;
  sto:hasClassification sto:ProductionSystemModelData ;
  sto:hasClassification sto:RAMIEnterprise ;
  sto:hasClassification sto:RAMIFunctionalLayer ;
  sto:hasClassification sto:RAMIWorkCenter ;
  sto:hasDomain sto:IndustrialAutomation ;
  sto:hasOfficialResource <https://webstore.iec.ch/publication/6871> ;
  sto:hasPublicationDate "2012-02-22"^^xsd:date ;
  sto:hasPublisher sto:IEC ;
  sto:relatedTo sto:IEC_62237 ;
  sto:relatedTo sto:IEC_62337 ;
.
sto:IEC_62424
  a owl:NamedIndividual ;
  a foaf:Document ;
  a sto:Publication ;
  a sto:Standard ;
  terms:creator sto:IEC ;
  terms:license sto:PrivateLicenseDocument ;
  dul:isComponentOf sto:IEC_62714 ;
  rdfs:comment "CAEX (Computer Aided Engineering Exchange) is a neutral data format that allows storage of hierarchical object information, e.g. the hierarchical architecture of a plant. On a certain abstraction level, a plant consists in modules or components that are interconnected. CAEX allows storage of those modules or components by means of objects. Object oriented concepts as encapsulation, classes, class libraries, instances, instance hierarchies, inheritance, relations, attributes and interfaces are explicitly supported. CAEX bases on XML and is defined as XML schema (xsd file). The original intention of developing CAEX was the industrial lack of a common and established data exchange between process engineering tools and process control engineering tools. However, CAEX can be applied to all types of static object information, e.g. plant topologies, document topologies, product topologies, petri nets, but also for non-technical applications like phylogenetic trees."@en ;
  rdfs:label "IEC 62424"@en ;
  foaf:maker sto:IEC ;
  sto:hasDBpediaResource <http://dbpedia.org/resource/CAEX> ;
  sto:hasOfficialResource <https://webstore.iec.ch/publication/25442> ;
  sto:hasPublisher sto:IEC ;
  sto:hasTag "CAEX"@en ;
  sto:hasWikipediaArticle <https://en.wikipedia.org/wiki/CAEX> ;
.
sto:IEC_62443
  a owl:NamedIndividual ;
  a foaf:Document ;
  a sto:Publication ;
  a sto:Standard ;
  a sto:StandardClassification ;
  terms:creator sto:ANSI ;
  terms:creator sto:IEC ;
  terms:creator sto:ISA ;
  terms:license sto:PrivateLicenseDocument ;
  dul:associatedWith sto:Identification ;
  rdfs:comment "Defines procedures for implementing electronically secure Industrial Automation and Control Systems."@en ;
  rdfs:comment "ISA/IEC-62443 is a series of standards, technical reports, and related information that define procedures for implementing electronically secure Industrial Automation and Control Systems (IACS). This guidance applies to end-users (i.e. asset owner), system integrators, security practitioners, and control systems manufacturers responsible for manufacturing, designing, implementing, or managing industrial automation and control systems."@en ;
  rdfs:label "IEC 62443"@en ;
  skos:altLabel "ISA 99" ;
  skos:note "TODO" ;
  foaf:maker sto:ANSI ;
  foaf:maker sto:IEC ;
  foaf:maker sto:ISA ;
  sto:alignsWith sto:Identification ;
  sto:hasClassification rami:Security ;
  sto:hasClassification sto:CrossLevel ;
  sto:hasClassification sto:IDSRAMCertification ;
  sto:hasClassification sto:IIRASecurity ;
  sto:hasDBpediaResource <http://dbpedia.org/page/Cyber_security_standards#ISA/IEC-62443_(formerly_ISA-99)> ;
  sto:hasDeveloper sto:ANSI ;
  sto:hasDeveloper sto:ISA ;
  sto:hasMotivation "Cyber attacks threat the industry and can cause damage to property and personal injury and affect the image of companies. The Standard allows to define procedures for implementing electronically secure Industrial Automation and Control Systems (IACS). This guidance applies to end-users, system integrators, security practitioners, and control systems manufacturers responsible for manufacturing, designing, implementing, or managing industrial automation and control systems"@en ;
  sto:hasOfficialResource <https://webstore.iec.ch/publication/7029> ;
  sto:hasOfficialResource <https://webstore.iec.ch/publication/7033> ;
  sto:hasPublisher sto:ANSI ;
  sto:hasPublisher sto:IEC ;
  sto:hasPublisher sto:ISA ;
  sto:hasTag "Electronically secure Industrial Automation and Control Systems"@en ;
  sto:hasTag "Network and system security for industrial-process measurement and control"@en ;
  sto:hasWikipediaArticle <https://en.wikipedia.org/wiki/Cyber_security_standards#ISA.2FIEC-62443_.28formerly_ISA-99.29> ;
.
sto:IEC_62453
  a owl:NamedIndividual ;
  a foaf:Document ;
  a sto:Publication ;
  a sto:Standard ;
  terms:creator sto:IEC ;
  rdfs:comment "Field device tool (FDT) interface specification - Overview and guidance"@en ;
  rdfs:label "IEC 62453"@en ;
  foaf:maker sto:IEC ;
  sto:hasClassification rami:Configuration ;
  sto:hasClassification sto:RAMIControlDevice ;
  sto:hasClassification sto:RAMIFieldDevice ;
  sto:hasClassification sto:RAMIStation ;
  sto:hasMotivation "FDT is an interface for integration of devices into a system (e.g. control system or engineering system). The standard supports factory automation as well as process automation with a wide range of fieldbus protocols. The interface defines fieldbus-independent mechanisms for accessing data and functions of the devices."@en ;
  sto:hasOfficialResource <https://webstore.iec.ch/publication/7040> ;
  sto:hasPublisher sto:IEC ;
  sto:hasTag "FDT"@en ;
  sto:relatedTo sto:DIN_SPEC_16592 ;
  sto:relatedTo sto:IEC_61131 ;
  sto:relatedTo sto:IEC_61360 ;
  sto:relatedTo sto:IEC_61499 ;
  sto:relatedTo sto:IEC_61804 ;
  sto:relatedTo sto:IEC_61850 ;
  sto:relatedTo sto:IEC_61987_X ;
  sto:relatedTo sto:IEC_62424 ;
  sto:relatedTo sto:IEC_62453 ;
  sto:relatedTo sto:IEC_62541 ;
  sto:relatedTo sto:IEC_62714 ;
  sto:relatedTo sto:ISO_13584 ;
  sto:relatedTo sto:ISO_14306 ;
  sto:relatedTo sto:ISO_15746 ;
  sto:relatedTo sto:ISO_15926 ;
  sto:relatedTo sto:ISO_18629 ;
  sto:relatedTo sto:ISO_18828-2 ;
  sto:relatedTo sto:ISO_20922 ;
  sto:relatedTo sto:ISO_22400 ;
  sto:relatedTo sto:ISO_29002 ;
  sto:relatedTo sto:ISO_ASTM_52915 ;
  sto:relatedTo sto:ISO_PAS_17506 ;
  sto:relatedTo sto:MathML ;
  sto:relatedTo sto:SysML ;
  sto:relatedTo sto:eClass ;
.
sto:IEC_62541
  a owl:NamedIndividual ;
  a foaf:Document ;
  a sto:Publication ;
  a sto:Standard ;
  terms:license sto:GPLv2 ;
  terms:license sto:OpenLicenseDocument ;
  rdfs:comment "OPC Unified Architecture (OPC UA) is an industrial M2M communication protocol for interoperability developed by the OPC Foundation. It is the successor to Open Platform Communications (OPC). Although developed by the same organization, OPC UA differs significantly from its predecessor. The Foundation's goal for this project was to provide a path forward from the original OPC communications model (namely the Microsoft Windows only process exchange COM/DCOM) to a cross-platform service-oriented architecture (SOA) for process control, while enhancing security and providing an information model."@en ;
  rdfs:label "IEC 62541"@en ;
  sto:hasAvailableLanguage lang:eng ;
  sto:hasClassification sto:Communication ;
  sto:hasClassification sto:DataSovereignty ;
  sto:hasClassification sto:IDSRAMSystemLayer ;
  sto:hasClassification sto:IICFFrameworkLayer ;
  sto:hasClassification sto:IIRAApplicationDomain ;
  sto:hasClassification sto:IIRAOperationsDomain ;
  sto:hasClassification sto:InformationDomain ;
  sto:hasClassification sto:RAMICommunicationlayer ;
  sto:hasClassification sto:RAMIConnectedWorld ;
  sto:hasClassification sto:RAMIControlDevice ;
  sto:hasClassification sto:RAMIEnterprise ;
  sto:hasClassification sto:RAMIFieldDevice ;
  sto:hasClassification sto:RAMIStation ;
  sto:hasClassification sto:RAMIWorkCenter ;
  sto:hasClassification sto:SCADALevel ;
  sto:hasDBpediaResource <http://dbpedia.org/resource/OPC_Unified_Architecture> ;
  sto:hasDeveloper sto:OPC_Foundation ;
  sto:hasDomain sto:IndustrialAutomation ;
  sto:hasOfficialResource <https://opcfoundation.org/about/opc-technologies/opc-ua/> ;
  sto:hasPublisher sto:IEC ;
  sto:hasTag "OPC UA"@en ;
  sto:hasTargetConcern sto:AutonomousCommunication ;
  sto:hasWikipediaArticle <https://en.wikipedia.org/wiki/OPC_Unified_Architecture> ;
  sto:relatedTo sto:DIN_SPEC_16592 ;
  sto:relatedTo sto:IEC_61131 ;
  sto:relatedTo sto:IEC_61360 ;
  sto:relatedTo sto:IEC_61499 ;
  sto:relatedTo sto:IEC_61804 ;
  sto:relatedTo sto:IEC_61850 ;
  sto:relatedTo sto:IEC_61987_X ;
  sto:relatedTo sto:IEC_62424 ;
  sto:relatedTo sto:IEC_62453 ;
  sto:relatedTo sto:IEC_62541 ;
  sto:relatedTo sto:IEC_62714 ;
  sto:relatedTo sto:ISO_13584 ;
  sto:relatedTo sto:ISO_14306 ;
  sto:relatedTo sto:ISO_15746 ;
  sto:relatedTo sto:ISO_15926 ;
  sto:relatedTo sto:ISO_18629 ;
  sto:relatedTo sto:ISO_18828-2 ;
  sto:relatedTo sto:ISO_20922 ;
  sto:relatedTo sto:ISO_22400 ;
  sto:relatedTo sto:ISO_29002 ;
  sto:relatedTo sto:ISO_ASTM_52915 ;
  sto:relatedTo sto:ISO_PAS_17506 ;
  sto:relatedTo sto:MathML ;
  sto:relatedTo sto:SysML ;
  sto:relatedTo sto:eClass ;
  sto:useStructureOf sto:IEC_61804 ;
.
sto:IEC_62591
  a owl:NamedIndividual ;
  a foaf:Document ;
  a sto:Publication ;
  a sto:Standard ;
  terms:creator sto:IEC ;
  rdfs:comment "Industrial networks - Wireless communication network and communication profiles."@en ;
  rdfs:label "IEC 62591"@en ;
  foaf:maker sto:IEC ;
  sto:hasDBpediaResource <http://dbpedia.org/page/WirelessHART> ;
  sto:hasOfficialResource <https://webstore.iec.ch/publication/24433> ;
  sto:hasPublisher sto:IEC ;
  sto:hasWikipediaArticle <https://en.wikipedia.org/wiki/WirelessHART> ;
.
sto:IEC_62656
  a owl:NamedIndividual ;
  a foaf:Document ;
  a sto:Publication ;
  a sto:Standard ;
  terms:creator sto:IEC ;
  rdfs:comment "Specifies the logical structure for a set of spreadsheets, used as data parcels, to define, transfer and register product ontologies"@en ;
  rdfs:label "IEC 62656"@en ;
  foaf:maker sto:IEC ;
  sto:hasOfficialResource <https://webstore.iec.ch/publication/7326> ;
  sto:hasPublisher sto:IEC ;
.
sto:IEC_62714
  a owl:NamedIndividual ;
  a foaf:Document ;
  a sto:Publication ;
  a sto:Standard ;
  terms:creator sto:IEC ;
  terms:license sto:OpenLicenseDocument ;
  rdfs:comment "Engineering data exchange format for use in industrial automation systems engineering - Automation markup language - Architecture and general requirements"@en ;
  rdfs:label "IEC 62714"@en ;
  foaf:maker sto:IEC ;
  sto:hasClassification rami:Engineering ;
  sto:hasClassification sto:ProductionSystemEngineering ;
  sto:hasClassification sto:RAMIControlDevice ;
  sto:hasClassification sto:RAMIFieldDevice ;
  sto:hasClassification sto:RAMIInformationLayer ;
  sto:hasClassification sto:RAMIProduct ;
  sto:hasDBpediaResource <http://dbpedia.org/resource/AutomationML> ;
  sto:hasOfficialResource <https://www.automationml.org/> ;
  sto:hasPublisher sto:IEC ;
  sto:hasTag "AML"@en ;
  sto:hasTag "AutomationML"@en ;
  sto:hasWikipediaArticle <https://en.wikipedia.org/wiki/AutomationML> ;
  sto:relatedTo sto:DIN_SPEC_16592 ;
  sto:relatedTo sto:IEC_61131 ;
  sto:relatedTo sto:IEC_61360 ;
  sto:relatedTo sto:IEC_61499 ;
  sto:relatedTo sto:IEC_61804 ;
  sto:relatedTo sto:IEC_61850 ;
  sto:relatedTo sto:IEC_61987_X ;
  sto:relatedTo sto:IEC_62424 ;
  sto:relatedTo sto:IEC_62453 ;
  sto:relatedTo sto:IEC_62541 ;
  sto:relatedTo sto:IEC_62714 ;
  sto:relatedTo sto:ISO_13584 ;
  sto:relatedTo sto:ISO_14306 ;
  sto:relatedTo sto:ISO_15746 ;
  sto:relatedTo sto:ISO_15926 ;
  sto:relatedTo sto:ISO_18629 ;
  sto:relatedTo sto:ISO_18828-2 ;
  sto:relatedTo sto:ISO_20922 ;
  sto:relatedTo sto:ISO_22400 ;
  sto:relatedTo sto:ISO_29002 ;
  sto:relatedTo sto:ISO_ASTM_52915 ;
  sto:relatedTo sto:ISO_PAS_17506 ;
  sto:relatedTo sto:MathML ;
  sto:relatedTo sto:SysML ;
  sto:relatedTo sto:eClass ;
  sto:uses sto:MathML ;
.
sto:IEC_62769_P1
  a owl:NamedIndividual ;
  a sto:standard ;
  terms:creator sto:IEC ;
  terms:title "Field device integration (FDI) - Part 1: Overview"@en ;
  rdfs:comment "IEC 62769-1:2015 describes the concepts and overview of the Field Device Integration (FDI) specifications. The detailed motivation for the creation of this technology is also described. It helps to understand the other parts of this multi-part standard."@en ;
  rdfs:label "IEC 62769-1:2015  "@en ;
  foaf:maker sto:IEC ;
  sto:hasAvailableLanguage lang:eng ;
  sto:hasAvailableLanguage lang:fra ;
  sto:hasEdition "1.0"^^xsd:float ;
  sto:hasFileSize sto:FileSizeIEC_62769_P1 ;
  sto:hasICS sto:ICS_25_040_40 ;
  sto:hasICS sto:ICS_35_100_05 ;
  sto:hasOfficialResource <https://webstore.iec.ch/publication/22453> ;
  sto:hasPages "64"^^xsd:int ;
  sto:hasPublicationDate "2015-05-12"^^xsd:date ;
  sto:hasPublisher sto:IEC ;
  sto:hasStabilityDate "2019"^^xsd:gYear ;
  sto:hasTag "IEC 62769-1:2015   "@en ;
  sto:hasTechnicalCommittee sto:TC_65 ;
.
sto:IEC_62794
  a owl:NamedIndividual ;
  a foaf:Document ;
  a sto:Publication ;
  a sto:Standard ;
  a sto:TechnicalReport ;
  terms:creator sto:IEC ;
  terms:hasLicense "Private"@en ;
  terms:license sto:PrivateLicenseDocument ;
  rdfs:comment "Industrial-process measurement, control and automation - Reference model for representation of production facilities (digital factory)"@en ;
  rdfs:label "IEC TR 62794"@en ;
  foaf:maker sto:IEC ;
  sto:hasClassification rami:AdminShellGeneral ;
  sto:hasClassification sto:RAMIControlDevice ;
  sto:hasClassification sto:RAMIFieldDevice ;
  sto:hasClassification sto:RAMIStation ;
  sto:hasClassification sto:RAMIWorkCenter ;
  sto:hasMotivation "The standards for Digital Factory define methods and information models, which are required for self description of I40-components. "@en ;
  sto:hasOfficialResource <https://webstore.iec.ch/publication/7433> ;
  sto:hasPublisher sto:IEC ;
  sto:hasTag "DF/TR"@en ;
  sto:relatedTo sto:IEC_62794 ;
  sto:relatedTo sto:IEC_62832 ;
.
sto:IEC_62832
  a owl:NamedIndividual ;
  a foaf:Document ;
  a sto:Publication ;
  a sto:Standard ;
  a sto:TechnicalSpecification ;
  terms:creator sto:IEC ;
  terms:language lang:eng ;
  rdfs:comment "Industrial-process measurement, control and automation - Digital factory framework - Part 1: General principles"@en ;
  rdfs:label "IEC TS 62832-1:2016 "@en ;
  foaf:maker sto:IEC ;
  sto:hasAvailableLanguage lang:eng ;
  sto:hasClassification rami:AdminShellGeneral ;
  sto:hasClassification sto:RAMIControlDevice ;
  sto:hasClassification sto:RAMIFieldDevice ;
  sto:hasClassification sto:RAMIStation ;
  sto:hasClassification sto:RAMIWorkCenter ;
  sto:hasEdition "1.0"^^xsd:float ;
  sto:hasFileSize sto:FileSizeIEC_62832 ;
  sto:hasICS sto:ICS_25_040_40 ;
  sto:hasOfficialResource <https://webstore.iec.ch/publication/33023> ;
  sto:hasPages "47"^^xsd:int ;
  sto:hasPublicationDate "2016-12-16"^^xsd:date ;
  sto:hasPublisher sto:IEC ;
  sto:hasStabilityDate "2020"^^xsd:gYear ;
  sto:hasTechnicalCommittee sto:TC_65 ;
  sto:relatedTo sto:IEC_62794 ;
  sto:relatedTo sto:IEC_62832 ;
.
sto:IEC_62837
  a owl:NamedIndividual ;
  a foaf:Document ;
  a sto:Publication ;
  a sto:Standard ;
  terms:creator sto:IEC ;
  rdfs:comment "Provides to the technical committees a framework for the development and adaptation of documents in order to improve energy efficiency in manufacturing, process control and industrial facility management."@en ;
  rdfs:label "IEC 62837"@en ;
  foaf:maker sto:IEC ;
  sto:hasOfficialResource <https://webstore.iec.ch/publication/7446> ;
  sto:hasPublisher sto:IEC ;
.
sto:IEC_62890
  a owl:NamedIndividual ;
  a foaf:Document ;
  a sto:Publication ;
  a sto:Standard ;
  terms:creator sto:IEC ;
  terms:license sto:PrivateLicenseDocument ;
  rdfs:comment "Defines standards for lifecycle management for systems and products used in industrial process measurement, control and automation"@en ;
  rdfs:comment "MES KPIs"@en ;
  rdfs:label "IEC 62890"@en ;
  foaf:maker sto:IEC ;
  sto:hasClassification rami:Lifecycle_Status ;
  sto:hasClassification sto:ProductionLifeCycleDataManagement ;
  sto:hasClassification sto:RAMIStation ;
  sto:hasClassification sto:RAMIWorkCenter ;
  sto:hasMotivation "Stations need to describe their operational state and performance parameters towards superior I4.0-Components"@en ;
  sto:hasOfficialResource <http://www.iec.ch/dyn/www/f?p=103:38:16824039984463::::FSP_ORG_ID,FSP_APEX_PAGE,FSP_PROJECT_ID:1250,23,20929> ;
  sto:hasPublisher sto:IEC ;
  sto:hasTag "IEC 62890"@en ;
.
sto:IEC_81714
  a owl:NamedIndividual ;
  a foaf:Document ;
  a sto:Publication ;
  a sto:Standard ;
  terms:creator sto:IEC ;
  terms:creator sto:ISO ;
  rdfs:comment "ISO/IEC 81714 Design of graphical symbols for use in the technical documentation of products -- Part 3: Classification of connect nodes, networks and their encoding-- specifies requirements concerning the classification of connect nodes assigned to graphical symbols, being a representation of functional and product concepts."@en ;
  rdfs:label "IEC 81714"@en ;
  foaf:maker sto:IEC ;
  foaf:maker sto:ISO ;
  sto:hasClassification rami:Engineering ;
  sto:hasClassification rami:Identification ;
  sto:hasClassification sto:ModelingPractice ;
  sto:hasClassification sto:RAMIAssetlayer ;
  sto:hasClassification sto:RAMIProduct ;
  sto:hasDomain sto:CAD ;
  sto:hasOfficialResource <https://www.iso.org/standard/40134.html> ;
  sto:hasPublicationDate "2004-10-01"^^xsd:date ;
  sto:hasPublisher sto:IEC ;
  sto:hasPublisher sto:ISO ;
.
sto:IEC_PAS_63088
  a owl:NamedIndividual ;
  a foaf:Document ;
  a sto:Publication ;
  a sto:Standard ;
  terms:creator sto:IEC ;
  rdfs:comment "IEC PAS 63088:2017(E) describes a reference architecture model in the form of a cubic layer model, RAMI model"@en ;
  rdfs:label "IEC PAS 63088"@en ;
  foaf:maker sto:IEC ;
  sto:hasOfficialResource <https://webstore.iec.ch/publication/30082?lipi=urn%3Ali%3Apage%3Ad_flagship3_pulse_read%3B2vZf0%2FOGS2CeRjny8ARziQ%3D%3D> ;
  sto:hasPublicationDate "2017-03-07"^^xsd:date ;
  sto:hasPublisher sto:IEC ;
  sto:hasTag "RAMI 4.0" ;
.
sto:IEC_TS_62832
  a owl:NamedIndividual ;
  a sto:TechnicalSpecification ;
  terms:license sto:PrivateLicenseDocument ;
  rdfs:comment "Digital Factory Reference model TS"@en ;
  rdfs:label "IEC TS 62832"@en ;
  sto:hasClassification rami:AdminShellGeneral ;
  sto:hasClassification sto:RAMIControlDevice ;
  sto:hasClassification sto:RAMIFieldDevice ;
  sto:hasClassification sto:RAMIStation ;
  sto:hasClassification sto:RAMIWorkCenter ;
  sto:hasMotivation "The standards for Digital Factory define methods and information models, which are required for self description of I40-components. IEC TS 62832 defines methods, which allow to validate or plan connections between assets."@en ;
  sto:hasOfficialResource <https://webstore.iec.ch/publication/33023> ;
  sto:hasPublisher sto:IEC ;
  sto:hasTag "DF/TS"@en ;
.
sto:IEEE
  a owl:NamedIndividual ;
  a foaf:Organization ;
  a sto:StandardOrganization ;
  terms:description "IEEE and its members inspire a global community to innovate for a better tomorrow through highly cited publications, conferences, technology standards, and professional and educational activities. IEEE is the trusted “voice” for engineering, computing, and technology information around the globe."@en ;
  rdfs:seeAlso <https://www.ieee.org/> ;
  sto:abbreviation "IEEE"@en ;
  sto:hasWikipediaArticle <http://wikipedia.org/wiki/Institute_of_Electrical_and_Electronics_Engineers> ;
  sto:orgName "Institute of Electrical and Electronics Engineers"@en ;
.
sto:IEEE_1377-2012
  a owl:NamedIndividual ;
  a foaf:Document ;
  a sto:Publication ;
  a sto:Standard ;
  terms:creator sto:sebastian ;
  rdfs:comment "IEEE Standard for Utility Industry Metering Communication Protocol Application Layer (source: https://www.postscapes.com/internet-of-things-protocols/)"@en ;
  rdfs:label "IEEE 1377-2012"@en ;
  sto:hasOfficialResource <http://standards.ieee.org/findstds/standard/1377-2012.html> ;
.
sto:IEEE_1451
  a owl:NamedIndividual ;
  a foaf:Document ;
  a sto:Publication ;
  a sto:Standard ;
  terms:creator sto:sebastian ;
  rdfs:comment "The IEEE 1451, a family of Smart Transducer Interface Standards, describes a set of open, common, network-independent communication interfaces for connecting transducers (sensors or actuators) to microprocessors, instrumentation systems, and control/field networks. (source: https://www.postscapes.com/internet-of-things-protocols/)"@en ;
  rdfs:label "IEEE 1451"@en ;
  sto:hasOfficialResource <http://grouper.ieee.org/groups/1451/0/body%20frame_files/Family-of-1451_handout.htm> ;
.
sto:IEEE_1686
  a owl:NamedIndividual ;
  a foaf:Document ;
  a sto:Publication ;
  a sto:Standard ;
  terms:creator sto:IEEE ;
  terms:title "Standard for Intelligent Electronic Devices Cyber Security Capabilities"@en ;
  rdfs:comment "The functions and features to be provided in intelligent electronic devices (IEDs) to accommodate critical infrastructure protection programs are defined in this standard. Security regarding the access, operation, configuration, firmware revision and data retrieval from an IED are addressed. Communications for the purpose of power system protection (teleprotection) are not addressed in this standard."@en ;
  rdfs:label "IEEE 1686"@en ;
  foaf:maker sto:IEEE ;
  sto:hasClassification sto:IDSRAMSecurity ;
  sto:hasDBpediaResource <http://dbpedia.org/resource/IEEE_Smart_Grid> ;
  sto:hasDeveloper sto:IEEE ;
  sto:hasOfficialResource <https://standards.ieee.org/standard/1686-2007.html> ;
  sto:hasPublisher sto:IEEE ;
  sto:hasWikipediaArticle <https://en.wikipedia.org/wiki/IEEE_Smart_Grid> ;
.
sto:IEEE_1856
  a owl:NamedIndividual ;
  a foaf:Document ;
  a sto:Publication ;
  a sto:Standard ;
  terms:creator sto:sebastian ;
  rdfs:comment "Standard Framework for Prognostics and Health Management of Electronic Systems (source: https://www.postscapes.com/internet-of-things-protocols/)"@en ;
  rdfs:label "IEEE 1856"@en ;
  sto:hasOfficialResource <http://standards.ieee.org/develop/project/1856.html> ;
.
sto:IEEE_1888-3-2013
  a owl:NamedIndividual ;
  a foaf:Document ;
  a sto:Publication ;
  a sto:Standard ;
  terms:creator sto:sebastian ;
  rdfs:comment " - IEEE Standard for Ubiquitous Green Community Control Network: Security (source: https://www.postscapes.com/internet-of-things-protocols/)"@en ;
  rdfs:label "IEEE 1888.3-2013"@en ;
  sto:hasOfficialResource <http://standards.ieee.org/findstds/standard/1888.3-2013.html> ;
.
sto:IEEE_1905_1-2013
  a owl:NamedIndividual ;
  a foaf:Document ;
  a sto:Publication ;
  a sto:Standard ;
  terms:creator sto:sebastian ;
  rdfs:comment "IEEE Standard for a Convergent Digital Home Network for Heterogeneous Technologies (source: https://www.postscapes.com/internet-of-things-protocols/)"@en ;
  rdfs:label "IEEE 1905.1-2013"@en ;
  sto:hasOfficialResource <http://standards.ieee.org/findstds/standard/1905.1-2013.html> ;
.
sto:IEEE_2413
  a owl:NamedIndividual ;
  a foaf:Document ;
  a sto:Publication ;
  a sto:Standard ;
  terms:creator sto:sebastian ;
  rdfs:comment "IEEE P2413 - Standard for an Architectural Framework for the Internet of Things (IoT) (source: https://www.postscapes.com/internet-of-things-protocols/)"@en ;
  rdfs:label "IEEE 2413"@en ;
  sto:hasOfficialResource <https://standards.ieee.org/develop/project/2413.html> ;
.
sto:IEEE_42010
  a owl:NamedIndividual ;
  owl:sameAs sto:ISO_42010 ;
.
sto:IEEE_802
  a owl:NamedIndividual ;
  a foaf:Document ;
  a sto:Publication ;
  a sto:Standard ;
  terms:creator sto:sebastian ;
  rdfs:comment "IEEE 802.15.4 is a standard which specifies the physical layer and media access control for low-rate wireless personal area networks (LR-WPANs). It is maintained by the IEEE 802.15 working group. It is the basis for the ZigBee,ISA100.11a, WirelessHART, and MiWi specifications, each of which further extends the standard by developing the upper layers which are not defined in IEEE 802.15.4. Alternatively, it can be used with 6LoWPAN and standard Internet protocols to build a wireless embedded Internet. (source: https://www.postscapes.com/internet-of-things-protocols/)"@en ;
  rdfs:label "IEEE 802.15.4"@en ;
  sto:hasWikipediaArticle <https://en.wikipedia.org/wiki/IEEE_802.15.4> ;
.
sto:IEEE_802_16-2012
  a owl:NamedIndividual ;
  a foaf:Document ;
  a sto:Publication ;
  a sto:Standard ;
  terms:creator sto:sebastian ;
  rdfs:comment "IEEE Standard for Air Interface for Broadband Wireless Access Systems (source: https://www.postscapes.com/internet-of-things-protocols/)"@en ;
  rdfs:label "IEEE 802.16p-2012"@en ;
  sto:hasOfficialResource <http://standards.ieee.org/findstds/standard/802.16p-2012.html> ;
.
sto:IEEE_P1828
  a owl:NamedIndividual ;
  a foaf:Document ;
  a sto:Publication ;
  a sto:Standard ;
  terms:creator sto:sebastian ;
  rdfs:comment "Standard for Systems With Virtual Components (source: https://www.postscapes.com/internet-of-things-protocols/)"@en ;
  rdfs:label "IEEE P1828"@en ;
  sto:hasOfficialResource <http://standards.ieee.org/develop/project/1828.html> ;
.
sto:IETF
  a owl:NamedIndividual ;
  a foaf:Organization ;
  a sto:StandardOrganization ;
  rdfs:comment "TODO: complete annotations etc." ;
  rdfs:label "IETF"@en ;
  rdfs:seeAlso <http://wikipedia.org/wiki/Internet_Engineering_Task_Force> ;
  rdfs:seeAlso <http://www.ietf.org/> ;
  sto:abbreviation "IETF"@en ;
  sto:hasWikipediaArticle <http://wikipedia.org/wiki/Internet_Engineering_Task_Force> ;
  sto:orgName "Internet Engineering Task Force"@en ;
.
sto:IIC
  a owl:NamedIndividual ;
  a foaf:Organization ;
  a sto:IIoTConsortium ;
  a sto:StandardOrganization ;
  terms:creator sto:sebastian ;
  dul:associatedWith sto:IIRA ;
  rdfs:comment "Founded in 2014 to further development, adoption and wide-spread use of interconnected machines, intelligent analytics and people at work. (source: https://www.postscapes.com/internet-of-things-protocols/)"@en ;
  rdfs:label "IIC"@en ;
  rdfs:label "Industrial Internet Consortium"@en ;
  sto:hasOfficialResource <http://www.iiconsortium.org/> ;
.
sto:IICF
  a owl:NamedIndividual ;
  a foaf:Document ;
  a sto:Publication ;
  terms:title "Industrial Internet Connectivity Framework"@en ;
  rdfs:isDefinedBy <https://www.iiconsortium.org/IICF.htm> ;
  rdfs:label "IICF"@en ;
  rdfs:seeAlso <https://www.iiconsortium.org/pdf/IIC_PUB_G5_V1.01_PB_20180228.pdf> ;
  sto:hasClassification sto:IIRAConnectivity ;
.
sto:IICFFrameworkLayer
  a owl:NamedIndividual ;
  a sto:IicfConnectivityLayer ;
  a sto:StandardClassification ;
  dul:associatedWith sto:DDS ;
  dul:associatedWith sto:IDSRAMGovernance ;
  dul:associatedWith sto:IDSRAMSystemLayer ;
  dul:associatedWith sto:IEC_62541 ;
  dul:associatedWith sto:oneM2M ;
  dul:associatedWith <https://www.wikidata.org/wiki/Q1548249> ;
  dul:isPartOf sto:IIRAConnectivity ;
  rdfs:comment "IICF Framework Layer an instance of the IICF Connectivity Layer"@en ;
  rdfs:comment "IICF Framework Layer"@en ;
  rdfs:isDefinedBy <https://www.iiconsortium.org/pdf/IIC_PUB_G5_V1.01_PB_20180228.pdf> ;
  rdfs:label "IICF Framework Layer"@en ;
  sto:alignsWith sto:IDSRAMGovernance ;
  sto:alignsWith sto:IDSRAMSystemLayer ;
  sto:frames sto:Authentication ;
  sto:frames sto:Communication ;
  sto:frames sto:DataAccess ;
  sto:frames sto:DataDiscovery ;
  sto:frames sto:Governance ;
  sto:frames sto:Identification ;
  sto:frames sto:IdentityManagement ;
  sto:frames sto:IntegrityProtection ;
  sto:frames sto:Interoperability ;
  sto:frames sto:QualityOfService ;
  sto:frames sto:SecureCommunication ;
  sto:frames sto:Security ;
  sto:frames sto:SemanticInteroperability ;
  sto:frames sto:ServiceDescription ;
  sto:frames sto:ServiceDiscovery ;
  sto:frames sto:SyntacticInteroperability ;
  sto:frames sto:Trustworthiness ;
.
sto:IICFFrameworkLayerAnno
  a <https://www.w3.org/ns/oaAnnotation> ;
  <https://www.w3.org/ns/oahasBody> sto:IICFFrameworkLayer ;
  <https://www.w3.org/ns/oahasTarget> [
      a <https://www.w3.org/ns/oaSpecificResource> ;
      terms:format "pdf" ;
      <https://www.w3.org/ns/oahasSelector> [
          a <https://www.w3.org/ns/oaRangeSelector> ;
          <https://www.w3.org/ns/oahasEndSelector> [
              a <https://www.w3.org/ns/oaXPathSelector> ;
              rdf:value "Page 17" ;
            ] ;
          <https://www.w3.org/ns/oahasStartSelector> [
              a <https://www.w3.org/ns/oaXPathSelector> ;
              rdf:value "Page 14" ;
            ] ;
        ] ;
      <https://www.w3.org/ns/oahasSource> sto:The_Industrial_Internet_of_Things_Volume_G5_Connectivity_Framework ;
    ] ;
.
sto:IICFLinkLayer
  a owl:NamedIndividual ;
  a sto:IicfConnectivityLayer ;
  a sto:StandardClassification ;
  dul:associatedWith sto:IEEE_802 ;
  dul:associatedWith sto:IEEE_802_16-2012 ;
  dul:associatedWith sto:WiFi ;
  dul:isPartOf sto:IIRAConnectivity ;
  rdfs:label "IICF Link Layer"@en ;
  sto:frames sto:Communication ;
.
sto:IICFLinkLayerAnno
  a <https://www.w3.org/ns/oaAnnotation> ;
  <https://www.w3.org/ns/oahasBody> sto:IICFLinkLayer ;
  <https://www.w3.org/ns/oahasTarget> [
      a <https://www.w3.org/ns/oaSpecificResource> ;
      terms:format "pdf" ;
      <https://www.w3.org/ns/oahasSelector> [
          a <https://www.w3.org/ns/oaRangeSelector> ;
          <https://www.w3.org/ns/oahasEndSelector> [
              a <https://www.w3.org/ns/oaXPathSelector> ;
              rdf:value "Page 17" ;
            ] ;
          <https://www.w3.org/ns/oahasStartSelector> [
              a <https://www.w3.org/ns/oaXPathSelector> ;
              rdf:value "Page 14" ;
            ] ;
        ] ;
      <https://www.w3.org/ns/oahasSource> sto:The_Industrial_Internet_of_Things_Volume_G5_Connectivity_Framework ;
    ] ;
.
sto:IICFNetworkLayer
  a owl:NamedIndividual ;
  a sto:IicfConnectivityLayer ;
  a sto:StandardClassification ;
  dul:associatedWith sto:IPv6 ;
  dul:isPartOf sto:IIRAConnectivity ;
  rdfs:label "IICF Network Layer"@en ;
  sto:frames sto:Communication ;
  sto:frames sto:IPv4Support ;
  sto:frames sto:IPv6Support ;
  sto:frames sto:Interoperability ;
  sto:frames sto:SyntacticInteroperability ;
.
sto:IICFNetworkLayerAnno
  a <https://www.w3.org/ns/oaAnnotation> ;
  <https://www.w3.org/ns/oahasBody> sto:IICFNetworkLayer ;
  <https://www.w3.org/ns/oahasTarget> [
      a <https://www.w3.org/ns/oaSpecificResource> ;
      terms:format "pdf" ;
      <https://www.w3.org/ns/oahasSelector> [
          a <https://www.w3.org/ns/oaRangeSelector> ;
          <https://www.w3.org/ns/oahasEndSelector> [
              a <https://www.w3.org/ns/oaXPathSelector> ;
              rdf:value "Page 17" ;
            ] ;
          <https://www.w3.org/ns/oahasStartSelector> [
              a <https://www.w3.org/ns/oaXPathSelector> ;
              rdf:value "Page 14" ;
            ] ;
        ] ;
      <https://www.w3.org/ns/oahasSource> sto:The_Industrial_Internet_of_Things_Volume_G5_Connectivity_Framework ;
    ] ;
.
sto:IICFPhysicalLayer
  a owl:NamedIndividual ;
  a sto:IicfConnectivityLayer ;
  a sto:StandardClassification ;
  dul:associatedWith sto:IEEE_802 ;
  dul:associatedWith sto:IEEE_802_16-2012 ;
  dul:isPartOf sto:IIRAConnectivity ;
  rdfs:label "IICF Physical Layer" ;
  sto:frames sto:Communication ;
.
sto:IICFPhysicalLayerAnno
  a <https://www.w3.org/ns/oaAnnotation> ;
  <https://www.w3.org/ns/oahasBody> sto:IICFPhysicalLayer ;
  <https://www.w3.org/ns/oahasTarget> [
      a <https://www.w3.org/ns/oaSpecificResource> ;
      terms:format "pdf" ;
      <https://www.w3.org/ns/oahasSelector> [
          a <https://www.w3.org/ns/oaRangeSelector> ;
          <https://www.w3.org/ns/oahasEndSelector> [
              a <https://www.w3.org/ns/oaXPathSelector> ;
              rdf:value "Page 17" ;
            ] ;
          <https://www.w3.org/ns/oahasStartSelector> [
              a <https://www.w3.org/ns/oaXPathSelector> ;
              rdf:value "Page 14" ;
            ] ;
        ] ;
      <https://www.w3.org/ns/oahasSource> sto:The_Industrial_Internet_of_Things_Volume_G5_Connectivity_Framework ;
    ] ;
.
sto:IICFTansportLayer
  a owl:NamedIndividual ;
  a sto:IicfConnectivityLayer ;
  a sto:StandardClassification ;
  dul:associatedWith sto:HTTP ;
  dul:associatedWith sto:HTTP2 ;
  dul:associatedWith sto:IEC_61158 ;
  dul:associatedWith sto:ISO_20922 ;
  dul:associatedWith sto:RFC_2616 ;
  dul:associatedWith sto:RFC_793 ;
  dul:associatedWith sto:RFC_8323 ;
  dul:associatedWith sto:UDP ;
  dul:isPartOf sto:IIRAConnectivity ;
  rdfs:label "IICF Transport Layer"@en ;
  sto:frames sto:CardinalityOfDataSources ;
  sto:frames sto:CardinalityOfParticipants ;
  sto:frames sto:Communication ;
  sto:frames sto:EndpointInvocation ;
  sto:frames sto:Interoperability ;
  sto:frames sto:Multilaterism ;
  sto:frames sto:SecureCommunication ;
  sto:frames sto:Security ;
  sto:frames sto:ServiceComposition ;
  sto:frames sto:SyntacticInteroperability ;
  sto:frames sto:TimeSynchronization ;
  sto:frames sto:Trustworthiness ;
  sto:frames sto:Unicast ;
.
sto:IICFTansportLayerAnno
  a <https://www.w3.org/ns/oaAnnotation> ;
  <https://www.w3.org/ns/oahasBody> sto:IICFTansportLayer ;
  <https://www.w3.org/ns/oahasTarget> [
      a <https://www.w3.org/ns/oaSpecificResource> ;
      terms:format "pdf" ;
      <https://www.w3.org/ns/oahasSelector> [
          a <https://www.w3.org/ns/oaRangeSelector> ;
          <https://www.w3.org/ns/oahasEndSelector> [
              a <https://www.w3.org/ns/oaXPathSelector> ;
              rdf:value "Page 17" ;
            ] ;
          <https://www.w3.org/ns/oahasStartSelector> [
              a <https://www.w3.org/ns/oaXPathSelector> ;
              rdf:value "Page 14" ;
            ] ;
        ] ;
      <https://www.w3.org/ns/oahasSource> sto:The_Industrial_Internet_of_Things_Volume_G5_Connectivity_Framework ;
    ] ;
.
sto:IICVocabulary
  a owl:NamedIndividual ;
  a foaf:Document ;
  a sto:Publication ;
  a sto:StandardClassification ;
  terms:creator sto:IIC ;
  terms:creator sto:sebastian ;
  dul:associatedWith sto:IDSRAMInformationLayer ;
  rdfs:label "IIC Vocabulary"@en ;
  foaf:maker sto:IIC ;
  sto:alignsWith sto:IDSRAMInformationLayer ;
  sto:hasPublisher sto:IIC ;
  sto:isDescribedin sto:IIRA ;
.
sto:IIC_PUB_G1_V1_80_20170131
  a <https://www.w3.org/ns/oaSpecificResource> ;
  rdfs:label "The Industrial Internet of Things Volume G1: Reference Architecture IIC:PUB:G1:V1.80:20170131"@en ;
  sto:hasOpenResource <https://www.iiconsortium.org/IIC_PUB_G1_V1.80_2017-01-31.pdf> ;
.
sto:IIRA
  a owl:NamedIndividual ;
  a sto:ArchitectureDescription ;
  a sto:StandardizationFramework ;
  rdfs:comment "The IIRA addresses the need for a common architecture framework to develop interoperable IIoT systems for diverse applications across a broad spectrum of industrial verticals in the public and private sectors to achieve the true promise of IIoT."@en ;
  rdfs:label "Industrial Internet Reference Architecture"@en ;
  skos:altLabel "IIRA" ;
  skos:note "Publications referred: 1. The Industrial Internet of Things Volume G1: Reference Architecture (IIC:PUB:G1:V1.80:20170131)" ;
  sto:hasOfficialResource <http://www.iiconsortium.org/IIRA.htm> ;
  sto:hasPublisher sto:IIC ;
  sto:hasTargetConcern <http://purl.oclc.org/NET/mvco.owl#EndUser> ;
  sto:hasTargetConcern sto:BusinessValue ;
  sto:hasTargetConcern sto:DecisionMaker ;
  sto:hasTargetConcern sto:Developer ;
  sto:hasTargetConcern sto:MaintenanceCost ;
  sto:hasTargetConcern sto:ProductLiability ;
  sto:hasTargetConcern sto:ProductManager ;
  sto:hasTargetConcern sto:ReturnOnInvestment ;
  sto:hasTargetConcern sto:SystemEngineer ;
  sto:hasTargetConcern sto:SystemOperator ;
  sto:hasTargetConcern <https://www.wikidata.org/wiki/Q1548249> ;
.
sto:IIRAApplicationDomain
  a owl:NamedIndividual ;
  a sto:IIRAFunctionalDomain ;
  a sto:StandardClassification ;
  dul:associatedWith sto:BdvaCloudAndHighPerformanceComputing ;
  dul:associatedWith sto:EdgecrossItSystemsLayer ;
  dul:associatedWith sto:FiwareAdvancedUi ;
  dul:associatedWith sto:FiwareCloudHosting ;
  dul:associatedWith sto:IDSRAMProcessLayer ;
  dul:associatedWith sto:RAMIFunctionalLayer ;
  dul:associatedWith sto:RAMIInformationLayer ;
  dul:isPartOf sto:IIRAFunctionalViewpoint ;
  rdfs:label "IIRA Application Domain"@en ;
  skos:note "Publications referred: 'IIC:PUB:G1:V1.80:20170131' '6.4 THE APPLICATION DOMAIN' 'Page 34' " ;
  sto:alignsWith sto:BdvaCloudAndHighPerformanceComputing ;
  sto:alignsWith sto:EdgecrossItSystemsLayer ;
  sto:alignsWith sto:FiwareAdvancedUi ;
  sto:alignsWith sto:FiwareCloudHosting ;
  sto:alignsWith sto:IDSRAMProcessLayer ;
  sto:alignsWith sto:RAMIFunctionalLayer ;
  sto:alignsWith sto:RAMIInformationLayer ;
  sto:frames sto:BdvaDataViualisationAndUserInteraction ;
  sto:frames sto:DataProcessing ;
  sto:frames sto:EndpointInvocation ;
  sto:frames sto:Interoperability ;
  sto:frames sto:SyntacticInteroperability ;
  sto:isDescribedin sto:IIRA ;
.
sto:IIRAApplicationDomainAnno
  a <https://www.w3.org/ns/oaAnnotation> ;
  <https://www.w3.org/ns/oahasBody> sto:IIRAApplicationDomain ;
  <https://www.w3.org/ns/oahasTarget> [
      a <https://www.w3.org/ns/oaSpecificResource> ;
      terms:format "pdf" ;
      <https://www.w3.org/ns/oahasSelector> [
          a <https://www.w3.org/ns/oaRangeSelector> ;
          <https://www.w3.org/ns/oahasEndSelector> [
              a <https://www.w3.org/ns/oaXPathSelector> ;
              rdf:value "Page 35" ;
            ] ;
          <https://www.w3.org/ns/oahasStartSelector> [
              a <https://www.w3.org/ns/oaXPathSelector> ;
              rdf:value "Page 34" ;
            ] ;
        ] ;
      <https://www.w3.org/ns/oahasSource> sto:The_Industrial_Internet_of_Things_Volume_G1_Reference_Architecture ;
    ] ;
.
sto:IIRABusinessDomain
  a owl:NamedIndividual ;
  a sto:IIRAFunctionalDomain ;
  a sto:StandardClassification ;
  dul:associatedWith sto:IDSRAMBusinessLayer ;
  dul:associatedWith sto:OceanSystemViewpoint ;
  dul:associatedWith sto:RAMIBusinessLayer ;
  dul:isPartOf sto:IIRAFunctionalViewpoint ;
  rdfs:label "IIRA Business Domain"@en ;
  skos:note "Publications referred: 'IIC:PUB:G1:V1.80:20170131' '6.5 THE BUSINESS DOMAIN' 'Page 34' " ;
  sto:alignsWith sto:IDSRAMBusinessLayer ;
  sto:alignsWith sto:OceanSystemViewpoint ;
  sto:alignsWith sto:RAMIBusinessLayer ;
  sto:frames rami:ProcessPlanning ;
  sto:isDescribedin sto:IIRA ;
.
sto:IIRABusinessDomainAnno
  a <https://www.w3.org/ns/oaAnnotation> ;
  <https://www.w3.org/ns/oahasBody> sto:IIRABusinessDomain ;
  <https://www.w3.org/ns/oahasTarget> [
      a <https://www.w3.org/ns/oaSpecificResource> ;
      terms:format "pdf" ;
      <https://www.w3.org/ns/oahasSelector> [
          a <https://www.w3.org/ns/oaRangeSelector> ;
          <https://www.w3.org/ns/oahasEndSelector> [
              a <https://www.w3.org/ns/oaXPathSelector> ;
              rdf:value "Page 35" ;
            ] ;
          <https://www.w3.org/ns/oahasStartSelector> [
              a <https://www.w3.org/ns/oaXPathSelector> ;
              rdf:value "Page 34" ;
            ] ;
        ] ;
      <https://www.w3.org/ns/oahasSource> sto:The_Industrial_Internet_of_Things_Volume_G1_Reference_Architecture ;
    ] ;
.
sto:IIRABusinessViewpoint
  a owl:NamedIndividual ;
  a sto:StandardClassification ;
  a sto:Viewpoint ;
  terms:creator sto:sebastian ;
  dul:associatedWith sto:IviBusinessLayer ;
  dul:associatedWith sto:OceanBusinessViewpoint ;
  dul:associatedWith sto:OceanMarketplaceViewpoint ;
  rdfs:comment "The business viewpoint frames economic aspects and business relations regarded by the IIC Reference Architecture."@en ;
  rdfs:label "IIRA Business Viewpoint"@en ;
  skos:note "Publications referred: '(IIC:PUB:G1:V1.80:20170131' '3.5.1 BUSINESS VIEWPOINT' 'Page 15' " ;
  sto:alignsWith sto:IviBusinessLayer ;
  sto:alignsWith sto:OceanBusinessViewpoint ;
  sto:alignsWith sto:OceanMarketplaceViewpoint ;
  sto:frames sto:BusinessContext ;
  sto:frames sto:BusinessValue ;
  sto:frames sto:MaintenanceCost ;
  sto:frames sto:ProductLiability ;
  sto:frames sto:Resilience ;
  sto:frames sto:ReturnOnInvestment ;
  sto:frames sto:Safety ;
  sto:frames sto:Security ;
  sto:frames sto:Trustworthiness ;
  sto:isDescribedin sto:IIRA ;
.
sto:IIRABusinessViewpointAnno
  a <https://www.w3.org/ns/oaAnnotation> ;
  <https://www.w3.org/ns/oahasBody> sto:IIRABusinessViewpoint ;
  <https://www.w3.org/ns/oahasTarget> [
      a <https://www.w3.org/ns/oaSpecificResource> ;
      terms:format "pdf" ;
      <https://www.w3.org/ns/oahasSelector> [
          a <https://www.w3.org/ns/oaRangeSelector> ;
          <https://www.w3.org/ns/oahasEndSelector> [
              a <https://www.w3.org/ns/oaXPathSelector> ;
              rdf:value "Page 22" ;
            ] ;
          <https://www.w3.org/ns/oahasStartSelector> [
              a <https://www.w3.org/ns/oaXPathSelector> ;
              rdf:value "Page 20" ;
            ] ;
        ] ;
      <https://www.w3.org/ns/oahasSource> sto:The_Industrial_Internet_of_Things_Volume_G1_Reference_Architecture ;
    ] ;
.
sto:IIRAConnectivity
  a owl:NamedIndividual ;
  a sto:IIRACrosscuttingFunction ;
  a sto:StandardClassification ;
  dul:associatedWith sto:BdvaDataProcessingArchitectures ;
  dul:associatedWith sto:DecisionMaker ;
  dul:associatedWith sto:DtpSystemView ;
  dul:associatedWith sto:FiwareApplicationsServicesAndDataDelivery ;
  dul:associatedWith sto:IEC_62541 ;
  dul:associatedWith sto:IICF ;
  dul:associatedWith sto:IotaEvolutionInteroperability ;
  dul:associatedWith sto:LinkLayer ;
  dul:associatedWith sto:NgsiLdApiOperation ;
  dul:associatedWith sto:RAMICommunicationlayer ;
  dul:associatedWith sto:REST ;
  dul:associatedWith sto:oneM2M ;
  dul:associatedWith <https://www.wikidata.org/wiki/Q1548249> ;
  dul:isPartOf sto:IIRAFunctionalViewpoint ;
  rdfs:label "IIRA Connectivity"@en ;
  sto:alignsWith sto:BdvaDataProcessingArchitectures ;
  sto:alignsWith sto:DtpSystemView ;
  sto:alignsWith sto:FiwareApplicationsServicesAndDataDelivery ;
  sto:alignsWith sto:IotaEvolutionInteroperability ;
  sto:alignsWith sto:NgsiLdApiOperation ;
  sto:alignsWith sto:RAMICommunicationlayer ;
  sto:frames sto:Authentication ;
  sto:frames sto:CardinalityOfDataSources ;
  sto:frames sto:CardinalityOfParticipants ;
  sto:frames sto:Communication ;
  sto:frames sto:DataAccess ;
  sto:frames sto:DataDiscovery ;
  sto:frames sto:DynamicAdjustability ;
  sto:frames sto:EndpointInvocation ;
  sto:frames sto:Evolvability ;
  sto:frames sto:Governance ;
  sto:frames sto:IPv4Support ;
  sto:frames sto:IPv6Support ;
  sto:frames sto:Identification ;
  sto:frames sto:IdentityManagement ;
  sto:frames sto:IntegrityProtection ;
  sto:frames sto:Interoperability ;
  sto:frames sto:Multilaterism ;
  sto:frames sto:NetworkPerformance ;
  sto:frames sto:QualityOfService ;
  sto:frames sto:Reliability ;
  sto:frames sto:Resilience ;
  sto:frames sto:Safety ;
  sto:frames sto:Scalability ;
  sto:frames sto:SecureCommunication ;
  sto:frames sto:Security ;
  sto:frames sto:SemanticInteroperability ;
  sto:frames sto:ServiceChoreography ;
  sto:frames sto:ServiceComposition ;
  sto:frames sto:ServiceDeployment ;
  sto:frames sto:ServiceDescription ;
  sto:frames sto:ServiceDiscovery ;
  sto:frames sto:ServiceLifecycleManagement ;
  sto:frames sto:ServiceOrchestration ;
  sto:frames sto:SyntacticInteroperability ;
  sto:frames sto:TimeSynchronization ;
  sto:frames sto:Trustworthiness ;
  sto:frames sto:Unicast ;
  sto:isDescribedin sto:IIRA ;
.
sto:IIRAConnectivityAnno
  a <https://www.w3.org/ns/oaAnnotation> ;
  <https://www.w3.org/ns/oahasBody> sto:IIRAConnectivity ;
  <https://www.w3.org/ns/oahasTarget> [
      a <https://www.w3.org/ns/oaSpecificResource> ;
      terms:format "pdf" ;
      <https://www.w3.org/ns/oahasSelector> [
          a <https://www.w3.org/ns/oaRangeSelector> ;
          <https://www.w3.org/ns/oahasEndSelector> [
              a <https://www.w3.org/ns/oaXPathSelector> ;
              rdf:value "Page 127" ;
            ] ;
          <https://www.w3.org/ns/oahasStartSelector> [
              a <https://www.w3.org/ns/oaXPathSelector> ;
              rdf:value "Page 8" ;
            ] ;
        ] ;
      <https://www.w3.org/ns/oahasSource> sto:The_Industrial_Internet_of_Things_Volume_G5_Connectivity_Framework ;
    ] ;
.
sto:IIRAControlDomain
  a owl:NamedIndividual ;
  a sto:IIRAFunctionalDomain ;
  a sto:StandardClassification ;
  dul:associatedWith sto:EdgecrossEdgeComputingLayer ;
  dul:associatedWith sto:FiwareIotServicesEnablement ;
  dul:associatedWith sto:IDSRAMSystemLayer ;
  dul:associatedWith sto:IotaInformationViewpoint ;
  dul:associatedWith sto:NgsiLdApiOperation ;
  dul:associatedWith sto:RAMIIntegrationLayer ;
  dul:associatedWith sto:xRoadProtocolsInterfaces ;
  dul:isPartOf sto:IIRAFunctionalViewpoint ;
  rdfs:label "IIRA Control Domain"@en ;
  skos:note "Publications referred: 'IIC:PUB:G1:V1.80:20170131' '6.1 THE CONTROL DOMAIN' 'Page 27' " ;
  sto:alignsWith sto:EdgecrossEdgeComputingLayer ;
  sto:alignsWith sto:FiwareIotServicesEnablement ;
  sto:alignsWith sto:IDSRAMSystemLayer ;
  sto:alignsWith sto:IotaInformationViewpoint ;
  sto:alignsWith sto:NgsiLdApiOperation ;
  sto:alignsWith sto:RAMIIntegrationLayer ;
  sto:alignsWith sto:xRoadProtocolsInterfaces ;
  sto:frames sto:Actuation ;
  sto:frames sto:AssetManagement ;
  sto:frames sto:Communication ;
  sto:frames sto:EdgeAnalytics ;
  sto:frames sto:IoT ;
  sto:frames sto:Sensing ;
  sto:frames sto:VirtualEntity ;
  sto:isDescribedin sto:IIRA ;
.
sto:IIRAControlDomainAnno
  a <https://www.w3.org/ns/oaAnnotation> ;
  <https://www.w3.org/ns/oahasBody> sto:IIRAControlDomain ;
  <https://www.w3.org/ns/oahasTarget> [
      a <https://www.w3.org/ns/oaSpecificResource> ;
      terms:format "pdf" ;
      <https://www.w3.org/ns/oahasSelector> [
          a <https://www.w3.org/ns/oaRangeSelector> ;
          <https://www.w3.org/ns/oahasEndSelector> [
              a <https://www.w3.org/ns/oaXPathSelector> ;
              rdf:value "Page 30" ;
            ] ;
          <https://www.w3.org/ns/oahasStartSelector> [
              a <https://www.w3.org/ns/oaXPathSelector> ;
              rdf:value "Page 27" ;
            ] ;
        ] ;
      <https://www.w3.org/ns/oahasSource> sto:The_Industrial_Internet_of_Things_Volume_G1_Reference_Architecture ;
    ] ;
.
sto:IIRACrosscuttingFunction
  a owl:Class ;
  a owl:NamedIndividual ;
  terms:creator sto:sebastian ;
  terms:creator "sebastian"@en ;
  rdfs:comment "Often these enabling functions, the so-called crosscutting functions, need to be made available across many of the system functional components. For Reference Architecture 6: Functional Viewpoint example, system functions need to be connected so they can interact with each other to complete functionality at the system level."@en ;
  rdfs:label "IIRA Crosscutting Function"@en ;
  rdfs:subClassOf sto:StandardClassification ;
  rdfs:subClassOf [
      a owl:Restriction ;
      owl:hasValue sto:IIRAFunctionalViewpoint ;
      owl:onProperty dul:isPartOf ;
    ] ;
  skos:note "Publications referred: 'IIC:PUB:G1:V1.80:20170131' '6.6 CROSSCUTTING FUNCTIONS AND SYSTEM CHARACTERISTICS' 'Page 34' " ;
.
sto:IIRACrosscuttingFunctionAnno
  a <https://www.w3.org/ns/oaAnnotation> ;
  <https://www.w3.org/ns/oahasBody> sto:IIRACrosscuttingFunction ;
  <https://www.w3.org/ns/oahasTarget> [
      a <https://www.w3.org/ns/oaSpecificResource> ;
      terms:format "pdf" ;
      <https://www.w3.org/ns/oahasSelector> [
          a <https://www.w3.org/ns/oaRangeSelector> ;
          <https://www.w3.org/ns/oahasEndSelector> [
              a <https://www.w3.org/ns/oaXPathSelector> ;
              rdf:value "Page 36" ;
            ] ;
          <https://www.w3.org/ns/oahasStartSelector> [
              a <https://www.w3.org/ns/oaXPathSelector> ;
              rdf:value "Page 34" ;
            ] ;
        ] ;
      <https://www.w3.org/ns/oahasSource> sto:The_Industrial_Internet_of_Things_Volume_G1_Reference_Architecture ;
    ] ;
.
sto:IIRADistributedDataManagement
  a owl:NamedIndividual ;
  a sto:IIRACrosscuttingFunction ;
  a sto:StandardClassification ;
  terms:creator sto:sebastian ;
  dul:associatedWith sto:FiwareCloudHosting ;
  dul:associatedWith sto:RAMICommunicationlayer ;
  dul:isPartOf sto:IIRAFunctionalViewpoint ;
  rdfs:label "IIRA Distributed Data Management"@en ;
  sto:alignsWith sto:FiwareCloudHosting ;
  sto:alignsWith sto:RAMICommunicationlayer ;
  sto:frames sto:Interoperability ;
  sto:frames sto:SemanticInteroperability ;
  sto:isDescribedin sto:IIRA ;
.
sto:IIRAFunctionalDomain
  a owl:Class ;
  rdfs:label "IIRA Functional Domain"@en ;
  rdfs:subClassOf sto:StandardClassification ;
  rdfs:subClassOf [
      a owl:Restriction ;
      owl:hasValue sto:IIRA ;
      owl:onProperty sto:isDescribedin ;
    ] ;
  rdfs:subClassOf [
      a owl:Restriction ;
      owl:hasValue sto:IIRAFunctionalViewpoint ;
      owl:onProperty dul:isPartOf ;
    ] ;
.
sto:IIRAFunctionalViewpoint
  a owl:NamedIndividual ;
  a sto:StandardClassification ;
  a sto:Viewpoint ;
  terms:creator sto:sebastian ;
  terms:creator "The IIRA Functional Viewpoint contains the IIRA Domains in order to describe technical relations and communications between the several dimensions of IoT devices."@en ;
  terms:creator "sebastian"@en ;
  dul:associatedWith sto:IDSRAMReferenceArchitectureModel ;
  dul:associatedWith sto:IotaFunctionalViewpoint ;
  dul:associatedWith sto:OceanSystemViewpoint ;
  rdfs:comment "The IIRA Functional Viewpoint contains the IIRA Domains in order to describe technical relations and communications between the several dimensions of IoT devices."@en ;
  rdfs:label "IIRA Functional Viewpoint"@en ;
  skos:note "Publications referred: '(IIC:PUB:G1:V1.80:20170131' '3.5.3 FUNCTIONAL VIEWPOINT' 'Page 16' " ;
  sto:alignsWith sto:IDSRAMReferenceArchitectureModel ;
  sto:alignsWith sto:IotaFunctionalViewpoint ;
  sto:alignsWith sto:OceanSystemViewpoint ;
  sto:frames rami:ProcessPlanning ;
  sto:frames sto:AccessPolicy ;
  sto:frames sto:Actuation ;
  sto:frames sto:Authentication ;
  sto:frames sto:Authorization ;
  sto:frames sto:Availability ;
  sto:frames sto:BdvaDataViualisationAndUserInteraction ;
  sto:frames sto:CardinalityOfDataSources ;
  sto:frames sto:CardinalityOfParticipants ;
  sto:frames sto:CloudComputing ;
  sto:frames sto:Communication ;
  sto:frames sto:DataAccess ;
  sto:frames sto:DataAccessControl ;
  sto:frames sto:DataAnalytics ;
  sto:frames sto:DataAtRest ;
  sto:frames sto:DataDiscovery ;
  sto:frames sto:DataInMotion ;
  sto:frames sto:DataProcessing ;
  sto:frames sto:DataProtection ;
  sto:frames sto:DataSovereignty ;
  sto:frames sto:DynamicAdjustability ;
  sto:frames sto:EndpointInvocation ;
  sto:frames sto:Evolvability ;
  sto:frames sto:Governance ;
  sto:frames sto:IPv4Support ;
  sto:frames sto:IPv6Support ;
  sto:frames sto:Identification ;
  sto:frames sto:IdentityManagement ;
  sto:frames sto:IntegrityProtection ;
  sto:frames sto:Interoperability ;
  sto:frames sto:IoT ;
  sto:frames sto:Multilaterism ;
  sto:frames sto:NetworkPerformance ;
  sto:frames sto:Privacy ;
  sto:frames sto:QualityOfService ;
  sto:frames sto:RealTimeAnalytics ;
  sto:frames sto:Reliability ;
  sto:frames sto:Resilience ;
  sto:frames sto:Safety ;
  sto:frames sto:Scalability ;
  sto:frames sto:SecureCommunication ;
  sto:frames sto:Security ;
  sto:frames sto:SecurityConfiguration ;
  sto:frames sto:SemanticInteroperability ;
  sto:frames sto:Sensing ;
  sto:frames sto:ServiceAccessControl ;
  sto:frames sto:ServiceChoreography ;
  sto:frames sto:ServiceComposition ;
  sto:frames sto:ServiceDeployment ;
  sto:frames sto:ServiceDescription ;
  sto:frames sto:ServiceDiscovery ;
  sto:frames sto:ServiceIsolation ;
  sto:frames sto:ServiceLevelAgreements ;
  sto:frames sto:ServiceLifecycleManagement ;
  sto:frames sto:ServiceOrchestration ;
  sto:frames sto:StreamProcessing ;
  sto:frames sto:SyntacticInteroperability ;
  sto:frames sto:TimeSynchronization ;
  sto:frames sto:Trustworthiness ;
  sto:frames sto:Unicast ;
  sto:isDescribedin sto:IIRA ;
.
sto:IIRAFunctionalViewpointAnno
  a <https://www.w3.org/ns/oaAnnotation> ;
  <https://www.w3.org/ns/oahasBody> sto:IIRAFunctionalViewpoint ;
  <https://www.w3.org/ns/oahasTarget> [
      a <https://www.w3.org/ns/oaSpecificResource> ;
      terms:format "pdf" ;
      <https://www.w3.org/ns/oahasSelector> [
          a <https://www.w3.org/ns/oaRangeSelector> ;
          <https://www.w3.org/ns/oahasEndSelector> [
              a <https://www.w3.org/ns/oaXPathSelector> ;
              rdf:value "Page 38" ;
            ] ;
          <https://www.w3.org/ns/oahasStartSelector> [
              a <https://www.w3.org/ns/oaXPathSelector> ;
              rdf:value "Page 25" ;
            ] ;
        ] ;
      <https://www.w3.org/ns/oahasSource> sto:The_Industrial_Internet_of_Things_Volume_G1_Reference_Architecture ;
    ] ;
.
sto:IIRAImplementationViewpoint
  a owl:NamedIndividual ;
  a sto:StandardClassification ;
  a sto:Viewpoint ;
  dul:associatedWith sto:ControlDomain ;
  dul:associatedWith sto:DtpDeploymentView ;
  dul:associatedWith sto:FIWARE ;
  dul:associatedWith sto:IDSRAMSystemLayer ;
  dul:associatedWith sto:IIRAApplicationDomain ;
  dul:associatedWith sto:IIRABusinessDomain ;
  dul:associatedWith sto:IIRAOperationsDomain ;
  dul:associatedWith sto:InformationDomain ;
  dul:associatedWith sto:IotaDeploymentOperationViewpoint ;
  dul:associatedWith sto:NgsiLdArchitecture ;
  dul:associatedWith sto:xRoadDeploymentView ;
  rdfs:label "IIRA Implementation Viewpoint"@en ;
  skos:note "Publications referred: '(IIC:PUB:G1:V1.80:20170131' '3.5.4 IMPLEMENTATION VIEWPOINT' 'Page 16' " ;
  sto:alignsWith sto:DtpDeploymentView ;
  sto:alignsWith sto:FIWARE ;
  sto:alignsWith sto:IotaDeploymentOperationViewpoint ;
  sto:alignsWith sto:NgsiLdArchitecture ;
  sto:alignsWith sto:xRoadDeploymentView ;
  sto:frames sto:CloudComputing ;
  sto:frames sto:Communication ;
  sto:frames sto:DataProcessing ;
  sto:frames sto:EdgeComputing ;
  sto:frames sto:EndpointDescription ;
  sto:frames sto:Interoperability ;
  sto:frames sto:SemanticInteroperability ;
  sto:isDescribedin sto:IIRA ;
.
sto:IIRAImplementationViewpointAnno
  a <https://www.w3.org/ns/oaAnnotation> ;
  <https://www.w3.org/ns/oahasBody> sto:IIRAImplementationViewpoint ;
  <https://www.w3.org/ns/oahasTarget> [
      a <https://www.w3.org/ns/oaSpecificResource> ;
      terms:format "pdf" ;
      <https://www.w3.org/ns/oahasSelector> [
          a <https://www.w3.org/ns/oaRangeSelector> ;
          <https://www.w3.org/ns/oahasEndSelector> [
              a <https://www.w3.org/ns/oaXPathSelector> ;
              rdf:value "Page 47" ;
            ] ;
          <https://www.w3.org/ns/oahasStartSelector> [
              a <https://www.w3.org/ns/oaXPathSelector> ;
              rdf:value "Page 38" ;
            ] ;
        ] ;
      <https://www.w3.org/ns/oahasSource> sto:The_Industrial_Internet_of_Things_Volume_G1_Reference_Architecture ;
    ] ;
.
sto:IIRAIndustrialAnalytics
  a owl:NamedIndividual ;
  a sto:IIRACrosscuttingFunction ;
  a sto:StandardClassification ;
  dul:isPartOf sto:IIRAFunctionalViewpoint ;
  sto:isDescribedin sto:IIRA ;
.
sto:IIRAInformationDomain
  a owl:NamedIndividual ;
  a sto:IIRAFunctionalDomain ;
  a sto:StandardClassification ;
  dul:associatedWith sto:BdvaDataAnalytics ;
  dul:associatedWith sto:BdvaDataProcessingArchitectures ;
  dul:associatedWith sto:DtpSystemView ;
  dul:associatedWith sto:EdgecrossEdgeComputingLayer ;
  dul:associatedWith sto:IDSRAMInformationLayer ;
  dul:associatedWith sto:IDSRAMProcessLayer ;
  dul:associatedWith sto:IotaInformationViewpoint ;
  dul:associatedWith sto:NgsiLdInformationModel ;
  dul:associatedWith sto:RAMIInformationLayer ;
  dul:isPartOf sto:IIRAFunctionalViewpoint ;
  rdfs:label "IIRA Information Domain"@en ;
  skos:note "Publications referred: 'IIC:PUB:G1:V1.80:20170131' '6.3 THE INFORMATION DOMAIN' 'Page 32' " ;
  sto:alignsWith sto:BdvaDataAnalytics ;
  sto:alignsWith sto:BdvaDataProcessingArchitectures ;
  sto:alignsWith sto:DtpSystemView ;
  sto:alignsWith sto:EdgecrossEdgeComputingLayer ;
  sto:alignsWith sto:IDSRAMInformationLayer ;
  sto:alignsWith sto:IDSRAMProcessLayer ;
  sto:alignsWith sto:IotaInformationViewpoint ;
  sto:alignsWith sto:NgsiLdInformationModel ;
  sto:alignsWith sto:RAMIInformationLayer ;
  sto:frames sto:DataAnalytics ;
  sto:frames sto:DataProcessing ;
  sto:frames sto:Interoperability ;
  sto:frames sto:SemanticInteroperability ;
  sto:frames sto:StreamProcessing ;
  sto:frames sto:SyntacticInteroperability ;
  sto:isDescribedin sto:IIRA ;
.
sto:IIRAInformationDomainAnno
  a <https://www.w3.org/ns/oaAnnotation> ;
  <https://www.w3.org/ns/oahasBody> sto:IIRAInformationDomain ;
  <https://www.w3.org/ns/oahasTarget> [
      a <https://www.w3.org/ns/oaSpecificResource> ;
      terms:format "pdf" ;
      <https://www.w3.org/ns/oahasSelector> [
          a <https://www.w3.org/ns/oaRangeSelector> ;
          <https://www.w3.org/ns/oahasEndSelector> [
              a <https://www.w3.org/ns/oaXPathSelector> ;
              rdf:value "Page 34" ;
            ] ;
          <https://www.w3.org/ns/oahasStartSelector> [
              a <https://www.w3.org/ns/oaXPathSelector> ;
              rdf:value "Page 32" ;
            ] ;
        ] ;
      <https://www.w3.org/ns/oahasSource> sto:The_Industrial_Internet_of_Things_Volume_G1_Reference_Architecture ;
    ] ;
.
sto:IIRAIntelligentAndResilientControl
  a owl:NamedIndividual ;
  a sto:IIRACrosscuttingFunction ;
  a sto:StandardClassification ;
  dul:isPartOf sto:IIRAFunctionalViewpoint ;
  rdfs:comment """There is a renewed movement to distribute computational capability toward the network peripheries, away from concentrated computation centers, to benefit from a reduction in movement of data and communication latency, and enhancement in local intelligent control and, more importantly, resilience.
source: Industrial Internet Reference Archietcture"""@en ;
  rdfs:label "IIRA Intelligent and Resilient Control"@en ;
  sto:isDescribedin sto:IIRA ;
.
sto:IIRAOperationsDomain
  a owl:NamedIndividual ;
  a sto:IIRAFunctionalDomain ;
  a sto:StandardClassification ;
  dul:associatedWith sto:DtpSystemView ;
  dul:associatedWith sto:EdgecrossEdgeComputingLayer ;
  dul:associatedWith sto:IDSRAMProcessLayer ;
  dul:associatedWith sto:IotaInformationViewpoint ;
  dul:associatedWith sto:IviActivityView ;
  dul:associatedWith sto:RAMIFunctionalLayer ;
  dul:isPartOf sto:IIRAFunctionalViewpoint ;
  rdfs:label "IIRA Operation Domain"@en ;
  skos:note "Publications referred: 'IIC:PUB:G1:V1.80:20170131' '6.2 THE OPERATIONS DOMAIN' 'Page 30' " ;
  sto:alignsWith sto:DtpSystemView ;
  sto:alignsWith sto:EdgecrossEdgeComputingLayer ;
  sto:alignsWith sto:IDSRAMProcessLayer ;
  sto:alignsWith sto:IotaInformationViewpoint ;
  sto:alignsWith sto:IviActivityView ;
  sto:alignsWith sto:RAMIFunctionalLayer ;
  sto:frames sto:DataAnalytics ;
  sto:frames sto:RealTimeAnalytics ;
  sto:frames sto:ServiceDeployment ;
  sto:frames sto:ServiceLifecycleManagement ;
  sto:isDescribedin sto:IIRA ;
.
sto:IIRAOperationsDomainAnno
  a <https://www.w3.org/ns/oaAnnotation> ;
  <https://www.w3.org/ns/oahasBody> sto:IIRAOperationsDomain ;
  <https://www.w3.org/ns/oahasTarget> [
      a <https://www.w3.org/ns/oaSpecificResource> ;
      terms:format "pdf" ;
      <https://www.w3.org/ns/oahasSelector> [
          a <https://www.w3.org/ns/oaRangeSelector> ;
          <https://www.w3.org/ns/oahasEndSelector> [
              a <https://www.w3.org/ns/oaXPathSelector> ;
              rdf:value "Page 32" ;
            ] ;
          <https://www.w3.org/ns/oahasStartSelector> [
              a <https://www.w3.org/ns/oaXPathSelector> ;
              rdf:value "Page 30" ;
            ] ;
        ] ;
      <https://www.w3.org/ns/oahasSource> sto:The_Industrial_Internet_of_Things_Volume_G1_Reference_Architecture ;
    ] ;
.
sto:IIRAPhysicalSystems
  a owl:NamedIndividual ;
  a sto:StandardClassification ;
  terms:creator sto:sebastian ;
  terms:creator "sebastian" ;
  dul:associatedWith sto:EdgecrossFacilityLayer ;
  dul:associatedWith sto:IDSRAMSystemLayer ;
  dul:associatedWith sto:IviAssetView ;
  dul:associatedWith sto:RAMIAssetlayer ;
  dul:isPartOf sto:IIRAFunctionalViewpoint ;
  rdfs:comment "Computational capabilities ranging from very limited (e.g. in a smart sensor) to reasonably rich (e.g. a cluster of servers) are placed in, attached to or collocated with physical systems (e.g. in smart sensors, devices or machines). These capabilities are connected through a variety of connectivity technologies including wireless."@en ;
  rdfs:label "IIRA Physical Systems"@en ;
  sto:alignsWith sto:EdgecrossFacilityLayer ;
  sto:alignsWith sto:IDSRAMSystemLayer ;
  sto:alignsWith sto:IviAssetView ;
  sto:alignsWith sto:RAMIAssetlayer ;
  sto:hasOfficialResource <https://www.iiconsortium.org/IIRA.htm> ;
  sto:isDescribedin sto:IIRA ;
.
sto:IIRAPrivacy
  a owl:NamedIndividual ;
  a sto:IIRASystemCharacteristics ;
  a sto:StandardClassification ;
  dul:associatedWith sto:DtpSecurityPrivacy ;
  dul:isPartOf sto:IIRAFunctionalViewpoint ;
  rdfs:label "IIRA Privacy"@en ;
  sto:alignsWith sto:DtpSecurityPrivacy ;
  sto:frames sto:DataSovereignty ;
  sto:frames sto:Privacy ;
  sto:frames sto:Trustworthiness ;
  sto:isDescribedin sto:IIRA ;
.
sto:IIRAReliability
  a owl:NamedIndividual ;
  a sto:IIRASystemCharacteristics ;
  a sto:StandardClassification ;
  dul:isPartOf sto:IIRAFunctionalViewpoint ;
  rdfs:label "IIRA Reliability"@en ;
  skos:note "Publications referred: '<https://www.iiconsortium.org/pdf/IIC_PUB_G4_V1.00_PB-3.pdf IIC:PUB:G4:V1.0:PB:20160926>' '3.4 RELIABILITY' 'Page 18'" ;
  sto:frames sto:Reliability ;
  sto:frames sto:Trustworthiness ;
  sto:isDescribedin sto:IIRA ;
.
sto:IIRAReliabilityAnno
  a <https://www.w3.org/ns/oaAnnotation> ;
  <https://www.w3.org/ns/oahasBody> sto:IIRAReliability ;
  <https://www.w3.org/ns/oahasTarget> [
      a <https://www.w3.org/ns/oaSpecificResource> ;
      terms:format "pdf" ;
      <https://www.w3.org/ns/oahasSelector> [
          a <https://www.w3.org/ns/oaRangeSelector> ;
          <https://www.w3.org/ns/oahasEndSelector> [
              a <https://www.w3.org/ns/oaXPathSelector> ;
              rdf:value "Page 19" ;
            ] ;
          <https://www.w3.org/ns/oahasStartSelector> [
              a <https://www.w3.org/ns/oaXPathSelector> ;
              rdf:value "Page 18" ;
            ] ;
        ] ;
      <https://www.w3.org/ns/oahasSource> sto:Industrial_Internet_of_Things_Volume_G4_Security_Framework ;
    ] ;
.
sto:IIRAResilience
  a owl:NamedIndividual ;
  a sto:IIRASystemCharacteristics ;
  a sto:StandardClassification ;
  dul:isPartOf sto:IIRAFunctionalViewpoint ;
  rdfs:label "IIRA Resilience"@en ;
  sto:isDescribedin sto:IIRA ;
.
sto:IIRAResilienceAnno
  a <https://www.w3.org/ns/oaAnnotation> ;
  <https://www.w3.org/ns/oahasBody> sto:IIRAResilience ;
  <https://www.w3.org/ns/oahasTarget> [
      a <https://www.w3.org/ns/oaSpecificResource> ;
      terms:format "pdf" ;
      <https://www.w3.org/ns/oahasSelector> [
          a <https://www.w3.org/ns/oaRangeSelector> ;
          <https://www.w3.org/ns/oahasEndSelector> [
              a <https://www.w3.org/ns/oaXPathSelector> ;
              rdf:value "Page 19" ;
            ] ;
          <https://www.w3.org/ns/oahasStartSelector> [
              a <https://www.w3.org/ns/oaXPathSelector> ;
              rdf:value "Page 18" ;
            ] ;
        ] ;
      <https://www.w3.org/ns/oahasSource> sto:Industrial_Internet_of_Things_Volume_G4_Security_Framework ;
    ] ;
  <https://www.w3.org/ns/oahasTarget> [
      a <https://www.w3.org/ns/oaSpecificResource> ;
      terms:format "pdf" ;
      <https://www.w3.org/ns/oahasSelector> [
          a <https://www.w3.org/ns/oaRangeSelector> ;
          <https://www.w3.org/ns/oahasEndSelector> [
              a <https://www.w3.org/ns/oaXPathSelector> ;
              rdf:value "Page 20" ;
            ] ;
          <https://www.w3.org/ns/oahasStartSelector> [
              a <https://www.w3.org/ns/oaXPathSelector> ;
              rdf:value "Page 19" ;
            ] ;
        ] ;
      <https://www.w3.org/ns/oahasSource> sto:Industrial_Internet_of_Things_Volume_G4_Security_Framework ;
    ] ;
.
sto:IIRASafety
  a owl:NamedIndividual ;
  a sto:IIRASystemCharacteristics ;
  a sto:StandardClassification ;
  dul:isPartOf sto:IIRAFunctionalViewpoint ;
  rdfs:label "IIRA Safety"@en ;
  sto:isDescribedin sto:IIRA ;
.
sto:IIRASafetyAnno
  a <https://www.w3.org/ns/oaAnnotation> ;
  <https://www.w3.org/ns/oahasBody> sto:IIRASafety ;
  <https://www.w3.org/ns/oahasTarget> [
      a <https://www.w3.org/ns/oaSpecificResource> ;
      terms:format "pdf" ;
      <https://www.w3.org/ns/oahasSelector> [
          a <https://www.w3.org/ns/oaRangeSelector> ;
          <https://www.w3.org/ns/oahasEndSelector> [
              a <https://www.w3.org/ns/oaXPathSelector> ;
              rdf:value "Page 18" ;
            ] ;
          <https://www.w3.org/ns/oahasStartSelector> [
              a <https://www.w3.org/ns/oaXPathSelector> ;
              rdf:value "Page 17" ;
            ] ;
        ] ;
      <https://www.w3.org/ns/oahasSource> sto:Industrial_Internet_of_Things_Volume_G4_Security_Framework ;
    ] ;
.
sto:IIRAScalability
  a owl:NamedIndividual ;
  a sto:IIRASystemCharacteristics ;
  a sto:StandardClassification ;
  dul:associatedWith sto:FiwareCloudHosting ;
  dul:isPartOf sto:IIRAFunctionalViewpoint ;
  rdfs:label "IIRA Scalability"@en ;
  sto:alignsWith sto:FiwareCloudHosting ;
  sto:frames sto:Scalability ;
  sto:isDescribedin sto:IIRA ;
.
sto:IIRASecurity
  a owl:NamedIndividual ;
  a sto:IIRASystemCharacteristics ;
  a sto:StandardClassification ;
  terms:creator sto:sebastian ;
  dul:associatedWith sto:DataOwner ;
  dul:associatedWith sto:DecisionMaker ;
  dul:associatedWith sto:DtpSecurityPrivacy ;
  dul:associatedWith sto:FiwareSecurity ;
  dul:associatedWith sto:IDSRAMSecurity ;
  dul:associatedWith sto:IotaAvailabilityResilience ;
  dul:associatedWith sto:IotaTrustSecurityPrivacy ;
  dul:associatedWith <https://www.wikidata.org/wiki/Q1548249> ;
  dul:isPartOf sto:IIRAFunctionalViewpoint ;
  rdfs:label "IIRA Security"@en ;
  sto:alignsWith sto:DtpSecurityPrivacy ;
  sto:alignsWith sto:FiwareSecurity ;
  sto:alignsWith sto:IDSRAMSecurity ;
  sto:alignsWith sto:IotaAvailabilityResilience ;
  sto:alignsWith sto:IotaTrustSecurityPrivacy ;
  sto:frames sto:AccessPolicy ;
  sto:frames sto:Authorization ;
  sto:frames sto:Availability ;
  sto:frames sto:CloudComputing ;
  sto:frames sto:Communication ;
  sto:frames sto:DataAccessControl ;
  sto:frames sto:DataAtRest ;
  sto:frames sto:DataInMotion ;
  sto:frames sto:DataProcessing ;
  sto:frames sto:DataProtection ;
  sto:frames sto:DataSovereignty ;
  sto:frames sto:Identification ;
  sto:frames sto:IdentityManagement ;
  sto:frames sto:IntegrityProtection ;
  sto:frames sto:Privacy ;
  sto:frames sto:Reliability ;
  sto:frames sto:Resilience ;
  sto:frames sto:Safety ;
  sto:frames sto:SecureCommunication ;
  sto:frames sto:Security ;
  sto:frames sto:SecurityConfiguration ;
  sto:frames sto:ServiceAccessControl ;
  sto:frames sto:ServiceIsolation ;
  sto:frames sto:ServiceLevelAgreements ;
  sto:frames sto:ServiceLifecycleManagement ;
  sto:frames sto:Trustworthiness ;
  sto:isDescribedin sto:IIRA ;
.
sto:IIRASecurityAnno
  a <https://www.w3.org/ns/oaAnnotation> ;
  <https://www.w3.org/ns/oahasBody> sto:IIRASecurity ;
  <https://www.w3.org/ns/oahasTarget> [
      a <https://www.w3.org/ns/oaSpecificResource> ;
      terms:format "pdf" ;
      <https://www.w3.org/ns/oahasSelector> [
          a <https://www.w3.org/ns/oaRangeSelector> ;
          <https://www.w3.org/ns/oahasEndSelector> [
              a <https://www.w3.org/ns/oaXPathSelector> ;
              rdf:value "Page 121" ;
            ] ;
          <https://www.w3.org/ns/oahasStartSelector> [
              a <https://www.w3.org/ns/oaXPathSelector> ;
              rdf:value "Page 11" ;
            ] ;
        ] ;
      <https://www.w3.org/ns/oahasSource> sto:Industrial_Internet_of_Things_Volume_G4_Security_Framework ;
    ] ;
.
sto:IIRASecurityFramework
  a owl:NamedIndividual ;
  a sto:StandardClassification ;
  terms:creator sto:sebastian ;
  dul:associatedWith sto:BdvaCyberSecurityTrust ;
  dul:associatedWith sto:BdvaDataProtection ;
  dul:associatedWith sto:IDSRAMSecurity ;
  dul:associatedWith sto:xRoadSystemComponents ;
  rdfs:label "IIC Security Framework"@en ;
  skos:note "Publications referred: '<https://www.iiconsortium.org/pdf/IIC_PUB_G4_V1.00_PB-3.pdf IIC:PUB:G4:V1.0:PB:20160926>'" ;
  sto:alignsWith sto:BdvaCyberSecurityTrust ;
  sto:alignsWith sto:BdvaDataProtection ;
  sto:alignsWith sto:IDSRAMSecurity ;
  sto:alignsWith sto:xRoadSystemComponents ;
  sto:hasOfficialResource <https://www.iiconsortium.org/IISF.htm> ;
.
sto:IIRASecurityFrameworkAnno
  a <https://www.w3.org/ns/oaAnnotation> ;
  <https://www.w3.org/ns/oahasBody> sto:IIRASecurityFramework ;
  <https://www.w3.org/ns/oahasTarget> [
      a <https://www.w3.org/ns/oaSpecificResource> ;
      terms:format "pdf" ;
      <https://www.w3.org/ns/oahasSelector> [
          a <https://www.w3.org/ns/oaRangeSelector> ;
          <https://www.w3.org/ns/oahasEndSelector> [
              a <https://www.w3.org/ns/oaXPathSelector> ;
              rdf:value "Page 121" ;
            ] ;
          <https://www.w3.org/ns/oahasStartSelector> [
              a <https://www.w3.org/ns/oaXPathSelector> ;
              rdf:value "Page 11" ;
            ] ;
        ] ;
      <https://www.w3.org/ns/oahasSource> sto:Industrial_Internet_of_Things_Volume_G4_Security_Framework ;
    ] ;
  <https://www.w3.org/ns/oahasTarget> [
      a <https://www.w3.org/ns/oaSpecificResource> ;
      terms:format "pdf" ;
      <https://www.w3.org/ns/oahasSelector> [
          a <https://www.w3.org/ns/oaRangeSelector> ;
          <https://www.w3.org/ns/oahasEndSelector> [
              a <https://www.w3.org/ns/oaXPathSelector> ;
              rdf:value "Page 121" ;
            ] ;
          <https://www.w3.org/ns/oahasStartSelector> [
              a <https://www.w3.org/ns/oaXPathSelector> ;
              rdf:value "Page 11" ;
            ] ;
        ] ;
      <https://www.w3.org/ns/oahasSource> sto:Industrial_Internet_of_Things_Volume_G4_Security_Framework ;
    ] ;
.
sto:IIRASystemCharacteristics
  a owl:Class ;
  rdfs:label "IIRA System Characteristic"@en ;
  rdfs:subClassOf sto:StandardClassification ;
  rdfs:subClassOf [
      a owl:Restriction ;
      owl:hasValue sto:IIRA ;
      owl:onProperty sto:isDescribedin ;
    ] ;
  rdfs:subClassOf [
      a owl:Restriction ;
      owl:hasValue sto:IIRAFunctionalViewpoint ;
      owl:onProperty dul:isPartOf ;
    ] ;
.
sto:IIRAUsageViewpoint
  a owl:NamedIndividual ;
  a sto:StandardClassification ;
  a sto:Viewpoint ;
  dul:associatedWith sto:BdvaDataViualisationAndUserInteraction ;
  dul:associatedWith sto:DtpEcosystemView ;
  dul:associatedWith sto:FiwareAdvancedUi ;
  dul:associatedWith sto:IviManagementView ;
  rdfs:label "IIRA Usage Viewpoint"@en ;
  skos:note "Publications referred: '(IIC:PUB:G1:V1.80:20170131' '3.5.2 USAGE VIEWPOINT' 'Page 16' " ;
  sto:alignsWith sto:BdvaDataViualisationAndUserInteraction ;
  sto:alignsWith sto:DtpEcosystemView ;
  sto:alignsWith sto:FiwareAdvancedUi ;
  sto:alignsWith sto:IviManagementView ;
  sto:frames rami:ProcessPlanning ;
  sto:frames sto:DynamicAdjustability ;
  sto:frames sto:Evolvability ;
  sto:frames sto:RoleCategorization ;
  sto:frames sto:ServiceChoreography ;
  sto:frames sto:ServiceComposition ;
  sto:frames sto:ServiceDeployment ;
  sto:frames sto:ServiceLifecycleManagement ;
  sto:frames sto:ServiceOrchestration ;
  sto:isDescribedin sto:IIRA ;
.
sto:IIRAUsageViewpointAnno
  a <https://www.w3.org/ns/oaAnnotation> ;
  <https://www.w3.org/ns/oahasBody> sto:IIRAUsageViewpoint ;
  <https://www.w3.org/ns/oahasTarget> [
      a <https://www.w3.org/ns/oaSpecificResource> ;
      terms:format "pdf" ;
      <https://www.w3.org/ns/oahasSelector> [
          a <https://www.w3.org/ns/oaRangeSelector> ;
          <https://www.w3.org/ns/oahasEndSelector> [
              a <https://www.w3.org/ns/oaXPathSelector> ;
              rdf:value "Page 25" ;
            ] ;
          <https://www.w3.org/ns/oahasStartSelector> [
              a <https://www.w3.org/ns/oaXPathSelector> ;
              rdf:value "Page 22" ;
            ] ;
        ] ;
      <https://www.w3.org/ns/oahasSource> sto:The_Industrial_Internet_of_Things_Volume_G1_Reference_Architecture ;
    ] ;
.
sto:IIoTConsortium
  a owl:Class ;
  a owl:NamedIndividual ;
  terms:creator sto:sebastian ;
  terms:creator "sebastian" ;
  rdfs:subClassOf foaf:Organization ;
.
sto:IPSO
  a owl:NamedIndividual ;
  a foaf:Organization ;
  a sto:IIoTConsortium ;
  terms:creator sto:sebastian ;
  rdfs:comment "The Alliance is a global non-profit organization serving the various communities seeking to establish the Internet Protocol as the network for the connection of Smart Objects by providing coordinated marketing efforts available to the general public. (source: https://www.postscapes.com/internet-of-things-protocols/)"@en ;
  rdfs:label "IPSO"@en ;
  sto:hasOfficialResource <http://www.ipso-alliance.org/> ;
.
sto:IPv4Support
  a owl:NamedIndividual ;
  a sto:Concern ;
  terms:creator sto:sebastian ;
  <http://voag.linkedmodel.org/voag#hasStakeholder> "System Architect"@en ;
  rdfs:comment "Communication with non-IPv6 networks must be possible (IPv4, others)."@en ;
  rdfs:label "IPv4 Support"@en ;
  rdfs:seeAlso "IoT-A Requirement UNI.313" ;
  sto:hasDBpediaResource <http://dbpedia.org/resource/Internet_Protocol> ;
  sto:supports sto:SyntacticInteroperability ;
.
sto:IPv6
  a owl:NamedIndividual ;
  a foaf:Document ;
  a sto:Publication ;
  a sto:TechnicalSpecification ;
  terms:creator sto:sebastian ;
  rdfs:comment "IPv6, is an Internet Layer protocol for packet-switched internetworking and provides end-to-end datagram transmission across multiple IP networks. (source: https://www.postscapes.com/internet-of-things-protocols/)"@en ;
  rdfs:label "IPv6"@en ;
  sto:hasTargetConcern sto:SyntacticInteroperability ;
  sto:hasWikipediaArticle <https://en.wikipedia.org/wiki/IPv6> ;
.
sto:IPv6Support
  a owl:NamedIndividual ;
  a sto:Concern ;
  terms:creator sto:sebastian ;
  <http://voag.linkedmodel.org/voag#hasStakeholder> "System Architect"@en ;
  rdfs:comment "A system built using the ARM shall use/support common-addressing-schemes such as IPv6."@en ;
  rdfs:label "IPv6 Support"@en ;
  rdfs:seeAlso "IoT-A Requirement UNI.312" ;
  sto:hasDBpediaResource <http://dbpedia.org/resource/Internet_Protocol> ;
  sto:supports sto:SyntacticInteroperability ;
.
sto:ISA
  a owl:NamedIndividual ;
  a foaf:Organization ;
  a sto:StandardOrganization ;
  rdfs:comment "The International Society of Automation (www.isa.org) is a nonprofit professional association that sets the standard for those who apply engineering and technology to improve the management, safety, and cybersecurity of modern automation and control systems used across industry and critical infrastructure. Founded in 1945, ISA develops widely used global standards; certifies industry professionals; provides education and training; publishes books and technical articles; hosts conferences and exhibits; and provides networking and career development programs for its 40,000 members and 400,000 customers around the world."@en ;
  sto:abbreviation "ISA" ;
  sto:formationDate "1945-04-28"^^xsd:date ;
  sto:hasDBpediaResource <http://dbpedia.org/resource/International_Society_of_Automation> ;
  sto:hasHeadquaterIn dbr:_North_Carolina ;
  sto:hasOfficialResource <https://www.isa.org/> ;
  sto:hasWikipediaArticle <https://en.wikipedia.org/wiki/International_Society_of_Automation> ;
  sto:orgName "International Society of Automation"@en ;
.
sto:ISA-95
  a owl:NamedIndividual ;
  a foaf:Document ;
  a sto:Publication ;
  a sto:Standard ;
  terms:creator sto:ANSI ;
  terms:creator sto:ISA ;
  rdfs:comment "ANSI/ISA-95, or ISA-95 as it is more commonly referred, is an international standard from the International Society of Automation for developing an automated interface between enterprise and control systems. This standard has been developed for global manufacturers. It was developed to be applied in all industries, and in all sorts of processes, like batch processes, continuous and repetitive processes.There are 5 parts of the ISA-95 standard.ISA-95 Models"@en ;
  rdfs:label "ISA 95"@en ;
  foaf:maker sto:ANSI ;
  foaf:maker sto:ISA ;
  sto:hasDBpediaResource <http://dbpedia.org/resource/ANSI/ISA-95> ;
  sto:hasDeveloper sto:ANSI ;
  sto:hasDeveloper sto:ISA ;
  sto:hasOfficialResource <https://www.isa.org/isa95/> ;
  sto:hasPublisher sto:ANSI ;
  sto:hasPublisher sto:ISA ;
  sto:hasWikipediaArticle <https://en.wikipedia.org/wiki/ANSI/ISA-95> ;
  sto:relatedTo sto:B2MML ;
  sto:relatedTo sto:IEC_62264 ;
  sto:relatedTo sto:ISA-95 ;
.
sto:ISA10011a
  a owl:NamedIndividual ;
  a foaf:Document ;
  a sto:Publication ;
  a sto:TechnicalSpecification ;
  terms:creator sto:sebastian ;
  rdfs:comment "ISA100.11a is a wireless networking technology standard developed by the International Society of Automation (ISA). The official description is Wireless Systems for Industrial Automation: Process Control and Related Application. (source: https://www.postscapes.com/internet-of-things-protocols/)"@en ;
  rdfs:label "ISA100.11a"@en ;
  sto:hasWikipediaArticle <https://en.wikipedia.org/wiki/ISA100.11a> ;
.
sto:ISA95
  a owl:NamedIndividual ;
  a sto:StandardClassification ;
  rdfs:comment "Describes the ISA95 as a Standarization Initiative that classifies Standards"@en ;
  rdfs:label "ISA 95"@en ;
  sto:isDescribedin sto:IotaReferenceArchitecture ;
.
sto:ISA95Level
  a owl:Class ;
  rdfs:comment "Describes the ISA95 levels to classify the industry Standards according to those levels. Eg., Device, SCADA, etc. It has strong relation to the RAMI Hierarchy levels"@en ;
  rdfs:label "ISA 95 Level"@en ;
  rdfs:subClassOf sto:StandardClassification ;
.
sto:ISA_62443
  a owl:NamedIndividual ;
  a foaf:Document ;
  a sto:Publication ;
  a sto:Standard ;
  rdfs:label "ISA_62443"@en ;
  sto:publisher sto:ISA ;
.
sto:ISO
  a dul:Collection ;
  a owl:NamedIndividual ;
  a foaf:Organization ;
  a sto:StandardOrganization ;
  rdfs:comment "Is an independent, non-governmental organization, the members of which are the standards organizations of the 162 member countries. It is the world's largest developer of voluntary international standards and facilitates world trade by providing common standards between nations. Nearly twenty thousand standards have been set covering everything from manufactured products and technology to food safety, agriculture and healthcare."@en ;
  rdfs:comment "The International Organization for Standardization (ISO) is an international standard-setting body composed of representatives from various national standards organizations."@en ;
  sto:abbreviation "ISO" ;
  sto:belongsTo dbr:Switzerland ;
  sto:formationDate "1947-02-23"^^xsd:date ;
  sto:hasDBpediaResource <http://dbpedia.org/page/International_Organization_for_Standardization> ;
  sto:hasHeadquaterIn dbr:Geneva ;
  sto:hasOfficialResource <https://www.iso.org> ;
  sto:hasOfficialResource <https://www.iso.org/about-us.html> ;
  sto:hasWikipediaArticle <https://en.wikipedia.org/wiki/International_Organization_for_Standardization> ;
  sto:orgName "International Organization for Standardization"@en ;
  sto:orgName "Internationale Organisation für Normung"@de ;
  sto:orgName "Organisation internationale de normalisation"@fr ;
  sto:orgName "The International Organization for Standardization"@en ;
  sto:orgName "Международная организация по стандартизации"@ru ;
.
sto:ISO_10303
  a owl:NamedIndividual ;
  a foaf:Document ;
  a sto:Publication ;
  a sto:Standard ;
  terms:creator sto:ISO ;
  rdfs:comment "Standard for the Exchange of Product model data. ISO 10303 can represent 3D objects in Computer-aided design (CAD) and related information."@en ;
  rdfs:label "ISO 10303"@en ;
  skos:note "TODO - Split properly and classify it - check the NIST paper" ;
  foaf:maker sto:ISO ;
  sto:hasClassification sto:ProductLifeCycleManagement ;
  sto:hasDBpediaResource <http://dbpedia.org/page/ISO_10303> ;
  sto:hasOfficialResource <https://www.steptools.com/stds/step/> ;
  sto:hasPublisher sto:ISO ;
  sto:hasWikipediaArticle <https://en.wikipedia.org/wiki/ISO_10303> ;
  sto:relatedTo sto:ISO_10303 ;
  sto:relatedTo sto:ISO_8062-4 ;
.
sto:ISO_1101
  a owl:NamedIndividual ;
  a foaf:Document ;
  a sto:Publication ;
  a sto:Standard ;
  terms:creator sto:ISO ;
  rdfs:comment "Geometrical product specifications (GPS) -- Geometrical tolerancing -- Tolerances of form, orientation, location and run-out"@en ;
  rdfs:label "ISO 1101"@en ;
  foaf:maker sto:ISO ;
  sto:hasClassification sto:ModelingPractice ;
  sto:hasClassification sto:RAMIAssetlayer ;
  sto:hasClassification sto:RAMIProduct ;
  sto:hasOfficialResource <https://www.iso.org/standard/66777.html> ;
  sto:hasPublicationDate "2017-02-01"^^xsd:date ;
  sto:hasPublisher sto:ISO ;
.
sto:ISO_11404
  a owl:NamedIndividual ;
  a sto:Standard ;
  rdfs:comment "Information technology -- General-Purpose Datatypes (GPD)"@en ;
  rdfs:label "ISO/IEC 11404"@en ;
  sto:hasDeveloper sto:IEC ;
  sto:hasDeveloper sto:ISO ;
  sto:hasOfficialResource <https://webstore.iec.ch/publication/9602> ;
  sto:hasOfficialResource <https://www.iso.org/standard/39479.html> ;
  sto:hasOpenResource <http://www.open-std.org/jtc1/sc22/open/n3620.pdf> ;
  sto:hasPublicationDate "2007-12-01"^^xsd:date ;
  sto:hasPublisher sto:ISO ;
  sto:hasWikipediaArticle <https://en.wikipedia.org/wiki/ISO/IEC_11404> ;
.
sto:ISO_11783
  a owl:NamedIndividual ;
  a foaf:Document ;
  a sto:Publication ;
  a sto:Standard ;
  terms:creator sto:ISO ;
  rdfs:comment "ISO 11783, known as Tractors and machinery for agriculture and forestry—Serial control and communications data network is a communication protocol for the agriculture industry based on the SAE J1939 protocol (which includes CANbus)."@en ;
  rdfs:label "ISO 11783"@en ;
  foaf:maker sto:ISO ;
  sto:hasDBpediaResource <http://dbpedia.org/resource/ISO_11783> ;
  sto:hasOfficialResource <https://www.iso.org/standard/61646.html> ;
  sto:hasPublisher sto:ISO ;
  sto:hasWikipediaArticle <https://en.wikipedia.org/wiki/ISO_11783> ;
  sto:relatedTo sto:ISO_11783 ;
  sto:relatedTo sto:ISO_11898-1 ;
.
sto:ISO_11898-1
  a owl:NamedIndividual ;
  a foaf:Document ;
  a sto:Publication ;
  a sto:Standard ;
  terms:creator sto:ISO ;
  rdfs:comment "Used mainly for Road vehicles Controller area network (CAN) Data link layer and physical signalling."@en ;
  rdfs:label "ISO 11898-1"@en ;
  foaf:maker sto:ISO ;
  sto:hasClassification rami:Engineering ;
  sto:hasClassification rami:Safety ;
  sto:hasClassification sto:RAMICommunicationlayer ;
  sto:hasDBpediaResource <http://dbpedia.org/page/CAN_bus> ;
  sto:hasDomain sto:IndustrialAutomation ;
  sto:hasOfficialResource <https://www.iso.org/standard/63648.html> ;
  sto:hasPublicationDate "2015-12-01"^^xsd:date ;
  sto:hasPublisher sto:ISO ;
  sto:hasTag "CAN Bus"@en ;
  sto:relatedTo sto:ISO_11783 ;
  sto:relatedTo sto:ISO_11898-1 ;
.
sto:ISO_1302
  a owl:NamedIndividual ;
  a foaf:Document ;
  a sto:Publication ;
  a sto:Standard ;
  rdfs:comment "Geometrical product specifications Standards"@en ;
  rdfs:label "ISO 1302"@en ;
  sto:hasClassification sto:ModelingPractice ;
  sto:hasOfficialResource <https://www.iso.org/standard/28089.html> ;
  sto:hasPublicationDate "2002-02-01"^^xsd:date ;
.
sto:ISO_13374
  a owl:NamedIndividual ;
  a foaf:Document ;
  a sto:Publication ;
  a sto:Standard ;
  terms:creator sto:ISO ;
  rdfs:comment "Condition monitoring and diagnostics of machines -- Data processing, communication and presentation"@en ;
  rdfs:label "ISO 13374"@en ;
  foaf:maker sto:ISO ;
  sto:hasClassification rami:ConditionMonitoring ;
  sto:hasClassification sto:ProductionSystemEngineering ;
  sto:hasClassification sto:RAMIBusinessLayer ;
  sto:hasClassification sto:RAMIEnterprise ;
  sto:hasDomain sto:IndustrialAutomation ;
  sto:hasOfficialResource <https://www.iso.org/standard/61131.html> ;
  sto:hasPublicationDate "2012-02-01"^^xsd:date ;
  sto:hasPublisher sto:ISO ;
  sto:relatedTo sto:ISO_13374 ;
  sto:relatedTo sto:ISO_15704 ;
  sto:relatedTo sto:ISO_19439 ;
.
sto:ISO_13485
  a owl:NamedIndividual ;
  a foaf:Document ;
  a sto:Publication ;
  a sto:Standard ;
  terms:creator sto:ISO ;
  rdfs:comment "Medical devices -- Quality management systems -- Requirements for regulatory purposes."@en ;
  rdfs:label "ISO 13485"@en ;
  foaf:maker sto:ISO ;
  sto:hasClassification rami:Safety ;
  sto:hasDBpediaResource <http://dbpedia.org/page/ISO_13485> ;
  sto:hasOfficialResource <https://www.iso.org/iso-9001-quality-management.html> ;
  sto:hasPublisher sto:ISO ;
  sto:hasTargetConcern sto:QualityOfService ;
.
sto:ISO_13584
  a owl:NamedIndividual ;
  a foaf:Document ;
  a sto:Publication ;
  a sto:Standard ;
  terms:creator sto:ISO ;
  terms:license sto:PrivateLicenseDocument ;
  rdfs:comment "ISO 13584 is a series of International Standards for the computer-sensible representation and exchange of parts library data. The objective is to provide a mechanism capable of transferring parts library data, independent from any particular system. The nature of this description makes it suitable not only for the exchange of files containing parts libraries, but also as a basis for implementing and sharing databases of parts library data, and archiving"@en ;
  rdfs:label "ISO 13584"@en ;
  foaf:maker sto:ISO ;
  sto:hasClassification sto:ProductCatalogData ;
  sto:hasDBpediaResource <http://dbpedia.org/resource/ISO_13584> ;
  sto:hasMotivation "Standard data elements (properties) are used as elements in administration shell"@en ;
  sto:hasOfficialResource <https://webstore.iec.ch/publication/5380%0Ahttp://www.iso.org/iso/catalogue_detail.htm?csnumber=43423> ;
  sto:hasPublisher sto:ISO ;
  sto:hasTag "Industrial automation systems and integration"@en ;
  sto:hasWikipediaArticle <https://en.wikipedia.org/wiki/ISO_13584> ;
  sto:relatedTo sto:DIN_SPEC_16592 ;
  sto:relatedTo sto:IEC_61131 ;
  sto:relatedTo sto:IEC_61360 ;
  sto:relatedTo sto:IEC_61499 ;
  sto:relatedTo sto:IEC_61804 ;
  sto:relatedTo sto:IEC_61850 ;
  sto:relatedTo sto:IEC_61987_X ;
  sto:relatedTo sto:IEC_62424 ;
  sto:relatedTo sto:IEC_62453 ;
  sto:relatedTo sto:IEC_62541 ;
  sto:relatedTo sto:IEC_62714 ;
  sto:relatedTo sto:ISO_13584 ;
  sto:relatedTo sto:ISO_14306 ;
  sto:relatedTo sto:ISO_15746 ;
  sto:relatedTo sto:ISO_15926 ;
  sto:relatedTo sto:ISO_18629 ;
  sto:relatedTo sto:ISO_18828-2 ;
  sto:relatedTo sto:ISO_20922 ;
  sto:relatedTo sto:ISO_22400 ;
  sto:relatedTo sto:ISO_29002 ;
  sto:relatedTo sto:ISO_ASTM_52915 ;
  sto:relatedTo sto:ISO_PAS_17506 ;
  sto:relatedTo sto:MathML ;
  sto:relatedTo sto:SysML ;
  sto:relatedTo sto:eClass ;
.
sto:ISO_13849
  a owl:NamedIndividual ;
  a foaf:Document ;
  a sto:Publication ;
  a sto:Standard ;
  terms:creator sto:ISO ;
  rdfs:comment "Provides safety requirements and guidance on the principles for the design and integration of safety-related parts of control systems (SRP/CS), including the design of software."@en ;
  rdfs:label "ISO 13849"@en ;
  foaf:maker sto:ISO ;
  <https://w3id.org/i40/hasTargetConcern> sto:Safety ;
  sto:hasClassification rami:Safety ;
  sto:hasClassification sto:IDSRAMCertification ;
  sto:hasClassification sto:IIRASecurity ;
  sto:hasDBpediaResource <http://dbpedia.org/resource/ISO_13849> ;
  sto:hasDomain "Safety of machinery"@en ;
  sto:hasOfficialResource <http://www.iso.org/iso/home/store/catalogue_tc/catalogue_detail.htm?csnumber=69883> ;
  sto:hasPublisher sto:ISO ;
  sto:hasWikipediaArticle <https://en.wikipedia.org/wiki/ISO_13849> ;
  sto:relatedTo sto:IEC_61508 ;
  sto:relatedTo sto:IEC_61511 ;
  sto:relatedTo sto:IEC_62061 ;
  sto:relatedTo sto:ISO_13849 ;
.
sto:ISO_14306
  a owl:NamedIndividual ;
  a foaf:Document ;
  a sto:Publication ;
  a sto:Standard ;
  terms:creator sto:ISO ;
  rdfs:comment "It provides the description of the structure and content for a binary file having the extension of .jt. A binary file with the .jt extension is generally referred to as a JT file. The JT format described in ISO 14306:2012 is used primarily in industrial use cases as the means for capturing and repurposing lightweight 3D product definition data"@en ;
  rdfs:label "ISO 14306"@en ;
  foaf:maker sto:ISO ;
  sto:hasClassification rami:Engineering ;
  sto:hasClassification rami:Identification ;
  sto:hasClassification rami:ProcessPlanning ;
  sto:hasClassification sto:ProductionSystemModelData ;
  sto:hasClassification sto:RAMIAssetlayer ;
  sto:hasClassification sto:RAMIProduct ;
  sto:hasDomain sto:CAD ;
  sto:hasOfficialResource <https://www.iso.org/standard/60572.html> ;
  sto:hasPublicationDate "2017-07-01"^^xsd:date ;
  sto:hasPublisher sto:ISO ;
  sto:relatedTo sto:DIN_SPEC_16592 ;
  sto:relatedTo sto:IEC_61131 ;
  sto:relatedTo sto:IEC_61360 ;
  sto:relatedTo sto:IEC_61499 ;
  sto:relatedTo sto:IEC_61804 ;
  sto:relatedTo sto:IEC_61850 ;
  sto:relatedTo sto:IEC_61987_X ;
  sto:relatedTo sto:IEC_62424 ;
  sto:relatedTo sto:IEC_62453 ;
  sto:relatedTo sto:IEC_62541 ;
  sto:relatedTo sto:IEC_62714 ;
  sto:relatedTo sto:ISO_13584 ;
  sto:relatedTo sto:ISO_14306 ;
  sto:relatedTo sto:ISO_15746 ;
  sto:relatedTo sto:ISO_15926 ;
  sto:relatedTo sto:ISO_18629 ;
  sto:relatedTo sto:ISO_18828-2 ;
  sto:relatedTo sto:ISO_20922 ;
  sto:relatedTo sto:ISO_22400 ;
  sto:relatedTo sto:ISO_29002 ;
  sto:relatedTo sto:ISO_ASTM_52915 ;
  sto:relatedTo sto:ISO_PAS_17506 ;
  sto:relatedTo sto:MathML ;
  sto:relatedTo sto:SysML ;
  sto:relatedTo sto:eClass ;
.
sto:ISO_14443
  a owl:NamedIndividual ;
  a foaf:Document ;
  a sto:Publication ;
  a sto:Standard ;
  terms:creator sto:IEC ;
  terms:creator sto:ISO ;
  rdfs:comment "ISO 14443 Identification cards -- Contactless integrated circuit cards -- Proximity cards is an international standard that defines proximity cards used for identification, and the transmission protocols for communicating with it"@en ;
  rdfs:label "ISO 14443"@en ;
  foaf:maker sto:IEC ;
  foaf:maker sto:ISO ;
  sto:hasPublisher sto:IEC ;
  sto:hasPublisher sto:ISO ;
.
sto:ISO_14739-1
  a owl:NamedIndividual ;
  a foaf:Document ;
  a sto:Publication ;
  a sto:Standard ;
  terms:creator sto:ISO ;
  rdfs:comment "Document management -- 3D use of Product Representation Compact (PRC) format-ISO 14739-1:2014 describes PRC 10001 of a product representation compact (PRC) file format for three dimensional (3D) content data. This format is designed to be included in PDF (ISO 32000) and other similar document formats for the purpose of 3D visualization and exchange. "@en ;
  rdfs:label "ISO 14739-1"@en ;
  skos:altLabel "STEP"@en ;
  foaf:maker sto:ISO ;
  sto:hasClassification sto:ProductModelDataExchange ;
  sto:hasDomain sto:CAD ;
  sto:hasOfficialResource <https://www.iso.org/standard/54948.html> ;
  sto:hasPublicationDate "2014-12-01"^^xsd:date ;
  sto:hasPublisher sto:ISO ;
.
sto:ISO_15408
  a owl:NamedIndividual ;
  a foaf:Document ;
  a sto:Publication ;
  a sto:Standard ;
  dc11:title "Common Criteria for Information Technology Security Evaluation"@en ;
  terms:creator sto:ISO ;
  rdfs:comment "The Common Criteria for Information Technology Security Evaluation (abbreviated as Common Criteria or CC) is an international standard (ISO/IEC 15408) for computer security certification"@en ;
  rdfs:label "ISO/IEC 15408"@en ;
  foaf:maker sto:ISO ;
  sto:hasClassification sto:IIRASecurity ;
  sto:hasOfficialResource <https://webstore.iec.ch/publication/10255> ;
  sto:hasOfficialResource <https://www.iso.org/standard/50341.html> ;
  sto:hasOfficialResource <https://www.niap-ccevs.org/Documents_and_Guidance/cc_docs.cfm> ;
  sto:hasOpenResource <http://comsec.spb.ru/matherials/is/iso15408-1.pdf> ;
  sto:hasOpenResource <http://www.comsec.spb.ru/matherials/is/iso15408-3.pdf> ;
  sto:hasPublisher sto:ISO ;
  sto:hasWikipediaArticle <http://wikipedia.org/wiki/Common_Criteria_for_Information_Technology_Security_Evaluation> ;
.
sto:ISO_15459
  a owl:NamedIndividual ;
  a foaf:Document ;
  a sto:Publication ;
  a sto:Standard ;
  terms:creator sto:IEC ;
  terms:creator sto:ISO ;
  foaf:maker sto:IEC ;
  foaf:maker sto:ISO ;
  sto:hasPublisher sto:IEC ;
  sto:hasPublisher sto:ISO ;
.
sto:ISO_15531
  a owl:NamedIndividual ;
  a foaf:Document ;
  a sto:Publication ;
  a sto:Standard ;
  terms:creator sto:ISO ;
  rdfs:comment "This Standard models manufacturing management data such as, Resources management data (Resource model); Time related features (Time model); Flow management data in manufacturing (Flow management model)."@en ;
  rdfs:isDefinedBy "https://www.researchgate.net/publication/220171079_ISO_15531_MANDATE_a_standardised_data_model_for_manufacturing_management" ;
  rdfs:label "ISO 15531"@en ;
  foaf:maker sto:ISO ;
  sto:hasDomain sto:IndustrialProcessMeasurementControl ;
  sto:hasOfficialResource <https://www.iso.org/standard/28144.html> ;
  sto:hasPublisher sto:ISO ;
  sto:relatedTo sto:ISO_15531 ;
  sto:relatedTo sto:ISO_15531-2x ;
  sto:relatedTo sto:ISO_15531-3x ;
  sto:relatedTo sto:ISO_15531-4x ;
.
sto:ISO_15531-2x
  a owl:NamedIndividual ;
  a foaf:Document ;
  a sto:Publication ;
  a sto:Standard ;
  a sto:StandardPart ;
  dul:isComponentOf sto:ISO_15531 ;
  rdfs:comment "Production data for external exchanges. refering to the representation of product information to be exchanged with the external environment (customers and suppliers), with the aim to model the main production information exchanged between industrial companies, in order to improve exchanges and integration through the use of EDI protocols."@en ;
  rdfs:isDefinedBy "https://www.researchgate.net/publication/220171079_ISO_15531_MANDATE_a_standardised_data_model_for_manufacturing_management" ;
  rdfs:label "ISO 15531 2x series"@en ;
  sto:relatedTo sto:ISO_15531 ;
  sto:relatedTo sto:ISO_15531-2x ;
  sto:relatedTo sto:ISO_15531-3x ;
  sto:relatedTo sto:ISO_15531-4x ;
.
sto:ISO_15531-3x
  a owl:NamedIndividual ;
  a foaf:Document ;
  a sto:Publication ;
  a sto:Standard ;
  a sto:StandardPart ;
  dul:isComponentOf sto:ISO_15531 ;
  rdfs:comment "Manufacturing resource usage management data : refering to the way of managing the use of resources, such as resource configuration and capabilities, operation management of manufacturing devices, installations and facilities."@en ;
  rdfs:comment "Manufacturing resource usage management data sto: refering to the way of managing the use of resources, such as resource configuration and capabilities, operation management of manufacturing devices, installations and facilities."@en ;
  rdfs:isDefinedBy "https://www.researchgate.net/publication/220171079_ISO_15531_MANDATE_a_standardised_data_model_for_manufacturing_management" ;
  rdfs:label "ISO 15531 3x series"@en ;
  sto:relatedTo sto:ISO_15531 ;
  sto:relatedTo sto:ISO_15531-2x ;
  sto:relatedTo sto:ISO_15531-3x ;
  sto:relatedTo sto:ISO_15531-4x ;
.
sto:ISO_15531-4x
  a owl:NamedIndividual ;
  a foaf:Document ;
  a sto:Publication ;
  a sto:Standard ;
  a sto:StandardPart ;
  dul:isComponentOf sto:ISO_15531 ;
  rdfs:comment "Manufacturing flow management data : refering to the material flow control and aiming at the representation of data and elements supporting the control and monitoring of the flow of materials in manufacturing processes."@en ;
  rdfs:comment "Manufacturing flow management data sto: refering to the material flow control and aiming at the representation of data and elements supporting the control and monitoring of the flow of materials in manufacturing processes."@en ;
  rdfs:isDefinedBy "https://www.researchgate.net/publication/220171079_ISO_15531_MANDATE_a_standardised_data_model_for_manufacturing_management" ;
  rdfs:label "ISO 15531 4x series"@en ;
  sto:relatedTo sto:ISO_15531 ;
  sto:relatedTo sto:ISO_15531-2x ;
  sto:relatedTo sto:ISO_15531-3x ;
  sto:relatedTo sto:ISO_15531-4x ;
.
sto:ISO_15704
  a owl:NamedIndividual ;
  a foaf:Document ;
  a sto:Publication ;
  a sto:Standard ;
  terms:creator sto:ISO ;
  rdfs:comment "Identifies requirements for enterprise-reference architectures and methodologies"@en ;
  rdfs:label "ISO 15704"@en ;
  foaf:maker sto:ISO ;
  sto:hasClassification rami:Other ;
  sto:hasClassification sto:RAMIBusinessLayer ;
  sto:hasClassification sto:RAMIEnterprise ;
  sto:hasDomain sto:IndustrialAutomation ;
  sto:hasOfficialResource <https://www.iso.org/standard/28777.html> ;
  sto:hasPublicationDate "2000-06-01"^^xsd:date ;
  sto:hasPublisher sto:ISO ;
  sto:relatedTo sto:ISO_13374 ;
  sto:relatedTo sto:ISO_15704 ;
  sto:relatedTo sto:ISO_19439 ;
.
sto:ISO_15746
  a owl:NamedIndividual ;
  a foaf:Document ;
  a sto:Publication ;
  a sto:Standard ;
  terms:creator sto:ISO ;
  rdfs:comment "Automation systems and integration -- Integration of advanced process control and optimization capabilities for manufacturing systems."@en ;
  rdfs:label "ISO 15746"@en ;
  foaf:maker sto:ISO ;
  sto:hasClassification rami:Engineering ;
  sto:hasClassification sto:ProductLifeCycleManagement ;
  sto:hasClassification sto:RAMICommunicationlayer ;
  sto:hasClassification sto:RAMIControlDevice ;
  sto:hasClassification sto:RAMIFieldDevice ;
  sto:hasClassification sto:RAMIFunctional ;
  sto:hasClassification sto:RAMIInformationLayer ;
  sto:hasClassification sto:RAMIIntegrationLayer ;
  sto:hasClassification sto:RAMIProduct ;
  sto:hasDomain sto:IndustrialAutomation ;
  sto:hasOfficialResource <https://www.iso.org/standard/61131.html> ;
  sto:hasPublicationDate "2015-04-01"^^xsd:date ;
  sto:hasPublisher sto:ISO ;
  sto:relatedTo sto:DIN_SPEC_16592 ;
  sto:relatedTo sto:IEC_61131 ;
  sto:relatedTo sto:IEC_61360 ;
  sto:relatedTo sto:IEC_61499 ;
  sto:relatedTo sto:IEC_61804 ;
  sto:relatedTo sto:IEC_61850 ;
  sto:relatedTo sto:IEC_61987_X ;
  sto:relatedTo sto:IEC_62424 ;
  sto:relatedTo sto:IEC_62453 ;
  sto:relatedTo sto:IEC_62541 ;
  sto:relatedTo sto:IEC_62714 ;
  sto:relatedTo sto:ISO_13584 ;
  sto:relatedTo sto:ISO_14306 ;
  sto:relatedTo sto:ISO_15746 ;
  sto:relatedTo sto:ISO_15926 ;
  sto:relatedTo sto:ISO_18629 ;
  sto:relatedTo sto:ISO_18828-2 ;
  sto:relatedTo sto:ISO_20922 ;
  sto:relatedTo sto:ISO_22400 ;
  sto:relatedTo sto:ISO_29002 ;
  sto:relatedTo sto:ISO_ASTM_52915 ;
  sto:relatedTo sto:ISO_PAS_17506 ;
  sto:relatedTo sto:MathML ;
  sto:relatedTo sto:SysML ;
  sto:relatedTo sto:eClass ;
.
sto:ISO_15926
  a owl:NamedIndividual ;
  a foaf:Document ;
  a sto:Publication ;
  a sto:Standard ;
  terms:creator sto:ISO ;
  rdfs:comment "Industrial automation systems and integration -- Integration of life-cycle data for process plants including oil and gas production facilities."@en ;
  rdfs:label "ISO 15926"@en ;
  foaf:maker sto:ISO ;
  sto:hasClassification rami:Configuration ;
  sto:hasClassification rami:Engineering ;
  sto:hasClassification sto:ProductLifeCycleManagement ;
  sto:hasClassification sto:RAMIIntegrationLayer ;
  sto:hasClassification sto:RAMIProduct ;
  sto:hasDomain sto:IndustrialAutomation ;
  sto:hasOfficialResource <https://www.iso.org/standard/29557.html> ;
  sto:hasPublicationDate "2003-12-01"^^xsd:date ;
  sto:hasPublisher sto:ISO ;
  sto:relatedTo sto:DIN_SPEC_16592 ;
  sto:relatedTo sto:IEC_61131 ;
  sto:relatedTo sto:IEC_61360 ;
  sto:relatedTo sto:IEC_61499 ;
  sto:relatedTo sto:IEC_61804 ;
  sto:relatedTo sto:IEC_61850 ;
  sto:relatedTo sto:IEC_61987_X ;
  sto:relatedTo sto:IEC_62424 ;
  sto:relatedTo sto:IEC_62453 ;
  sto:relatedTo sto:IEC_62541 ;
  sto:relatedTo sto:IEC_62714 ;
  sto:relatedTo sto:ISO_13584 ;
  sto:relatedTo sto:ISO_14306 ;
  sto:relatedTo sto:ISO_15746 ;
  sto:relatedTo sto:ISO_15926 ;
  sto:relatedTo sto:ISO_18629 ;
  sto:relatedTo sto:ISO_18828-2 ;
  sto:relatedTo sto:ISO_20922 ;
  sto:relatedTo sto:ISO_22400 ;
  sto:relatedTo sto:ISO_29002 ;
  sto:relatedTo sto:ISO_ASTM_52915 ;
  sto:relatedTo sto:ISO_PAS_17506 ;
  sto:relatedTo sto:MathML ;
  sto:relatedTo sto:SysML ;
  sto:relatedTo sto:eClass ;
.
sto:ISO_16739
  a owl:NamedIndividual ;
  a foaf:Document ;
  a sto:Publication ;
  a sto:Standard ;
  terms:creator sto:ISO ;
  rdfs:comment "Industry Foundation Classes (IFC) for data sharing in the construction and facility management industries."@en ;
  rdfs:label "ISO 16739"@en ;
  foaf:maker sto:ISO ;
  sto:hasClassification rami:Lifecycle_Status ;
  sto:hasClassification sto:ProductLifeCycleManagement ;
  sto:hasClassification sto:RAMIStation ;
  sto:hasClassification sto:RAMIWorkCenter ;
  sto:hasDomain sto:IndustrialAutomation ;
  sto:hasOfficialResource <https://www.iso.org/standard/51622.html> ;
  sto:hasPublicationDate "2013-04-01"^^xsd:date ;
  sto:hasPublisher sto:ISO ;
  sto:relatedTo sto:IEC_62890 ;
  sto:relatedTo sto:ISO_16739 ;
.
sto:ISO_16792
  a owl:NamedIndividual ;
  a foaf:Document ;
  a sto:Publication ;
  a sto:Standard ;
  terms:creator sto:ISO ;
  rdfs:comment "ISO 16792 Technical product documentation -- Digital product definition data practices-It supports two methods of application: model-only and model and drawing in digital format."@en ;
  rdfs:label "ISO 16792"@en ;
  foaf:maker sto:ISO ;
  sto:hasClassification sto:ModelingPractice ;
  sto:hasClassification sto:RAMIAssetlayer ;
  sto:hasClassification sto:RAMIProduct ;
  sto:hasDomain sto:CAD ;
  sto:hasOfficialResource <https://www.iso.org/standard/56865.html> ;
  sto:hasPublicationDate "2015-12-01"^^xsd:date ;
  sto:hasPublisher sto:ISO ;
.
sto:ISO_18629
  a owl:NamedIndividual ;
  a foaf:Document ;
  a sto:Publication ;
  a sto:Standard ;
  terms:creator sto:ISO ;
  rdfs:comment "ISO 18629-1:2004 provides a general overview of the different series of parts of ISO 18629, which defines a process specification language aimed at identifying, formally defining and structuring the semantic concepts intrinsic to the capture and exchange of process information related to discrete manufacturing."@en ;
  rdfs:label "ISO 19629"@en ;
  foaf:maker sto:ISO ;
  sto:hasClassification rami:Configuration ;
  sto:hasClassification rami:Engineering ;
  sto:hasClassification sto:ProductModelDataExchange ;
  sto:hasClassification sto:RAMICommunicationlayer ;
  sto:hasClassification sto:RAMIControlDevice ;
  sto:hasClassification sto:RAMIFieldDevice ;
  sto:hasClassification sto:RAMIFunctionalLayer ;
  sto:hasClassification sto:RAMIInformationLayer ;
  sto:hasClassification sto:RAMIIntegrationLayer ;
  sto:hasClassification sto:RAMIProduct ;
  sto:hasDomain sto:IndustrialAutomation ;
  sto:hasOfficialResource <https://www.iso.org/standard/35431.html> ;
  sto:hasPublicationDate "2004-11-01"^^xsd:date ;
  sto:hasPublisher sto:ISO ;
  sto:hasTag "PSL"@en ;
  sto:hasWikipediaArticle <https://en.wikipedia.org/wiki/Process_Specification_Language> ;
  sto:relatedTo sto:DIN_SPEC_16592 ;
  sto:relatedTo sto:IEC_61131 ;
  sto:relatedTo sto:IEC_61360 ;
  sto:relatedTo sto:IEC_61499 ;
  sto:relatedTo sto:IEC_61804 ;
  sto:relatedTo sto:IEC_61850 ;
  sto:relatedTo sto:IEC_61987_X ;
  sto:relatedTo sto:IEC_62424 ;
  sto:relatedTo sto:IEC_62453 ;
  sto:relatedTo sto:IEC_62541 ;
  sto:relatedTo sto:IEC_62714 ;
  sto:relatedTo sto:ISO_13584 ;
  sto:relatedTo sto:ISO_14306 ;
  sto:relatedTo sto:ISO_15746 ;
  sto:relatedTo sto:ISO_15926 ;
  sto:relatedTo sto:ISO_18629 ;
  sto:relatedTo sto:ISO_18828-2 ;
  sto:relatedTo sto:ISO_20922 ;
  sto:relatedTo sto:ISO_22400 ;
  sto:relatedTo sto:ISO_29002 ;
  sto:relatedTo sto:ISO_ASTM_52915 ;
  sto:relatedTo sto:ISO_PAS_17506 ;
  sto:relatedTo sto:MathML ;
  sto:relatedTo sto:SysML ;
  sto:relatedTo sto:eClass ;
.
sto:ISO_18828-2
  a owl:NamedIndividual ;
  a foaf:Document ;
  a sto:Publication ;
  a sto:Standard ;
  terms:creator sto:ISO ;
  rdfs:comment "Industrial automation systems and integration -- Standardized procedures for production systems engineering."@en ;
  rdfs:label "ISO 18828-2"@en ;
  foaf:maker sto:ISO ;
  sto:hasClassification rami:Engineering ;
  sto:hasClassification sto:RAMIControlDevice ;
  sto:hasClassification sto:RAMIEnterprise ;
  sto:hasClassification sto:RAMIFieldDevice ;
  sto:hasClassification sto:RAMIProduct ;
  sto:hasClassification sto:RAMIStation ;
  sto:hasClassification sto:RAMIWorkCenter ;
  sto:hasDomain sto:IndustrialAutomation ;
  sto:hasOfficialResource <https://www.iso.org/standard/63505.html> ;
  sto:hasPublicationDate "2016-10-01"^^xsd:date ;
  sto:hasPublisher sto:ISO ;
  sto:relatedTo sto:DIN_SPEC_16592 ;
  sto:relatedTo sto:IEC_61131 ;
  sto:relatedTo sto:IEC_61360 ;
  sto:relatedTo sto:IEC_61499 ;
  sto:relatedTo sto:IEC_61804 ;
  sto:relatedTo sto:IEC_61850 ;
  sto:relatedTo sto:IEC_61987_X ;
  sto:relatedTo sto:IEC_62424 ;
  sto:relatedTo sto:IEC_62453 ;
  sto:relatedTo sto:IEC_62541 ;
  sto:relatedTo sto:IEC_62714 ;
  sto:relatedTo sto:ISO_13584 ;
  sto:relatedTo sto:ISO_14306 ;
  sto:relatedTo sto:ISO_15746 ;
  sto:relatedTo sto:ISO_15926 ;
  sto:relatedTo sto:ISO_18629 ;
  sto:relatedTo sto:ISO_18828-2 ;
  sto:relatedTo sto:ISO_20922 ;
  sto:relatedTo sto:ISO_22400 ;
  sto:relatedTo sto:ISO_29002 ;
  sto:relatedTo sto:ISO_ASTM_52915 ;
  sto:relatedTo sto:ISO_PAS_17506 ;
  sto:relatedTo sto:MathML ;
  sto:relatedTo sto:SysML ;
  sto:relatedTo sto:eClass ;
.
sto:ISO_19439
  a owl:NamedIndividual ;
  a foaf:Document ;
  a sto:Publication ;
  a sto:Standard ;
  terms:creator sto:ISO ;
  dul:associatedWith sto:Certification ;
  rdfs:comment "Provides a unified conceptual basis for model-based enterprise engineering that enables consistency, convergence and interoperability of the various modelling methodologies and supporting tools."@en ;
  rdfs:label "ISO 19439"@en ;
  foaf:maker sto:ISO ;
  sto:hasClassification sto:RAMIBusinessLayer ;
  sto:hasDBpediaResource <http://dbpedia.org/page/ISO_19439> ;
  sto:hasOfficialResource <https://www.iso.org/standard/33833.html> ;
  sto:hasPublisher sto:ISO ;
  sto:hasWikipediaArticle <https://en.wikipedia.org/wiki/ISO_19439> ;
  sto:relatedTo sto:ISO_13374 ;
  sto:relatedTo sto:ISO_15704 ;
  sto:relatedTo sto:ISO_19439 ;
.
sto:ISO_19440
  a owl:NamedIndividual ;
  a foaf:Document ;
  a sto:Publication ;
  a sto:Standard ;
  terms:creator sto:ISO ;
  rdfs:comment "Enterprise integration -- Constructs for enterprise modelling-specifies the characteristics of the core constructs necessary for computer-supported modelling of enterprises conforming to ISO 19439.."@en ;
  rdfs:label "ISO 19440"@en ;
  foaf:maker sto:ISO ;
  sto:hasClassification rami:Engineering ;
  sto:hasClassification sto:EnterpriseLevel ;
  sto:hasClassification sto:RAMIEnterprise ;
  sto:hasClassification sto:RAMIIntegrationLayer ;
  sto:hasClassification sto:RAMIProduct ;
  sto:hasDomain sto:EnterpriseIntegration ;
  sto:hasOfficialResource <https://www.iso.org/standard/33834.html> ;
  sto:hasPublicationDate "2007-12-01"^^xsd:date ;
  sto:hasPublisher sto:ISO ;
  sto:relatedTo sto:BPMN ;
  sto:relatedTo sto:ISO_19440 ;
.
sto:ISO_19770
  a owl:NamedIndividual ;
  a foaf:Document ;
  a sto:Publication ;
  a sto:Standard ;
  terms:creator sto:IEC ;
  terms:creator sto:ISO ;
  terms:title "Information technology — Software asset management"@en ;
  rdfs:comment "International standards in the ISO/IEC 19770 family of standards for IT asset management (ITAM) address both the processes and technology for managing software assets and related IT assets. Broadly speaking, the standard family belongs to the set of Software Asset Management (or SAM) standards and is integrated with other Management System Standards."@en ;
  rdfs:label "ISO/IEC 19770"@en ;
  foaf:maker sto:IEC ;
  foaf:maker sto:ISO ;
  sto:hasClassification sto:IIRASecurity ;
  sto:hasDBpediaResource <http://dbpedia.org/resource/ISO/IEC_19770> ;
  sto:hasDeveloper sto:ISO ;
  sto:hasPublicationDate "2017-12-01"^^xsd:date ;
  sto:hasPublisher sto:IEC ;
  sto:hasPublisher sto:ISO ;
  sto:hasWikipediaArticle <https://en.wikipedia.org/wiki/ISO/IEC_19770> ;
.
sto:ISO_19941
  a owl:NamedIndividual ;
  a foaf:Document ;
  a sto:Publication ;
  a sto:Standard ;
  terms:creator sto:sebastian ;
  terms:title "Cloud Computing - Interoperability and Portability"@en ;
  rdfs:comment ""@en ;
  rdfs:label "ISO/IEC 19941:2017"@en ;
  sto:hasOfficialResource <http://standards.iso.org/ittf/PubliclyAvailableStandards/c066639_ISO_IEC_19941_2017.zip> ;
  sto:hasTargetConcern sto:CloudComputing ;
.
sto:ISO_20140_5
  a owl:NamedIndividual ;
  a foaf:Document ;
  a sto:Publication ;
  a sto:Standard ;
  terms:creator sto:ISO ;
  rdfs:comment "Automation systems and integration -- Evaluating energy efficiency and other factors of manufacturing systems that influence the environment"@en ;
  rdfs:label "ISO 20140-5"@en ;
  foaf:maker sto:ISO ;
  sto:hasClassification rami:EnergyEfficiency ;
  sto:hasOfficialResource <http://www.iso.org/iso/catalogue_detail.htm?csnumber=54809> ;
  sto:hasPublisher sto:ISO ;
  sto:hasTag "Energy Efficiency"@en ;
.
sto:ISO_20140_P1
  a owl:NamedIndividual ;
  a foaf:Document ;
  a sto:Publication ;
  a sto:Standard ;
  terms:creator sto:ISO ;
  terms:title "Automation systems and integration -- Evaluating energy efficiency and other factors of manufacturing systems that influence the environment -- Part 1: Overview and general principles"@en ;
  rdfs:comment ""@en ;
  rdfs:label "ISO 20140-1:2013"@en ;
  foaf:maker sto:ISO ;
  sto:frames sto:EnergyEfficiency ;
  sto:hasClassification sto:IIRASecurity ;
  sto:hasDeveloper sto:ISO ;
  sto:hasOfficialResource <https://www.iso.org/standard/54809.html> ;
  sto:hasPublicationDate "2013-05-01"^^xsd:date ;
  sto:hasPublisher sto:ISO ;
.
sto:ISO_20546
  a owl:NamedIndividual ;
  a foaf:Document ;
  a sto:Publication ;
  a sto:Standard ;
  terms:creator sto:IEC ;
  terms:creator sto:ISO ;
  terms:title "Big data -- Overview and vocabulary"@en ;
  rdfs:comment "TODO: check with other reference architecture standards"@en ;
  rdfs:label "ISO/IEC 20546"@en ;
  foaf:maker sto:IEC ;
  foaf:maker sto:ISO ;
  sto:hasPublisher sto:IEC ;
  sto:hasPublisher sto:ISO ;
.
sto:ISO_20547-3
  a owl:NamedIndividual ;
  a foaf:Document ;
  a sto:Publication ;
  a sto:Standard ;
  terms:creator sto:IEC ;
  terms:creator sto:ISO ;
  terms:title "Big data reference architecture -- Part 3: Reference architecture"@en ;
  rdfs:comment "TODO: how is this standard related to other reference architecture description formats?"@en ;
  rdfs:comment "under development (as from 2018-07-23)"@en ;
  rdfs:label "ISO/IEC DIS 20547-3"@en ;
  foaf:maker sto:IEC ;
  foaf:maker sto:ISO ;
  sto:hasOfficialResource <https://www.iso.org/standard/71277.html> ;
  sto:hasPublisher sto:IEC ;
  sto:hasPublisher sto:ISO ;
.
sto:ISO_20547-4
  a owl:NamedIndividual ;
  a foaf:Document ;
  a sto:Publication ;
  a sto:Standard ;
  terms:creator sto:IEC ;
  terms:creator sto:ISO ;
  terms:title "Big data reference architecture -- Part 4: Security and privacy"@en ;
  rdfs:comment "TODO: check with other reference architecture description frameworks"@en ;
  rdfs:comment "under development (as from 2018-07-23)"@en ;
  rdfs:label "ISO/IEC AWI 20547-4"@en ;
  foaf:maker sto:IEC ;
  foaf:maker sto:ISO ;
  sto:hasOfficialResource <https://www.iso.org/standard/71278.html> ;
  sto:hasPublisher sto:IEC ;
  sto:hasPublisher sto:ISO ;
.
sto:ISO_20922
  a owl:NamedIndividual ;
  a foaf:Document ;
  a sto:Publication ;
  a sto:Standard ;
  terms:creator sto:IBM ;
  terms:creator sto:IEC ;
  terms:creator sto:ISO ;
  terms:creator sto:OASIS ;
  rdfs:comment "ISO/IEC 20922:2016 is a Client Server publish/subscribe messaging transport protocol. It is light weight, open, simple, and designed so as to be easy to implement. These characteristics make it ideal for use in many situations, including constrained environments such as for communication in Machine to Machine (M2M) and Internet of Things (IoT) contexts where a small code footprint is required and/or network bandwidth is at a premium."@en ;
  rdfs:label "ISO 20922"@en ;
  foaf:maker sto:IBM ;
  foaf:maker sto:IEC ;
  foaf:maker sto:ISO ;
  foaf:maker sto:OASIS ;
  sto:hasClassification sto:InformationDomain ;
  sto:hasClassification sto:TansportLayer ;
  sto:hasDBpediaResource <http://dbpedia.org/resource/MQTT> ;
  sto:hasDeveloper sto:IBM ;
  sto:hasDeveloper sto:OASIS ;
  sto:hasDomain sto:M2M ;
  sto:hasOfficialResource <http://mqtt.org/> ;
  sto:hasOfficialResource <https://www.iso.org/standard/69466.html> ;
  sto:hasPublisher sto:IEC ;
  sto:hasPublisher sto:ISO ;
  sto:hasWikipediaArticle <https://en.wikipedia.org/wiki/MQTT> ;
  sto:relatedTo sto:DIN_SPEC_16592 ;
  sto:relatedTo sto:IEC_61131 ;
  sto:relatedTo sto:IEC_61360 ;
  sto:relatedTo sto:IEC_61499 ;
  sto:relatedTo sto:IEC_61804 ;
  sto:relatedTo sto:IEC_61850 ;
  sto:relatedTo sto:IEC_61987_X ;
  sto:relatedTo sto:IEC_62424 ;
  sto:relatedTo sto:IEC_62453 ;
  sto:relatedTo sto:IEC_62541 ;
  sto:relatedTo sto:IEC_62714 ;
  sto:relatedTo sto:ISO_13584 ;
  sto:relatedTo sto:ISO_14306 ;
  sto:relatedTo sto:ISO_15746 ;
  sto:relatedTo sto:ISO_15926 ;
  sto:relatedTo sto:ISO_18629 ;
  sto:relatedTo sto:ISO_18828-2 ;
  sto:relatedTo sto:ISO_20922 ;
  sto:relatedTo sto:ISO_22400 ;
  sto:relatedTo sto:ISO_29002 ;
  sto:relatedTo sto:ISO_ASTM_52915 ;
  sto:relatedTo sto:ISO_PAS_17506 ;
  sto:relatedTo sto:MathML ;
  sto:relatedTo sto:SysML ;
  sto:relatedTo sto:eClass ;
.
sto:ISO_22400
  a owl:NamedIndividual ;
  a foaf:Document ;
  a sto:Publication ;
  a sto:Standard ;
  terms:creator sto:ISO ;
  rdfs:comment "Automation systems and integration -- Key performance indicators (KPIs) for manufacturing operations management."@en ;
  rdfs:label "ISO 22400"@en ;
  foaf:maker sto:ISO ;
  sto:hasClassification rami:ConditionMonitoring ;
  sto:hasClassification rami:Lifecycle_Status ;
  sto:hasClassification sto:RAMIBusinessLayer ;
  sto:hasClassification sto:RAMIConnectedWorld ;
  sto:hasClassification sto:RAMIControlDevice ;
  sto:hasClassification sto:RAMIEnterprise ;
  sto:hasClassification sto:RAMIFieldDevice ;
  sto:hasClassification sto:RAMIStation ;
  sto:hasClassification sto:RAMIWorkCenter ;
  sto:hasDomain sto:IndustrialAutomation ;
  sto:hasOfficialResource <https://www.iso.org/standard/54497.html> ;
  sto:hasPublicationDate "2014-01-01"^^xsd:date ;
  sto:hasPublisher sto:ISO ;
  sto:relatedTo sto:DIN_SPEC_16592 ;
  sto:relatedTo sto:IEC_61131 ;
  sto:relatedTo sto:IEC_61360 ;
  sto:relatedTo sto:IEC_61499 ;
  sto:relatedTo sto:IEC_61804 ;
  sto:relatedTo sto:IEC_61850 ;
  sto:relatedTo sto:IEC_61987_X ;
  sto:relatedTo sto:IEC_62424 ;
  sto:relatedTo sto:IEC_62453 ;
  sto:relatedTo sto:IEC_62541 ;
  sto:relatedTo sto:IEC_62714 ;
  sto:relatedTo sto:ISO_13584 ;
  sto:relatedTo sto:ISO_14306 ;
  sto:relatedTo sto:ISO_15746 ;
  sto:relatedTo sto:ISO_15926 ;
  sto:relatedTo sto:ISO_18629 ;
  sto:relatedTo sto:ISO_18828-2 ;
  sto:relatedTo sto:ISO_20922 ;
  sto:relatedTo sto:ISO_22400 ;
  sto:relatedTo sto:ISO_29002 ;
  sto:relatedTo sto:ISO_ASTM_52915 ;
  sto:relatedTo sto:ISO_PAS_17506 ;
  sto:relatedTo sto:MathML ;
  sto:relatedTo sto:SysML ;
  sto:relatedTo sto:eClass ;
.
sto:ISO_22745-11
  a owl:NamedIndividual ;
  a foaf:Document ;
  a sto:Publication ;
  a sto:Standard ;
  terms:creator sto:ISO ;
  rdfs:comment "ISO 22745-11:2010 provides guidelines that are recommended for the development of terminology for concepts in an open technical dictionary (OTD).Compliance with these guidelines is not required in order for a term or definition to be included in an OTD. These guidelines are provided as a framework for developers of industrial terminology to ensure that definitions are consistent and understandable. Terminology that complies with these guidelines will be marked as such in the OTD. This will allow a user to perform a search that filters terminology based on compliance with ISO 22745-11:2010."@en ;
  rdfs:label "ISO 22745-11"@en ;
  foaf:maker sto:ISO ;
  sto:hasClassification sto:ProductCatalogData ;
  sto:hasClassification sto:RAMIAssetlayer ;
  sto:hasClassification sto:RAMIProduct ;
  sto:hasDomain sto:IndustrialAutomation ;
  sto:hasOfficialResource <https://www.iso.org/standard/53999.html> ;
  sto:hasPublicationDate "2010-02-01"^^xsd:date ;
  sto:hasPublisher sto:ISO ;
.
sto:ISO_24760
  a owl:NamedIndividual ;
  a foaf:Document ;
  a sto:Publication ;
  a sto:Standard ;
  a sto:StandardClassification ;
  terms:creator sto:IEC ;
  dul:associatedWith sto:Identification ;
  foaf:maker sto:IEC ;
  sto:alignsWith sto:Identification ;
  sto:hasClassification rami:Safety ;
  sto:hasClassification rami:Security ;
  sto:hasClassification sto:IIRASecurity ;
  sto:hasClassification sto:ProductModelDataExchange ;
  sto:hasClassification sto:RAMIControlDevice ;
  sto:hasClassification sto:RAMIFieldDevice ;
  sto:hasClassification sto:RAMIInformationLayer ;
  sto:hasClassification sto:RAMIProduct ;
  sto:hasClassification sto:RAMIStation ;
  sto:hasDomain sto:ITSecurity ;
  sto:hasPublicationDate "2011-01-12"^^xsd:date ;
  sto:hasPublisher sto:IEC ;
  sto:relatedTo sto:IEC_24760 ;
  sto:relatedTo sto:IEC_62443 ;
  sto:relatedTo sto:ISO_24760 ;
.
sto:ISO_26262
  a owl:NamedIndividual ;
  a foaf:Document ;
  a sto:Publication ;
  a sto:Standard ;
  terms:creator sto:ISO ;
  terms:title "Road vehicles – Functional safety"@en ;
  rdfs:comment "ISO 26262, titled \"Road vehicles – Functional safety\", is an international standard for functional safety of electrical and/or electronic systems in production automobiles defined by the International Organization for Standardization (ISO) in 2011."@en ;
  rdfs:label "ISO 26262"@en ;
  foaf:maker sto:ISO ;
  sto:hasClassification sto:IDSRAMCertification ;
  sto:hasClassification sto:Safety ;
  sto:hasDBpediaResource <http://dbpedia.org/resource/ISO_26262> ;
  sto:hasDomain sto:ITSecurity ;
  sto:hasOfficialResource <https://www.iso.org/obp/ui/#iso:std:iso:26262:-1:ed-1:v1:en> ;
  sto:hasPublisher sto:ISO ;
  sto:hasWikipediaArticle <https://en.wikipedia.org/wiki/ISO_26262> ;
.
sto:ISO_27000
  a owl:NamedIndividual ;
  a foaf:Document ;
  a sto:Publication ;
  a sto:Standard ;
  terms:creator sto:ISO ;
  rdfs:comment "The ISO/IEC 27000 family of standards helps organizations keep information assets secure. Using this family of standards will help your organization manage the security of assets such as financial information, intellectual property, employee details or information entrusted to you by third parties."@en ;
  rdfs:label "IEC 27000"@en ;
  rdfs:label "ISO 27000"@en ;
  rdfs:label "ISO/IEC 27000"@en ;
  foaf:maker sto:ISO ;
  sto:hasClassification sto:IDSRAMSecurity ;
  sto:hasDBpediaResource <http://dbpedia.org/resource/IEC_27000> ;
  sto:hasMotivation "Provides best practices for information security management. A critical issue for Industry 4.0 "@en ;
  sto:hasOfficialResource <http://www.27000.org/> ;
  sto:hasPublisher sto:ISO ;
  sto:hasTag "Information Security Management Systems"@en ;
  sto:hasWikipediaArticle <https://en.wikipedia.org/wiki/ISO/IEC_27000> ;
.
sto:ISO_27001
  a owl:NamedIndividual ;
  a foaf:Document ;
  a sto:Publication ;
  a sto:Standard ;
  terms:creator sto:IEC ;
  terms:creator sto:ISO ;
  rdfs:comment "ISO/IEC 27001 is an information security standard, part of the ISO/IEC 27000 family of standards."@en ;
  rdfs:label "ISO 27001"@en ;
  rdfs:label "ISO/IEC 27001"@en ;
  foaf:maker sto:IEC ;
  foaf:maker sto:ISO ;
  sto:hasClassification sto:IDSRAMCertification ;
  sto:hasClassification sto:IDSRAMSecurity ;
  sto:hasClassification sto:IIRASecurity ;
  sto:hasDBpediaResource <http://dbpedia.org/resource/ISO/IEC_27001> ;
  sto:hasDomain sto:ITSecurity ;
  sto:hasOfficialResource <https://www.iso.org/isoiec-27001-information-security.html> ;
  sto:hasPublisher sto:IEC ;
  sto:hasPublisher sto:ISO ;
  sto:hasWikipediaArticle <https://en.wikipedia.org/wiki/ISO/IEC_27001> ;
.
sto:ISO_27017
  a owl:NamedIndividual ;
  a foaf:Document ;
  a sto:Publication ;
  a sto:Standard ;
  dc11:title "Code of practice for information security controls based on ISO/IEC 27002 for cloud services"@en ;
  terms:creator sto:IEC ;
  terms:creator sto:ISO ;
  rdfs:comment "The ISO/IEC 270172 standard provides guidance on the information security elements of cloud computing. It assists with the implementation of cloud-specific information security controls, supplementing the guidance in ISO 27000 series standards."@en ;
  rdfs:label "ISO/IEC 27017"@en ;
  foaf:maker sto:IEC ;
  foaf:maker sto:ISO ;
  sto:hasClassification sto:IIRASecurity ;
  sto:hasDBpediaResource <http://dbpedia.org/resource/ISO/IEC_27000-series> ;
  sto:hasDomain sto:ITSecurity ;
  sto:hasOfficialResource <https://www.iso.org/standard/43757.html> ;
  sto:hasPublicationDate "2015-12-01"^^xsd:date ;
  sto:hasPublisher sto:IEC ;
  sto:hasPublisher sto:ISO ;
  sto:hasWikipediaArticle <https://en.wikipedia.org/wiki/ISO/IEC_27000-series> ;
.
sto:ISO_27018
  a owl:NamedIndividual ;
  a foaf:Document ;
  a sto:Publication ;
  a sto:Standard ;
  dc11:title "Information technology -- Security techniques -- Code of practice for protection of personally identifiable information (PII) in public clouds acting as PII processors"@en ;
  terms:creator sto:IEC ;
  terms:creator sto:ISO ;
  rdfs:comment "ISO/IEC 27018:2014 establishes commonly accepted control objectives, controls and guidelines for implementing measures to protect Personally Identifiable Information (PII) in accordance with the privacy principles in ISO/IEC 29100 for the public cloud computing environment."@en ;
  rdfs:label "ISO/IEC 27018"@en ;
  foaf:maker sto:IEC ;
  foaf:maker sto:ISO ;
  sto:hasClassification sto:IIRAPrivacy ;
  sto:hasClassification sto:IIRASecurity ;
  sto:hasDBpediaResource <http://dbpedia.org/resource/ISO/IEC_27000-series> ;
  sto:hasOfficialResource <https://webstore.iec.ch/publication/11302> ;
  sto:hasOfficialResource <https://www.iso.org/standard/61498.html> ;
  sto:hasOpenResource <https://ciostrategycouncil.com/wp-content/uploads/2018/04/W_ISO-IEC-27018-2014.pdf> ;
  sto:hasPublicationDate "2014-08-01"^^xsd:date ;
  sto:hasPublisher sto:IEC ;
  sto:hasPublisher sto:ISO ;
  sto:hasWikipediaArticle <https://en.wikipedia.org/wiki/ISO/IEC_27000-series> ;
.
sto:ISO_27019
  a owl:NamedIndividual ;
  a foaf:Document ;
  a sto:Publication ;
  a sto:Standard ;
  terms:creator sto:ISO ;
  terms:title "Guidance for information security management of power supply control systems based on ISO/IEC 27002"@en ;
  rdfs:comment "The specification serves as a guidance for introducing ISO/IEC 27002 into the energy domain."@en ;
  rdfs:label "ISO 27019"@en ;
  foaf:maker sto:ISO ;
  sto:hasClassification sto:IDSRAMCertification ;
  sto:hasOfficialResource <https://www.beuth.de/de/technische-regel/din-iso-iec-tr-27019/223679647> ;
  sto:hasPublisher sto:ISO ;
.
sto:ISO_27031
  a owl:NamedIndividual ;
  a foaf:Document ;
  a sto:Domain ;
  a sto:Publication ;
  a sto:Standard ;
  dc11:title "Guidelines for information and communication technology readiness for business continuity"@en ;
  terms:creator sto:IEC ;
  terms:creator sto:ISO ;
  rdfs:comment "ISO/IEC 27031:2011 describes the concepts and principles of information and comunication technology (ICT) readiness for business continuity, and provides a framework of methods and processes to identify and specify all aspects (such as performance criteria, design, and implementation) for improving an organization's ICT readiness to ensure business continuity."@en ;
  rdfs:label "ISO/IEC 27031"@en ;
  foaf:maker sto:IEC ;
  foaf:maker sto:ISO ;
  sto:domainName "Business Continuity"@en ;
  sto:hasClassification sto:IIRASecurity ;
  sto:hasOfficialResource <https://webstore.iec.ch/publication/11304> ;
  sto:hasOfficialResource <https://www.iso.org/standard/44374.html> ;
  sto:hasPublicationDate "2011-03-01"^^xsd:date ;
  sto:hasPublisher sto:IEC ;
  sto:hasPublisher sto:ISO ;
.
sto:ISO_27036
  a owl:NamedIndividual ;
  a foaf:Document ;
  a sto:Publication ;
  a sto:Standard ;
  dc11:title "Information security for supplier relationships"@en ;
  terms:creator sto:IEC ;
  terms:creator sto:ISO ;
  rdfs:comment """ISO/IEC 27036-4:2016 provides cloud service customers and cloud service providers with guidance on

a) gaining visibility into the information security risks associated with the use of cloud services and managing those risks effectively, and

b) responding to risks specific to the acquisition or provision of cloud services that can have an information security impact on organizations using these services."""@en ;
  rdfs:label "ISO/IEC 27036"@en ;
  foaf:maker sto:IEC ;
  foaf:maker sto:ISO ;
  sto:hasClassification sto:IIRASecurity ;
  sto:hasDBpediaResource <http://dbpedia.org/resource/ISO/IEC_27000-series> ;
  sto:hasOfficialResource <https://webstore.iec.ch/publication/11314> ;
  sto:hasOfficialResource <https://www.iso.org/standard/59689.html> ;
  sto:hasOpenResource <https://wodzinski.waw.pl/data/_uploaded/file/c059648_ISO_IEC_27036-1_2014.pdf> ;
  sto:hasPublicationDate "2016-10-01"^^xsd:date ;
  sto:hasPublisher sto:IEC ;
  sto:hasPublisher sto:ISO ;
  sto:hasWikipediaArticle <https://en.wikipedia.org/wiki/ISO/IEC_27000-series> ;
.
sto:ISO_29002
  a owl:NamedIndividual ;
  a foaf:Document ;
  a sto:Publication ;
  a sto:Standard ;
  terms:creator sto:ISO ;
  rdfs:comment "ISO 29002 is an interoperability standard, which provides a repository to be used in various ISO XML formats. It is used in ontoML."@en ;
  rdfs:label "ISO 29002"@en ;
  foaf:maker sto:ISO ;
  sto:hasDomain sto:IndustrialProcessMeasurementControl ;
  sto:hasOfficialResource <https://www.iso.org/standard/53617.html> ;
  sto:hasPublicationDate "2010-04-01"^^xsd:date ;
  sto:hasPublisher sto:ISO ;
  sto:relatedTo sto:DIN_SPEC_16592 ;
  sto:relatedTo sto:IEC_61131 ;
  sto:relatedTo sto:IEC_61360 ;
  sto:relatedTo sto:IEC_61499 ;
  sto:relatedTo sto:IEC_61804 ;
  sto:relatedTo sto:IEC_61850 ;
  sto:relatedTo sto:IEC_61987_X ;
  sto:relatedTo sto:IEC_62424 ;
  sto:relatedTo sto:IEC_62453 ;
  sto:relatedTo sto:IEC_62541 ;
  sto:relatedTo sto:IEC_62714 ;
  sto:relatedTo sto:ISO_13584 ;
  sto:relatedTo sto:ISO_14306 ;
  sto:relatedTo sto:ISO_15746 ;
  sto:relatedTo sto:ISO_15926 ;
  sto:relatedTo sto:ISO_18629 ;
  sto:relatedTo sto:ISO_18828-2 ;
  sto:relatedTo sto:ISO_20922 ;
  sto:relatedTo sto:ISO_22400 ;
  sto:relatedTo sto:ISO_29002 ;
  sto:relatedTo sto:ISO_ASTM_52915 ;
  sto:relatedTo sto:ISO_PAS_17506 ;
  sto:relatedTo sto:MathML ;
  sto:relatedTo sto:SysML ;
  sto:relatedTo sto:eClass ;
.
sto:ISO_29100
  a owl:NamedIndividual ;
  a foaf:Document ;
  a sto:Publication ;
  a sto:Standard ;
  terms:creator sto:IEC ;
  terms:creator sto:ISO ;
  terms:title "Privacy framework"@en ;
  rdfs:comment """‘Privacy framework’1 provides a guideline that specifies a common privacy terminology, defines actors and roles in processing PII, describes privacy safeguarding considerations, and includes references to known privacy principles for Information technology.
source: IIC SF"""@en ;
  rdfs:label "ISO/IEC 29100"@en ;
  foaf:maker sto:IEC ;
  foaf:maker sto:ISO ;
  sto:hasClassification sto:IIRAPrivacy ;
  sto:hasClassification sto:IIRASecurity ;
  sto:hasOfficialResource <https://webstore.iec.ch/publication/11322> ;
  sto:hasOfficialResource <https://www.iso.org/standard/45123.html> ;
  sto:hasOpenResource <https://pecb.com/pdf/whitepapers/30-Whitepapers-iso-29100-how-can-organizations-secure-its-privacy-network.pdf> ;
  sto:hasPublicationDate "2011-12-01"^^xsd:date ;
  sto:hasPublisher sto:IEC ;
  sto:hasPublisher sto:ISO ;
.
sto:ISO_29101
  a owl:NamedIndividual ;
  a foaf:Document ;
  a sto:Publication ;
  a sto:Standard ;
  terms:creator sto:IEC ;
  terms:creator sto:ISO ;
  terms:title "Privacy architecture framework"@en ;
  terms:title "Privacy impact assessment–Guidelines"@en ;
  rdfs:comment "Code of practice for protection of personally identifiable information (PII) in public clouds acting as PII processors"@en ;
  rdfs:label "ISO/IEC 29101"@en ;
  foaf:maker sto:IEC ;
  foaf:maker sto:ISO ;
  sto:hasClassification sto:IIRAPrivacy ;
  sto:hasOfficialResource <https://www.iso.org/standard/45124.html> ;
  sto:hasPublicationDate "2013-10-01"^^xsd:date ;
  sto:hasPublisher sto:IEC ;
  sto:hasPublisher sto:ISO ;
.
sto:ISO_29115
  a owl:NamedIndividual ;
  a foaf:Document ;
  a sto:Publication ;
  a sto:Standard ;
  terms:creator sto:IEC ;
  terms:creator sto:ISO ;
  rdfs:label "ISO/IEC 29115"@en ;
  foaf:maker sto:IEC ;
  foaf:maker sto:ISO ;
  sto:hasClassification sto:IIRASecurity ;
  sto:hasPublisher sto:IEC ;
  sto:hasPublisher sto:ISO ;
  sto:hasTargetConcern sto:Authentication ;
  sto:hasTargetConcern sto:Identification ;
.
sto:ISO_29134
  a owl:NamedIndividual ;
  a foaf:Document ;
  a sto:Publication ;
  a sto:Standard ;
  dc11:title "Privacy impact assessment–Guidelines"@en ;
  terms:creator sto:IEC ;
  terms:creator sto:ISO ;
  rdfs:comment "‘Privacy impact assessment–Guidelines’ proposes a methodology to conduct assessments on the impact of privacy."@en ;
  rdfs:label "ISO/IEC 29134"@en ;
  foaf:maker sto:IEC ;
  foaf:maker sto:ISO ;
  sto:hasClassification sto:IIRAPrivacy ;
  sto:hasDomain sto:ITSecurity ;
  sto:hasOfficialResource <https://www.iso.org/standard/62289.html> ;
  sto:hasPublicationDate "2017-06-01"^^xsd:date ;
  sto:hasPublisher sto:IEC ;
  sto:hasPublisher sto:ISO ;
.
sto:ISO_29161
  a owl:NamedIndividual ;
  a foaf:Document ;
  a sto:Publication ;
  a sto:Standard ;
  terms:creator sto:IEC ;
  terms:creator sto:ISO ;
  rdfs:comment "ISO/IEC 29161:2016 establishes a unique identification scheme for the Internet of Things (IoT), based on existing and evolving data structures."@en ;
  rdfs:label "ISO 29161" ;
  foaf:maker sto:IEC ;
  foaf:maker sto:ISO ;
  sto:hasOfficialResource <https://www.iso.org/standard/45240.html> ;
  sto:hasPublicationDate "2016-08-01"^^xsd:date ;
  sto:hasPublisher sto:IEC ;
  sto:hasPublisher sto:ISO ;
.
sto:ISO_29190
  a owl:NamedIndividual ;
  a foaf:Document ;
  a sto:Publication ;
  a sto:Standard ;
  terms:creator sto:IEC ;
  terms:creator sto:ISO ;
  terms:title "Privacy capability assessment model"@en ;
  rdfs:comment "‘Privacy capability assessment model’ provides high-level guidance to organizations about assessing their capability to manage privacy-related processes."@en ;
  rdfs:label "ISO/IEC 29190"@en ;
  foaf:maker sto:IEC ;
  foaf:maker sto:ISO ;
  sto:hasClassification sto:IIRAPrivacy ;
  sto:hasClassification sto:IIRASecurity ;
  sto:hasOfficialResource <https://webstore.iec.ch/publication/23118> ;
  sto:hasOfficialResource <https://www.iso.org/standard/45269.html> ;
  sto:hasOpenResource <https://www.sis.se/api/document/preview/919384/> ;
  sto:hasPublicationDate "2015-08-01"^^xsd:date ;
  sto:hasPublisher sto:IEC ;
  sto:hasPublisher sto:ISO ;
.
sto:ISO_42010
  a owl:NamedIndividual ;
  a foaf:Document ;
  a sto:Domain ;
  a sto:Publication ;
  a sto:Standard ;
  terms:creator sto:IEC ;
  terms:creator sto:ISO ;
  terms:title "Systems and software engineering — Architecture description"@en ;
  rdfs:comment """ISO/IEC/IEEE 42010:2011 defines requirements on the description of system, software and enterprise architectures. It aims to standardise the practice of architecture description by defining standard terms, presenting a conceptual foundation for expressing, communicating and reviewing architectures and specifying requirements that apply to architecture descriptions, architecture frameworks and architecture description languages.

Following its predecessor, IEEE Std 1471, the standard makes a strict distinction between Architectures and Architecture Descriptions.

The description of ISO/IEC/IEEE 42010 in this article is based upon the standard published in 2011."""@en ;
  rdfs:label "ISO/IEC 42010"@en ;
  foaf:maker sto:IEC ;
  foaf:maker sto:ISO ;
  sto:domainName "Reference Architecture Description"@en ;
  sto:hasDBpediaResource <http://dbpedia.org/resource/ISO/IEC_42010> ;
  sto:hasOfficialResource <https://www.iso.org/standard/50508.html> ;
  sto:hasPublisher sto:IEC ;
  sto:hasPublisher sto:ISO ;
  sto:hasWikipediaArticle <https://en.wikipedia.org/wiki/ISO/IEC_42010> ;
.
sto:ISO_50001
  a owl:NamedIndividual ;
  a foaf:Document ;
  a sto:Publication ;
  a sto:Standard ;
  terms:creator sto:ISO ;
  rdfs:comment "Energy management systems – Requirements with guidance for use is a specification created by the International Organization for Standardization (ISO) for an energy management system."@en ;
  rdfs:label "ISO 50001"@en ;
  foaf:maker sto:ISO ;
  sto:hasClassification sto:CrossLevel ;
  sto:hasDBpediaResource <http://dbpedia.org/page/ISO_50001> ;
  sto:hasOfficialResource <https://www.iso.org/iso-50001-energy-management.html> ;
  sto:hasPublisher sto:ISO ;
  sto:hasTargetConcern sto:Energy_management ;
.
sto:ISO_5459
  a owl:NamedIndividual ;
  a foaf:Document ;
  a sto:Publication ;
  a sto:Standard ;
  terms:creator sto:ISO ;
  rdfs:comment "Geometrical product specifications (GPS) -- Geometrical tolerancing -- Datums and datum systems--ISO 5459:2011 specifies terminology, rules and methodology for the indication and understanding of datums and datum systems in technical product documentation"@en ;
  rdfs:label "ISO 5459"@en ;
  foaf:maker sto:ISO ;
  sto:hasClassification sto:ModelingPractice ;
  sto:hasClassification sto:RAMIAssetlayer ;
  sto:hasClassification sto:RAMIProduct ;
  sto:hasDomain sto:M2M ;
  sto:hasOfficialResource <https://www.iso.org/standard/40358.html> ;
  sto:hasPublicationDate "2011-08-01"^^xsd:date ;
  sto:hasPublisher sto:ISO ;
.
sto:ISO_8062-4
  a owl:NamedIndividual ;
  a foaf:Document ;
  a sto:Publication ;
  a sto:Standard ;
  terms:creator sto:ISO ;
  rdfs:comment "Geometrical product specifications (GPS) -- Dimensional and geometrical tolerances for moulded parts -- General tolerances for castings using profile tolerancing in a general datum system"@en ;
  rdfs:label "ISO 8062-4"@en ;
  foaf:maker sto:ISO ;
  sto:hasClassification sto:ProductionSystemModelData ;
  sto:hasClassification sto:RAMIAssetlayer ;
  sto:hasClassification sto:RAMIProduct ;
  sto:hasOfficialResource <https://www.iso.org/standard/60774.html> ;
  sto:hasPublicationDate "2017-07-01"^^xsd:date ;
  sto:hasPublisher sto:ISO ;
  sto:hasTag "Automation systems and integration"@en ;
  sto:relatedTo sto:ISO_10303 ;
  sto:relatedTo sto:ISO_8062-4 ;
.
sto:ISO_9000
  a owl:NamedIndividual ;
  a foaf:Document ;
  a sto:Publication ;
  a sto:Standard ;
  terms:creator sto:ISO ;
  rdfs:comment "The ISO 9000 family of quality management systems standards is designed to help organizations ensure that they meet the needs of customers and other stakeholders while meeting statutory and regulatory requirements related to a product or program."@en ;
  rdfs:label "ISO 9000"@en ;
  foaf:maker sto:ISO ;
  sto:hasClassification sto:CrossLevel ;
  sto:hasClassification sto:IDSRAMCertification ;
  sto:hasDBpediaResource <http://dbpedia.org/page/ISO_9000> ;
  sto:hasOfficialResource <https://www.iso.org/iso-9001-quality-management.html> ;
  sto:hasPublisher sto:ISO ;
  sto:hasTargetConcern sto:QualityOfService ;
  sto:hasWikipediaArticle <https://en.wikipedia.org/wiki/ISO_9000> ;
.
sto:ISO_9594
  a owl:NamedIndividual ;
  a foaf:Document ;
  a sto:Publication ;
  a sto:Standard ;
  terms:creator sto:ISO ;
  rdfs:label "ISO/IEC 9594"@en ;
  rdfs:label "X.509"@en ;
  foaf:maker sto:ISO ;
  sto:hasClassification sto:DataSovereignty ;
  sto:hasClassification sto:IDSRAMCertification ;
  sto:hasClassification sto:IDSRAMSecurity ;
  sto:hasOfficialResource <https://tools.ietf.org/html/rfc5280> ;
  sto:hasPublisher sto:ISO ;
.
sto:ISO_9594-8
  a owl:NamedIndividual ;
  a foaf:Document ;
  a sto:Publication ;
  a sto:Standard ;
  terms:creator sto:ISO ;
  terms:title "Information technology -- Open Systems Interconnection -- The Directory -- Part 8: Public-key and attribute certificate frameworks"@en ;
  rdfs:comment """ISO/IEC 9594-8:2017 addresses some of the security requirements in the areas of authentication and other security services through the provision of a set of frameworks upon which full services can be based. Specifically, this Recommendation | International Standard defines frameworks for:

- public-key certificates; and

- attribute certificates."""@en ;
  rdfs:label "ISO/IEC 9594-8"@en ;
  rdfs:seeAlso <https://tools.ietf.org/html/rfc5280> ;
  foaf:maker sto:ISO ;
  sto:hasClassification sto:DataSovereignty ;
  sto:hasClassification sto:IDSRAMCertification ;
  sto:hasClassification sto:IDSRAMSecurity ;
  sto:hasOfficialResource <https://tools.ietf.org/html/rfc5280> ;
  sto:hasOfficialResource <https://www.iso.org/standard/72557.html> ;
  sto:hasPublisher sto:ISO ;
.
sto:ISO_ASTM_52915
  a owl:NamedIndividual ;
  a foaf:Document ;
  a sto:Publication ;
  a sto:Standard ;
  terms:creator sto:ISO ;
  rdfs:comment "ISO ASTM 52915:2016 provides the specification for the Additive Manufacturing File Format (AMF), an interchange format to address the current and future needs of additive manufacturing technology."@en ;
  rdfs:label "ISO ASTM 52915"@en ;
  foaf:maker sto:ISO ;
  sto:hasClassification rami:Engineering ;
  sto:hasClassification rami:Identification ;
  sto:hasClassification sto:ProductionSystemEngineering ;
  sto:hasClassification sto:RAMIAssetlayer ;
  sto:hasClassification sto:RAMIProduct ;
  sto:hasDomain sto:IndustrialAutomation ;
  sto:hasOfficialResource <https://www.iso.org/standard/60572.html> ;
  sto:hasPublicationDate "2016-02-01"^^xsd:date ;
  sto:hasPublisher sto:ISO ;
  sto:relatedTo sto:DIN_SPEC_16592 ;
  sto:relatedTo sto:IEC_61131 ;
  sto:relatedTo sto:IEC_61360 ;
  sto:relatedTo sto:IEC_61499 ;
  sto:relatedTo sto:IEC_61804 ;
  sto:relatedTo sto:IEC_61850 ;
  sto:relatedTo sto:IEC_61987_X ;
  sto:relatedTo sto:IEC_62424 ;
  sto:relatedTo sto:IEC_62453 ;
  sto:relatedTo sto:IEC_62541 ;
  sto:relatedTo sto:IEC_62714 ;
  sto:relatedTo sto:ISO_13584 ;
  sto:relatedTo sto:ISO_14306 ;
  sto:relatedTo sto:ISO_15746 ;
  sto:relatedTo sto:ISO_15926 ;
  sto:relatedTo sto:ISO_18629 ;
  sto:relatedTo sto:ISO_18828-2 ;
  sto:relatedTo sto:ISO_20922 ;
  sto:relatedTo sto:ISO_22400 ;
  sto:relatedTo sto:ISO_29002 ;
  sto:relatedTo sto:ISO_ASTM_52915 ;
  sto:relatedTo sto:ISO_PAS_17506 ;
  sto:relatedTo sto:MathML ;
  sto:relatedTo sto:SysML ;
  sto:relatedTo sto:eClass ;
.
sto:ISO_PAS_17506
  a owl:NamedIndividual ;
  a foaf:Document ;
  a sto:Publication ;
  a sto:Standard ;
  terms:creator sto:ISO ;
  dul:isComponentOf sto:IEC_62714 ;
  rdfs:comment "ISO-PAS 17506-2012 describes the COLLADA schema. COLLADA is a COLLAborative Design Activity that defines an XML-based schema to enable 3D authoring applications to freely exchange digital assets without loss of information, enabling multiple software packages to be combined into extremely powerful tool chains."@en ;
  rdfs:comment "SO/PAS 17506:2012 describes the COLLADA schema. COLLADA is a COLLAborative Design Activity that defines an XML-based schema to enable 3D authoring applications to freely exchange digital assets without loss of information, enabling multiple software packages to be combined into extremely powerful tool chains. The purpose of ISO/PAS 17506:2012 is to provide a specification for the COLLADA schema in sufficient detail to enable software developers to create tools to process COLLADA resources. In particular, it is relevant to those who import to or export from digital content creation (DCC) applications, 3D interactive applications and tool chains, prototyping tools, real-time visualization applications such as those used in the video game and movie industries, and CAD tools. ISO/PAS 17506:2012 covers the initial design and specifications of the COLLADA schema, as well as a minimal set of requirements for COLLADA exporters. "@en ;
  rdfs:label "ISO PAS 17506"@en ;
  foaf:maker sto:ISO ;
  sto:hasDBpediaResource <http://dbpedia.org/resource/COLLADA> ;
  sto:hasDeveloper sto:ISO ;
  sto:hasOfficialResource <https://www.iso.org/standard/59902.html> ;
  sto:hasPublisher sto:ISO ;
  sto:hasWikipediaArticle <https://en.wikipedia.org/wiki/COLLADA> ;
  sto:relatedTo sto:DIN_SPEC_16592 ;
  sto:relatedTo sto:IEC_61131 ;
  sto:relatedTo sto:IEC_61360 ;
  sto:relatedTo sto:IEC_61499 ;
  sto:relatedTo sto:IEC_61804 ;
  sto:relatedTo sto:IEC_61850 ;
  sto:relatedTo sto:IEC_61987_X ;
  sto:relatedTo sto:IEC_62424 ;
  sto:relatedTo sto:IEC_62453 ;
  sto:relatedTo sto:IEC_62541 ;
  sto:relatedTo sto:IEC_62714 ;
  sto:relatedTo sto:ISO_13584 ;
  sto:relatedTo sto:ISO_14306 ;
  sto:relatedTo sto:ISO_15746 ;
  sto:relatedTo sto:ISO_15926 ;
  sto:relatedTo sto:ISO_18629 ;
  sto:relatedTo sto:ISO_18828-2 ;
  sto:relatedTo sto:ISO_20922 ;
  sto:relatedTo sto:ISO_22400 ;
  sto:relatedTo sto:ISO_29002 ;
  sto:relatedTo sto:ISO_ASTM_52915 ;
  sto:relatedTo sto:ISO_PAS_17506 ;
  sto:relatedTo sto:MathML ;
  sto:relatedTo sto:SysML ;
  sto:relatedTo sto:eClass ;
.
sto:ISO_TS_14649-201
  a owl:NamedIndividual ;
  a foaf:Document ;
  a sto:Publication ;
  a sto:Standard ;
  terms:creator sto:ISO ;
  rdfs:comment "SO/TS 14649-201:2011 specifies the technology-specific machine tool description data elements needed as process data for manufacturing and machine characteristics. The machine tool descriptions covered in this schema are, initially, milling machines, machining centres, turning machines and multi-tasking machines.ISO/TS 14649-201:2011 is not intended to replace existing machine tool description standards, but to cover the specific needs of manufacturing resource description for manufacturing needs in the technologies described in ISO 14649."@en ;
  rdfs:label "ISO TS 14649-201"@en ;
  foaf:maker sto:ISO ;
  sto:hasClassification rami:Configuration ;
  sto:hasClassification rami:Engineering ;
  sto:hasClassification rami:Safety ;
  sto:hasClassification sto:ProductionSystemModelData ;
  sto:hasClassification sto:RAMIAssetlayer ;
  sto:hasClassification sto:RAMIIntegrationLayer ;
  sto:hasClassification sto:RAMIProduct ;
  sto:hasDomain sto:IndustrialAutomation ;
  sto:hasOfficialResource <https://www.iso.org/standard/60042.html> ;
  sto:hasPublicationDate "2011-12-01"^^xsd:date ;
  sto:hasPublisher sto:ISO ;
.
sto:ITManager
  rdfs:comment " An IT manager is responsible for the functioning of the IT services of an organisation." ;
  rdfs:label "IT Manager"@en ;
  rdfs:seeAlso "IIC:PUB:G1:V1.80:20170131" ;
  rdfs:type sto:Stakeholder ;
  skos:note "Publications referred: 'IIC:PUB:G1:V1.80:20170131' '1.5 AUDIENCE' 'Page 7' " ;
  sto:hasWikipediaArticle "https://en.wikipedia.org/wiki/Information_technology_management#IT_managers" ;
.
sto:ITSecurity
  a owl:NamedIndividual ;
  a sto:Domain ;
  rdfs:label "IT Security"@en ;
  skos:altLabel "Information Security Management"@en ;
.
sto:IVRA
  a owl:NamedIndividual ;
  a sto:ArchitectureDescription ;
  a sto:StandardizationFramework ;
  dul:associatedWith sto:Ivi ;
  rdfs:comment "The Reference Architecture (IVRA) of the Industrial Value Chain Initive (IVI) proposes a system architecture for the manufactoring domain targeting interoperability and communicational aspects."@en ;
  rdfs:label "Industrial Value Chain Reference Architecture"@en ;
  skos:altLabel "IVRA"@en ;
  sto:hasOfficialResource <https://iv-i.org/wp-test/wp-content/uploads/2017/09/doc_161208_Industrial_Value_Chain_Reference_Architecture.pdf> ;
.
sto:Identification
  a owl:NamedIndividual ;
  a sto:Concern ;
  a sto:StandardClassification ;
  dul:associatedWith rami:Identification ;
  dul:associatedWith sto:IEC_24760 ;
  dul:associatedWith sto:IEC_62443 ;
  dul:associatedWith sto:ISO_24760 ;
  rdfs:comment "The concern how to identify a participant (client, endpoint etc.) in the internet."@en ;
  rdfs:label "Identification"@en ;
  rdfs:seeAlso "IoT-A Requirement UNI.030" ;
  rdfs:seeAlso "IoT-A Requirement UNI.425" ;
  rdfs:seeAlso "IoT-A Requirement UNI.428" ;
  rdfs:seeAlso "IoT-A Requirement UNI.622" ;
  skos:note "Publications referred: '<https://doi.org/10.1016/j.jksuci.2016.10.003>' 'Survey on domain specific IoT architectures' 'Page 299'" ;
  sto:alignsWith rami:Identification ;
  sto:alignsWith sto:IEC_24760 ;
  sto:alignsWith sto:IEC_62443 ;
  sto:alignsWith sto:ISO_24760 ;
  sto:hasDBpediaResource <http://dbpedia.org/resource/Identification_(information)> ;
  sto:supports sto:IdentityManagement ;
.
sto:IdentityManagement
  a owl:NamedIndividual ;
  a sto:Concern ;
  terms:creator sto:sebastian ;
  rdfs:comment "In computer security, identity and access management (IAM) is the security and business discipline that \"enables the right individuals to access the right resources at the right times and for the right reasons\".It addresses the need to ensure appropriate access to resources across increasingly heterogeneous technology environments and to meet increasingly rigorous compliance requirements. (source: wikipedia)"@en ;
  rdfs:label "Identity Management"@en ;
  rdfs:seeAlso "IoT-A Requirement UNI.048" ;
  rdfs:seeAlso "IoT-A Requirement UNI.432" ;
  rdfs:seeAlso "https://ieeexplore.ieee.org/document/6188257"@en ;
  rdfs:seeAlso "https://ieeexplore.ieee.org/document/7488250" ;
  rdfs:seeAlso "https://ieeexplore.ieee.org/document/7919553"@en ;
  sto:hasDBpediaResource <http://dbpedia.org/resource/Identity_management> ;
  sto:supports sto:NonRepudiation ;
.
sto:IicfConnectivityLayer
  a owl:Class ;
  rdfs:comment "Connectivity Layer of the Internet Connectivity Framework"@en ;
  rdfs:isDefinedBy <https://www.iiconsortium.org/pdf/IIC_PUB_G5_V1.01_PB_20180228.pdf> ;
  rdfs:label "IICF Connectivity Layer"@en ;
  rdfs:subClassOf sto:StandardClassification ;
  rdfs:subClassOf [
      a owl:Restriction ;
      owl:hasValue sto:IIRAConnectivity ;
      owl:onProperty dul:isPartOf ;
    ] ;
.
sto:IicfConnectivityLayerAnno
  a <https://www.w3.org/ns/oaAnnotation> ;
  <https://www.w3.org/ns/oahasBody> sto:IicfConnectivityLayer ;
  <https://www.w3.org/ns/oahasTarget> [
      a <https://www.w3.org/ns/oaSpecificResource> ;
      terms:format "pdf" ;
      <https://www.w3.org/ns/oahasSelector> [
          a <https://www.w3.org/ns/oaRangeSelector> ;
          <https://www.w3.org/ns/oahasEndSelector> [
              a <https://www.w3.org/ns/oaXPathSelector> ;
              rdf:value "Page 17" ;
            ] ;
          <https://www.w3.org/ns/oahasStartSelector> [
              a <https://www.w3.org/ns/oaXPathSelector> ;
              rdf:value "Page 14" ;
            ] ;
        ] ;
      <https://www.w3.org/ns/oahasSource> sto:The_Industrial_Internet_of_Things_Volume_G5_Connectivity_Framework ;
    ] ;
.
sto:IndustrialAutomation
  a owl:NamedIndividual ;
  a sto:Domain ;
  rdfs:comment "Industrial automation deals primarily with the automation of manufacturing, quality control and material handling processes. General purpose controllers for industrial processes include Programmable logic controllers, stand-alone I/O modules, and computers. Industrial automation is to replace the decision making of humans and manual command-response activities with the use of mechanized equipment and logical programming commands. One trend is increased use of Machine vision to provide automatic inspection and robot guidance functions, another is a continuing increase in the use of robots. Industrial automation is simply done at the industrial level."@en ;
  rdfs:label "Industrial Automation"@en ;
  sto:domainName "Industrial Automation"@en ;
  sto:hasDBpediaResource <http://dbpedia.org/resource/Category:IndustrialAutomation> ;
  sto:hasWikipediaArticle <https://en.wikipedia.org/wiki/Automation> ;
.
sto:IndustrialProcessMeasurementControl
  a owl:NamedIndividual ;
  a sto:Domain ;
  rdfs:comment "Industrial process measurement and control"@en ;
  sto:domainName "Industrial process measurement and control"@en ;
.
sto:Industrial_Internet_Architecture_Version_1
  a <https://www.w3.org/ns/oaSpecificResource> ;
  rdfs:label "Industrial Internet Architecture Version 1"@en ;
  sto:hasOpenResource <http://en.aii-alliance.org/uploadfile/2017/0307/Industrial.pdf> ;
.
sto:Industrial_Internet_of_Things_Volume_G4_Security_Framework
  a <https://www.w3.org/ns/oaSpecificResource> ;
  rdfs:label "Industrial Internet of Things Volume G4: Security Framework"@en ;
  skos:note "Industrial Internet of Things Volume G4: Security Framework IIC:PUB:G4:V1.0:PB:20160926" ;
  sto:hasOpenResource <https://www.iiconsortium.org/pdf/IIC_PUB_G4_V1.00_PB-3.pdf> ;
.
sto:Industrial_Value_Chain_Reference_Architecture_IVRA
  a <https://www.w3.org/ns/oaSpecificResource> ;
  rdfs:label "Industrial Value Chain Reference Architecture (IVRA)"@en ;
  skos:note "Industrial Value Chain Reference Architecture (IVRA) Industrial Value Chain Initiative " ;
  sto:hasOpenResource <https://iv-i.org/docs/doc_161208_Industrial_Value_Chain_Reference_Architecture.pdf> ;
.
sto:Industrial_Value_Chain_Reference_Architecture_IVRA_Next
  a <https://www.w3.org/ns/oaSpecificResource> ;
  rdfs:label "Industrial Value Chain Reference Architecture (IVRA)- Next"@en ;
  skos:note "Industrial Value Chain Reference Architecture (IVRA) Industrial Value Chain Initiative Next" ;
  sto:hasOpenResource <https://www.innovation4.cn/library/r26680> ;
.
sto:InformationSecurity
  a owl:NamedIndividual ;
  a sto:Concern ;
  terms:creator sto:SebastianBader ;
  rdfs:comment ""@en ;
  rdfs:label "Information Security"@en ;
  rdfs:seeAlso "https://ieeexplore.ieee.org/document/8552311"@en ;
  sto:supports sto:Security ;
.
sto:Information_Privacy
  a owl:NamedIndividual ;
  a sto:Concern ;
  terms:creator sto:MuhammadUsman ;
  rdfs:comment """The IoT utilizes different sort of object distinguishing proof advancements, e.g., RFID, 2D-standardized tags and so forth. Since each kind of day by day use articles
will convey these recognizable proof labels and insert the particular object data, it is important to take legal protection measures and prevent unauthorized access."""@en ;
  rdfs:label "Information Privacy"@en ;
  rdfs:seeAlso "https://ieeexplore.ieee.org/document/6188257"@en ;
  sto:hasWikipediaArticle "https://en.wikipedia.org/wiki/Information_privacy"@en ;
  sto:supports sto:Privacy ;
.
sto:IntegrityProtection
  a owl:NamedIndividual ;
  a sto:Concern ;
  terms:creator sto:sebastian ;
  <http://voag.linkedmodel.org/voag#hasStakeholder> "Device/Service Owner" ;
  rdfs:comment "In telecommunications, the term system integrity has the following meanings: 1. * That condition of a system wherein its mandated operational and technical parameters are within the prescribed limits. 2. * The quality of an AIS when it performs its intended function in an unimpaired manner, free from deliberate or inadvertent unauthorized manipulation of the system. 3. * The state that exists when there is complete assurance that under all conditions an IT system is based on the logical correctness and reliability of the operating system, the logical completeness of the hardware and software that implement the protection mechanisms, and data integrity. (source: wikipedia)"@en ;
  rdfs:comment "Integrity protection and verification of the software stack installed; local integrity protection would be something like trusted boot; remote integrity verification means support for remote attestation."@en ;
  rdfs:label "Integrity Protection and Verification"@en ;
  rdfs:seeAlso "IoT-A Requirement UNI.066" ;
  rdfs:seeAlso "IoT-A Requirement UNI.603" ;
  rdfs:seeAlso "IoT-A Requirement UNI.620" ;
  skos:altLabel "Attestation"@en ;
  sto:hasDBpediaResource <http://dbpedia.org/resource/System_integrity> ;
  sto:supports sto:DeviceSecurity ;
.
sto:InterfaceNetworksDevices
  a owl:NamedIndividual ;
  a sto:FiwareChapter ;
  a sto:StandardClassification ;
  terms:creator sto:sebastian ;
  dul:associatedWith sto:IDSRAMProcessLayer ;
  dul:associatedWith sto:IDSRAMSystemLayer ;
  dul:associatedWith sto:NgsiLdArchitecture ;
  dul:associatedWith sto:OpenDaylight ;
  rdfs:comment """The GEs in the I2ND chapter provide three sets of functionalities.

The first is an advanced integration middleware to be used by all FIWARE GEs with high performance communication needs

Open networking elements enable cloud network application developers to build value-added services in private, enterprise and public settings.

The third set of functionalities enables the management of robots by means of platform components and interfaces towards other FIWARE GEs, allowing users to develop smarter and faster robotic applications."""@en ;
  rdfs:label "FIWARE Interface to Networks and Devices"@en ;
  sto:alignsWith sto:IDSRAMProcessLayer ;
  sto:alignsWith sto:IDSRAMSystemLayer ;
  sto:alignsWith sto:NgsiLdArchitecture ;
  sto:frames sto:CloudComputing ;
  sto:frames sto:DataDescription ;
  sto:frames sto:DataProcessing ;
  sto:frames sto:DataSovereignty ;
  sto:frames sto:EndpointDescription ;
  sto:frames sto:EndpointInvocation ;
  sto:frames sto:Interoperability ;
  sto:frames sto:IoT ;
  sto:frames sto:Privacy ;
  sto:frames sto:QualityOfService ;
  sto:frames sto:Scalability ;
  sto:frames sto:Security ;
  sto:frames sto:SemanticInteroperability ;
  sto:frames sto:ServiceComposition ;
  sto:frames sto:ServiceDescription ;
  sto:frames sto:ServiceOrchestration ;
  sto:frames sto:SyntacticInteroperability ;
  sto:frames sto:Trustworthiness ;
  sto:isDescribedin sto:FIWARE ;
.
sto:InterfaceNetworksDevicesAnno
  a <https://www.w3.org/ns/oaAnnotation> ;
  <https://www.w3.org/ns/oahasBody> sto:InterfaceNetworksDevices ;
  <https://www.w3.org/ns/oahasTarget> [
      a <https://www.w3.org/ns/oaSpecificResource> ;
      <https://www.w3.org/ns/oahasSource> <https://forge.fiware.org/plugins/mediawiki/wiki/fiware/index.php/Interface_to_Networks_and_Devices_(I2ND)_Architecture_R3> ;
    ] ;
.
sto:InternationalClassificationForStandards
  a owl:Class ;
  a owl:NamedIndividual ;
  rdfs:comment "Serves as a structure for catalogues of international, regional and national standards and other normative documents, and as a basis for standing-order systems."@en ;
  rdfs:label "International Classification For Standards"@en ;
  rdfs:seeAlso <https://www.iso.org/publication/PUB100033.html> ;
  sto:abbreviation "ICS"@en ;
  sto:hasOfficialResource <https://www.iso.org/publication/PUB100033.html> ;
.
sto:Interoperability
  a owl:NamedIndividual ;
  a sto:Concern ;
  <http://voag.linkedmodel.org/voag#hasStakeholder> <https://w3id.org/i40/GeneralMAnager> ;
  <http://voag.linkedmodel.org/voag#hasStakeholder> <https://www.wikidata.org/wiki/Q1548249> ;
  rdfs:comment "A systems ability to connect with other systems."@en ;
  rdfs:comment "Interoperability refers to the ability of two or more devices from the same vendor, or different vendors, to exchange information and use that information for correct co-operation [IEC61850-2010]."@en ;
  rdfs:label "Interoperability"@en ;
  rdfs:seeAlso "IoT-A Requirement UNI.008" ;
  rdfs:seeAlso "IoT-A Requirement UNI.010" ;
  rdfs:seeAlso "IoT-A Requirement UNI.023" ;
  rdfs:seeAlso "IoT-A Requirement UNI.042" ;
  rdfs:seeAlso "IoT-A Requirement UNI.047" ;
  rdfs:seeAlso "IoT-A Requirement UNI.093" ;
  rdfs:seeAlso "IoT-A Requirement UNI.094" ;
  rdfs:seeAlso "IoT-A Requirement UNI.232" ;
  rdfs:seeAlso "IoT-A Requirement UNI.712" ;
  rdfs:seeAlso "https://dl.acm.org/citation.cfm?doid=3266237.3266263"@en ;
  rdfs:seeAlso "https://ieeexplore.ieee.org/document/8249113"@en ;
  sto:hasDBpediaResource <http://dbpedia.org/resource/Interoperability> ;
.
sto:IoT
  a owl:NamedIndividual ;
  a sto:Concern ;
  terms:title "Internet of Things"@en ;
  rdfs:comment "The internet of things (IoT) is the internetworking of physical devices, vehicles (also referred to as \"connected devices\" and \"smart devices\"), buildings and other items—embedded with electronics, software, sensors, actuators, and network connectivity that enable these objects to collect and exchange data. (source: wikipedia)"@en ;
  rdfs:label "IoT"@en ;
  rdfs:seeAlso "IoT-A Requirement UNI.213" ;
  sto:hasDBpediaResource <http://dbpedia.org/resource/Internet_of_things> ;
.
sto:IoTA
  a owl:NamedIndividual ;
  a foaf:Organization ;
  a sto:IIoTConsortium ;
  terms:title "IoT Architecture"@en ;
  dul:associatedWith sto:IotaReferenceArchitecture ;
  rdfs:comment "After much discussion about the core concepts of the IoT for several years, in 2009 a group of researchers from more than 20 large industrial companies and research institutions joined forces to lay the foundation for the much needed common ground or a common “architecture” for the Internet of Things: the IoTArchitecture project (IoT-A) was born. IoT-A has become the European Commission’s flagship project in the European Union’s Seventh Framework Program for Research and Development with respect to establishing an architecture for the Internet of Things."@en ;
  rdfs:label "IoT-A"@en ;
  rdfs:seeAlso <http://open-platforms.eu/standard_protocol/iot-a-architectural-reference-model/> ;
.
sto:IoTivity
  a owl:NamedIndividual ;
  a foaf:Document ;
  a sto:Publication ;
  a sto:TechnicalSpecification ;
  terms:creator sto:sebastian ;
  rdfs:comment "IoTivity is an open source project hosted by the Linux Foundation, and sponsored by the OIC. (source: https://www.postscapes.com/internet-of-things-protocols/)"@en ;
  rdfs:label "IoTivity"@en ;
  sto:hasOfficialResource <https://www.iotivity.org/> ;
.
sto:IotaAvailabilityResilience
  a owl:NamedIndividual ;
  a sto:IotaPerspective ;
  a sto:StandardClassification ;
  dul:associatedWith sto:Security ;
  rdfs:label "IoT-A Availability and Resilience"@en ;
  sto:alignsWith sto:Security ;
  sto:frames sto:Availability ;
  sto:frames sto:Resilience ;
  sto:frames sto:Security ;
  sto:frames sto:Trustworthiness ;
  sto:isDescribedin sto:IotaReferenceArchitecture ;
.
sto:IotaAvailabilityResilienceAnno
  a <https://www.w3.org/ns/oaAnnotation> ;
  <https://www.w3.org/ns/oahasBody> sto:IotaAvailabilityResilience ;
  <https://www.w3.org/ns/oahasTarget> [
      a <https://www.w3.org/ns/oaSpecificResource> ;
      terms:format "pdf" ;
      <https://www.w3.org/ns/oahasSelector> [
          a <https://www.w3.org/ns/oaRangeSelector> ;
          <https://www.w3.org/ns/oahasEndSelector> [
              a <https://www.w3.org/ns/oaXPathSelector> ;
              rdf:value "Page 156" ;
            ] ;
          <https://www.w3.org/ns/oahasStartSelector> [
              a <https://www.w3.org/ns/oaXPathSelector> ;
              rdf:value "Page 155" ;
            ] ;
        ] ;
      <https://www.w3.org/ns/oahasSource> sto:Final_architectural_reference_model_for_the_IoT_v3_0 ;
    ] ;
.
sto:IotaDeploymentOperationViewpoint
  a owl:NamedIndividual ;
  a sto:StandardClassification ;
  a sto:Viewpoint ;
  terms:creator sto:sebastian ;
  dul:associatedWith sto:IDSRAMSystemLayer ;
  dul:associatedWith sto:IIRAImplementationViewpoint ;
  rdfs:label "IoT-A Deployment and Operation"@en ;
  sto:alignsWith sto:IDSRAMSystemLayer ;
  sto:alignsWith sto:IIRAImplementationViewpoint ;
  sto:frames rami:EnergyEfficiency ;
  sto:frames sto:DynamicAdjustability ;
  sto:frames sto:Evolvability ;
  sto:frames sto:ServiceChoreography ;
  sto:frames sto:ServiceComposition ;
  sto:frames sto:ServiceDeployment ;
  sto:frames sto:ServiceLifecycleManagement ;
  sto:frames sto:ServiceOrchestration ;
  sto:isDescribedin sto:IotaReferenceArchitecture ;
.
sto:IotaDeploymentOperationViewpointAnno
  a <https://www.w3.org/ns/oaAnnotation> ;
  <https://www.w3.org/ns/oahasBody> sto:IotaDeploymentOperationViewpoint ;
  <https://www.w3.org/ns/oahasTarget> [
      a <https://www.w3.org/ns/oaSpecificResource> ;
      terms:format "pdf" ;
      <https://www.w3.org/ns/oahasSelector> [
          a <https://www.w3.org/ns/oaRangeSelector> ;
          <https://www.w3.org/ns/oahasEndSelector> [
              a <https://www.w3.org/ns/oaXPathSelector> ;
              rdf:value "Page 149" ;
            ] ;
          <https://www.w3.org/ns/oahasStartSelector> [
              a <https://www.w3.org/ns/oaXPathSelector> ;
              rdf:value "Page 141" ;
            ] ;
        ] ;
      <https://www.w3.org/ns/oahasSource> sto:Final_architectural_reference_model_for_the_IoT_v3_0 ;
    ] ;
.
sto:IotaEvolutionInteroperability
  a owl:NamedIndividual ;
  a sto:IotaPerspective ;
  a sto:StandardClassification ;
  dul:associatedWith sto:IIRAConnectivity ;
  dul:associatedWith sto:RAMIIntegrationLayer ;
  rdfs:label "IoT-A Evolution and Interoperability"@en ;
  sto:alignsWith sto:IIRAConnectivity ;
  sto:alignsWith sto:RAMIIntegrationLayer ;
  sto:frames sto:DynamicAdjustability ;
  sto:frames sto:Evolvability ;
  sto:frames sto:Interoperability ;
  sto:frames sto:ServiceChoreography ;
  sto:frames sto:ServiceComposition ;
  sto:frames sto:ServiceOrchestration ;
  sto:isDescribedin sto:IotaReferenceArchitecture ;
.
sto:IotaEvolutionInteroperabilityAnno
  a <https://www.w3.org/ns/oaAnnotation> ;
  <https://www.w3.org/ns/oahasBody> sto:IotaEvolutionInteroperability ;
  <https://www.w3.org/ns/oahasTarget> [
      a <https://www.w3.org/ns/oaSpecificResource> ;
      terms:format "pdf" ;
      <https://www.w3.org/ns/oahasSelector> [
          a <https://www.w3.org/ns/oaRangeSelector> ;
          <https://www.w3.org/ns/oahasEndSelector> [
              a <https://www.w3.org/ns/oaXPathSelector> ;
              rdf:value "Page 151" ;
            ] ;
          <https://www.w3.org/ns/oahasStartSelector> [
              a <https://www.w3.org/ns/oaXPathSelector> ;
              rdf:value "Page 150" ;
            ] ;
        ] ;
      <https://www.w3.org/ns/oahasSource> sto:Final_architectural_reference_model_for_the_IoT_v3_0 ;
    ] ;
.
sto:IotaFunctionalViewpoint
  a owl:NamedIndividual ;
  a sto:StandardClassification ;
  a sto:Viewpoint ;
  terms:creator sto:sebastian ;
  dul:associatedWith sto:IDSRAMProcessLayer ;
  dul:associatedWith sto:IDSRAMSecurity ;
  dul:associatedWith sto:IIRAFunctionalViewpoint ;
  dul:associatedWith sto:RAMIAssetlayer ;
  dul:associatedWith sto:RAMIFunctional ;
  rdfs:label "IoT-A Functional Viewpoint"@en ;
  sto:alignsWith sto:IDSRAMProcessLayer ;
  sto:alignsWith sto:IDSRAMSecurity ;
  sto:alignsWith sto:IIRAFunctionalViewpoint ;
  sto:alignsWith sto:RAMIAssetlayer ;
  sto:alignsWith sto:RAMIFunctionalLayer ;
  sto:frames rami:Configuration ;
  sto:frames rami:ProcessPlanning ;
  sto:frames sto:Authentication ;
  sto:frames sto:Authorization ;
  sto:frames sto:Communication ;
  sto:frames sto:DataSovereignty ;
  sto:frames sto:IdentityManagement ;
  sto:frames sto:Privacy ;
  sto:frames sto:Security ;
  sto:frames sto:ServiceChoreography ;
  sto:frames sto:ServiceComposition ;
  sto:frames sto:ServiceOrchestration ;
  sto:frames sto:ThingRepresentation ;
  sto:frames sto:Trustworthiness ;
  sto:frames sto:VirtualEntity ;
  sto:isDescribedin sto:IotaReferenceArchitecture ;
.
sto:IotaFunctionalViewpointAnno
  a <https://www.w3.org/ns/oaAnnotation> ;
  <https://www.w3.org/ns/oahasBody> sto:IotaFunctionalViewpoint ;
  <https://www.w3.org/ns/oahasTarget> [
      a <https://www.w3.org/ns/oaSpecificResource> ;
      terms:format "pdf" ;
      <https://www.w3.org/ns/oahasSelector> [
          a <https://www.w3.org/ns/oaRangeSelector> ;
          <https://www.w3.org/ns/oahasEndSelector> [
              a <https://www.w3.org/ns/oaXPathSelector> ;
              rdf:value "Page 126" ;
            ] ;
          <https://www.w3.org/ns/oahasStartSelector> [
              a <https://www.w3.org/ns/oaXPathSelector> ;
              rdf:value "Page 105" ;
            ] ;
        ] ;
      <https://www.w3.org/ns/oahasSource> sto:Final_architectural_reference_model_for_the_IoT_v3_0 ;
    ] ;
.
sto:IotaInformationViewpoint
  a owl:NamedIndividual ;
  a sto:StandardClassification ;
  a sto:Viewpoint ;
  terms:creator sto:sebastian ;
  dul:associatedWith sto:IDSRAMInformationLayer ;
  dul:associatedWith sto:IDSRAMProcessLayer ;
  dul:associatedWith sto:IIRAControlDomain ;
  dul:associatedWith sto:IIRAOperationsDomain ;
  dul:associatedWith sto:InformationDomain ;
  dul:associatedWith sto:RAMICommunicationlayer ;
  rdfs:comment "One of the main purposes of connected and smart objects in the IoT is the exchange of information between each other and also with external systems. Therefore the way how to define, structure, store, process, manage and exchange information is very important. The information view helps to generate an overview about static information structure and dynamic information flow. (source: Bassi et al.: Enabling Things to Talk)"@en ;
  rdfs:label "IoT-A Information Viewpoint"@en ;
  sto:alignsWith sto:IDSRAMInformationLayer ;
  sto:alignsWith sto:IDSRAMProcessLayer ;
  sto:alignsWith sto:IIRAControlDomain ;
  sto:alignsWith sto:IIRAOperationsDomain ;
  sto:alignsWith sto:InformationDomain ;
  sto:alignsWith sto:RAMICommunicationlayer ;
  sto:frames sto:Communication ;
  sto:frames sto:DataAnalytics ;
  sto:frames sto:DataAtRest ;
  sto:frames sto:DataInMotion ;
  sto:frames sto:DataLifecycleManagment ;
  sto:frames sto:EndpointInvocation ;
  sto:frames sto:Interoperability ;
  sto:frames sto:SemanticInteroperability ;
  sto:frames sto:ServiceDescription ;
  sto:frames sto:SyntacticInteroperability ;
  sto:frames sto:ThingRepresentation ;
  sto:frames sto:VirtualEntity ;
  sto:hasOfficialResource <http://doi.org/10.1007/978-3-642-40403-0> ;
  sto:isDescribedin sto:IotaReferenceArchitecture ;
.
sto:IotaInformationViewpointAnno
  a <https://www.w3.org/ns/oaAnnotation> ;
  <https://www.w3.org/ns/oahasBody> sto:IotaInformationViewpoint ;
  <https://www.w3.org/ns/oahasTarget> [
      a <https://www.w3.org/ns/oaSpecificResource> ;
      terms:format "pdf" ;
      <https://www.w3.org/ns/oahasSelector> [
          a <https://www.w3.org/ns/oaRangeSelector> ;
          <https://www.w3.org/ns/oahasEndSelector> [
              a <https://www.w3.org/ns/oaXPathSelector> ;
              rdf:value "Page 141" ;
            ] ;
          <https://www.w3.org/ns/oahasStartSelector> [
              a <https://www.w3.org/ns/oaXPathSelector> ;
              rdf:value "Page 126" ;
            ] ;
        ] ;
      <https://www.w3.org/ns/oahasSource> sto:Final_architectural_reference_model_for_the_IoT_v3_0 ;
    ] ;
.
sto:IotaPerformanceScalability
  a owl:NamedIndividual ;
  a sto:IotaPerspective ;
  a sto:StandardClassification ;
  rdfs:label "IoT-A Performance and Scalability"@en ;
  sto:frames sto:Communication ;
  sto:frames sto:Interoperability ;
  sto:frames sto:NetworkPerformance ;
  sto:frames sto:QualityOfService ;
  sto:frames sto:Scalability ;
  sto:frames sto:SemanticInteroperability ;
  sto:frames sto:ServiceDescription ;
  sto:isDescribedin sto:IotaReferenceArchitecture ;
.
sto:IotaPerformanceScalabilityAnno
  a <https://www.w3.org/ns/oaAnnotation> ;
  <https://www.w3.org/ns/oahasBody> sto:IotaPerformanceScalability ;
  <https://www.w3.org/ns/oahasTarget> [
      a <https://www.w3.org/ns/oaSpecificResource> ;
      terms:format "pdf" ;
      <https://www.w3.org/ns/oahasSelector> [
          a <https://www.w3.org/ns/oaRangeSelector> ;
          <https://www.w3.org/ns/oahasEndSelector> [
              a <https://www.w3.org/ns/oaXPathSelector> ;
              rdf:value "Page 152" ;
            ] ;
          <https://www.w3.org/ns/oahasStartSelector> [
              a <https://www.w3.org/ns/oaXPathSelector> ;
              rdf:value "Page 151" ;
            ] ;
        ] ;
      <https://www.w3.org/ns/oahasSource> sto:Final_architectural_reference_model_for_the_IoT_v3_0 ;
    ] ;
.
sto:IotaPerspective
  a owl:Class ;
  a owl:NamedIndividual ;
  terms:creator sto:sebastian ;
  rdfs:label "IoT-A Perspective"@en ;
  rdfs:subClassOf sto:StandardClassification ;
.
sto:IotaPerspectiveAnno
  a <https://www.w3.org/ns/oaAnnotation> ;
  <https://www.w3.org/ns/oahasBody> sto:IotaPerspective ;
  <https://www.w3.org/ns/oahasTarget> [
      a <https://www.w3.org/ns/oaSpecificResource> ;
      terms:format "pdf" ;
      <https://www.w3.org/ns/oahasSelector> [
          a <https://www.w3.org/ns/oaRangeSelector> ;
          <https://www.w3.org/ns/oahasEndSelector> [
              a <https://www.w3.org/ns/oaXPathSelector> ;
              rdf:value "Page 156" ;
            ] ;
          <https://www.w3.org/ns/oahasStartSelector> [
              a <https://www.w3.org/ns/oaXPathSelector> ;
              rdf:value "Page 149" ;
            ] ;
        ] ;
      <https://www.w3.org/ns/oahasSource> sto:Final_architectural_reference_model_for_the_IoT_v3_0 ;
    ] ;
.
sto:IotaReferenceArchitecture
  a owl:NamedIndividual ;
  a sto:ArchitectureDescription ;
  a sto:StandardizationFramework ;
  terms:creator sto:sebastian ;
  rdfs:label "IoT-A Reference Architecture"@en ;
  sto:hasPublisher sto:IoTA ;
.
sto:IotaReferenceArchitectureAnno
  a <https://www.w3.org/ns/oaAnnotation> ;
  <https://www.w3.org/ns/oahasBody> sto:IotaReferenceArchitecture ;
  <https://www.w3.org/ns/oahasTarget> [
      a <https://www.w3.org/ns/oaSpecificResource> ;
      terms:format "pdf" ;
      <https://www.w3.org/ns/oahasSelector> [
          a <https://www.w3.org/ns/oaRangeSelector> ;
          <https://www.w3.org/ns/oahasEndSelector> [
              a <https://www.w3.org/ns/oaXPathSelector> ;
              rdf:value "Page 482" ;
            ] ;
          <https://www.w3.org/ns/oahasStartSelector> [
              a <https://www.w3.org/ns/oaXPathSelector> ;
              rdf:value "Page 1" ;
            ] ;
        ] ;
      <https://www.w3.org/ns/oahasSource> sto:Final_architectural_reference_model_for_the_IoT_v3_0 ;
    ] ;
.
sto:IotaTrustSecurityPrivacy
  a owl:NamedIndividual ;
  a sto:IotaPerspective ;
  a sto:StandardClassification ;
  dul:associatedWith sto:IDSRAMSecurity ;
  dul:associatedWith sto:IIRASecurity ;
  rdfs:label "IoT-A Trust Security and Privacy"@en ;
  sto:alignsWith sto:IDSRAMSecurity ;
  sto:alignsWith sto:Security ;
  sto:frames sto:DataSovereignty ;
  sto:frames sto:Privacy ;
  sto:frames sto:Security ;
  sto:frames sto:Trustworthiness ;
  sto:isDescribedin sto:IotaReferenceArchitecture ;
.
sto:IotaTrustSecurityPrivacyAnno
  a <https://www.w3.org/ns/oaAnnotation> ;
  <https://www.w3.org/ns/oahasBody> sto:IotaTrustSecurityPrivacy ;
  <https://www.w3.org/ns/oahasTarget> [
      a <https://www.w3.org/ns/oaSpecificResource> ;
      terms:format "pdf" ;
      <https://www.w3.org/ns/oahasSelector> [
          a <https://www.w3.org/ns/oaRangeSelector> ;
          <https://www.w3.org/ns/oahasEndSelector> [
              a <https://www.w3.org/ns/oaXPathSelector> ;
              rdf:value "Page 155" ;
            ] ;
          <https://www.w3.org/ns/oahasStartSelector> [
              a <https://www.w3.org/ns/oaXPathSelector> ;
              rdf:value "Page 152" ;
            ] ;
        ] ;
      <https://www.w3.org/ns/oahasSource> sto:Final_architectural_reference_model_for_the_IoT_v3_0 ;
    ] ;
.
sto:IpsoAppFramework
  a owl:NamedIndividual ;
  a foaf:Document ;
  a sto:Publication ;
  a sto:TechnicalSpecification ;
  terms:creator sto:sebastian ;
  rdfs:comment "IPSO Application Framework (PDF): This design defines sets of REST interfaces that may be used by a smart object to represent its available resources, interact with other smart objects and backend services. This framework is designed to be complementary to existing Web profiles including SEP2 and oBIX. (source: https://www.postscapes.com/internet-of-things-protocols/)"@en ;
  rdfs:label "IPSO App Framework"@en ;
  sto:hasOfficialResource <http://www.ipso-alliance.org/wp-content/media/draft-ipso-app-framework-04.pdf> ;
.
sto:Ivi
  a owl:NamedIndividual ;
  a foaf:Organization ;
  a sto:IIoTConsortium ;
  terms:creator sto:sebastian ;
  terms:title "Industrial Value Chain Initiative"@en ;
  rdfs:comment "The Industrial Value Chain Initiative (IVI) is a forum to design a new society by combining manufacturing and information technologies, and for all enterprises to take an initiative collaboratively."@en ;
  rdfs:label "IVI"@en ;
  sto:hasOfficialResource <https://iv-i.org/> ;
.
sto:IviActivityLayer
  a owl:NamedIndividual ;
  a sto:IviLayer ;
  a sto:StandardClassification ;
  terms:creator sto:sebastian ;
  dul:associatedWith rami:Engineering ;
  dul:associatedWith sto:Manufacturing ;
  rdfs:comment "The activity layer has a view point of activities actually conducted at various places in manufacturers. People and machines acting voluntarily, human activity, machine processes, and information as an object og such activities and processes are brought up for discussion. In every production site of every manufacturer, concrete manufacturing activities are conducted in a different way. (source: IVRA-Next)"@en ;
  rdfs:label "IVI Activity Layer"@en ;
  sto:alignsWith rami:Engineering ;
  sto:alignsWith sto:Manufacturing ;
  sto:frames rami:ProcessPlanning ;
  sto:isDescribedin sto:IVRA ;
.
sto:IviActivityLayerAnno
  a <https://www.w3.org/ns/oaAnnotation> ;
  <https://www.w3.org/ns/oahasBody> sto:IviActivityLayer ;
  <https://www.w3.org/ns/oahasTarget> [
      a <https://www.w3.org/ns/oaSpecificResource> ;
      terms:format "pdf" ;
      <https://www.w3.org/ns/oahasSelector> [
          a <https://www.w3.org/ns/oaRangeSelector> ;
          <https://www.w3.org/ns/oahasEndSelector> [
              a <https://www.w3.org/ns/oaXPathSelector> ;
              rdf:value "Page 5" ;
            ] ;
          <https://www.w3.org/ns/oahasStartSelector> [
              a <https://www.w3.org/ns/oaXPathSelector> ;
              rdf:value "Page 4" ;
            ] ;
        ] ;
      <https://www.w3.org/ns/oahasSource> sto:Industrial_Value_Chain_Reference_Architecture_IVRA_Next ;
    ] ;
.
sto:IviActivityView
  a owl:NamedIndividual ;
  a sto:StandardClassification ;
  a sto:Viewpoint ;
  terms:creator sto:sebastian ;
  dul:associatedWith rami:Engineering ;
  dul:associatedWith sto:IIRAOperationsDomain ;
  rdfs:label "IVI Activity View"@en ;
  sto:alignsWith rami:Engineering ;
  sto:alignsWith sto:IIRAOperationsDomain ;
  sto:frames sto:Manufacturing ;
  sto:isDescribedin sto:IVRA ;
.
sto:IviActivityViewAnno
  a <https://www.w3.org/ns/oaAnnotation> ;
  <https://www.w3.org/ns/oahasBody> sto:IviActivityView ;
  <https://www.w3.org/ns/oahasTarget> [
      a <https://www.w3.org/ns/oaSpecificResource> ;
      terms:format "pdf" ;
      <https://www.w3.org/ns/oahasSelector> [
          a <https://www.w3.org/ns/oaRangeSelector> ;
          <https://www.w3.org/ns/oahasEndSelector> [
              a <https://www.w3.org/ns/oaXPathSelector> ;
              rdf:value "Page 3" ;
            ] ;
          <https://www.w3.org/ns/oahasStartSelector> [
              a <https://www.w3.org/ns/oaXPathSelector> ;
              rdf:value "Page 2" ;
            ] ;
        ] ;
      <https://www.w3.org/ns/oahasSource> sto:Industrial_Value_Chain_Reference_Architecture_IVRA ;
    ] ;
.
sto:IviAssetView
  a owl:NamedIndividual ;
  a sto:StandardClassification ;
  a sto:Viewpoint ;
  terms:creator sto:sebastian ;
  dul:associatedWith sto:IIRAPhysicalSystems ;
  dul:associatedWith sto:RAMIAssetlayer ;
  rdfs:label "IVI Asset View"@en ;
  sto:alignsWith sto:IIRAPhysicalSystems ;
  sto:alignsWith sto:RAMIAssetlayer ;
  sto:frames sto:ThingRepresentation ;
  sto:isDescribedin sto:IVRA ;
.
sto:IviAssetViewAnno
  a <https://www.w3.org/ns/oaAnnotation> ;
  <https://www.w3.org/ns/oahasBody> sto:IviAssetView ;
  <https://www.w3.org/ns/oahasTarget> [
      a <https://www.w3.org/ns/oaSpecificResource> ;
      terms:format "pdf" ;
      <https://www.w3.org/ns/oahasSelector> [
          a <https://www.w3.org/ns/oaRangeSelector> ;
          <https://www.w3.org/ns/oahasEndSelector> [
              a <https://www.w3.org/ns/oaXPathSelector> ;
              rdf:value "Page 2" ;
            ] ;
          <https://www.w3.org/ns/oahasStartSelector> [
              a <https://www.w3.org/ns/oaXPathSelector> ;
              rdf:value "Page 1" ;
            ] ;
        ] ;
      <https://www.w3.org/ns/oahasSource> sto:Industrial_Value_Chain_Reference_Architecture_IVRA ;
    ] ;
.
sto:IviBusinessLayer
  a owl:NamedIndividual ;
  a sto:IviLayer ;
  a sto:StandardClassification ;
  terms:creator sto:sebastian ;
  dul:associatedWith sto:IIRABusinessViewpoint ;
  dul:associatedWith sto:RAMIBusinessLayer ;
  rdfs:comment "In the business layer, from a perspective of enterprise management, the focus of discussions is placed on the fundamentel structure of manufacturing, organization forms for manufacturing, presence of essential perspectives and axes as well as a philosophy and concept of values underpinning the big picture. (source: IVRA-Next)"@en ;
  rdfs:label "IVI Business Layer"@en ;
  sto:alignsWith sto:IIRABusinessViewpoint ;
  sto:alignsWith sto:RAMIBusinessLayer ;
  sto:frames sto:BusinessContext ;
  sto:frames sto:BusinessTransactions ;
  sto:isDescribedin sto:IVRA ;
.
sto:IviBusinessLayerAnno
  a <https://www.w3.org/ns/oaAnnotation> ;
  <https://www.w3.org/ns/oahasBody> sto:IviBusinessLayer ;
  <https://www.w3.org/ns/oahasTarget> [
      a <https://www.w3.org/ns/oaSpecificResource> ;
      terms:format "pdf" ;
      <https://www.w3.org/ns/oahasSelector> [
          a <https://www.w3.org/ns/oaRangeSelector> ;
          <https://www.w3.org/ns/oahasEndSelector> [
              a <https://www.w3.org/ns/oaXPathSelector> ;
              rdf:value "Page 5" ;
            ] ;
          <https://www.w3.org/ns/oahasStartSelector> [
              a <https://www.w3.org/ns/oaXPathSelector> ;
              rdf:value "Page 4" ;
            ] ;
        ] ;
      <https://www.w3.org/ns/oahasSource> sto:Industrial_Value_Chain_Reference_Architecture_IVRA_Next ;
    ] ;
.
sto:IviLayer
  a owl:Class ;
  rdfs:comment "A IVI Layer describes one of three layers of smart manufactoring as proposed by the Industrial Value Chain Initiative (IVI)."@en ;
  rdfs:isDefinedBy <https://iv-i.org/wp/wp-content/uploads/2018/04/IVRA-Next_en.pdf> ;
  rdfs:label "IVI Layer"@en ;
  rdfs:subClassOf sto:StandardClassification ;
.
sto:IviManagementView
  a owl:NamedIndividual ;
  a sto:StandardClassification ;
  a sto:Viewpoint ;
  terms:creator sto:sebastian ;
  dul:associatedWith sto:IIRAUsageViewpoint ;
  dul:associatedWith sto:RAMIFunctionalLayer ;
  rdfs:label "IVI Management View"@en ;
  sto:alignsWith sto:IIRAUsageViewpoint ;
  sto:alignsWith sto:RAMIFunctionalLayer ;
  sto:frames sto:BusinessContext ;
  sto:frames sto:BusinessTransactions ;
  sto:frames sto:ServiceLevelAgreements ;
  sto:frames sto:ServiceLifecycleManagement ;
  sto:isDescribedin sto:IVRA ;
.
sto:IviManagementViewAnno
  a <https://www.w3.org/ns/oaAnnotation> ;
  <https://www.w3.org/ns/oahasBody> sto:IviManagementView ;
  <https://www.w3.org/ns/oahasTarget> [
      a <https://www.w3.org/ns/oaSpecificResource> ;
      terms:format "pdf" ;
      <https://www.w3.org/ns/oahasSelector> [
          a <https://www.w3.org/ns/oaRangeSelector> ;
          <https://www.w3.org/ns/oahasEndSelector> [
              a <https://www.w3.org/ns/oaXPathSelector> ;
              rdf:value "Page 4" ;
            ] ;
          <https://www.w3.org/ns/oahasStartSelector> [
              a <https://www.w3.org/ns/oaXPathSelector> ;
              rdf:value "Page 3" ;
            ] ;
        ] ;
      <https://www.w3.org/ns/oahasSource> sto:Industrial_Value_Chain_Reference_Architecture_IVRA ;
    ] ;
.
sto:IviSpecificationLayer
  a owl:NamedIndividual ;
  a sto:IviLayer ;
  a sto:StandardClassification ;
  terms:creator sto:sebastian ;
  dul:associatedWith rami:Engineering ;
  dul:associatedWith rami:TypeDevelopment ;
  rdfs:comment "In the specification layer, the following will be considered: Specific operations based on human activities and machine processes and the things and information items that are their subjects, as well as the data and their attributes that are the subject of the processes executed by logic in software. (source: IVRA-Next)"@en ;
  rdfs:label "IVI Specification Layer"@en ;
  sto:alignsWith rami:Engineering ;
  sto:alignsWith rami:TypeDevelopment ;
  sto:frames sto:DataProcessing ;
  sto:isDescribedin sto:IVRA ;
.
sto:IviSpecificationLayerAnno
  a <https://www.w3.org/ns/oaAnnotation> ;
  <https://www.w3.org/ns/oahasBody> sto:IviSpecificationLayer ;
  <https://www.w3.org/ns/oahasTarget> [
      a <https://www.w3.org/ns/oaSpecificResource> ;
      terms:format "pdf" ;
      <https://www.w3.org/ns/oahasSelector> [
          a <https://www.w3.org/ns/oaRangeSelector> ;
          <https://www.w3.org/ns/oahasEndSelector> [
              a <https://www.w3.org/ns/oaXPathSelector> ;
              rdf:value "Page 5" ;
            ] ;
          <https://www.w3.org/ns/oahasStartSelector> [
              a <https://www.w3.org/ns/oaXPathSelector> ;
              rdf:value "Page 4" ;
            ] ;
        ] ;
      <https://www.w3.org/ns/oahasSource> sto:Industrial_Value_Chain_Reference_Architecture_IVRA_Next ;
    ] ;
.
sto:JMS
  a owl:NamedIndividual ;
  a foaf:Document ;
  a sto:Publication ;
  a sto:TechnicalSpecification ;
  terms:creator sto:sebastian ;
  rdfs:comment "JMS (Java Message Service) - A Java Message Oriented Middleware (MOM) API for sending messages between two or more clients. (source: https://www.postscapes.com/internet-of-things-protocols/)"@en ;
  rdfs:label "JMS"@en ;
.
sto:Jurisdictional_Issues
  a owl:NamedIndividual ;
  a sto:Concern ;
  terms:creator sto:MuhammadUsman ;
  rdfs:comment "It is often challenging to alter resources, for example, the server or data centres to a particular geographic area. Load balancing service provider of the cloud, the availability of the network, or the performance of the data centre are few factors that determine where the data is stored. Accordingly, an organization data might be stored in a different location with various legal jurisdictions and diverse laws concerning the security issues, such as the protection and interruptions of the data"@en ;
  rdfs:label "Jurisdictional Issues"@en ;
  rdfs:seeAlso "https://dl.acm.org/citation.cfm?doid=3108421.3108426"@en ;
  sto:hasWikipediaArticle "https://en.wikipedia.org/wiki/Jurisdiction"@en ;
  sto:supports sto:CloudComputing ;
.
sto:KATS
  a owl:NamedIndividual ;
  a foaf:Organization ;
  a sto:StandardOrganization ;
  dul:associatedWith sto:IEC ;
  dul:associatedWith sto:ISO ;
  dul:isMemberOf sto:IEC ;
  dul:isMemberOf sto:ISO ;
  rdfs:comment "Korean Agency for Technology and Standards is the government standards organization for South Korea. It is part of the Ministry of Knowledge Economy. It is authorized to regulate and manage the legal measures of South Korea by the current Measures Act."@en ;
  rdfs:label "Korean Agency for Technology and Standards"@en ;
  sto:abbreviation "KATS"@de ;
  sto:belongsTo dbr:South_Korea ;
  sto:hasDBpediaResource <http://dbpedia.org/page/Korean_Agency_for_Technology_and_Standards> ;
  sto:hasHeadquaterIn dbr:Eumseong ;
  sto:hasWikipediaArticle <https://en.wikipedia.org/wiki/Korean_Agency_for_Technology_and_Standards> ;
  sto:orgName "Korean Agency for Technology and Standards"@en ;
.
sto:KeyRock
  a owl:NamedIndividual ;
  a foaf:Document ;
  a sto:Publication ;
  a sto:TechnicalSpecification ;
  dul:associatedWith sto:FiwareDataContextManagement ;
  dul:associatedWith sto:FiwareSecurity ;
  sto:hasTargetConcern sto:IdentityManagement ;
.
sto:LLAP
  a owl:NamedIndividual ;
  a foaf:Document ;
  a sto:Publication ;
  a sto:TechnicalSpecification ;
  terms:creator sto:sebastian ;
  rdfs:comment "LLAP (lightweight local automation protocol): is a simple short message that is sent between inteligent objects using normal text, it's not like TCP/IP, bluetooth, zigbee, 6lowpan, WiFi etc which achieve at a low level 'how' to move data around. This means LLAP can run over any communication medium. The three strengths of LLAP are, it'll run on anything now, anything in the future and it's easily understandable by humans. (source: https://www.postscapes.com/internet-of-things-protocols/)"@en ;
  rdfs:label "LLAP"@en ;
  sto:hasOfficialResource <http://openkontrol.org/llap/index.php/openkontrol/69-LLAP%20-%20Lightweight%20Local%20Automation%20Protocol> ;
.
sto:LWM2M
  a owl:NamedIndividual ;
  a foaf:Document ;
  a sto:Publication ;
  a sto:TechnicalSpecification ;
  terms:creator sto:sebastian ;
  rdfs:comment "LWM2M (Lightweight M2M) is a system standard in the Open Mobile Alliance. It includes DTLS, CoAP, Block, Observe, SenML and Resource Directory and weaves them into a device-server interface along with an Object structure. (source: https://www.postscapes.com/internet-of-things-protocols/)"@en ;
  rdfs:label "LWM2M"@en ;
  sto:hasOfficialResource <http://yucianga.info/?p=786> ;
.
sto:LatencyReduction
  a owl:NamedIndividual ;
  a sto:Concern ;
  terms:creator sto:MuhammadUsman ;
  rdfs:comment "Latency is a time interval between the stimulation and response, or, from a more general point of view, a time delay between the cause and the effect of some physical change in the system being observed."@en ;
  rdfs:label "LatencyReduction"@en ;
  rdfs:seeAlso "https://ieeexplore.ieee.org/document/7488250" ;
  sto:hasWikipediaArticle "https://en.wikipedia.org/wiki/Latency_(engineering)"@en ;
  sto:supports sto:Communication ;
.
sto:LinkedData
  a owl:NamedIndividual ;
  a foaf:Document ;
  a sto:Publication ;
  a sto:TechnicalSpecification ;
.
sto:LoRaWAN
  a owl:NamedIndividual ;
  a foaf:Document ;
  a sto:Publication ;
  a sto:TechnicalSpecification ;
  terms:creator sto:sebastian ;
  rdfs:comment "LoRaWAN - Network protocol intended for wireless battery operated Things in regional, national or global network. (source: https://www.postscapes.com/internet-of-things-protocols/)"@en ;
  rdfs:label "LoRaWAN"@en ;
  sto:hasOfficialResource <https://www.lora-alliance.org/What-Is-LoRa/Technology> ;
.
sto:LoWPAN
  a owl:NamedIndividual ;
  a foaf:Document ;
  a sto:Publication ;
  a sto:TechnicalSpecification ;
  terms:creator sto:IETF ;
  terms:creator sto:sebastian ;
  rdfs:comment "6LoWPAN is an acronym of IPv6 over Low power Wireless Personal Area Networks. It is an adaption layer for IPv6 over IEEE802.15.4 links. This protocol operates only in the 2.4 GHz frequency range with 250 kbps transfer rate. (source: https://www.postscapes.com/internet-of-things-protocols/)"@en ;
  rdfs:label "6LoWPAN"@en ;
  foaf:maker sto:IETF ;
  sto:hasClassification sto:IIRAConnectivity ;
  sto:hasClassification sto:RAMICommunicationlayer ;
  sto:hasDBpediaResource <http://dbpedia.org/resource/6LoWPAN> ;
  sto:hasDeveloper sto:IETF ;
  sto:hasPublisher sto:IETF ;
  sto:hasTargetConcern sto:Communication ;
  sto:hasWikipediaArticle <https://en.wikipedia.org/wiki/6LoWPAN> ;
.
sto:Logging
  a owl:NamedIndividual ;
  a sto:Concern ;
  rdfs:comment "The process of recording incidents and events regarding a specific service, data resource or device in order to make status changes transparent."@en ;
  rdfs:label "Logging"@en ;
  rdfs:seeAlso "IoT-A Requirement UNI.409" ;
  rdfs:seeAlso "IoT-A Requirement UNI.710" ;
  sto:hasDBpediaResource <http://dbpedia.org/resource/Data_logger> ;
  sto:supports sto:DataUsageControl ;
  sto:supports sto:ServiceAccessControl ;
.
sto:Long_Term_Business_Sustainability
  a owl:NamedIndividual ;
  a sto:Concern ;
  terms:creator sto:MuhammadUsman ;
  rdfs:comment "The provider should not go broke, be financially in a close-fitting corner or close down the business. Organizations should be sure and know how to move your data to another cloud provider. And should know how to have a backup at another public cloud of data for redundancy"@en ;
  rdfs:label "Long Term Business Sustainability"@en ;
  rdfs:seeAlso "https://dl.acm.org/citation.cfm?doid=3286606.3286865"@en ;
  sto:hasWikipediaArticle "https://en.wikipedia.org/wiki/Sustainability"@en ;
  sto:supports sto:BusinessContext ;
.
sto:LowPowerWiFi
  a owl:NamedIndividual ;
  a foaf:Document ;
  a sto:Publication ;
  a sto:TechnicalSpecification ;
.
sto:LsDL
  a owl:NamedIndividual ;
  a foaf:Document ;
  a sto:Publication ;
  a sto:TechnicalSpecification ;
  terms:creator sto:sebastian ;
  rdfs:comment "LsDL (Lemonbeat smart Device Language) - XML-based device language for service oriented devices. (source: https://www.postscapes.com/internet-of-things-protocols/)"@en ;
  rdfs:label "LsDL"@en ;
  sto:hasOfficialResource <http://www.lemonbeat.com/lsdl/> ;
.
sto:LteMtc
  a owl:NamedIndividual ;
  a foaf:Document ;
  a sto:Publication ;
  a sto:TechnicalSpecification ;
  terms:creator sto:sebastian ;
  rdfs:comment "LTE-MTC (LTE-Machine Type Communication) - Standards-based family of technologies supports several technology categories, such as Cat-1 and CatM1, suitable for the IoT. (source: https://www.postscapes.com/internet-of-things-protocols/)"@en ;
  rdfs:label "LTE-MTC"@en ;
  sto:hasOfficialResource <http://www.gsma.com/connectedliving/long-term-evolution-machine-type-communication-lte-mtc-cat-m1/> ;
.
sto:M2M
  a owl:NamedIndividual ;
  a sto:Domain ;
  rdfs:comment "Machine to machine refers to direct communication between devices using any communications channel, including wired and wireless"@en ;
  rdfs:label "Machine to Machine"@en ;
  sto:domainName "Machine to machine Communication"@en ;
  sto:hasDBpediaResource <http://dbpedia.org/resource/Machine_to_machine> ;
  sto:hasWikipediaArticle <https://en.wikipedia.org/wiki/Machine_to_machine> ;
.
sto:MESA
  a owl:NamedIndividual ;
  a foaf:Organization ;
  a sto:StandardOrganization ;
  rdfs:comment "The Manufacturing Enterprise Solutions Association International is a global community of manufacturers, producers, industry leaders, and solution providers who are focused on driving business results from manufacturing information."@en ;
  sto:abbreviation "MESA" ;
  sto:formationDate "1992-01-01"^^xsd:date ;
  sto:hasDBpediaResource <http://dbpedia.org/page/Manufacturing_Enterprise_Solutions_Association> ;
  sto:hasHeadquaterIn dbr:_Arizona ;
  sto:hasOfficialResource <http://www.mesa.org/en/index.asp> ;
  sto:hasWikipediaArticle <https://en.wikipedia.org/wiki/Manufacturing_Enterprise_Solutions_Association> ;
  sto:orgName "Manufacturing Enterprise Solutions Association"@en ;
.
sto:MIIT
  a owl:NamedIndividual ;
  a foaf:Organization ;
  a sto:StandardOrganization ;
  rdfs:comment "Ministry of Industry and Information Technology (MIIT) of the Chinese government, established in March 2008, is the state agency of the People's Republic of China responsible for regulation and development of the postal service, Internet, wireless, broadcasting, communications, production of electronic and information goods, software industry and the promotion of the national knowledge economy."@en ;
  sto:abbreviation "MIIT" ;
  sto:belongsTo dbr:China ;
  sto:formationDate "2008-03-01"^^xsd:date ;
  sto:hasDBpediaResource <http://dbpedia.org/page/Ministry_of_Industry_and_Information_Technology> ;
  sto:hasHeadquaterIn dbr:Beijing ;
  sto:hasOfficialResource <http://www.miit.gov.cn/> ;
  sto:hasWikipediaArticle <https://en.wikipedia.org/wiki/Ministry_of_Industry_and_Information_Technology> ;
  sto:orgName "Ministry of Industry and Information Technology"@en ;
.
sto:MOMLevel
  a owl:NamedIndividual ;
  a sto:ISA95Level ;
  a sto:StandardClassification ;
  rdfs:comment "Describes the MOM level according to the ISA95 level classification."@en ;
  rdfs:label "MOM Level"@en ;
  skos:definition "Manufacturing Operation Management Level according to ISA 95"@en ;
.
sto:MTConnect
  a owl:NamedIndividual ;
  a foaf:Document ;
  a sto:Publication ;
  a sto:Standard ;
  terms:creator sto:MTConnect_Institute ;
  rdfs:comment "MTConnect is a protocol designed for the exchange of data between shop floor equipment and software applications used for monitoring and data analysis. MTConnect is referred to as a read-only standard, meaning that it only defines the extraction (reading) of data from control devices, not the writing of data to a control device. Freely available, open standards are used for all aspects of MTConnect. Data from shop floor devices is presented in XML format, and is retrieved from information providers, called Agents, using Hypertext Transfer Protocol (HTTP) as the underlying transport protocol. MTConnect provides a RESTful interface, which means the interface is stateless. No session must be established to retrieve data from an MTConnect Agent, and no logon or logoff sequence is required (unless overlying security protocols are added which do). Lightweight Directory Access Protocol (LDAP) is recommended for discovery services."@en ;
  rdfs:label "MTConnect"@en ;
  foaf:maker sto:MTConnect_Institute ;
  sto:hasClassification sto:DeviceLevel ;
  sto:hasDBpediaResource <http://dbpedia.org/resource/MTConnect> ;
  sto:hasDeveloper sto:MTConnect_Institute ;
  sto:hasOfficialResource <http://www.mtconnect.org/standard-documents> ;
  sto:hasPublisher sto:MTConnect_Institute ;
  sto:hasTag "MTConnect"@en ;
  sto:hasWikipediaArticle <https://en.wikipedia.org/wiki/MTConnect> ;
.
sto:MTConnect_Institute
  a owl:NamedIndividual ;
  a foaf:Organization ;
  a sto:StandardOrganization ;
  rdfs:comment "MTConnect Institute is a collaborative effort to develop technical standards and specifications intended to foster greater interoperability between automation/control applications, field systems/devices, and business/office applications in the manufacturing industry (\"MTConnect Specifications\"), as well as schema, prototype software examples, and related documentation in order to facilitate the implementation of the MTConnect Specifications in compliant applications, drivers, and other services"@en ;
  sto:abbreviation "MTC" ;
  sto:formationDate "2006-01-01"^^xsd:date ;
  sto:hasOfficialResource <https://w3id.org/i40/www.mtconnect.org> ;
  sto:orgName "MTConnect Institute"@en ;
.
sto:MachineLearning
  a owl:NamedIndividual ;
  a sto:Concern ;
  terms:creator sto:sebastian ;
  rdfs:comment "Machine learning is the subfield of computer science that \"gives computers the ability to learn without being explicitly programmed\" (Arthur Samuel, 1959). Evolved from the study of pattern recognition and computational learning theory in artificial intelligence, machine learning explores the study and construction of algorithms that can learn from and make predictions on data – such algorithms overcome following strictly static program instructions by making data-driven predictions or decisions, through building a model from sample inputs. (source: wikipedia)"@en ;
  rdfs:label "Machine Learning"@en ;
  sto:hasDBpediaResource <http://dbpedia.org/resource/Machine_learning> ;
  sto:supports sto:AI ;
.
sto:MaintenanceCost
  a owl:NamedIndividual ;
  a sto:Concern ;
  rdfs:comment "The ability of a system to be maintained."@en ;
  rdfs:label "Maintenance Cost"@en ;
  skos:note "Publications referred: '<https://www.openfogconsortium.org/wp-content/uploads/OpenFog_Reference_Architecture_2_09_17-FINAL.pdf> OPFRA001.020817' '3 Use Cases for Fog' 'Page 13' " ;
  skos:note "Publications referred: 'IIC:PUB:G1:V1.80:20170131' '4 BUSINESS VIEWPOINT' 'Page 20' " ;
  sto:supports sto:BusinessContext ;
.
sto:Manufacturing
  a owl:NamedIndividual ;
  a sto:StandardClassification ;
  dul:associatedWith sto:IviActivityLayer ;
  sto:alignsWith sto:IviActivityLayer ;
.
sto:ManufacturingModelData
  a owl:NamedIndividual ;
  a sto:ProductDevelopmentLifeCycle ;
  a sto:StandardClassification ;
  rdfs:comment "Manufacturing Model Data Standards define the data needed to manufacture a product from a design."@en ;
  rdfs:label "Manufacturing Model Data"@en ;
  sto:isDescribedin sto:NISTInitiative ;
.
sto:MathML
  a owl:NamedIndividual ;
  a foaf:Document ;
  a sto:Publication ;
  a sto:Standard ;
  terms:creator sto:W3C ;
  rdfs:comment "MathML is a low-level specification for mathematical and scientific content on the Web and beyond"@en ;
  rdfs:label "MathML"@en ;
  foaf:maker sto:W3C ;
  sto:hasDBpediaResource <http://dbpedia.org/page/MathML> ;
  sto:hasOfficialResource <https://www.w3.org/Math/> ;
  sto:hasPublisher sto:W3C ;
  sto:hasWikipediaArticle <https://en.wikipedia.org/wiki/MathML> ;
  sto:relatedTo sto:DIN_SPEC_16592 ;
  sto:relatedTo sto:IEC_61131 ;
  sto:relatedTo sto:IEC_61360 ;
  sto:relatedTo sto:IEC_61499 ;
  sto:relatedTo sto:IEC_61804 ;
  sto:relatedTo sto:IEC_61850 ;
  sto:relatedTo sto:IEC_61987_X ;
  sto:relatedTo sto:IEC_62424 ;
  sto:relatedTo sto:IEC_62453 ;
  sto:relatedTo sto:IEC_62541 ;
  sto:relatedTo sto:IEC_62714 ;
  sto:relatedTo sto:ISO_13584 ;
  sto:relatedTo sto:ISO_14306 ;
  sto:relatedTo sto:ISO_15746 ;
  sto:relatedTo sto:ISO_15926 ;
  sto:relatedTo sto:ISO_18629 ;
  sto:relatedTo sto:ISO_18828-2 ;
  sto:relatedTo sto:ISO_20922 ;
  sto:relatedTo sto:ISO_22400 ;
  sto:relatedTo sto:ISO_29002 ;
  sto:relatedTo sto:ISO_ASTM_52915 ;
  sto:relatedTo sto:ISO_PAS_17506 ;
  sto:relatedTo sto:MathML ;
  sto:relatedTo sto:SysML ;
  sto:relatedTo sto:eClass ;
.
sto:MessagePriority
  a owl:NamedIndividual ;
  a sto:Concern ;
  <http://voag.linkedmodel.org/voag#hasStakeholder> <https://www.wikidata.org/wiki/Q1548249> ;
  <http://voag.linkedmodel.org/voag#hasStakeholder> <owl:Developer> ;
  rdfs:comment "Message precedence is an indicator attached to a message indicating its level of urgency. (source: wikipedia)"@en ;
  rdfs:label "Message precedence"@en ;
  rdfs:seeAlso "IoT-A Requirement UNI.028" ;
  sto:hasDBpediaResource <http://dbpedia.org/resource/Message_precedence> ;
  sto:supports sto:Communication ;
.
sto:Mihini
  a owl:NamedIndividual ;
  a foaf:Document ;
  a sto:Publication ;
  a sto:TechnicalSpecification ;
  terms:creator sto:sebastian ;
  rdfs:comment "Mihini/M3DA: The Mihini agent is a software component that acts as a mediator between an M2M server and the applications running on an embedded gateway. M3DA is a protocol optimized for the transport of binary M2M data. It is made available in the Mihini project both for means of Device Management, by easing the manipulation and synchronization of a device's data model, and for means of Asset Management, by allowing user applications to exchange typed data/commands back and forth with an M2M server, in a way that optimizes the use of bandwidth (source: https://www.postscapes.com/internet-of-things-protocols/)"@en ;
  rdfs:label "Mihini"@en ;
  sto:hasOfficialResource <https://wiki.eclipse.org/Mihini/M3DA_Specification> ;
.
sto:MobilDevices
  a owl:NamedIndividual ;
  a sto:Concern ;
  terms:creator sto:MuhammadUsman ;
  rdfs:comment """How to handle the massive mobility of vehicles? In the case of an application scenario that involves connected vehicles, mobility is a major issue and includes data consumer as well as data producer. In this particular case, one of the influencing factors is the potential speed of a vehicle. High-speed mobility may
lead to situations in which a request for data or a service may not be answered before the vehicle disconnects and re-connects to another network entry point. This leads to unfulfilled requests and potential duplication of efforts."""@en ;
  rdfs:label "Mobil Devices"@en ;
  rdfs:seeAlso "https://dl.acm.org/citation.cfm?doid=3098208.3098210" ;
  rdfs:seeAlso "https://en.wikipedia.org/wiki/Connected_car"@en ;
  rdfs:seeAlso "https://ieeexplore.ieee.org/document/6188257"@en ;
  sto:supports sto:IoT ;
.
sto:ModBus
  a owl:NamedIndividual ;
  a foaf:Document ;
  a sto:Publication ;
  a sto:Standard ;
  terms:creator sto:SE ;
  rdfs:comment "Modbus is a serial communications protocol to be used in Programmable logic controllers (PLCs)."@en ;
  rdfs:label "ModBus"@en ;
  foaf:maker sto:SE ;
  sto:hasClassification sto:RAMIIntegrationLayer ;
  sto:hasDBpediaResource <http://dbpedia.org/page/Modbus> ;
  sto:hasOfficialResource <http://www.modbus.org/> ;
  sto:hasPublisher sto:SE ;
  sto:hasTag "Modbus"@en ;
  sto:hasWikipediaArticle <https://en.wikipedia.org/wiki/Modbus> ;
.
sto:ModelingPractice
  a owl:NamedIndividual ;
  a sto:ProductDevelopmentLifeCycle ;
  a sto:StandardClassification ;
  rdfs:comment "Modeling practice standards define digital product-definition data practices for both two-dimensional (2D) drawings and three-dimensional (3D) models."@en ;
  rdfs:label "Modeling Practice"@en ;
  sto:isDescribedin sto:NISTInitiative ;
.
sto:MuhammadUsman
  a owl:NamedIndividual ;
  a foaf:Person ;
  rdfs:label "Muhammad Usman"@en ;
.
sto:Multicast
  rdfs:seeAlso "IoT-A Requirement UNI.302" ;
  rdfs:seeAlso "IoT-A Requirement UNI.303" ;
  rdfs:seeAlso "IoT-A Requirement UNI.304" ;
  rdfs:seeAlso "IoT-A Requirement UNI.305" ;
.
sto:Multilaterism
  a owl:NamedIndividual ;
  a sto:Concern ;
  terms:creator sto:sebastian ;
  rdfs:comment "Data Artefacts are received by 1 to m Data Consumer."@en ;
  rdfs:label "Multilateralism"@en ;
  skos:altLabel "Cardinality of Participants"@en ;
  skos:altLabel "Multicast"@en ;
  sto:supports sto:CardinalityOfDataSources ;
.
sto:MultipleIdenities
  rdfs:seeAlso "IoT-A Requirement UNI.320" ;
.
sto:MultipleIdentities
  a owl:NamedIndividual ;
  a sto:Concern ;
  terms:creator sto:sebastian ;
  rdfs:comment "Devices must be able to switch between different networks without losing connections (Network handover/handoff support)."@en ;
  rdfs:label "Multiple Identities"@en ;
  rdfs:seeAlso "UNI.320"@en ;
  sto:supports sto:IdentityManagement ;
.
sto:NERC
  a owl:NamedIndividual ;
  a foaf:Organization ;
  a sto:StandardOrganization ;
  terms:description "The North American Electric Reliability Corporation (NERC) is a not-for-profit international regulatory authority whose mission is to assure the effective and efficient reduction of risks to the reliability and security of the grid. NERC develops and enforces Reliability Standards; annually assesses seasonal and long‐term reliability; monitors the bulk power system through system awareness; and educates, trains, and certifies industry personnel. NERC’s area of responsibility spans the continental United States, Canada, and the northern portion of Baja California, Mexico. NERC is the electric reliability organization (ERO) for North America, subject to oversight by the Federal Energy Regulatory Commission (FERC) and governmental authorities in Canada. NERC's jurisdiction includes users, owners, and operators of the bulk power system, which serves more than 334 million people."@en ;
  rdfs:seeAlso <https://www.nerc.com/Pages/default.aspx> ;
  sto:abbreviation "NERC"@en ;
  sto:hasWikipediaArticle <https://wikipedia.org/wiki/North_American_Electric_Reliability_Corporation> ;
  sto:orgName "North American Electric Reliability Corporation"@en ;
.
sto:NFC
  a owl:NamedIndividual ;
  a foaf:Document ;
  a sto:Publication ;
  a sto:TechnicalSpecification ;
  terms:creator sto:sebastian ;
  rdfs:comment "Based on the standard ISO/IEC 18092:2004, using inductive coupled devices at a center frequency of13.56 MHz. The data rate is up to 424 kbps and the rangeis with a few meters short compared to the wireless sensornetworks. (source: https://www.postscapes.com/internet-of-things-protocols/)"@en ;
  rdfs:label "NFC"@en ;
  sto:hasClassification sto:OpenFogNodeView ;
  sto:hasOfficialResource <http://www.nfc-forum.org/home/> ;
.
sto:NGSI
  a owl:NamedIndividual ;
  a foaf:Document ;
  a sto:Publication ;
  a sto:TechnicalSpecification ;
  terms:creator sto:FIWARE ;
  terms:creator sto:sebastian ;
  terms:title "Next Generation Service Interface"@en ;
  rdfs:comment """The FIWARE NGSI (Next Generation Service Interface) API defines
-    a data model for context information, based on a simple information model using the notion of context entities
-    a context data interface for exchanging information by means of query, subscription, and update operations
-    a context availability interface for exchanging information on how to obtain context information (whether to separate the two interfaces is currently under discussion)."""@en ;
  rdfs:label "NGSI"@en ;
  foaf:maker sto:FIWARE ;
  sto:hasOfficialResource <http://fiware.github.io/specifications/ngsiv2/stable/> ;
  sto:hasPublisher sto:FIWARE ;
.
sto:NGSI_Context_Information_Management_API
  a owl:Class ;
  terms:title "NGSI-LD" ;
  rdfs:label "NGSI Context Information Management API"@en ;
  rdfs:subClassOf sto:StandardClassification ;
  rdfs:subClassOf [
      a owl:Restriction ;
      owl:hasValue sto:FIWARE ;
      owl:onProperty sto:isDescribedin ;
    ] ;
.
sto:NIST
  a owl:NamedIndividual ;
  a foaf:Organization ;
  a sto:StandardOrganization ;
  rdfs:comment "The National Institute of Standards and Technology (NIST) is a measurement standards laboratory, and a non-regulatory agency of the United States Department of Commerce."@en ;
  sto:abbreviation "NIST" ;
  sto:belongsTo dbr:United_States ;
  sto:formationDate "1901-01-01"^^xsd:date ;
  sto:hasDBpediaResource <http://dbpedia.org/page/National_Institute_of_Standards_and_Technology> ;
  sto:hasHeadquaterIn dbr:_Maryland ;
  sto:hasOfficialResource <https://www.nist.gov/> ;
  sto:hasWikipediaArticle <https://en.wikipedia.org/wiki/National_Institute_of_Standards_and_Technology> ;
  sto:orgName "National Institute of Standards and Technology"@en ;
.
sto:NISTIR_8062
  a owl:NamedIndividual ;
  a foaf:Document ;
  a sto:Publication ;
  a sto:Standard ;
  dc11:title "Privacy Risk Management for Federal Information Systems"@en ;
  terms:creator sto:NIST ;
  rdfs:comment "This document provides an introduction to the concepts of privacy engineering and risk management for federal information systems. These concepts establish the basis for a common vocabulary to facilitate better understanding and communication of privacy risk within federal information systems, and the effective implementation of privacy principles. This publication introduces two key components to support the application of privacy engineering and risk management: privacy engineering objectives and a privacy risk model."@en ;
  rdfs:label "NIST Internal Report (NISTIR) 8062"@en ;
  rdfs:label "NISTIR 8062"@en ;
  foaf:maker sto:NIST ;
  sto:hasClassification sto:IIRAPrivacy ;
  sto:hasOfficialResource <https://doi.org/10.6028/NIST.IR.8062> ;
  sto:hasPublicationDate "2017-04-01"^^xsd:date ;
  sto:hasPublisher sto:NIST ;
.
sto:NISTIR_8107
  a owl:NamedIndividual ;
  a foaf:Document ;
  a sto:Publication ;
  a sto:Standard ;
  a sto:StandardClassification ;
  rdfs:comment "Describes the NIST Initiative"@en ;
  rdfs:isDefinedBy <http://nvlpubs.nist.gov/nistpubs/ir/2016/NIST.IR.8107.pdf> ;
  rdfs:label "NISTIR_8107"@en ;
  skos:note "TODO - improve this classification" ;
  sto:isDescribedin sto:BusinessProcessExecution ;
  sto:isDescribedin sto:SCM ;
.
sto:NISTInitiative
  a owl:NamedIndividual ;
  a sto:StandardizationFramework ;
  rdfs:comment "Describes the National Institute of Standards and Technology Initiative, i.e., NIST which provides a standard landascape"@en ;
  rdfs:isDefinedBy <http://nvlpubs.nist.gov/nistpubs/ir/2016/NIST.IR.8107.pdf> ;
  rdfs:label "NIST Initiative"@en ;
  sto:hasPublisher sto:NIST ;
.
sto:NIST_500-291
  a owl:NamedIndividual ;
  a foaf:Document ;
  a sto:Domain ;
  a sto:Publication ;
  a sto:Standard ;
  terms:creator sto:NIST ;
  terms:title "NIST Cloud Computing Standards Roadmap"@en ;
  rdfs:comment "The NIST Cloud Computing Standards Roadmap Working Group has surveyed the existing standards landscape for security, portability, and interoperability standards/models/studies/use cases, etc., relevant to cloud computing. Using this available information, current standards, standards gaps, and standardization priorities are identified in this document. The NIST Definition of Cloud Computing identified cloud computing as a model for enabling ubiquitous, convenient, on-demand network access to a shared pool of configurable computing resources (e.g., networks, servers, storage, applications, and services) that can be rapidly provisioned and released with minimal management effort or service provider interaction."@en ;
  rdfs:label "NIST 500-291"@en ;
  foaf:maker sto:NIST ;
  sto:domainName "Cloud Computing"@en ;
  sto:hasClassification sto:IIRASecurity ;
  sto:hasOfficialResource <https://www.nist.gov/publications/nist-sp-500-291-nist-cloud-computing-standards-roadmap> ;
  sto:hasPublicationDate "2011-08-10"^^xsd:date ;
  sto:hasPublisher sto:NIST ;
.
sto:NIST_500-292
  a owl:NamedIndividual ;
  a foaf:Document ;
  a sto:Domain ;
  a sto:Publication ;
  a sto:Standard ;
  dc11:title "NIST Cloud Computing Reference Architecture"@en ;
  terms:creator sto:NIST ;
  rdfs:comment "The adoption of cloud computing into the Federal Government and its implementation depend upon a variety of technical and non-technical factors. A fundamental reference point, based on the NIST definition of Cloud Computing, is needed to describe an overall framework that can be used government-wide. This document presents the NIST Cloud Computing Reference Architecture (RA) and Taxonomy (Tax) that will accurately communicate the components and offerings of cloud computing."@en ;
  rdfs:label "NIST 500-292"@en ;
  foaf:maker sto:NIST ;
  sto:domainName "Cloud Computing"@en ;
  sto:hasClassification sto:Security ;
  sto:hasOfficialResource <https://www.nist.gov/publications/nist-cloud-computing-reference-architecture> ;
  sto:hasPublicationDate "2011-09-09"^^xsd:date ;
  sto:hasPublisher sto:NIST ;
.
sto:NIST_500-293
  a owl:NamedIndividual ;
  a foaf:Document ;
  a sto:Domain ;
  a sto:Publication ;
  a sto:Standard ;
  terms:creator sto:NIST ;
  terms:language lang:eng ;
  terms:title "US Government Cloud Computing Technology Roadmap"@en ;
  rdfs:comment "The National Institute of Standards and Technology (NIST), consistent with its mission, has a technology leadership role in support of United States Government (USG) secure and effective adoption of the Cloud Computing model to reduce costs and improve services. This role is described in the 2011 Federal Cloud Computing Strategy as “... a central one in defining and advancing standards, and collaborating with USG Agency CIOs, private sector experts, and international bodies to identify and reach consensus on cloud computing technology & standardization priorities.” This NIST Cloud Computing program and initiative to develop a USG Cloud Computing Technology Roadmap is one of several complementary and parallel USG initiatives defined in the broader Federal Cloud Computing Strategy referenced above. The Federal Cloud Computing Strategy characterizes cloud computing as a “profound economic and technical shift (with) great potential to reduce the cost of federal Information Technology (IT) systems while … improving IT capabilities and stimulating innovation in IT solutions.” In the technology vision of Federal Cloud Computing Strategy success, USG agencies will be able to easily locate desired IT services in a mature and competitive marketplace, rapidly procure access to these services, and use them to deliver innovative mission solutions. Cloud services will be secure, interoperable, and reliable. Agencies will be able to switch between providers easily and with minimal cost, and receive equal or superior service."@en ;
  rdfs:label "NIST 500-293"@en ;
  foaf:maker sto:NIST ;
  sto:domainName "Cloud Computing"@en ;
  sto:hasAvailableLanguage lang:eng ;
  sto:hasClassification sto:IIRASecurity ;
  sto:hasOfficialResource <https://www.nist.gov/publications/us-government-cloud-computing-technology-roadmap-volume-i-high-priority-requirements?pub_id=915112> ;
  sto:hasPublicationDate "2014-10-21"^^xsd:date ;
  sto:hasPublisher sto:NIST ;
.
sto:NIST_800-144
  a owl:NamedIndividual ;
  a foaf:Document ;
  a sto:Domain ;
  a sto:Publication ;
  a sto:Standard ;
  terms:creator sto:NIST ;
  terms:title "Guidelines on Security and Privacy in Public Cloud Computing"@en ;
  rdfs:comment "Cloud computing can and does mean different things to different people. The common characteristics most interpretations share are on-demand scalability of highly available and reliable pooled computing resources, secure access to metered services from nearly anywhere, and displacement of data and services from inside to outside the organization. While aspects of these characteristics have been realized to a certain extent, cloud computing remains a work in progress. This publication provides an overview of the security and privacy challenges pertinent to public cloud computing and points out considerations organizations should take when outsourcing data, applications, and infrastructure to a public cloud environment."@en ;
  rdfs:label "NIST 800-144"@en ;
  foaf:maker sto:NIST ;
  sto:domainName "Cloud Computing"@en ;
  sto:hasClassification sto:IIRASecurity ;
  sto:hasOfficialResource <https://csrc.nist.gov/publications/detail/sp/800-144/final> ;
  sto:hasPublicationDate "2011-12-01"^^xsd:date ;
  sto:hasPublisher sto:NIST ;
.
sto:NIST_800-146
  a owl:NamedIndividual ;
  a foaf:Document ;
  a sto:Publication ;
  a sto:Standard ;
  dc11:title "Cloud Computing Synopsis and Recommendations"@en ;
  terms:creator sto:NIST ;
  rdfs:comment "This document reprises the NIST-established definition of cloud computing, describes cloud computing benefits and open issues, presents an overview of major classes of cloud technology, and provides guidelines and recommendations on how organizations should consider the relative opportunities and risks of cloud computing."@en ;
  rdfs:label "NIST 800-146"@en ;
  foaf:maker sto:NIST ;
  sto:hasClassification sto:IIRASecurity ;
  sto:hasOfficialResource <https://csrc.nist.gov/publications/detail/sp/800-146/final> ;
  sto:hasPublicationDate "2012-05-01"^^xsd:date ;
  sto:hasPublisher sto:NIST ;
.
sto:NanoIP
  a owl:NamedIndividual ;
  a foaf:Document ;
  a sto:Publication ;
  a sto:TechnicalSpecification ;
  terms:creator sto:sebastian ;
  rdfs:comment "NanoIP, which stands for the nano Internet Protocol, is a concept that was created to bring Internet-like networking services to embedded and sensor devices, without the overhead of TCP/IP. NanoIP was designed with minimal overheads, wireless networking, and local addressing in mind. (source: https://www.postscapes.com/internet-of-things-protocols/)"@en ;
  rdfs:label "NanoIP"@en ;
  sto:hasOfficialResource <http://www.cwc.oulu.fi/nanoip/> ;
.
sto:NbIoT
  a owl:NamedIndividual ;
  a foaf:Document ;
  a sto:Publication ;
  a sto:TechnicalSpecification ;
  terms:creator sto:sebastian ;
  rdfs:comment "NB-IoT (Narrow-Band IoT) A technology being standardized by the 3GPP standards body. (source: https://www.postscapes.com/internet-of-things-protocols/)"@en ;
  rdfs:label "NB-IoT"@en ;
  sto:hasWikipediaArticle <https://en.wikipedia.org/wiki/NarrowBand_IOT> ;
.
sto:NetworkCongestionAvoidance
  a owl:NamedIndividual ;
  a sto:Concern ;
  terms:creator sto:sebastian ;
  rdfs:comment "While congestion avoidance is important in any large network, in low bandwidth mesh networks this is essential."@en ;
  rdfs:label "Network Congestion"@en ;
  rdfs:seeAlso "IoT-A Requirement UNI.615" ;
  sto:hasDBpediaResource <https://dbpedia.org/resource/Network_congestion> ;
  sto:hasWikipediaArticle <https://en.wikipedia.org/wiki/Network_congestion> ;
  sto:supports sto:QualityOfService ;
.
sto:NetworkPerformance
  a owl:NamedIndividual ;
  a sto:Concern ;
  rdfs:comment "Network performance refers to measures of service quality of a network as seen by the customer. There are many different ways to measure the performance of a network, as each network is different in nature and design. (source: wikidata)"@en ;
  rdfs:label "Network performance"@en ;
  rdfs:seeAlso "IoT-A Requirement UNI.252" ;
  sto:hasDBpediaResource <http://dbpedia.org/resource/Network_performance> ;
  sto:supports sto:Communication ;
  sto:supports sto:QualityOfService ;
.
sto:NetworkSecurity
  a owl:NamedIndividual ;
  a sto:Concern ;
  terms:creator sto:SebastianBader ;
  rdfs:comment """Data flow is an integral part of any cloud service over the network of computers or
clusters of systems using internet. Any intruder can analyze the data packet to detect any weakness in the system and can gain access to applications and data
using some kind of remote access mechanism and injection like SQL and some bad command, Denial of Service (DoS), Distributed DoS (DDoS), man in the
middle attacks, social networking attacks and some unauthorized attacks are the major entrance level attacks in cloud computing environment."""@en ;
  rdfs:label "network security"@en ;
  rdfs:seeAlso "https://ieeexplore.ieee.org/document/6188257"@en ;
  rdfs:seeAlso "https://ieeexplore.ieee.org/document/8249113"@en ;
  rdfs:seeAlso "https://ieeexplore.ieee.org/document/8552311"@en ;
  sto:hasWikipediaArticle "https://en.wikipedia.org/wiki/Audit"@en ;
  sto:hasWikipediaArticle "https://en.wikipedia.org/wiki/Network_security"@en ;
  sto:supports sto:Security ;
.
sto:NetworkVirtualization
  a owl:NamedIndividual ;
  a sto:Concern ;
  terms:creator sto:sebastian ;
  rdfs:comment "The system shall support network virtualisation, i.e. the usage of virtual overlay networks."@en ;
  rdfs:label "Network Virtualization"@en ;
  rdfs:seeAlso "IoT-A Requirement UNI.328" ;
  rdfs:seeAlso "UNI.328"@en ;
  sto:hasWikipediaArticle <https://en.wikipedia.org/wiki/Network_virtualization> ;
  sto:supports sto:Communication ;
.
sto:NgsiLdApiOperation
  a owl:NamedIndividual ;
  a sto:NGSI_Context_Information_Management_API ;
  a sto:StandardClassification ;
  dul:associatedWith sto:FiwareDataContextManagement ;
  dul:associatedWith sto:IDSRAMProcessLayer ;
  dul:associatedWith sto:IDSRAMSystemLayer ;
  dul:associatedWith sto:IIRAConnectivity ;
  dul:associatedWith sto:IIRAControlDomain ;
  rdfs:label "NGSI-LD API Operation"@en ;
  sto:alignsWith sto:FiwareDataContextManagement ;
  sto:alignsWith sto:IDSRAMProcessLayer ;
  sto:alignsWith sto:IDSRAMSystemLayer ;
  sto:alignsWith sto:IIRAConnectivity ;
  sto:alignsWith sto:IIRAControlDomain ;
  sto:frames sto:Communication ;
  sto:frames sto:EndpointInvocation ;
  sto:frames sto:Interoperability ;
  sto:frames sto:SyntacticInteroperability ;
  sto:isDescribedin sto:FIWARE ;
.
sto:NgsiLdArchitecture
  a owl:NamedIndividual ;
  a sto:NGSI_Context_Information_Management_API ;
  a sto:StandardClassification ;
  dul:associatedWith sto:FiwareApplicationsServicesAndDataDelivery ;
  dul:associatedWith sto:FiwareCloudHosting ;
  dul:associatedWith sto:IDSRAMSystemLayer ;
  dul:associatedWith sto:IIRAImplementationViewpoint ;
  dul:associatedWith sto:InterfaceNetworksDevices ;
  dul:associatedWith sto:RAMIIntegrationLayer ;
  rdfs:label "NGSI-LD Architecture"@en ;
  sto:alignsWith sto:FiwareApplicationsServicesAndDataDelivery ;
  sto:alignsWith sto:FiwareCloudHosting ;
  sto:alignsWith sto:IDSRAMSystemLayer ;
  sto:alignsWith sto:IIRAImplementationViewpoint ;
  sto:alignsWith sto:InterfaceNetworksDevices ;
  sto:alignsWith sto:RAMIIntegrationLayer ;
  sto:frames rami:ProcessPlanning ;
  sto:frames sto:Interoperability ;
  sto:frames sto:SyntacticInteroperability ;
  sto:isDescribedin sto:FIWARE ;
.
sto:NgsiLdDataRepresentation
  a owl:NamedIndividual ;
  a sto:NGSI_Context_Information_Management_API ;
  a sto:StandardClassification ;
  dul:associatedWith sto:FiwareDataContextManagement ;
  dul:associatedWith sto:IDSRAMInformationLayer ;
  dul:associatedWith sto:RAMIFunctionalLayer ;
  dul:associatedWith sto:RDF ;
  rdfs:label "NGSI-LD Data Representation"@en ;
  sto:alignsWith sto:FiwareDataContextManagement ;
  sto:alignsWith sto:IDSRAMInformationLayer ;
  sto:alignsWith sto:RAMIFunctionalLayer ;
  sto:frames sto:DataDescription ;
  sto:frames sto:Interoperability ;
  sto:frames sto:SemanticInteroperability ;
  sto:isDescribedin sto:FIWARE ;
.
sto:NgsiLdInformationModel
  a owl:NamedIndividual ;
  a sto:NGSI_Context_Information_Management_API ;
  a sto:StandardClassification ;
  terms:creator sto:sebastian ;
  dul:associatedWith sto:FiwareDataContextManagement ;
  dul:associatedWith sto:IDSRAMInformationLayer ;
  dul:associatedWith sto:InformationDomain ;
  dul:associatedWith sto:RAMIInformationLayer ;
  rdfs:comment "The FIWARE data models have been harmonized to enable data portability for different applications including, but not limited, to Smart Cities. They are intended to be used together with FIWARE NGSI version 2. If you want to contribute and create additional data models, please have a look at our repository of data models and the data model development guidelines. (source: https://www.fiware.org/developers/data-models/)"@en ;
  rdfs:label "NGSI-LD Information Model"@en ;
  sto:alignsWith sto:FiwareDataContextManagement ;
  sto:alignsWith sto:IDSRAMInformationLayer ;
  sto:alignsWith sto:InformationDomain ;
  sto:alignsWith sto:RAMIInformationLayer ;
  sto:frames sto:DataAnalytics ;
  sto:frames sto:DataDescription ;
  sto:frames sto:GeospatialData ;
  sto:frames sto:Interoperability ;
  sto:frames sto:SemanticInteroperability ;
  sto:isDescribedin sto:FIWARE ;
.
sto:NonRepudiation
  a owl:NamedIndividual ;
  a sto:Concern ;
  terms:creator sto:sebastian ;
  rdfs:comment "In digital security, non-repudiation means:  (a)  A service that provides proof of the integrity and origin of data. (b) An authentication that can be said to be genuine with high confidence. The most common method of verifying the digital origin of data is through digital certificates, a form of public key infrastructure that includes digital signatures."@en ;
  rdfs:label "Non-repudiation"@en ;
  rdfs:seeAlso "IoT-A Requirement UNI.619" ;
  rdfs:seeAlso "https://ieeexplore.ieee.org/document/6188257"@en ;
  sto:hasDBpediaResource <https://dbpedia.org/resource/Non-repudiation> ;
  sto:hasWikipediaArticle <https://en.wikipedia.org/wiki/Non-repudiation> ;
  sto:supports sto:IntegrityProtection ;
.
sto:OAGIS
  a owl:NamedIndividual ;
  a foaf:Document ;
  a sto:Publication ;
  a sto:Standard ;
  terms:creator sto:OAGi ;
  rdfs:comment "The Open Applications Group Integration Specification (OAGIS) is an effort to provide a canonical business language for information integration. It uses XML as the common alphabet for defining business messages, and for identifying business processes (scenarios) that allow businesses and business applications to communicate."@en ;
  rdfs:label "OAGIS"@en ;
  foaf:maker sto:OAGi ;
  sto:hasOfficialResource <http://www.oagi.org/dnn2/DownloadsandResources/OAGIS100PublicDownload.aspx> ;
  sto:hasPublisher sto:OAGi ;
  sto:hasTag "Open Applications Group Integration Specification"@en ;
  sto:hasWikipediaArticle <https://de.wikipedia.org/wiki/Open_Application_Group_Integration_Specification> ;
.
sto:OAGi
  a owl:NamedIndividual ;
  a foaf:Organization ;
  a sto:StandardOrganization ;
  rdfs:comment "The Open Applications Group is a not-for-profit standards development organization. Founded in 1994, is focused on building enterprise ready process-based data exchange standards for both B2B and A2A integration."@en ;
  rdfs:label "OAGi"@en ;
  sto:abbreviation "OAGi" ;
  sto:formationDate "1994-01-01"^^xsd:date ;
  sto:hasHeadquaterIn dbr:_Georgia ;
  sto:hasOfficialResource <http://www.oagi.org/dnn2/Home.aspx> ;
  sto:orgName "Open Applications Group"@en ;
.
sto:OASIS
  a owl:NamedIndividual ;
  a foaf:Organization ;
  a sto:StandardOrganization ;
  rdfs:comment "The Organization for the Advancement of Structured Information Standards (OASIS) is a global nonprofit consortium that works on the development, convergence, and adoption of standards for security, Internet of Things, energy, content technologies, emergency management, and other areas."@en ;
  sto:abbreviation "OASIS" ;
  sto:formationDate "1993-01-01"^^xsd:date ;
  sto:hasDBpediaResource <http://dbpedia.org/page/OASIS_(organization)> ;
  sto:hasHeadquaterIn dbr:Boston ;
  sto:hasOfficialResource <https://www.oasis-open.org/> ;
  sto:hasWikipediaArticle <https://en.wikipedia.org/wiki/OASIS_(organization)> ;
  sto:orgName "Organization for the Advancement of Structured Information Standards"@en ;
.
sto:OCF_Core_Specification_VERSION_2_0_1
  a <https://www.w3.org/ns/oaSpecificResource> ;
  rdfs:label "OCF Core Specification VERSION 2.0.1 | February 11, 2019"@en ;
  sto:hasOpenResource <https://openconnectivity.org/specs/OCF_Core_Specification_v2.0.1.pdf> ;
.
sto:ODRL
  a owl:NamedIndividual ;
  a foaf:Document ;
  a sto:Publication ;
  a sto:Standard ;
  terms:creator sto:W3C ;
  rdfs:comment """The Open Digital Rights Language (ODRL) is a policy expression language that provides a flexible and interoperable information model, vocabulary, and encoding mechanisms for representing statements about the usage of content and services. The ODRL Information Model describes the underlying concepts, entities, and relationships that form the foundational basis for the semantics of the ODRL policies.
Policies are used to represent permitted and prohibited actions over a certain asset, as well as the obligations required to be meet by stakeholders. In addition, policies may be limited by constraints (e.g., temporal or spatial constraints) and duties (e.g. payments) may be imposed on permissions."""@en ;
  rdfs:label "ODRL"@en ;
  rdfs:label "Open Digital Rights Language"@en ;
  foaf:maker sto:W3C ;
  sto:hasClassification sto:IDSRAMInformationLayer ;
  sto:hasClassification sto:IDSRAMSecurity ;
  sto:hasOfficialResource <https://www.w3.org/TR/odrl-model/> ;
  sto:hasPublisher sto:W3C ;
.
sto:ODVA
  a owl:NamedIndividual ;
  a foaf:Organization ;
  a sto:StandardOrganization ;
  rdfs:comment "Founded in 1995, ODVA is a global association whose members comprise the world’s leading automation companies. ODVA’s mission is to advance open, interoperable information and communication technologies in industrial automation. ODVA recognizes its media independent network protocol, the Common Industrial Protocol or “CIP” — and the network adaptations of CIP — EtherNet/IP, DeviceNet, CompoNet and ControlNet — as its core technology and the primary common interest of its membership. For future interoperability of production systems and the integration of the production systems with other systems, ODVA embraces the adoption of commercial-off-the-shelf (COTS) and standard, unmodified Internet and Ethernet technologies as a guiding principle wherever possible. This principle is exemplified by EtherNet/IP — the world’s number one industrial Ethernet network."@en ;
  sto:abbreviation "ODVA" ;
  sto:formationDate "1995-01-01"^^xsd:date ;
  sto:hasDBpediaResource <http://dbpedia.org/resource/ODVA_(company)> ;
  sto:hasHeadquaterIn dbr:_Michigan ;
  sto:hasOfficialResource <https://www.odva.org> ;
  sto:hasWikipediaArticle <https://en.wikipedia.org/wiki/ODVA_(company)> ;
  sto:orgName "ODVA, Inc"@en ;
.
sto:OFRAAgilityPillar
  a owl:NamedIndividual ;
  a sto:StandardClassification ;
  terms:creator sto:sebastian ;
  rdfs:comment """The agility pillar addresses business operational decisions for an OpenFog RA deployment. It is not possible for humans alone to analyze the data generated at the scale predicted by IoT as the basis for rapid, sound business and operational decisions. The agility pillar focuses on transforming this volume of data into actionable insights. Agility also deals with the highly dynamic nature of fog deployments and the need to respond quickly to change.
source: OpenFog Reference Architecture"""@en ;
  rdfs:label "OpenFog Agility Pillar"@en ;
  skos:note "Publications referred: '<https://www.openfogconsortium.org/wp-content/uploads/OpenFog_Reference_Architecture_2_09_17-FINAL.pdf> OPFRA001.020817' '4.7 Agility Pillar' 'Page 31' " ;
  sto:frames sto:Agility ;
  sto:isDescribedin sto:OpenFogReferenceArchitecture ;
.
sto:OFRAAgilityPillarAnno
  a <https://www.w3.org/ns/oaAnnotation> ;
  <https://www.w3.org/ns/oahasBody> sto:OFRAAgilityPillar ;
  <https://www.w3.org/ns/oahasTarget> [
      a <https://www.w3.org/ns/oaSpecificResource> ;
      terms:format "pdf" ;
      <https://www.w3.org/ns/oahasSelector> [
          a <https://www.w3.org/ns/oaRangeSelector> ;
          <https://www.w3.org/ns/oahasEndSelector> [
              a <https://www.w3.org/ns/oaXPathSelector> ;
              rdf:value "Page 32" ;
            ] ;
          <https://www.w3.org/ns/oahasStartSelector> [
              a <https://www.w3.org/ns/oaXPathSelector> ;
              rdf:value "Page 31" ;
            ] ;
        ] ;
      <https://www.w3.org/ns/oahasSource> sto:OpenFog_Reference_Architecture_for_Fog_Computing ;
    ] ;
.
sto:OFRAAutonomyPillar
  a owl:NamedIndividual ;
  a sto:StandardClassification ;
  terms:creator sto:sebastian ;
  rdfs:comment "The autonomy pillar enables fog nodes to continue to deliver the designed functionality in the face of the external service failures. In this architecture, autonomy is supported throughout the hierarchy. Decision making will be made at all levels of a deployment’s hierarchy including near the device or higher order layers. Centralized decision-making in the cloud is no longer the only option. Autonomy at the network edge means intelligence from local devices and peer data can be used to fulfill the business’ mission at the point where it makes the most business sense."@en ;
  rdfs:label "OpenFog AutonomyPillar"@en ;
  skos:note "Publications referred: '<https://www.openfogconsortium.org/wp-content/uploads/OpenFog_Reference_Architecture_2_09_17-FINAL.pdf> OPFRA001.020817' '4.4 Autonomy Pillar' 'Page 27' " ;
  sto:frames sto:AutonomousCommunication ;
  sto:frames sto:AutonomousConfiguration ;
  sto:isDescribedin sto:OpenFogReferenceArchitecture ;
.
sto:OFRAAutonomyPillarAnno
  a <https://www.w3.org/ns/oaAnnotation> ;
  <https://www.w3.org/ns/oahasBody> sto:OFRAAutonomyPillar ;
  <https://www.w3.org/ns/oahasTarget> [
      a <https://www.w3.org/ns/oaSpecificResource> ;
      terms:format "pdf" ;
      <https://www.w3.org/ns/oahasSelector> [
          a <https://www.w3.org/ns/oaRangeSelector> ;
          <https://www.w3.org/ns/oahasEndSelector> [
              a <https://www.w3.org/ns/oaXPathSelector> ;
              rdf:value "Page 29" ;
            ] ;
          <https://www.w3.org/ns/oahasStartSelector> [
              a <https://www.w3.org/ns/oaXPathSelector> ;
              rdf:value "Page 27" ;
            ] ;
        ] ;
      <https://www.w3.org/ns/oahasSource> sto:OpenFog_Reference_Architecture_for_Fog_Computing ;
    ] ;
.
sto:OFRADataAnalyticsAndControlPerspective
  a owl:NamedIndividual ;
  a sto:StandardClassification ;
  terms:creator sto:sebastian ;
  rdfs:label "OpenFog Data Analytics and Control Perspective"@en ;
  sto:alignsWith sto:IIRAControlDomain ;
  sto:alignsWith sto:InformationDomain ;
  sto:frames sto:DataAnalytics ;
  sto:isDescribedin sto:OpenFogReferenceArchitecture ;
.
sto:OFRADataAnalyticsAndControlPerspectiveAnno
  a <https://www.w3.org/ns/oaAnnotation> ;
  <https://www.w3.org/ns/oahasBody> sto:OFRADataAnalyticsAndControlPerspective ;
  <https://www.w3.org/ns/oahasTarget> [
      a <https://www.w3.org/ns/oaSpecificResource> ;
      terms:format "pdf" ;
      <https://www.w3.org/ns/oahasSelector> [
          a <https://www.w3.org/ns/oaRangeSelector> ;
          <https://www.w3.org/ns/oahasEndSelector> [
              a <https://www.w3.org/ns/oaXPathSelector> ;
              rdf:value "Page 56" ;
            ] ;
          <https://www.w3.org/ns/oahasStartSelector> [
              a <https://www.w3.org/ns/oaXPathSelector> ;
              rdf:value "Page 54" ;
            ] ;
        ] ;
      <https://www.w3.org/ns/oahasSource> sto:OpenFog_Reference_Architecture_for_Fog_Computing ;
    ] ;
.
sto:OFRADeploymentViewpoint
  a owl:NamedIndividual ;
  a sto:Viewpoint ;
  terms:creator sto:sebastian ;
  rdfs:comment "How fog software and fog systems are deployed to address a given scenario is also very important. There are many deployment types ranging from embedded to large clustered systems that are fully interconnected. The deployment type(s) chosen are scenario specific, but key aspects of the architecture remain visible regardless of deployment type. However, some may grow or shrink in importance. source: OpenFog Reference Architecture"@en ;
  rdfs:label "OpenFog Deployment Viewpoint"@en ;
  sto:alignsWith sto:IIRAImplementationViewpoint ;
  sto:frames sto:ServiceDeployment ;
  sto:isDescribedin sto:OpenFogReferenceArchitecture ;
.
sto:OFRADeploymentViewpointAnno
  a <https://www.w3.org/ns/oaAnnotation> ;
  <https://www.w3.org/ns/oahasBody> sto:OFRADeploymentViewpoint ;
  <https://www.w3.org/ns/oahasTarget> [
      a <https://www.w3.org/ns/oaSpecificResource> ;
      terms:format "pdf" ;
      <https://www.w3.org/ns/oahasSelector> [
          a <https://www.w3.org/ns/oaRangeSelector> ;
          <https://www.w3.org/ns/oahasEndSelector> [
              a <https://www.w3.org/ns/oaXPathSelector> ;
              rdf:value "Page 40" ;
            ] ;
          <https://www.w3.org/ns/oahasStartSelector> [
              a <https://www.w3.org/ns/oaXPathSelector> ;
              rdf:value "Page 39" ;
            ] ;
        ] ;
      <https://www.w3.org/ns/oahasSource> sto:OpenFog_Reference_Architecture_for_Fog_Computing ;
    ] ;
.
sto:OFRAFunctionalViewpoint
  a owl:NamedIndividual ;
  a sto:Viewpoint ;
  terms:creator sto:sebastian ;
  rdfs:comment "The functional viewpoint of the architecture shows how we apply the OpenFog architectural elements and views to address the various concerns of the stakeholders to satisfy a given scenario. Each scenario chosen will focus on a different aspects and market opportunities for fog computing. We fully expect that the architectural description, views, and perspective may change over time. This change and refinement should be driven from testbeds and application of the OpenFog RA to multiple different markets we see as important to fog computing. source: OpenFog Reference Architecture"@en ;
  rdfs:label "OpenFog Functional Viewpoint"@en ;
  sto:isDescribedin sto:OpenFogReferenceArchitecture ;
.
sto:OFRAFunctionalViewpointAnno
  a <https://www.w3.org/ns/oaAnnotation> ;
  <https://www.w3.org/ns/oahasBody> sto:OFRAFunctionalViewpoint ;
  <https://www.w3.org/ns/oahasTarget> [
      a <https://www.w3.org/ns/oaSpecificResource> ;
      terms:format "pdf" ;
      <https://www.w3.org/ns/oahasSelector> [
          a <https://www.w3.org/ns/oaRangeSelector> ;
          <https://www.w3.org/ns/oahasEndSelector> [
              a <https://www.w3.org/ns/oaXPathSelector> ;
              rdf:value "Page 39" ;
            ] ;
          <https://www.w3.org/ns/oahasStartSelector> [
              a <https://www.w3.org/ns/oaXPathSelector> ;
              rdf:value "Page 38" ;
            ] ;
        ] ;
      <https://www.w3.org/ns/oahasSource> sto:OpenFog_Reference_Architecture_for_Fog_Computing ;
    ] ;
.
sto:OFRAHierarchyPillar
  a owl:NamedIndividual ;
  a sto:StandardClassification ;
  terms:creator sto:sebastian ;
  rdfs:comment "OpenFog RA computing resources can be seen as a logical hierarchy based on the functional requirements of an end-to-end IoT system. Depending on the scale and nature of the scenario being addressed, the hierarchy may be a network of smart and connected partitioned systems arranged in physical or logical layers, or it may collapse into a single physical system (scalability pillar). source: OpenFog Reference Architecture"@en ;
  rdfs:label "OpenFog Hierarchy Pillar"@en ;
  skos:note "Publications referred: '<https://www.openfogconsortium.org/wp-content/uploads/OpenFog_Reference_Architecture_2_09_17-FINAL.pdf> OPFRA001.020817' '4.8 Hierarchy Pillar' 'Page 31' " ;
  sto:frames sto:BusinessValue ;
  sto:frames sto:DataAnalytics ;
  sto:frames sto:Sensing ;
  sto:isDescribedin sto:OpenFogReferenceArchitecture ;
.
sto:OFRAHierarchyPillarAnno
  a <https://www.w3.org/ns/oaAnnotation> ;
  <https://www.w3.org/ns/oahasBody> sto:OFRAHierarchyPillar ;
  <https://www.w3.org/ns/oahasTarget> [
      a <https://www.w3.org/ns/oaSpecificResource> ;
      terms:format "pdf" ;
      <https://www.w3.org/ns/oahasSelector> [
          a <https://www.w3.org/ns/oaRangeSelector> ;
          <https://www.w3.org/ns/oahasEndSelector> [
              a <https://www.w3.org/ns/oaXPathSelector> ;
              rdf:value "Page 34" ;
            ] ;
          <https://www.w3.org/ns/oahasStartSelector> [
              a <https://www.w3.org/ns/oaXPathSelector> ;
              rdf:value "Page 31" ;
            ] ;
        ] ;
      <https://www.w3.org/ns/oahasSource> sto:OpenFog_Reference_Architecture_for_Fog_Computing ;
    ] ;
.
sto:OFRAItBusinessAndCrossFogApplicationsPerspective
  a owl:NamedIndividual ;
  a sto:StandardClassification ;
  terms:creator sto:sebastian ;
  rdfs:comment "Fog applications and services should have the flexibility to span and interoperate with various levels in a fog hierarchy. This is a foundational aspect of fog computing that enables a multi-vendor ecosystem. In addition, the data that is collected or generated by one fog node should be shareable with other nodes in the hierarchy. The figure below shows a cross-fog application spanning east to west nodes (it would also be able to span north to south). source: OpenFog Reference Architecture"@en ;
  rdfs:label "OpenFog IT Business and Cross-fog Applications Perspective"@en ;
  sto:frames sto:BusinessContext ;
  sto:isDescribedin sto:OpenFogReferenceArchitecture ;
.
sto:OFRAItBusinessAndCrossFogApplicationsPerspectiveAnno
  a <https://www.w3.org/ns/oaAnnotation> ;
  <https://www.w3.org/ns/oahasBody> sto:OFRAItBusinessAndCrossFogApplicationsPerspective ;
  <https://www.w3.org/ns/oahasTarget> [
      a <https://www.w3.org/ns/oaSpecificResource> ;
      terms:format "pdf" ;
      <https://www.w3.org/ns/oahasSelector> [
          a <https://www.w3.org/ns/oaRangeSelector> ;
          <https://www.w3.org/ns/oahasEndSelector> [
              a <https://www.w3.org/ns/oaXPathSelector> ;
              rdf:value "Page 57" ;
            ] ;
          <https://www.w3.org/ns/oahasStartSelector> [
              a <https://www.w3.org/ns/oaXPathSelector> ;
              rdf:value "Page 56" ;
            ] ;
        ] ;
      <https://www.w3.org/ns/oahasSource> sto:OpenFog_Reference_Architecture_for_Fog_Computing ;
    ] ;
.
sto:OFRAManageabilityPerspective
  a owl:NamedIndividual ;
  a sto:StandardClassification ;
  terms:creator sto:sebastian ;
  rdfs:comment "Many fog computing deployments involve machine vision, and associated human-like functions. As such, they have the ability to see, respond, remember, move, and make autonomous decisions in order to participate in other fog services. This range of actions requires a higher level of manageability than a traditional static model. In addition, fog nodes may be deployed in a wide range of locations: remote, fixed and non-fixed, and environmentally harsh conditions. source: OpenFog Reference Architecture"@en ;
  rdfs:label "OpenFog Manageability Perspective"@en ;
  sto:frames sto:AutonomousConfiguration ;
  sto:frames sto:ServiceLifecycleManagement ;
  sto:isDescribedin sto:OpenFogReferenceArchitecture ;
.
sto:OFRAManageabilityPerspectiveAnno
  a <https://www.w3.org/ns/oaAnnotation> ;
  <https://www.w3.org/ns/oahasBody> sto:OFRAManageabilityPerspective ;
  <https://www.w3.org/ns/oahasTarget> [
      a <https://www.w3.org/ns/oaSpecificResource> ;
      terms:format "pdf" ;
      <https://www.w3.org/ns/oahasSelector> [
          a <https://www.w3.org/ns/oaRangeSelector> ;
          <https://www.w3.org/ns/oahasEndSelector> [
              a <https://www.w3.org/ns/oaXPathSelector> ;
              rdf:value "Page 54" ;
            ] ;
          <https://www.w3.org/ns/oahasStartSelector> [
              a <https://www.w3.org/ns/oaXPathSelector> ;
              rdf:value "Page 51" ;
            ] ;
        ] ;
      <https://www.w3.org/ns/oahasSource> sto:OpenFog_Reference_Architecture_for_Fog_Computing ;
    ] ;
.
sto:OFRANodeView
  a owl:NamedIndividual ;
  a sto:Viewpoint ;
  terms:creator sto:sebastian ;
  dul:associatedWith sto:WiFi ;
  rdfs:comment "The node view is the lowest level view we currently utilize in the architectural description. The stakeholders involved in formulating the viewpoint (and subsequently this view) are the system on a chip designers, silicon manufacturers, firmware architects, and system architects. source: OpenFog Reference Architecture"@en ;
  rdfs:label "OpenFog Node View"@en ;
  sto:alignsWith sto:IDSRAMSystemLayer ;
  sto:alignsWith sto:IIRAPhysicalSystems ;
  sto:alignsWith sto:RAMIAssetlayer ;
  sto:frames sto:DataStorage ;
  sto:frames sto:NetworkPerformance ;
  sto:frames sto:PhysicalConnectivity ;
  sto:frames sto:Security ;
  sto:isDescribedin sto:OpenFogReferenceArchitecture ;
.
sto:OFRANodeViewAnno
  a <https://www.w3.org/ns/oaAnnotation> ;
  <https://www.w3.org/ns/oahasBody> sto:OFRANodeView ;
  <https://www.w3.org/ns/oahasTarget> [
      a <https://www.w3.org/ns/oaSpecificResource> ;
      terms:format "pdf" ;
      <https://www.w3.org/ns/oahasSelector> [
          a <https://www.w3.org/ns/oaRangeSelector> ;
          <https://www.w3.org/ns/oahasEndSelector> [
              a <https://www.w3.org/ns/oaXPathSelector> ;
              rdf:value "Page 73" ;
            ] ;
          <https://www.w3.org/ns/oahasStartSelector> [
              a <https://www.w3.org/ns/oaXPathSelector> ;
              rdf:value "Page 56" ;
            ] ;
        ] ;
      <https://www.w3.org/ns/oahasSource> sto:OpenFog_Reference_Architecture_for_Fog_Computing ;
    ] ;
.
sto:OFRAOpennessPillar
  a owl:NamedIndividual ;
  a sto:StandardClassification ;
  terms:creator sto:sebastian ;
  rdfs:comment """Openness is essential for the success of a ubiquitous fog computing ecosystem for IoT platforms and applications. Proprietary or single vendor solutions can result in limited supplier diversity, which can have a negative impact on system cost, quality and innovation. The openness pillar importance is highlighted in our desire for fully interoperable systems, supported by a vibrant supplier ecosystem.
source: OpenFog Reference Architecture"""@en ;
  rdfs:label "OpenFog Opennes Pillar"@en ;
  skos:note "Publications referred: '<https://www.openfogconsortium.org/wp-content/uploads/OpenFog_Reference_Architecture_2_09_17-FINAL.pdf> OPFRA001.020817' '4.3 Openness Pillar' 'Page 26' " ;
  sto:frames sto:Interoperability ;
  sto:frames sto:ServiceComposition ;
  sto:isDescribedin sto:OpenFogReferenceArchitecture ;
.
sto:OFRAOpennessPillarAnno
  a <https://www.w3.org/ns/oaAnnotation> ;
  <https://www.w3.org/ns/oahasBody> sto:OFRAOpennessPillar ;
  <https://www.w3.org/ns/oahasTarget> [
      a <https://www.w3.org/ns/oaSpecificResource> ;
      terms:format "pdf" ;
      <https://www.w3.org/ns/oahasSelector> [
          a <https://www.w3.org/ns/oaRangeSelector> ;
          <https://www.w3.org/ns/oahasEndSelector> [
              a <https://www.w3.org/ns/oaXPathSelector> ;
              rdf:value "Page 27" ;
            ] ;
          <https://www.w3.org/ns/oahasStartSelector> [
              a <https://www.w3.org/ns/oaXPathSelector> ;
              rdf:value "Page 26" ;
            ] ;
        ] ;
      <https://www.w3.org/ns/oahasSource> sto:OpenFog_Reference_Architecture_for_Fog_Computing ;
    ] ;
.
sto:OFRAPerformancePerspective
  a owl:NamedIndividual ;
  a sto:StandardClassification ;
  terms:creator sto:sebastian ;
  rdfs:label "Performance and Scale Perspective"@en ;
  sto:isDescribedin sto:OpenFogReferenceArchitecture ;
.
sto:OFRAPerformancePerspectiveAnno
  a <https://www.w3.org/ns/oaAnnotation> ;
  <https://www.w3.org/ns/oahasBody> sto:OFRAPerformancePerspective ;
  <https://www.w3.org/ns/oahasTarget> [
      a <https://www.w3.org/ns/oaSpecificResource> ;
      terms:format "pdf" ;
      <https://www.w3.org/ns/oahasSelector> [
          a <https://www.w3.org/ns/oaRangeSelector> ;
          <https://www.w3.org/ns/oahasEndSelector> [
              a <https://www.w3.org/ns/oaXPathSelector> ;
              rdf:value "Page 47" ;
            ] ;
          <https://www.w3.org/ns/oahasStartSelector> [
              a <https://www.w3.org/ns/oaXPathSelector> ;
              rdf:value "Page 46" ;
            ] ;
        ] ;
      <https://www.w3.org/ns/oahasSource> sto:OpenFog_Reference_Architecture_for_Fog_Computing ;
    ] ;
.
sto:OFRAProgrammabilityPillar
  a owl:NamedIndividual ;
  a sto:StandardClassification ;
  terms:creator sto:sebastian ;
  rdfs:comment """The programmability pillar enables highly adaptive deployments including support for programming at the software and hardware layers. This means that re-tasking a fog node or cluster of fog nodes for accommodating operational dynamics, can be completely automated. The re-tasking can be done with the help of the fog nodes inherent programmability interfaces which we describe using general purpose compute or accelerator interfaces.
source: OpenFog Reference Architecture"""@en ;
  rdfs:label "OpenFog Programmability Pillar"@en ;
  skos:note "Publications referred: '<https://www.openfogconsortium.org/wp-content/uploads/OpenFog_Reference_Architecture_2_09_17-FINAL.pdf> OPFRA001.020817' '4.5 Programmability Pillar' 'Page 29' " ;
  sto:frames sto:Programmability ;
  sto:isDescribedin sto:OpenFogReferenceArchitecture ;
.
sto:OFRAProgrammabilityPillarAnno
  a <https://www.w3.org/ns/oaAnnotation> ;
  <https://www.w3.org/ns/oahasBody> sto:OFRAProgrammabilityPillar ;
  <https://www.w3.org/ns/oahasTarget> [
      a <https://www.w3.org/ns/oaSpecificResource> ;
      terms:format "pdf" ;
      <https://www.w3.org/ns/oahasSelector> [
          a <https://www.w3.org/ns/oaRangeSelector> ;
          <https://www.w3.org/ns/oahasEndSelector> [
              a <https://www.w3.org/ns/oaXPathSelector> ;
              rdf:value "Page 30" ;
            ] ;
          <https://www.w3.org/ns/oahasStartSelector> [
              a <https://www.w3.org/ns/oaXPathSelector> ;
              rdf:value "Page 29" ;
            ] ;
        ] ;
      <https://www.w3.org/ns/oahasSource> sto:OpenFog_Reference_Architecture_for_Fog_Computing ;
    ] ;
.
sto:OFRAScalabilityPillar
  a owl:NamedIndividual ;
  a sto:StandardClassification ;
  terms:creator sto:sebastian ;
  rdfs:comment """The scalability pillar addresses the dynamic technical and business needs behind fog deployments. Elastic scalability cuts across all fog computing applications and verticals. The hierarchical properties of fog and its location at logical edges of networks add additional scaling opportunities.
source: OpenFog Reference Architecture"""@en ;
  rdfs:label "OpenFog Scalability Pillar"@en ;
  skos:note "Publications referred: '<https://www.openfogconsortium.org/wp-content/uploads/OpenFog_Reference_Architecture_2_09_17-FINAL.pdf> OPFRA001.020817' '4.2 Scalability Pillar' 'Page 24' " ;
  sto:frames sto:Scalability ;
  sto:isDescribedin sto:OpenFogReferenceArchitecture ;
.
sto:OFRAScalabilityPillarAnno
  a <https://www.w3.org/ns/oaAnnotation> ;
  <https://www.w3.org/ns/oahasBody> sto:OFRAScalabilityPillar ;
  <https://www.w3.org/ns/oahasTarget> [
      a <https://www.w3.org/ns/oaSpecificResource> ;
      terms:format "pdf" ;
      <https://www.w3.org/ns/oahasSelector> [
          a <https://www.w3.org/ns/oaRangeSelector> ;
          <https://www.w3.org/ns/oahasEndSelector> [
              a <https://www.w3.org/ns/oaXPathSelector> ;
              rdf:value "Page 26" ;
            ] ;
          <https://www.w3.org/ns/oahasStartSelector> [
              a <https://www.w3.org/ns/oaXPathSelector> ;
              rdf:value "Page 24" ;
            ] ;
        ] ;
      <https://www.w3.org/ns/oahasSource> sto:OpenFog_Reference_Architecture_for_Fog_Computing ;
    ] ;
.
sto:OFRASecurityPerspective
  a owl:NamedIndividual ;
  a sto:StandardClassification ;
  terms:creator sto:sebastian ;
  rdfs:label "OpenFog Security Perspective"@en ;
  sto:alignsWith rami:Security ;
  sto:alignsWith sto:BdvaCyberSecurityTrust ;
  sto:alignsWith sto:FiwareSecurity ;
  sto:alignsWith sto:IDSRAMSecurity ;
  sto:alignsWith sto:IIRASecurity ;
  sto:alignsWith sto:IIRASecurityFramework ;
  sto:alignsWith sto:IotaTrustSecurityPrivacy ;
  sto:alignsWith sto:OcfSecurity ;
  sto:frames sto:Availability ;
  sto:frames sto:Identification ;
  sto:frames sto:IntegrityProtection ;
  sto:frames sto:Privacy ;
  sto:frames sto:ServiceAccessControl ;
  sto:frames sto:Trustworthiness ;
  sto:isDescribedin sto:OpenFogReferenceArchitecture ;
.
sto:OFRASecurityPerspectiveAnno
  a <https://www.w3.org/ns/oaAnnotation> ;
  <https://www.w3.org/ns/oahasBody> sto:OFRASecurityPerspective ;
  <https://www.w3.org/ns/oahasTarget> [
      a <https://www.w3.org/ns/oaSpecificResource> ;
      terms:format "pdf" ;
      <https://www.w3.org/ns/oahasSelector> [
          a <https://www.w3.org/ns/oaRangeSelector> ;
          <https://www.w3.org/ns/oahasEndSelector> [
              a <https://www.w3.org/ns/oaXPathSelector> ;
              rdf:value "Page 51" ;
            ] ;
          <https://www.w3.org/ns/oahasStartSelector> [
              a <https://www.w3.org/ns/oaXPathSelector> ;
              rdf:value "Page 47" ;
            ] ;
        ] ;
      <https://www.w3.org/ns/oahasSource> sto:OpenFog_Reference_Architecture_for_Fog_Computing ;
    ] ;
.
sto:OFRASecurityPillar
  a owl:NamedIndividual ;
  a sto:StandardClassification ;
  terms:creator sto:sebastian ;
  rdfs:comment " Security implementations have many different descriptions and attributes such as privacy, anonymity, integrity, trust, attestation, verification, and measurement. These are key attributes for the OpenFog RA. Achieving the foundational elements for security requires an approach to discover, attest, and verify all smart and connected “things” before trust can be established source: OpenFog Reference Architecture"@en ;
  rdfs:comment """Security in the OpenFog RA is not a one-size-fits-all architecture. Rather, it describes all of the mechanisms that can be applied to make a fog node secure from silicon to software application. Business case, target market, and vertical use case, as well as the location of the node itself, will all create a set of requirements for that node. However, there are certain foundational parts of the architecture, which must be in place in order to build a secure execution environment.
source: OpenFog Reference Architecture"""@en ;
  rdfs:label "OpenFog Security Pillar"@en ;
  skos:note "Publications referred: ' <https://www.openfogconsortium.org/wp-content/uploads/OpenFog_Reference_Architecture_2_09_17-FINAL.pdf> OPFRA001.020817' '4.1 Security Pillar' 'Page 23' " ;
  sto:alignsWith rami:Security ;
  sto:alignsWith sto:BdvaCyberSecurityTrust ;
  sto:alignsWith sto:FiwareSecurity ;
  sto:alignsWith sto:IDSRAMSecurity ;
  sto:alignsWith sto:IIRASecurity ;
  sto:alignsWith sto:IIRASecurityFramework ;
  sto:alignsWith sto:IotaTrustSecurityPrivacy ;
  sto:alignsWith sto:OcfSecurity ;
  sto:alignsWith sto:OpenFogSecurityPerspective ;
  sto:frames sto:Security ;
  sto:isDescribedin sto:OpenFogReferenceArchitecture ;
.
sto:OFRASecurityPillarAnno
  a <https://www.w3.org/ns/oaAnnotation> ;
  <https://www.w3.org/ns/oahasBody> sto:OFRASecurityPillar ;
  <https://www.w3.org/ns/oahasTarget> [
      a <https://www.w3.org/ns/oaSpecificResource> ;
      terms:format "pdf" ;
      <https://www.w3.org/ns/oahasSelector> [
          a <https://www.w3.org/ns/oaRangeSelector> ;
          <https://www.w3.org/ns/oahasEndSelector> [
              a <https://www.w3.org/ns/oaXPathSelector> ;
              rdf:value "Page 24" ;
            ] ;
          <https://www.w3.org/ns/oahasStartSelector> [
              a <https://www.w3.org/ns/oaXPathSelector> ;
              rdf:value "Page 23" ;
            ] ;
        ] ;
      <https://www.w3.org/ns/oahasSource> sto:OpenFog_Reference_Architecture_for_Fog_Computing ;
    ] ;
  <https://www.w3.org/ns/oahasTarget> [
      a <https://www.w3.org/ns/oaSpecificResource> ;
      terms:format "pdf" ;
      <https://www.w3.org/ns/oahasSelector> [
          a <https://www.w3.org/ns/oaRangeSelector> ;
          <https://www.w3.org/ns/oahasEndSelector> [
              a <https://www.w3.org/ns/oaXPathSelector> ;
              rdf:value "Page 24" ;
            ] ;
          <https://www.w3.org/ns/oahasStartSelector> [
              a <https://www.w3.org/ns/oaXPathSelector> ;
              rdf:value "Page 23" ;
            ] ;
        ] ;
      <https://www.w3.org/ns/oahasSource> sto:OpenFog_Reference_Architecture_for_Fog_Computing ;
    ] ;
.
sto:OFRASoftwareView
  a owl:NamedIndividual ;
  a sto:Viewpoint ;
  terms:creator sto:sebastian ;
  rdfs:comment "OpenFog Software Architecture View"@en ;
  rdfs:comment "The software view of the OpenFog RA is composed of software running on a platform that is comprised of one or more node views coupled with other components to create a system addressing a given scenario. The stakeholders of the software view include the system integrators, software architects, solution designers, and application developers of a fog computing environment. The software running on fog platforms is used to satisfy a given deployment scenario. A robust fog deployment requires that the relationship between a fog node, fog platform, and fog software are seamless. source: OpenFog Reference Architecture"@en ;
  sto:alignsWith sto:IIRAApplicationDomain ;
  sto:frames sto:ServiceDiscovery ;
.
sto:OFRASoftwareViewAnno
  a <https://www.w3.org/ns/oaAnnotation> ;
  <https://www.w3.org/ns/oahasBody> sto:OFRASoftwareView ;
  <https://www.w3.org/ns/oahasTarget> [
      a <https://www.w3.org/ns/oaSpecificResource> ;
      terms:format "pdf" ;
      <https://www.w3.org/ns/oahasSelector> [
          a <https://www.w3.org/ns/oaRangeSelector> ;
          <https://www.w3.org/ns/oahasEndSelector> [
              a <https://www.w3.org/ns/oaXPathSelector> ;
              rdf:value "Page 89" ;
            ] ;
          <https://www.w3.org/ns/oahasStartSelector> [
              a <https://www.w3.org/ns/oaXPathSelector> ;
              rdf:value "Page 77" ;
            ] ;
        ] ;
      <https://www.w3.org/ns/oahasSource> sto:OpenFog_Reference_Architecture_for_Fog_Computing ;
    ] ;
.
sto:OFRASystemView
  a owl:NamedIndividual ;
  a sto:Viewpoint ;
  terms:creator sto:sebastian ;
  rdfs:comment "The system view of the OpenFog RA is composed of one or more node views coupled with other components to create a platform. The stakeholders which typically create these systems to facilitate a fog deployment comprise the concerns of this viewpoint. Subsequently this view is intended to address the concerns of the system architects, hardware OEMs, and platform manufacturers. They also need to understand the Node view such that the systems they create can be deployed to address a given scenario. source: OpenFog Reference Architecture"@en ;
  rdfs:label "OpenFog System Architecture View"@en ;
  sto:frames sto:PhysicalConnectivity ;
  sto:isDescribedin sto:OpenFogReferenceArchitecture ;
.
sto:OFRASystemViewAnno
  a <https://www.w3.org/ns/oaAnnotation> ;
  <https://www.w3.org/ns/oahasBody> sto:OFRASystemView ;
  <https://www.w3.org/ns/oahasTarget> [
      a <https://www.w3.org/ns/oaSpecificResource> ;
      terms:format "pdf" ;
      <https://www.w3.org/ns/oahasSelector> [
          a <https://www.w3.org/ns/oaRangeSelector> ;
          <https://www.w3.org/ns/oahasEndSelector> [
              a <https://www.w3.org/ns/oaXPathSelector> ;
              rdf:value "Page 78" ;
            ] ;
          <https://www.w3.org/ns/oahasStartSelector> [
              a <https://www.w3.org/ns/oaXPathSelector> ;
              rdf:value "Page 73" ;
            ] ;
        ] ;
      <https://www.w3.org/ns/oahasSource> sto:OpenFog_Reference_Architecture_for_Fog_Computing ;
    ] ;
.
sto:OFRA_RASPillar
  a owl:NamedIndividual ;
  a sto:StandardClassification ;
  terms:creator sto:sebastian ;
  rdfs:comment """Reliability, availability, and serviceability (RAS) is resident throughout successful system architectures and, as such, takes on great importance in the OpenFog RA. Hardware, software, and operations are the three main areas of the RAS pillar.
source: OpenFog Reference Architecture"""@en ;
  rdfs:label "OpenFog RAS Pillar"@en ;
  skos:note "Publications referred: '<https://www.openfogconsortium.org/wp-content/uploads/OpenFog_Reference_Architecture_2_09_17-FINAL.pdf> OPFRA001.020817' '4.6 Reliability, Availability, and Serviceability (RAS)Pillar' 'Page 29' " ;
  sto:frames sto:Availability ;
  sto:frames sto:MaintenanceCost ;
  sto:frames sto:Reliability ;
  sto:isDescribedin sto:OpenFogReferenceArchitecture ;
.
sto:OFRA_RASPillarAnno
  a <https://www.w3.org/ns/oaAnnotation> ;
  <https://www.w3.org/ns/oahasBody> sto:OFRA_RASPillar ;
  <https://www.w3.org/ns/oahasTarget> [
      a <https://www.w3.org/ns/oaSpecificResource> ;
      terms:format "pdf" ;
      <https://www.w3.org/ns/oahasSelector> [
          a <https://www.w3.org/ns/oaRangeSelector> ;
          <https://www.w3.org/ns/oahasEndSelector> [
              a <https://www.w3.org/ns/oaXPathSelector> ;
              rdf:value "Page 31" ;
            ] ;
          <https://www.w3.org/ns/oahasStartSelector> [
              a <https://www.w3.org/ns/oaXPathSelector> ;
              rdf:value "Page 29" ;
            ] ;
        ] ;
      <https://www.w3.org/ns/oahasSource> sto:OpenFog_Reference_Architecture_for_Fog_Computing ;
    ] ;
.
sto:OMA
  a owl:NamedIndividual ;
  a foaf:Organization ;
  a sto:IIoTConsortium ;
  terms:creator sto:sebastian ;
  rdfs:comment "OMA (Open Mobile Alliance) is the Leading Industry Forum for Developing Market Driven, Interoperable Mobile Service Enablers (source: https://www.postscapes.com/internet-of-things-protocols/)"@en ;
  rdfs:label "Open Mobile Alliance"@en ;
  sto:hasOfficialResource <http://openmobilealliance.org/about-oma/work-program/m2m-enablers/> ;
.
sto:OMALightweightM2M
  a owl:NamedIndividual ;
  a foaf:Document ;
  a sto:Publication ;
  a sto:TechnicalSpecification ;
  terms:creator sto:sebastian ;
  rdfs:comment "The motivation of LightweightM2M is to develop a fast deployable client-server specification to provide machine to machine service.<br> LightweightM2M is principly a device management protocol, but it should be designed to be able to extend to meet the requirements of applications. LightweightM2M is not restricted to device management, it should be able transfer service / application data. (source: https://www.postscapes.com/internet-of-things-protocols/)"@en ;
  rdfs:label "Lightweight M2M v1.0"@en ;
  sto:hasOfficialResource <http://technical.openmobilealliance.org/Technical/release_program/lightweightM2M_v1_0.aspx> ;
.
sto:OMG
  a owl:NamedIndividual ;
  a foaf:Organization ;
  a sto:StandardOrganization ;
  rdfs:comment "The Object Management Group (OMG) is an international, open membership, not-for-profit technology standards consortium. OMG Task Forces develop enterprise integration standards for a wide range of technologies and industries. OMG modeling standards enable visual design, execution and maintenance of software and other processes. Originally aimed at standardizing distributed object-oriented systems, the company now focuses on modeling (programs, systems and business processes) and model-based standards." ;
  sto:abbreviation "OMG" ;
  sto:formationDate "1989-01-01"^^xsd:date ;
  sto:hasDBpediaResource <http://dbpedia.org/resource/Object_Management_Group> ;
  sto:hasHeadquaterIn dbr:_Massachusetts ;
  sto:hasOfficialResource <http://www.omg.org/> ;
  sto:hasWikipediaArticle <https://en.wikipedia.org/wiki/Object_Management_Group> ;
  sto:orgName "Object Management Group"@en ;
.
sto:OMG_DDS
  a owl:NamedIndividual ;
  a foaf:Document ;
  a sto:Publication ;
  a sto:Standard ;
  terms:creator sto:OMG ;
  rdfs:comment "The Data Distribution Service for real-time systems (DDS) is an Object Management Group (OMG) machine-to-machine (sometimes called middleware) standard that aims to enable scalable, real-time, dependable, high-performance and interoperable data exchanges using a publish–subscribe pattern. DDS addresses the needs of applications like financial trading, air-traffic control, smart grid management, and other big data applications. The standard is used in applications such as smartphone operating systems, transportation systems and vehicles, software-defined radio, and by healthcare providers. DDS was promoted for use in the Internet of things."@en ;
  rdfs:label "OMG DDS"@en ;
  foaf:maker sto:OMG ;
  sto:hasClassification sto:IICFFrameworkLayer ;
  sto:hasClassification sto:IIRAConnectivity ;
  sto:hasDBpediaResource <http://dbpedia.org/page/Data_Distribution_Service> ;
  sto:hasOfficialResource <http://portals.omg.org/dds/> ;
  sto:hasPublisher sto:OMG ;
  sto:hasWikipediaArticle <https://en.wikipedia.org/wiki/Data_Distribution_Service> ;
  sto:relatedTo sto:IEC_29182-1 ;
  sto:relatedTo sto:IEC_61158 ;
  sto:relatedTo sto:IEC_61784 ;
  sto:relatedTo sto:OMG_DDS ;
.
sto:OPC_Foundation
  a owl:NamedIndividual ;
  a foaf:Organization ;
  a sto:StandardOrganization ;
  rdfs:comment "Is an industry consortium that creates and maintains standards for open connectivity of industrial automation devices and systems, such as industrial control systems and process control generally"@en ;
  rdfs:label "OPC Foundation"@en ;
  sto:abbreviation "OPC" ;
  sto:formationDate "1994-01-01"^^xsd:date ;
  sto:hasDBpediaResource <http://dbpedia.org/page/OPC_Foundation> ;
  sto:hasHeadquaterIn dbr:_Arizona ;
  sto:hasOfficialResource <https://opcfoundation.org/> ;
  sto:hasWikipediaArticle <https://en.wikipedia.org/wiki/OPC_Foundation> ;
  sto:orgName "OPC Foundation"@en ;
.
sto:OTrP
  a owl:NamedIndividual ;
  a foaf:Document ;
  a sto:Publication ;
  a sto:TechnicalSpecification ;
  terms:creator sto:sebastian ;
  rdfs:comment "Open Trust Protocol (OTrP) - A protocol to install, update, and delete applications and to manage security configuration in a Trusted Execution Environment (TEE). (source: https://www.postscapes.com/internet-of-things-protocols/)"@en ;
  rdfs:label "Open Trust Protocol"@en ;
  sto:hasOfficialResource <https://www.ietf.org/id/draft-pei-opentrustprotocol-01.txt> ;
.
sto:Objects_Safety_and_security
  a owl:NamedIndividual ;
  a sto:Concern ;
  terms:creator sto:MuhammadUsman ;
  rdfs:comment """The IoT comprises of a huge number of perception objects that spread over a few geographic zone; it is important to keep the intruder's access to the items that
may make physical harm them or may change their operation"""@en ;
  rdfs:label "Objects Safety and Security"@en ;
  rdfs:seeAlso "https://ieeexplore.ieee.org/document/6188257"@en ;
  sto:supports sto:Safety ;
  sto:supports sto:Security ;
.
sto:OceanBusinessViewpoint
  a owl:NamedIndividual ;
  a sto:StandardClassification ;
  a sto:Viewpoint ;
  dul:associatedWith sto:IIRABusinessViewpoint ;
  rdfs:label "Ocean Protocol Business Viewpoint"@en ;
  sto:alignsWith sto:IIRABusinessViewpoint ;
  sto:frames sto:BusinessContext ;
  sto:frames sto:BusinessTransactions ;
  sto:frames sto:RoleCategorization ;
  sto:frames sto:Trustworthiness ;
  sto:isDescribedin sto:OceanProtocol ;
.
sto:OceanBusinessViewpointAnno
  a <https://www.w3.org/ns/oaAnnotation> ;
  <https://www.w3.org/ns/oahasBody> sto:OceanBusinessViewpoint ;
  <https://www.w3.org/ns/oahasTarget> [
      a <https://www.w3.org/ns/oaSpecificResource> ;
      <https://www.w3.org/ns/oahasSelector> [
          a <https://www.w3.org/ns/oaRangeSelector> ;
          <https://www.w3.org/ns/oahasEndSelector> [
              a <https://www.w3.org/ns/oaXPathSelector> ;
              rdf:value "Page 41" ;
            ] ;
          <https://www.w3.org/ns/oahasStartSelector> [
              a <https://www.w3.org/ns/oaXPathSelector> ;
              rdf:value "Page 1" ;
            ] ;
        ] ;
      <https://www.w3.org/ns/oahasSource> sto:Ocean_Protocol_Business_Strategy_Oct_2017 ;
    ] ;
.
sto:OceanMarketplaceViewpoint
  a owl:NamedIndividual ;
  a sto:StandardClassification ;
  a sto:Viewpoint ;
  dul:associatedWith sto:IIRABusinessViewpoint ;
  rdfs:label "Ocean Protocol Marketplace Viewpoint"@en ;
  sto:alignsWith sto:IIRABusinessViewpoint ;
  sto:frames sto:BusinessContext ;
  sto:isDescribedin sto:OceanProtocol ;
.
sto:OceanMarketplaceViewpointAnno
  a <https://www.w3.org/ns/oaAnnotation> ;
  <https://www.w3.org/ns/oahasBody> sto:OceanMarketplaceViewpoint ;
  <https://www.w3.org/ns/oahasTarget> [
      a <https://www.w3.org/ns/oaSpecificResource> ;
      <https://www.w3.org/ns/oahasSelector> [
          a <https://www.w3.org/ns/oaRangeSelector> ;
          <https://www.w3.org/ns/oahasEndSelector> [
              a <https://www.w3.org/ns/oaXPathSelector> ;
              rdf:value "Page 27" ;
            ] ;
          <https://www.w3.org/ns/oahasStartSelector> [
              a <https://www.w3.org/ns/oaXPathSelector> ;
              rdf:value "Page 1" ;
            ] ;
        ] ;
      <https://www.w3.org/ns/oahasSource> sto:Ocean_Protocol_Reference_Marketplace_Framework_Feb_2019 ;
    ] ;
.
sto:OceanProtocol
  a owl:NamedIndividual ;
  a foaf:Document ;
  a sto:Publication ;
  a sto:StandardizationFramework ;
  a sto:TechnicalSpecification ;
  terms:creator sto:OceanProtocolFoundation ;
  rdfs:comment "Ocean is a decentralized protocol and network of artificial intelligence (AI) data/services. It incentivizes for a vast supply of relevant AI data/services. This network helps to power AI data/service marketplaces, as well as public commons data. The heart of Ocean’s network is a new construction: a Curated Proofs Market. CPMs bridge predicted relevance with actual relevance of each AI service, by having curation markets for cryptographic proofs (e.g. proof of data availability). (source: https://oceanprotocol.com/tech-whitepaper.pdf)"@en ;
  rdfs:label "Ocean Protocol"@en ;
  rdfs:seeAlso <https://oceanprotocol.com/tech-whitepaper.pdf> ;
  foaf:maker sto:OceanProtocolFoundation ;
  sto:hasDeveloper sto:OceanProtocolFoundation ;
  sto:hasOfficialResource <https://oceanprotocol.com/> ;
  sto:hasPublisher sto:OceanProtocolFoundation ;
.
sto:OceanProtocolFoundation
  a owl:NamedIndividual ;
  a foaf:Organization ;
  a sto:StandardOrganization ;
  terms:creator sto:sebastian ;
  rdfs:comment "Ocean Protocol is supported by a Singapore based non-profit foundation, whose mandate is to ensure open access to the protocol and platform, provide data governance, encourage the network ecosystem growth and take measures to ensure that the platform becomes ever more decentralized with time."@en ;
  rdfs:label "Ocean Protocol Foundation"@en ;
  sto:hasOfficialResource <https://oceanprotocol.com/> ;
.
sto:OceanSystemViewpoint
  a owl:NamedIndividual ;
  a sto:StandardClassification ;
  a sto:Viewpoint ;
  dul:associatedWith sto:DataConsumer ;
  dul:associatedWith sto:DataProvider ;
  dul:associatedWith sto:IDSRAMBusinessLayer ;
  dul:associatedWith sto:IDSRAMProcessLayer ;
  dul:associatedWith sto:IIRABusinessDomain ;
  dul:associatedWith sto:IIRAFunctionalViewpoint ;
  dul:associatedWith sto:RAMIFunctionalLayer ;
  rdfs:label "Ocean Protocol System Viewpoint"@en ;
  sto:alignsWith sto:IDSRAMBusinessLayer ;
  sto:alignsWith sto:IDSRAMProcessLayer ;
  sto:alignsWith sto:IIRABusinessDomain ;
  sto:alignsWith sto:IIRAFunctionalViewpoint ;
  sto:alignsWith sto:RAMIFunctionalLayer ;
  sto:frames sto:AI ;
  sto:frames sto:Authorization ;
  sto:frames sto:Availability ;
  sto:frames sto:BusinessContext ;
  sto:frames sto:BusinessTransactions ;
  sto:frames sto:DataAccess ;
  sto:frames sto:DataAccessControl ;
  sto:frames sto:DataAnalytics ;
  sto:frames sto:DataDiscovery ;
  sto:frames sto:DataSovereignty ;
  sto:frames sto:Governance ;
  sto:frames sto:Identification ;
  sto:frames sto:IdentityManagement ;
  sto:frames sto:IntegrityProtection ;
  sto:frames sto:Interoperability ;
  sto:frames sto:Privacy ;
  sto:frames sto:ProvenanceTracking ;
  sto:frames sto:Security ;
  sto:frames sto:ServiceLevelAgreements ;
  sto:frames sto:ServiceLifecycleManagement ;
  sto:frames sto:SyntacticInteroperability ;
  sto:frames sto:Trustworthiness ;
  sto:isDescribedin sto:OceanProtocol ;
.
sto:OceanSystemViewpointAnno
  a <https://www.w3.org/ns/oaAnnotation> ;
  <https://www.w3.org/ns/oahasBody> sto:OceanSystemViewpoint ;
  <https://www.w3.org/ns/oahasTarget> [
      a <https://www.w3.org/ns/oaSpecificResource> ;
      <https://www.w3.org/ns/oahasSelector> [
          a <https://www.w3.org/ns/oaRangeSelector> ;
          <https://www.w3.org/ns/oahasEndSelector> [
              a <https://www.w3.org/ns/oaXPathSelector> ;
              rdf:value "Page 59" ;
            ] ;
          <https://www.w3.org/ns/oahasStartSelector> [
              a <https://www.w3.org/ns/oaXPathSelector> ;
              rdf:value "Page 1" ;
            ] ;
        ] ;
      <https://www.w3.org/ns/oahasSource> sto:Ocean_Protocol_Technical_Whitepaper_Apr_2019 ;
    ] ;
.
sto:Ocean_Protocol_Business_Strategy_Oct_2017
  a <https://www.w3.org/ns/oaSpecificResource> ;
  rdfs:label "Ocean Protocol: A Decentralized Data Exchange Protocol,powered by blockchain technology and a cryptotoken. Business Strategy. Oct 2017"@en ;
  sto:hasOpenResource <https://oceanprotocol.com/business-strategy.pdf> ;
.
sto:Ocean_Protocol_Reference_Marketplace_Framework_Feb_2019
  a <https://www.w3.org/ns/oaSpecificResource> ;
  rdfs:label "Ocean Protocol: A Decentralized Data Exchange Protocol to Unlock Data for Artificial Intelligence. Reference Marketplace Framework. Feb 2019"@en ;
  sto:hasOpenResource <https://oceanprotocol.com/marketplace-framework.pdf> ;
.
sto:Ocean_Protocol_Technical_Whitepaper_Apr_2019
  a <https://www.w3.org/ns/oaSpecificResource> ;
  rdfs:label "Ocean Protocol: A Decentralized Substrate for AI Data & Services . Technical Whitepaper. Apr 2019"@en ;
  sto:hasOpenResource <https://oceanprotocol.com/tech-whitepaper.pdf> ;
.
sto:OcfCoreFramework
  a owl:NamedIndividual ;
  a sto:OcfBlock ;
  terms:creator sto:sebastian ;
  rdfs:label "OCF Core Framework"@en ;
  sto:frames sto:Communication ;
  sto:frames sto:EndpointInvocation ;
  sto:frames sto:Identification ;
  sto:frames sto:ServiceDiscovery ;
  sto:frames sto:SyntacticInteroperability ;
  sto:isDescribedin :OcfFramework ;
.
sto:OcfCoreFrameworkAnno
  a <https://www.w3.org/ns/oaAnnotation> ;
  <https://www.w3.org/ns/oahasBody> sto:OcfCoreFramework ;
  <https://www.w3.org/ns/oahasTarget> [
      a <https://www.w3.org/ns/oaSpecificResource> ;
      <https://www.w3.org/ns/oahasSelector> [
          a <https://www.w3.org/ns/oaRangeSelector> ;
          <https://www.w3.org/ns/oahasEndSelector> [
              a <https://www.w3.org/ns/oaXPathSelector> ;
              rdf:value "Page 14" ;
            ] ;
          <https://www.w3.org/ns/oahasStartSelector> [
              a <https://www.w3.org/ns/oaXPathSelector> ;
              rdf:value "Page 11" ;
            ] ;
        ] ;
      <https://www.w3.org/ns/oahasSource> sto:OCF_Core_Specification_VERSION_2_0_1 ;
    ] ;
.
sto:OcfDataModels
  a owl:NamedIndividual ;
  a sto:OcfBlock ;
  rdfs:label "OCF Data Models"@en ;
  sto:frames sto:SemanticInteroperability ;
  sto:isDescribedin sto:OcfFramework ;
.
sto:OcfDataModelsAnno
  a <https://www.w3.org/ns/oaAnnotation> ;
  <https://www.w3.org/ns/oahasBody> sto:OcfDataModels ;
  <https://www.w3.org/ns/oahasTarget> [
      a <https://www.w3.org/ns/oaSpecificResource> ;
      <https://www.w3.org/ns/oahasSelector> [
          a <https://www.w3.org/ns/oaRangeSelector> ;
          <https://www.w3.org/ns/oahasEndSelector> [
              a <https://www.w3.org/ns/oaXPathSelector> ;
              rdf:value "Page 14" ;
            ] ;
          <https://www.w3.org/ns/oahasStartSelector> [
              a <https://www.w3.org/ns/oaXPathSelector> ;
              rdf:value "Page 11" ;
            ] ;
        ] ;
      <https://www.w3.org/ns/oahasSource> sto:OCF_Core_Specification_VERSION_2_0_1 ;
    ] ;
.
sto:OcfFramework
  a owl:NamedIndividual ;
  a sto:StandardizationFramework ;
  terms:creator sto:sebastian ;
  rdfs:label "OCF Framework"@en ;
  sto:hasPublisher sto:OpenConnectivityFoundation ;
.
sto:OcfFrameworkAnno
  a <https://www.w3.org/ns/oaAnnotation> ;
  <https://www.w3.org/ns/oahasBody> sto:OcfFramework ;
  <https://www.w3.org/ns/oahasTarget> [
      a <https://www.w3.org/ns/oaSpecificResource> ;
      <https://www.w3.org/ns/oahasSelector> [
          a <https://www.w3.org/ns/oaRangeSelector> ;
          <https://www.w3.org/ns/oahasEndSelector> [
              a <https://www.w3.org/ns/oaXPathSelector> ;
              rdf:value "Page 14" ;
            ] ;
          <https://www.w3.org/ns/oahasStartSelector> [
              a <https://www.w3.org/ns/oaXPathSelector> ;
              rdf:value "Page 11" ;
            ] ;
        ] ;
      <https://www.w3.org/ns/oahasSource> sto:OCF_Core_Specification_VERSION_2_0_1 ;
    ] ;
.
sto:OcfL2Connectivity
  a owl:NamedIndividual ;
  a sto:OcfBlock ;
  rdfs:label "OCF L2 Connectivity"@en ;
  sto:frames sto:Connectivity ;
  sto:frames sto:SyntacticInteroperability ;
  sto:isDescribedin sto:OcfFramework ;
.
sto:OcfL2ConnectivityAnno
  a <https://www.w3.org/ns/oaAnnotation> ;
  <https://www.w3.org/ns/oahasBody> sto:OcfL2Connectivity ;
  <https://www.w3.org/ns/oahasTarget> [
      a <https://www.w3.org/ns/oaSpecificResource> ;
      <https://www.w3.org/ns/oahasSelector> [
          a <https://www.w3.org/ns/oaRangeSelector> ;
          <https://www.w3.org/ns/oahasEndSelector> [
              a <https://www.w3.org/ns/oaXPathSelector> ;
              rdf:value "Page 14" ;
            ] ;
          <https://www.w3.org/ns/oahasStartSelector> [
              a <https://www.w3.org/ns/oaXPathSelector> ;
              rdf:value "Page 11" ;
            ] ;
        ] ;
      <https://www.w3.org/ns/oahasSource> sto:OCF_Core_Specification_VERSION_2_0_1 ;
    ] ;
.
sto:OcfNetworking
  a owl:NamedIndividual ;
  a sto:OcfBlock ;
  terms:creator sto:sebastian ;
  dul:associatedWith sto:IPv6 ;
  rdfs:label "OCF Networking"@en ;
  sto:frames sto:Connectivity ;
  sto:frames sto:IPv6Support ;
  sto:isDescribedin sto:OcfFramework ;
.
sto:OcfNetworkingAnno
  a <https://www.w3.org/ns/oaAnnotation> ;
  <https://www.w3.org/ns/oahasBody> sto:OcfNetworking ;
  <https://www.w3.org/ns/oahasTarget> [
      a <https://www.w3.org/ns/oaSpecificResource> ;
      <https://www.w3.org/ns/oahasSelector> [
          a <https://www.w3.org/ns/oaRangeSelector> ;
          <https://www.w3.org/ns/oahasEndSelector> [
              a <https://www.w3.org/ns/oaXPathSelector> ;
              rdf:value "Page 14" ;
            ] ;
          <https://www.w3.org/ns/oahasStartSelector> [
              a <https://www.w3.org/ns/oaXPathSelector> ;
              rdf:value "Page 11" ;
            ] ;
        ] ;
      <https://www.w3.org/ns/oahasSource> sto:OCF_Core_Specification_VERSION_2_0_1 ;
    ] ;
.
sto:OcfSecurity
  a owl:NamedIndividual ;
  a sto:OcfBlock ;
  terms:creator sto:sebastian ;
  dul:associatedWith sto:RAML ;
  rdfs:label "OCF Security"@en ;
  rdfs:seeAlso <https://openconnectivity.org/industries/ocf-security> ;
  sto:alignsWith rami:Security ;
  sto:alignsWith sto:BdvaCyberSecurityTrust ;
  sto:alignsWith sto:FiwareSecurity ;
  sto:alignsWith sto:IDSRAMSecurity ;
  sto:alignsWith sto:IIRASecurity ;
  sto:alignsWith sto:IIRASecurityFramework ;
  sto:alignsWith sto:IotaTrustSecurityPrivacy ;
  sto:alignsWith sto:OpenFogSecurityPerspective ;
  sto:frames sto:Certification ;
  sto:frames sto:Connectivity ;
  sto:frames sto:SecureCommunication ;
  sto:hasPublisher sto:OpenConnectivityFoundation ;
  sto:isDescribedin sto:OcfFramework ;
.
sto:OcfSecurityAnno
  a <https://www.w3.org/ns/oaAnnotation> ;
  <https://www.w3.org/ns/oahasBody> sto:OcfSecurity ;
  <https://www.w3.org/ns/oahasTarget> [
      a <https://www.w3.org/ns/oaSpecificResource> ;
      <https://www.w3.org/ns/oahasSelector> [
          a <https://www.w3.org/ns/oaRangeSelector> ;
          <https://www.w3.org/ns/oahasEndSelector> [
              a <https://www.w3.org/ns/oaXPathSelector> ;
              rdf:value "Page 14" ;
            ] ;
          <https://www.w3.org/ns/oahasStartSelector> [
              a <https://www.w3.org/ns/oaXPathSelector> ;
              rdf:value "Page 11" ;
            ] ;
        ] ;
      <https://www.w3.org/ns/oahasSource> sto:OCF_Core_Specification_VERSION_2_0_1 ;
    ] ;
.
sto:OpenApi
  a owl:NamedIndividual ;
  a foaf:Document ;
  a sto:Publication ;
  a sto:TechnicalSpecification ;
  terms:creator sto:sebastian ;
  rdfs:comment "The OpenAPI Specification (originally known as the Swagger Specification) is a specification for machine-readable interface files for describing, producing, consuming, and visualizing RESTful web services. A variety of tools can generate code, documentation and test cases given an interface file. Development of the OpenAPI Specification (OAS) is overseen by the Open API Initiative, an open source collaborative project of the Linux Foundation. (source: wikipedia)"@en ;
  rdfs:label "OpenAPI"@en ;
  sto:hasDBpediaResource <http://dbpedia.org/resource/OpenAPI_Specification> ;
.
sto:OpenConnectivityFoundation
  a owl:NamedIndividual ;
  a sto:StandardOrganization ;
  rdfs:comment "The Open Connectivity Foundation (OCF) is an industry group whose stated mission is to develop specification standards, promote a set of interoperability guidelines, and provide a certification program for devices involved in the Internet of Things (IoT). It has become one of the biggest industrial connectivity standards organizations for IoT, including in its membership Samsung Electronics, Intel, Microsoft, Qualcomm and Electrolux. Currently, there are more than 300 member companies. source: wikipedia"@en ;
  rdfs:label "Open Connectivity Foundation" ;
  rdfs:seeAlso <https://openconnectivity.org/> ;
  sto:hasDBpediaResource <https://dbpedia.org/resource/Open_Connectivity_Foundation> ;
.
sto:OpenDaylight
  a owl:NamedIndividual ;
  a foaf:Document ;
  a sto:Publication ;
  a sto:TechnicalSpecification ;
  terms:creator sto:sebastian ;
  terms:creator "sebastian" ;
.
sto:OpenFogArchitecture
  a owl:NamedIndividual ;
  a sto:Publication ;
  dc11:title "OpenFog Architecture Overview"@en ;
  terms:creator sto:sebastian ;
  rdfs:comment "The OpenFog Architecture is a system-level architecture that extends elements of compute, networking and storage across the cloud through to the edge of the network. This approach is particularly suited to IoT systems and accelerates the decision-making velocity. This architecture serves a specific subset of business problems that can’t be successfully implemented using “cloud only” based architectures or relying solely on intelligent edge devices. OpenFog should be thought of as complementary to, and an extension of the traditional cloud based model where implementations of the architecture can reside in multiple layers of a network’s topology. The goal of the OpenFog architecture is to facilitate deployments which highlight interoperability, performance, security, scalability, programmability, reliability, availability, serviceability, and agility. Proprietary or single vendor solutions can result in limited supplier diversity, which can have a negative impact on market adoption, system cost, quality and innovation."@en ;
  rdfs:label "OpenFog Architecture Whitepaper" ;
  sto:hasDBpediaResource <http://dbpedia.org/resource/OpenFog_Consortium> ;
  sto:hasOfficialResource <https://www.openfogconsortium.org/white-paper-reference-architecture/white-paper-download-open-fog-reference-architecture/> ;
  sto:hasPublisher sto:OpenFogConsortium ;
.
sto:OpenFogConsortium
  a owl:NamedIndividual ;
  a sto:IIoTConsortium ;
  rdfs:comment "The OpenFog Consortium work is done by committees and workgroups focused on specific tasks aligned to our mission. This work includes technical work; influencing standards development through liaisons with other organizations; testbed; promoting innovation and industry interest in fog computing; and industry education."@en ;
  rdfs:label "OpenFog Consortium" ;
  rdfs:label "OpenFog Consortium"@en ;
  sto:hasOfficialResource <https://www.openfogconsortium.org/> ;
  sto:seeAlso <https://www.openfogconsortium.org/> ;
.
sto:OpenFogReferenceArchitecture
  a owl:NamedIndividual ;
  a sto:ArchitectureDescription ;
  a sto:StandardizationFramework ;
  terms:creator sto:sebastian ;
  rdfs:comment "The OpenFog Reference Architecture (OpenFog RA) is intended to help business leaders, software developers, silicon architects, and system designers create and maintain the hardware, software and system elements necessary for fog computing."@en ;
  rdfs:label "OpenFog Reference Architecture"@en ;
  sto:hasOfficialResource <https://www.openfogconsortium.org/ra/> ;
  sto:hasPublisher :OpenFogConsortium ;
.
sto:OpenFog_Reference_Architecture_for_Fog_Computing
  a <https://www.w3.org/ns/oaSpecificResource> ;
  rdfs:label "OpenFog Reference Architecture for Fog Computing"@en ;
  sto:hasOpenResource <https://www.openfogconsortium.org/wp-content/uploads/OpenFog_Reference_Architecture_2_09_17-FINAL.pdf> ;
.
sto:OpenLicenseDocument
  a terms:LicenseDocument ;
  a owl:NamedIndividual ;
  rdfs:comment "Open or Free License"@en ;
  rdfs:label "Open or Free License"@en ;
  rdfs:seeAlso <https://en.wikipedia.org/wiki/Free_license> ;
.
sto:OpenWSN
  a owl:NamedIndividual ;
  a foaf:Document ;
  a sto:Publication ;
  a sto:TechnicalSpecification ;
  terms:creator sto:sebastian ;
  rdfs:comment "OpenWSN Serves as a repository for open-source implementations of protocol stacks based on Internet of Things standards, using a variety of hardware and software platforms. (source: https://www.postscapes.com/internet-of-things-protocols/)"@en ;
  rdfs:label "OpenWSN"@en ;
  sto:hasOfficialResource <https://openwsn.atlassian.net/wiki/pages/viewpage.action?pageId=688187> ;
.
sto:OrionContextBroker
  a owl:NamedIndividual ;
  a foaf:Document ;
  a sto:Publication ;
  a sto:TechnicalSpecification ;
  terms:creator sto:sebastian ;
  dul:associatedWith sto:FIWARE ;
  rdfs:label "ORION Context Broker"@en ;
.
sto:Performance
  a owl:NamedIndividual ;
  a sto:Concern ;
  terms:creator sto:MuhammadUsman ;
  rdfs:comment "Performance is completion of a task with application of knowledge, skills and abilities"@en ;
  rdfs:label "Performance"@en ;
  rdfs:seeAlso "https://ieeexplore.ieee.org/document/8249113"@en ;
  rdfs:seeAlso "https://ieeexplore.ieee.org/document/8463303"@en ;
  sto:hasWikipediaArticle "https://en.wikipedia.org/wiki/Performance"@en ;
  sto:supports sto:BusinessContext ;
.
sto:PeriodicCommunication
  a owl:NamedIndividual ;
  a sto:Concern ;
  <http://voag.linkedmodel.org/voag#hasStakeholder> <https://www.wikidata.org/wiki/Q1548249> ;
  rdfs:label "Periodic Communication"@en ;
  rdfs:seeAlso "IoT-A Requirement UNI.005" ;
  sto:supports sto:EventDrivenMessaging ;
.
sto:PhysicalConnectivity
  a owl:NamedIndividual ;
  a sto:Concern ;
  terms:creator sto:sebastian ;
  rdfs:comment "Physical Connectivity is the concern including all aspects of low-level connectivity and transporting a physical (electrical) signal from A to B. This might be achieved through wired connections (e.g. ethernet) but also wireless (e.g. WIFI)."@en ;
  rdfs:label "Physical Connectivity"@en ;
  sto:supports sto:Interoperability ;
.
sto:PhysicalWeb
  a owl:NamedIndividual ;
  a foaf:Document ;
  a sto:Publication ;
  a sto:TechnicalSpecification ;
  terms:creator sto:sebastian ;
  rdfs:comment "Physical Web - The Physical Web enables you to see a list of URLs being broadcast by objects in the environment around you with a Bluetooth Low Energy (BLE) beacon. (source: https://www.postscapes.com/internet-of-things-protocols/)"@en ;
  rdfs:label "Physical Web"@en ;
  sto:hasOfficialResource <https://google.github.io/physical-web/faq> ;
.
sto:PlantManager
  rdfs:comment " A plant manager is responsible for the functioning of a plant/facility." ;
  rdfs:label "Plant Manager"@en ;
  rdfs:seeAlso "IIC:PUB:G1:V1.80:20170131" ;
  rdfs:type sto:Stakeholder ;
  skos:altLabel "Facility Manager"@en ;
  skos:note "Publications referred: 'IIC:PUB:G1:V1.80:20170131' '1.5 AUDIENCE' 'Page 7' " ;
  sto:hasWikipediaArticle "https://en.wikipedia.org/wiki/Facility_management#Role_of_the_facilities_manager" ;
.
sto:PlatformIndustry40
  a owl:NamedIndividual ;
  a foaf:Organization ;
  a sto:IIoTConsortium ;
  terms:creator sto:sebastian ;
  terms:creator "sebastian" ;
  dul:associatedWith sto:RAMI ;
  rdfs:label "Platform Industry 4.0"@en ;
  rdfs:label "Plattform Industrie 4.0"@de ;
.
sto:Privacy
  a owl:NamedIndividual ;
  a sto:Concern ;
  terms:creator sto:sebastian ;
  rdfs:comment "Information privacy, or data privacy (or data protection), is the relationship between collection and dissemination of data, technology, the public expectation of privacy, and the legal and political issues surrounding them. Privacy concerns exist wherever personally identifiable information or other sensitive information is collected, stored, used, and finally destroyed or deleted – in digital form or otherwise. Improper or non-existent disclosure control can be the root cause for privacy issues. Data privacy issues can arise in response to information from a wide range of sources, such as: * Healthcare records * Criminal justice investigations and proceedings * Financial institutions and transactions * Biological traits, such as genetic material * Residence and geographic records * Ethnicity * Privacy breach * Location-based service and geolocation * Web surfing behavior or user preferences using persistent cookies. (source: wikipedia)"@en ;
  rdfs:label "Privacy"@en ;
  rdfs:seeAlso "IoT-A Requirement UNI.423" ;
  rdfs:seeAlso "IoT-A Requirement UNI.424" ;
  rdfs:seeAlso "IoT-A Requirement UNI.606" ;
  rdfs:seeAlso "IoT-A Requirement UNI.623" ;
  rdfs:seeAlso "https://dl.acm.org/citation.cfm?doid=3098208.3098210" ;
  rdfs:seeAlso "https://ieeexplore.ieee.org/document/6188257"@en ;
  rdfs:seeAlso "https://ieeexplore.ieee.org/document/7919553"@en ;
  sto:hasDBpediaResource <http://dbpedia.org/resource/Information_privacy> ;
  sto:supports sto:DataSovereignty ;
  sto:supports sto:Trustworthiness ;
.
sto:PrivateLicenseDocument
  a terms:LicenseDocument ;
  a owl:NamedIndividual ;
  rdfs:comment "Published under a Private License."@en ;
  rdfs:label "Private License"@en ;
  rdfs:seeAlso <https://en.wikipedia.org/wiki/Trade_secret> ;
.
sto:Priyanka
  a owl:NamedIndividual ;
  a foaf:Person ;
  rdfs:label "Priyanka Nanjappa"@en ;
  foaf:familyName "Nanjappa" ;
  foaf:name sto:Priyanka ;
  foaf:name "Priyanka" ;
.
sto:ProcessIsolation
  a owl:NamedIndividual ;
  a sto:Concern ;
  terms:creator sto:MuhammadUsman ;
  rdfs:comment "\"Isolation would be another issue at the edge of the network. In mobile OS, if an application fails or crashes, the whole system will usually crash and reboot. Or in a distributed system the shared resource could be managed with different synchronization mechanisms such as a lock or token ring. \""@en ;
  rdfs:label "Isolation"@en ;
  rdfs:seeAlso "https://ieeexplore.ieee.org/document/7488250" ;
  sto:hasWikipediaArticle "https://en.wikipedia.org/wiki/Process_isolation"@en ;
  sto:supports sto:IntegrityProtection ;
.
sto:ProductCatalogData
  a owl:NamedIndividual ;
  a sto:ProductDevelopmentLifeCycle ;
  a sto:StandardClassification ;
  rdfs:comment "Product catalog data standards support the description of particular instances of products or parts in a uniform, vendor-neutral way."@en ;
  rdfs:label "Product Catalog Data"@en ;
  sto:isDescribedin sto:NISTInitiative ;
.
sto:ProductDevelopmentLifeCycle
  a owl:Class ;
  rdfs:comment "PLM is the process of managing the entire lifecycle of a product from inception, through engineering design and manufacture, to service and disposal of manufactured products. Related areas are PLMManagement, Modeling Practice, Product Model Data exchange, Manufacturing Model Data, Product Catalog Data."@en ;
  rdfs:comment "Product Development Life-Cycle Phase"@en ;
  rdfs:isDefinedBy "https://en.wikipedia.org/wiki/Product_lifecycle" ;
  rdfs:label "Product Development Life Cycle"@en ;
  rdfs:subClassOf sto:StandardClassification ;
.
sto:ProductLiability
  a owl:NamedIndividual ;
  a sto:Concern ;
  rdfs:label "Product Liability"@en ;
  skos:note "Publications referred: '(IIC:PUB:G1:V1.80:20170131' '4 BUSINESS VIEWPOINT' 'Page 20' " ;
  sto:supports sto:BusinessContext ;
.
sto:ProductLifeCycleManagement
  a owl:NamedIndividual ;
  a sto:ProductDevelopmentLifeCycle ;
  a sto:StandardClassification ;
  rdfs:comment "Product lifecycle data management focuses on the needs of long-term retention and access to data consistently throughout the product lifecycle."@en ;
  rdfs:label "Production Life Cycle Management"@en ;
  sto:isDescribedin sto:NISTInitiative ;
.
sto:ProductManager
  a <http://voag.linkedmodel.org/voag#StakeholderGroup> ;
  a owl:NamedIndividual ;
  a sto:Stakeholder ;
  rdfs:comment ""@en ;
  rdfs:label "Product Manager"@en ;
  skos:note "Publications referred: '(IIC:PUB:G1:V1.80:20170131' '3.5.1 BUSINESS VIEWPOINT' 'Page 15' 'Priyanka'" ;
.
sto:ProductModelDataExchange
  a owl:NamedIndividual ;
  a sto:ProductDevelopmentLifeCycle ;
  a sto:StandardClassification ;
  rdfs:comment "These standards capture the representation of product and engineering information to enable data exchange between CAD software from different vendors."@en ;
  rdfs:label "Product Model Data Exchange"@en ;
  sto:isDescribedin sto:NISTInitiative ;
.
sto:ProductionLifeCycleDataManagement
  a owl:NamedIndividual ;
  a sto:ProductionSystemLifeCycle ;
  a sto:StandardClassification ;
  rdfs:comment "Production lifecycle data management standards define general models of data integration, sharing, exchange, and hand-over for lifecycle support of production facilities."@en ;
  rdfs:label "Production Life Cycle Data Management"@en ;
  sto:isDescribedin sto:NISTInitiative ;
.
sto:ProductionSystemEngineering
  a owl:NamedIndividual ;
  a sto:ProductionSystemLifeCycle ;
  a sto:StandardClassification ;
  rdfs:comment "Standards can interconnect engineering tools from different disciplines, e.g., system engineering, mechanical plant engineering, electrical design, process engineering, process control engineering, Human Machine Interface (HMI) development, PLC programming, and robotic programming."@en ;
  rdfs:label "Production System Engineering"@en ;
  sto:isDescribedin sto:NISTInitiative ;
.
sto:ProductionSystemLifeCycle
  a owl:Class ;
  rdfs:comment "Collections of machines, equipment, and auxiliary systems organized to create goods and services from various resources."@en ;
  rdfs:isDefinedBy <http://nvlpubs.nist.gov/nistpubs/ir/2016/NIST.IR.8107.pdf> ;
  rdfs:label "Production System Life Cycle"@en ;
  rdfs:subClassOf sto:StandardClassification ;
.
sto:ProductionSystemMaintenance
  a owl:NamedIndividual ;
  a sto:ProductionSystemLifeCycle ;
  a sto:StandardClassification ;
  rdfs:comment "Classifies standards define data processing, communication, and presentation standards for condition monitoring and diagnostics of machines, for maintaining the adequate performance of the system, and for searching ways to improve performance"@en ;
  rdfs:label "Production System Maintenance"@en ;
  sto:isDescribedin sto:NISTInitiative ;
.
sto:ProductionSystemModelData
  a owl:NamedIndividual ;
  a sto:ProductionSystemLifeCycle ;
  a sto:StandardClassification ;
  rdfs:comment "Provide information models for factory and production system design. They enhance information exchange among stakeholders, and enable virtual commissioning, which can improve manufacturing agility and reduce manufacturing cost."@en ;
  rdfs:label "Production System Model Data"@en ;
  sto:isDescribedin sto:NISTInitiative ;
.
sto:Programmability
  a owl:NamedIndividual ;
  a sto:Concern ;
  dul:isComponentOf sto:EdgeComputing ;
  rdfs:comment "In the edge computing, computation is offloaded from the cloud, and the edge nodes are most likely heterogeneous platforms. In this case, the runtime of these nodes differ from each other, and the programmer faces huge difficulties to write an application that may be deployed in the edge computing paradigm." ;
  rdfs:label "Programmability" ;
  rdfs:seeAlso "https://dl.acm.org/citation.cfm?doid=3210240.3226062" ;
  rdfs:seeAlso "https://ieeexplore.ieee.org/document/7488250" ;
  skos:note "Publications referred: ' <https://www.openfogconsortium.org/wp-content/uploads/OpenFog_Reference_Architecture_2_09_17-FINAL.pdf> OPFRA001.020817' '4.5 Programmability Pillar' 'Page 29' " ;
  sto:supports sto:EdgeComputing ;
.
sto:ProjectManager
  a <http://voag.linkedmodel.org/voag#StakeholderGroup> ;
  a owl:NamedIndividual ;
.
sto:ProvenanceTracking
  a owl:NamedIndividual ;
  a sto:Concern ;
  terms:creator sto:sebastian ;
  <http://voag.linkedmodel.org/voag#hasStakeholder> <http://purl.oclc.org/NET/mvco.owl#EndUser> ;
  rdfs:comment "Data provenance includes the data's origins, what happens to it and where it moves/moved over time."@en ;
  rdfs:label "Provenance Tracking"@en ;
  rdfs:seeAlso "IoT-A Requirement UNI.041" ;
  rdfs:seeAlso "IoT-A Requirement UNI.606" ;
  sto:hasDBpediaResource <http://dbpedia.org/resource/Data_lineage> ;
  sto:supports sto:Security ;
.
sto:Pseudonimity
  a owl:NamedIndividual ;
  a sto:Concern ;
  terms:creator sto:sebastian ;
  rdfs:comment "While complete anonymity is not feasibe in an IoT scenario, pseudonimity should be supported."@en ;
  rdfs:label "Pseudonimity"@en ;
  rdfs:seeAlso "IoT-A Requirement UNI.624" ;
  sto:hasDBpediaResource <http://dbpedia.org/resource/Pseudonymity> ;
  sto:supports sto:Anonymity ;
.
sto:PublicLicenseDocument
  a terms:LicenseDocument ;
  a owl:NamedIndividual ;
  rdfs:comment "Published under a Public License."@en ;
  rdfs:label "Public License"@en ;
  rdfs:seeAlso <https://en.wikipedia.org/wiki/Public_copyright_license> ;
.
sto:Publication
  a owl:Class ;
  rdfs:comment """Specifies a Publication. E.g., International Standards,Technical Specifications,Publicly Available Specifications,Amendments
                Technical Corrigenda,Interpretation Sheets,Technical Reports,Guides"""@en ;
  rdfs:isDefinedBy sto:IEC ;
  rdfs:label "Publication"@en ;
  rdfs:seeAlso <http://www.iec.ch/standardsdev/publications/> ;
  rdfs:subClassOf foaf:Document ;
.
sto:QIF
  a owl:NamedIndividual ;
  a foaf:Document ;
  a sto:Publication ;
  a sto:Standard ;
  terms:creator sto:DMSC ;
  rdfs:comment " Quality Information Framework (QIF) standard defines an integrated set of information models which enable the effective exchange of metrology data throughout the entire manufacturing quality measurement process"@en ;
  rdfs:isDefinedBy "http://qifstandards.org/about-qif/" ;
  rdfs:label "Quality Information Framework"@en ;
  skos:note "Is implemented in XML" ;
  foaf:maker sto:DMSC ;
  sto:hasOfficialResource <http://qifstandards.org/> ;
  sto:hasPublisher sto:DMSC ;
.
sto:QUIC
  a owl:NamedIndividual ;
  a foaf:Document ;
  a sto:Publication ;
  a sto:TechnicalSpecification ;
  terms:creator sto:sebastian ;
  rdfs:comment "QUIC (Quick UDP Internet Connections, pronounced quick) supports a set of multiplexed connections between two endpoints over User Datagram Protocol (UDP), and was designed to provide security protection equivalent to TLS/SSL, along with reduced connection and transport latency, and bandwidth estimation in each direction to avoid congestion. (source: https://www.postscapes.com/internet-of-things-protocols/)"@en ;
  rdfs:label "QUIC"@en ;
  sto:hasOfficialResource <https://en.wikipedia.org/wiki/QUIC> ;
.
sto:QualityOfService
  a owl:NamedIndividual ;
  a sto:Concern ;
  rdfs:comment "Quality of service (QoS) is the overall performance of a telephony or computer network, particularly the performance seen by the users of the network. To quantitatively measure quality of service, several related aspects of the network service are often considered, such as error rates, bit rate, throughput, transmission delay, availability, jitter, etc. In the field of computer networking and other packet-switched telecommunication networks, quality of service refers to traffic prioritization and resource reservation control mechanisms rather than the achieved service quality. (source: wikipedia)"@en ;
  rdfs:label "Quality of Service"@en ;
  rdfs:seeAlso "IoT-A Requirement UNI.613" ;
  rdfs:seeAlso "IoT-A Requirement UNI.614" ;
  rdfs:seeAlso "IoT-A Requirement UNI.717" ;
  rdfs:seeAlso "https://dl.acm.org/citation.cfm?doid=3098208.3098210" ;
  rdfs:seeAlso "https://dl.acm.org/citation.cfm?doid=3266237.3266263"@en ;
  rdfs:seeAlso "https://ieeexplore.ieee.org/document/7919553"@en ;
  sto:hasDBpediaResource <http://dbpedia.org/resource/Quality_of_service> ;
  sto:supports sto:ServiceDescription ;
.
sto:RAMI
  a owl:NamedIndividual ;
  a sto:StandardizationFramework ;
  rdfs:comment "Describes the RAMI model"@en ;
  rdfs:comment "Describes the Reference Architecture Model for Industry 4.0, i.e., the RAMI Initiative."@en ;
  rdfs:isDefinedBy "https://www.plattform-i40.de/I40/Redaktion/EN/Downloads/Publikation/structure-of-the-administration-shell.html" ;
  rdfs:label "RAMI 4.0"@en ;
  sto:hasPublisher sto:PlatformIndustry40 ;
.
sto:RAMIAssetlayer
  a owl:NamedIndividual ;
  a rami:RAMIITLayer ;
  a sto:StandardClassification ;
  dul:associatedWith rami:Lifecycle_Status ;
  dul:associatedWith sto:EdgecrossFacilityLayer ;
  dul:associatedWith sto:IIRAPhysicalSystems ;
  dul:associatedWith sto:IotaFunctionalViewpoint ;
  dul:associatedWith sto:IviAssetView ;
  rdfs:label "RAMI Asset Layer"@en ;
  sto:alignsWith sto:EdgecrossFacilityLayer ;
  sto:alignsWith sto:IIRAPhysicalSystems ;
  sto:alignsWith sto:IotaFunctionalViewpoint ;
  sto:alignsWith sto:IviAssetView ;
  sto:frames sto:Communication ;
  sto:frames sto:Identification ;
  sto:frames sto:IdentityManagement ;
  sto:frames sto:Interoperability ;
  sto:frames sto:Security ;
  sto:frames sto:SemanticInteroperability ;
  sto:frames sto:ThingDescription ;
  sto:frames sto:ThingRepresentation ;
  sto:frames sto:Trustworthiness ;
  sto:frames sto:VirtualEntity ;
  sto:isDescribedin sto:RAMI ;
.
sto:RAMIAssetlayerAnno
  a <https://www.w3.org/ns/oaAnnotation> ;
  <https://www.w3.org/ns/oahasBody> sto:RAMIAssetlayer ;
  <https://www.w3.org/ns/oahasTarget> [
      a <https://www.w3.org/ns/oaSpecificResource> ;
      terms:format "pdf" ;
      <https://www.w3.org/ns/oahasSelector> [
          a <https://www.w3.org/ns/oaRangeSelector> ;
          <https://www.w3.org/ns/oahasEndSelector> [
              a <https://www.w3.org/ns/oaXPathSelector> ;
              rdf:value "Page 23" ;
            ] ;
          <https://www.w3.org/ns/oahasStartSelector> [
              a <https://www.w3.org/ns/oaXPathSelector> ;
              rdf:value "Page 22" ;
            ] ;
        ] ;
      <https://www.w3.org/ns/oahasSource> sto:DIN_SPEC_91345 ;
    ] ;
.
sto:RAMIBody
  a owl:NamedIndividual ;
  a sto:StandardizationFramework ;
  dul:isPartOf sto:AdministrationShell ;
  rdfs:comment "TODO: Find better class assignement"@en ;
  rdfs:label "Administration Shell Body"@en ;
  sto:hasPublisher sto:PlatformIndustry40 ;
.
sto:RAMIBodyAnno
  a <https://www.w3.org/ns/oaAnnotation> ;
  <https://www.w3.org/ns/oahasBody> sto:RAMIBody ;
  <https://www.w3.org/ns/oahasTarget> [
      a <https://www.w3.org/ns/oaSpecificResource> ;
      terms:format "pdf" ;
      <https://www.w3.org/ns/oahasSelector> [
          a <https://www.w3.org/ns/oaRangeSelector> ;
          <https://www.w3.org/ns/oahasEndSelector> [
              a <https://www.w3.org/ns/oaXPathSelector> ;
              rdf:value "Page 31" ;
            ] ;
          <https://www.w3.org/ns/oahasStartSelector> [
              a <https://www.w3.org/ns/oaXPathSelector> ;
              rdf:value "Page 30" ;
            ] ;
        ] ;
      <https://www.w3.org/ns/oahasSource> sto:DIN_SPEC_91345 ;
    ] ;
.
sto:RAMIBusinessLayer
  a owl:NamedIndividual ;
  a rami:RAMIITLayer ;
  a sto:StandardClassification ;
  dul:associatedWith sto:IDSRAMBusinessLayer ;
  dul:associatedWith sto:IDSRAMGovernance ;
  dul:associatedWith sto:IIRABusinessDomain ;
  dul:associatedWith sto:IviBusinessLayer ;
  rdfs:label "RAMI Business Layer"@en ;
  sto:alignsWith sto:IDSRAMBusinessLayer ;
  sto:alignsWith sto:IDSRAMGovernance ;
  sto:alignsWith sto:IIRABusinessDomain ;
  sto:alignsWith sto:IviBusinessLayer ;
  sto:frames rami:ProcessPlanning ;
  sto:frames sto:BusinessContext ;
  sto:frames sto:ServiceComposition ;
  sto:frames sto:ServiceOrchestration ;
  sto:isDescribedin sto:RAMI ;
.
sto:RAMIBusinessLayerAnno
  a <https://www.w3.org/ns/oaAnnotation> ;
  <https://www.w3.org/ns/oahasBody> sto:RAMIBusinessLayer ;
  <https://www.w3.org/ns/oahasTarget> [
      a <https://www.w3.org/ns/oaSpecificResource> ;
      terms:format "pdf" ;
      <https://www.w3.org/ns/oahasSelector> [
          a <https://www.w3.org/ns/oaRangeSelector> ;
          <https://www.w3.org/ns/oahasEndSelector> [
              a <https://www.w3.org/ns/oaXPathSelector> ;
              rdf:value "Page 21" ;
            ] ;
          <https://www.w3.org/ns/oahasStartSelector> [
              a <https://www.w3.org/ns/oaXPathSelector> ;
              rdf:value "Page 20" ;
            ] ;
        ] ;
      <https://www.w3.org/ns/oahasSource> sto:DIN_SPEC_91345 ;
    ] ;
.
sto:RAMICommunicationlayer
  a owl:NamedIndividual ;
  a rami:RAMIITLayer ;
  a sto:StandardClassification ;
  dul:associatedWith sto:FiwareIotServicesEnablement ;
  dul:associatedWith sto:IDSRAMSystemLayer ;
  dul:associatedWith sto:IIRAConnectivity ;
  dul:associatedWith sto:IIRADistributedDataManagement ;
  dul:associatedWith sto:IotaInformationViewpoint ;
  rdfs:label "RAMI Communication Layer"@en ;
  sto:alignsWith sto:FiwareIotServicesEnablement ;
  sto:alignsWith sto:IDSRAMSystemLayer ;
  sto:alignsWith sto:IIRAConnectivity ;
  sto:alignsWith sto:IIRADistributedDataManagement ;
  sto:alignsWith sto:IotaInformationViewpoint ;
  sto:frames sto:DataAccess ;
  sto:frames sto:EndpointInvocation ;
  sto:frames sto:Interoperability ;
  sto:frames sto:ProvenanceTracking ;
  sto:frames sto:Security ;
  sto:frames sto:SyntacticInteroperability ;
  sto:frames sto:Trustworthiness ;
  sto:isDescribedin sto:RAMI ;
.
sto:RAMICommunicationlayerAnno
  a <https://www.w3.org/ns/oaAnnotation> ;
  <https://www.w3.org/ns/oahasBody> sto:RAMICommunicationlayer ;
  <https://www.w3.org/ns/oahasTarget> [
      a <https://www.w3.org/ns/oaSpecificResource> ;
      terms:format "pdf" ;
      <https://www.w3.org/ns/oahasSelector> [
          a <https://www.w3.org/ns/oaRangeSelector> ;
          <https://www.w3.org/ns/oahasEndSelector> [
              a <https://www.w3.org/ns/oaXPathSelector> ;
              rdf:value "Page 22" ;
            ] ;
          <https://www.w3.org/ns/oahasStartSelector> [
              a <https://www.w3.org/ns/oaXPathSelector> ;
              rdf:value "Page 21" ;
            ] ;
        ] ;
      <https://www.w3.org/ns/oahasSource> sto:DIN_SPEC_91345 ;
    ] ;
.
sto:RAMIConnectedWorld
  a owl:NamedIndividual ;
  a rami:RAMIHierarchyLevel ;
  a sto:StandardClassification ;
  sto:frames sto:Interoperability ;
  sto:frames sto:SemanticInteroperability ;
  sto:frames sto:ThingDescription ;
  sto:isDescribedin sto:RAMI ;
.
sto:RAMIConnectedWorldAnno
  a <https://www.w3.org/ns/oaAnnotation> ;
  <https://www.w3.org/ns/oahasBody> sto:RAMIConnectedWorld ;
  <https://www.w3.org/ns/oahasTarget> [
      a <https://www.w3.org/ns/oaSpecificResource> ;
      terms:format "pdf" ;
      <https://www.w3.org/ns/oahasSelector> [
          a <https://www.w3.org/ns/oaRangeSelector> ;
          <https://www.w3.org/ns/oahasEndSelector> [
              a <https://www.w3.org/ns/oaXPathSelector> ;
              rdf:value "Page 24" ;
            ] ;
          <https://www.w3.org/ns/oahasStartSelector> [
              a <https://www.w3.org/ns/oaXPathSelector> ;
              rdf:value "Page 23" ;
            ] ;
        ] ;
      <https://www.w3.org/ns/oahasSource> sto:DIN_SPEC_91345 ;
    ] ;
.
sto:RAMIControlDevice
  a owl:NamedIndividual ;
  a rami:RAMIHierarchyLevel ;
  a sto:StandardClassification ;
  sto:isDescribedin sto:RAMI ;
.
sto:RAMIControlDeviceAnno
  a <https://www.w3.org/ns/oaAnnotation> ;
  <https://www.w3.org/ns/oahasBody> sto:RAMIControlDevice ;
  <https://www.w3.org/ns/oahasTarget> [
      a <https://www.w3.org/ns/oaSpecificResource> ;
      terms:format "pdf" ;
      <https://www.w3.org/ns/oahasSelector> [
          a <https://www.w3.org/ns/oaRangeSelector> ;
          <https://www.w3.org/ns/oahasEndSelector> [
              a <https://www.w3.org/ns/oaXPathSelector> ;
              rdf:value "Page 24" ;
            ] ;
          <https://www.w3.org/ns/oahasStartSelector> [
              a <https://www.w3.org/ns/oaXPathSelector> ;
              rdf:value "Page 23" ;
            ] ;
        ] ;
      <https://www.w3.org/ns/oahasSource> sto:DIN_SPEC_91345 ;
    ] ;
.
sto:RAMIEnterprise
  a owl:NamedIndividual ;
  a rami:RAMIHierarchyLevel ;
  a sto:StandardClassification ;
  sto:isDescribedin sto:RAMI ;
.
sto:RAMIEnterpriseAnno
  a <https://www.w3.org/ns/oaAnnotation> ;
  <https://www.w3.org/ns/oahasBody> sto:RAMIEnterprise ;
  <https://www.w3.org/ns/oahasTarget> [
      a <https://www.w3.org/ns/oaSpecificResource> ;
      terms:format "pdf" ;
      <https://www.w3.org/ns/oahasSelector> [
          a <https://www.w3.org/ns/oaRangeSelector> ;
          <https://www.w3.org/ns/oahasEndSelector> [
              a <https://www.w3.org/ns/oaXPathSelector> ;
              rdf:value "Page 24" ;
            ] ;
          <https://www.w3.org/ns/oahasStartSelector> [
              a <https://www.w3.org/ns/oaXPathSelector> ;
              rdf:value "Page 23" ;
            ] ;
        ] ;
      <https://www.w3.org/ns/oahasSource> sto:DIN_SPEC_91345 ;
    ] ;
.
sto:RAMIFieldDevice
  a owl:NamedIndividual ;
  a rami:RAMIHierarchyLevel ;
  a sto:StandardClassification ;
  sto:frames sto:Manufacturing ;
  sto:isDescribedin sto:RAMI ;
.
sto:RAMIFieldDeviceAnno
  a <https://www.w3.org/ns/oaAnnotation> ;
  <https://www.w3.org/ns/oahasBody> sto:RAMIFieldDevice ;
  <https://www.w3.org/ns/oahasTarget> [
      a <https://www.w3.org/ns/oaSpecificResource> ;
      terms:format "pdf" ;
      <https://www.w3.org/ns/oahasSelector> [
          a <https://www.w3.org/ns/oaRangeSelector> ;
          <https://www.w3.org/ns/oahasEndSelector> [
              a <https://www.w3.org/ns/oaXPathSelector> ;
              rdf:value "Page 24" ;
            ] ;
          <https://www.w3.org/ns/oahasStartSelector> [
              a <https://www.w3.org/ns/oaXPathSelector> ;
              rdf:value "Page 23" ;
            ] ;
        ] ;
      <https://www.w3.org/ns/oahasSource> sto:DIN_SPEC_91345 ;
    ] ;
.
sto:RAMIFunctionalLayer
  a owl:NamedIndividual ;
  a rami:RAMIITLayer ;
  a sto:StandardClassification ;
  dul:associatedWith sto:BdvaDataAnalytics ;
  dul:associatedWith sto:BdvaDataViualisationAndUserInteraction ;
  dul:associatedWith sto:DtpSystemView ;
  dul:associatedWith sto:IDSRAMProcessLayer ;
  dul:associatedWith sto:IIRAApplicationDomain ;
  dul:associatedWith sto:IIRAOperationsDomain ;
  dul:associatedWith sto:IotaFunctionalViewpoint ;
  dul:associatedWith sto:IviManagementView ;
  dul:associatedWith sto:NgsiLdDataRepresentation ;
  dul:associatedWith sto:OceanSystemViewpoint ;
  dul:associatedWith sto:xRoadSystemComponents ;
  rdfs:label "RAMI Functional Layer"@en ;
  sto:alignsWith sto:BdvaDataAnalytics ;
  sto:alignsWith sto:BdvaDataViualisationAndUserInteraction ;
  sto:alignsWith sto:DtpSystemView ;
  sto:alignsWith sto:IDSRAMProcessLayer ;
  sto:alignsWith sto:IIRAApplicationDomain ;
  sto:alignsWith sto:IIRAOperationsDomain ;
  sto:alignsWith sto:IotaFunctionalViewpoint ;
  sto:alignsWith sto:IviManagementView ;
  sto:alignsWith sto:NgsiLdDataRepresentation ;
  sto:alignsWith sto:OceanSystemViewpoint ;
  sto:alignsWith sto:xRoadSystemComponents ;
  sto:frames sto:EndpointDescription ;
  sto:frames sto:Interoperability ;
  sto:frames sto:RoleCategorization ;
  sto:frames sto:SemanticInteroperability ;
  sto:frames sto:ServiceDescription ;
  sto:isDescribedin sto:RAMI ;
.
sto:RAMIFunctionalLayerAnno
  a <https://www.w3.org/ns/oaAnnotation> ;
  <https://www.w3.org/ns/oahasBody> sto:RAMIFunctionalLayer ;
  <https://www.w3.org/ns/oahasTarget> [
      a <https://www.w3.org/ns/oaSpecificResource> ;
      terms:format "pdf" ;
      <https://www.w3.org/ns/oahasSelector> [
          a <https://www.w3.org/ns/oaRangeSelector> ;
          <https://www.w3.org/ns/oahasEndSelector> [
              a <https://www.w3.org/ns/oaXPathSelector> ;
              rdf:value "Page 21" ;
            ] ;
          <https://www.w3.org/ns/oahasStartSelector> [
              a <https://www.w3.org/ns/oaXPathSelector> ;
              rdf:value "Page 20" ;
            ] ;
        ] ;
      <https://www.w3.org/ns/oahasSource> sto:DIN_SPEC_91345 ;
    ] ;
.
sto:RAMIHeader
  a owl:NamedIndividual ;
  a sto:StandardClassification ;
  a sto:StandardizationFramework ;
  dul:isPartOf sto:AdministrationShell ;
  rdfs:label "Administration Shell Header"@en ;
  skos:note "find better class assignment"@en ;
  sto:frames rami:Lifecycle_Status ;
  sto:frames sto:BusinessContext ;
  sto:frames sto:DataAccess ;
  sto:frames sto:EndpointInvocation ;
  sto:frames sto:Identification ;
  sto:frames sto:IdentityManagement ;
  sto:frames sto:Interoperability ;
  sto:frames sto:Security ;
  sto:frames sto:SemanticInteroperability ;
  sto:frames sto:SyntacticInteroperability ;
  sto:frames sto:ThingDescription ;
  sto:frames sto:ThingRepresentation ;
  sto:frames sto:Trustworthiness ;
  sto:hasPublisher sto:PlatformIndustry40 ;
.
sto:RAMIHeaderAnno
  a <https://www.w3.org/ns/oaAnnotation> ;
  <https://www.w3.org/ns/oahasBody> sto:RAMIHeader ;
  <https://www.w3.org/ns/oahasTarget> [
      a <https://www.w3.org/ns/oaSpecificResource> ;
      terms:format "pdf" ;
      <https://www.w3.org/ns/oahasSelector> [
          a <https://www.w3.org/ns/oaRangeSelector> ;
          <https://www.w3.org/ns/oahasEndSelector> [
              a <https://www.w3.org/ns/oaXPathSelector> ;
              rdf:value "Page 31" ;
            ] ;
          <https://www.w3.org/ns/oahasStartSelector> [
              a <https://www.w3.org/ns/oaXPathSelector> ;
              rdf:value "Page 30" ;
            ] ;
        ] ;
      <https://www.w3.org/ns/oahasSource> sto:DIN_SPEC_91345 ;
    ] ;
.
sto:RAMIInformationLayer
  a owl:NamedIndividual ;
  a rami:RAMIITLayer ;
  a sto:StandardClassification ;
  dul:associatedWith sto:BdvaDataAnalytics ;
  dul:associatedWith sto:BdvaDataManagement ;
  dul:associatedWith sto:EdgecrossEdgeComputingLayer ;
  dul:associatedWith sto:IDSRAMInformationLayer ;
  dul:associatedWith sto:IIRAApplicationDomain ;
  dul:associatedWith sto:InformationDomain ;
  dul:associatedWith sto:NgsiLdInformationModel ;
  rdfs:label "RAMI Information Layer"@en ;
  sto:alignsWith sto:BdvaDataAnalytics ;
  sto:alignsWith sto:BdvaDataManagement ;
  sto:alignsWith sto:EdgecrossEdgeComputingLayer ;
  sto:alignsWith sto:IDSRAMInformationLayer ;
  sto:alignsWith sto:IIRAApplicationDomain ;
  sto:alignsWith sto:InformationDomain ;
  sto:alignsWith sto:NgsiLdInformationModel ;
  sto:frames sto:DataAnalytics ;
  sto:frames sto:DataDescription ;
  sto:frames sto:DataProcessing ;
  sto:frames sto:IntegrityProtection ;
  sto:frames sto:Interoperability ;
  sto:frames sto:Security ;
  sto:frames sto:SemanticInteroperability ;
  sto:frames sto:StreamProcessing ;
  sto:frames sto:Trustworthiness ;
  sto:isDescribedin sto:RAMI ;
.
sto:RAMIInformationLayerAnno
  a <https://www.w3.org/ns/oaAnnotation> ;
  <https://www.w3.org/ns/oahasBody> sto:RAMIInformationLayer ;
  <https://www.w3.org/ns/oahasTarget> [
      a <https://www.w3.org/ns/oaSpecificResource> ;
      terms:format "pdf" ;
      <https://www.w3.org/ns/oahasSelector> [
          a <https://www.w3.org/ns/oaRangeSelector> ;
          <https://www.w3.org/ns/oahasEndSelector> [
              a <https://www.w3.org/ns/oaXPathSelector> ;
              rdf:value "Page 22" ;
            ] ;
          <https://www.w3.org/ns/oahasStartSelector> [
              a <https://www.w3.org/ns/oaXPathSelector> ;
              rdf:value "Page 21" ;
            ] ;
        ] ;
      <https://www.w3.org/ns/oahasSource> sto:DIN_SPEC_91345 ;
    ] ;
.
sto:RAMIIntegrationLayer
  a owl:NamedIndividual ;
  a rami:RAMIITLayer ;
  a sto:StandardClassification ;
  dul:associatedWith sto:DtpSystemView ;
  dul:associatedWith sto:EdgecrossEdgeComputingLayer ;
  dul:associatedWith sto:EdgecrossItSystemsLayer ;
  dul:associatedWith sto:FiwareIotServicesEnablement ;
  dul:associatedWith sto:IDSRAMSystemLayer ;
  dul:associatedWith sto:IIRAControlDomain ;
  dul:associatedWith sto:IotaEvolutionInteroperability ;
  dul:associatedWith sto:NgsiLdArchitecture ;
  dul:associatedWith sto:xRoadDeploymentView ;
  dul:associatedWith sto:xRoadProtocolsInterfaces ;
  rdfs:label "RAMI Integration Layer"@en ;
  sto:alignsWith sto:DtpSystemView ;
  sto:alignsWith sto:EdgecrossEdgeComputingLayer ;
  sto:alignsWith sto:EdgecrossItSystemsLayer ;
  sto:alignsWith sto:FiwareIotServicesEnablement ;
  sto:alignsWith sto:IDSRAMSystemLayer ;
  sto:alignsWith sto:IIRAControlDomain ;
  sto:alignsWith sto:IotaEvolutionInteroperability ;
  sto:alignsWith sto:NgsiLdArchitecture ;
  sto:alignsWith sto:xRoadDeploymentView ;
  sto:alignsWith sto:xRoadProtocolsInterfaces ;
  sto:frames sto:Interoperability ;
  sto:frames sto:SemanticInteroperability ;
  sto:frames sto:ThingDescription ;
  sto:frames sto:ThingRepresentation ;
  sto:frames sto:UserInteraction ;
  sto:isDescribedin sto:RAMI ;
.
sto:RAMIIntegrationLayerAnno
  a <https://www.w3.org/ns/oaAnnotation> ;
  <https://www.w3.org/ns/oahasBody> sto:RAMIIntegrationLayer ;
  <https://www.w3.org/ns/oahasTarget> [
      a <https://www.w3.org/ns/oaSpecificResource> ;
      terms:format "pdf" ;
      <https://www.w3.org/ns/oahasSelector> [
          a <https://www.w3.org/ns/oaRangeSelector> ;
          <https://www.w3.org/ns/oahasEndSelector> [
              a <https://www.w3.org/ns/oaXPathSelector> ;
              rdf:value "Page 23" ;
            ] ;
          <https://www.w3.org/ns/oahasStartSelector> [
              a <https://www.w3.org/ns/oaXPathSelector> ;
              rdf:value "Page 22" ;
            ] ;
        ] ;
      <https://www.w3.org/ns/oahasSource> sto:DIN_SPEC_91345 ;
    ] ;
.
sto:RAMIProduct
  a owl:NamedIndividual ;
  a rami:RAMIHierarchyLevel ;
  a sto:StandardClassification ;
  sto:frames sto:Manufacturing ;
  sto:isDescribedin sto:RAMI ;
.
sto:RAMIProductAnno
  a <https://www.w3.org/ns/oaAnnotation> ;
  <https://www.w3.org/ns/oahasBody> sto:RAMIProduct ;
  <https://www.w3.org/ns/oahasTarget> [
      a <https://www.w3.org/ns/oaSpecificResource> ;
      terms:format "pdf" ;
      <https://www.w3.org/ns/oahasSelector> [
          a <https://www.w3.org/ns/oaRangeSelector> ;
          <https://www.w3.org/ns/oahasEndSelector> [
              a <https://www.w3.org/ns/oaXPathSelector> ;
              rdf:value "Page 24" ;
            ] ;
          <https://www.w3.org/ns/oahasStartSelector> [
              a <https://www.w3.org/ns/oaXPathSelector> ;
              rdf:value "Page 23" ;
            ] ;
        ] ;
      <https://www.w3.org/ns/oahasSource> sto:DIN_SPEC_91345 ;
    ] ;
.
sto:RAMIStation
  a owl:NamedIndividual ;
  a rami:RAMIHierarchyLevel ;
  a sto:StandardClassification ;
  sto:isDescribedin sto:RAMI ;
.
sto:RAMIStationAnno
  a <https://www.w3.org/ns/oaAnnotation> ;
  <https://www.w3.org/ns/oahasBody> sto:RAMIStation ;
  <https://www.w3.org/ns/oahasTarget> [
      a <https://www.w3.org/ns/oaSpecificResource> ;
      terms:format "pdf" ;
      <https://www.w3.org/ns/oahasSelector> [
          a <https://www.w3.org/ns/oaRangeSelector> ;
          <https://www.w3.org/ns/oahasEndSelector> [
              a <https://www.w3.org/ns/oaXPathSelector> ;
              rdf:value "Page 24" ;
            ] ;
          <https://www.w3.org/ns/oahasStartSelector> [
              a <https://www.w3.org/ns/oaXPathSelector> ;
              rdf:value "Page 23" ;
            ] ;
        ] ;
      <https://www.w3.org/ns/oahasSource> sto:DIN_SPEC_91345 ;
    ] ;
.
sto:RAMIWorkCenter
  a owl:NamedIndividual ;
  a rami:RAMIHierarchyLevel ;
  a sto:StandardClassification ;
  sto:isDescribedin sto:RAMI ;
.
sto:RAMIWorkCenterAnno
  a <https://www.w3.org/ns/oaAnnotation> ;
  <https://www.w3.org/ns/oahasBody> sto:RAMIWorkCenter ;
  <https://www.w3.org/ns/oahasTarget> [
      a <https://www.w3.org/ns/oaSpecificResource> ;
      terms:format "pdf" ;
      <https://www.w3.org/ns/oahasSelector> [
          a <https://www.w3.org/ns/oaRangeSelector> ;
          <https://www.w3.org/ns/oahasEndSelector> [
              a <https://www.w3.org/ns/oaXPathSelector> ;
              rdf:value "Page 24" ;
            ] ;
          <https://www.w3.org/ns/oahasStartSelector> [
              a <https://www.w3.org/ns/oaXPathSelector> ;
              rdf:value "Page 23" ;
            ] ;
        ] ;
      <https://www.w3.org/ns/oahasSource> sto:DIN_SPEC_91345 ;
    ] ;
.
sto:RAML
  a owl:NamedIndividual ;
  a foaf:Document ;
  a sto:Publication ;
  a sto:TechnicalSpecification ;
  terms:creator sto:sebastian ;
  rdfs:comment "RAML (RESTful API Modeling Language) - Makes it easy to manage the whole API lifecycle from design to sharing. It's concise - you only write what you need to define - and reusable.  (source: https://www.postscapes.com/internet-of-things-protocols/)"@en ;
  rdfs:label "RAML"@en ;
  sto:hasOfficialResource <http://raml.org/> ;
.
sto:RDF
  a owl:NamedIndividual ;
  a foaf:Document ;
  a sto:Publication ;
  a sto:TechnicalSpecification ;
.
sto:REST
  a owl:NamedIndividual ;
  a foaf:Document ;
  a sto:Publication ;
  a sto:TechnicalSpecification ;
  terms:creator sto:sebastian ;
  dul:associatedWith sto:DtpDeploymentView ;
  rdfs:comment "REST (Representational state transfer) - RESTful HTTP (source: https://www.postscapes.com/internet-of-things-protocols/)"@en ;
  rdfs:label "REST"@en ;
  sto:hasWikipediaArticle <https://en.wikipedia.org/wiki/Representational_state_transfer> ;
.
sto:RFC_1122
  a owl:NamedIndividual ;
  a foaf:Document ;
  a sto:Publication ;
  a sto:Standard ;
  terms:creator sto:IETF ;
  terms:title "Requirements for Internet Hosts -- Communication Layers"@en ;
  rdfs:comment "This is one RFC of a pair that defines and discusses the requirements for Internet host software.  This RFC covers the communications protocol layers: link layer, IP layer, and transport layer; its companion RFC-1123 covers the application and support protocols."@en ;
  rdfs:label "RFC 1122"@en ;
  foaf:maker sto:IETF ;
  sto:hasClassification sto:IIRAConnectivity ;
  sto:hasClassification sto:NetworkLayer ;
  sto:hasOfficialResource <https://tools.ietf.org/html/rfc1122> ;
  sto:hasPublisher sto:IETF ;
.
sto:RFC_2616
  a owl:NamedIndividual ;
  a foaf:Document ;
  a sto:Publication ;
  a sto:Standard ;
  terms:creator sto:IETF ;
  rdfs:comment "The Hypertext Transfer Protocol (HTTP) is an application-level protocol for distributed, collaborative, hypermedia information systems. It is a generic, stateless, protocol which can be used for many tasks beyond its use for hypertext, such as name servers and distributed object management systems, through extension of its request methods, error codes and headers. A feature of HTTP is the typing and negotiation of data representation, allowing systems to be built independently of the data being transferred."@en ;
  rdfs:label "HTTP/1.1"@en ;
  rdfs:label "RFC 2616"@en ;
  skos:altLabel "HTTP/1.1"@en ;
  foaf:maker sto:IETF ;
  sto:hasClassification sto:IDSRAMSystemLayer ;
  sto:hasClassification sto:IIRAFunctionalViewpoint ;
  sto:hasClassification sto:RAMICommunicationlayer ;
  sto:hasClassification sto:TansportLayer ;
  sto:hasOfficialResource <https://tools.ietf.org/html/rfc2817> ;
  sto:hasOfficialResource <https://www.ietf.org/rfc/rfc2616> ;
  sto:hasPublisher sto:IETF ;
.
sto:RFC_2818
  a owl:NamedIndividual ;
  a foaf:Document ;
  a sto:Publication ;
  a sto:Standard ;
  terms:creator sto:IETF ;
  rdfs:comment "This memo describes how to use TLS to secure HTTP connections over  the Internet. Current practice is to layer HTTP over SSL (the predecessor to TLS), distinguishing secured traffic from insecure traffic by the use of a different server port. This document documents that practice using TLS. A companion document describes a method for using HTTP/TLS over the same port as normal HTTP [RFC2817]."@en ;
  rdfs:label "HTTPS"@en ;
  rdfs:label "RFC 2818"@en ;
  foaf:maker sto:IETF ;
  sto:hasClassification sto:IDSRAMSecurity ;
  sto:hasClassification sto:IDSRAMSystemLayer ;
  sto:hasPublisher sto:IETF ;
.
sto:RFC_4511
  a owl:NamedIndividual ;
  a foaf:Document ;
  a sto:Publication ;
  a sto:TechnicalSpecification ;
  terms:creator sto:IETF ;
  terms:creator sto:sebastian ;
  terms:title "Lightweight Directory Access Protocol"@en ;
  rdfs:label "LDAP"@en ;
  foaf:maker sto:IETF ;
  sto:hasDeveloper sto:IETF ;
  sto:hasOfficialResource <https://tools.ietf.org/html/rfc4511> ;
  sto:hasPublisher sto:IETF ;
  sto:hasTargetConcern sto:CrossDomainIdentityManagement ;
  sto:hasWikipediaArticle <https://en.wikipedia.org/wiki/Lightweight_Directory_Access_Protocol> ;
.
sto:RFC_5246
  a owl:NamedIndividual ;
  a foaf:Document ;
  a sto:Publication ;
  a sto:Standard ;
  terms:creator sto:IETF ;
  terms:description "This document specifies Version 1.2 of the Transport Layer Security (TLS) protocol.  The TLS protocol provides communications security over the Internet.  The protocol allows client/server applications to communicate in a way that is designed to prevent eavesdropping, tampering, or message forgery."@en ;
  rdfs:comment "This document specifies Version 1.2 of the Transport Layer Security (TLS) protocol.  The TLS protocol provides communications security over the Internet.  The protocol allows client/server applications to communicate in a way that is designed to prevent eavesdropping, tampering, or message forgery."@en ;
  rdfs:label "RFC 5246"@en ;
  foaf:maker sto:IETF ;
  sto:hasClassification sto:DataSovereignty ;
  sto:hasClassification sto:IDSRAMSecurity ;
  sto:hasOfficialResource <https://tools.ietf.org/html/rfc5246> ;
  sto:hasPublisher sto:IETF ;
.
sto:RFC_6750
  a owl:NamedIndividual ;
  a foaf:Document ;
  a sto:Publication ;
  a sto:Standard ;
  terms:creator sto:IETF ;
  terms:description "This specification describes how to use bearer tokens in HTTP requests to access OAuth 2.0 protected resources.  Any party in possession of a bearer token (a \"bearer\") can use it to get access to the associated resources (without demonstrating possession of a cryptographic key).  To prevent misuse, bearer tokens need to be protected from disclosure in storage and in transport."@en ;
  dul:associatedWith sto:DtpArchitecture ;
  rdfs:comment "This specification describes how to use bearer tokens in HTTP requests to access OAuth 2.0 protected resources.  Any party in possession of a bearer token (a \"bearer\") can use it to get access to the associated resources (without demonstrating possession of a cryptographic key).  To prevent misuse, bearer tokens need to be protected from disclosure in storage and in transport."@en ;
  rdfs:label "RFC 6750"@en ;
  skos:altLabel "OAuth2.0"@en ;
  foaf:maker sto:IETF ;
  sto:hasClassification sto:IDSRAMSecurity ;
  sto:hasDBpediaResource <http://dbpedia.org/resource/OAuth> ;
  sto:hasOfficialResource <https://tools.ietf.org/html/rfc6750> ;
  sto:hasPublisher sto:IETF ;
.
sto:RFC_7252
  a owl:NamedIndividual ;
  a foaf:Document ;
  a sto:Publication ;
  a sto:Standard ;
  terms:creator sto:IETF ;
  terms:title "The Constrained Application Protocol"@en ;
  rdfs:comment "The Constrained Application Protocol (CoAP) is a specialized web transfer protocol for use with constrained nodes and constrained (e.g., low-power, lossy) networks.  The nodes often have 8-bit microcontrollers with small amounts of ROM and RAM, while constrained networks such as IPv6 over Low-Power Wireless Personal Area Networks (6LoWPANs) often have high packet error rates and a typical throughput of 10s of kbit/s.  The protocol is designed for machine-to-machine (M2M) applications such as smart energy and building automation."@en ;
  rdfs:label "RFC 7252"@en ;
  skos:altLabel "CoAP"@en ;
  foaf:maker sto:IETF ;
  sto:hasClassification sto:IIRAOperationsDomain ;
  sto:hasClassification sto:TansportLayer ;
  sto:hasOfficialResource <https://tools.ietf.org/html/rfc7252> ;
  sto:hasPublicationDate "2014-06-01"^^xsd:date ;
  sto:hasPublisher sto:IETF ;
.
sto:RFC_7519
  a owl:NamedIndividual ;
  a foaf:Document ;
  a sto:Publication ;
  a sto:Standard ;
  terms:creator sto:IETF ;
  terms:description "JSON Web Token (JWT) is a compact, URL-safe means of representing claims to be transferred between two parties.  The claims in a JWT are encoded as a JSON object that is used as the payload of a JSON Web Signature (JWS) structure or as the plaintext of a JSON Web Encryption (JWE) structure, enabling the claims to be digitally signed or integrity protected with a Message Authentication Code (MAC) and/or encrypted."@en ;
  rdfs:comment "JSON Web Token (JWT) is a compact, URL-safe means of representing claims to be transferred between two parties.  The claims in a JWT are encoded as a JSON object that is used as the payload of a JSON Web Signature (JWS) structure or as the plaintext of a JSON Web Encryption (JWE) structure, enabling the claims to be digitally signed or integrity protected with a Message Authentication Code (MAC) and/or encrypted."@en ;
  rdfs:label "JSON Web Token"@en ;
  rdfs:label "RFC 7519"@en ;
  foaf:maker sto:IETF ;
  sto:hasClassification sto:DataSovereignty ;
  sto:hasClassification sto:IDSRAMSecurity ;
  sto:hasOfficialResource <https://tools.ietf.org/html/rfc7519> ;
  sto:hasPublisher sto:IETF ;
.
sto:RFC_7540
  a owl:NamedIndividual ;
  a foaf:Document ;
  a sto:Publication ;
  a sto:Standard ;
  terms:creator sto:IETF ;
  rdfs:comment """This specification describes an optimized expression of the semantics of the Hypertext Transfer Protocol (HTTP), referred to as HTTP version 2 (HTTP/2).  HTTP/2 enables a more efficient use of network resources and a reduced perception of latency by introducing header field compression and allowing multiple concurrent exchanges on the same connection.  It also introduces unsolicited push of  representations from servers to clients.

This specification is an alternative to, but does not obsolete, the HTTP/1.1 message syntax.  HTTP's existing semantics remain unchanged."""@en ;
  rdfs:label "HTTP/2"@en ;
  rdfs:label "RFC 7540"@en ;
  foaf:maker sto:IETF ;
  sto:hasClassification sto:IDSRAMInteroperability ;
  sto:hasClassification sto:IDSRAMSystemLayer ;
  sto:hasClassification sto:IIRAFunctionalViewpoint ;
  sto:hasClassification sto:RAMICommunicationlayer ;
  sto:hasClassification sto:TansportLayer ;
  sto:hasPublisher sto:IETF ;
.
sto:RFC_7642
  a owl:NamedIndividual ;
  a foaf:Document ;
  a sto:Publication ;
  a sto:Standard ;
  terms:creator sto:IETF ;
  terms:creator sto:sebastian ;
  terms:creator "sebastian" ;
  terms:title "SCIM Use Cases"@en ;
  rdfs:comment "This document provides definitions and an overview of the System for Cross-domain Identity Management (SCIM).  It lays out the system's concepts, models and flows, and includes user scenarios, use cases, and requirements."@en ;
  rdfs:label "RFC 7642"@en ;
  foaf:maker sto:IETF ;
  sto:hasClassification sto:FiwareSecurity ;
  sto:hasDeveloper sto:IETF ;
  sto:hasOfficialResource <https://tools.ietf.org/html/draft-ietf-scim-use-cases-08> ;
  sto:hasPublisher sto:IETF ;
  sto:hasTargetConcern sto:IdentityManagement ;
.
sto:RFC_7643
  a owl:NamedIndividual ;
  a foaf:Document ;
  a sto:Publication ;
  a sto:Standard ;
  terms:creator sto:IETF ;
  terms:creator sto:sebastian ;
  terms:creator "sebastian" ;
  terms:title "SCIM Core Schema"@en ;
  rdfs:comment "This document provides a platform neutral schema and extension model for representing users and groups and other resource types in JSON format.  This schema is intended for exchange and use with cloud service providers."@en ;
  rdfs:label "RFC 7643"@en ;
  foaf:maker sto:IETF ;
  sto:hasClassification sto:FiwareSecurity ;
  sto:hasDeveloper sto:IETF ;
  sto:hasOfficialResource <https://tools.ietf.org/html/draft-ietf-scim-core-schema-22> ;
  sto:hasPublisher sto:IETF ;
  sto:hasTargetConcern sto:IdentityManagement ;
.
sto:RFC_7644
  a owl:NamedIndividual ;
  a foaf:Document ;
  a sto:Publication ;
  a sto:Standard ;
  terms:creator sto:IETF ;
  terms:creator sto:sebastian ;
  terms:creator "sebastian" ;
  terms:title "SCIM API"@en ;
  rdfs:comment "The System for Cross-Domain Identity Management (SCIM) specification is an HTTP based protocol that makes managing identities in multi domain scenarios easier to support through a standardized service. Examples include but are not limited to enterprise to cloud service providers, and inter-cloud based scenarios.  The specification suite seeks to build upon experience with existing schemas and deployments, placing specific emphasis on simplicity of development and integration, while applying existing authentication, authorization, and privacy models.  SCIM's intent is to reduce the cost and complexity of user management operations by providing a common user schema, an extension model, and a service protocol defined by this document."@en ;
  rdfs:label "RFC 7644"@en ;
  foaf:maker sto:IETF ;
  sto:hasClassification sto:FiwareSecurity ;
  sto:hasDeveloper sto:IETF ;
  sto:hasOfficialResource <https://tools.ietf.org/html/draft-ietf-scim-api-19> ;
  sto:hasPublisher sto:IETF ;
  sto:hasTargetConcern sto:IdentityManagement ;
.
sto:RFC_768
  a owl:NamedIndividual ;
  a foaf:Document ;
  a sto:Publication ;
  a sto:Standard ;
  terms:creator sto:IETF ;
  terms:title "User Datagram Protocol (UDP)"@en ;
  rdfs:comment "In computer networking, the User Datagram Protocol (UDP) is one of the core members of the Internet protocol suite. The protocol was designed by David P. Reed in 1980 and formally defined in RFC 768. With UDP, computer applications can send messages, in this case referred to as datagrams, to other hosts on an Internet Protocol (IP) network. Prior communications are not required in order to set up communication channels or data paths."@en ;
  rdfs:label "RFC 768"@en ;
  foaf:maker sto:IETF ;
  sto:hasClassification sto:TansportLayer ;
  sto:hasDBpediaResource <http://dbpedia.org/resource/User_Datagram_Protocol> ;
  sto:hasOfficialResource <https://tools.ietf.org/html/rfc768> ;
  sto:hasPublisher sto:IETF ;
  sto:hasWikipediaArticle <https://en.wikipedia.org/wiki/User_Datagram_Protocol> ;
.
sto:RFC_793
  a owl:NamedIndividual ;
  a foaf:Document ;
  a sto:Publication ;
  a sto:Standard ;
  terms:creator sto:IETF ;
  terms:title "TRANSMISSION CONTROL PROTOCOL"@en ;
  rdfs:comment """This document describes the DoD Standard Transmission Control Protocol
(TCP).  There have been nine earlier editions of the ARPA TCP
 specification on which this standard is based, and the present text draws heavily from them.  There have been many contributors to this work both in terms of concepts and in terms of text.  This edition clarifies several details and removes the end-of-letter buffer-size adjustments,
 and redescribes the letter mechanism as a push function."""@en ;
  rdfs:label "RFC 793"@en ;
  foaf:maker sto:IETF ;
  sto:hasClassification sto:IDSRAMSystemLayer ;
  sto:hasClassification sto:TansportLayer ;
  sto:hasOfficialResource <https://tools.ietf.org/html/rfc793> ;
  sto:hasPublisher sto:IETF ;
.
sto:RFC_8323
  a owl:NamedIndividual ;
  a foaf:Document ;
  a sto:Publication ;
  a sto:TechnicalSpecification ;
  terms:creator sto:IETF ;
  terms:creator sto:sebastian ;
  rdfs:comment "CoAP (Constrained Application Protocol) is an application layer protocol that is intended for use in resource-constrained internet devices, such as WSN nodes. CoAP is designed to easily translate to HTTP for simplified integration with the web, while also meeting specialized requirements such as multicast support, very low overhead, and simplicity. The CoRE group has proposed the following features for CoAP: RESTful protocol design minimizing the complexity of mapping with HTTP, Low header overhead and parsing complexity, URI and content-type support, Support for the discovery of resources provided by known CoAP services. Simple subscription for a resource, and resulting push notifications, Simple caching based on max-age. (source: https://www.postscapes.com/internet-of-things-protocols/)"@en ;
  rdfs:label "CoAP"@en ;
  foaf:maker sto:IETF ;
  sto:hasClassification sto:IIRAConnectivity ;
  sto:hasClassification sto:RAMICommunicationlayer ;
  sto:hasDBpediaResource <http://dbpedia.org/resource/Constrained_Application_Protocol> ;
  sto:hasDeveloper sto:IETF ;
  sto:hasOfficialResource <https://tools.ietf.org/html/rfc8323> ;
  sto:hasPublisher sto:IETF ;
  sto:hasWikipediaArticle <http://en.wikipedia.org/wiki/Constrained_Application_Protocol> ;
.
sto:ROLL
  a owl:NamedIndividual ;
  a foaf:Document ;
  a sto:Publication ;
  a sto:TechnicalSpecification ;
  terms:creator sto:sebastian ;
  rdfs:comment "ROLL / RPL (IPv6 routing for low power/lossy networks) (source: https://www.postscapes.com/internet-of-things-protocols/)"@en ;
  rdfs:label "ROLL"@en ;
  sto:hasOfficialResource <https://datatracker.ietf.org/wg/roll/> ;
.
sto:RPMA
  a owl:NamedIndividual ;
  a foaf:Document ;
  a sto:Publication ;
  a sto:TechnicalSpecification ;
  terms:creator sto:sebastian ;
  rdfs:comment "RPMA (Random phase multiple access) A technology communication system employing direct-sequence spread spectrum (DSSS) with multiple access. (source: https://www.postscapes.com/internet-of-things-protocols/)"@en ;
  rdfs:label "RPMA"@en ;
  sto:hasWikipediaArticle <https://en.wikipedia.org/wiki/Random_phase_multiple_access> ;
.
sto:RadioActivityControl
  a owl:NamedIndividual ;
  a sto:Concern ;
  <http://voag.linkedmodel.org/voag#hasStakeholder> <http://dbpedia.org/ontology/developer> ;
  rdfs:comment "The user shall be able to control the radio activity of the system."@en ;
  rdfs:label "Radio activity control"@en ;
  rdfs:seeAlso "IoT-A Requirement UNI.021" ;
  sto:supports sto:EnergyControl ;
.
sto:ReactiveStreams
  a owl:NamedIndividual ;
  a foaf:Document ;
  a sto:Publication ;
  a sto:TechnicalSpecification ;
  terms:creator sto:sebastian ;
  rdfs:comment "A standard for asynchronous stream processing with non-blocking back pressure on the JVM. (source: https://www.postscapes.com/internet-of-things-protocols/)"@en ;
  rdfs:label "Reactive Streams"@en ;
  sto:hasOfficialResource <http://www.reactive-streams.org/> ;
.
sto:RealTimeAnalytics
  a owl:NamedIndividual ;
  a sto:Concern ;
  <http://voag.linkedmodel.org/voag#hasStakeholder> <http://purl.oclc.org/NET/mvco.owl#EndUser> ;
  rdfs:comment "In computer science, real-time computing (RTC), or reactive computing describes hardware and software systems subject to a \"real-time constraint\", for example from event to system response. Real-time programs must guarantee response within specified time constraints, often referred to as \"deadlines\". Systems of this type whose correctness depends on their temporal aspects as well as their functional aspects. Real-time responses are often understood to be in the order of milliseconds, and sometimes microseconds."@en ;
  rdfs:label "Real Time Analytics"@en ;
  rdfs:seeAlso "IoT-A Requirement UNI.020" ;
  sto:hasDBpediaResource <http://dbpedia.org/resource/Real-time_computing> ;
  sto:supports sto:DataAnalytics ;
.
sto:Regulatory_Compliance
  a owl:NamedIndividual ;
  a sto:Concern ;
  terms:creator sto:MuhammadUsman ;
  rdfs:comment "Organizations are ultimately legally responsible for their process compliance and data security, Even though the data is in a public cloud."@en ;
  rdfs:label "Regulatory Compliance"@en ;
  rdfs:seeAlso "https://dl.acm.org/citation.cfm?doid=3286606.3286865"@en ;
  skos:narrower sto:Compliance ;
  sto:hasWikipediaArticle "https://en.wikipedia.org/wiki/Regulatory_compliance"@en ;
.
sto:RelevantSubject
  a owl:Class ;
  rdfs:comment "A subject that is relevant in the context of a standard (IEC standards in specific). As specified in IEC Website ."@en ;
  rdfs:label "Relevant Subject"@en ;
.
sto:Reliability
  a owl:NamedIndividual ;
  a sto:Concern ;
  terms:creator sto:sebastian ;
  rdfs:comment "In computer networking, a reliable protocol provides reliability properties with respect to the delivery of data to the intended recipient(s), as opposed to an unreliable protocol, which does not provide notifications to the sender as to the delivery of transmitted data. (source: wikipedia)"@en ;
  rdfs:label "Reliability"@en ;
  rdfs:seeAlso "IoT-A Requirement UNI.065" ;
  rdfs:seeAlso "https://dl.acm.org/citation.cfm?doid=3266237.3266263"@en ;
  rdfs:seeAlso "https://ieeexplore.ieee.org/document/7488250" ;
  rdfs:seeAlso "https://ieeexplore.ieee.org/document/8463303"@en ;
  skos:note "Publications referred: '<https://www.iiconsortium.org/pdf/IIC_PUB_G4_V1.00_PB-3.pdf IIC:PUB:G4:V1.0:PB:20160926>'" ;
  skos:note "Publications referred: '<https://www.openfogconsortium.org/wp-content/uploads/OpenFog_Reference_Architecture_2_09_17-FINAL.pdf> OPFRA001.020817' '4.6 Reliability, Availability, and Serviceability (RAS)Pillar' 'Page 29' " ;
  sto:hasDBpediaResource <http://dbpedia.org/resource/Reliability_(computer_networking)> ;
  sto:supports sto:Trustworthiness ;
.
sto:Resilience
  a owl:NamedIndividual ;
  a sto:Concern ;
  terms:creator sto:sebastian ;
  <http://voag.linkedmodel.org/voag#hasStakeholder> <http://dbpedia.org/ontology/generalManager> ;
  <http://voag.linkedmodel.org/voag#hasStakeholder> <https://www.wikidata.org/wiki/Q1548249> ;
  rdfs:comment "Resilience is the ability to provide and maintain an acceptable level of service in the face of faults and challenges to normal operation.” Threats and challenges for services can range from simple misconfiguration over large scale natural disasters to targeted attacks. As such, network resilience touches a very wide range of topics. In order to increase the resilience of a given communication network, the probable challenges and risks have to be identified and appropriate resilience metrics have to be defined for the service to be protected. (source: wikipedia)"@en ;
  rdfs:label "Resilience"@en ;
  rdfs:seeAlso "IoT-A Requirement UNI.012" ;
  rdfs:seeAlso "IoT-A Requirement UNI.040" ;
  rdfs:seeAlso "IoT-A Requirement UNI.058" ;
  rdfs:seeAlso "IoT-A Requirement UNI.064" ;
  rdfs:seeAlso "IoT-A Requirement UNI.718" ;
  rdfs:seeAlso "https://ieeexplore.ieee.org/document/7919553"@en ;
  sto:hasDBpediaResource <http://dbpedia.org/resource/Resilience_(network)> ;
  sto:supports sto:Trustworthiness ;
.
sto:ReturnOnInvestment
  a owl:NamedIndividual ;
  a sto:Concern ;
  rdfs:label "Return On Investment"@en ;
  skos:note "Publications referred: '(IIC:PUB:G1:V1.80:20170131' '4 BUSINESS VIEWPOINT' 'Page 20' " ;
  sto:supports sto:BusinessContext ;
.
sto:RiskManagement
  a owl:NamedIndividual ;
  a sto:Concern ;
  terms:creator sto:MuhammadUsman ;
  rdfs:comment """Organizations will be generally exposed to a broad range of different risks, by adopting the cloud computing. Managing these risks is very important concern, as the successful implementation of cloud computing relies upon the appropriate managing, reducing, as well as mitigating these risks linked to
cloud computing"""@en ;
  rdfs:label "Risk Management"@en ;
  rdfs:seeAlso "https://dl.acm.org/citation.cfm?doid=3108421.3108426"@en ;
  sto:hasDBpediaResource "http://dbpedia.org/page/Risk_management"@en ;
  sto:hasWikipediaArticle "https://en.wikipedia.org/wiki/Risk_management"@en ;
  sto:supports sto:BusinessContext ;
.
sto:RoleCategorization
  a owl:NamedIndividual ;
  a sto:Concern ;
  terms:creator sto:sebastian ;
  rdfs:comment "The necessity to categorize participants of a network (users or components) by roles according to the contributions they provide and the demands they have. Examples are identity provider, analytics service, data provider etc. Not to be confused with 'role-based access control', which distinguishes users according to their organizational group, e.g. adimistrators, managers, data analysts etc."@en ;
  rdfs:label "Role Categorization"@en ;
  sto:supports sto:IdentityManagement ;
.
sto:RuralElectrification
  a owl:NamedIndividual ;
  a sto:RelevantSubject ;
  rdfs:comment "Bringing electricity into remote areas"@en ;
  rdfs:label "Rural Electrification"@en ;
  sto:hasWikipediaArticle <https://en.wikipedia.org/wiki/Rural_electrification> ;
.
sto:SCADALevel
  a owl:NamedIndividual ;
  a sto:ISA95Level ;
  a sto:StandardClassification ;
  rdfs:comment "Describes the SCADA level according to the ISA95 level classification."@en ;
  rdfs:label "SCADA Level"@en ;
  skos:definition "Supervisory control and data acquisition according to ISA 95"@en ;
  sto:isDescribedin sto:ISA95 ;
.
sto:SCIM
  a owl:NamedIndividual ;
  a foaf:Document ;
  a sto:Publication ;
  a sto:TechnicalSpecification ;
  terms:creator sto:IETF ;
  terms:creator sto:sebastian ;
  terms:creator "sebastian" ;
  terms:title "IETF System for Cross-domain Identity Management (SCIM) 2.0"@en ;
  dul:associatedWith sto:FiwareSecurity ;
  dul:associatedWith sto:RFC_7642 ;
  dul:associatedWith sto:RFC_7643 ;
  dul:associatedWith sto:RFC_7644 ;
  rdfs:comment "The System for Cross-domain Identity Management (SCIM) specification is designed to make managing user identities in cloud-based applications and services easier. The specification suite seeks to build upon experience with existing schemas and deployments, placing specific emphasis on simplicity of development and integration, while applying existing authentication, authorization, and privacy models. Its intent is to reduce the cost and complexity of user management operations by providing a common user schema and extension model, as well as binding documents to provide patterns for exchanging this schema using standard protocols. In essence: make it fast, cheap, and easy to move users in to, out of, and around the cloud."@en ;
  rdfs:label "SCIM"@en ;
  foaf:maker sto:IETF ;
  sto:hasDBpediaResource <http://dbpedia.org/resource/System_for_Cross-domain_Identity_Management> ;
  sto:hasPublisher sto:IETF ;
  sto:hasTargetConcern sto:CrossDomainIdentityManagement ;
  sto:hasWikipediaArticle <https://en.wikipedia.org/wiki/System_for_Cross-domain_Identity_Management> ;
.
sto:SCM
  a owl:NamedIndividual ;
  a sto:BusinessCycleSCM ;
  rdfs:comment "Describes Plan-Source-Make-Deliver-Return cycle for managing the manufacturing supply chain."@en ;
  rdfs:label "Supply Chain Management"@en ;
  sto:isDescribedin sto:NISTInitiative ;
.
sto:SCOR
  a owl:NamedIndividual ;
  a foaf:Document ;
  a sto:Publication ;
  a sto:Standard ;
  terms:creator sto:APICS ;
  rdfs:comment "APICS Supply Chain Operations Reference."@en ;
  rdfs:label "SCOR"@en ;
  foaf:maker sto:APICS ;
  sto:hasClassification sto:SCM ;
  sto:hasDBpediaResource <http://dbpedia.org/page/Supply-chain_operations_reference> ;
  sto:hasDeveloper sto:APICS ;
  sto:hasOfficialResource <http://www.apics.org/apics-for-business/products-and-services/apics-scc-frameworks/scor> ;
  sto:hasTag "SCOR"@en ;
  sto:hasWikipediaArticle <https://en.wikipedia.org/wiki/Supply-chain_operations_reference> ;
.
sto:SE
  a owl:NamedIndividual ;
  a foaf:Organization ;
  a sto:StandardOrganization ;
  rdfs:comment "The Broadband Forum is a non-profit industry consortium dedicated to developing broadband network specifications. Members include telecommunications networking and service provider companies, broadband device and equipment vendors, consultants and independent testing labs (ITLs). Service provider members are primarily wire-line service providers (non-mobile) telephone companies."@en ;
  sto:abbreviation "SE" ;
  sto:formationDate "1936-01-01"^^xsd:date ;
  sto:hasDBpediaResource <http://dbpedia.org/page/Schneider_Electric> ;
  sto:hasHeadquaterIn dbr:Paris ;
  sto:hasOfficialResource <http://www.schneider-electric.com/ww/en/> ;
  sto:hasWikipediaArticle <https://en.wikipedia.org/wiki/Schneider_Electric> ;
  sto:orgName "Schneider Electric"@en ;
.
sto:SENML
  a owl:NamedIndividual ;
  a foaf:Document ;
  a sto:Publication ;
  a sto:TechnicalSpecification ;
  terms:creator sto:sebastian ;
  rdfs:comment "SENML (Media Types for Sensor Markup Language) - A simple sensor, such as a temperature sensor, could use this media type in protocols such as HTTP or CoAP to transport the measurements of the sensor or to be configured.  (source: https://www.postscapes.com/internet-of-things-protocols/)"@en ;
  rdfs:label "SENML"@en ;
  sto:hasOfficialResource <https://tools.ietf.org/html/draft-jennings-senml-08> ;
.
sto:SMCP
  a owl:NamedIndividual ;
  a foaf:Document ;
  a sto:Publication ;
  a sto:TechnicalSpecification ;
  terms:creator sto:sebastian ;
  rdfs:comment "SMCP — A C-based CoAP stack which is suitable for embedded environments. Features include: Support draft-ietf-core-coap-13, Fully asynchronous I/O, Supports both BSD sockets and UIP. (source: https://www.postscapes.com/internet-of-things-protocols/)"@en ;
  rdfs:label "SMCP"@en ;
  sto:hasOfficialResource <https://github.com/darconeous/smcp/tree/smcp-0.6> ;
.
sto:SOAP
  a owl:NamedIndividual ;
  a foaf:Document ;
  a sto:Publication ;
  a sto:TechnicalSpecification ;
  terms:creator sto:sebastian ;
  rdfs:comment "SOAP (Simple Object Access Protocol) (source: https://www.postscapes.com/internet-of-things-protocols/)"@en ;
  rdfs:label "SOAP"@en ;
  sto:hasWikipediaArticle <https://en.wikipedia.org/wiki/SOAP> ;
.
sto:SSI
  a owl:NamedIndividual ;
  a foaf:Document ;
  a sto:Publication ;
  a sto:TechnicalSpecification ;
  terms:creator sto:sebastian ;
  rdfs:comment "SSI (Simple Sensor Interface) is a simple communications protocol designed for data transfer between computers or user terminals and smart sensors. (source: https://www.postscapes.com/internet-of-things-protocols/)"@en ;
  rdfs:label "SSI"@en ;
  sto:hasWikipediaArticle <https://en.wikipedia.org/wiki/Simple_Sensor_Interface_protocol> ;
.
sto:SSN
  a owl:NamedIndividual ;
  a foaf:Document ;
  a sto:Publication ;
  a sto:TechnicalSpecification ;
  terms:creator sto:sebastian ;
  rdfs:comment "Semantic Sensor Net Ontology - W3C This ontology describes sensors and observations, and related concepts. It does not describe domain concepts, time, locations, etc. these are intended to be included from other ontologies via OWL imports. (source: https://www.postscapes.com/internet-of-things-protocols/)"@en ;
  rdfs:label "SSN"@en ;
  sto:hasOfficialResource <https://www.w3.org/2005/Incubator/ssn/wiki/Semantic_Sensor_Net_Ontology> ;
.
sto:STOMP
  a owl:NamedIndividual ;
  a foaf:Document ;
  a sto:Publication ;
  a sto:TechnicalSpecification ;
  terms:creator sto:sebastian ;
  rdfs:comment "STOMP - The Simple Text Oriented Messaging Protocol (source: https://www.postscapes.com/internet-of-things-protocols/)"@en ;
  rdfs:label "STOMP"@en ;
  sto:hasOfficialResource <https://stomp.github.io/implementations.html> ;
.
sto:Safety
  a owl:NamedIndividual ;
  a sto:Concern ;
  terms:creator sto:sebastian ;
  rdfs:comment "Functional safety (as defined by the IDS) is the ability of a system to prevent physical damage."@en ;
  rdfs:comment "Safety is the state of being \"safe\" (from French sauf), the condition of being protected from harm or other non-desirable outcomes. Safety can also refer to the control of recognized hazards in order to achieve an acceptable level of risk. (source: wikipedia)"@en ;
  rdfs:label "Safety"@en ;
  sto:hasDBpediaResource <http://dbpedia.org/resource/Safety> ;
  sto:supports sto:Trustworthiness ;
.
sto:Scalability
  a owl:NamedIndividual ;
  a sto:Concern ;
  terms:creator sto:sebastian ;
  rdfs:comment "Scalability is the capability of a system, network, or process to handle a growing amount of work, or its potential to be enlarged in order to accommodate that growth. For example, it can refer to the capability of a system to increase its total output under an increased load when resources (typically hardware) are added. An analogous meaning is implied when the word is used in an economic context, where scalability of a company implies that the underlying business model offers the potential for economic growth within the company. Scalability, as a property of systems, is generally difficult to define and in any particular case it is necessary to define the specific requirements for scalability on those dimensions that are deemed important. It is a highly significant issue in electronics systems, databases, routers, and networking. (source: wikipedia)"@en ;
  rdfs:label "Scalability"@en ;
  rdfs:seeAlso "IoT-A Requirement UNI.026" ;
  rdfs:seeAlso "IoT-A Requirement UNI.234" ;
  rdfs:seeAlso "IoT-A Requirement UNI.511" ;
  rdfs:seeAlso "IoT-A Requirement UNI.711" ;
  rdfs:seeAlso "https://dl.acm.org/citation.cfm?doid=3266237.3266263"@en ;
  rdfs:seeAlso "https://ieeexplore.ieee.org/document/6188257"@en ;
  rdfs:seeAlso "https://ieeexplore.ieee.org/document/8327600" ;
  sto:hasDBpediaResource <http://dbpedia.org/resource/Scalability> ;
.
sto:SebastianBader
  a owl:NamedIndividual ;
.
sto:SecureCommunication
  a owl:NamedIndividual ;
  a sto:Concern ;
  terms:creator sto:sebastian ;
  <http://voag.linkedmodel.org/voag#hasStakeholder> <http://dbpedia.org/ontology/developer> ;
  <http://voag.linkedmodel.org/voag#hasStakeholder> <http://purl.oclc.org/NET/mvco.owl#EndUser> ;
  <http://voag.linkedmodel.org/voag#hasStakeholder> <https://w3id.org/i40/SystemArchitect> ;
  rdfs:comment <http://dbpedia.org/resource/Secure_communication> ;
  rdfs:comment "This concern frames everything necessary to establish and conduct a secure communication channel, which cannot be read, intercepted or altered by a third party. Especially relevant are encrypting techniques."@en ;
  rdfs:label "Secure Communication"@en ;
  rdfs:seeAlso "IoT-A Requirement UNI.022" ;
  rdfs:seeAlso "IoT-A Requirement UNI.062" ;
  rdfs:seeAlso "IoT-A Requirement UNI.501" ;
  rdfs:seeAlso "IoT-A Requirement UNI.607" ;
  rdfs:seeAlso "IoT-A Requirement UNI.608" ;
  rdfs:seeAlso "IoT-A Requirement UNI.609" ;
  rdfs:seeAlso "https://ieeexplore.ieee.org/document/7919553"@en ;
  sto:supports sto:Communication ;
  sto:supports sto:IntegrityProtection ;
.
sto:Security
  a owl:NamedIndividual ;
  a sto:Concern ;
  terms:creator sto:sebastian ;
  <http://voag.linkedmodel.org/voag#hasStakeholder> <http://dbpedia.org/ontology/generalManager> ;
  <http://voag.linkedmodel.org/voag#hasStakeholder> <https://www.wikidata.org/wiki/Q1548249> ;
  rdfs:comment "Information security, sometimes shortened to InfoSec, is the practice of defending information from unauthorized access, use, disclosure, disruption, modification, inspection, recording or destruction. It is a general term that can be used regardless of the form the data may take (e.g. electronic, physical). (source: wikipedia)"@en ;
  rdfs:label "Security"@en ;
  rdfs:seeAlso "IoT-A Requirement UNI.040" ;
  rdfs:seeAlso "IoT-A Requirement UNI.507" ;
  rdfs:seeAlso "IoT-A Requirement UNI.626" ;
  rdfs:seeAlso "IoT-A Requirement UNI.719" ;
  rdfs:seeAlso "https://dl.acm.org/citation.cfm?doid=3266237.3266263"@en ;
  rdfs:seeAlso "https://ieeexplore.ieee.org/document/7919553"@en ;
  sto:hasDBpediaResource <http://dbpedia.org/resource/Information_security> ;
  sto:supports sto:Privacy ;
.
sto:SecurityConfiguration
  a owl:NamedIndividual ;
  a sto:Concern ;
  rdfs:comment "Users should be able to monitor and control the security and privacy settings of all the devices that they own."@en ;
  rdfs:label "Security Configuration"@en ;
  rdfs:seeAlso "IoT-A Requirement UNI.625" ;
  sto:hasDBpediaResource <http://dbpedia.org/resource/Hardening_(computing)> ;
  sto:supports sto:Security ;
.
sto:SelectionOfServiceProvider
  a owl:NamedIndividual ;
  a sto:Concern ;
  terms:creator sto:MuhammadUsman ;
  rdfs:comment """Due to the diversity of cloud computing service suppliers, it is a challenge for organizations to pick am appropriate service supplier. In selection of a cloud provider, organizations ought to look at different elements, like the reputation and size of the company of service supplier, in terms of number of employees,
share of the market, as well as their other resources"""@en ;
  rdfs:label "Selection of Service Provider"@en ;
  rdfs:seeAlso "https://dl.acm.org/citation.cfm?doid=3108421.3108426"@en ;
  sto:hasWikipediaArticle "https://en.wikipedia.org/wiki/Service_provider"@en ;
  sto:supports sto:BusinessContext ;
  sto:supports sto:CloudComputing ;
.
sto:SemanticInteroperability
  a owl:NamedIndividual ;
  a sto:Concern ;
  terms:creator sto:sebastian ;
  <http://voag.linkedmodel.org/voag#hasStakeholder> <http://dbpedia.org/ontology/developer> ;
  rdfs:comment """Beyond the ability of two or more computer systems to exchange information, semantic interoperability is the ability to automatically interpret the information exchanged meaningfully and accurately in order to produce useful results as defined by the end users of both systems. To achieve semantic interoperability, both sides must refer to a common information exchange reference model. 
source: <https://en.wikipedia.org/wiki/Interoperability>"""@en ;
  rdfs:label "Semantic Interoperability"@en ;
  rdfs:seeAlso "IoT-A Requirement UNI.003" ;
  rdfs:seeAlso "IoT-A Requirement UNI.070" ;
  rdfs:seeAlso "IoT-A Requirement UNI.073" ;
  rdfs:seeAlso "IoT-A Requirement UNI.213" ;
  rdfs:seeAlso "IoT-A Requirement UNI.426" ;
  rdfs:seeAlso "IoT-A Requirement UNI.427" ;
  skos:note "Publications referred: '<https://doi.org/10.1016/j.jksuci.2016.10.003>' '3.2. Direction toward Io<*>' 'Page 315'" ;
  sto:hasDBpediaResource <http://dbpedia.org/resource/Semantic_interoperability> ;
  sto:supports sto:Interoperability ;
.
sto:Sensing
  a owl:NamedIndividual ;
  a sto:Concern ;
  terms:creator sto:sebastian ;
  rdfs:comment "The concern of being able to measure values from a defined environment."@en ;
  rdfs:label "Sensing"@en ;
  skos:note "Publications referred: 'IIC:PUB:G1:V1.80:20170131' '6.1 THE CONTROL DOMAIN' 'Page 28' " ;
  sto:hasDBpediaResource <http://dbpedia.org/resource/Sensor> ;
  sto:supports sto:IoT ;
.
sto:SensorML
  a owl:NamedIndividual ;
  a foaf:Document ;
  a sto:Publication ;
  a sto:TechnicalSpecification ;
  terms:creator sto:sebastian ;
  rdfs:comment "SensorML provides standard models and an XML encoding for describing sensors and measurement processes. (source: https://www.postscapes.com/internet-of-things-protocols/)"@en ;
  rdfs:label "SensorML"@en ;
  sto:hasWikipediaArticle <https://en.wikipedia.org/wiki/SensorML> ;
.
sto:ServiceAccessControl
  a owl:NamedIndividual ;
  a sto:Concern ;
  terms:creator sto:sebastian ;
  dul:associatedWith sto:DataAccessControl ;
  rdfs:comment "Service access control is the selective restriction of access to a specific (web) service or process. The act of accessing may mean consuming, entering, or using. Permission to access a service is called service authorization. Locks and login credentials are two analogous mechanisms of access control. (source: wikipedia)"@en ;
  rdfs:label "Service Access Control"@en ;
  rdfs:seeAlso "IoT-A Requirement UNI.611" ;
  sto:hasDBpediaResource <http://dbpedia.org/resource/Network_Access_Control> ;
  sto:supports sto:Authorization ;
.
sto:ServiceChoreography
  a owl:NamedIndividual ;
  a sto:Concern ;
  terms:creator sto:sebastian ;
  rdfs:comment "2 to n Data Apps/Services/Data Provider are connected (without a central coordinator)"@en ;
  rdfs:comment "Service choreography is a form of service composition in which the interaction protocol between several partner services is defined from a global perspective.The intuition underlying the notion of service choreography can be summarised as follows: “Dancers dance following a global scenario without a single point of control\" That is, at run-time each participant in a service choreography executes its part of it (i.e. its role) according to the behavior of the other participants.A choreography's role specifies the expected messaging behavior of the participants that will play it in terms of the sequencing and timing of the messages that they can consume and produce. (source: wikipedia)"@en ;
  rdfs:label "Service Choreography"@en ;
  rdfs:seeAlso "IoT-A Requirement UNI.096" ;
  rdfs:seeAlso "IoT-A Requirement UNI.704" ;
  sto:hasDBpediaResource <http://dbpedia.org/resource/Service_choreography> ;
  sto:supports sto:ServiceComposition ;
.
sto:ServiceComposition
  a owl:NamedIndividual ;
  a sto:Concern ;
  terms:creator sto:sebastian ;
  <http://voag.linkedmodel.org/voag#hasStakeholder> <https://www.wikidata.org/wiki/Q1548249> ;
  rdfs:comment "2 to n Data Apps/Devices/Services are connected"@en ;
  rdfs:comment "In computing, service composability is a design principle, applied within the service-orientation design paradigm, that encourages the design of services that can be reused in multiple solutions that are themselves made up of composed services. The ability to recompose the service is ideally independent of the size and complexity of the service composition. This principle is directly responsible for the agility promised by SOA as it promotes composing new solutions by reusing existing services. (source: wikipedia)"@en ;
  rdfs:label "Service Composition"@en ;
  rdfs:seeAlso "IoT-A Requirement UNI.014" ;
  rdfs:seeAlso "IoT-A Requirement UNI.031" ;
  rdfs:seeAlso "IoT-A Requirement UNI.043" ;
  rdfs:seeAlso "IoT-A Requirement UNI.089" ;
  rdfs:seeAlso "IoT-A Requirement UNI.094" ;
  rdfs:seeAlso "IoT-A Requirement UNI.234" ;
  rdfs:seeAlso "IoT-A Requirement UNI.244" ;
  rdfs:seeAlso "IoT-A Requirement UNI.245" ;
  rdfs:seeAlso "IoT-A Requirement UNI.247" ;
  rdfs:seeAlso "IoT-A Requirement UNI.251" ;
  rdfs:seeAlso "IoT-A Requirement UNI.253" ;
  sto:hasDBpediaResource <http://dbpedia.org/resource/Service_composition> ;
  sto:supports sto:interoperability ;
.
sto:ServiceDeployment
  a owl:NamedIndividual ;
  a sto:Concern ;
  rdfs:comment "Software deployment is all of the activities that make a software system available for use. The general deployment process consists of several interrelated activities with possible transitions between them. These activities can occur at the producer side or at the consumer side or both. Because every software system is unique, the precise processes or procedures within each activity can hardly be defined. Therefore, \"deployment\" should be interpreted as a general process that has to be customized according to specific requirements or characteristics. (source: wikipedia)"@en ;
  rdfs:label "Service Deployment"@en ;
  rdfs:seeAlso "IoT-A Requirement UNI.429" ;
  sto:hasDBpediaResource <http://dbpedia.org/resource/Software_deployment> ;
  sto:supports sto:ServiceLifecycleManagement ;
.
sto:ServiceDescription
  a owl:NamedIndividual ;
  a sto:Concern ;
  terms:creator sto:sebastian ;
  <http://voag.linkedmodel.org/voag#hasStakeholder> <http://dbpedia.org/ontology/developer> ;
  rdfs:comment "A Service Description plays an important role in enabling access to a service. Most service description languages are designed for machine consumption, allowing for the automatic creation of code skeletons, easier search, and classification of services. However, people may also find descriptions useful to learn about the use of parameters or the precise semantics of some operation.  (https://www.w3.org/standards/webofservices/description)"@en ;
  rdfs:label "Service Description"@en ;
  rdfs:seeAlso "IoT-A Requirement UNI.004" ;
  rdfs:seeAlso "IoT-A Requirement UNI.036" ;
  rdfs:seeAlso "IoT-A Requirement UNI.042" ;
  rdfs:seeAlso "IoT-A Requirement UNI.240" ;
  rdfs:seeAlso "IoT-A Requirement UNI.715" ;
  sto:supports sto:SemanticInteroperability ;
.
sto:ServiceDescriptions
  rdfs:seeAlso "IoT-A Requirement UNI.244" ;
.
sto:ServiceDiscovery
  a owl:NamedIndividual ;
  a sto:Concern ;
  terms:creator sto:sebastian ;
  rdfs:comment "How to find desired (Web) services, Data Apps, functionalities."@en ;
  rdfs:label "Service Discovery"@en ;
  rdfs:seeAlso "IoT-A Requirement UNI.406" ;
  rdfs:seeAlso "IoT-A Requirement UNI.408" ;
  rdfs:seeAlso "IoT-A Requirement UNI.414" ;
  rdfs:seeAlso "IoT-A Requirement UNI.415" ;
  rdfs:seeAlso "IoT-A Requirement UNI.416" ;
  rdfs:seeAlso "IoT-A Requirement UNI.422" ;
  rdfs:seeAlso "IoT-A Requirement UNI.427" ;
  skos:note "Publications referred: '<https://doi.org/10.1016/j.jksuci.2016.10.003>' '2.8.2. Societal data service' 'Page 309'" ;
  sto:hasDBpediaResource <http://dbpedia.org/resource/Service_discovery> ;
.
sto:ServiceIsolation
  a owl:NamedIndividual ;
  a sto:Concern ;
  terms:creator sto:sebastian ;
  rdfs:comment "Service isolation via a process group (as done with Docker) or by least privilege with clear separation and support for additional security modules (as done by trustme)."@en ;
  rdfs:label "Service Isolation"@en ;
  skos:narrower sto:Isolation ;
  sto:hasDBpediaResource <http://dbpedia.org/resource/Process_isolation> ;
.
sto:ServiceLevelAgreements
  a owl:NamedIndividual ;
  a sto:Concern ;
  terms:creator sto:sebastian ;
  rdfs:comment "A service-level agreement (SLA) is defined as an official commitment that prevails between a service provider and the customer. Particular aspects of the service – quality, availability, responsibilities – are agreed between the service provider and the service user. The most common component of SLA is that the services should be provided to the customer as agreed upon in the contract. As an example, Internet service providers and telcos will commonly include service level agreements within the terms of their contracts with customers to define the level(s) of service being sold in plain language terms. In this case the SLA will typically have a technical definition in terms of mean time between failures (MTBF), mean time to repair or mean time to recovery (MTTR); identifying which party is responsible for reporting faults or paying fees; responsibility for various data rates; throughput; jitter; or similar measurable details. (source: wikipedia)"@en ;
  rdfs:label "Service level agreement"@en ;
  rdfs:seeAlso "IoT-A Requirement UNI.060" ;
  sto:hasDBpediaResource "http://dbpedia.org/resource/Service-level_agreement"^^xsd:anyURI ;
  sto:supports sto:ServiceLifecycleManagement ;
.
sto:ServiceLifecycleManagement
  a owl:NamedIndividual ;
  a sto:Concern ;
  <http://voag.linkedmodel.org/voag#hasStakeholder> <https://w3id.org/i40/SystemArchitect> ;
  rdfs:comment "Information lifecycle management (ILM) refers to strategies for administering storage systems on computing devices. ILM is the practice of applying certain policies to effective information management. This practice had its basis in the management of information in paper or other physical forms (microfilm, negatives, photographs, audio or video recordings and other assets). ILM includes every phase of a \"record\" from its beginning to its end. And while it is generally applied to information that rises to the classic definition of a record (and thus related to records management), it applies to all informational assets. (source: wikipedia)"@en ;
  rdfs:label "Service life-cycle management"@en ;
  rdfs:seeAlso "IoT-A Requirement UNI.087" ;
  sto:hasDBpediaResource <http://dbpedia.org/resource/Information_lifecycle_management> ;
.
sto:ServiceOrchestration
  a owl:NamedIndividual ;
  a sto:Concern ;
  terms:creator sto:sebastian ;
  <http://voag.linkedmodel.org/voag#hasStakeholder> <https://www.wikidata.org/wiki/Q1548249> ;
  rdfs:comment "A Service/Data App are connected with Data Provider, other Services/Data Apps in order to fulfill a certain task, orchestrates by a central entity."@en ;
  rdfs:label "Service Orchestration"@en ;
  rdfs:seeAlso "IoT-A Requirement UNI.010" ;
  rdfs:seeAlso "https://dl.acm.org/citation.cfm?doid=3098208.3098210" ;
  skos:note "Publications referred: '<https://doi.org/10.1016/j.jksuci.2016.10.003>' '2.2.2. Middleware enablement' 'Page 300'" ;
  sto:hasDBpediaResource <http://dbpedia.org/resource/Orchestration_(computing)> ;
  sto:hasWikipediaArticle "https://en.wikipedia.org/wiki/Deployment"@en ;
  sto:hasWikipediaArticle "https://en.wikipedia.org/wiki/Orchestration_(computing)"@en ;
  sto:supports sto:ServiceComposition ;
.
sto:ServiceSelection
  a owl:NamedIndividual ;
  a sto:Concern ;
  terms:creator sto:sebastian ;
  rdfs:comment "The ability of a system to invoke or deploy the desired service/Data App."@en ;
  rdfs:label "Service Selection"@en ;
  sto:supports sto:ServiceComposition ;
.
sto:Service_Recovery
  a owl:NamedIndividual ;
  a sto:Concern ;
  terms:creator sto:MuhammadUsman ;
  rdfs:comment "Organizations should make sure that the cloud provider imitates the data and provides services in case the major site is down. Find out the time to restore services and the data loss if any, in case the chief site goes down."@en ;
  rdfs:label "Service Recovery"@en ;
  rdfs:seeAlso "https://dl.acm.org/citation.cfm?doid=3286606.3286865"@en ;
  sto:hasWikipediaArticle "https://en.wikipedia.org/wiki/Service_recovery"@en ;
  sto:supports sto:CloudComputing ;
  sto:supports sto:Reliability ;
.
sto:SmartCity
  a owl:NamedIndividual ;
  a sto:RelevantSubject ;
  rdfs:comment " A city that collects data which is used for better Maintenance of it's resources"@en ;
  rdfs:label " Smart City"@en ;
  sto:hasWikipediaArticle <https://en.wikipedia.org/wiki/Smart_city> ;
.
sto:SmartEnergy
  a owl:NamedIndividual ;
  a sto:RelevantSubject ;
  rdfs:comment " Intelligent technologies in value chain of energy industry"@en ;
  rdfs:label " Smart Energy"@en ;
  sto:hasWikipediaArticle <https://translate.google.com/translate?hl=en&sl=de&u=https://de.wikipedia.org/wiki/Smart_Energy&prev=search> ;
.
sto:SmartGrid
  a owl:NamedIndividual ;
  a sto:RelevantSubject ;
  rdfs:comment "An electrical grid having smart appliances"@en ;
  rdfs:label "Smart Grid"@en ;
  sto:hasWikipediaArticle <https://en.wikipedia.org/wiki/Smart_grid> ;
.
sto:Software_Updates
  a owl:NamedIndividual ;
  a sto:Concern ;
  terms:creator sto:MuhammadUsman ;
  rdfs:comment "Software update is the process that prevents compromise an IoT based  system. Organizations are yet to be geared up with mechanisms to Remotely Patch Connected Devices."@en ;
  rdfs:label "Software Updates"@en ;
  rdfs:seeAlso "https://ieeexplore.ieee.org/document/7919553"@en ;
  sto:hasWikipediaArticle "https://en.wikipedia.org/wiki/Wikipedia:Software_updates"@en ;
  sto:supports sto:Evolvability ;
.
sto:SpatialModeling
  a owl:NamedIndividual ;
  a sto:Concern ;
  rdfs:comment "A system shall have a semantic understanding of distance and location."@en ;
  rdfs:label "Spatial modeling"@en ;
  rdfs:seeAlso "IoT-A Requirement UNI.098" ;
  sto:hasDBpediaResource <http://dbpedia.org/resource/Spatial_analysis> ;
  sto:supports sto:DataDescription ;
  sto:supports sto:SemanticInteroperability ;
.
sto:Stakeholder
  rdfs:comment " A stakeholder is an individual, team, organization or classes thereof,having an interest in a concern and by extension an interest in the viewpoint and system." ;
  rdfs:label "Stakeholder"@en ;
  rdfs:seeAlso "IIC:PUB:G1:V1.80:20170131" ;
  rdfs:subClassOf foaf:Person ;
  rdfs:type owl:class ;
  skos:note "Publications referred: 'IIC:PUB:G1:V1.80:20170131' '4.1 STAKEHOLDERS' 'Page 20' " ;
  sto:hasWikipediaArticle "https://en.wikipedia.org/wiki/Stakeholder" ;
.
sto:Standard
  a owl:Class ;
  cc:attributionName "Copyright © 2016 IEC Geneva, Switzerland." ;
  cc:attributionURL <http://www.iec.ch> ;
  rdfs:comment "A document, established by consensus and approved by a recognized body, that provides, for common and repeated use, rules, guidelines or characteristics for activities or their results, aimed at the achievement of the optimum degree of order in a given context."@en ;
  rdfs:isDefinedBy sto:IEC ;
  rdfs:label "Standard"@en ;
  rdfs:seeAlso <http://www.iec.ch/standardsdev/publications/is.htm> ;
  rdfs:subClassOf sto:Publication ;
  sto:abbreviation "IS" ;
.
sto:StandardClassification
  a owl:Class ;
  a owl:NamedIndividual ;
  terms:creator sto:irlan ;
  rdfs:comment "Describes categorization areas that the different Standardizations Initiatives use to category Standards."@en ;
  rdfs:label "Standard Classification"@en ;
.
sto:StandardOrganization
  a owl:Class ;
  rdfs:comment "Define the standards organizations that develop and publish industry standards"@en ;
  rdfs:label "StandardOrganization"@en ;
  rdfs:subClassOf foaf:Organization ;
.
sto:StandardPart
  a owl:Class ;
  rdfs:comment "Typically Standards are divided into parts. E.g., ISA 95 has part Part 1: Models and Terminology, Part 2: Object Model Attributes, etc."@en ;
  rdfs:label "StandardPart" ;
  rdfs:subClassOf sto:Publication ;
.
sto:StandardizationFramework
  a owl:Class ;
  a owl:NamedIndividual ;
  terms:creator sto:irlan ;
  rdfs:comment "Describes existings Standardizations Initiatives, e.g, RAMI, NIST."@en ;
  rdfs:label "Standarization Framework"@en ;
  skos:altLabel "Reference Architecture"@en ;
.
sto:StreamProcessing
  a owl:NamedIndividual ;
  a sto:Concern ;
  terms:creator sto:sebastian ;
  rdfs:comment "Stream processing is a computer programming paradigm, equivalent to dataflow programming, event stream processing, and reactive programming, that allows some applications to more easily exploit a limited form of parallel processing. (source: wikipedia)"@en ;
  rdfs:label "Stream processing"@en ;
  sto:hasDBpediaResource <http://dbpedia.org/resource/Stream_processing> ;
  sto:supports sto:DataProcessing ;
.
sto:SyntacticInteroperability
  a owl:NamedIndividual ;
  a sto:Concern ;
  terms:creator sto:sebastian ;
  rdfs:comment "If two or more systems are capable of communicating with each other, they exhibit syntactic interoperability when using specified data formats and communication protocols. XML or SQL standards are among the tools of syntactic interoperability. This is also true for lower-level data formats, such as ensuring alphabetical characters are stored in a same variation of ASCII or a Unicode format (for English or international text) in all the communicating systems. source: <https://en.wikipedia.org/wiki/Interoperability>"@en ;
  rdfs:label "Syntactic Interoperability"@en ;
  rdfs:seeAlso "IoT-A Requirement UNI.071" ;
  rdfs:seeAlso "IoT-A Requirement UNI.096" ;
  rdfs:seeAlso "IoT-A Requirement UNI.241" ;
  rdfs:seeAlso "IoT-A Requirement UNI.318" ;
  rdfs:seeAlso "IoT-A Requirement UNI.326" ;
  rdfs:seeAlso "IoT-A Requirement UNI.327" ;
  rdfs:seeAlso "IoT-A Requirement UNI.506" ;
  rdfs:seeAlso "IoT-A Requirement UNI.709" ;
  rdfs:seeAlso "UNI.327"@en ;
  skos:note "Publications referred: '<https://doi.org/10.1016/j.jksuci.2016.10.003>' '2.8.2. Societal data service' 'Page 308'" ;
  sto:hasWikipediaArticle <https://en.wikipedia.org/wiki/Unified_interoperability#Syntactic_interoperability> ;
  sto:supports sto:Interoperability ;
.
sto:SyntacticInteroperablity
  rdfs:seeAlso "IoT-A Requirement UNI.311" ;
  rdfs:seeAlso "IoT-A Requirement UNI.312" ;
  rdfs:seeAlso "IoT-A Requirement UNI.313" ;
  rdfs:seeAlso "IoT-A Requirement UNI.315" ;
.
sto:SysML
  a owl:NamedIndividual ;
  a foaf:Document ;
  a sto:Publication ;
  a sto:Standard ;
  terms:creator sto:OMG ;
  rdfs:comment "The OMG Systems Modeling Language (OMG SysML) is a general-purpose graphical modeling language for specifying, analyzing, designing, and verifying complex systems that may include hardware, software, information, personnel, procedures, and facilities. In particular, the language provides graphical representations with a semantic foundation for modeling system requirements, behavior, structure, and parametrics, which is used to integrate with other engineering analysis models. It represents a subset of UML 2 with extensions needed to satisfy the requirements of the UML for Systems Engineering RFP as indicated in Figure 1. SysML leverages the OMG XML Metadata Interchange (XMI®) to exchange modeling data between tools, and is also intended to be compatible with the evolving ISO 10303-233 systems engineering data interchange standard."@en ;
  rdfs:label "Systems Modeling Language"@en ;
  foaf:maker sto:OMG ;
  sto:hasDBpediaResource <http://dbpedia.org/resource/Systems_Modeling_Language> ;
  sto:hasDeveloper sto:OMG ;
  sto:hasOfficialResource <http://sysml.org/> ;
  sto:hasOfficialResource <http://www.omgsysml.org/what-is-sysml.htm> ;
  sto:hasPublisher sto:OMG ;
  sto:hasWikipediaArticle <https://en.wikipedia.org/wiki/Systems_Modeling_Language> ;
  sto:relatedTo sto:DIN_SPEC_16592 ;
  sto:relatedTo sto:IEC_61131 ;
  sto:relatedTo sto:IEC_61360 ;
  sto:relatedTo sto:IEC_61499 ;
  sto:relatedTo sto:IEC_61804 ;
  sto:relatedTo sto:IEC_61850 ;
  sto:relatedTo sto:IEC_61987_X ;
  sto:relatedTo sto:IEC_62424 ;
  sto:relatedTo sto:IEC_62453 ;
  sto:relatedTo sto:IEC_62541 ;
  sto:relatedTo sto:IEC_62714 ;
  sto:relatedTo sto:ISO_13584 ;
  sto:relatedTo sto:ISO_14306 ;
  sto:relatedTo sto:ISO_15746 ;
  sto:relatedTo sto:ISO_15926 ;
  sto:relatedTo sto:ISO_18629 ;
  sto:relatedTo sto:ISO_18828-2 ;
  sto:relatedTo sto:ISO_20922 ;
  sto:relatedTo sto:ISO_22400 ;
  sto:relatedTo sto:ISO_29002 ;
  sto:relatedTo sto:ISO_ASTM_52915 ;
  sto:relatedTo sto:ISO_PAS_17506 ;
  sto:relatedTo sto:MathML ;
  sto:relatedTo sto:SysML ;
  sto:relatedTo sto:eClass ;
.
sto:SystemEngineer
  a <http://voag.linkedmodel.org/voag#StakeholderGroup> ;
  a owl:NamedIndividual ;
  a sto:Stakeholder ;
  rdfs:comment ""@en ;
  rdfs:label "System Engineer"@en ;
  skos:note "Publications referred: '(IIC:PUB:G1:V1.80:20170131' '3.5.1 BUSINESS VIEWPOINT' 'Page 15' 'Priyanka'" ;
.
sto:SystemEvolution
  a owl:NamedIndividual ;
  a sto:Concern ;
  terms:creator sto:sebastian ;
  rdfs:comment "Software evolution is the term used in software engineering (specifically software maintenance) to refer to the process of developing software initially, then repeatedly updating it for various reasons. (source: wikipedia)"@en ;
  rdfs:label "System evolution"@en ;
  rdfs:seeAlso "IoT-A Requirement UNI.211" ;
  rdfs:seeAlso "IoT-A Requirement UNI.229" ;
  sto:hasDBpediaResource <http://dbpedia.org/resource/Software_evolution> ;
  sto:supports sto:Evolvability ;
.
sto:SystemOperator
  a <http://voag.linkedmodel.org/voag#StakeholderGroup> ;
  a owl:NamedIndividual ;
.
sto:SystemRecovery
  a owl:NamedIndividual ;
  a sto:Concern ;
  terms:creator sto:SebastianBader ;
  rdfs:comment ""@en ;
  rdfs:label "System Recovery"@en ;
  sto:supports sto:Reliability ;
.
sto:TC_1
  a owl:NamedIndividual ;
  a sto:TechnicalCommittee ;
  terms:title "Terminology" ;
  rdfs:comment "To sanction the terms and definitions used in the different electrotechnical fields and to determine the equivalence of the terms used in the different languages. As a consequence, to prepare an International Electrotechnical Vocabulary aiming at the standardization and coordination of the terms relating to electrical sciences and techniques for use in the technical language and literature, in teaching, in technical specifications and in commercial exchanges, and at giving their equivalents in the different languages."@en ;
  rdfs:label "TC 1"@en ;
.
sto:TC_103
  a owl:NamedIndividual ;
  a sto:TechnicalCommittee ;
  terms:title "Transmitting equipment for radiocommunication"@en ;
  rdfs:comment """Standardization of transmitting equipment for radiocommunications purposes and electronic devices employing similar
techniques. The standardization work deals with methods of measurement, safety requirements and transmitter control and Interconnection"""@en ;
  rdfs:label "TC 103"@en ;
.
sto:TC_25
  a owl:NamedIndividual ;
  a sto:TechnicalCommittee ;
  terms:title "Quantities and units"@en ;
  rdfs:comment "To prepare international standards on quantities and units to be used in electrical technology. Such standards may relate to their definitions, names, letter symbols and use; to the relations in which they appear; and to the signs and symbols used with them."@en ;
  rdfs:label "TC 25"@en ;
.
sto:TC_3
  a owl:NamedIndividual ;
  a sto:TechnicalCommittee ;
  terms:title "Information structures and elements, identification and marking principles, documentation and graphical symbols"@en ;
  rdfs:comment "To prepare standards for the electrotechnical and related fields regarding:1) methods and rules associated with the human interpretation of information. This refers to:- presentation of information in technical documentation,- graphical symbols for use in technical documentation,- graphical symbols for the human interaction with equipment,2) methods and rules associated with the handling of information in computer sensible form. This refers to:- information models for the purpose of technical documentation and the exchange of technical information, and the identification of further needs for such models,- definition of data element types and data sets for use in information models and technical documentation, and for exchange of technical information.It includes definition and co-ordination of the information required during the whole life cycle of a device, system, or plant.3) General and safety application concerning the man-machine interface, marking and identification in electrical installations and equipment, marking systems and general rules for:- the meanings of colours and alternative means, when used for marking and identification,- the arrangement of indicating devices and actuators,- coding principles for indicating and actuating devices,- terminal designation of electrical and electronic components, apparatus and equipment,- the termination designation of certain designated conductors,- marking of electrical and electronic equipment with ratings related to supply and to its properties,- marking of bare and insulated conductors.These standards are principally intended for use by technical committees in the preparation of standards in accordance with the principles laid down in IEC Guide 104: Guide to the drafting of Safety Standards, and the role of committees with Safety Pilot Functions and Safety Group Functions, and in ISO/IEC Guide 51: Guidelines for the inclusion of safety aspects in standards."@en ;
  rdfs:label "TC 3"@en ;
.
sto:TC_40
  a owl:NamedIndividual ;
  a sto:TechnicalCommittee ;
  terms:title "Capacitors and resistors for electronic equipment"@en ;
  rdfs:comment "To prepare international standards for:a) Capacitors, resistors, thermistors and varistors intended for use in electronic equipment.b) Capacitors, resistors and inductors and complete electromagnetic interference (EMI) suppression filter units for EMI suppression (see note).c) Passive integrated circuits or networks containing resistors, capacitors, inductors or their combinations. For the dimensional standardization of the final package, requirements laid down by TC 47 shall be adopted whenever possible.d) Packaging of electronic components for automatic handling, which is an activity undertaken on behalf of all relevant component technical committees.e) Electric double layer capacitors for use in electric and electronic equipment.Note: In this work, use has to be made as far as possible of any relevant work of TC 51 on inductors, the CISPR on the measurement of EMI suppression characteristics and TC 77 on electromagnetic compatibility (EMC). Liaison has also to be maintained with TC 61, TC 66, TC 108 and other appropriate IEC Technical Committees on the safety aspects of EMI suppression components and filter units."@en ;
  rdfs:label "TC 40"@en ;
.
sto:TC_44
  a owl:NamedIndividual ;
  a sto:TechnicalCommittee ;
  terms:title "Safety of machinery - Electrotechnical aspects"@en ;
  rdfs:comment "Standardization in the field of the application of electro-technical equipment and systems to machinery (including a group of machines working together in a coordinated manner, excluding higher-level systems aspects) not portable by hand while working, but which may include mobile equipment. The equipment covered commences at the point of connection of the electrical supply to the machinery.Standardization of interfaces (excluding local area networks and fieldbus) between control equipment and the electro-technical equipment of machinery.Standardization of electrotechnical equipment and systems relating to the safeguarding of persons from hazards of the machinery, its associated equipment and the environment.To coordinate with ISO all matters concerning the safety of machinery.."@en ;
  rdfs:label "TC 44"@en ;
.
sto:TC_56
  a owl:NamedIndividual ;
  a sto:TechnicalCommittee ;
  terms:title "Dependability"@en ;
  rdfs:comment """To prepare international standards in the field of dependability, in all appropriate technological areas, including those not normally dealt with by IEC Technical Committees. Dependability covers the availability performance and its influencing factors: reliability performance, maintainability performance and maintenance support performance (including management of obsolescence). The standards provide systematic methods and tools for the dependability assessment and management of equipment, services and systems throughout their life cycles.
The standards cover generic aspects on reliability and maintainability programme management, testing and analytical techniques, software and system dependability, life cycle costing, technical risk analysis and project risk management. This includes standards related to product issues from component reliability to guidance for engineering dependability of systems, standards related to process issues from technological risk analysis to integrated logistics support and standards related to management issues from dependability program management to managing for obsolescence.
The application of these standards may raise safety related issues, though the standards themselves do not cover safety. They may be applied to business risk analysis but these risk areas are not dealt with by TC 56."""@en ;
  rdfs:label "TC 56"@en ;
.
sto:TC_57
  a owl:NamedIndividual ;
  a sto:TechnicalCommittee ;
  terms:title "Power systems management and associated information exchange"@en ;
  rdfs:comment """To prepare international standards for power systems control equipment and systems including EMS (Energy Management Systems), SCADA (Supervisory Control And Data Acquisition), distribution automation, teleprotection, and associated information exchange for real-time and non-real-time information, used in the planning, operation and maintenance of power systems. Power systems management comprises control within control centres, substations and individual pieces of primary equipment including telecontrol and interfaces to equipment, systems and databases, which may be outside the scope of TC 57. The special conditions in a high voltage environment have to be taken into consideration.
Note 1: Standards prepared by other technical committees of the IEC and organizations such as ITU and ISO shall be used where applicable.
Note 2: Although the work of TC 57 is chiefly concerned with standards for electric power systems, these standards may also be useful for application by the relevant bodies to other geographical widespread processes.
Note 3: Whereas standards related to measuring and protection relays and to the control and monitoring equipment used with these systems are treated by TC 95, TC 57 deals with the interface to the control systems and the transmission aspects for teleprotection systems. Whereas standards related to equipment for electrical measurement and load control are treated by TC 13, TC 57 deals with the interface of equipment for interconnection lines and industrial consumers and producers requiring energy management type interfaces to the control system."""@en ;
  rdfs:label "TC 57"@en ;
.
sto:TC_65
  a owl:NamedIndividual ;
  a sto:TechnicalCommittee ;
  terms:title "Industrial-process measurement, control and automation"@en ;
  rdfs:comment "To prepare international standards for systems and elements used for industrial-process measurement and control concerning continuous and batch processes."@en ;
  rdfs:label "TC 65"@en ;
.
sto:TC_66
  a owl:NamedIndividual ;
  a sto:TechnicalCommittee ;
  terms:title "Safety of measuring"@en ;
  terms:title "control and laboratory equipment"@en ;
  rdfs:comment """To prepare safety standards for test and measurement equipment, industrial-process control equipment, and laboratory equipment wherever they are used.
Such equipment includes:
a) equipment and systems to measure, test, generate, and analyse, simple and complex electromagnetic quantities and equipment that by electromagnetic means measure physical quantities.
Note: Aspects of this equipment other than safety are covered by other technical committees.
b) equipment and systems for industrial-process measurement and control.
Note: Aspects of this equipment other than safety are covered by TC 65 except that SC 65A has a Horizontal Safety Function relating to the functional safety of electrical/electronic/ programmable electronic systems and SC 65B is responsible for the functional safety of programmable controllers.
c) laboratory equipment for analysis, handling and preparation of materials.
Note: This equipment includes measuring instruments, systems and their accessories, for preparation, treatment and analysis of materials in the fields of research, medicine, industry and education, and for environmental monitoring.
TC 66 has a Group Safety Function in accordance with IEC Guide 104 for the equipment in categories a) to c) above."""@en ;
  rdfs:label "TC 66"@en ;
.
sto:TC_77
  a owl:NamedIndividual ;
  a sto:TechnicalCommittee ;
  terms:title "Electromagnetic compatibility"@en ;
  rdfs:comment """Standardization - to prepare standards and technical reports - in the field of electromagnetic compatibility (EMC), with
particular emphasis on general application and use by product committees. (Horizontal function). The scope covers the following aspects of EMC:
- Immunity and related items, over the whole frequency range: basic and generic standards, - emission in the low frequency range (f <= 9 kHz, e.g. harmonics and voltage fluctuations): basic, generic and product (family) standards,
- emission in the high frequency range (f > 9 kHz): disturbances not covered by CISPR 10 (1992), in co-ordination with CISPR (e.g. mains signalling).
Product immunity standards are not included. However, at the request of product committees, TC 77 may also prepare such standards under the co-ordination of ACEC.
Horizontal Safety Function: Electromagnetic compatibility in so far as safety aspects are involved."""@en ;
  rdfs:label "TC 77"@en ;
.
sto:TC_79
  a owl:NamedIndividual ;
  a sto:TechnicalCommittee ;
  terms:title "Alarm and electronic security systems"@en ;
  rdfs:comment "To prepare international standards for the protection of buildings, persons, areas and properties against fraudulent actions having the purpose to enter in a place or to take or to use something without permission and other threat related to persons.The scope includes, but is not limited to equipment and systems, either used by ordinary persons or by trained people in the following residential and non residential applications:- Access control systems- Alarm transmission systems- Video surveillance systems- Combined and/or integrated systems even including fire alarm systems*- Fire detection and fire alarm systems*- Intruder and hold-up alarm systems- Remote receiving and/or surveillance centres- Social alarm systems.These systems can be used for providing a local or remote alarm; they can be used for calling private guards, social assistance, fire brigade or police force. They can be used for recording and transmission of dated or undated information, sounds, pictures of places and people for surveillance purposes. The standards cover:- terminology;- technical characteristics regarding performance criteria, reliable operation, installation, maintenance;- testing for detection, monitoring, recording, triggering an alarm and transmission to a remote centre including procedures and protocols for communication.Electrical safety, environmental conditions and behaviour of alarm systems regarding electromagnetic compatibility are also considered with reference to the appropriate standards (e.g. Guide ISO/IEC 51).* ISO/TC21/SC3 is in charge of the production of standards for \"Fire detection and alarm systems\"."@en ;
  rdfs:label "TC 79"@en ;
.
sto:TC_8
  a owl:NamedIndividual ;
  a sto:TechnicalCommittee ;
  terms:title "Systems aspects of electrical energy supply"@en ;
  rdfs:comment "To prepare and coordinate, in co-operation with other TC/SCs, the development of international standards and other deliverables with emphasis on overall system aspects of electricity supply systems and acceptable balance between cost and quality for the users of electrical energy. Electricity supply system encompasses transmission and distribution networks, generators and loads with their network interfaces."@en ;
  rdfs:label "TC 8"@en ;
.
sto:TC_88
  a owl:NamedIndividual ;
  a sto:TechnicalCommittee ;
  terms:title "Wind energy generation systems"@en ;
  rdfs:comment """TC 88 standardization in the field of wind energy generation systems including wind turbines, wind power plants onshore and offshore and interaction with the electrical system(s) to which energy is supplied.

These standards address site suitability and resource assessment, design
requirements, engineering integrity, modeling requirements, measurement techniques, test procedures, operation and maintenance. Their purpose is to provide a basis for design, quality assurance and technical aspects for certification. The standards address site-specific conditions, all systems and subsystems of wind turbines and wind power plants, such as mechanical, and electrical systems, support structures, control and protection as well as communication systems for monitoring, centralized and distributed control and evaluation, implementation of grid connection requirements for wind power plants, and environmental aspects of wind power development. The TC 88 standards will be developed based on and in agreement with appropriate IEC/ISO standards."""@en ;
  rdfs:label "TC 88"@en ;
.
sto:TC_91
  a owl:NamedIndividual ;
  a sto:TechnicalCommittee ;
  terms:title "Electronics assembly technology"@en ;
  rdfs:comment "To prepare international standards on design, manufacturing and testing of electronic assemblies including the requirements and tests for materials and components used to manufacture circuit boards and electronic assemblies, as well as the formats of electronic data and libraries for describing these products and processes."@en ;
  rdfs:label "TC 91"@en ;
.
sto:TC_94
  a owl:NamedIndividual ;
  a sto:TechnicalCommittee ;
  terms:title "All-or-nothing electrical relays"@en ;
  rdfs:comment """To prepare international standards applicable to all-or-nothing electrical relays used in the various fields of Electrical Engineering covered by the IEC, normally produced in very large
numbers as components of electromechanical or electronic
equipment and eventually submitted to Quality Assurance requirements based on sampling techniques."""@en ;
  rdfs:label "TC 94"@en ;
.
sto:TC_95
  a owl:NamedIndividual ;
  a sto:TechnicalCommittee ;
  terms:title "Measuring relays and protection equipment"@en ;
  rdfs:comment "Standardisation of measuring relays and protection equipment used in various fields of electrical engineering covered by IEC, taking into a ccount combinations of devices to form schemes for power system protection including the control, monitoring and process interface equipment used with those systems.Excluded are the following:All devices covered by standards prepared by other IEC Technical Committees, for example instrument transformers (TC 38)."@en ;
  rdfs:label "TC 95"@en ;
.
sto:TS-0009
  a owl:NamedIndividual ;
  a foaf:Document ;
  a sto:Publication ;
  a sto:Standard ;
  terms:creator sto:oneM2M ;
  terms:title "HTTP Protocol Binding"@en ;
  rdfs:comment """The present document will cover the protocol specific part of communication protocol used by oneM2M compliant systems as RESTful HTTP binding.
The scope of the present document is (not limited to as shown below):
• Binding oneM2M Protocol primitive types to HTTP method.
• Binding oneM2M response status codes (successful/unsuccessful) to HTTP response codes.
• Binding oneM2M RESTful resources to HTTP resources.
The present document is depending on Core Protocol specification (oneM2M TS-0004) for data types."""@en ;
  rdfs:label "TS-0009"@en ;
  foaf:maker sto:oneM2M ;
  sto:hasClassification sto:IICFFrameworkLayer ;
  sto:hasOfficialResource <https://w3id.org/i40/www.onem2m.org/images/files/deliverables/Release2A/TS-0009-HTTP_Protocol_Binding-v_2_13_1.pdf> ;
  sto:hasPublisher sto:oneM2M ;
.
sto:TSMP
  a owl:NamedIndividual ;
  a foaf:Document ;
  a sto:Publication ;
  a sto:TechnicalSpecification ;
  terms:creator sto:sebastian ;
  rdfs:comment "Time Synchronized Mesh Protocol (TSMP): A communications protocol for self-organizing networks of wireless devices called motes. TSMP devices stay synchronized to each other and communicate in timeslots, similar to other TDM (time-division multiplexing) systems. (source: https://www.postscapes.com/internet-of-things-protocols/)"@en ;
  rdfs:label "TSMP"@en ;
  sto:hasWikipediaArticle <https://en.wikipedia.org/wiki/TSMP> ;
.
sto:TechnicalCommittee
  a owl:Class ;
  a owl:NamedIndividual ;
  rdfs:comment "Specifies the representitive code name of the Technical Committee that covers a Standard for e.g, TC 1, SC 3C. Many thousand experts carry out standardization work in the IEC in TCs (technical committees) and SCs (subcommittees), in hundreds of working groups, project and maintenance teams. They represent the national electrotechnical needs of IEC Member countries and of many Affiliates at the global level in the IEC. These technical experts are sent by industry, governments, test and research laboratories, academia and even consumer groups to work on the global, neutral and independent platform of the IEC. That's where they develop globally relevant, voluntary, consensus based IEC International Standards."@en ;
  rdfs:isDefinedBy sto:IEC ;
  rdfs:label "Technical Committee"@en ;
  rdfs:seeAlso <http://www.iec.ch/dyn/www/f?p=103:62:9979528650478:::62:FSP_ORG_ID,FSP_LANG_ID:,25> ;
  rdfs:subClassOf foaf:Organization ;
  skos:note "1.sto:       a property explaining that TC and SC are managed by SMB (Standardization Management Board) needs to be added" ;
  sto:abbreviation "TC" ;
.
sto:TechnicalReport
  a owl:Class ;
  a owl:NamedIndividual ;
  cc:attributionURL "http://www.iec.ch" ;
  rdfs:comment "Specifies that a given Publication is a Technical Report"@en ;
  rdfs:comment "Technical Reports contain collected data of a kind different from that normally published as an International Standard, for example data obtained from a survey carried out among national committees, data of work in other international organizations or data on \"the state of the art\" in relation to standards of national committees on a particular subject.Technical Reports are entirely informative in nature and shall not contain matter implying that they are normative"@en ;
  rdfs:isDefinedBy sto:IEC ;
  rdfs:label "Technical Report"@en ;
  rdfs:seeAlso <http://www.iec.ch/standardsdev/publications/tr.htm> ;
  rdfs:subClassOf sto:Publication ;
  sto:abbreviation "TR" ;
.
sto:TechnicalSpecification
  a owl:Class ;
  a owl:NamedIndividual ;
  cc:attributionURL <http://www.iec.ch> ;
  cc:attributionURL "http://www.iec.ch" ;
  rdfs:comment "Specifies that a given Publication is a Technical Specification"@en ;
  rdfs:comment "Technical Specifications are often published when the subject under question is still under development or when insufficient consensus for approval of an International Standard is available.Technical Specifications approach International Standards in terms of detail and completeness, but have not yet passed through all approval stages either because consensus has not been reached or because standardization is seen to be premature."@en ;
  rdfs:isDefinedBy sto:IEC ;
  rdfs:label "Technical Specification"@en ;
  rdfs:seeAlso <http://www.iec.ch/standardsdev/publications/ts.htm> ;
  rdfs:subClassOf sto:Publication ;
  sto:abbreviation "TS" ;
.
sto:Technology
  a owl:Class ;
  a owl:NamedIndividual ;
  terms:creator sto:sebastian ;
  terms:creator "sebastian"@en ;
  rdfs:comment "A Technology is an implementation of one or many standards in order to achieve a goal."@en ;
  rdfs:label "Technology"@en ;
  rdfs:subClassOf sto:Publication ;
.
sto:Telehash
  a owl:NamedIndividual ;
  a foaf:Document ;
  a sto:Publication ;
  a sto:TechnicalSpecification ;
  terms:creator sto:sebastian ;
  rdfs:comment "Telehash - JSON+UDP+DHT=Freedom: A secure wire protocol powering a decentralized overlay network for apps and devices. (source: https://www.postscapes.com/internet-of-things-protocols/)"@en ;
  rdfs:label "Telehash"@en ;
  sto:hasOfficialResource <http://telehash.org/> ;
.
sto:The_Industrial_Internet_of_Things_Volume_G1_Reference_Architecture
  a <https://www.w3.org/ns/oaSpecificResource> ;
  rdfs:label "Industrial Internet Architecture Version 1"@en ;
  skos:note "The Industrial Internet of Things Volume G1: Reference Architecture IIC:PUB:G1:V1.80:20170131" ;
  sto:hasOpenResource <https://www.iiconsortium.org/IIC_PUB_G1_V1.80_2017-01-31.pdf> ;
.
sto:The_Industrial_Internet_of_Things_Volume_G5_Connectivity_Framework
  a <https://www.w3.org/ns/oaSpecificResource> ;
  rdfs:label "The Industrial Internet of Things Volume G5: Connectivity Framework "@en ;
  skos:note "The Industrial Internet of Things Volume G5: Connectivity Framework IIC:PUB:G5:V1.0:PB:20170228" ;
  sto:hasOpenResource <https://www.iiconsortium.org/pdf/IIC_PUB_G5_V1.0_PB_20170228.pdf> ;
.
sto:ThingDescription
  a owl:NamedIndividual ;
  a sto:Concern ;
  terms:creator sto:sebastian ;
  <http://voag.linkedmodel.org/voag#hasStakeholder> <https://www.wikidata.org/wiki/Q1548249> ;
  <http://voag.linkedmodel.org/voag#hasStakeholder> <owl:Developer> ;
  rdfs:comment "'Things' in terms of physical objects in the IoT need to be described in order to identify them and to provide further information."@en ;
  rdfs:label "Thing description"@en ;
  rdfs:seeAlso "IoT-A Requirement UNI.036" ;
  rdfs:seeAlso "IoT-A Requirement UNI.042" ;
  rdfs:seeAlso "IoT-A Requirement UNI.213" ;
  rdfs:seeAlso "IoT-A Requirement UNI.237" ;
  rdfs:seeAlso "IoT-A Requirement UNI.240" ;
  rdfs:seeAlso "IoT-A Requirement UNI.404" ;
  rdfs:seeAlso "IoT-A Requirement UNI.509" ;
  rdfs:seeAlso "IoT-A Requirement UNI.512" ;
  sto:supports sto:SemanticInteroperability ;
.
sto:ThingMobility
  a owl:NamedIndividual ;
  a sto:Concern ;
  terms:creator sto:sebastian ;
  rdfs:comment "A Thing in terms of Internet of Things (IoT) needs to be moveable."@en ;
  rdfs:label "Thing mobility"@en ;
  rdfs:seeAlso "IoT-A Requirement UNI.050" ;
  rdfs:seeAlso "IoT-A Requirement UNI.233" ;
  sto:supports sto:DataAccess ;
  sto:supports sto:IoT ;
  sto:supports sto:ServiceDeployment ;
.
sto:ThingRepresentation
  a owl:NamedIndividual ;
  a sto:Concern ;
  terms:creator sto:sebastian ;
  rdfs:comment "Physical objects need to be represented."@en ;
  rdfs:label "Thing representation"@en ;
  rdfs:seeAlso "IoT-A Requirement UNI.239" ;
  sto:supports sto:IoT ;
.
sto:Thread
  a owl:NamedIndividual ;
  a foaf:Document ;
  a sto:Publication ;
  a sto:Standard ;
  terms:creator sto:sebastian ;
  rdfs:comment "Thread - Built on open standards and IPv6 technology with 6LoWPAN as its foundation. (source: https://www.postscapes.com/internet-of-things-protocols/)"@en ;
  rdfs:label "Thread"@en ;
  sto:hasOfficialResource <http://www.threadgroup.org/About.aspx> ;
.
sto:TimeSynchronization
  a owl:NamedIndividual ;
  a sto:Concern ;
  terms:creator sto:sebastian ;
  <http://voag.linkedmodel.org/voag#hasStakeholder> <https://w3id.org/i40/Developer> ;
  rdfs:label "Time Synchronization"@en ;
  rdfs:seeAlso "IoT-A Requirement UNI.089" ;
  sto:hasDBpediaResource <http://dbpedia.org/resource/Synchronization_(computer_science)> ;
  sto:hasDBpediaResource "Synchronization refers to one of two distinct but related concepts: synchronization of processes, and synchronization of data. Process synchronization refers to the idea that multiple processes are to join up or handshake at a certain point, in order to reach an agreement or commit to a certain sequence of action. Data synchronization refers to the idea of keeping multiple copies of a dataset in coherence with one another, or to maintain data integrity. Process synchronization primitives are commonly used to implement data synchronization. (sourc: wikipedia)"@en ;
  sto:supports sto:ServiceComposition ;
.
sto:TrustedConnector
  a owl:NamedIndividual ;
  a sto:Technology ;
  terms:creator sto:sebastian ;
  terms:creator "sebastian" ;
  dul:associatedWith sto:DIN_SPEC_27070 ;
  dul:associatedWith sto:IDSRAMReferenceArchitectureModel ;
  rdfs:comment "The advent of the Industrial Internet of Things (IIoT) also raises challenges with respect to security and privacy of sensitive and personal data that is created by sensors and processed by services hosted in different administrative domains. The Industrial Data Space initiative addresses these challenges and proposes a secure edge gateway platform named \"Trusted Connector\". In this report, we introduce the main security building blocks of the Trusted Connector and point out how they help protecting business-critical data and preserving the user's privacy."@en ;
  rdfs:label "IDS Trusted Connector"@en ;
  sto:alignsWith sto:DIN_SPEC_27070 ;
  sto:hasOfficialResource <https://arxiv.org/abs/1804.09442> ;
.
sto:Trustworthiness
  a owl:NamedIndividual ;
  a sto:Concern ;
  terms:creator sto:sebastian ;
  rdfs:comment "Trustworthiness is the degree of confidence one has that the system performs as expected in respect to all the key system characteristics in the face of environmental disruptions, human errors, system faults and attacks. source: IISF"@en ;
  rdfs:label "Trustworthiness"@en ;
  rdfs:seeAlso "IoT-A Requirement UNI.062" ;
  rdfs:seeAlso "IoT-A Requirement UNI.602" ;
  rdfs:seeAlso "IoT-A Requirement UNI.613" ;
  rdfs:seeAlso "https://dl.acm.org/citation.cfm?doid=3180465.3180470" ;
  rdfs:seeAlso "https://ieeexplore.ieee.org/document/6188257"@en ;
  sto:hasDBpediaResource <http://dbpedia.org/resource/Software_trustworthiness> ;
.
sto:UDP
  a owl:NamedIndividual ;
  a foaf:Document ;
  a sto:Publication ;
  a sto:Standard ;
  terms:creator sto:sebastian ;
  rdfs:comment "UDP (User Datagram Protocol) - A simple OSI transport layer protocol for client/server network applications based on Internet Protocol (IP). UDP is the main alternative to TCP and one of the oldest network protocols in existence, introduced in 1980. UDP is often used in applications specially tuned for real-time performance."@en ;
  rdfs:label "UDP"@en ;
  sto:hasOfficialResource <https://tools.ietf.org/html/rfc768> ;
.
sto:UN-CEFACT
  a owl:NamedIndividual ;
  a foaf:Organization ;
  a sto:StandardOrganization ;
  rdfs:comment "UN/CEFACT is the United Nations Centre for Trade Facilitation and Electronic Business. It was established as an intergovernmental body of the United Nations Economic Commission for Europe (UNECE) in 1996 and evolved from UNECE’s long tradition of work in trade facilitation."@en ;
  sto:abbreviation "UN/CEFACT" ;
  sto:hasDBpediaResource <http://dbpedia.org/page/UN/CEFACT> ;
  sto:hasHeadquaterIn dbr:Geneva ;
  sto:hasOfficialResource <https://www.unece.org/cefact/> ;
  sto:hasWikipediaArticle <https://en.wikipedia.org/wiki/UN/CEFACT> ;
  sto:orgName "United Nations Centre for Trade Facilitation and Electronic Business"@en ;
.
sto:UPnP
  a owl:NamedIndividual ;
  a foaf:Document ;
  a sto:Publication ;
  a sto:TechnicalSpecification ;
  terms:creator sto:sebastian ;
  rdfs:comment "UPnP (Universal Plug and Play) - Now managed by the Open Connectivity Foundation is a set of networking protocols that permits networked devices to seamlessly discover each other's presence on the network and establish functional network services for data sharing, communications, and entertainment.(source: https://www.postscapes.com/internet-of-things-protocols/)"@en ;
  rdfs:label "UPnP"@en ;
  sto:hasOfficialResource <https://openconnectivity.org/upnp> ;
.
sto:URI
  a owl:NamedIndividual ;
  a foaf:Document ;
  a sto:Publication ;
  a sto:TechnicalSpecification ;
.
sto:Unicast
  a owl:NamedIndividual ;
  a sto:Concern ;
  terms:creator sto:sebastian ;
  rdfs:comment "one-to-one connectivity"@en ;
  rdfs:label "Unicast"@en ;
  rdfs:seeAlso "IoT-A Requirement UNI.301" ;
  rdfs:seeAlso "IoT-A Requirement UNI.304" ;
  sto:supports sto:CardinalityOfDataSources ;
.
sto:UnreliableNetwork
  a owl:NamedIndividual ;
  a sto:Concern ;
  terms:creator sto:sebastian ;
  <http://voag.linkedmodel.org/voag#hasStakeholder> "Developer"@en ;
  <http://voag.linkedmodel.org/voag#hasStakeholder> "System Architect"@en ;
  rdfs:comment "Productive systems must inherently cover issues caused by unreliable networks."@en ;
  rdfs:label "Unreliable Network"@en ;
  rdfs:seeAlso "IoT-A Requirement UNI.308" ;
  rdfs:seeAlso "IoT-A Requirement UNI.318" ;
  sto:supports sto:Reliability ;
.
sto:UserInteraction
  a owl:NamedIndividual ;
  a sto:Concern ;
  terms:creator sto:sebastian ;
  <http://voag.linkedmodel.org/voag#hasStakeholder> <http://purl.oclc.org/NET/mvco.owl#EndUser> ;
  rdfs:comment "Interaction design, often abbreviated as IxD, is defined as \"the practice of designing interactive digital products, environments, systems, and services.\" While the digital side of this statement is true, Interaction design is also valid when creating physical (non-digital) products, covering the ideology of how a user may interact with it. (source: wikipedia)"@en ;
  rdfs:label "User Interaction"@en ;
  rdfs:seeAlso "IoT-A Requirement UNI.019" ;
  rdfs:seeAlso "IoT-A Requirement UNI.092" ;
  rdfs:seeAlso "IoT-A Requirement UNI.214" ;
  rdfs:seeAlso "IoT-A Requirement UNI.252" ;
  sto:hasDBpediaResource <http://dbpedia.org/resource/Interaction_design> ;
  sto:supports sto:UserExperience ;
.
sto:UserPreferences
  a owl:NamedIndividual ;
  a sto:Concern ;
  terms:creator sto:sebastian ;
  rdfs:comment "Users can have the possibility to prefer one service over another for any reason."@en ;
  rdfs:label "User Preferences"@en ;
  rdfs:seeAlso "IoT-A Requirement UNI.253" ;
  sto:supports sto:ServiceLevelAgreements ;
.
sto:VDI
  a owl:NamedIndividual ;
  a foaf:Organization ;
  a sto:StandardOrganization ;
  terms:creator sto:sebastian ;
  terms:creator "sebastian" ;
  rdfs:comment "Verein Deutscher Ingenieure (VDI) (English: Association of German Engineers) is an organization with over 150,000 engineers and natural scientists. More than 12,000 honorary experts process the latest findings every year to promote the technology location. Established in 1856, the VDI is today the largest engineering association in Western Europe. The role of the VDI in Germany is comparable to that of the American Society of Civil Engineers (ASCE) in the United States or Engineers Australia (EA) in Australia barring the broader field of work of the VDI. The VDI is not a union. The association promotes the advancement of technology and represents the interests of engineers and of engineering businesses in Germany."@en ;
  rdfs:label "VDI"@en ;
  sto:abbreviation "VDI"@en ;
  sto:formationDate "1856-05-12"^^xsd:date ;
  sto:hasDBpediaResource <http://dbpedia.org/resource/VDI> ;
  sto:hasHeadquaterIn dbr:Berlin ;
  sto:hasOfficialResource <http://www.vdi.eu/> ;
  sto:hasWikipediaArticle <https://en.wikipedia.org/wiki/VDI> ;
  sto:orgName "Association of German Engineers"@en ;
  sto:orgName "Verein Deutscher Ingenieure"@de ;
.
sto:VDI_VDE_2182
  a owl:NamedIndividual ;
  a sto:Standard ;
  terms:creator sto:VDI ;
  terms:creator "sebastian" ;
  terms:license sto:PrivateLicenseDocument ;
  terms:title "IT-security for industrial automation"@en ;
  terms:title "Informationssicherheit in der industriellen Automatisierung"@de ;
  rdfs:comment "This guideline describes how specific measures can be implemented in order to guarantee the IT security of automated machines and plant; aspects of the automation devices, automation systems, and automation applications used are considered. A uniform, feasible procedure for ensuring IT security throughout the entire life cycle of automation devices, systems, and applications is described, based on common terms and definitions agreed by the manufacturers of automation devices and systems and their users (e.g., machine manufacturers, integrators, operators). The life cycle covers the development, integration, operation, migration, and decommissioning phases.This guideline defines a simple procedure model for the development and description of IT Security. The model consists of eight steps."@en ;
  rdfs:label "VDI/VDE 2182"@en ;
  foaf:maker sto:VDI ;
  sto:hasClassification rami:Security ;
  sto:hasDeveloper sto:VDI ;
  sto:hasOfficialResource <http://www.vdi.eu/nc/guidelines/vdivde_2182_blatt_1-informationssicherheit_in_der_industriellen_automatisierung_allgemeines_vorgehensmode/> ;
  sto:hasPublisher sto:VDI ;
.
sto:VDMA
  a owl:NamedIndividual ;
  a foaf:Organization ;
  a sto:StandardOrganization ;
  rdfs:comment "The Mechanical Engineering Industry Association (Verband Deutscher Maschinen- und Anlagenbau – VDMA) has its headquarters in Frankfurt am Main, Germany, and represents around 3,200 members, making it the largest industry association in Europe. The Association represents the interests of the predominantly medium-sized companies in the mechanical engineering industry towards policymakers and society, as well as towards business, the scientific community, public authorities and the media. With more than one million employees and a turnover of around EUR 218 billion (2015), mechanical and plant engineering is Germany’s largest employer in the industrial sector.In addition, VDMA sees itself as a platform that provides its member companies with various networks where they can discuss technological challenges, interdisciplinary issues and many other topics."@en ;
  sto:abbreviation "VDMA" ;
  sto:formationDate "1892-11-15"^^xsd:date ;
  sto:hasDBpediaResource <http://dbpedia.org/resource/VDMA> ;
  sto:hasHeadquaterIn dbr:Frankfurt ;
  sto:hasOfficialResource <http://www.vdma.org> ;
  sto:hasWikipediaArticle <https://en.wikipedia.org/wiki/Mechanical_Engineering_Industry_Association> ;
  sto:orgName "Mechanical Engineering Industry Association"@en ;
  sto:orgName "Verband Deutscher Maschinen- und Anlagenbau"@de ;
.
sto:VDMA_24582
  a owl:NamedIndividual ;
  a foaf:Document ;
  a sto:Publication ;
  a sto:Standard ;
  terms:creator sto:VDMA ;
  rdfs:comment "Fieldbus neutral reference architecture for Condition Monitoring in production automation"@en ;
  rdfs:label "VDMA 24582"@en ;
  foaf:maker sto:VDMA ;
  sto:hasClassification rami:ConditionMonitoring ;
  sto:hasOfficialResource <https://www.vdma.org/documents/105628/2244593/Inhalt+VDMA+24582_en.pdf/> ;
  sto:hasPublisher sto:VDMA ;
.
sto:VendorLockin
  a owl:NamedIndividual ;
  a sto:Concern ;
  terms:creator sto:MuhammadUsman ;
  rdfs:comment """There is a lot of competition among vendors to dominate the cloud market. According to Columbus’ report, a study conducted by IDG Cloud Computing
Study realized that Cloud investment rose by 19% in larger scale enterprises consisting of more than a thousand employees who spend a mean of $3.3 million
annually."""@en ;
  rdfs:label "Vendor Lockin"@en ;
  rdfs:seeAlso "https://ieeexplore.ieee.org/document/7987175"@en ;
  sto:hasWikipediaArticle "https://en.wikipedia.org/wiki/Vendor_lock-in"@en ;
  sto:supports sto:BusinessContext ;
  sto:supports sto:CloudComputing ;
.
sto:Viewpoint
  a owl:Class ;
  a owl:NamedIndividual ;
  terms:creator "sebastian" ;
  rdfs:comment "ISO 42010 definition of a Viewpoint"@en ;
  rdfs:label "Viewpoint" ;
  rdfs:seeAlso <https://www.iso.org/standard/50508.html> ;
  rdfs:subClassOf sto:StandardClassification ;
  sto:hasDBpediaResource <http://dbpedia.org/resource/ISO/IEC_42010> ;
  sto:hasOfficialResource <http://www.iso-architecture.org/42010/> ;
  sto:hasWikipediaArticle <https://en.wikipedia.org/wiki/ISO/IEC_42010#Conceptual_Model_-_Architecture_Viewpoint> ;
.
sto:VirtualEntities
  rdfs:seeAlso "IoT-A Requirement UNI.409" ;
.
sto:VirtualEntity
  a owl:NamedIndividual ;
  a sto:Concern ;
  terms:creator sto:sebastian ;
  rdfs:comment "Entities are provided through a virtual form."@en ;
  rdfs:label "Virtual Entity"@en ;
  rdfs:seeAlso "UNI.030"@en ;
  rdfs:seeAlso "UNI.066"@en ;
  rdfs:seeAlso "UNI.402"@en ;
  skos:note "Publications referred: 'IIC:PUB:G1:V1.80:20170131' '6.1 THE CONTROL DOMAIN' 'Page 28' " ;
  sto:hasDBpediaResource <http://dbpedia.org/resource/Digital_twin> ;
  sto:supports sto:ThingRepresentation ;
.
sto:W3C
  a owl:NamedIndividual ;
  a foaf:Organization ;
  a sto:StandardOrganization ;
  rdfs:comment "The World Wide Web Consortium (W3C) is the main international standards organization for the World Wide Web (abbreviated WWW or W3). Founded and currently led by Tim Berners-Lee, the consortium is made up of member organizations which maintain full-time staff for the purpose of working together in the development of standards for the World Wide Web. As of 4 November 2015, the World Wide Web Consortium (W3C) has 408 members. The W3C also engages in education and outreach, develops software and serves as an open forum for discussion about the Web."@en ;
  rdfs:label "W3C"@en ;
  sto:abbreviation "W3C" ;
  sto:formationDate "1994-10-01"^^xsd:date ;
  sto:hasDBpediaResource <http://dbpedia.org/resource/World_Wide_Web_Consortium> ;
  sto:hasHeadquaterIn dbr:_Massachusetts ;
  sto:hasOfficialResource <https://www.w3.org/> ;
  sto:hasWikipediaArticle <https://en.wikipedia.org/wiki/World_Wide_Web_Consortium> ;
  sto:orgName "World Wide Web Consortium"@en ;
.
sto:W3C_DCAT
  a owl:NamedIndividual ;
  a foaf:Document ;
  a sto:Publication ;
  a sto:Standard ;
  terms:creator sto:W3C ;
  terms:creator sto:sebastian ;
  rdfs:comment """DCAT is an RDF vocabulary designed to facilitate interoperability between data catalogs published on the Web. This document defines the schema and provides examples for its use.

By using DCAT to describe datasets in data catalogs, publishers increase discoverability and enable applications easily to consume metadata from multiple catalogs. It further enables decentralized publishing of catalogs and facilitates federated dataset search across sites. Aggregated DCAT metadata can serve as a manifest file to facilitate digital preservation."""@en ;
  rdfs:label "DCAT"@en ;
  foaf:maker sto:W3C ;
  sto:hasDBpediaResource <http://dbpedia.org/resource/Data_Catalog_Vocabulary> ;
  sto:hasDeveloper sto:W3C ;
  sto:hasOfficialResource <https://www.w3.org/TR/vocab-dcat/> ;
  sto:hasPublisher sto:W3C ;
  sto:hasWikipediaArticle <https://en.wikipedia.org/wiki/Data_Catalog_Vocabulary> ;
.
sto:W3C_OWL
  a owl:NamedIndividual ;
  a foaf:Document ;
  a sto:Publication ;
  a sto:Standard ;
  terms:creator sto:W3C ;
  terms:license sto:PublicLicenseDocument ;
  rdfs:comment "The W3C Web Ontology Language (OWL) is a Semantic Web language designed to represent rich and complex knowledge about things, groups of things, and relations between things. OWL is a computational logic-based language such that knowledge expressed in OWL can be exploited by computer programs, e.g., to verify the consistency of that knowledge or to make implicit knowledge explicit. OWL documents, known as ontologies, can be published in the World Wide Web and may refer to or be referred from other OWL ontologies. OWL is part of the W3C’s Semantic Web technology stack, which includes RDF, RDFS, SPARQL, etc."@en ;
  rdfs:label "Web Ontology Language"@en ;
  foaf:maker sto:W3C ;
  sto:hasDBpediaResource <http://dbpedia.org/resource/Web_Ontology_Language> ;
  sto:hasOfficialResource <https://www.w3.org/OWL/> ;
  sto:hasPublisher sto:W3C ;
  sto:hasTag "OWL"@en ;
  sto:hasWikipediaArticle <https://en.wikipedia.org/wiki/Web_Ontology_Language?oldformat=true> ;
  sto:relatedTo sto:W3C_RDF ;
.
sto:W3C_RDF
  a owl:NamedIndividual ;
  a foaf:Document ;
  a sto:Publication ;
  a sto:Standard ;
  terms:creator sto:W3C ;
  terms:license sto:PublicLicenseDocument ;
  rdfs:comment "RDF is a standard model for data interchange on the Web. RDF has features that facilitate data merging even if the underlying schemas differ, and it specifically supports the evolution of schemas over time without requiring all the data consumers to be changed. "@en ;
  rdfs:label "Resource Description Framework"@en ;
  foaf:maker sto:W3C ;
  sto:hasDBpediaResource <http://dbpedia.org/resource/Resource_Description_Framework> ;
  sto:hasOfficialResource <https://www.w3.org/RDF/> ;
  sto:hasPublisher sto:W3C ;
  sto:hasTag "RDF"@en ;
  sto:hasWikipediaArticle <https://en.wikipedia.org/wiki/Resource_Description_Framework> ;
.
sto:W3C_RIF
  a owl:NamedIndividual ;
  a foaf:Document ;
  a sto:Publication ;
  a sto:Standard ;
  terms:creator sto:W3C ;
  terms:license sto:PublicLicenseDocument ;
  rdfs:comment "The Rule Interchange Format (RIF) is a W3C Recommendation. RIF is part of the infrastructure for the semantic web, along with (principally) SPARQL, RDF and OWL. Although originally envisioned by many as a rules layer for the semantic web, in reality the design of RIF is based on the observation that there are many rules languages in existence, and what is needed is to exchange rules between them."@en ;
  rdfs:label "Rule Interchange Format"@en ;
  foaf:maker sto:W3C ;
  sto:hasDBpediaResource <http://dbpedia.org/resource/Rule_Interchange_Format> ;
  sto:hasOfficialResource <https://www.w3.org/TR/rif-overview/> ;
  sto:hasPublisher sto:W3C ;
  sto:hasTag "RIF"@en ;
  sto:hasWikipediaArticle <https://en.wikipedia.org/wiki/Rule_Interchange_Format> ;
  sto:relatedTo sto:W3C_OWL ;
.
sto:W3C_SPARQL
  a owl:NamedIndividual ;
  a foaf:Document ;
  a sto:Publication ;
  a sto:Standard ;
  terms:creator sto:W3C ;
  terms:license sto:PublicLicenseDocument ;
  rdfs:comment "The SPARQL Protocol and RDF Query Language (SPARQL) is a query language and protocol for RDF. This document specifies the SPARQL Protocol; it describes a means for conveying SPARQL queries and updates to a SPARQL processing service and returning the results via HTTP to the entity that requested them. This protocol was developed by the W3C SPARQL Working Group, part of the Semantic Web Activity as described in the activity statement ."@en ;
  rdfs:label "SPARQL"@en ;
  foaf:maker sto:W3C ;
  sto:hasDBpediaResource <http://dbpedia.org/resource/SPARQL> ;
  sto:hasOfficialResource <https://www.w3.org/SPARQL> ;
  sto:hasPublisher sto:W3C ;
  sto:hasTag "SPARQL"@en ;
  sto:hasWikipediaArticle <https://en.wikipedia.org/wiki/SPARQL> ;
  sto:relatedTo sto:W3C_RDF ;
.
sto:Weave
  a owl:NamedIndividual ;
  a foaf:Document ;
  a sto:Publication ;
  a sto:TechnicalSpecification ;
  terms:creator sto:sebastian ;
  rdfs:comment "A communications platform for IoT devices that enables device setup, phone-to-device-to-cloud communication, and user interaction from mobile devices and the web. (source: https://www.postscapes.com/internet-of-things-protocols/)"@en ;
  rdfs:label "Weave"@en ;
  sto:hasOfficialResource <https://developers.google.com/weave/> ;
.
sto:WebSocket
  a owl:NamedIndividual ;
  a foaf:Document ;
  a sto:Publication ;
  a sto:TechnicalSpecification ;
  terms:creator sto:sebastian ;
  rdfs:comment "The WebSocket specification — developed as part of the HTML5 initiative — introduced the WebSocket JavaScript interface, which defines a full-duplex single socket connection over which messages can be sent between client and server. The WebSocket standard simplifies much of the complexity around bi-directional web communication and connection management. (source: https://www.postscapes.com/internet-of-things-protocols/)"@en ;
  rdfs:label "WebSocket"@en ;
  sto:hasOfficialResource <https://websocket.org/> ;
.
sto:Weightless
  a owl:NamedIndividual ;
  a foaf:Document ;
  a sto:Publication ;
  a sto:TechnicalSpecification ;
  terms:creator sto:sebastian ;
  rdfs:comment "Weightless is a proposed proprietary open wireless technology standard for exchanging data between a base station and thousands of machines around it (using wavelength radio transmissions in unoccupied TV transmission channels) with high levels of security.  (source: https://www.postscapes.com/internet-of-things-protocols/)"@en ;
  rdfs:label "Weightless"@en ;
  sto:hasOfficialResource <http://www.weightless.org/> ;
.
sto:WiFi
  a owl:NamedIndividual ;
  a foaf:Document ;
  a sto:Publication ;
  a sto:TechnicalSpecification ;
  terms:creator sto:sebastian ;
  rdfs:label "WiFi"@en ;
  sto:hasClassification sto:OpenFogNodeView ;
  sto:hasOfficialResource <https://www.wi-fi.org/> ;
.
sto:WiMax
  a owl:NamedIndividual ;
  a foaf:Document ;
  a sto:Publication ;
  a sto:TechnicalSpecification ;
  terms:creator sto:sebastian ;
  rdfs:comment "WiMax is based on the standard IEEE 802.16 and is intended for wireless metropolitan area networks. The range is different for fixed stations, where it can go up to 50 km and mobile devices with 5 to 15 km. WiMAx operates at frequencies between 2.5 GHz to 5.8 GHz with a transferrate of 40 Mbps.  (source: https://www.postscapes.com/internet-of-things-protocols/)"@en ;
  rdfs:label "WiMax"@en ;
  sto:hasWikipediaArticle <https://en.wikipedia.org/wiki/WiMAX> ;
.
sto:WiSunAlliance
  a owl:NamedIndividual ;
  a foaf:Organization ;
  a sto:IIoTConsortium ;
  terms:creator sto:sebastian ;
  rdfs:comment "The Wi-SUN Alliance seeks to advance seamless connectivity by promoting IEEE 802.15.4g standard based interoperability for global regional markets. (source: https://www.postscapes.com/internet-of-things-protocols/)"@en ;
  rdfs:label "Wi-SUN Alliance"@en ;
  sto:hasOfficialResource <http://www.wi-sun.org/> ;
.
sto:WirelessHart
  a owl:NamedIndividual ;
  a foaf:Document ;
  a sto:Publication ;
  a sto:TechnicalSpecification ;
  terms:creator sto:sebastian ;
  rdfs:comment "WirelessHART technology provides a robust wireless protocol for the full range of process measurement, control, and asset management applications. (source: https://www.postscapes.com/internet-of-things-protocols/)"@en ;
  rdfs:label "WirelessHart"@en ;
  sto:hasOfficialResource <http://www.hartcomm.org/protocol/wihart/wireless_technology.html> ;
.
sto:WolframLanguage
  a owl:NamedIndividual ;
  a foaf:Document ;
  a sto:Publication ;
  a sto:TechnicalSpecification ;
  terms:creator sto:sebastian ;
  rdfs:comment "A symbolic representation of each device. Then there are a standard set of Wolfram Language functions like DeviceRead, DeviceExecute, DeviceReadBuffer and DeviceReadTimeSeries that perform operations related to the device. (source: https://www.postscapes.com/internet-of-things-protocols/)"@en ;
  rdfs:label "Wolfram Language"@en ;
  sto:hasOfficialResource <https://reference.wolfram.com/language/guide/ConnectingToDevices.html> ;
.
sto:Written
  a terms:LinguisticSystem ;
  a owl:NamedIndividual ;
  rdfs:comment "Describes a Written Linguistic System"@en ;
  rdfs:label "Written"@en ;
.
sto:X509
  a owl:NamedIndividual ;
  a foaf:Document ;
  a sto:Publication ;
  a sto:Standard ;
  terms:creator sto:sebastian ;
  rdfs:comment "Standard for public key infrastructure (PKI) to manage digital certificates and public-key encryption. A key part of the Transport Layer Security protocol used to secure web and email communication.  (source: https://www.postscapes.com/internet-of-things-protocols/)"@en ;
  rdfs:label "X.509"@en ;
  sto:hasWikipediaArticle <https://en.wikipedia.org/wiki/X.509> ;
.
sto:XACML
  a owl:NamedIndividual ;
  a foaf:Document ;
  a sto:Publication ;
  a sto:TechnicalSpecification ;
  dul:associatedWith sto:FiwareSecurity ;
  sto:hasTargetConcern sto:Authorization ;
  sto:hasTargetConcern sto:DataAccessControl ;
.
sto:XMPP
  a owl:NamedIndividual ;
  a foaf:Document ;
  a sto:Publication ;
  a sto:TechnicalSpecification ;
  terms:creator sto:sebastian ;
  rdfs:comment "XMPP (Extensible Messaging and Presence Protocol): An open technology for real-time communication, which powers a wide range of applications including instant messaging, presence, multi-party chat, voice and video calls, collaboration, lightweight middleware, content syndication, and generalized routing of XML data. (source: https://www.postscapes.com/internet-of-things-protocols/)"@en ;
  rdfs:label "XMPP"@en ;
  sto:hasOfficialResource <https://xmpp.org/> ;
.
sto:XMPP-IoT
  a owl:NamedIndividual ;
  a foaf:Document ;
  a sto:Publication ;
  a sto:TechnicalSpecification ;
  terms:creator sto:sebastian ;
  rdfs:comment "XMPP-IoT: In the same manor as XMPP silently has created people to people communication interoperable. We are aiming to make communication machine to people and machine to machine interoperable. (source: https://www.postscapes.com/internet-of-things-protocols/)"@en ;
  rdfs:label "XMPP-IoT"@en ;
  sto:hasOfficialResource <https://github.com/joachimlindborg/XMPP-IoT> ;
.
sto:X_Road_Architecture_Technical_Specification
  a <https://www.w3.org/ns/oaSpecificResource> ;
  rdfs:label "X-Road Architecture Technical Specification Version: 1.0 18.09.2015 15 pages Doc. ID: ARC-G"@en ;
  sto:hasOpenResource <https://www.riha.ee/api/v1/systems/70006317-xroad-center/files/257bc950-9149-25be-496b-f54b6a608791> ;
.
sto:ZVEI
  a owl:NamedIndividual ;
  a foaf:Organization ;
  a sto:StandardOrganization ;
  terms:title "German Electrical and Electronic Manufacturers' Association"@en ;
  terms:title "Zentralverband Elektrotechnik- und Elektronikindustrie"@de ;
  rdfs:comment "The ZVEI is one of the most important manufacturers' associations in Germany. It represents the interests of a high-tech branch with a very widely varied and extremely dynamic product portfolio."@en ;
  rdfs:label "ZVEI"@en ;
  sto:hasOfficialResource <https://www.zvei.org/> ;
.
sto:ZigBee
  a owl:NamedIndividual ;
  a foaf:Document ;
  a sto:Publication ;
  a sto:TechnicalSpecification ;
  terms:creator sto:sebastian ;
  rdfs:comment "The ZigBee protocol uses the 802.15.4 standard and operates in the 2.4 GHz frequency range with 250 kbps. The maximum number of nodes in the network is 1024 with a range up to 200 meter. ZigBee can use 128 bit AES encryption. (source: https://www.postscapes.com/internet-of-things-protocols/)"@en ;
  rdfs:label "ZigBee"@en ;
  sto:hasOfficialResource <http://www.zigbee.org/> ;
.
sto:abbreviation
  a owl:DatatypeProperty ;
  rdfs:comment "Abbreviated  name of the thing."@en ;
  rdfs:domain owl:Thing ;
  rdfs:label "has Abbreviated Name"@en ;
  rdfs:range rdf:PlainLiteral ;
.
sto:alignsWith
  a owl:ObjectProperty ;
  a owl:SymmetricProperty ;
  rdfs:comment "indicates that some Standard Classification entity has a similar scope as another. This property most probably is symmetric but not transitive."@en ;
  rdfs:domain sto:StandardClassification ;
  rdfs:label "alignes With"@en ;
  rdfs:range sto:StandardClassification ;
  rdfs:subPropertyOf dul:associatedWith ;
  owl:inverseOf sto:alignsWith ;
.
sto:belongsTo
  a owl:NamedIndividual ;
  a owl:ObjectProperty ;
  terms:creator sto:irlan ;
  rdfs:comment "A Standard Organization that belongs to the country"@en ;
  rdfs:domain foaf:Organization ;
  rdfs:label "belongs To"@en ;
  rdfs:range dbo:Country ;
.
sto:bitkom
  a owl:NamedIndividual ;
  a foaf:Organization ;
  a sto:StandardOrganization ;
  terms:creator sto:sebastian ;
  terms:title "Bundesverband Informationswirtschaft, Telekommunikation und neue Medien"@de ;
  terms:title "German Association for IT, Telecommunications and New Media"@en ;
  rdfs:label "Bitkom"@en ;
  sto:hasOfficialResource <https://www.bitkom.org/> ;
  sto:hasWikipediaArticle <https://de.wikipedia.org/wiki/Bundesverband_Informationswirtschaft,_Telekommunikation_und_neue_Medien'> ;
.
sto:domainName
  a owl:DatatypeProperty ;
  rdfs:comment "Points the Standard with the name of the Industrial Domain"@en ;
  rdfs:domain sto:Domain ;
  rdfs:label "has Domain Name"@en ;
  rdfs:range rdf:PlainLiteral ;
.
sto:eClass
  a owl:NamedIndividual ;
  a foaf:Document ;
  a sto:Publication ;
  a sto:Standard ;
  terms:creator sto:eClassAssoc ;
  rdfs:comment "eCl@ss is the cross-industry product data standard for classification and clear description of products and services."@en ;
  rdfs:label "eClass"@en ;
  foaf:maker sto:eClassAssoc ;
  sto:hasClassification rami:Engineering ;
  sto:hasClassification sto:RAMIConnectedWorld ;
  sto:hasClassification sto:RAMIControlDevice ;
  sto:hasClassification sto:RAMIEnterprise ;
  sto:hasClassification sto:RAMIProduct ;
  sto:hasClassification sto:RAMIStation ;
  sto:hasClassification sto:RAMIWorkCenter ;
  sto:hasDBpediaResource <http://de.dbpedia.org/page/ECl@ss> ;
  sto:hasDeveloper sto:eClassAssoc ;
  sto:hasMotivation "Global identification, semantic description and automatic product classification"@en ;
  sto:hasOfficialResource <https://www.eclass.eu/eclasscontent/standard/overview.html.en> ;
  sto:hasPublisher sto:eClassAssoc ;
  sto:hasWikipediaArticle <https://de.wikipedia.org/wiki/ECl@ss> ;
  sto:relatedTo sto:DIN_SPEC_16592 ;
  sto:relatedTo sto:IEC_61131 ;
  sto:relatedTo sto:IEC_61360 ;
  sto:relatedTo sto:IEC_61499 ;
  sto:relatedTo sto:IEC_61804 ;
  sto:relatedTo sto:IEC_61850 ;
  sto:relatedTo sto:IEC_61987_X ;
  sto:relatedTo sto:IEC_62424 ;
  sto:relatedTo sto:IEC_62453 ;
  sto:relatedTo sto:IEC_62541 ;
  sto:relatedTo sto:IEC_62714 ;
  sto:relatedTo sto:ISO_13584 ;
  sto:relatedTo sto:ISO_14306 ;
  sto:relatedTo sto:ISO_15746 ;
  sto:relatedTo sto:ISO_15926 ;
  sto:relatedTo sto:ISO_18629 ;
  sto:relatedTo sto:ISO_18828-2 ;
  sto:relatedTo sto:ISO_20922 ;
  sto:relatedTo sto:ISO_22400 ;
  sto:relatedTo sto:ISO_29002 ;
  sto:relatedTo sto:ISO_ASTM_52915 ;
  sto:relatedTo sto:ISO_PAS_17506 ;
  sto:relatedTo sto:MathML ;
  sto:relatedTo sto:SysML ;
  sto:relatedTo sto:eClass ;
.
sto:eClassAssoc
  a owl:NamedIndividual ;
  a foaf:Organization ;
  a sto:StandardOrganization ;
  rdfs:comment "Der eCl@ss e. V. ist eine Non-Profit-Organisation, die den gleichnamigen Klassifikationsstandard branchenübergreifend international definiert, weiterentwickelt und verbreitet. Der Verein wird getragen von ordentlichen und fördernden Mitgliedern aus Unternehmen, Verbänden und Institutionen."@de ;
  sto:abbreviation "eCl@ss" ;
  sto:abbreviation "eClass" ;
  sto:formationDate "2000-11-14"^^xsd:date ;
  sto:hasHeadquaterIn dbr:Cologne ;
  sto:hasOfficialResource <https://www.eclass.eu> ;
  sto:hasWikipediaArticle <https://www.wikiwand.com/de/ECl@ss> ;
  sto:orgName "eCl@ss e. V."@de ;
.
sto:ebXML
  a owl:NamedIndividual ;
  a foaf:Document ;
  a sto:Publication ;
  a sto:Standard ;
  terms:creator sto:OASIS ;
  terms:creator sto:UN-CEFACT ;
  rdfs:comment "Electronic Business using eXtensible Markup Language, commonly known as e-business XML, or ebXML is a family of XML based standards whose mission is to provide an open, XML-based infrastructure that enables the global use of electronic business information in an interoperable, secure, and consistent manner by all trading partners."@en ;
  rdfs:label "ebXML"@en ;
  foaf:maker sto:OASIS ;
  foaf:maker sto:UN-CEFACT ;
  sto:hasClassification sto:BusinessProcessExecution ;
  sto:hasDBpediaResource <http://dbpedia.org/resource/EbXML> ;
  sto:hasOfficialResource <https://webstore.iec.ch/publication/24433> ;
  sto:hasPublisher sto:OASIS ;
  sto:hasPublisher sto:UN-CEFACT ;
  sto:hasTag "ebXML"@en ;
  sto:hasWikipediaArticle <https://en.wikipedia.org/wiki/EbXML> ;
.
sto:formationDate
  a owl:DatatypeProperty ;
  a owl:FunctionalProperty ;
  rdfs:comment "Formation date of the Organization"@en ;
  rdfs:domain sto:StandardOrganization ;
  rdfs:label "has Formation Date"@en ;
  rdfs:range xsd:date ;
.
sto:frames
  a owl:ObjectProperty ;
  rdfs:comment "A relation specifying that a vewpoint regards a Concern."@en ;
  rdfs:domain sto:StandardClassification ;
  rdfs:label "frames"@en ;
  rdfs:range sto:Concern ;
  rdfs:subPropertyOf dul:associatedWith ;
  sto:hasOfficialResource <http://www.iso-architecture.org/42010/> ;
.
sto:hasAvailableLanguage
  a owl:NamedIndividual ;
  a owl:ObjectProperty ;
  terms:creator sto:irlan ;
  rdfs:comment "Points to Languages in which the standard document is available, e.g., English, French, etc. Defined as subProperty of dcterms:language"@en ;
  rdfs:domain foaf:Document ;
  rdfs:label "has Available Language"@en ;
  rdfs:range terms:LinguisticSystem ;
  rdfs:subPropertyOf terms:language ;
.
sto:hasClassification
  a owl:NamedIndividual ;
  a owl:ObjectProperty ;
  terms:creator sto:irlan ;
  rdfs:comment "An Standard is isCategorizedBy a given Categorization Area which is connected to a specific Standarization Initiative"@en ;
  rdfs:domain sto:Publication ;
  rdfs:label "has Classification"@en ;
  rdfs:range sto:StandardClassification ;
.
sto:hasDBpediaResource
  a owl:AnnotationProperty ;
  rdfs:comment "Instance's DBpedia Resource"@en ;
  rdfs:label "has DBpedia Resource"@en ;
.
sto:hasDeveloper
  a owl:NamedIndividual ;
  a owl:ObjectProperty ;
  terms:creator sto:irlan ;
  rdfs:comment "The organization that developed this Standard"@en ;
  rdfs:domain sto:Publication ;
  rdfs:label "has Developer"@en ;
  rdfs:range sto:StandardOrganization ;
  rdfs:subPropertyOf foaf:maker ;
.
sto:hasDomain
  a owl:ObjectProperty ;
  terms:creator sto:irlan ;
  rdfs:comment "Describes the domain, in which the Publication is used, particularly, standards."@en ;
  rdfs:comment "Points to the domain in which the standard is used"@en ;
  rdfs:domain sto:Publication ;
  rdfs:label "has Domain"@en ;
  rdfs:range sto:Domain ;
.
sto:hasEdition
  a owl:DatatypeProperty ;
  rdfs:comment "Indicates the current Edition/Version number of the document."@en ;
  rdfs:domain foaf:Document ;
  rdfs:label "has Edition"@en ;
  rdfs:range xsd:float ;
.
sto:hasFileSize
  a owl:ObjectProperty ;
  rdfs:comment "The size of document file in some unit, e.g., 104 Kilobyte."@en ;
  rdfs:domain foaf:Document ;
  rdfs:label "has File Size"@en ;
  rdfs:range om2:Measure ;
  rdfs:seeAlso <https://webstore.iec.ch/webstore/webstore.nsf/xpFAQ.xsp?Open&id=ADMN-7NALM5> ;
  skos:note """1. Reference for om2:Measure <http://www.ontology-of-units-of-measure.org/page/om-2/Measure>
                         2. om2:Measure om2:hasNumericalValue xsd:float;
                         3. om2:Measure om2:hasUnit om2:Unit;
                         4. om2:hasUnit om2:InformationCapacityUnit; is another possibility for range that could not be verified.
                         5. rdfs:seeAlso <http://www.ontology-of-units-of-measure.org/page/om-2/kilobyte> 
                         6. Documentation on Measure <https://github.com/HajoRijgersberg/OM>""" ;
.
sto:hasHeadquaterIn
  a owl:NamedIndividual ;
  a owl:ObjectProperty ;
  terms:creator sto:irlan ;
  rdfs:comment "Denotes the countries in which the Headquarter of the organization who publishes the Standart"@en ;
  rdfs:domain sto:StandardOrganization ;
  rdfs:label "has Headquater In"@en ;
  rdfs:range dbo:Place ;
.
sto:hasICS
  a owl:ObjectProperty ;
  rdfs:comment "Serves as a catalogue of International Classification For Standards"@en ;
  rdfs:domain sto:Publication ;
  rdfs:label "has ICS"@en ;
  rdfs:range sto:InternationalClassificationForStandards ;
.
sto:hasImplementationFormat
  a owl:DatatypeProperty ;
  rdfs:comment "Describes the name of the implementation or serialization format of the Publication, e.g., XML, Document, binary, batch"@en ;
  rdfs:domain sto:Publication ;
  rdfs:label "has Implementation Format"@en ;
  rdfs:range rdfs:Literal ;
.
sto:hasMotivation
  a owl:ObjectProperty ;
  rdfs:domain sto:Publication ;
  rdfs:label "has Motivation"@en ;
  rdfs:range deo:Motivation ;
.
sto:hasObjective
  a owl:DatatypeProperty ;
  rdfs:comment "Specifies the objectives for the different ISA 95 levels."@en ;
  rdfs:domain sto:ISA95Level ;
  rdfs:label "has Objective"@en ;
  rdfs:range xsd:string ;
.
sto:hasOfficialResource
  a owl:DatatypeProperty ;
  rdfs:comment "Points to the URL of the official websilte from which published the document"@en ;
  rdfs:comment "Standard Official Website"@en ;
  rdfs:domain sto:Publication ;
  rdfs:label "has Official Resource"@en ;
  rdfs:range xsd:anyURI ;
.
sto:hasOntology
  a owl:DatatypeProperty ;
  rdfs:comment "Point to the URL of a recognized Ontology representation of the Standard"@en ;
  rdfs:domain sto:Publication ;
  rdfs:label "has Ontology"@en ;
  rdfs:range xsd:anyURI ;
.
sto:hasOpenResource
  a owl:DatatypeProperty ;
  rdfs:comment "points to the URLs of the resources(documents) openly available for the standard" ;
  rdfs:domain sto:Publication ;
  rdfs:label "has Open Resource"@en ;
  rdfs:range xsd:anyURI ;
.
sto:hasPages
  a owl:DatatypeProperty ;
  rdfs:comment "Indicates the number of pages in the document."@en ;
  rdfs:domain foaf:Document ;
  rdfs:label "has Pages"@en ;
  rdfs:range xsd:integer ;
.
sto:hasPreviousVersion
  a owl:ObjectProperty ;
  rdfs:comment "Indicates the list of Standards that are previous versions of a Standard. For example,IEC 60038:2009 has IEC 60038:1983+AMD1:1994+AMD2:1997,IEC 60038:1983/AMD2:1997,IEC 60038:1983/AMD1:1994,IEC 60038:1983,IEC 60038:1975/AMD1:1977,IEC 60038:1975,IEC 60038:1967,IEC 60038:1954,IEC 60038:1938,IEC 60038:1927 as previous versions."@en ;
  rdfs:label "has Previous Version"@en ;
  rdfs:subPropertyOf sto:relatedTo ;
.
sto:hasPublicationDate
  a owl:DatatypeProperty ;
  rdfs:comment "Publication date of the Publication"@en ;
  rdfs:domain sto:Publication ;
  rdfs:label "has Publication Date"@en ;
  rdfs:range xsd:date ;
.
sto:hasPublisher
  a owl:NamedIndividual ;
  a owl:ObjectProperty ;
  terms:creator sto:irlan ;
  rdfs:comment "The organization that published this Standard"@en ;
  rdfs:domain sto:Publication ;
  rdfs:label "has Publisher"@en ;
  rdfs:range sto:StandardOrganization ;
  rdfs:subPropertyOf foaf:maker ;
.
sto:hasStabilityDate
  a owl:DatatypeProperty ;
  rdfs:comment "Stability date of a publication. Publications are valid for a certain period, i.e., the Stability Period. This property defines the end of the stability period."@en ;
  rdfs:domain sto:Publication ;
  rdfs:label "has Stability Date"@en ;
  rdfs:range xsd:gYear ;
  rdfs:seeAlso <https://webstore.iec.ch/webstore/webstore.nsf/xpFAQ.xsp?Open&id=ADMN-7NALM5> ;
  skos:note "The data specified is not actually a Date but an Year" ;
.
sto:hasStatus
  a owl:DatatypeProperty ;
  rdfs:comment "Publication status of the Standard, e.g., Valid, Revised, Published, under preparation, Released"@en ;
  rdfs:domain sto:Publication ;
  rdfs:label "has Status"@en ;
  rdfs:range rdfs:Literal ;
.
sto:hasTag
  a owl:DatatypeProperty ;
  rdfs:comment "Points to the identification of the standards"@en ;
  rdfs:label "has Tag"@en ;
  rdfs:range rdfs:Literal ;
.
sto:hasTargetConcern
  a owl:ObjectProperty ;
  rdfs:comment "The relation declaring that a standard is relevant or targets a certain concern."@en ;
  rdfs:domain [
      a owl:Class ;
      owl:unionOf (
          sto:Standard
          sto:StandardizationFramework
        ) ;
    ] ;
  rdfs:label "has Target Concern"@en ;
  rdfs:range sto:Concern ;
  rdfs:subPropertyOf dul:associatedWith ;
.
sto:hasTask
  a owl:DatatypeProperty ;
  rdfs:comment "Specifies the tasks for the different ISA 95 levels."@en ;
  rdfs:domain sto:ISA95Level ;
  rdfs:label "has Task"@en ;
  rdfs:range xsd:string ;
.
sto:hasTechnicalCommittee
  a owl:ObjectProperty ;
  rdfs:comment "Specifies the Technical Committee or a Sub-Committee that is responsible for creation and maintenance of a standard"@en ;
  rdfs:domain sto:Publication ;
  rdfs:label "has Technical Committee"@en ;
  rdfs:range sto:TechnicalCommittee ;
.
sto:hasWikipediaArticle
  a owl:AnnotationProperty ;
  a owl:DatatypeProperty ;
  rdfs:comment "Wikipedia Article about the Standard"@en ;
  rdfs:label "has Wikipedia Article"@en ;
.
sto:hasstatus
  a owl:AnnotationProperty ;
.
sto:iShare
  a owl:NamedIndividual ;
  a foaf:Organization ;
  dul:associatedWith sto:HTTP ;
  dul:associatedWith sto:ISO_9594 ;
  dul:associatedWith sto:REST ;
  dul:associatedWith sto:RFC_5246 ;
  dul:associatedWith sto:RFC_7519 ;
  dul:associatedWith sto:XACML ;
  rdfs:comment "iSHARE is a uniform set of agreements or a scheme for identification, authentication and authorization. All companies that join the iSHARE Scheme comply with the set of agreements. They all use the same methods to both provide and gain access to data. (source: iShare: 'It is not a platform…')"@en ;
  rdfs:label "iShare"@en ;
  sto:hasOfficialResource <https://www.ishareworks.org/> ;
  sto:hasTargetConcern sto:Identification ;
  sto:hasTargetConcern sto:Interoperability ;
.
sto:identifies
  a owl:ObjectProperty ;
  rdfs:comment "ISO 42010 relation between an architecture description on the on hand and stakeholders and concerns on the other." ;
  rdfs:label "identifies" ;
  rdfs:subPropertyOf dul:associatedWith ;
.
sto:introductionXtee
  a owl:NamedIndividual ;
  a foaf:Document ;
  a sto:Publication ;
  a sto:TechnicalReport ;
  terms:creator sto:EstonianInformationSystemAuthority ;
  rdfs:comment "It is a guide intended for those who want to acquaint themselves more thoroughly with the X-tee (e.g. theose who are working for an organisation which will soon join the X-tee). It introduces the X-tee’s complex terminological system slowly and in a comprehensible way, so that the reader can painlessly achieve the preliminary familiarity with the X-tee necessary to engage with more explicitly technical and complex manuals. (source: https://www.ria.ee/en/state-information-system/x-tee/introduction-x-tee.html)"@en ;
  rdfs:label "Introduction of X-tee"@en ;
  foaf:maker sto:EstonianInformationSystemAuthority ;
  sto:hasClassification sto:xRoadDeploymentView ;
  sto:hasClassification sto:xRoadProtocolsInterfaces ;
  sto:hasClassification sto:xRoadSystemComponents ;
  sto:hasClassification sto:xRoadTechnologyMatrix ;
  sto:hasOfficialResource <https://www.ria.ee/en/state-information-system/x-tee/introduction-x-tee.html> ;
  sto:hasPublisher sto:EstonianInformationSystemAuthority ;
.
sto:irlan
  a owl:NamedIndividual ;
  a foaf:Person ;
  rdfs:label "Irlan Grangel" ;
  foaf:familyName "Grangel" ;
  foaf:mbox "irlangrangel2003@gmail.com" ;
  foaf:name "Irlan" ;
.
sto:isDescribedin
  a owl:ObjectProperty ;
  rdfs:comment "Links the Standarization Frameworks with the Classification of Standards"@en ;
  rdfs:domain sto:StandardClassification ;
  rdfs:label "is Described in"@en ;
  rdfs:range sto:StandardizationFramework ;
.
sto:isImplementationOf
  a owl:NamedIndividual ;
  a owl:ObjectProperty ;
  terms:creator sto:irlan ;
  rdfs:comment "Represent the relation that connects two standards when standard A is the implementation of standard B, e.g., B2MML isImplementationOf ISA-95."@en ;
  rdfs:label "is Implementation Of"@en ;
  rdfs:subPropertyOf sto:relatedTo ;
.
sto:isPartOf
  a owl:AnnotationProperty ;
.
sto:isRelevantFor
  a owl:ObjectProperty ;
  rdfs:comment "An Standard is concerned with Relevant Subjects"@en ;
  rdfs:domain sto:Standard ;
  rdfs:label "is Relevant for"@en ;
  rdfs:range sto:RelevantSubject ;
.
sto:mDNS
  a owl:NamedIndividual ;
  a foaf:Document ;
  a sto:Publication ;
  a sto:TechnicalSpecification ;
  terms:creator sto:sebastian ;
  rdfs:comment "mDNS (multicast Domain Name System) - Resolves host names to IP addresses within small networks that do not include a local name server. (source: https://www.postscapes.com/internet-of-things-protocols/)"@en ;
  rdfs:label "mDNS"@en ;
  sto:hasWikipediaArticle <https://en.wikipedia.org/wiki/Multicast_DNS> ;
.
sto:oneM2M
  a owl:NamedIndividual ;
  a foaf:Organization ;
  a sto:StandardOrganization ;
  rdfs:comment "The purpose and goal of oneM2M is to develop technical specifications which address the need for a common M2M Service Layer that can be readily embedded within various hardware and software, and relied upon to connect the myriad of devices in the field with M2M application servers worldwide. A critical objective of oneM2M is to attract and actively involve organizations from M2M-related business domains such as: telematics and intelligent transportation, healthcare, utilities, industrial automation, smart homes, etc."@en ;
  rdfs:label "oneM2M"@en ;
  sto:hasOfficialResource <http://www.onem2m.org/about-onem2m/why-onem2m> ;
.
sto:openAAS
  a owl:NamedIndividual ;
  a foaf:Document ;
  a sto:Publication ;
  a sto:TechnicalSpecification ;
  terms:creator sto:sebastian ;
  terms:creator "sebastian" ;
  dul:associatedWith sto:AdministrationShell ;
  rdfs:comment """Im Open Source Projekt „openAAS“ – die Abkürzung „AAS“ steht für den englischen Begriff „Asset Administration Shell“, zu Deutsch „Verwaltungsschale“ – arbeitet der ZVEI gemeinsam mit der RWTH Aachen und Unternehmen aus Maschinenbau und Elektroindustrie daran, Industrie 4.0 in die Praxis
umzusetzen. Die Veranschaulichung und Erprobung einer Industrie-4.0-konformen Verwaltungsschale stehen im Mittelpunkt. Dies ist Voraussetzung für eine international erfolgreiche Technologieverifikation
und Standardisierung."""@de ;
  rdfs:comment "openAAS is an open source project to establish a Platform Industry 4.0 conform Administration Shell with open software."@en ;
  rdfs:label "openAAS"@en ;
.
sto:orgName
  a owl:DatatypeProperty ;
  rdfs:comment "Name of the Organization"@en ;
  rdfs:domain sto:StandardOrganization ;
  rdfs:label "Org Name"@en ;
  rdfs:range rdf:PlainLiteral ;
.
sto:publisher
  a owl:AnnotationProperty ;
.
sto:relatedTo
  a owl:NamedIndividual ;
  a owl:ObjectProperty ;
  a owl:SymmetricProperty ;
  a owl:TransitiveProperty ;
  terms:creator sto:irlan ;
  rdfs:comment "Represent any type of relation that connects two standards."@en ;
  rdfs:label "related To"@en ;
  owl:inverseOf sto:relatedTo ;
  skos:altLabel "has Associated Standard"@en ;
.
sto:sebastian
  a owl:NamedIndividual ;
  a foaf:Person ;
  rdfs:label "Sebastian Bader"@en ;
  foaf:familyName "Bader" ;
  foaf:name sto:sebastian ;
  foaf:name "Sebastian" ;
  sto:hasOfficialResource <https://sebastianrbader.de> ;
.
sto:seeAlso
  a owl:AnnotationProperty ;
.
sto:stoPartName
  a owl:DatatypeProperty ;
  rdfs:comment "Name of the standard part."@en ;
  rdfs:domain sto:StandardPart ;
  rdfs:label "std Part Name"@en ;
  rdfs:range xsd:string ;
.
sto:supports
  a owl:ObjectProperty ;
  rdfs:comment "A relation between two different concerns where dealing with the subject Concern supports in achieving the object concern"@en ;
  rdfs:domain sto:Concern ;
  rdfs:label "supports" ;
  rdfs:range sto:Concern ;
.
sto:uIP
  a owl:NamedIndividual ;
  a foaf:Document ;
  a sto:Publication ;
  a sto:TechnicalSpecification ;
  terms:creator sto:sebastian ;
  rdfs:comment "The uIP is an open source TCP/IP stack capable of being used with tiny 8- and 16-bit microcontrollers. It was initially developed by Adam Dunkels of the 'Networked Embedded Systems' group at the Swedish Institute of Computer Science, licensed under a BSD style license, and further developed by a wide group of developers. (source: https://www.postscapes.com/internet-of-things-protocols/)"@en ;
  rdfs:label "uIP"@en ;
  sto:hasWikipediaArticle <https://en.wikipedia.org/wiki/UIP_%28micro_IP%29> ;
.
sto:useStructureOf
  a owl:NamedIndividual ;
  a owl:ObjectProperty ;
  terms:creator sto:irlan ;
  rdfs:comment "Standard A uses the structure of Standard B. For example, OPC UA uses Structure Of IEC_61804 (EDDL)"@en ;
  rdfs:label "use Structure Of"@en ;
  rdfs:subPropertyOf sto:relatedTo ;
.
sto:uses
  a owl:NamedIndividual ;
  a owl:ObjectProperty ;
  terms:creator sto:irlan ;
  rdfs:comment "Defines that Standard A uses Standard B. For example, IEC_62714(AML) uses MathML."@en ;
  rdfs:label "uses"@en ;
  rdfs:subPropertyOf sto:relatedTo ;
.
sto:xRoadDeploymentView
  a owl:NamedIndividual ;
  a sto:StandardClassification ;
  a sto:xRoadSection ;
  dul:associatedWith sto:IDSRAMSystemLayer ;
  dul:associatedWith sto:IIRAImplementationViewpoint ;
  dul:associatedWith sto:RAMIIntegrationLayer ;
  rdfs:label "x-road Deplyoment View"@en ;
  sto:alignsWith sto:IDSRAMSystemLayer ;
  sto:alignsWith sto:IIRAImplementationViewpoint ;
  sto:alignsWith sto:RAMIIntegrationLayer ;
  sto:frames sto:Communication ;
  sto:frames sto:DataAccess ;
  sto:frames sto:Security ;
  sto:frames sto:ServiceDeployment ;
  sto:frames sto:ServiceLifecycleManagement ;
  sto:frames sto:Trustworthiness ;
  sto:isDescribedin sto:xTee ;
.
sto:xRoadDeploymentViewAnno
  a <https://www.w3.org/ns/oaAnnotation> ;
  <https://www.w3.org/ns/oahasBody> sto:xRoadDeploymentView ;
  <https://www.w3.org/ns/oahasTarget> [
      a <https://www.w3.org/ns/oaSpecificResource> ;
      <https://www.w3.org/ns/oahasSelector> [
          a <https://www.w3.org/ns/oaRangeSelector> ;
          <https://www.w3.org/ns/oahasEndSelector> [
              a <https://www.w3.org/ns/oaXPathSelector> ;
              rdf:value "Page 16" ;
            ] ;
          <https://www.w3.org/ns/oahasStartSelector> [
              a <https://www.w3.org/ns/oaXPathSelector> ;
              rdf:value "Page 15" ;
            ] ;
        ] ;
      <https://www.w3.org/ns/oahasSource> sto:X_Road_Architecture_Technical_Specification ;
    ] ;
.
sto:xRoadProtocolsInterfaces
  a owl:NamedIndividual ;
  a sto:StandardClassification ;
  a sto:xRoadSection ;
  dul:associatedWith sto:IDSRAMProcessLayer ;
  dul:associatedWith sto:IIRAControlDomain ;
  dul:associatedWith sto:RAMIIntegrationLayer ;
  rdfs:label "x-road Protocols and Interfaces"@en ;
  sto:alignsWith sto:IDSRAMProcessLayer ;
  sto:alignsWith sto:IIRAControlDomain ;
  sto:alignsWith sto:RAMIIntegrationLayer ;
  sto:frames sto:Communication ;
  sto:frames sto:Interoperability ;
  sto:frames sto:SyntacticInteroperability ;
  sto:isDescribedin sto:xTee ;
.
sto:xRoadProtocolsInterfacesAnno
  a <https://www.w3.org/ns/oaAnnotation> ;
  <https://www.w3.org/ns/oahasBody> sto:xRoadProtocolsInterfaces ;
  <https://www.w3.org/ns/oahasTarget> [
      a <https://www.w3.org/ns/oaSpecificResource> ;
      <https://www.w3.org/ns/oahasSelector> [
          a <https://www.w3.org/ns/oaRangeSelector> ;
          <https://www.w3.org/ns/oahasEndSelector> [
              a <https://www.w3.org/ns/oaXPathSelector> ;
              rdf:value "Page 14" ;
            ] ;
          <https://www.w3.org/ns/oahasStartSelector> [
              a <https://www.w3.org/ns/oaXPathSelector> ;
              rdf:value "Page 10" ;
            ] ;
        ] ;
      <https://www.w3.org/ns/oahasSource> sto:X_Road_Architecture_Technical_Specification ;
    ] ;
.
sto:xRoadSection
  a owl:Class ;
  rdfs:label "x-road Section"@en ;
  rdfs:subClassOf sto:StandardClassification ;
  rdfs:subClassOf [
      a owl:Restriction ;
      owl:hasValue sto:xTee ;
      owl:onProperty sto:isDescribedin ;
    ] ;
.
sto:xRoadSystemComponents
  a owl:NamedIndividual ;
  a sto:StandardClassification ;
  a sto:xRoadSection ;
  dul:associatedWith sto:IDSRAMBusinessLayer ;
  dul:associatedWith sto:IDSRAMProcessLayer ;
  dul:associatedWith sto:IIRASecurityFramework ;
  dul:associatedWith sto:RAMIFunctionalLayer ;
  rdfs:label "x-road System Components"@en ;
  sto:alignsWith sto:IDSRAMBusinessLayer ;
  sto:alignsWith sto:IDSRAMProcessLayer ;
  sto:alignsWith sto:IIRASecurityFramework ;
  sto:alignsWith sto:RAMIFunctionalLayer ;
  sto:frames sto:Authentication ;
  sto:frames sto:Communication ;
  sto:frames sto:IdentityManagement ;
  sto:frames sto:SecureCommunication ;
  sto:frames sto:Security ;
  sto:frames sto:SecurityConfiguration ;
  sto:frames sto:Trustworthiness ;
  sto:isDescribedin sto:xTee ;
.
sto:xRoadSystemComponentsAnno
  a <https://www.w3.org/ns/oaAnnotation> ;
  <https://www.w3.org/ns/oahasBody> sto:xRoadSystemComponents ;
  <https://www.w3.org/ns/oahasTarget> [
      a <https://www.w3.org/ns/oaSpecificResource> ;
      <https://www.w3.org/ns/oahasSelector> [
          a <https://www.w3.org/ns/oaRangeSelector> ;
          <https://www.w3.org/ns/oahasEndSelector> [
              a <https://www.w3.org/ns/oaXPathSelector> ;
              rdf:value "Page 10" ;
            ] ;
          <https://www.w3.org/ns/oahasStartSelector> [
              a <https://www.w3.org/ns/oaXPathSelector> ;
              rdf:value "Page 7" ;
            ] ;
        ] ;
      <https://www.w3.org/ns/oahasSource> sto:X_Road_Architecture_Technical_Specification ;
    ] ;
.
sto:xRoadTechnologyMatrix
  a owl:NamedIndividual ;
  a sto:StandardClassification ;
  a sto:xRoadSection ;
  rdfs:label "x-road Technology Matrix"@en ;
  sto:isDescribedin sto:xTee ;
.
sto:xRoadTechnologyMatrixAnno
  a <https://www.w3.org/ns/oaAnnotation> ;
  <https://www.w3.org/ns/oahasBody> sto:xRoadTechnologyMatrix ;
  <https://www.w3.org/ns/oahasTarget> [
      a <https://www.w3.org/ns/oaSpecificResource> ;
      <https://www.w3.org/ns/oahasSelector> [
          a <https://www.w3.org/ns/oaRangeSelector> ;
          <https://www.w3.org/ns/oahasEndSelector> [
              a <https://www.w3.org/ns/oaXPathSelector> ;
              rdf:value "Page 15" ;
            ] ;
          <https://www.w3.org/ns/oahasStartSelector> [
              a <https://www.w3.org/ns/oaXPathSelector> ;
              rdf:value "Page 14" ;
            ] ;
        ] ;
      <https://www.w3.org/ns/oahasSource> sto:X_Road_Architecture_Technical_Specification ;
    ] ;
.
sto:xTee
  a owl:NamedIndividual ;
  a sto:ArchitectureDescription ;
  a sto:StandardizationFramework ;
  rdfs:label "x-Tee"@en ;
  sto:hasPublisher :x-road ;
.
:
  a owl:NamedIndividual ;
  a owl:Ontology ;
  terms:created "2017-01-25"^^xsd:date ;
  terms:creator <http://data.semanticweb.org/person/steffen-lohmann> ;
  terms:creator sto:irlan ;
  terms:creator <https://www.linkedin.com/in/paul-baptista-601177b2> ;
  terms:modified "2017-09-08"^^xsd:date ;
  terms:modified "2019-01-23"^^xsd:date ;
  terms:publisher <http://de.dbpedia.org/resource/Fraunhofer-Gesellschaft> ;
  terms:rights "This work is distributed under a Creative Commons Attribution License (http://creativecommons.org/licenses/by/3.0/)."@en ;
  terms:title "Standards Ontology"@en ;
  vann:preferredNamespacePrefix "sto" ;
  vann:preferredNamespaceUri "https://w3id.org/i40/sto#" ;
  vann:preferredNamespaceUri "https://w3id.org/i40/sto/" ;
  doap:repository <https://github.com/i40-Tools/StandardsOntology> ;
  rdfs:comment "An ontology to describe standards related to Industry 4.0 and Smart Manufacturing"@en ;
  rdfs:comment "The Internet of things (IoT) is the network of devices such as vehicles, and home appliances that contain electronics, software, sensors, actuators, and connectivity which allows these things to connect, interact and exchange data."@en ;
  rdfs:label "Internet of Things (IOT)"@en ;
  owl:versionInfo "0.3" ;
  owl:versionInfo "0.4" ;
  foaf:maker <http://data.semanticweb.org/person/steffen-lohmann> ;
  foaf:maker sto:irlan ;
  foaf:maker <https://www.linkedin.com/in/paul-baptista-601177b2> ;
  sto:hasDBpediaResource "http://dbpedia.org/page/Internet_of_things"@en ;
  sto:hasOfficialResource <https://webstore.iec.ch/publication/153> ;
  sto:hasWikipediaArticle "https://en.wikipedia.org/wiki/Internet_of_things"@en ;
.
<https://w3id.org/i40/sto/10#IndustrialInternetStandardSystem>
  a owl:NamedIndividual ;
  a sto:Publication ;
  rdfs:comment "Industrial Internet involves all industrial segment and all entities of industry field and ICT field, and it’s forming a complicated and total new ecological system. With industrial system networking and collaboration increasing, lots of new standardization requirements rise. While considering about the problems for Industrial Internet such as standard lacking, standard lagging, and standard duplicated, under the guidance of the Ministry of Industry and Information Technology (MIIT), Alliance of Industrial Internet (referred to as AII hereinafter) launched the study on the Industrial Internet standard system. Based on Industrial Internet Architecture (Version 1.0) and research on Industrial Internet standard requirements, AII drafted the Report on Industrial Internet Standard System (Version 1.0). In this Report, we propose the general idea, basic principles, standard system framework, key standardization directions and promotion suggestions. It aims to provide a systemized guidance of Industrial  Internet standardization for the industrial communities, to provide references and basis for development and amendment of Industrial Internet national standards, industrial standards and group standards, and to provide support for Industrial Internet development."@en ;
  rdfs:label "Industrial Internet Standard System" ;
  sto:hasPublisher :AllianceOfIndustrialInternet ;
.
:AllianceIndustrieDuFutur
  a owl:NamedIndividual ;
  a sto:IIoTConsortium ;
  rdfs:label "Alliance Industrie du Futur"@en ;
  sto:hasHeadquaterIn :France ;
  sto:hasOfficialResource <http://www.industrie-dufutur.org/> ;
.
:AllianceOfIndustrialInternet
  a owl:NamedIndividual ;
  a sto:IIoTConsortium ;
  rdfs:label "Alliance of Industrial Internet"@en ;
  skos:altLabel "工业互联网产业联盟"@cn ;
  sto:hasHeadquaterIn dbr:China ;
  sto:seeAlso <http://www.aii-alliance.org/> ;
.
:ArrowheadProject
  a owl:NamedIndividual ;
  a foaf:Organization ;
  rdfs:label "Arrowhead Project" ;
  sto:seeAlso <http://www.arrowhead.eu/> ;
.
:BDVA
  a owl:NamedIndividual ;
  a foaf:Organization ;
  rdfs:label "Big Data Value Association" ;
  skos:altLabel "BDVA" ;
.
:Fiware
  a owl:NamedIndividual ;
  a foaf:Organization ;
  rdfs:label "FIWARE" ;
.
:France
  a dbo:Country ;
  a owl:NamedIndividual ;
.
:IndustrialInternetArchitecture
  a owl:NamedIndividual ;
  a sto:ArchitectureDescription ;
  rdfs:label "AII Industrial Internet Architecture"@en ;
  sto:hasOfficialResource <http://en.aii-alliance.org/uploadfile/2017/0307/Industrial.pdf> ;
  sto:hasPublisher :AllianceOfIndustrialInternet ;
.
:Italy
  a dbo:Country ;
  a owl:NamedIndividual ;
.
:Japan
  a dbo:Country ;
  a owl:NamedIndividual ;
.
:OcfBlock
  a owl:Class ;
  rdfs:label "OCF Framework Block" ;
  rdfs:subClassOf sto:StandardClassification ;
.
<https://w3id.org/i40/sto/VDI/VDE_2182>
  a owl:NamedIndividual ;
  a foaf:Document ;
  a sto:Publication ;
  a sto:Standard ;
  terms:creator sto:VDI ;
  terms:creator sto:sebastian ;
  terms:hasLicense "private"@en ;
  terms:title "IT-security for industrial automation"@en ;
  terms:title "Informationssicherheit in der industriellen Automatisierung"@de ;
  rdfs:comment "This guideline describes how specific measures can be implemented in order to guarantee the IT security of automated machines and plant; aspects of the automation devices, automation systems, and automation applications used are considered. A uniform, feasible procedure for ensuring IT security throughout the entire life cycle of automation devices, systems, and applications is described, based on common terms and definitions agreed by the manufacturers of automation devices and systems and their users (e.g., machine manufacturers, integrators, operators). The life cycle covers the development, integration, operation, migration, and decommissioning phases.This guideline defines a simple procedure model for the development and description of IT Security. The model consists of eight steps."@en ;
  rdfs:label "VDI/VDE 2182"@en ;
  foaf:maker sto:VDI ;
  sto:hasClassification rami:Security ;
  sto:hasDeveloper sto:VDI ;
  sto:hasOfficialResource <http://www.vdi.eu/nc/guidelines/vdivde_2182_blatt_1-informationssicherheit_in_der_industriellen_automatisierung_allgemeines_vorgehensmode/> ;
  sto:hasPublisher sto:VDI ;
.
:x-road
  a owl:NamedIndividual ;
  a sto:DataSharingInitiative ;
  rdfs:label "x-road" ;
.
ids:TrustedConnector
  a owl:NamedIndividual ;
  a sto:Technology ;
  terms:creator sto:IDSRAMReferenceArchitectureModel ;
  dul:associatedWith sto:AdministrationShell ;
  dul:associatedWith sto:IDSRAMReferenceArchitectureModel ;
  rdfs:comment "TODO: model IDS concepts correctly"@en ;
  rdfs:label "Trusted Connector"@en ;
  foaf:maker sto:IDSRAMReferenceArchitectureModel ;
  sto:alignsWith sto:AdministrationShell ;
.
<https://www.linkedin.com/in/paul-baptista-601177b2>
  a owl:NamedIndividual ;
  a foaf:Person ;
  rdfs:label "Paul Baptista" ;
.
<https://www.wikidata.org/wiki/Q1548249>
  a <http://voag.linkedmodel.org/voag#StakeholderGroup> ;
  a owl:NamedIndividual ;
  rdfs:label "System Architect"@en ;
.
[
  <http://swrl.stanford.edu/ontologies/3.3/swrla.owl#isRuleEnabled> true ;
].
[
  <http://swrl.stanford.edu/ontologies/3.3/swrla.owl#isRuleEnabled> true ;
].
